{"@context":{"@vocab":"https://schemas.ieee.org/2030.5/","sh":"http://www.w3.org/ns/shacl#","rdf":"http://www.w3.org/1999/02/22-rdf-syntax-ns#","rdfs":"http://www.w3.org/2000/01/rdf-schema#","xsd":"http://www.w3.org/2001/XMLSchema#","owl":"http://www.w3.org/2002/07/owl#"},"@graph":[{"@id":"DeviceCapabilityShape","@type":"sh:NodeShape","sh:targetClass":{"@id":"DeviceCapability"},"rdfs:comment":"Returned by the URI provided by DNS-SD, to allow clients to find the URIs to the resources in which they are interested.","sh:property":[{"sh:path":{"@id":"EndDeviceListLink"},"sh:maxCount":1,"sh:datatype":"xsd:string"},{"sh:path":{"@id":"MirrorUsagePointListLink"},"sh:maxCount":1,"sh:datatype":"xsd:string"},{"sh:path":{"@id":"SelfDeviceLink"},"sh:maxCount":1,"sh:datatype":"xsd:string"},{"sh:path":{"@id":"pollRate"},"sh:maxCount":1,"sh:minInclusive":0,"sh:maxInclusive":4294967295,"sh:datatype":"xsd:unsignedInt","rdfs:comment":"The default polling rate for this function set (this resource and all resources below), in seconds. If not specified, a default of 900 seconds (15 minutes) is used. It is RECOMMENDED a client poll the resources of this function set every pollRate seconds.","sh:defaultValue":"900"}]},{"@id":"AbstractDeviceShape","@type":"sh:NodeShape","sh:targetClass":{"@id":"AbstractDevice"},"rdfs:comment":"The EndDevice providing the resources available within the DeviceCapabilities.","sh:property":[{"sh:path":{"@id":"ConfigurationLink"},"sh:maxCount":1,"sh:datatype":"xsd:string"},{"sh:path":{"@id":"DERListLink"},"sh:maxCount":1,"sh:datatype":"xsd:string"},{"sh:path":{"@id":"deviceCategory"},"sh:in":["0","1","2","3","4","5","6","7","8","9","10","11","12","13","14","15","16","17","18","19","20","21","22","23","24","25"],"sh:maxCount":1,"sh:datatype":"xsd:string","rdfs:comment":"This field is for use in devices that can adjust energy usage (e.g., demand response, distributed energy resources).  For devices that do not respond to EndDeviceControls or DERControls (for instance, an ESI), this field should not have any bits set."},{"sh:path":{"@id":"DeviceInformationLink"},"sh:maxCount":1,"sh:datatype":"xsd:string"},{"sh:path":{"@id":"DeviceStatusLink"},"sh:maxCount":1,"sh:datatype":"xsd:string"},{"sh:path":{"@id":"FileStatusLink"},"sh:maxCount":1,"sh:datatype":"xsd:string"},{"sh:path":{"@id":"IPInterfaceListLink"},"sh:maxCount":1,"sh:datatype":"xsd:string"},{"sh:path":{"@id":"lFDI"},"sh:maxCount":1,"sh:datatype":"xsd:hexBinary","rdfs:comment":"Long form of device identifier. See the Security section for additional details."},{"sh:path":{"@id":"LoadShedAvailabilityListLink"},"sh:maxCount":1,"sh:datatype":"xsd:string"},{"sh:path":{"@id":"LogEventListLink"},"sh:maxCount":1,"sh:datatype":"xsd:string"},{"sh:path":{"@id":"PowerStatusLink"},"sh:maxCount":1,"sh:datatype":"xsd:string"},{"sh:path":{"@id":"sFDI"},"sh:minCount":1,"sh:maxCount":1,"sh:datatype":"xsd:integer","rdfs:comment":"Short form of device identifier, WITH the checksum digit. See the Security section for additional details."}]},{"@id":"DeviceStatusShape","@type":"sh:NodeShape","sh:targetClass":{"@id":"DeviceStatus"},"rdfs:comment":"Status of device","sh:property":[{"sh:path":{"@id":"changedTime"},"sh:minCount":1,"sh:maxCount":1,"sh:datatype":"xsd:integer","rdfs:comment":"The time at which the reported values were recorded."},{"sh:path":{"@id":"onCount"},"sh:maxCount":1,"sh:minInclusive":0,"sh:maxInclusive":65535,"sh:datatype":"xsd:unsignedShort","rdfs:comment":"The number of times that the device has been turned on: Count of \"device on\" times, since the last time the counter was reset"},{"sh:path":{"@id":"opState"},"sh:maxCount":1,"sh:minInclusive":0,"sh:maxInclusive":255,"sh:datatype":"xsd:unsignedByte","rdfs:comment":"Device operational state: \n0 - Not applicable / Unknown\n1 - Not operating\n2 - Operating\n3 - Starting up\n4 - Shutting down\n5 - At disconnect level\n6 - kW ramping\n7 - kVar ramping"},{"sh:path":{"@id":"opTime"},"sh:maxCount":1,"sh:minInclusive":0,"sh:maxInclusive":4294967295,"sh:datatype":"xsd:unsignedInt","rdfs:comment":"Total time device has operated: re-settable: Accumulated time in seconds since the last time the counter was reset."},{"sh:path":{"@id":"Temperature"},"sh:node":{"@id":"TemperatureShape"}},{"sh:path":{"@id":"TimeLink"},"sh:maxCount":1,"sh:datatype":"xsd:string"},{"sh:path":{"@id":"pollRate"},"sh:maxCount":1,"sh:minInclusive":0,"sh:maxInclusive":4294967295,"sh:datatype":"xsd:unsignedInt","rdfs:comment":"The default polling rate for this function set (this resource and all resources below), in seconds. If not specified, a default of 900 seconds (15 minutes) is used. It is RECOMMENDED a client poll the resources of this function set every pollRate seconds.","sh:defaultValue":"900"}]},{"@id":"EndDeviceShape","@type":"sh:NodeShape","sh:targetClass":{"@id":"EndDevice"},"rdfs:comment":"Asset container that performs one or more end device functions. Contains information about individual devices in the network.","sh:property":[{"sh:path":{"@id":"changedTime"},"sh:minCount":1,"sh:maxCount":1,"sh:datatype":"xsd:integer","rdfs:comment":"The time at which this resource was last modified or created."},{"sh:path":{"@id":"enabled"},"sh:maxCount":1,"sh:datatype":"xsd:boolean","rdfs:comment":"This attribute indicates whether or not an EndDevice is enabled, or registered, on the server. If a server sets this attribute to false, the device is no longer registered. It should be noted that servers can delete EndDevice instances, but using this attribute for some time is more convenient for clients."},{"sh:path":{"@id":"FlowReservationRequestListLink"},"sh:maxCount":1,"sh:datatype":"xsd:string"},{"sh:path":{"@id":"FlowReservationResponseListLink"},"sh:maxCount":1,"sh:datatype":"xsd:string"},{"sh:path":{"@id":"FunctionSetAssignmentsListLink"},"sh:maxCount":1,"sh:datatype":"xsd:string"},{"sh:path":{"@id":"postRate"},"sh:maxCount":1,"sh:minInclusive":0,"sh:maxInclusive":4294967295,"sh:datatype":"xsd:unsignedInt","rdfs:comment":"POST rate, or how often EndDevice and subordinate resources should be POSTed, in seconds. A client MAY indicate a preferred postRate when POSTing EndDevice. A server MAY add or modify postRate to indicate its preferred posting rate."},{"sh:path":{"@id":"RegistrationLink"},"sh:maxCount":1,"sh:datatype":"xsd:string"},{"sh:path":{"@id":"SubscriptionListLink"},"sh:maxCount":1,"sh:datatype":"xsd:string"}]},{"@id":"EndDeviceListShape","@type":"sh:NodeShape","sh:targetClass":{"@id":"EndDeviceList"},"rdfs:comment":"A List element to hold EndDevice objects.","sh:property":[{"sh:path":{"@id":"EndDevice"},"sh:node":{"@id":"EndDeviceShape"}},{"sh:path":{"@id":"pollRate"},"sh:maxCount":1,"sh:minInclusive":0,"sh:maxInclusive":4294967295,"sh:datatype":"xsd:unsignedInt","rdfs:comment":"The default polling rate for this function set (this resource and all resources below), in seconds. If not specified, a default of 900 seconds (15 minutes) is used. It is RECOMMENDED a client poll the resources of this function set every pollRate seconds.","sh:defaultValue":"900"}]},{"@id":"RegistrationShape","@type":"sh:NodeShape","sh:targetClass":{"@id":"Registration"},"rdfs:comment":"Registration represents an authorization to access the resources on a host.","sh:property":[{"sh:path":{"@id":"dateTimeRegistered"},"sh:minCount":1,"sh:maxCount":1,"sh:datatype":"xsd:integer","rdfs:comment":"Contains the time at which this registration was created, by which clients MAY prioritize information providers with the most recent registrations, when no additional direction from the consumer is available."},{"sh:path":{"@id":"pIN"},"sh:minCount":1,"sh:maxCount":1,"sh:minInclusive":0,"sh:maxInclusive":4294967295,"sh:datatype":"xsd:integer","rdfs:comment":"Contains the registration PIN number associated with the device, including the checksum digit."},{"sh:path":{"@id":"pollRate"},"sh:maxCount":1,"sh:minInclusive":0,"sh:maxInclusive":4294967295,"sh:datatype":"xsd:unsignedInt","rdfs:comment":"The default polling rate for this function set (this resource and all resources below), in seconds. If not specified, a default of 900 seconds (15 minutes) is used. It is RECOMMENDED a client poll the resources of this function set every pollRate seconds.","sh:defaultValue":"900"}]},{"@id":"SelfDeviceShape","@type":"sh:NodeShape","sh:targetClass":{"@id":"SelfDevice"},"rdfs:comment":"The EndDevice providing the resources available within the DeviceCapabilities.","sh:property":[{"sh:path":{"@id":"pollRate"},"sh:maxCount":1,"sh:minInclusive":0,"sh:maxInclusive":4294967295,"sh:datatype":"xsd:unsignedInt","rdfs:comment":"The default polling rate for this function set (this resource and all resources below), in seconds. If not specified, a default of 900 seconds (15 minutes) is used. It is RECOMMENDED a client poll the resources of this function set every pollRate seconds.","sh:defaultValue":"900"}]},{"@id":"TemperatureShape","@type":"sh:NodeShape","sh:targetClass":{"@id":"Temperature"},"rdfs:comment":"Specification of a temperature.","sh:property":[{"sh:path":{"@id":"multiplier"},"sh:in":[0,1,2,3,6,9],"sh:minCount":1,"sh:maxCount":1,"sh:datatype":"xsd:integer","rdfs:comment":"Multiplier for 'unit'."},{"sh:path":{"@id":"subject"},"sh:minCount":1,"sh:maxCount":1,"sh:minInclusive":0,"sh:maxInclusive":255,"sh:datatype":"xsd:unsignedByte","rdfs:comment":"The subject of the temperature measurement\n0 - Enclosure\n1 - Transformer\n2 - HeatSink"},{"sh:path":{"@id":"value"},"sh:minCount":1,"sh:maxCount":1,"sh:datatype":"xsd:short","rdfs:comment":"Value in Degrees Celsius (uom 23)."}]},{"@id":"FunctionSetAssignmentsBaseShape","@type":"sh:NodeShape","sh:targetClass":{"@id":"FunctionSetAssignmentsBase"},"rdfs:comment":"Defines a collection of function set instances that are to be used by one or more devices as indicated by the EndDevice object(s) of the server.","sh:property":[{"sh:path":{"@id":"CustomerAccountListLink"},"sh:maxCount":1,"sh:datatype":"xsd:string"},{"sh:path":{"@id":"DemandResponseProgramListLink"},"sh:maxCount":1,"sh:datatype":"xsd:string"},{"sh:path":{"@id":"DERProgramListLink"},"sh:maxCount":1,"sh:datatype":"xsd:string"},{"sh:path":{"@id":"FileListLink"},"sh:maxCount":1,"sh:datatype":"xsd:string"},{"sh:path":{"@id":"MessagingProgramListLink"},"sh:maxCount":1,"sh:datatype":"xsd:string"},{"sh:path":{"@id":"PrepaymentListLink"},"sh:maxCount":1,"sh:datatype":"xsd:string"},{"sh:path":{"@id":"ResponseSetListLink"},"sh:maxCount":1,"sh:datatype":"xsd:string"},{"sh:path":{"@id":"TariffProfileListLink"},"sh:maxCount":1,"sh:datatype":"xsd:string"},{"sh:path":{"@id":"TimeLink"},"sh:maxCount":1,"sh:datatype":"xsd:string"},{"sh:path":{"@id":"UsagePointListLink"},"sh:maxCount":1,"sh:datatype":"xsd:string"}]},{"@id":"FunctionSetAssignmentsShape","@type":"sh:NodeShape","sh:targetClass":{"@id":"FunctionSetAssignments"},"rdfs:comment":"Provides an identifiable, subscribable collection of resources for a particular device to consume.","sh:property":[{"sh:path":{"@id":"mRID"},"sh:minCount":1,"sh:maxCount":1,"sh:datatype":"xsd:string","rdfs:comment":"The global identifier of the object."},{"sh:path":{"@id":"description"},"sh:maxCount":1,"sh:datatype":"xsd:string","rdfs:comment":"The description is a human readable text describing or naming the object."},{"sh:path":{"@id":"version"},"sh:maxCount":1,"sh:minInclusive":0,"sh:maxInclusive":65535,"sh:datatype":"xsd:integer","rdfs:comment":"Contains the version number of the object. See the type definition for details."},{"sh:path":{"@id":"subscribable"},"sh:in":[0,1,2,3],"sh:maxCount":1,"sh:minInclusive":0,"sh:maxInclusive":255,"sh:datatype":"xsd:integer","rdfs:comment":"Indicates whether or not subscriptions are supported for this resource, and whether or not conditional (thresholds) are supported. If not specified, is \"not subscribable\" (0).","sh:defaultValue":"0"}]},{"@id":"FunctionSetAssignmentsListShape","@type":"sh:NodeShape","sh:targetClass":{"@id":"FunctionSetAssignmentsList"},"rdfs:comment":"A List element to hold FunctionSetAssignments objects.","sh:property":[{"sh:path":{"@id":"FunctionSetAssignments"},"sh:node":{"@id":"FunctionSetAssignmentsShape"}},{"sh:path":{"@id":"pollRate"},"sh:maxCount":1,"sh:minInclusive":0,"sh:maxInclusive":4294967295,"sh:datatype":"xsd:unsignedInt","rdfs:comment":"The default polling rate for this function set (this resource and all resources below), in seconds. If not specified, a default of 900 seconds (15 minutes) is used. It is RECOMMENDED a client poll the resources of this function set every pollRate seconds.","sh:defaultValue":"900"}]},{"@id":"ConditionShape","@type":"sh:NodeShape","sh:targetClass":{"@id":"Condition"},"rdfs:comment":"Indicates a condition that must be satisfied for the Notification to be triggered.","sh:property":[{"sh:path":{"@id":"attributeIdentifier"},"sh:minCount":1,"sh:maxCount":1,"sh:minInclusive":0,"sh:maxInclusive":255,"sh:datatype":"xsd:unsignedByte","rdfs:comment":"0 = Reading value\n1-255 = Reserved"},{"sh:path":{"@id":"lowerThreshold"},"sh:minCount":1,"sh:maxCount":1,"sh:datatype":"xsd:long","rdfs:comment":"The value of the lower threshold"},{"sh:path":{"@id":"upperThreshold"},"sh:minCount":1,"sh:maxCount":1,"sh:datatype":"xsd:long","rdfs:comment":"The value of the upper threshold"}]},{"@id":"SubscriptionBaseShape","@type":"sh:NodeShape","sh:targetClass":{"@id":"SubscriptionBase"},"rdfs:comment":"Holds the information related to a client subscription to receive updates to a resource automatically. The actual resources may be passed in the Notification by specifying a specific xsi:type for the Resource and passing the full representation.","sh:property":[{"sh:path":{"@id":"subscribedResource"},"sh:minCount":1,"sh:maxCount":1,"sh:datatype":"xsd:anyURI","rdfs:comment":"The resource for which the subscription applies. Query string parameters SHALL NOT be specified when subscribing to list resources.  Should a query string parameter be specified, servers SHALL ignore them."}]},{"@id":"SubscriptionShape","@type":"sh:NodeShape","sh:targetClass":{"@id":"Subscription"},"rdfs:comment":"Holds the information related to a client subscription to receive updates to a resource automatically.","sh:property":[{"sh:path":{"@id":"Condition"},"sh:maxCount":1,"sh:node":{"@id":"ConditionShape"}},{"sh:path":{"@id":"encoding"},"sh:minCount":1,"sh:maxCount":1,"sh:minInclusive":0,"sh:maxInclusive":255,"sh:datatype":"xsd:unsignedByte","rdfs:comment":"0 - application/sep+xml\n1 - application/sep-exi\n2-255 - reserved"},{"sh:path":{"@id":"level"},"sh:minCount":1,"sh:maxCount":1,"sh:datatype":"xsd:string","rdfs:comment":"Contains the preferred schema and extensibility level indication such as \"+S1\""},{"sh:path":{"@id":"limit"},"sh:minCount":1,"sh:maxCount":1,"sh:minInclusive":0,"sh:maxInclusive":4294967295,"sh:datatype":"xsd:unsignedInt","rdfs:comment":"This element is used to indicate the maximum number of list items that should be included in a notification when the subscribed resource changes. This limit is meant to be functionally equivalent to the \u2018limit\u2019 query string parameter, but applies to both list resources as well as other resources.  For list resources, if a limit of \u20180\u2019 is specified, then notifications SHALL contain a list resource with results=\u20190\u2019 (equivalent to a simple change notification).  For list resources, if a limit greater than \u20180\u2019 is specified, then notifications SHALL contain a list resource with results equal to the limit specified (or less, should the list contain fewer items than the limit specified or should the server be unable to provide the requested number of items for any reason) and follow the same rules for list resources (e.g., ordering).  For non-list resources, if a limit of \u20180\u2019 is specified, then notifications SHALL NOT contain a resource representation (equivalent to a simple change notification).  For non-list resources, if a limit greater than \u20180\u2019 is specified, then notifications SHALL contain the representation of the changed resource."},{"sh:path":{"@id":"notificationURI"},"sh:minCount":1,"sh:maxCount":1,"sh:datatype":"xsd:anyURI","rdfs:comment":"The resource to which to post the notifications about the requested subscribed resource. Because this URI will exist on a server other than the one being POSTed to, this attribute SHALL be a fully-qualified absolute URI, not a relative reference."}]},{"@id":"SubscriptionListShape","@type":"sh:NodeShape","sh:targetClass":{"@id":"SubscriptionList"},"rdfs:comment":"A List element to hold Subscription objects.","sh:property":[{"sh:path":{"@id":"Subscription"},"sh:node":{"@id":"SubscriptionShape"}},{"sh:path":{"@id":"pollRate"},"sh:maxCount":1,"sh:minInclusive":0,"sh:maxInclusive":4294967295,"sh:datatype":"xsd:unsignedInt","rdfs:comment":"The default polling rate for this function set (this resource and all resources below), in seconds. If not specified, a default of 900 seconds (15 minutes) is used. It is RECOMMENDED a client poll the resources of this function set every pollRate seconds.","sh:defaultValue":"900"}]},{"@id":"NotificationShape","@type":"sh:NodeShape","sh:targetClass":{"@id":"Notification"},"rdfs:comment":"Holds the information related to a client subscription to receive updates to a resource automatically. The actual resources may be passed in the Notification by specifying a specific xsi:type for the Resource and passing the full representation.","sh:property":[{"sh:path":{"@id":"newResourceURI"},"sh:maxCount":1,"sh:datatype":"xsd:anyURI","rdfs:comment":"The new location of the resource, if moved. This attribute SHALL be a fully-qualified absolute URI, not a relative reference."},{"sh:path":{"@id":"Resource"},"sh:maxCount":1,"sh:node":{"@id":"ResourceShape"}},{"sh:path":{"@id":"status"},"sh:minCount":1,"sh:maxCount":1,"sh:minInclusive":0,"sh:maxInclusive":255,"sh:datatype":"xsd:unsignedByte","rdfs:comment":"0 = Default Status\n1 = Subscription canceled, no additional information\n2 = Subscription canceled, resource moved\n3 = Subscription canceled, resource definition changed (e.g., a new version of IEEE 2030.5)\n4 = Subscription canceled, resource deleted\nAll other values reserved."},{"sh:path":{"@id":"subscriptionURI"},"sh:minCount":1,"sh:maxCount":1,"sh:datatype":"xsd:anyURI","rdfs:comment":"The subscription from which this notification was triggered. This attribute SHALL be a fully-qualified absolute URI, not a relative reference."}]},{"@id":"NotificationListShape","@type":"sh:NodeShape","sh:targetClass":{"@id":"NotificationList"},"rdfs:comment":"A List element to hold Notification objects.","sh:property":[{"sh:path":{"@id":"Notification"},"sh:node":{"@id":"NotificationShape"}}]},{"@id":"AppliedTargetReductionShape","@type":"sh:NodeShape","sh:targetClass":{"@id":"AppliedTargetReduction"},"rdfs:comment":"Specifies the value of the TargetReduction applied by the device.","sh:property":[{"sh:path":{"@id":"type"},"sh:in":[0,1,2,3,4,5,6,7,8,9,10,11,12],"sh:minCount":1,"sh:maxCount":1,"sh:minInclusive":0,"sh:maxInclusive":255,"sh:datatype":"xsd:integer","rdfs:comment":"Enumerated field representing the type of reduction requested."},{"sh:path":{"@id":"value"},"sh:minCount":1,"sh:maxCount":1,"sh:minInclusive":0,"sh:maxInclusive":65535,"sh:datatype":"xsd:unsignedShort","rdfs:comment":"Indicates the requested amount of the relevant commodity to be reduced."}]},{"@id":"DrResponseShape","@type":"sh:NodeShape","sh:targetClass":{"@id":"DrResponse"},"rdfs:comment":"A response to a Demand Response Load Control (EndDeviceControl) message.","sh:property":[{"sh:path":{"@id":"ApplianceLoadReduction"},"sh:maxCount":1,"sh:node":{"@id":"ApplianceLoadReductionShape"}},{"sh:path":{"@id":"AppliedTargetReduction"},"sh:maxCount":1,"sh:node":{"@id":"AppliedTargetReductionShape"}},{"sh:path":{"@id":"DutyCycle"},"sh:maxCount":1,"sh:node":{"@id":"DutyCycleShape"}},{"sh:path":{"@id":"Offset"},"sh:maxCount":1,"sh:node":{"@id":"OffsetShape"}},{"sh:path":{"@id":"overrideDuration"},"sh:maxCount":1,"sh:minInclusive":0,"sh:maxInclusive":65535,"sh:datatype":"xsd:unsignedShort","rdfs:comment":"Indicates the amount of time, in seconds, that the client partially opts-out during the demand response event. When overriding within the allowed override duration, the client SHALL send a partial opt-out (Response status code 8) for partial opt-out upon completion, with the total time the event was overridden (this attribute) populated. The client SHALL send a no participation status response (status type 10) if the user partially opts-out for longer than EndDeviceControl.overrideDuration."},{"sh:path":{"@id":"SetPoint"},"sh:maxCount":1,"sh:node":{"@id":"SetPointShape"}}]},{"@id":"ResponseShape","@type":"sh:NodeShape","sh:targetClass":{"@id":"Response"},"rdfs:comment":"The Response object is the generic response data repository which is extended for specific function sets.","sh:property":[{"sh:path":{"@id":"createdDateTime"},"sh:maxCount":1,"sh:datatype":"xsd:integer","rdfs:comment":"The createdDateTime field contains the date and time when the acknowledgement/status occurred in the client. The client will provide the timestamp to ensure the proper time is captured in case the response is delayed in reaching the server (server receipt time would not be the same as the actual confirmation time). The time reported from the client should be relative to the time server indicated by the FunctionSetAssignment that also indicated the event resource; if no FunctionSetAssignment exists, the time of the server where the event resource was hosted."},{"sh:path":{"@id":"endDeviceLFDI"},"sh:minCount":1,"sh:maxCount":1,"sh:datatype":"xsd:hexBinary","rdfs:comment":"Contains the LFDI of the device providing the response."},{"sh:path":{"@id":"status"},"sh:maxCount":1,"sh:minInclusive":0,"sh:maxInclusive":255,"sh:datatype":"xsd:unsignedByte","rdfs:comment":"The status field contains the acknowledgement or status. Each event type (DRLC, DER, Price, or Text) can return different status information (e.g. an Acknowledge will be returned for a Price event where a DRLC event can return Event Received, Event Started, and Event Completed). The Status field value definitions are defined in Table 27: Response Types by Function Set."},{"sh:path":{"@id":"subject"},"sh:minCount":1,"sh:maxCount":1,"sh:datatype":"xsd:string","rdfs:comment":"The subject field provides a method to match the response with the originating event. It is populated with the mRID of the original object."}]},{"@id":"ResponseListShape","@type":"sh:NodeShape","sh:targetClass":{"@id":"ResponseList"},"rdfs:comment":"A List element to hold Response objects.","sh:property":[{"sh:path":{"@id":"Response"},"sh:node":{"@id":"ResponseShape"}}]},{"@id":"ResponseSetShape","@type":"sh:NodeShape","sh:targetClass":{"@id":"ResponseSet"},"rdfs:comment":"A container for a ResponseList.","sh:property":[{"sh:path":{"@id":"ResponseListLink"},"sh:maxCount":1,"sh:datatype":"xsd:string"}]},{"@id":"ResponseSetListShape","@type":"sh:NodeShape","sh:targetClass":{"@id":"ResponseSetList"},"rdfs:comment":"A List element to hold ResponseSet objects.","sh:property":[{"sh:path":{"@id":"ResponseSet"},"sh:node":{"@id":"ResponseSetShape"}},{"sh:path":{"@id":"pollRate"},"sh:maxCount":1,"sh:minInclusive":0,"sh:maxInclusive":4294967295,"sh:datatype":"xsd:unsignedInt","rdfs:comment":"The default polling rate for this function set (this resource and all resources below), in seconds. If not specified, a default of 900 seconds (15 minutes) is used. It is RECOMMENDED a client poll the resources of this function set every pollRate seconds.","sh:defaultValue":"900"}]},{"@id":"TimeShape","@type":"sh:NodeShape","sh:targetClass":{"@id":"Time"},"rdfs:comment":"Contains the representation of time, constantly updated.","sh:property":[{"sh:path":{"@id":"currentTime"},"sh:minCount":1,"sh:maxCount":1,"sh:datatype":"xsd:integer","rdfs:comment":"The current time, in the format defined by TimeType."},{"sh:path":{"@id":"dstEndTime"},"sh:minCount":1,"sh:maxCount":1,"sh:datatype":"xsd:integer","rdfs:comment":"Time at which daylight savings ends (dstOffset no longer applied).  Result of dstEndRule calculation."},{"sh:path":{"@id":"dstOffset"},"sh:minCount":1,"sh:maxCount":1,"sh:datatype":"xsd:integer","rdfs:comment":"Daylight savings time offset from local standard time. A typical practice is advancing clocks one hour when daylight savings time is in effect, which would result in a positive dstOffset."},{"sh:path":{"@id":"dstStartTime"},"sh:minCount":1,"sh:maxCount":1,"sh:datatype":"xsd:integer","rdfs:comment":"Time at which daylight savings begins (apply dstOffset).  Result of dstStartRule calculation."},{"sh:path":{"@id":"localTime"},"sh:maxCount":1,"sh:datatype":"xsd:integer","rdfs:comment":"Local time: localTime = currentTime + tzOffset (+ dstOffset when in effect)."},{"sh:path":{"@id":"quality"},"sh:minCount":1,"sh:maxCount":1,"sh:minInclusive":0,"sh:maxInclusive":255,"sh:datatype":"xsd:unsignedByte","rdfs:comment":"Metric indicating the quality of the time source from which the service acquired time. Lower (smaller) quality enumeration values are assumed to be more accurate.\n3 - time obtained from external authoritative source such as NTP\n4 - time obtained from level 3 source\n5 - time manually set or obtained from level 4 source\n6 - time obtained from level 5 source\n7 - time intentionally uncoordinated\nAll other values are reserved for future use."},{"sh:path":{"@id":"tzOffset"},"sh:minCount":1,"sh:maxCount":1,"sh:datatype":"xsd:integer","rdfs:comment":"Local time zone offset from currentTime. Does not include any daylight savings time offsets. For American time zones, a negative tzOffset SHALL be used (eg, EST = GMT-5 which is -18000)."},{"sh:path":{"@id":"pollRate"},"sh:maxCount":1,"sh:minInclusive":0,"sh:maxInclusive":4294967295,"sh:datatype":"xsd:unsignedInt","rdfs:comment":"The default polling rate for this function set (this resource and all resources below), in seconds. If not specified, a default of 900 seconds (15 minutes) is used. It is RECOMMENDED a client poll the resources of this function set every pollRate seconds.","sh:defaultValue":"900"}]},{"@id":"DeviceInformationShape","@type":"sh:NodeShape","sh:targetClass":{"@id":"DeviceInformation"},"rdfs:comment":"Contains identification and other information about the device that changes very infrequently, typically only when updates are applied, if ever.","sh:property":[{"sh:path":{"@id":"DRLCCapabilities"},"sh:maxCount":1,"sh:node":{"@id":"DRLCCapabilitiesShape"}},{"sh:path":{"@id":"functionsImplemented"},"sh:maxCount":1,"sh:datatype":"xsd:hexBinary","rdfs:comment":"Bitmap indicating the function sets used by the device as a client.\n0 - Device Capability\n1 - Self Device Resource\n2 - End Device Resource\n3 - Function Set Assignments\n4 - Subscription/Notification Mechanism\n5 - Response\n6 - Time\n7 - Device Information\n8 - Power Status\n9 - Network Status\n10 - Log Event\n11 - Configuration Resource\n12 - Software Download\n13 - DRLC\n14 - Metering\n15 - Pricing\n16 - Messaging\n17 - Billing\n18 - Prepayment\n19 - Flow Reservation\n20 - DER Control"},{"sh:path":{"@id":"gpsLocation"},"sh:maxCount":1,"sh:node":{"@id":"GPSLocationTypeShape"},"rdfs:comment":"GPS location of this device."},{"sh:path":{"@id":"lFDI"},"sh:minCount":1,"sh:maxCount":1,"sh:datatype":"xsd:hexBinary","rdfs:comment":"Long form device identifier. See the Security section for full details."},{"sh:path":{"@id":"mfDate"},"sh:minCount":1,"sh:maxCount":1,"sh:datatype":"xsd:integer","rdfs:comment":"Date/time of manufacture"},{"sh:path":{"@id":"mfHwVer"},"sh:minCount":1,"sh:maxCount":1,"sh:datatype":"xsd:string","rdfs:comment":"Manufacturer hardware version"},{"sh:path":{"@id":"mfID"},"sh:minCount":1,"sh:maxCount":1,"sh:minInclusive":0,"sh:maxInclusive":4294967295,"sh:datatype":"xsd:integer","rdfs:comment":"The manufacturer's IANA Enterprise Number."},{"sh:path":{"@id":"mfInfo"},"sh:maxCount":1,"sh:datatype":"xsd:string","rdfs:comment":"Manufacturer dependent information related to the manufacture of this device"},{"sh:path":{"@id":"mfModel"},"sh:minCount":1,"sh:maxCount":1,"sh:datatype":"xsd:string","rdfs:comment":"Manufacturer's model number"},{"sh:path":{"@id":"mfSerNum"},"sh:minCount":1,"sh:maxCount":1,"sh:datatype":"xsd:string","rdfs:comment":"Manufacturer assigned serial number"},{"sh:path":{"@id":"primaryPower"},"sh:in":[0,1,2,3,4,5],"sh:minCount":1,"sh:maxCount":1,"sh:minInclusive":0,"sh:maxInclusive":255,"sh:datatype":"xsd:integer","rdfs:comment":"Primary source of power."},{"sh:path":{"@id":"secondaryPower"},"sh:in":[0,1,2,3,4,5],"sh:minCount":1,"sh:maxCount":1,"sh:minInclusive":0,"sh:maxInclusive":255,"sh:datatype":"xsd:integer","rdfs:comment":"Secondary source of power"},{"sh:path":{"@id":"SupportedLocaleListLink"},"sh:maxCount":1,"sh:datatype":"xsd:string"},{"sh:path":{"@id":"swActTime"},"sh:minCount":1,"sh:maxCount":1,"sh:datatype":"xsd:integer","rdfs:comment":"Activation date/time of currently running software"},{"sh:path":{"@id":"swVer"},"sh:minCount":1,"sh:maxCount":1,"sh:datatype":"xsd:string","rdfs:comment":"Currently running software version"},{"sh:path":{"@id":"pollRate"},"sh:maxCount":1,"sh:minInclusive":0,"sh:maxInclusive":4294967295,"sh:datatype":"xsd:unsignedInt","rdfs:comment":"The default polling rate for this function set (this resource and all resources below), in seconds. If not specified, a default of 900 seconds (15 minutes) is used. It is RECOMMENDED a client poll the resources of this function set every pollRate seconds.","sh:defaultValue":"900"}]},{"@id":"DRLCCapabilitiesShape","@type":"sh:NodeShape","sh:targetClass":{"@id":"DRLCCapabilities"},"rdfs:comment":"Contains information about the static capabilities of the device, to allow service providers to know what types of functions are supported, what the normal operating ranges and limits are, and other similar information, in order to provide better suggestions of applicable programs to receive the maximum benefit.","sh:property":[{"sh:path":{"@id":"averageEnergy"},"sh:minCount":1,"sh:maxCount":1,"sh:node":{"@id":"RealEnergyShape"},"rdfs:comment":"The average hourly energy usage when in normal operating mode."},{"sh:path":{"@id":"maxDemand"},"sh:minCount":1,"sh:maxCount":1,"sh:node":{"@id":"ActivePowerShape"},"rdfs:comment":"The maximum demand rating of this end device."},{"sh:path":{"@id":"optionsImplemented"},"sh:minCount":1,"sh:maxCount":1,"sh:datatype":"xsd:hexBinary","rdfs:comment":"Bitmap indicating the DRLC options implemented by the device.\n0 - Target reduction (kWh)\n1 - Target reduction (kW)\n2 - Target reduction (Watts)\n3 - Target reduction (Cubic Meters)\n4 - Target reduction (Cubic Feet)\n5 - Target reduction (US Gallons)\n6 - Target reduction (Imperial Gallons)\n7 - Target reduction (BTUs)\n8 - Target reduction (Liters)\n9 - Target reduction (kPA (gauge))\n10 - Target reduction (kPA (absolute))\n11 - Target reduction (Mega Joule)\n12 - Target reduction (Unitless)\n13-15 - Reserved\n16 - Temperature set point\n17 - Temperature offset\n18 - Duty cycle\n19 - Load adjustment percentage\n20 - Appliance load reduction\n21-31 - Reserved"}]},{"@id":"SupportedLocaleShape","@type":"sh:NodeShape","sh:targetClass":{"@id":"SupportedLocale"},"rdfs:comment":"Specifies a locale that is supported","sh:property":[{"sh:path":{"@id":"locale"},"sh:minCount":1,"sh:maxCount":1,"sh:datatype":"xsd:string","rdfs:comment":"The code for a locale that is supported"}]},{"@id":"SupportedLocaleListShape","@type":"sh:NodeShape","sh:targetClass":{"@id":"SupportedLocaleList"},"rdfs:comment":"A List element to hold SupportedLocale objects.","sh:property":[{"sh:path":{"@id":"SupportedLocale"},"sh:node":{"@id":"SupportedLocaleShape"}}]},{"@id":"PowerStatusShape","@type":"sh:NodeShape","sh:targetClass":{"@id":"PowerStatus"},"rdfs:comment":"Contains the status of the device's power sources","sh:property":[{"sh:path":{"@id":"batteryStatus"},"sh:minCount":1,"sh:maxCount":1,"sh:minInclusive":0,"sh:maxInclusive":255,"sh:datatype":"xsd:unsignedByte","rdfs:comment":"Battery system status\n\n0 = unknown\n1 = normal (more than LowChargeThreshold remaining)\n2 = low (less than LowChargeThreshold remaining) \n3 = depleted (0% charge remaining)\n4 = not applicable (mains powered only)"},{"sh:path":{"@id":"changedTime"},"sh:minCount":1,"sh:maxCount":1,"sh:datatype":"xsd:integer","rdfs:comment":"The time at which the reported values were recorded."},{"sh:path":{"@id":"currentPowerSource"},"sh:in":[0,1,2,3,4,5],"sh:minCount":1,"sh:maxCount":1,"sh:minInclusive":0,"sh:maxInclusive":255,"sh:datatype":"xsd:integer","rdfs:comment":"This value will be fixed for devices powered by a single source.  This value may change for devices able to transition between multiple power sources (mains to battery backup, etc.)."},{"sh:path":{"@id":"estimatedChargeRemaining"},"sh:maxCount":1,"sh:minInclusive":0,"sh:maxInclusive":65535,"sh:datatype":"xsd:integer","rdfs:comment":"Estimate of remaining battery charge as a percent of full charge."},{"sh:path":{"@id":"estimatedTimeRemaining"},"sh:maxCount":1,"sh:minInclusive":0,"sh:maxInclusive":4294967295,"sh:datatype":"xsd:unsignedInt","rdfs:comment":"Estimated time (in seconds) to total battery charge depletion (under current load)"},{"sh:path":{"@id":"PEVInfo"},"sh:maxCount":1,"sh:node":{"@id":"PEVInfoShape"}},{"sh:path":{"@id":"sessionTimeOnBattery"},"sh:maxCount":1,"sh:minInclusive":0,"sh:maxInclusive":4294967295,"sh:datatype":"xsd:unsignedInt","rdfs:comment":"If the device has a battery, this is the time since the device last switched to battery power, or the time since the device was restarted, whichever is less, in seconds."},{"sh:path":{"@id":"totalTimeOnBattery"},"sh:maxCount":1,"sh:minInclusive":0,"sh:maxInclusive":4294967295,"sh:datatype":"xsd:unsignedInt","rdfs:comment":"If the device has a battery, this is the total time the device has been on battery power, in seconds. It may be reset when the battery is replaced."},{"sh:path":{"@id":"pollRate"},"sh:maxCount":1,"sh:minInclusive":0,"sh:maxInclusive":4294967295,"sh:datatype":"xsd:unsignedInt","rdfs:comment":"The default polling rate for this function set (this resource and all resources below), in seconds. If not specified, a default of 900 seconds (15 minutes) is used. It is RECOMMENDED a client poll the resources of this function set every pollRate seconds.","sh:defaultValue":"900"}]},{"@id":"PEVInfoShape","@type":"sh:NodeShape","sh:targetClass":{"@id":"PEVInfo"},"rdfs:comment":"Contains attributes that can be exposed by PEVs and other devices that have charging requirements.","sh:property":[{"sh:path":{"@id":"chargingPowerNow"},"sh:minCount":1,"sh:maxCount":1,"sh:node":{"@id":"ActivePowerShape"},"rdfs:comment":"This is the actual power flow in or out of the charger or inverter. This is calculated by the vehicle based on actual measurements. This number is positive for charging."},{"sh:path":{"@id":"energyRequestNow"},"sh:minCount":1,"sh:maxCount":1,"sh:node":{"@id":"RealEnergyShape"},"rdfs:comment":"This is the amount of energy that must be transferred from the grid to EVSE and PEV to achieve the target state of charge allowing for charger efficiency and any vehicle and EVSE parasitic loads. This is calculated by the vehicle and changes throughout the connection as forward or reverse power flow change the battery state of charge.  This number is positive for charging."},{"sh:path":{"@id":"maxForwardPower"},"sh:minCount":1,"sh:maxCount":1,"sh:node":{"@id":"ActivePowerShape"},"rdfs:comment":"This is maximum power transfer capability that could be used for charging the PEV to perform the requested energy transfer.  It is the lower of the vehicle or EVSE physical power limitations. It is not based on economic considerations. The vehicle may draw less power than this value based on its charging cycle. The vehicle defines this parameter. This number is positive for charging power flow."},{"sh:path":{"@id":"minimumChargingDuration"},"sh:minCount":1,"sh:maxCount":1,"sh:minInclusive":0,"sh:maxInclusive":4294967295,"sh:datatype":"xsd:unsignedInt","rdfs:comment":"This is computed by the PEV based on the charging profile to complete the energy transfer if the maximum power is authorized.  The value will never be smaller than the ratio of the energy request to the power request because the charging profile may not allow the maximum power to be used throughout the transfer.   This is a critical parameter for determining whether any slack time exists in the charging cycle between the current time and the TCIN."},{"sh:path":{"@id":"targetStateOfCharge"},"sh:minCount":1,"sh:maxCount":1,"sh:minInclusive":0,"sh:maxInclusive":65535,"sh:datatype":"xsd:integer","rdfs:comment":"This is the target state of charge that is to be achieved during charging before the time of departure (TCIN).  The default value is 100%. The value cannot be set to a value less than the actual state of charge."},{"sh:path":{"@id":"timeChargeIsNeeded"},"sh:minCount":1,"sh:maxCount":1,"sh:datatype":"xsd:integer","rdfs:comment":"Time Charge is Needed (TCIN) is the time that the PEV is expected to depart. The value is manually entered using controls and displays in the vehicle or on the EVSE or using a mobile device.  It is authenticated and saved by the PEV.  This value may be updated during a charging session."},{"sh:path":{"@id":"timeChargingStatusPEV"},"sh:minCount":1,"sh:maxCount":1,"sh:datatype":"xsd:integer","rdfs:comment":"This is the time that the parameters are updated, except for changes to TCIN."}]},{"@id":"IEEE_802_15_4Shape","@type":"sh:NodeShape","sh:targetClass":{"@id":"IEEE_802_15_4"},"rdfs:comment":"Contains 802.15.4 link layer specific attributes.","sh:property":[{"sh:path":{"@id":"capabilityInfo"},"sh:minCount":1,"sh:maxCount":1,"sh:datatype":"xsd:hexBinary","rdfs:comment":"As defined by IEEE 802.15.4"},{"sh:path":{"@id":"NeighborListLink"},"sh:maxCount":1,"sh:datatype":"xsd:string"},{"sh:path":{"@id":"shortAddress"},"sh:minCount":1,"sh:maxCount":1,"sh:minInclusive":0,"sh:maxInclusive":65535,"sh:datatype":"xsd:unsignedShort","rdfs:comment":"As defined by IEEE 802.15.4"}]},{"@id":"IPAddrShape","@type":"sh:NodeShape","sh:targetClass":{"@id":"IPAddr"},"rdfs:comment":"An Internet Protocol address object.","sh:property":[{"sh:path":{"@id":"address"},"sh:minCount":1,"sh:maxCount":1,"sh:datatype":"xsd:hexBinary","rdfs:comment":"An IP address value."},{"sh:path":{"@id":"RPLInstanceListLink"},"sh:maxCount":1,"sh:datatype":"xsd:string"}]},{"@id":"IPAddrListShape","@type":"sh:NodeShape","sh:targetClass":{"@id":"IPAddrList"},"rdfs:comment":"List of IPAddr instances.","sh:property":[{"sh:path":{"@id":"IPAddr"},"sh:node":{"@id":"IPAddrShape"}}]},{"@id":"IPInterfaceShape","@type":"sh:NodeShape","sh:targetClass":{"@id":"IPInterface"},"rdfs:comment":"Specific IPInterface resource.  This resource may be thought of as network status information for a specific network (IP) layer interface.","sh:property":[{"sh:path":{"@id":"ifDescr"},"sh:maxCount":1,"sh:datatype":"xsd:string","rdfs:comment":"Use rules from [RFC 2863]."},{"sh:path":{"@id":"ifHighSpeed"},"sh:maxCount":1,"sh:minInclusive":0,"sh:maxInclusive":4294967295,"sh:datatype":"xsd:unsignedInt","rdfs:comment":"Use rules from [RFC 2863]."},{"sh:path":{"@id":"ifInBroadcastPkts"},"sh:maxCount":1,"sh:minInclusive":0,"sh:maxInclusive":4294967295,"sh:datatype":"xsd:unsignedInt","rdfs:comment":"Use rules from [RFC 2863]."},{"sh:path":{"@id":"ifIndex"},"sh:maxCount":1,"sh:minInclusive":0,"sh:maxInclusive":4294967295,"sh:datatype":"xsd:unsignedInt","rdfs:comment":"Use rules from [RFC 2863]."},{"sh:path":{"@id":"ifInDiscards"},"sh:maxCount":1,"sh:minInclusive":0,"sh:maxInclusive":4294967295,"sh:datatype":"xsd:unsignedInt","rdfs:comment":"Use rules from [RFC 2863]. Can be thought of as Input Datagrams Discarded."},{"sh:path":{"@id":"ifInErrors"},"sh:maxCount":1,"sh:minInclusive":0,"sh:maxInclusive":4294967295,"sh:datatype":"xsd:unsignedInt","rdfs:comment":"Use rules from [RFC 2863]."},{"sh:path":{"@id":"ifInMulticastPkts"},"sh:maxCount":1,"sh:minInclusive":0,"sh:maxInclusive":4294967295,"sh:datatype":"xsd:unsignedInt","rdfs:comment":"Use rules from [RFC 2863]. Can be thought of as Multicast Datagrams Received."},{"sh:path":{"@id":"ifInOctets"},"sh:maxCount":1,"sh:minInclusive":0,"sh:maxInclusive":4294967295,"sh:datatype":"xsd:unsignedInt","rdfs:comment":"Use rules from [RFC 2863]. Can be thought of as Bytes Received."},{"sh:path":{"@id":"ifInUcastPkts"},"sh:maxCount":1,"sh:minInclusive":0,"sh:maxInclusive":4294967295,"sh:datatype":"xsd:unsignedInt","rdfs:comment":"Use rules from [RFC 2863]. Can be thought of as Datagrams Received."},{"sh:path":{"@id":"ifInUnknownProtos"},"sh:maxCount":1,"sh:minInclusive":0,"sh:maxInclusive":4294967295,"sh:datatype":"xsd:unsignedInt","rdfs:comment":"Use rules from [RFC 2863]. Can be thought of as Datagrams with Unknown Protocol Received."},{"sh:path":{"@id":"ifMtu"},"sh:maxCount":1,"sh:minInclusive":0,"sh:maxInclusive":4294967295,"sh:datatype":"xsd:unsignedInt","rdfs:comment":"Use rules from [RFC 2863]."},{"sh:path":{"@id":"ifName"},"sh:maxCount":1,"sh:datatype":"xsd:string","rdfs:comment":"Use rules from [RFC 2863]."},{"sh:path":{"@id":"ifOperStatus"},"sh:maxCount":1,"sh:minInclusive":0,"sh:maxInclusive":255,"sh:datatype":"xsd:unsignedByte","rdfs:comment":"Use rules and assignments from [RFC 2863]."},{"sh:path":{"@id":"ifOutBroadcastPkts"},"sh:maxCount":1,"sh:minInclusive":0,"sh:maxInclusive":4294967295,"sh:datatype":"xsd:unsignedInt","rdfs:comment":"Use rules from [RFC 2863]. Can be thought of as Broadcast Datagrams Sent."},{"sh:path":{"@id":"ifOutDiscards"},"sh:maxCount":1,"sh:minInclusive":0,"sh:maxInclusive":4294967295,"sh:datatype":"xsd:unsignedInt","rdfs:comment":"Use rules from [RFC 2863]. Can be thought of as Output Datagrams Discarded."},{"sh:path":{"@id":"ifOutErrors"},"sh:maxCount":1,"sh:minInclusive":0,"sh:maxInclusive":4294967295,"sh:datatype":"xsd:unsignedInt","rdfs:comment":"Use rules from [RFC 2863]."},{"sh:path":{"@id":"ifOutMulticastPkts"},"sh:maxCount":1,"sh:minInclusive":0,"sh:maxInclusive":4294967295,"sh:datatype":"xsd:unsignedInt","rdfs:comment":"Use rules from [RFC 2863]. Can be thought of as Multicast Datagrams Sent."},{"sh:path":{"@id":"ifOutOctets"},"sh:maxCount":1,"sh:minInclusive":0,"sh:maxInclusive":4294967295,"sh:datatype":"xsd:unsignedInt","rdfs:comment":"Use rules from [RFC 2863]. Can be thought of as Bytes Sent."},{"sh:path":{"@id":"ifOutUcastPkts"},"sh:maxCount":1,"sh:minInclusive":0,"sh:maxInclusive":4294967295,"sh:datatype":"xsd:unsignedInt","rdfs:comment":"Use rules from [RFC 2863]. Can be thought of as Datagrams Sent."},{"sh:path":{"@id":"ifPromiscuousMode"},"sh:maxCount":1,"sh:datatype":"xsd:boolean","rdfs:comment":"Use rules from [RFC 2863]."},{"sh:path":{"@id":"ifSpeed"},"sh:maxCount":1,"sh:minInclusive":0,"sh:maxInclusive":4294967295,"sh:datatype":"xsd:unsignedInt","rdfs:comment":"Use rules from [RFC 2863]."},{"sh:path":{"@id":"ifType"},"sh:maxCount":1,"sh:minInclusive":0,"sh:maxInclusive":65535,"sh:datatype":"xsd:unsignedShort","rdfs:comment":"Use rules and assignments from [RFC 2863]."},{"sh:path":{"@id":"IPAddrListLink"},"sh:maxCount":1,"sh:datatype":"xsd:string"},{"sh:path":{"@id":"lastResetTime"},"sh:maxCount":1,"sh:datatype":"xsd:long","rdfs:comment":"Similar to ifLastChange in [RFC 2863]."},{"sh:path":{"@id":"lastUpdatedTime"},"sh:maxCount":1,"sh:datatype":"xsd:long","rdfs:comment":"The date/time of the reported status."},{"sh:path":{"@id":"LLInterfaceListLink"},"sh:maxCount":1,"sh:datatype":"xsd:string"}]},{"@id":"IPInterfaceListShape","@type":"sh:NodeShape","sh:targetClass":{"@id":"IPInterfaceList"},"rdfs:comment":"List of IPInterface instances.","sh:property":[{"sh:path":{"@id":"IPInterface"},"sh:node":{"@id":"IPInterfaceShape"}},{"sh:path":{"@id":"pollRate"},"sh:maxCount":1,"sh:minInclusive":0,"sh:maxInclusive":4294967295,"sh:datatype":"xsd:unsignedInt","rdfs:comment":"The default polling rate for this function set (this resource and all resources below), in seconds. If not specified, a default of 900 seconds (15 minutes) is used. It is RECOMMENDED a client poll the resources of this function set every pollRate seconds.","sh:defaultValue":"900"}]},{"@id":"LLInterfaceShape","@type":"sh:NodeShape","sh:targetClass":{"@id":"LLInterface"},"rdfs:comment":"A link-layer interface object.","sh:property":[{"sh:path":{"@id":"CRCerrors"},"sh:minCount":1,"sh:maxCount":1,"sh:minInclusive":0,"sh:maxInclusive":4294967295,"sh:datatype":"xsd:unsignedInt","rdfs:comment":"Contains the number of CRC errors since reset."},{"sh:path":{"@id":"EUI64"},"sh:minCount":1,"sh:maxCount":1,"sh:datatype":"xsd:hexBinary","rdfs:comment":"Contains the EUI-64 of the link layer interface. 48 bit MAC addresses SHALL be changed into an EUI-64 using the method defined in [RFC 4291], Appendix A. (The method is to insert \"0xFFFE\" as described in the reference.)"},{"sh:path":{"@id":"IEEE_802_15_4"},"sh:maxCount":1,"sh:node":{"@id":"IEEE_802_15_4Shape"}},{"sh:path":{"@id":"linkLayerType"},"sh:minCount":1,"sh:maxCount":1,"sh:minInclusive":0,"sh:maxInclusive":255,"sh:datatype":"xsd:unsignedByte","rdfs:comment":"Specifies the type of link layer interface associated with the IPInterface. Values are below.\n0 = Unspecified \n1 = IEEE 802.3 (Ethernet)\n2 = IEEE 802.11 (WLAN)\n3 = IEEE 802.15 (PAN)\n4 = IEEE 1901 (PLC)\nAll other values reserved."},{"sh:path":{"@id":"LLAckNotRx"},"sh:maxCount":1,"sh:minInclusive":0,"sh:maxInclusive":4294967295,"sh:datatype":"xsd:unsignedInt","rdfs:comment":"Number of times an ACK was not received for a frame transmitted (when ACK was requested)."},{"sh:path":{"@id":"LLCSMAFail"},"sh:maxCount":1,"sh:minInclusive":0,"sh:maxInclusive":4294967295,"sh:datatype":"xsd:unsignedInt","rdfs:comment":"Number of times CSMA failed."},{"sh:path":{"@id":"LLFramesDropRx"},"sh:maxCount":1,"sh:minInclusive":0,"sh:maxInclusive":4294967295,"sh:datatype":"xsd:unsignedInt","rdfs:comment":"Number of dropped receive frames."},{"sh:path":{"@id":"LLFramesDropTx"},"sh:maxCount":1,"sh:minInclusive":0,"sh:maxInclusive":4294967295,"sh:datatype":"xsd:unsignedInt","rdfs:comment":"Number of dropped transmit frames."},{"sh:path":{"@id":"LLFramesRx"},"sh:maxCount":1,"sh:minInclusive":0,"sh:maxInclusive":4294967295,"sh:datatype":"xsd:unsignedInt","rdfs:comment":"Number of link layer frames received."},{"sh:path":{"@id":"LLFramesTx"},"sh:maxCount":1,"sh:minInclusive":0,"sh:maxInclusive":4294967295,"sh:datatype":"xsd:unsignedInt","rdfs:comment":"Number of link layer frames transmitted."},{"sh:path":{"@id":"LLMediaAccessFail"},"sh:maxCount":1,"sh:minInclusive":0,"sh:maxInclusive":4294967295,"sh:datatype":"xsd:unsignedInt","rdfs:comment":"Number of times access to media failed."},{"sh:path":{"@id":"LLOctetsRx"},"sh:maxCount":1,"sh:minInclusive":0,"sh:maxInclusive":4294967295,"sh:datatype":"xsd:unsignedInt","rdfs:comment":"Number of Bytes received."},{"sh:path":{"@id":"LLOctetsTx"},"sh:maxCount":1,"sh:minInclusive":0,"sh:maxInclusive":4294967295,"sh:datatype":"xsd:unsignedInt","rdfs:comment":"Number of Bytes transmitted."},{"sh:path":{"@id":"LLRetryCount"},"sh:maxCount":1,"sh:minInclusive":0,"sh:maxInclusive":4294967295,"sh:datatype":"xsd:unsignedInt","rdfs:comment":"Number of MAC transmit retries."},{"sh:path":{"@id":"LLSecurityErrorRx"},"sh:maxCount":1,"sh:minInclusive":0,"sh:maxInclusive":4294967295,"sh:datatype":"xsd:unsignedInt","rdfs:comment":"Number of receive security errors."},{"sh:path":{"@id":"loWPAN"},"sh:maxCount":1,"sh:node":{"@id":"loWPANShape"}}]},{"@id":"LLInterfaceListShape","@type":"sh:NodeShape","sh:targetClass":{"@id":"LLInterfaceList"},"rdfs:comment":"List of LLInterface instances.","sh:property":[{"sh:path":{"@id":"LLInterface"},"sh:node":{"@id":"LLInterfaceShape"}}]},{"@id":"loWPANShape","@type":"sh:NodeShape","sh:targetClass":{"@id":"loWPAN"},"rdfs:comment":"Contains information specific to 6LoWPAN.","sh:property":[{"sh:path":{"@id":"octetsRx"},"sh:maxCount":1,"sh:minInclusive":0,"sh:maxInclusive":4294967295,"sh:datatype":"xsd:unsignedInt","rdfs:comment":"Number of Bytes received"},{"sh:path":{"@id":"octetsTx"},"sh:maxCount":1,"sh:minInclusive":0,"sh:maxInclusive":4294967295,"sh:datatype":"xsd:unsignedInt","rdfs:comment":"Number of Bytes transmitted"},{"sh:path":{"@id":"packetsRx"},"sh:minCount":1,"sh:maxCount":1,"sh:minInclusive":0,"sh:maxInclusive":4294967295,"sh:datatype":"xsd:unsignedInt","rdfs:comment":"Number of packets received"},{"sh:path":{"@id":"packetsTx"},"sh:minCount":1,"sh:maxCount":1,"sh:minInclusive":0,"sh:maxInclusive":4294967295,"sh:datatype":"xsd:unsignedInt","rdfs:comment":"Number of packets transmitted"},{"sh:path":{"@id":"rxFragError"},"sh:minCount":1,"sh:maxCount":1,"sh:minInclusive":0,"sh:maxInclusive":4294967295,"sh:datatype":"xsd:unsignedInt","rdfs:comment":"Number of errors receiving fragments"}]},{"@id":"NeighborShape","@type":"sh:NodeShape","sh:targetClass":{"@id":"Neighbor"},"rdfs:comment":"Contains 802.15.4 link layer specific attributes.","sh:property":[{"sh:path":{"@id":"isChild"},"sh:minCount":1,"sh:maxCount":1,"sh:datatype":"xsd:boolean","rdfs:comment":"True if the neighbor is a child."},{"sh:path":{"@id":"linkQuality"},"sh:minCount":1,"sh:maxCount":1,"sh:minInclusive":0,"sh:maxInclusive":255,"sh:datatype":"xsd:unsignedByte","rdfs:comment":"The quality of the link, as defined by 802.15.4"},{"sh:path":{"@id":"shortAddress"},"sh:minCount":1,"sh:maxCount":1,"sh:minInclusive":0,"sh:maxInclusive":65535,"sh:datatype":"xsd:unsignedShort","rdfs:comment":"As defined by IEEE 802.15.4"}]},{"@id":"NeighborListShape","@type":"sh:NodeShape","sh:targetClass":{"@id":"NeighborList"},"rdfs:comment":"List of 15.4 neighbors.","sh:property":[{"sh:path":{"@id":"Neighbor"},"sh:node":{"@id":"NeighborShape"}}]},{"@id":"RPLInstanceShape","@type":"sh:NodeShape","sh:targetClass":{"@id":"RPLInstance"},"rdfs:comment":"Specific RPLInstance resource.  This resource may be thought of as network status information for a specific RPL instance associated with IPInterface.","sh:property":[{"sh:path":{"@id":"DODAGid"},"sh:minCount":1,"sh:maxCount":1,"sh:minInclusive":0,"sh:maxInclusive":255,"sh:datatype":"xsd:unsignedByte","rdfs:comment":"See [RFC 6550]."},{"sh:path":{"@id":"DODAGroot"},"sh:minCount":1,"sh:maxCount":1,"sh:datatype":"xsd:boolean","rdfs:comment":"See [RFC 6550]."},{"sh:path":{"@id":"flags"},"sh:minCount":1,"sh:maxCount":1,"sh:minInclusive":0,"sh:maxInclusive":255,"sh:datatype":"xsd:unsignedByte","rdfs:comment":"See [RFC 6550]."},{"sh:path":{"@id":"groundedFlag"},"sh:minCount":1,"sh:maxCount":1,"sh:datatype":"xsd:boolean","rdfs:comment":"See [RFC 6550]."},{"sh:path":{"@id":"MOP"},"sh:minCount":1,"sh:maxCount":1,"sh:minInclusive":0,"sh:maxInclusive":255,"sh:datatype":"xsd:unsignedByte","rdfs:comment":"See [RFC 6550]."},{"sh:path":{"@id":"PRF"},"sh:minCount":1,"sh:maxCount":1,"sh:minInclusive":0,"sh:maxInclusive":255,"sh:datatype":"xsd:unsignedByte","rdfs:comment":"See [RFC 6550]."},{"sh:path":{"@id":"rank"},"sh:minCount":1,"sh:maxCount":1,"sh:minInclusive":0,"sh:maxInclusive":65535,"sh:datatype":"xsd:unsignedShort","rdfs:comment":"See [RFC 6550]."},{"sh:path":{"@id":"RPLInstanceID"},"sh:minCount":1,"sh:maxCount":1,"sh:minInclusive":0,"sh:maxInclusive":255,"sh:datatype":"xsd:unsignedByte","rdfs:comment":"See [RFC 6550]."},{"sh:path":{"@id":"RPLSourceRoutesListLink"},"sh:maxCount":1,"sh:datatype":"xsd:string"},{"sh:path":{"@id":"versionNumber"},"sh:minCount":1,"sh:maxCount":1,"sh:minInclusive":0,"sh:maxInclusive":255,"sh:datatype":"xsd:unsignedByte","rdfs:comment":"See [RFC 6550]."}]},{"@id":"RPLInstanceListShape","@type":"sh:NodeShape","sh:targetClass":{"@id":"RPLInstanceList"},"rdfs:comment":"List of RPLInstances associated with the IPinterface.","sh:property":[{"sh:path":{"@id":"RPLInstance"},"sh:node":{"@id":"RPLInstanceShape"}}]},{"@id":"RPLSourceRoutesShape","@type":"sh:NodeShape","sh:targetClass":{"@id":"RPLSourceRoutes"},"rdfs:comment":"A RPL source routes object.","sh:property":[{"sh:path":{"@id":"DestAddress"},"sh:minCount":1,"sh:maxCount":1,"sh:datatype":"xsd:hexBinary","rdfs:comment":"See [RFC 6554]."},{"sh:path":{"@id":"SourceRoute"},"sh:minCount":1,"sh:maxCount":1,"sh:datatype":"xsd:hexBinary","rdfs:comment":"See [RFC 6554]."}]},{"@id":"RPLSourceRoutesListShape","@type":"sh:NodeShape","sh:targetClass":{"@id":"RPLSourceRoutesList"},"rdfs:comment":"List or RPL source routes if the hosting device is the DODAGroot","sh:property":[{"sh:path":{"@id":"RPLSourceRoutes"},"sh:node":{"@id":"RPLSourceRoutesShape"}}]},{"@id":"LogEventShape","@type":"sh:NodeShape","sh:targetClass":{"@id":"LogEvent"},"rdfs:comment":"A time stamped instance of a significant event detected by the device.","sh:property":[{"sh:path":{"@id":"createdDateTime"},"sh:minCount":1,"sh:maxCount":1,"sh:datatype":"xsd:integer","rdfs:comment":"The date and time that the event occurred."},{"sh:path":{"@id":"details"},"sh:maxCount":1,"sh:datatype":"xsd:string","rdfs:comment":"Human readable text that MAY be used to transmit additional details about the event. A host MAY remove this field when received."},{"sh:path":{"@id":"extendedData"},"sh:maxCount":1,"sh:minInclusive":0,"sh:maxInclusive":4294967295,"sh:datatype":"xsd:unsignedInt","rdfs:comment":"May be used to transmit additional details about the event."},{"sh:path":{"@id":"functionSet"},"sh:minCount":1,"sh:maxCount":1,"sh:minInclusive":0,"sh:maxInclusive":255,"sh:datatype":"xsd:unsignedByte","rdfs:comment":"If the profileID indicates this is IEEE 2030.5, the functionSet is defined by IEEE 2030.5 and SHALL be one of the values from the table below (IEEE 2030.5 function set identifiers). If the profileID is anything else, the functionSet is defined by the identified profile. \n0\tGeneral (not specific to a function set)\n1\tPublish and Subscribe\n2\tEnd Device\n3\tFunction Set Assignment\n4\tResponse\n5\tDemand Response and Load Control\n6\tMetering\n7\tPricing\n8\tMessaging\n9\tBilling\n10\tPrepayment\n11\tDistributed Energy Resources\n12\tTime\n13\tSoftware  Download\n14\tDevice Information\n15\tPower Status\n16\tNetwork Status\n17\tLog Event List\n18\tConfiguration\n19\tSecurity\nAll other values are reserved."},{"sh:path":{"@id":"logEventCode"},"sh:minCount":1,"sh:maxCount":1,"sh:minInclusive":0,"sh:maxInclusive":255,"sh:datatype":"xsd:unsignedByte","rdfs:comment":"An 8 bit unsigned integer. logEventCodes are scoped to a profile and a function set. If the profile is IEEE 2030.5, the logEventCode is defined by IEEE 2030.5 within one of the function sets of IEEE 2030.5. If the profile is anything else, the logEventCode is defined by the specified profile."},{"sh:path":{"@id":"logEventID"},"sh:minCount":1,"sh:maxCount":1,"sh:minInclusive":0,"sh:maxInclusive":65535,"sh:datatype":"xsd:unsignedShort","rdfs:comment":"This 16-bit value, combined with createdDateTime, profileID, and logEventPEN, should provide a reasonable level of uniqueness."},{"sh:path":{"@id":"logEventPEN"},"sh:minCount":1,"sh:maxCount":1,"sh:minInclusive":0,"sh:maxInclusive":4294967295,"sh:datatype":"xsd:integer","rdfs:comment":"The Private Enterprise Number(PEN) of the entity that defined the profileID, functionSet, and logEventCode of the logEvent. IEEE 2030.5-assigned logEventCodes SHALL use the IEEE 2030.5 PEN.  Combinations of profileID, functionSet, and logEventCode SHALL have unique meaning within a logEventPEN and are defined by the owner of the PEN."},{"sh:path":{"@id":"profileID"},"sh:minCount":1,"sh:maxCount":1,"sh:minInclusive":0,"sh:maxInclusive":255,"sh:datatype":"xsd:unsignedByte","rdfs:comment":"The profileID identifies which profile (HA, BA, SE, etc) defines the following event information.\n0\tNot profile specific.\n1\tVendor Defined\n2\tIEEE 2030.5\n3\tHome Automation\n4\tBuilding Automation\nAll other values are reserved."}]},{"@id":"LogEventListShape","@type":"sh:NodeShape","sh:targetClass":{"@id":"LogEventList"},"rdfs:comment":"A List element to hold LogEvent objects.","sh:property":[{"sh:path":{"@id":"LogEvent"},"sh:node":{"@id":"LogEventShape"}},{"sh:path":{"@id":"pollRate"},"sh:maxCount":1,"sh:minInclusive":0,"sh:maxInclusive":4294967295,"sh:datatype":"xsd:unsignedInt","rdfs:comment":"The default polling rate for this function set (this resource and all resources below), in seconds. If not specified, a default of 900 seconds (15 minutes) is used. It is RECOMMENDED a client poll the resources of this function set every pollRate seconds.","sh:defaultValue":"900"}]},{"@id":"ConfigurationShape","@type":"sh:NodeShape","sh:targetClass":{"@id":"Configuration"},"rdfs:comment":"This resource contains various settings to control the operation of the device","sh:property":[{"sh:path":{"@id":"currentLocale"},"sh:minCount":1,"sh:maxCount":1,"sh:datatype":"xsd:string","rdfs:comment":"[RFC 4646] identifier of the language-region currently in use."},{"sh:path":{"@id":"PowerConfiguration"},"sh:maxCount":1,"sh:node":{"@id":"PowerConfigurationShape"}},{"sh:path":{"@id":"PriceResponseCfgListLink"},"sh:maxCount":1,"sh:datatype":"xsd:string"},{"sh:path":{"@id":"TimeConfiguration"},"sh:maxCount":1,"sh:node":{"@id":"TimeConfigurationShape"}},{"sh:path":{"@id":"userDeviceName"},"sh:minCount":1,"sh:maxCount":1,"sh:datatype":"xsd:string","rdfs:comment":"User assigned, convenience name used for network browsing displays, etc.  Example \"My Thermostat\""},{"sh:path":{"@id":"pollRate"},"sh:maxCount":1,"sh:minInclusive":0,"sh:maxInclusive":4294967295,"sh:datatype":"xsd:unsignedInt","rdfs:comment":"The default polling rate for this function set (this resource and all resources below), in seconds. If not specified, a default of 900 seconds (15 minutes) is used. It is RECOMMENDED a client poll the resources of this function set every pollRate seconds.","sh:defaultValue":"900"}]},{"@id":"PowerConfigurationShape","@type":"sh:NodeShape","sh:targetClass":{"@id":"PowerConfiguration"},"rdfs:comment":"Contains configuration related to the device's power sources","sh:property":[{"sh:path":{"@id":"batteryInstallTime"},"sh:maxCount":1,"sh:datatype":"xsd:integer","rdfs:comment":"Time/Date at which battery was installed,"},{"sh:path":{"@id":"lowChargeThreshold"},"sh:maxCount":1,"sh:minInclusive":0,"sh:maxInclusive":4294967295,"sh:datatype":"xsd:unsignedInt","rdfs:comment":"In context of the PowerStatus resource, this is the value of EstimatedTimeRemaining below which BatteryStatus \"low\" is indicated and the PS_LOW_BATTERY is raised."}]},{"@id":"PriceResponseCfgShape","@type":"sh:NodeShape","sh:targetClass":{"@id":"PriceResponseCfg"},"rdfs:comment":"Configuration data that specifies how price responsive devices SHOULD respond to price changes while acting upon a given RateComponent.","sh:property":[{"sh:path":{"@id":"consumeThreshold"},"sh:minCount":1,"sh:maxCount":1,"sh:datatype":"xsd:integer","rdfs:comment":"Price responsive clients acting upon the associated RateComponent SHOULD consume the associated commodity while the price is less than this threshold."},{"sh:path":{"@id":"maxReductionThreshold"},"sh:minCount":1,"sh:maxCount":1,"sh:datatype":"xsd:integer","rdfs:comment":"Price responsive clients acting upon the associated RateComponent SHOULD reduce consumption to the maximum extent possible while the price is greater than this threshold."},{"sh:path":{"@id":"RateComponentLink"},"sh:minCount":1,"sh:maxCount":1,"sh:datatype":"xsd:string"}]},{"@id":"PriceResponseCfgListShape","@type":"sh:NodeShape","sh:targetClass":{"@id":"PriceResponseCfgList"},"rdfs:comment":"A List element to hold PriceResponseCfg objects.","sh:property":[{"sh:path":{"@id":"PriceResponseCfg"},"sh:node":{"@id":"PriceResponseCfgShape"}}]},{"@id":"TimeConfigurationShape","@type":"sh:NodeShape","sh:targetClass":{"@id":"TimeConfiguration"},"rdfs:comment":"Contains attributes related to the configuration of the time service.","sh:property":[{"sh:path":{"@id":"dstEndRule"},"sh:in":["0","1","2","3","4","5","6","7"],"sh:minCount":1,"sh:maxCount":1,"sh:datatype":"xsd:string","rdfs:comment":"Rule to calculate end of daylight savings time in the current year.  Result of dstEndRule must be greater than result of dstStartRule."},{"sh:path":{"@id":"dstOffset"},"sh:minCount":1,"sh:maxCount":1,"sh:datatype":"xsd:integer","rdfs:comment":"Daylight savings time offset from local standard time."},{"sh:path":{"@id":"dstStartRule"},"sh:in":["0","1","2","3","4","5","6","7"],"sh:minCount":1,"sh:maxCount":1,"sh:datatype":"xsd:string","rdfs:comment":"Rule to calculate start of daylight savings time in the current year. Result of dstEndRule must be greater than result of dstStartRule."},{"sh:path":{"@id":"tzOffset"},"sh:minCount":1,"sh:maxCount":1,"sh:datatype":"xsd:integer","rdfs:comment":"Local time zone offset from UTCTime. Does not include any daylight savings time offsets."}]},{"@id":"FileShape","@type":"sh:NodeShape","sh:targetClass":{"@id":"File"},"rdfs:comment":"This resource contains various meta-data describing a file's characteristics.  The meta-data provides general file information and also is used to support filtered queries of file lists","sh:property":[{"sh:path":{"@id":"activateTime"},"sh:maxCount":1,"sh:datatype":"xsd:integer","rdfs:comment":"This element MUST be set to the date/time at which this file is activated. If the activation time is less than or equal to current time, the LD MUST immediately place the file into the activated state (in the case of a firmware file, the file is now the running image).  If the activation time is greater than the current time, the LD MUST wait until the specified activation time is reached, then MUST place the file into the activated state. Omission of this element means that the LD MUST NOT take any action to activate the file until a subsequent GET to this File resource provides an activateTime."},{"sh:path":{"@id":"fileURI"},"sh:minCount":1,"sh:maxCount":1,"sh:datatype":"xsd:anyURI","rdfs:comment":"This element MUST be set to the URI location of the file binary artifact.  This is the BLOB (binary large object) that is actually loaded by the LD"},{"sh:path":{"@id":"lFDI"},"sh:maxCount":1,"sh:datatype":"xsd:hexBinary","rdfs:comment":"This element MUST be set to the LFDI of the device for which this file in targeted."},{"sh:path":{"@id":"mfHwVer"},"sh:maxCount":1,"sh:datatype":"xsd:string","rdfs:comment":"This element MUST be set to the hardware version for which this file is targeted."},{"sh:path":{"@id":"mfID"},"sh:minCount":1,"sh:maxCount":1,"sh:minInclusive":0,"sh:maxInclusive":4294967295,"sh:datatype":"xsd:integer","rdfs:comment":"This element MUST be set to the manufacturer's Private Enterprise Number (assigned by IANA)."},{"sh:path":{"@id":"mfModel"},"sh:minCount":1,"sh:maxCount":1,"sh:datatype":"xsd:string","rdfs:comment":"This element MUST be set to the manufacturer model number for which this file is targeted. The syntax and semantics are left to the manufacturer."},{"sh:path":{"@id":"mfSerNum"},"sh:maxCount":1,"sh:datatype":"xsd:string","rdfs:comment":"This element MUST be set to the manufacturer serial number for which this file is targeted. The syntax and semantics are left to the manufacturer."},{"sh:path":{"@id":"mfVer"},"sh:minCount":1,"sh:maxCount":1,"sh:datatype":"xsd:string","rdfs:comment":"This element MUST be set to the software version information for this file. The syntax and semantics are left to the manufacturer."},{"sh:path":{"@id":"size"},"sh:minCount":1,"sh:maxCount":1,"sh:minInclusive":0,"sh:maxInclusive":4294967295,"sh:datatype":"xsd:unsignedInt","rdfs:comment":"This element MUST be set to the total size (in bytes) of the file referenced by fileURI."},{"sh:path":{"@id":"type"},"sh:minCount":1,"sh:maxCount":1,"sh:datatype":"xsd:hexBinary","rdfs:comment":"A value indicating the type of the file.  MUST be one of the following values:\n00 = Software Image\n01 = Security Credential\n02 = Configuration\n03 = Log\n04\u20137FFF = reserved\n8000-FFFF = Manufacturer defined"}]},{"@id":"FileListShape","@type":"sh:NodeShape","sh:targetClass":{"@id":"FileList"},"rdfs:comment":"A List element to hold File objects.","sh:property":[{"sh:path":{"@id":"File"},"sh:node":{"@id":"FileShape"}},{"sh:path":{"@id":"pollRate"},"sh:maxCount":1,"sh:minInclusive":0,"sh:maxInclusive":4294967295,"sh:datatype":"xsd:unsignedInt","rdfs:comment":"The default polling rate for this function set (this resource and all resources below), in seconds. If not specified, a default of 900 seconds (15 minutes) is used. It is RECOMMENDED a client poll the resources of this function set every pollRate seconds.","sh:defaultValue":"900"}]},{"@id":"FileStatusShape","@type":"sh:NodeShape","sh:targetClass":{"@id":"FileStatus"},"rdfs:comment":"This object provides status of device file load and activation operations.","sh:property":[{"sh:path":{"@id":"activateTime"},"sh:maxCount":1,"sh:datatype":"xsd:integer","rdfs:comment":"Date/time at which this File, referred to by FileLink, will be activated. Omission of or presence and value of this element MUST exactly match omission or presence and value of the activateTime element from the File resource."},{"sh:path":{"@id":"FileLink"},"sh:maxCount":1,"sh:datatype":"xsd:string"},{"sh:path":{"@id":"loadPercent"},"sh:minCount":1,"sh:maxCount":1,"sh:minInclusive":0,"sh:maxInclusive":255,"sh:datatype":"xsd:unsignedByte","rdfs:comment":"This element MUST be set to the percentage of the file, indicated by FileLink, that was loaded during the latest load attempt. This value MUST be reset to 0 each time a load attempt is started for the File indicated by FileLink. This value MUST be increased when an LD receives HTTP response containing file content. This value MUST be set to 100 when the full content of the file has been received by the LD"},{"sh:path":{"@id":"nextRequestAttempt"},"sh:minCount":1,"sh:maxCount":1,"sh:datatype":"xsd:integer","rdfs:comment":"This element MUST be set to the time at which the LD will issue its next GET request for file content from the File indicated by FileLink"},{"sh:path":{"@id":"request503Count"},"sh:minCount":1,"sh:maxCount":1,"sh:minInclusive":0,"sh:maxInclusive":65535,"sh:datatype":"xsd:unsignedShort","rdfs:comment":"This value MUST be reset to 0 when FileLink is first pointed at a new File. This value MUST be incremented each time an \n\nLD receives a 503 error from the FS."},{"sh:path":{"@id":"requestFailCount"},"sh:minCount":1,"sh:maxCount":1,"sh:minInclusive":0,"sh:maxInclusive":65535,"sh:datatype":"xsd:unsignedShort","rdfs:comment":"This value MUST be reset to 0 when FileLink is first pointed at a new File. This value MUST be incremented each time a GET request for file content failed. 503 errors MUST be excluded from this counter."},{"sh:path":{"@id":"status"},"sh:minCount":1,"sh:maxCount":1,"sh:minInclusive":0,"sh:maxInclusive":255,"sh:datatype":"xsd:unsignedByte","rdfs:comment":"Current loading status of the file indicated by FileLink. This element MUST be set to one of the following values:\n0 - No load operation in progress\n1 - File load in progress (first request for file content has been issued by LD)\n2 - File load failed\n3 - File loaded successfully (full content of file has been received by the LD), signature verification in progress\n4 - File signature verification failed\n5 - File signature verified, waiting to activate file.\n6 - File activation failed\n7 - File activation in progress  \n8 - File activated successfully (this state may not be reached/persisted through an image activation)\n9-255 - Reserved for future use."},{"sh:path":{"@id":"statusTime"},"sh:minCount":1,"sh:maxCount":1,"sh:datatype":"xsd:integer","rdfs:comment":"This element MUST be set to the time at which file status transitioned to the value indicated in the status element."},{"sh:path":{"@id":"pollRate"},"sh:maxCount":1,"sh:minInclusive":0,"sh:maxInclusive":4294967295,"sh:datatype":"xsd:unsignedInt","rdfs:comment":"The default polling rate for this function set (this resource and all resources below), in seconds. If not specified, a default of 900 seconds (15 minutes) is used. It is RECOMMENDED a client poll the resources of this function set every pollRate seconds.","sh:defaultValue":"900"}]},{"@id":"LoadShedAvailabilityListShape","@type":"sh:NodeShape","sh:targetClass":{"@id":"LoadShedAvailabilityList"},"rdfs:comment":"A List element to hold LoadShedAvailability objects.","sh:property":[{"sh:path":{"@id":"LoadShedAvailability"},"sh:node":{"@id":"LoadShedAvailabilityShape"}},{"sh:path":{"@id":"pollRate"},"sh:maxCount":1,"sh:minInclusive":0,"sh:maxInclusive":4294967295,"sh:datatype":"xsd:unsignedInt","rdfs:comment":"The default polling rate for this function set (this resource and all resources below), in seconds. If not specified, a default of 900 seconds (15 minutes) is used. It is RECOMMENDED a client poll the resources of this function set every pollRate seconds.","sh:defaultValue":"900"}]},{"@id":"ApplianceLoadReductionShape","@type":"sh:NodeShape","sh:targetClass":{"@id":"ApplianceLoadReduction"},"rdfs:comment":"The ApplianceLoadReduction object is used by a Demand Response service provider to provide signals for ENERGY STAR compliant appliances. See the definition of ApplianceLoadReductionType for more information.","sh:property":[{"sh:path":{"@id":"type"},"sh:in":[0,1],"sh:minCount":1,"sh:maxCount":1,"sh:minInclusive":0,"sh:maxInclusive":255,"sh:datatype":"xsd:integer","rdfs:comment":"Indicates the type of appliance load reduction requested."}]},{"@id":"DemandResponseProgramShape","@type":"sh:NodeShape","sh:targetClass":{"@id":"DemandResponseProgram"},"rdfs:comment":"Demand response program.","sh:property":[{"sh:path":{"@id":"ActiveEndDeviceControlListLink"},"sh:maxCount":1,"sh:datatype":"xsd:string"},{"sh:path":{"@id":"availabilityUpdatePercentChangeThreshold"},"sh:maxCount":1,"sh:minInclusive":0,"sh:maxInclusive":65535,"sh:datatype":"xsd:integer","rdfs:comment":"This attribute allows program providers to specify the requested granularity of updates to LoadShedAvailability sheddablePercent. If not present, or set to 0, then updates to LoadShedAvailability SHALL NOT be provided. If present and greater than zero, then clients SHALL provide their LoadShedAvailability if it has not previously been provided, and thereafter if the difference between the previously provided value and the current value of LoadShedAvailability sheddablePercent is greater than availabilityUpdatePercentChangeThreshold."},{"sh:path":{"@id":"availabilityUpdatePowerChangeThreshold"},"sh:maxCount":1,"sh:node":{"@id":"ActivePowerShape"},"rdfs:comment":"This attribute allows program providers to specify the requested granularity of updates to LoadShedAvailability sheddablePower. If not present, or set to 0, then updates to LoadShedAvailability SHALL NOT be provided. If present and greater than zero, then clients SHALL provide their LoadShedAvailability if it has not previously been provided, and thereafter if the difference between the previously provided value and the current value of LoadShedAvailability sheddablePower is greater than availabilityUpdatePowerChangeThreshold."},{"sh:path":{"@id":"EndDeviceControlListLink"},"sh:maxCount":1,"sh:datatype":"xsd:string"},{"sh:path":{"@id":"primacy"},"sh:minCount":1,"sh:maxCount":1,"sh:minInclusive":0,"sh:maxInclusive":255,"sh:datatype":"xsd:integer","rdfs:comment":"Indicates the relative primacy of the provider of this program."}]},{"@id":"DemandResponseProgramListShape","@type":"sh:NodeShape","sh:targetClass":{"@id":"DemandResponseProgramList"},"rdfs:comment":"A List element to hold DemandResponseProgram objects.","sh:property":[{"sh:path":{"@id":"DemandResponseProgram"},"sh:node":{"@id":"DemandResponseProgramShape"}},{"sh:path":{"@id":"pollRate"},"sh:maxCount":1,"sh:minInclusive":0,"sh:maxInclusive":4294967295,"sh:datatype":"xsd:unsignedInt","rdfs:comment":"The default polling rate for this function set (this resource and all resources below), in seconds. If not specified, a default of 900 seconds (15 minutes) is used. It is RECOMMENDED a client poll the resources of this function set every pollRate seconds.","sh:defaultValue":"900"}]},{"@id":"DutyCycleShape","@type":"sh:NodeShape","sh:targetClass":{"@id":"DutyCycle"},"rdfs:comment":"Duty cycle control is a device specific issue and is managed by the device.  The duty cycle of the device under control should span the shortest practical time period in accordance with the nature of the device under control and the intent of the request for demand reduction.  The default factory setting SHOULD be three minutes for each 10% of duty cycle.  This indicates that the default time period over which a duty cycle is applied is 30 minutes, meaning a 10% duty cycle would cause a device to be ON for 3 minutes.   The \u201coff state\u201d SHALL precede the \u201con state\u201d.","sh:property":[{"sh:path":{"@id":"normalValue"},"sh:minCount":1,"sh:maxCount":1,"sh:minInclusive":0,"sh:maxInclusive":255,"sh:datatype":"xsd:unsignedByte","rdfs:comment":"Contains the maximum On state duty cycle applied by the end device, as a percentage of time.  The field not present indicates that this field has not been used by the end device."}]},{"@id":"EndDeviceControlShape","@type":"sh:NodeShape","sh:targetClass":{"@id":"EndDeviceControl"},"rdfs:comment":"Instructs an EndDevice to perform a specified action.","sh:property":[{"sh:path":{"@id":"ApplianceLoadReduction"},"sh:maxCount":1,"sh:node":{"@id":"ApplianceLoadReductionShape"}},{"sh:path":{"@id":"deviceCategory"},"sh:in":["0","1","2","3","4","5","6","7","8","9","10","11","12","13","14","15","16","17","18","19","20","21","22","23","24","25"],"sh:minCount":1,"sh:maxCount":1,"sh:datatype":"xsd:string","rdfs:comment":"Specifies the bitmap indicating  the categories of devices that SHOULD respond. Devices SHOULD ignore events that do not indicate their device category."},{"sh:path":{"@id":"drProgramMandatory"},"sh:minCount":1,"sh:maxCount":1,"sh:datatype":"xsd:boolean","rdfs:comment":"A flag to indicate if the EndDeviceControl is considered a mandatory event as defined by the service provider issuing the EndDeviceControl. The drProgramMandatory flag alerts the client/user that they will be subject to penalty or ineligibility based on the service provider\u2019s program rules for that deviceCategory."},{"sh:path":{"@id":"DutyCycle"},"sh:maxCount":1,"sh:node":{"@id":"DutyCycleShape"}},{"sh:path":{"@id":"loadShiftForward"},"sh:minCount":1,"sh:maxCount":1,"sh:datatype":"xsd:boolean","rdfs:comment":"Indicates that the event intends to increase consumption. A value of true indicates the intention to increase usage value, and a value of false indicates the intention to decrease usage."},{"sh:path":{"@id":"Offset"},"sh:maxCount":1,"sh:node":{"@id":"OffsetShape"}},{"sh:path":{"@id":"overrideDuration"},"sh:maxCount":1,"sh:minInclusive":0,"sh:maxInclusive":65535,"sh:datatype":"xsd:unsignedShort","rdfs:comment":"The overrideDuration attribute provides a duration, in seconds, for which a client device is allowed to override this EndDeviceControl and still meet the contractual agreement with a service provider without opting out. If overrideDuration is not specified, then it SHALL default to 0."},{"sh:path":{"@id":"SetPoint"},"sh:maxCount":1,"sh:node":{"@id":"SetPointShape"}},{"sh:path":{"@id":"TargetReduction"},"sh:maxCount":1,"sh:node":{"@id":"TargetReductionShape"}}]},{"@id":"EndDeviceControlListShape","@type":"sh:NodeShape","sh:targetClass":{"@id":"EndDeviceControlList"},"rdfs:comment":"A List element to hold EndDeviceControl objects.","sh:property":[{"sh:path":{"@id":"EndDeviceControl"},"sh:node":{"@id":"EndDeviceControlShape"}}]},{"@id":"LoadShedAvailabilityShape","@type":"sh:NodeShape","sh:targetClass":{"@id":"LoadShedAvailability"},"rdfs:comment":"Indicates current consumption status and ability to shed load.","sh:property":[{"sh:path":{"@id":"availabilityDuration"},"sh:maxCount":1,"sh:minInclusive":0,"sh:maxInclusive":4294967295,"sh:datatype":"xsd:unsignedInt","rdfs:comment":"Indicates for how many seconds the consuming device will be able to reduce consumption at the maximum response level."},{"sh:path":{"@id":"DemandResponseProgramLink"},"sh:maxCount":1,"sh:datatype":"xsd:string"},{"sh:path":{"@id":"sheddablePercent"},"sh:maxCount":1,"sh:minInclusive":0,"sh:maxInclusive":65535,"sh:datatype":"xsd:integer","rdfs:comment":"Maximum percent of current operating load that is estimated to be sheddable."},{"sh:path":{"@id":"sheddablePower"},"sh:maxCount":1,"sh:node":{"@id":"ActivePowerShape"},"rdfs:comment":"Maximum amount of current operating load that is estimated to be sheddable, in Watts."}]},{"@id":"OffsetShape","@type":"sh:NodeShape","sh:targetClass":{"@id":"Offset"},"rdfs:comment":"If a temperature offset is sent that causes the heating or cooling temperature set point to exceed the limit boundaries that are programmed into the device, the device SHALL respond by setting the temperature at the limit.\nIf an EDC is being targeted at multiple devices or to a device that controls multiple devices (e.g., EMS), it can provide multiple Offset types within one EDC. For events with multiple Offset types, a client SHALL select the Offset that best fits their operating function. \nAlternatively, an event with a single Offset type can be targeted at an EMS in order to request a percentage load reduction on the average energy usage of the entire premise. An EMS SHOULD use the Metering function set to determine the initial load in the premise, reduce energy consumption by controlling devices at its disposal, and at the conclusion of the event, once again use the Metering function set to determine if the desired load reduction was achieved.","sh:property":[{"sh:path":{"@id":"coolingOffset"},"sh:maxCount":1,"sh:minInclusive":0,"sh:maxInclusive":255,"sh:datatype":"xsd:unsignedByte","rdfs:comment":"The value change requested for the cooling offset, in degree C / 10. The value should be added to the normal set point for cooling, or if loadShiftForward is true, then the value should be subtracted from the normal set point."},{"sh:path":{"@id":"heatingOffset"},"sh:maxCount":1,"sh:minInclusive":0,"sh:maxInclusive":255,"sh:datatype":"xsd:unsignedByte","rdfs:comment":"The value change requested for the heating offset, in degree C / 10. The value should be subtracted for heating, or if loadShiftForward is true, then the value should be added to the normal set point."},{"sh:path":{"@id":"loadAdjustmentPercentageOffset"},"sh:maxCount":1,"sh:minInclusive":0,"sh:maxInclusive":65535,"sh:datatype":"xsd:integer","rdfs:comment":"The value change requested for the load adjustment percentage. The value should be subtracted from the normal setting, or if loadShiftForward is true, then the value should be added to the normal setting."}]},{"@id":"SetPointShape","@type":"sh:NodeShape","sh:targetClass":{"@id":"SetPoint"},"rdfs:comment":"The SetPoint object is used to apply specific temperature set points to a temperature control device. The values of the heatingSetpoint and coolingSetpoint attributes SHALL be calculated as follows:\nCooling/Heating Temperature Set Point / 100 = temperature in degrees Celsius where -273.15\u00b0C &lt;= temperature &lt;= 327.67\u00b0C, corresponding to a Cooling and/or Heating Temperature Set Point. The maximum resolution this format allows is 0.01\u00b0C. \nThe field not present in a Response indicates that this field has not been used by the end device. \nIf a temperature is sent that exceeds the temperature limit boundaries that are programmed into the device, the device SHALL respond by setting the temperature at the limit.","sh:property":[{"sh:path":{"@id":"coolingSetpoint"},"sh:maxCount":1,"sh:datatype":"xsd:short","rdfs:comment":"This attribute represents the cooling temperature set point in degrees Celsius / 100. (Hundredths of a degree C)"},{"sh:path":{"@id":"heatingSetpoint"},"sh:maxCount":1,"sh:datatype":"xsd:short","rdfs:comment":"This attribute represents the heating temperature set point in degrees Celsius / 100. (Hundredths of a degree C)"}]},{"@id":"TargetReductionShape","@type":"sh:NodeShape","sh:targetClass":{"@id":"TargetReduction"},"rdfs:comment":"The TargetReduction object is used by a Demand Response service provider to provide a RECOMMENDED threshold that a device/premises should maintain its consumption below. For example, a service provider can provide a RECOMMENDED threshold of some kWh for a 3-hour event. This means that the device/premises would maintain its consumption below the specified limit for the specified period.","sh:property":[{"sh:path":{"@id":"type"},"sh:in":[0,1,2,3,4,5,6,7,8,9,10,11,12],"sh:minCount":1,"sh:maxCount":1,"sh:minInclusive":0,"sh:maxInclusive":255,"sh:datatype":"xsd:integer","rdfs:comment":"Indicates the type of reduction requested."},{"sh:path":{"@id":"value"},"sh:minCount":1,"sh:maxCount":1,"sh:minInclusive":0,"sh:maxInclusive":65535,"sh:datatype":"xsd:unsignedShort","rdfs:comment":"Indicates the requested amount of the relevant commodity to be reduced."}]},{"@id":"MeterReadingShape","@type":"sh:NodeShape","sh:targetClass":{"@id":"MeterReading"},"rdfs:comment":"Set of values obtained from the meter.","sh:property":[{"sh:path":{"@id":"RateComponentListLink"},"sh:maxCount":1,"sh:datatype":"xsd:string"},{"sh:path":{"@id":"ReadingLink"},"sh:maxCount":1,"sh:datatype":"xsd:string"},{"sh:path":{"@id":"ReadingSetListLink"},"sh:maxCount":1,"sh:datatype":"xsd:string"},{"sh:path":{"@id":"ReadingTypeLink"},"sh:minCount":1,"sh:maxCount":1,"sh:datatype":"xsd:string"}]},{"@id":"MeterReadingListShape","@type":"sh:NodeShape","sh:targetClass":{"@id":"MeterReadingList"},"rdfs:comment":"A List element to hold MeterReading objects.","sh:property":[{"sh:path":{"@id":"MeterReading"},"sh:node":{"@id":"MeterReadingShape"}}]},{"@id":"ReadingShape","@type":"sh:NodeShape","sh:targetClass":{"@id":"Reading"},"rdfs:comment":"Specific value measured by a meter or other asset.","sh:property":[{"sh:path":{"@id":"localID"},"sh:maxCount":1,"sh:datatype":"xsd:hexBinary","rdfs:comment":"The local identifier for this reading within the reading set. localIDs are assigned in order of creation time. For interval data, this value SHALL increase with each interval time, and for block/tier readings, localID SHALL not be specified."},{"sh:path":{"@id":"subscribable"},"sh:in":[0,1,2,3],"sh:maxCount":1,"sh:minInclusive":0,"sh:maxInclusive":255,"sh:datatype":"xsd:integer","rdfs:comment":"Indicates whether or not subscriptions are supported for this resource, and whether or not conditional (thresholds) are supported. If not specified, is \"not subscribable\" (0).","sh:defaultValue":"0"}]},{"@id":"ReadingListShape","@type":"sh:NodeShape","sh:targetClass":{"@id":"ReadingList"},"rdfs:comment":"A List element to hold Reading objects.","sh:property":[{"sh:path":{"@id":"Reading"},"sh:node":{"@id":"ReadingShape"}}]},{"@id":"ReadingSetShape","@type":"sh:NodeShape","sh:targetClass":{"@id":"ReadingSet"},"rdfs:comment":"A set of Readings of the ReadingType indicated by the parent MeterReading.","sh:property":[{"sh:path":{"@id":"ReadingListLink"},"sh:maxCount":1,"sh:datatype":"xsd:string"}]},{"@id":"ReadingSetListShape","@type":"sh:NodeShape","sh:targetClass":{"@id":"ReadingSetList"},"rdfs:comment":"A List element to hold ReadingSet objects.","sh:property":[{"sh:path":{"@id":"ReadingSet"},"sh:node":{"@id":"ReadingSetShape"}}]},{"@id":"ReadingTypeShape","@type":"sh:NodeShape","sh:targetClass":{"@id":"ReadingType"},"rdfs:comment":"Type of data conveyed by a specific Reading. See IEC 61968 Part 9 Annex C for full definitions of these values.","sh:property":[{"sh:path":{"@id":"accumulationBehaviour"},"sh:in":[0,3,4,6,9,12],"sh:maxCount":1,"sh:minInclusive":0,"sh:maxInclusive":255,"sh:datatype":"xsd:integer","rdfs:comment":"The \u201caccumulation behaviour\u201d indicates how the value is represented to accumulate over time."},{"sh:path":{"@id":"calorificValue"},"sh:maxCount":1,"sh:node":{"@id":"UnitValueTypeShape"},"rdfs:comment":"The amount of heat generated when a given mass of fuel is completely burned. The CalorificValue is used to convert the measured volume or mass of gas into kWh. The CalorificValue attribute represents the current active value."},{"sh:path":{"@id":"commodity"},"sh:in":[0,1,2,4,7,8,9,10,11,12,13],"sh:maxCount":1,"sh:minInclusive":0,"sh:maxInclusive":255,"sh:datatype":"xsd:integer","rdfs:comment":"Indicates the commodity applicable to this ReadingType."},{"sh:path":{"@id":"conversionFactor"},"sh:maxCount":1,"sh:node":{"@id":"UnitValueTypeShape"},"rdfs:comment":"Accounts for changes in the volume of gas based on temperature and pressure. The ConversionFactor attribute represents the current active value. The ConversionFactor is dimensionless. The default value for the ConversionFactor is 1, which means no conversion is applied. A price server can advertise a new/different value at any time."},{"sh:path":{"@id":"dataQualifier"},"sh:in":[0,2,8,9,12,29,30],"sh:maxCount":1,"sh:minInclusive":0,"sh:maxInclusive":255,"sh:datatype":"xsd:integer","rdfs:comment":"The data type can be used to describe a salient attribute of the data. Possible values are average, absolute, and etc."},{"sh:path":{"@id":"flowDirection"},"sh:in":[0,1,19],"sh:maxCount":1,"sh:minInclusive":0,"sh:maxInclusive":255,"sh:datatype":"xsd:integer","rdfs:comment":"Anything involving current might have a flow direction. Possible values include forward and reverse."},{"sh:path":{"@id":"intervalLength"},"sh:maxCount":1,"sh:minInclusive":0,"sh:maxInclusive":4294967295,"sh:datatype":"xsd:unsignedInt","rdfs:comment":"Default interval length specified in seconds."},{"sh:path":{"@id":"kind"},"sh:in":[0,3,8,12,37],"sh:maxCount":1,"sh:minInclusive":0,"sh:maxInclusive":255,"sh:datatype":"xsd:integer","rdfs:comment":"Compound class that contains kindCategory and kindIndex"},{"sh:path":{"@id":"maxNumberOfIntervals"},"sh:maxCount":1,"sh:minInclusive":0,"sh:maxInclusive":255,"sh:datatype":"xsd:unsignedByte","rdfs:comment":"To be populated for mirrors of interval data to set the expected number of intervals per ReadingSet. Servers may discard intervals received that exceed this number."},{"sh:path":{"@id":"numberOfConsumptionBlocks"},"sh:maxCount":1,"sh:minInclusive":0,"sh:maxInclusive":255,"sh:datatype":"xsd:unsignedByte","rdfs:comment":"Number of consumption blocks. 0 means not applicable, and is the default if not specified. The value needs to be at least 1 if any actual prices are provided."},{"sh:path":{"@id":"numberOfTouTiers"},"sh:maxCount":1,"sh:minInclusive":0,"sh:maxInclusive":255,"sh:datatype":"xsd:unsignedByte","rdfs:comment":"The number of TOU tiers that can be used by any resource configured by this ReadingType. Servers SHALL populate this value with the largest touTier value that will <i>ever</i> be used while this ReadingType is in effect. Servers SHALL set numberOfTouTiers equal to the number of standard TOU tiers plus the number of CPP tiers that may be used while this ReadingType is in effect. Servers SHALL specify a value between 0 and 255 (inclusive) for numberOfTouTiers (servers providing flat rate pricing SHOULD set numberOfTouTiers to 0, as in practice there is no difference between having no tiers and having one tier)."},{"sh:path":{"@id":"phase"},"sh:in":[0,32,33,40,64,65,66,128,129,132,224],"sh:maxCount":1,"sh:minInclusive":0,"sh:maxInclusive":255,"sh:datatype":"xsd:integer","rdfs:comment":"Contains phase information associated with the type."},{"sh:path":{"@id":"powerOfTenMultiplier"},"sh:in":[0,1,2,3,6,9],"sh:maxCount":1,"sh:datatype":"xsd:integer","rdfs:comment":"Indicates the power of ten multiplier applicable to the unit of measure of this ReadingType."},{"sh:path":{"@id":"subIntervalLength"},"sh:maxCount":1,"sh:minInclusive":0,"sh:maxInclusive":4294967295,"sh:datatype":"xsd:unsignedInt","rdfs:comment":"Default sub-interval length specified in seconds for Readings of ReadingType. Some demand calculations are done over a number of smaller intervals. For example, in a rolling demand calculation, the demand value is defined as the rolling sum of smaller intervals over the intervalLength. The subintervalLength is the length of the smaller interval in this calculation. It SHALL be an integral division of the intervalLength. The number of sub-intervals can be calculated by dividing the intervalLength by the subintervalLength."},{"sh:path":{"@id":"supplyLimit"},"sh:maxCount":1,"sh:datatype":"xsd:unsignedLong","rdfs:comment":"Reflects the supply limit set in the meter. This value can be compared to the Reading value to understand if limits are being approached or exceeded. Units follow the same definition as in this ReadingType."},{"sh:path":{"@id":"tieredConsumptionBlocks"},"sh:maxCount":1,"sh:datatype":"xsd:boolean","rdfs:comment":"Specifies whether or not the consumption blocks are differentiated by TOUTier or not. Default is false, if not specified.\ntrue = consumption accumulated over individual tiers\nfalse = consumption accumulated over all tiers"},{"sh:path":{"@id":"uom"},"sh:in":[0,5,6,23,29,31,33,38,42,61,63,65,67,69,71,72,73,106,119,122,125,128,129,130,131,132,133,134,137,140,155,169],"sh:maxCount":1,"sh:minInclusive":0,"sh:maxInclusive":255,"sh:datatype":"xsd:integer","rdfs:comment":"Indicates the measurement type for the units of measure for the readings of this type."}]},{"@id":"UsagePointShape","@type":"sh:NodeShape","sh:targetClass":{"@id":"UsagePoint"},"rdfs:comment":"Logical point on a network at which consumption or production is either physically measured (e.g. metered) or estimated (e.g. unmetered street lights).","sh:property":[{"sh:path":{"@id":"deviceLFDI"},"sh:maxCount":1,"sh:datatype":"xsd:hexBinary","rdfs:comment":"The LFDI of the source device. This attribute SHALL be present when mirroring."},{"sh:path":{"@id":"MeterReadingListLink"},"sh:maxCount":1,"sh:datatype":"xsd:string"}]},{"@id":"UsagePointListShape","@type":"sh:NodeShape","sh:targetClass":{"@id":"UsagePointList"},"rdfs:comment":"A List element to hold UsagePoint objects.","sh:property":[{"sh:path":{"@id":"UsagePoint"},"sh:node":{"@id":"UsagePointShape"}},{"sh:path":{"@id":"pollRate"},"sh:maxCount":1,"sh:minInclusive":0,"sh:maxInclusive":4294967295,"sh:datatype":"xsd:unsignedInt","rdfs:comment":"The default polling rate for this function set (this resource and all resources below), in seconds. If not specified, a default of 900 seconds (15 minutes) is used. It is RECOMMENDED a client poll the resources of this function set every pollRate seconds.","sh:defaultValue":"900"}]},{"@id":"ConsumptionTariffIntervalShape","@type":"sh:NodeShape","sh:targetClass":{"@id":"ConsumptionTariffInterval"},"rdfs:comment":"One of a sequence of thresholds defined in terms of consumption quantity of a service such as electricity, water, gas, etc. It defines the steps or blocks in a step tariff structure, where startValue simultaneously defines the entry value of this step and the closing value of the previous step. Where consumption is greater than startValue, it falls within this block and where consumption is less than or equal to startValue, it falls within one of the previous blocks.","sh:property":[{"sh:path":{"@id":"consumptionBlock"},"sh:in":[0,1,2,3,4,5,6,7,8,9,10,11,12,13,14,15,16],"sh:minCount":1,"sh:maxCount":1,"sh:minInclusive":0,"sh:maxInclusive":255,"sh:datatype":"xsd:integer","rdfs:comment":"Indicates the consumption block related to the reading. If not specified, is assumed to be \"0 - N/A\"."},{"sh:path":{"@id":"EnvironmentalCost"},"sh:node":{"@id":"EnvironmentalCostShape"}},{"sh:path":{"@id":"price"},"sh:maxCount":1,"sh:datatype":"xsd:integer","rdfs:comment":"The charge for this rate component, per unit of measure defined by the associated ReadingType, in currency specified in TariffProfile. \n\nThe Pricing service provider determines the appropriate price attribute value based on its applicable regulatory rules. For example, price could be net or inclusive of applicable taxes, fees, or levies.\n\nThe Billing function set provides the ability to represent billing information in a more detailed manner."},{"sh:path":{"@id":"startValue"},"sh:minCount":1,"sh:maxCount":1,"sh:datatype":"xsd:unsignedLong","rdfs:comment":"The lowest level of consumption that defines the starting point of this consumption step or block. Thresholds start at zero for each billing period.    \n\nIf specified, the first ConsumptionTariffInterval.startValue for a TimeTariffInteral instance SHALL begin at \"0.\" Subsequent ConsumptionTariffInterval.startValue elements SHALL be greater than the previous one."}]},{"@id":"ConsumptionTariffIntervalListShape","@type":"sh:NodeShape","sh:targetClass":{"@id":"ConsumptionTariffIntervalList"},"rdfs:comment":"A List element to hold ConsumptionTariffInterval objects.","sh:property":[{"sh:path":{"@id":"ConsumptionTariffInterval"},"sh:node":{"@id":"ConsumptionTariffIntervalShape"}}]},{"@id":"EnvironmentalCostShape","@type":"sh:NodeShape","sh:targetClass":{"@id":"EnvironmentalCost"},"rdfs:comment":"Provides alternative or secondary price information for the relevant RateComponent. Supports jurisdictions that seek to convey the environmental price per unit of the specified commodity not expressed in currency.\n\nImplementers and consumers can use this attribute to prioritize operations of their HAN devices (e.g., PEV charging during times of high availability of renewable electricity resources).","sh:property":[{"sh:path":{"@id":"amount"},"sh:minCount":1,"sh:maxCount":1,"sh:minInclusive":0,"sh:maxInclusive":4294967295,"sh:datatype":"xsd:unsignedInt","rdfs:comment":"The estimated or actual environmental or other cost, per commodity unit defined by the ReadingType, for this RateComponent (e.g., grams of carbon dioxide emissions each per kWh)."},{"sh:path":{"@id":"costKind"},"sh:in":[0,1,2,3],"sh:minCount":1,"sh:maxCount":1,"sh:minInclusive":0,"sh:maxInclusive":255,"sh:datatype":"xsd:integer","rdfs:comment":"The kind of cost referred to in the amount."},{"sh:path":{"@id":"costLevel"},"sh:minCount":1,"sh:maxCount":1,"sh:minInclusive":0,"sh:maxInclusive":255,"sh:datatype":"xsd:unsignedByte","rdfs:comment":"The relative level of the amount attribute.  In conjunction with numCostLevels, this attribute informs a device of the relative scarcity of the amount attribute (e.g., a high or low availability of renewable generation).\n\nnumCostLevels and costLevel values SHALL ascend in order of scarcity, where \"0\" signals the lowest relative cost and higher values signal increasing cost.  For example, if numCostLevels is equal to \u201c3,\u201d then if the lowest relative costLevel were equal to \u201c0,\u201d devices would assume this is the lowest relative period to operate.  Likewise, if the costLevel in the next TimeTariffInterval instance is equal to \u201c1,\u201d then the device would assume it is relatively more expensive, in environmental terms, to operate during this TimeTariffInterval instance than the previous one.\n\nThere is no limit to the number of relative price levels other than that indicated in the attribute type, but for practicality, service providers should strive for simplicity and recognize the diminishing returns derived from increasing the numCostLevel value greater than four."},{"sh:path":{"@id":"numCostLevels"},"sh:minCount":1,"sh:maxCount":1,"sh:minInclusive":0,"sh:maxInclusive":255,"sh:datatype":"xsd:unsignedByte","rdfs:comment":"The number of all relative cost levels. \n\nIn conjunction with costLevel, numCostLevels signals the relative scarcity of the commodity for the duration of the TimeTariffInterval instance (e.g., a relative indication of cost). This is useful in providing context for nominal cost signals to consumers or devices that might see a range of amount values from different service providres or from the same service provider."}]},{"@id":"RateComponentShape","@type":"sh:NodeShape","sh:targetClass":{"@id":"RateComponent"},"rdfs:comment":"Specifies the applicable charges for a single component of the rate, which could be generation price or consumption price, for example.","sh:property":[{"sh:path":{"@id":"ActiveTimeTariffIntervalListLink"},"sh:maxCount":1,"sh:datatype":"xsd:string"},{"sh:path":{"@id":"flowRateEndLimit"},"sh:maxCount":1,"sh:node":{"@id":"UnitValueTypeShape"},"rdfs:comment":"Specifies the maximum flow rate (e.g. kW for electricity) for which this RateComponent applies, for the usage point and given rate / tariff. \n\nIn combination with flowRateStartLimit, allows a service provider to define the demand or output characteristics for the particular tariff design.  If a server includes the flowRateEndLimit attribute, then it SHALL also include flowRateStartLimit attribute.\n\nFor example, a service provider\u2019s tariff limits customers to 20 kWs of demand for the given rate structure.  Above this threshold (from 20-50 kWs), there are different demand charges per unit of consumption.  The service provider can use flowRateStartLimit and flowRateEndLimit to describe the demand characteristics of the different rates.  Similarly, these attributes can be used to describe limits on premises DERs that might be producing a commodity and sending it back into the distribution network. \n\nNote: At the time of writing, service provider tariffs with demand-based components were not originally identified as being in scope, and service provider tariffs vary widely in their use of demand components and the method for computing charges.  It is expected that industry groups (e.g., OpenSG) will document requirements in the future that the IEEE 2030.5 community can then use as source material for the next version of IEEE 2030.5."},{"sh:path":{"@id":"flowRateStartLimit"},"sh:maxCount":1,"sh:node":{"@id":"UnitValueTypeShape"},"rdfs:comment":"Specifies the minimum flow rate (e.g., kW for electricity) for which this RateComponent applies, for the usage point and given rate / tariff.\n\nIn combination with flowRateEndLimit, allows a service provider to define the demand or output characteristics for the particular tariff design.  If a server includes the flowRateStartLimit attribute, then it SHALL also include flowRateEndLimit attribute."},{"sh:path":{"@id":"ReadingTypeLink"},"sh:minCount":1,"sh:maxCount":1,"sh:datatype":"xsd:string","rdfs:comment":"Provides indication of the ReadingType with which this price is associated."},{"sh:path":{"@id":"roleFlags"},"sh:minCount":1,"sh:maxCount":1,"sh:datatype":"xsd:string","rdfs:comment":"Specifies the roles that this usage point has been assigned."},{"sh:path":{"@id":"TimeTariffIntervalListLink"},"sh:minCount":1,"sh:maxCount":1,"sh:datatype":"xsd:string"}]},{"@id":"RateComponentListShape","@type":"sh:NodeShape","sh:targetClass":{"@id":"RateComponentList"},"rdfs:comment":"A List element to hold RateComponent objects.","sh:property":[{"sh:path":{"@id":"RateComponent"},"sh:node":{"@id":"RateComponentShape"}}]},{"@id":"TariffProfileShape","@type":"sh:NodeShape","sh:targetClass":{"@id":"TariffProfile"},"rdfs:comment":"A schedule of charges; structure that allows the definition of tariff structures such as step (block) and time of use (tier) when used in conjunction with TimeTariffInterval and ConsumptionTariffInterval.","sh:property":[{"sh:path":{"@id":"currency"},"sh:in":[0,36,124,840,978],"sh:maxCount":1,"sh:minInclusive":0,"sh:maxInclusive":65535,"sh:datatype":"xsd:integer","rdfs:comment":"The currency code indicating the currency for this TariffProfile."},{"sh:path":{"@id":"pricePowerOfTenMultiplier"},"sh:in":[0,1,2,3,6,9],"sh:maxCount":1,"sh:datatype":"xsd:integer","rdfs:comment":"Indicates the power of ten multiplier for the price attribute."},{"sh:path":{"@id":"primacy"},"sh:minCount":1,"sh:maxCount":1,"sh:minInclusive":0,"sh:maxInclusive":255,"sh:datatype":"xsd:integer","rdfs:comment":"Indicates the relative primacy of the provider of this program."},{"sh:path":{"@id":"rateCode"},"sh:maxCount":1,"sh:datatype":"xsd:string","rdfs:comment":"The rate code for this tariff profile.  Provided by the Pricing service provider per its internal business needs and practices and provides a method to identify the specific rate code for the TariffProfile instance.  This would typically not be communicated to the user except to facilitate troubleshooting due to its service provider-specific technical nature."},{"sh:path":{"@id":"RateComponentListLink"},"sh:maxCount":1,"sh:datatype":"xsd:string"},{"sh:path":{"@id":"serviceCategoryKind"},"sh:in":[0,1,2,3,4,5,6],"sh:minCount":1,"sh:maxCount":1,"sh:minInclusive":0,"sh:maxInclusive":255,"sh:datatype":"xsd:integer","rdfs:comment":"The kind of service provided by this usage point."}]},{"@id":"TariffProfileListShape","@type":"sh:NodeShape","sh:targetClass":{"@id":"TariffProfileList"},"rdfs:comment":"A List element to hold TariffProfile objects.","sh:property":[{"sh:path":{"@id":"TariffProfile"},"sh:node":{"@id":"TariffProfileShape"}},{"sh:path":{"@id":"pollRate"},"sh:maxCount":1,"sh:minInclusive":0,"sh:maxInclusive":4294967295,"sh:datatype":"xsd:unsignedInt","rdfs:comment":"The default polling rate for this function set (this resource and all resources below), in seconds. If not specified, a default of 900 seconds (15 minutes) is used. It is RECOMMENDED a client poll the resources of this function set every pollRate seconds.","sh:defaultValue":"900"}]},{"@id":"TimeTariffIntervalShape","@type":"sh:NodeShape","sh:targetClass":{"@id":"TimeTariffInterval"},"rdfs:comment":"Describes the time-differentiated portion of the RateComponent, if applicable, and provides the ability to specify multiple time intervals, each with its own consumption-based components and other attributes.","sh:property":[{"sh:path":{"@id":"ConsumptionTariffIntervalListLink"},"sh:maxCount":1,"sh:datatype":"xsd:string"},{"sh:path":{"@id":"touTier"},"sh:in":[0,1,2,3,4,5,6,7,8,9,10,11,12,13,14,15],"sh:minCount":1,"sh:maxCount":1,"sh:minInclusive":0,"sh:maxInclusive":255,"sh:datatype":"xsd:integer","rdfs:comment":"Indicates the time of use tier related to the reading. If not specified, is assumed to be \"0 - N/A\"."}]},{"@id":"TimeTariffIntervalListShape","@type":"sh:NodeShape","sh:targetClass":{"@id":"TimeTariffIntervalList"},"rdfs:comment":"A List element to hold TimeTariffInterval objects.","sh:property":[{"sh:path":{"@id":"TimeTariffInterval"},"sh:node":{"@id":"TimeTariffIntervalShape"}}]},{"@id":"MessagingProgramShape","@type":"sh:NodeShape","sh:targetClass":{"@id":"MessagingProgram"},"rdfs:comment":"Provides a container for collections of text messages.","sh:property":[{"sh:path":{"@id":"ActiveTextMessageListLink"},"sh:maxCount":1,"sh:datatype":"xsd:string"},{"sh:path":{"@id":"locale"},"sh:minCount":1,"sh:maxCount":1,"sh:datatype":"xsd:string","rdfs:comment":"Indicates the language and region of the messages in this collection."},{"sh:path":{"@id":"primacy"},"sh:minCount":1,"sh:maxCount":1,"sh:minInclusive":0,"sh:maxInclusive":255,"sh:datatype":"xsd:integer","rdfs:comment":"Indicates the relative primacy of the provider of this program."},{"sh:path":{"@id":"TextMessageListLink"},"sh:maxCount":1,"sh:datatype":"xsd:string"}]},{"@id":"MessagingProgramListShape","@type":"sh:NodeShape","sh:targetClass":{"@id":"MessagingProgramList"},"rdfs:comment":"A List element to hold MessagingProgram objects.","sh:property":[{"sh:path":{"@id":"MessagingProgram"},"sh:node":{"@id":"MessagingProgramShape"}},{"sh:path":{"@id":"pollRate"},"sh:maxCount":1,"sh:minInclusive":0,"sh:maxInclusive":4294967295,"sh:datatype":"xsd:unsignedInt","rdfs:comment":"The default polling rate for this function set (this resource and all resources below), in seconds. If not specified, a default of 900 seconds (15 minutes) is used. It is RECOMMENDED a client poll the resources of this function set every pollRate seconds.","sh:defaultValue":"900"}]},{"@id":"TextMessageShape","@type":"sh:NodeShape","sh:targetClass":{"@id":"TextMessage"},"rdfs:comment":"Text message such as a notification.","sh:property":[{"sh:path":{"@id":"originator"},"sh:maxCount":1,"sh:datatype":"xsd:string","rdfs:comment":"Indicates the human-readable name of the publisher of the message"},{"sh:path":{"@id":"priority"},"sh:in":[0,1,2,3],"sh:minCount":1,"sh:maxCount":1,"sh:minInclusive":0,"sh:maxInclusive":255,"sh:datatype":"xsd:integer","rdfs:comment":"The priority is used to inform the client of the priority of the particular message.  Devices with constrained or limited resources for displaying Messages should use this attribute to determine how to handle displaying currently active Messages (e.g. if a device uses a scrolling method with a single Message viewable at a time it MAY want to push a low priority Message to the background and bring a newly received higher priority Message to the foreground)."},{"sh:path":{"@id":"textMessage"},"sh:minCount":1,"sh:maxCount":1,"sh:datatype":"xsd:string","rdfs:comment":"The textMessage attribute contains the actual UTF-8 encoded text to be displayed in conjunction with the messageLength attribute which contains the overall length of the textMessage attribute.  Clients and servers SHALL support a reception of a Message of 100 bytes in length.  Messages that exceed the clients display size will be left to the client to choose what method to handle the message (truncation, scrolling, etc.)."}]},{"@id":"TextMessageListShape","@type":"sh:NodeShape","sh:targetClass":{"@id":"TextMessageList"},"rdfs:comment":"A List element to hold TextMessage objects.","sh:property":[{"sh:path":{"@id":"TextMessage"},"sh:node":{"@id":"TextMessageShape"}}]},{"@id":"BillingPeriodShape","@type":"sh:NodeShape","sh:targetClass":{"@id":"BillingPeriod"},"rdfs:comment":"A Billing Period relates to the period of time on which a customer is billed.  As an example the billing period interval for a particular customer might be 31 days starting on July 1, 2011. The start date and interval can change on each billing period. There may also be multiple billing periods related to a customer agreement to support different tariff structures.","sh:property":[{"sh:path":{"@id":"billLastPeriod"},"sh:maxCount":1,"sh:datatype":"xsd:long","rdfs:comment":"The amount of the bill for the previous billing period."},{"sh:path":{"@id":"billToDate"},"sh:maxCount":1,"sh:datatype":"xsd:long","rdfs:comment":"The bill amount related to the billing period as of the statusTimeStamp."},{"sh:path":{"@id":"interval"},"sh:minCount":1,"sh:maxCount":1,"sh:node":{"@id":"DateTimeIntervalShape"},"rdfs:comment":"The time interval for this billing period."},{"sh:path":{"@id":"statusTimeStamp"},"sh:maxCount":1,"sh:datatype":"xsd:integer","rdfs:comment":"The date / time of the last update of this resource."}]},{"@id":"BillingPeriodListShape","@type":"sh:NodeShape","sh:targetClass":{"@id":"BillingPeriodList"},"rdfs:comment":"A List element to hold BillingPeriod objects.","sh:property":[{"sh:path":{"@id":"BillingPeriod"},"sh:node":{"@id":"BillingPeriodShape"}}]},{"@id":"BillingMeterReadingBaseShape","@type":"sh:NodeShape","sh:targetClass":{"@id":"BillingMeterReadingBase"},"rdfs:comment":"Contains historical, target, and projection readings of various types, possibly associated with charges.","sh:property":[{"sh:path":{"@id":"BillingReadingSetListLink"},"sh:maxCount":1,"sh:datatype":"xsd:string"},{"sh:path":{"@id":"ReadingTypeLink"},"sh:maxCount":1,"sh:datatype":"xsd:string"}]},{"@id":"BillingReadingShape","@type":"sh:NodeShape","sh:targetClass":{"@id":"BillingReading"},"rdfs:comment":"Data captured at regular intervals of time. Interval data could be captured as incremental data, absolute data, or relative data. The source for the data is usually a tariff quantity or an engineering quantity. Data is typically captured in time-tagged, uniform, fixed-length intervals of 5 min, 10 min, 15 min, 30 min, or 60 min. However, consumption aggregations can also be represented with this class.","sh:property":[{"sh:path":{"@id":"Charge"},"sh:node":{"@id":"ChargeShape"}}]},{"@id":"BillingReadingListShape","@type":"sh:NodeShape","sh:targetClass":{"@id":"BillingReadingList"},"rdfs:comment":"A List element to hold BillingReading objects.","sh:property":[{"sh:path":{"@id":"BillingReading"},"sh:node":{"@id":"BillingReadingShape"}}]},{"@id":"BillingReadingSetShape","@type":"sh:NodeShape","sh:targetClass":{"@id":"BillingReadingSet"},"rdfs:comment":"Time sequence of readings of the same reading type.","sh:property":[{"sh:path":{"@id":"BillingReadingListLink"},"sh:maxCount":1,"sh:datatype":"xsd:string"}]},{"@id":"BillingReadingSetListShape","@type":"sh:NodeShape","sh:targetClass":{"@id":"BillingReadingSetList"},"rdfs:comment":"A List element to hold BillingReadingSet objects.","sh:property":[{"sh:path":{"@id":"BillingReadingSet"},"sh:node":{"@id":"BillingReadingSetShape"}}]},{"@id":"ChargeShape","@type":"sh:NodeShape","sh:targetClass":{"@id":"Charge"},"rdfs:comment":"Charges contain charges on a customer bill.  These could be items like taxes, levies, surcharges, rebates, or others.  This is meant to allow the HAN device to retrieve enough information to be able to reconstruct an estimate of what the total bill would look like. \n\nProviders can provide line item billing, including multiple charge kinds (e.g. taxes, surcharges) at whatever granularity desired, using as many Charges as desired during a billing period. There can also be any number of Charges associated with different ReadingTypes to distinguish between TOU tiers, consumption blocks, or demand charges.","sh:property":[{"sh:path":{"@id":"description"},"sh:maxCount":1,"sh:datatype":"xsd:string","rdfs:comment":"A description of the charge."},{"sh:path":{"@id":"kind"},"sh:in":[0,1,2,3,4],"sh:maxCount":1,"sh:minInclusive":0,"sh:maxInclusive":255,"sh:datatype":"xsd:integer","rdfs:comment":"The type (kind) of charge."},{"sh:path":{"@id":"value"},"sh:minCount":1,"sh:maxCount":1,"sh:datatype":"xsd:integer","rdfs:comment":"A monetary charge."}]},{"@id":"CustomerAccountShape","@type":"sh:NodeShape","sh:targetClass":{"@id":"CustomerAccount"},"rdfs:comment":"Assignment of a group of products and services purchased by the Customer through a CustomerAgreement, used as a mechanism for customer billing and payment. It contains common information from the various types of CustomerAgreements to create billings (invoices) for a Customer and receive payment.","sh:property":[{"sh:path":{"@id":"currency"},"sh:minCount":1,"sh:maxCount":1,"sh:minInclusive":0,"sh:maxInclusive":65535,"sh:datatype":"xsd:unsignedShort","rdfs:comment":"The ISO 4217 code indicating the currency applicable to the bill amounts in the summary. See list at http://www.unece.org/cefact/recommendations/rec09/rec09_ecetrd203.pdf"},{"sh:path":{"@id":"customerAccount"},"sh:maxCount":1,"sh:datatype":"xsd:string","rdfs:comment":"The account number for the customer (if applicable)."},{"sh:path":{"@id":"CustomerAgreementListLink"},"sh:maxCount":1,"sh:datatype":"xsd:string"},{"sh:path":{"@id":"customerName"},"sh:maxCount":1,"sh:datatype":"xsd:string","rdfs:comment":"The name of the customer."},{"sh:path":{"@id":"pricePowerOfTenMultiplier"},"sh:in":[0,1,2,3,6,9],"sh:minCount":1,"sh:maxCount":1,"sh:datatype":"xsd:integer","rdfs:comment":"Indicates the power of ten multiplier for the prices in this function set."},{"sh:path":{"@id":"ServiceSupplierLink"},"sh:maxCount":1,"sh:datatype":"xsd:string"}]},{"@id":"CustomerAccountListShape","@type":"sh:NodeShape","sh:targetClass":{"@id":"CustomerAccountList"},"rdfs:comment":"A List element to hold CustomerAccount objects.","sh:property":[{"sh:path":{"@id":"CustomerAccount"},"sh:node":{"@id":"CustomerAccountShape"}},{"sh:path":{"@id":"pollRate"},"sh:maxCount":1,"sh:minInclusive":0,"sh:maxInclusive":4294967295,"sh:datatype":"xsd:unsignedInt","rdfs:comment":"The default polling rate for this function set (this resource and all resources below), in seconds. If not specified, a default of 900 seconds (15 minutes) is used. It is RECOMMENDED a client poll the resources of this function set every pollRate seconds.","sh:defaultValue":"900"}]},{"@id":"CustomerAgreementShape","@type":"sh:NodeShape","sh:targetClass":{"@id":"CustomerAgreement"},"rdfs:comment":"Agreement between the customer and the service supplier to pay for service at a specific service location. It records certain billing information about the type of service provided at the service location and is used during charge creation to determine the type of service.","sh:property":[{"sh:path":{"@id":"ActiveBillingPeriodListLink"},"sh:maxCount":1,"sh:datatype":"xsd:string"},{"sh:path":{"@id":"ActiveProjectionReadingListLink"},"sh:maxCount":1,"sh:datatype":"xsd:string"},{"sh:path":{"@id":"ActiveTargetReadingListLink"},"sh:maxCount":1,"sh:datatype":"xsd:string"},{"sh:path":{"@id":"BillingPeriodListLink"},"sh:maxCount":1,"sh:datatype":"xsd:string"},{"sh:path":{"@id":"HistoricalReadingListLink"},"sh:maxCount":1,"sh:datatype":"xsd:string"},{"sh:path":{"@id":"PrepaymentLink"},"sh:maxCount":1,"sh:datatype":"xsd:string"},{"sh:path":{"@id":"ProjectionReadingListLink"},"sh:maxCount":1,"sh:datatype":"xsd:string"},{"sh:path":{"@id":"serviceAccount"},"sh:maxCount":1,"sh:datatype":"xsd:string","rdfs:comment":"The account number of the service account (if applicable)."},{"sh:path":{"@id":"serviceLocation"},"sh:maxCount":1,"sh:datatype":"xsd:string","rdfs:comment":"The address or textual description of the service location."},{"sh:path":{"@id":"TargetReadingListLink"},"sh:maxCount":1,"sh:datatype":"xsd:string"},{"sh:path":{"@id":"TariffProfileLink"},"sh:maxCount":1,"sh:datatype":"xsd:string"},{"sh:path":{"@id":"UsagePointLink"},"sh:maxCount":1,"sh:datatype":"xsd:string"}]},{"@id":"CustomerAgreementListShape","@type":"sh:NodeShape","sh:targetClass":{"@id":"CustomerAgreementList"},"rdfs:comment":"A List element to hold CustomerAgreement objects.","sh:property":[{"sh:path":{"@id":"CustomerAgreement"},"sh:node":{"@id":"CustomerAgreementShape"}}]},{"@id":"HistoricalReadingListShape","@type":"sh:NodeShape","sh:targetClass":{"@id":"HistoricalReadingList"},"rdfs:comment":"A List element to hold HistoricalReading objects.","sh:property":[{"sh:path":{"@id":"HistoricalReading"},"sh:datatype":"xsd:string"}]},{"@id":"ProjectionReadingListShape","@type":"sh:NodeShape","sh:targetClass":{"@id":"ProjectionReadingList"},"rdfs:comment":"A List element to hold ProjectionReading objects.","sh:property":[{"sh:path":{"@id":"ProjectionReading"},"sh:datatype":"xsd:string"}]},{"@id":"TargetReadingListShape","@type":"sh:NodeShape","sh:targetClass":{"@id":"TargetReadingList"},"rdfs:comment":"A List element to hold TargetReading objects.","sh:property":[{"sh:path":{"@id":"TargetReading"},"sh:datatype":"xsd:string"}]},{"@id":"ServiceSupplierShape","@type":"sh:NodeShape","sh:targetClass":{"@id":"ServiceSupplier"},"rdfs:comment":"Organisation that provides services to Customers.","sh:property":[{"sh:path":{"@id":"email"},"sh:maxCount":1,"sh:datatype":"xsd:string","rdfs:comment":"E-mail address for this service supplier."},{"sh:path":{"@id":"phone"},"sh:maxCount":1,"sh:datatype":"xsd:string","rdfs:comment":"Human-readable phone number for this service supplier."},{"sh:path":{"@id":"providerID"},"sh:maxCount":1,"sh:minInclusive":0,"sh:maxInclusive":4294967295,"sh:datatype":"xsd:unsignedInt","rdfs:comment":"Contains the IANA PEN for the commodity provider."},{"sh:path":{"@id":"web"},"sh:maxCount":1,"sh:datatype":"xsd:string","rdfs:comment":"Website URI address for this service supplier."}]},{"@id":"ServiceSupplierListShape","@type":"sh:NodeShape","sh:targetClass":{"@id":"ServiceSupplierList"},"rdfs:comment":"A List element to hold ServiceSupplier objects.","sh:property":[{"sh:path":{"@id":"ServiceSupplier"},"sh:node":{"@id":"ServiceSupplierShape"}}]},{"@id":"AccountBalanceShape","@type":"sh:NodeShape","sh:targetClass":{"@id":"AccountBalance"},"rdfs:comment":"AccountBalance contains the regular credit and emergency credit balance for this given service or commodity prepay instance. It may also contain status information concerning the balance data.","sh:property":[{"sh:path":{"@id":"availableCredit"},"sh:minCount":1,"sh:maxCount":1,"sh:node":{"@id":"AccountingUnitShape"},"rdfs:comment":"AvailableCredit shows the balance of the sum of credits minus the sum of charges. In a Central Wallet mode this value may be passed down to the Prepayment server via an out-of-band mechanism. In Local or ESI modes, this value may be calculated based upon summation of CreditRegister transactions minus consumption charges calculated using Metering (and possibly Pricing) function set data. This value may be negative; for instance, if disconnection is prevented due to a Supply Interruption Override."},{"sh:path":{"@id":"creditStatus"},"sh:in":[0,1,2,3],"sh:maxCount":1,"sh:minInclusive":0,"sh:maxInclusive":255,"sh:datatype":"xsd:integer","rdfs:comment":"CreditStatus identifies whether the present value of availableCredit is considered OK, low, exhausted, or negative."},{"sh:path":{"@id":"emergencyCredit"},"sh:maxCount":1,"sh:node":{"@id":"AccountingUnitShape"},"rdfs:comment":"EmergencyCredit is the amount of credit still available for the given service or commodity prepayment instance. If both availableCredit and emergyCredit are exhausted, then service will typically be disconnected."},{"sh:path":{"@id":"emergencyCreditStatus"},"sh:in":[0,1,2,3],"sh:maxCount":1,"sh:minInclusive":0,"sh:maxInclusive":255,"sh:datatype":"xsd:integer","rdfs:comment":"EmergencyCreditStatus identifies whether the present value of emergencyCredit is considered OK, low, exhausted, or negative."}]},{"@id":"AccountingUnitShape","@type":"sh:NodeShape","sh:targetClass":{"@id":"AccountingUnit"},"rdfs:comment":"Unit for accounting; use either 'energyUnit' or 'currencyUnit' to specify the unit for 'value'.","sh:property":[{"sh:path":{"@id":"energyUnit"},"sh:maxCount":1,"sh:node":{"@id":"RealEnergyShape"},"rdfs:comment":"Unit of service."},{"sh:path":{"@id":"monetaryUnit"},"sh:in":[0,36,124,840,978],"sh:minCount":1,"sh:maxCount":1,"sh:minInclusive":0,"sh:maxInclusive":65535,"sh:datatype":"xsd:integer","rdfs:comment":"Unit of currency."},{"sh:path":{"@id":"multiplier"},"sh:in":[0,1,2,3,6,9],"sh:minCount":1,"sh:maxCount":1,"sh:datatype":"xsd:integer","rdfs:comment":"Multiplier for the 'energyUnit' or 'monetaryUnit'."},{"sh:path":{"@id":"value"},"sh:minCount":1,"sh:maxCount":1,"sh:datatype":"xsd:integer","rdfs:comment":"Value of the monetary aspect"}]},{"@id":"CreditRegisterShape","@type":"sh:NodeShape","sh:targetClass":{"@id":"CreditRegister"},"rdfs:comment":"CreditRegister instances define a credit-modifying transaction. Typically this would be a credit-adding transaction, but may be a subtracting transaction (perhaps in response to an out-of-band debt signal).","sh:property":[{"sh:path":{"@id":"creditAmount"},"sh:minCount":1,"sh:maxCount":1,"sh:node":{"@id":"AccountingUnitShape"},"rdfs:comment":"CreditAmount is the amount of credit being added by a particular CreditRegister transaction. Negative values indicate that credit is being subtracted."},{"sh:path":{"@id":"creditType"},"sh:in":[0,1,2,3],"sh:maxCount":1,"sh:minInclusive":0,"sh:maxInclusive":255,"sh:datatype":"xsd:integer","rdfs:comment":"CreditType indicates whether the credit transaction applies to regular or emergency credit."},{"sh:path":{"@id":"effectiveTime"},"sh:minCount":1,"sh:maxCount":1,"sh:datatype":"xsd:integer","rdfs:comment":"EffectiveTime identifies the time at which the credit transaction goes into effect. For credit addition transactions, this is typically the moment at which the transaction takes place. For credit subtraction transactions, (e.g., non-fuel debt recovery transactions initiated from a back-haul or ESI) this may be a future time at which credit is deducted."},{"sh:path":{"@id":"token"},"sh:minCount":1,"sh:maxCount":1,"sh:datatype":"xsd:string","rdfs:comment":"Token is security data that authenticates the legitimacy of the transaction. The details of this token are not defined by IEEE 2030.5. How a Prepayment server handles this field is left as vendor specific implementation or will be defined by one or more other standards."}]},{"@id":"CreditRegisterListShape","@type":"sh:NodeShape","sh:targetClass":{"@id":"CreditRegisterList"},"rdfs:comment":"A List element to hold CreditRegister objects.","sh:property":[{"sh:path":{"@id":"CreditRegister"},"sh:node":{"@id":"CreditRegisterShape"}}]},{"@id":"PrepaymentShape","@type":"sh:NodeShape","sh:targetClass":{"@id":"Prepayment"},"rdfs:comment":"Prepayment (inherited from CIM SDPAccountingFunction)","sh:property":[{"sh:path":{"@id":"AccountBalanceLink"},"sh:minCount":1,"sh:maxCount":1,"sh:datatype":"xsd:string"},{"sh:path":{"@id":"ActiveCreditRegisterListLink"},"sh:maxCount":1,"sh:datatype":"xsd:string"},{"sh:path":{"@id":"ActiveSupplyInterruptionOverrideListLink"},"sh:maxCount":1,"sh:datatype":"xsd:string"},{"sh:path":{"@id":"creditExpiryLevel"},"sh:maxCount":1,"sh:node":{"@id":"AccountingUnitShape"},"rdfs:comment":"CreditExpiryLevel is the set point for availableCredit at which the service level may be changed. The typical value for this attribute is 0, regardless of whether the account balance is measured in a monetary or commodity basis. The units for this attribute SHALL match the units used for availableCredit."},{"sh:path":{"@id":"CreditRegisterListLink"},"sh:minCount":1,"sh:maxCount":1,"sh:datatype":"xsd:string"},{"sh:path":{"@id":"lowCreditWarningLevel"},"sh:maxCount":1,"sh:node":{"@id":"AccountingUnitShape"},"rdfs:comment":"LowCreditWarningLevel is the set point for availableCredit at which the creditStatus attribute in the AccountBalance resource SHALL indicate that available credit is low. The units for this attribute SHALL match the units used for availableCredit. Typically, this value is set by the service provider."},{"sh:path":{"@id":"lowEmergencyCreditWarningLevel"},"sh:maxCount":1,"sh:node":{"@id":"AccountingUnitShape"},"rdfs:comment":"LowEmergencyCreditWarningLevel is the set point for emergencyCredit at which the creditStatus attribute in the AccountBalance resource SHALL indicate that emergencycredit is low. The units for this attribute SHALL match the units used for availableCredit. Typically, this value is set by the service provider."},{"sh:path":{"@id":"prepayMode"},"sh:in":[0,1,2,3],"sh:minCount":1,"sh:maxCount":1,"sh:minInclusive":0,"sh:maxInclusive":255,"sh:datatype":"xsd:integer","rdfs:comment":"PrepayMode specifies whether the given Prepayment instance is operating in Credit, Central Wallet, ESI, or Local prepayment mode. The Credit mode indicates that prepayment is not presently in effect. The other modes are described in the Overview Section above."},{"sh:path":{"@id":"PrepayOperationStatusLink"},"sh:minCount":1,"sh:maxCount":1,"sh:datatype":"xsd:string"},{"sh:path":{"@id":"SupplyInterruptionOverrideListLink"},"sh:minCount":1,"sh:maxCount":1,"sh:datatype":"xsd:string"},{"sh:path":{"@id":"UsagePoint"},"sh:node":{"@id":"UsagePointShape"}},{"sh:path":{"@id":"UsagePointLink"},"sh:maxCount":1,"sh:datatype":"xsd:string"}]},{"@id":"PrepaymentListShape","@type":"sh:NodeShape","sh:targetClass":{"@id":"PrepaymentList"},"rdfs:comment":"A List element to hold Prepayment objects.","sh:property":[{"sh:path":{"@id":"Prepayment"},"sh:node":{"@id":"PrepaymentShape"}},{"sh:path":{"@id":"pollRate"},"sh:maxCount":1,"sh:minInclusive":0,"sh:maxInclusive":4294967295,"sh:datatype":"xsd:unsignedInt","rdfs:comment":"The default polling rate for this function set (this resource and all resources below), in seconds. If not specified, a default of 900 seconds (15 minutes) is used. It is RECOMMENDED a client poll the resources of this function set every pollRate seconds.","sh:defaultValue":"900"}]},{"@id":"PrepayOperationStatusShape","@type":"sh:NodeShape","sh:targetClass":{"@id":"PrepayOperationStatus"},"rdfs:comment":"PrepayOperationStatus describes the status of the service or commodity being conditionally controlled by the Prepayment function set.","sh:property":[{"sh:path":{"@id":"creditTypeChange"},"sh:maxCount":1,"sh:node":{"@id":"CreditTypeChangeShape"},"rdfs:comment":"CreditTypeChange is used to define a pending change of creditTypeInUse, which will activate at a specified time."},{"sh:path":{"@id":"creditTypeInUse"},"sh:in":[0,1,2,3],"sh:maxCount":1,"sh:minInclusive":0,"sh:maxInclusive":255,"sh:datatype":"xsd:integer","rdfs:comment":"CreditTypeInUse identifies whether the present mode of operation is consuming regular credit or emergency credit."},{"sh:path":{"@id":"serviceChange"},"sh:maxCount":1,"sh:node":{"@id":"ServiceChangeShape"},"rdfs:comment":"ServiceChange is used to define a pending change of serviceStatus, which will activate at a specified time."},{"sh:path":{"@id":"serviceStatus"},"sh:in":[0,1,2,3,4,5],"sh:minCount":1,"sh:maxCount":1,"sh:minInclusive":0,"sh:maxInclusive":255,"sh:datatype":"xsd:integer","rdfs:comment":"ServiceStatus identifies whether the service is connected or disconnected, or armed for connection or disconnection."}]},{"@id":"ServiceChangeShape","@type":"sh:NodeShape","sh:targetClass":{"@id":"ServiceChange"},"rdfs:comment":"Specifies a change to the service status.","sh:property":[{"sh:path":{"@id":"newStatus"},"sh:in":[0,1,2,3,4,5],"sh:minCount":1,"sh:maxCount":1,"sh:minInclusive":0,"sh:maxInclusive":255,"sh:datatype":"xsd:integer","rdfs:comment":"The new service status, to take effect at the time specified by startTime"},{"sh:path":{"@id":"startTime"},"sh:minCount":1,"sh:maxCount":1,"sh:datatype":"xsd:integer","rdfs:comment":"The date/time when the change is to take effect."}]},{"@id":"SupplyInterruptionOverrideShape","@type":"sh:NodeShape","sh:targetClass":{"@id":"SupplyInterruptionOverride"},"rdfs:comment":"SupplyInterruptionOverride: There may be periods of time when social, regulatory or other concerns mean that service should not be interrupted, even when available credit has been exhausted. Each Prepayment instance links to a List of SupplyInterruptionOverride instances. Each SupplyInterruptionOverride defines a contiguous period of time during which supply SHALL NOT be interrupted.","sh:property":[{"sh:path":{"@id":"description"},"sh:maxCount":1,"sh:datatype":"xsd:string","rdfs:comment":"The description is a human readable text describing or naming the object."},{"sh:path":{"@id":"interval"},"sh:minCount":1,"sh:maxCount":1,"sh:node":{"@id":"DateTimeIntervalShape"},"rdfs:comment":"Interval defines the period of time during which supply should not be interrupted."}]},{"@id":"SupplyInterruptionOverrideListShape","@type":"sh:NodeShape","sh:targetClass":{"@id":"SupplyInterruptionOverrideList"},"rdfs:comment":"A List element to hold SupplyInterruptionOverride objects.","sh:property":[{"sh:path":{"@id":"SupplyInterruptionOverride"},"sh:node":{"@id":"SupplyInterruptionOverrideShape"}}]},{"@id":"CreditTypeChangeShape","@type":"sh:NodeShape","sh:targetClass":{"@id":"CreditTypeChange"},"rdfs:comment":"Specifies a change to the credit type.","sh:property":[{"sh:path":{"@id":"newType"},"sh:in":[0,1,2,3],"sh:minCount":1,"sh:maxCount":1,"sh:minInclusive":0,"sh:maxInclusive":255,"sh:datatype":"xsd:integer","rdfs:comment":"The new credit type, to take effect at the time specified by startTime"},{"sh:path":{"@id":"startTime"},"sh:minCount":1,"sh:maxCount":1,"sh:datatype":"xsd:integer","rdfs:comment":"The date/time when the change is to take effect."}]},{"@id":"RequestStatusShape","@type":"sh:NodeShape","sh:targetClass":{"@id":"RequestStatus"},"rdfs:comment":"The RequestStatus object is used to indicate the current status of a Flow Reservation Request.","sh:property":[{"sh:path":{"@id":"dateTime"},"sh:minCount":1,"sh:maxCount":1,"sh:datatype":"xsd:integer","rdfs:comment":"The dateTime attribute will provide a timestamp of when the request status was set. dateTime MUST be set to the time at which the status change occurred, not a time in the future or past."},{"sh:path":{"@id":"requestStatus"},"sh:minCount":1,"sh:maxCount":1,"sh:minInclusive":0,"sh:maxInclusive":255,"sh:datatype":"xsd:unsignedByte","rdfs:comment":"Field representing the request status type. \n0 = Requested\n1 = Cancelled\nAll other values reserved."}]},{"@id":"FlowReservationRequestShape","@type":"sh:NodeShape","sh:targetClass":{"@id":"FlowReservationRequest"},"rdfs:comment":"Used to request flow transactions. Client EndDevices submit a request for charging or discharging from the server. The server creates an associated FlowReservationResponse containing the charging parameters and interval to provide a lower aggregated demand at the premises, or within a larger part of the distribution system.","sh:property":[{"sh:path":{"@id":"creationTime"},"sh:minCount":1,"sh:maxCount":1,"sh:datatype":"xsd:integer","rdfs:comment":"The time at which the request was created."},{"sh:path":{"@id":"durationRequested"},"sh:maxCount":1,"sh:minInclusive":0,"sh:maxInclusive":65535,"sh:datatype":"xsd:unsignedShort","rdfs:comment":"A value that is calculated by the storage device that defines the minimum duration, in seconds, that it will take to complete the actual flow transaction, including any ramp times and conditioning times, if applicable."},{"sh:path":{"@id":"energyRequested"},"sh:minCount":1,"sh:maxCount":1,"sh:node":{"@id":"SignedRealEnergyShape"},"rdfs:comment":"Indicates the total amount of energy, in Watt-Hours, requested to be transferred between the storage device and the electric power system. Positive values indicate charging and negative values indicate discharging. This sign convention is different than for the DER function where discharging is positive.  Note that the energyRequestNow attribute in the PowerStatus Object must always represent a charging solution and it is not allowed to have a negative value."},{"sh:path":{"@id":"intervalRequested"},"sh:minCount":1,"sh:maxCount":1,"sh:node":{"@id":"DateTimeIntervalShape"},"rdfs:comment":"The time window during which the flow reservation is needed. For example, if an electric vehicle is set with a 7:00 AM time charge is needed, and price drops to the lowest tier at 11:00 PM, then this window would likely be from 11:00 PM until 7:00 AM."},{"sh:path":{"@id":"powerRequested"},"sh:minCount":1,"sh:maxCount":1,"sh:node":{"@id":"ActivePowerShape"},"rdfs:comment":"Indicates the sustained level of power, in Watts, that is requested. For charging this is calculated by the storage device and it represents the charging system capability (which for an electric vehicle must also account for any power limitations due to the EVSE control pilot). For discharging, a lower value than the inverter capability can be used as a target."},{"sh:path":{"@id":"RequestStatus"},"sh:minCount":1,"sh:maxCount":1,"sh:node":{"@id":"RequestStatusShape"}}]},{"@id":"FlowReservationRequestListShape","@type":"sh:NodeShape","sh:targetClass":{"@id":"FlowReservationRequestList"},"rdfs:comment":"A List element to hold FlowReservationRequest objects.","sh:property":[{"sh:path":{"@id":"FlowReservationRequest"},"sh:node":{"@id":"FlowReservationRequestShape"}},{"sh:path":{"@id":"pollRate"},"sh:maxCount":1,"sh:minInclusive":0,"sh:maxInclusive":4294967295,"sh:datatype":"xsd:unsignedInt","rdfs:comment":"The default polling rate for this function set (this resource and all resources below), in seconds. If not specified, a default of 900 seconds (15 minutes) is used. It is RECOMMENDED a client poll the resources of this function set every pollRate seconds.","sh:defaultValue":"900"}]},{"@id":"FlowReservationResponseShape","@type":"sh:NodeShape","sh:targetClass":{"@id":"FlowReservationResponse"},"rdfs:comment":"The server may modify the charging or discharging parameters and interval to provide a lower aggregated demand at the premises, or within a larger part of the distribution system.","sh:property":[{"sh:path":{"@id":"energyAvailable"},"sh:minCount":1,"sh:maxCount":1,"sh:node":{"@id":"SignedRealEnergyShape"},"rdfs:comment":"Indicates the amount of energy available."},{"sh:path":{"@id":"powerAvailable"},"sh:minCount":1,"sh:maxCount":1,"sh:node":{"@id":"ActivePowerShape"},"rdfs:comment":"Indicates the amount of power available."},{"sh:path":{"@id":"subject"},"sh:minCount":1,"sh:maxCount":1,"sh:datatype":"xsd:string","rdfs:comment":"The subject field provides a method to match the response with the originating event. It is populated with the mRID of the corresponding FlowReservationRequest object."}]},{"@id":"FlowReservationResponseListShape","@type":"sh:NodeShape","sh:targetClass":{"@id":"FlowReservationResponseList"},"rdfs:comment":"A List element to hold FlowReservationResponse objects.","sh:property":[{"sh:path":{"@id":"FlowReservationResponse"},"sh:node":{"@id":"FlowReservationResponseShape"}},{"sh:path":{"@id":"pollRate"},"sh:maxCount":1,"sh:minInclusive":0,"sh:maxInclusive":4294967295,"sh:datatype":"xsd:unsignedInt","rdfs:comment":"The default polling rate for this function set (this resource and all resources below), in seconds. If not specified, a default of 900 seconds (15 minutes) is used. It is RECOMMENDED a client poll the resources of this function set every pollRate seconds.","sh:defaultValue":"900"}]},{"@id":"DefaultDERControlShape","@type":"sh:NodeShape","sh:targetClass":{"@id":"DefaultDERControl"},"rdfs:comment":"Contains control mode information to be used if no active DERControl is found.","sh:property":[{"sh:path":{"@id":"DERControlBase"},"sh:minCount":1,"sh:maxCount":1,"sh:node":{"@id":"DERControlBaseShape"}},{"sh:path":{"@id":"setESDelay"},"sh:maxCount":1,"sh:minInclusive":0,"sh:maxInclusive":4294967295,"sh:datatype":"xsd:unsignedInt","rdfs:comment":"Enter service delay, in hundredths of a second. When present, this value SHALL update the value of the corresponding setting (DERSettings::setESDelay)."},{"sh:path":{"@id":"setESHighFreq"},"sh:maxCount":1,"sh:minInclusive":0,"sh:maxInclusive":65535,"sh:datatype":"xsd:unsignedShort","rdfs:comment":"Enter service frequency high. Specified in hundredths of Hz. When present, this value SHALL update the value of the corresponding setting (DERSettings::setESHighFreq)."},{"sh:path":{"@id":"setESHighVolt"},"sh:maxCount":1,"sh:datatype":"xsd:short","rdfs:comment":"Enter service voltage high. Specified as an effective percent voltage, defined as (100% * (locally measured voltage - setVRefOfs) / setVRef), in hundredths of a percent. When present, this value SHALL update the value of the corresponding setting (DERSettings::setESHighVolt)."},{"sh:path":{"@id":"setESLowFreq"},"sh:maxCount":1,"sh:minInclusive":0,"sh:maxInclusive":65535,"sh:datatype":"xsd:unsignedShort","rdfs:comment":"Enter service frequency low. Specified in hundredths of Hz. When present, this value SHALL update the value of the corresponding setting (DERSettings::setESLowFreq)."},{"sh:path":{"@id":"setESLowVolt"},"sh:maxCount":1,"sh:datatype":"xsd:short","rdfs:comment":"Enter service voltage low. Specified as an effective percent voltage, defined as (100% * (locally measured voltage - setVRefOfs) / setVRef), in hundredths of a percent. When present, this value SHALL update the value of the corresponding setting (DERSettings::setESLowVolt)."},{"sh:path":{"@id":"setESRampTms"},"sh:maxCount":1,"sh:minInclusive":0,"sh:maxInclusive":4294967295,"sh:datatype":"xsd:unsignedInt","rdfs:comment":"Enter service ramp time, in hundredths of a second. When present, this value SHALL update the value of the corresponding setting (DERSettings::setESRampTms)."},{"sh:path":{"@id":"setESRandomDelay"},"sh:maxCount":1,"sh:minInclusive":0,"sh:maxInclusive":4294967295,"sh:datatype":"xsd:unsignedInt","rdfs:comment":"Enter service randomized delay, in hundredths of a second. When present, this value SHALL update the value of the corresponding setting (DERSettings::setESRandomDelay)."},{"sh:path":{"@id":"setGradW"},"sh:maxCount":1,"sh:minInclusive":0,"sh:maxInclusive":65535,"sh:datatype":"xsd:unsignedShort","rdfs:comment":"Set default rate of change (ramp rate) of active power output due to command or internal action, defined in %setWMax / second.  Resolution is in hundredths of a percent/second. A value of 0 means there is no limit. Interpreted as a percentage change in output capability limit per second when used as a default ramp rate. When present, this value SHALL update the value of the corresponding setting (DERSettings::setGradW)."},{"sh:path":{"@id":"setSoftGradW"},"sh:maxCount":1,"sh:minInclusive":0,"sh:maxInclusive":65535,"sh:datatype":"xsd:unsignedShort","rdfs:comment":"Set soft-start rate of change (soft-start ramp rate) of active power output due to command or internal action, defined in %setWMax / second.  Resolution is in hundredths of a percent/second. A value of 0 means there is no limit. Interpreted as a percentage change in output capability limit per second when used as a ramp rate. When present, this value SHALL update the value of the corresponding setting (DERSettings::setSoftGradW)."}]},{"@id":"FreqDroopTypeShape","@type":"sh:NodeShape","sh:targetClass":{"@id":"FreqDroopType"},"rdfs:comment":"Type for Frequency-Droop (Frequency-Watt) operation.","sh:property":[{"sh:path":{"@id":"dBOF"},"sh:minCount":1,"sh:maxCount":1,"sh:minInclusive":0,"sh:maxInclusive":4294967295,"sh:datatype":"xsd:unsignedInt","rdfs:comment":"Frequency droop dead band for over-frequency conditions. In thousandths of Hz."},{"sh:path":{"@id":"dBUF"},"sh:minCount":1,"sh:maxCount":1,"sh:minInclusive":0,"sh:maxInclusive":4294967295,"sh:datatype":"xsd:unsignedInt","rdfs:comment":"Frequency droop dead band for under-frequency conditions. In thousandths of Hz."},{"sh:path":{"@id":"kOF"},"sh:minCount":1,"sh:maxCount":1,"sh:minInclusive":0,"sh:maxInclusive":65535,"sh:datatype":"xsd:unsignedShort","rdfs:comment":"Frequency droop per-unit frequency change for over-frequency conditions corresponding to 1 per-unit power output change. In thousandths, unitless."},{"sh:path":{"@id":"kUF"},"sh:minCount":1,"sh:maxCount":1,"sh:minInclusive":0,"sh:maxInclusive":65535,"sh:datatype":"xsd:unsignedShort","rdfs:comment":"Frequency droop per-unit frequency change for under-frequency conditions corresponding to 1 per-unit power output change. In thousandths, unitless."},{"sh:path":{"@id":"openLoopTms"},"sh:minCount":1,"sh:maxCount":1,"sh:minInclusive":0,"sh:maxInclusive":65535,"sh:datatype":"xsd:unsignedShort","rdfs:comment":"Open loop response time, the duration from a step change in control signal input until the output changes by 90% of its final change before any overshoot, in hundredths of a second. Resolution is 1/100 sec. A value of 0 is used to mean no limit."}]},{"@id":"DERShape","@type":"sh:NodeShape","sh:targetClass":{"@id":"DER"},"rdfs:comment":"Contains links to DER resources.","sh:property":[{"sh:path":{"@id":"AssociatedDERProgramListLink"},"sh:maxCount":1,"sh:datatype":"xsd:string"},{"sh:path":{"@id":"AssociatedUsagePointLink"},"sh:maxCount":1,"sh:datatype":"xsd:string"},{"sh:path":{"@id":"CurrentDERProgramLink"},"sh:maxCount":1,"sh:datatype":"xsd:string"},{"sh:path":{"@id":"DERAvailabilityLink"},"sh:maxCount":1,"sh:datatype":"xsd:string"},{"sh:path":{"@id":"DERCapabilityLink"},"sh:maxCount":1,"sh:datatype":"xsd:string"},{"sh:path":{"@id":"DERSettingsLink"},"sh:maxCount":1,"sh:datatype":"xsd:string"},{"sh:path":{"@id":"DERStatusLink"},"sh:maxCount":1,"sh:datatype":"xsd:string"}]},{"@id":"DERListShape","@type":"sh:NodeShape","sh:targetClass":{"@id":"DERList"},"rdfs:comment":"A List element to hold DER objects.","sh:property":[{"sh:path":{"@id":"DER"},"sh:node":{"@id":"DERShape"}},{"sh:path":{"@id":"pollRate"},"sh:maxCount":1,"sh:minInclusive":0,"sh:maxInclusive":4294967295,"sh:datatype":"xsd:unsignedInt","rdfs:comment":"The default polling rate for this function set (this resource and all resources below), in seconds. If not specified, a default of 900 seconds (15 minutes) is used. It is RECOMMENDED a client poll the resources of this function set every pollRate seconds.","sh:defaultValue":"900"}]},{"@id":"DERSettingsShape","@type":"sh:NodeShape","sh:targetClass":{"@id":"DERSettings"},"rdfs:comment":"Distributed energy resource settings","sh:property":[{"sh:path":{"@id":"modesEnabled"},"sh:in":["0","1","2","3","4","5","6","7","8","9","10","11","12","13","14","15","16","17","18","19","20","21","22","23","24","25","26"],"sh:maxCount":1,"sh:datatype":"xsd:string","rdfs:comment":"Bitmap indicating the DER Controls enabled on the device. See DERControlType for values. If a control is supported (see DERCapability::modesSupported), but not enabled, the control will not be executed if encountered."},{"sh:path":{"@id":"setESDelay"},"sh:maxCount":1,"sh:minInclusive":0,"sh:maxInclusive":4294967295,"sh:datatype":"xsd:unsignedInt","rdfs:comment":"Enter service delay, in hundredths of a second."},{"sh:path":{"@id":"setESHighFreq"},"sh:maxCount":1,"sh:minInclusive":0,"sh:maxInclusive":65535,"sh:datatype":"xsd:unsignedShort","rdfs:comment":"Enter service frequency high. Specified in hundredths of Hz."},{"sh:path":{"@id":"setESHighVolt"},"sh:maxCount":1,"sh:datatype":"xsd:short","rdfs:comment":"Enter service voltage high. Specified as an effective percent voltage, defined as (100% * (locally measured voltage - setVRefOfs) / setVRef), in hundredths of a percent."},{"sh:path":{"@id":"setESLowFreq"},"sh:maxCount":1,"sh:minInclusive":0,"sh:maxInclusive":65535,"sh:datatype":"xsd:unsignedShort","rdfs:comment":"Enter service frequency low. Specified in hundredths of Hz."},{"sh:path":{"@id":"setESLowVolt"},"sh:maxCount":1,"sh:datatype":"xsd:short","rdfs:comment":"Enter service voltage low. Specified as an effective percent voltage, defined as (100% * (locally measured voltage - setVRefOfs) / setVRef), in hundredths of a percent."},{"sh:path":{"@id":"setESRampTms"},"sh:maxCount":1,"sh:minInclusive":0,"sh:maxInclusive":4294967295,"sh:datatype":"xsd:unsignedInt","rdfs:comment":"Enter service ramp time, in hundredths of a second."},{"sh:path":{"@id":"setESRandomDelay"},"sh:maxCount":1,"sh:minInclusive":0,"sh:maxInclusive":4294967295,"sh:datatype":"xsd:unsignedInt","rdfs:comment":"Enter service randomized delay, in hundredths of a second."},{"sh:path":{"@id":"setGradW"},"sh:minCount":1,"sh:maxCount":1,"sh:minInclusive":0,"sh:maxInclusive":65535,"sh:datatype":"xsd:unsignedShort","rdfs:comment":"Set default rate of change (ramp rate) of active power output due to command or internal action, defined in %setWMax / second.  Resolution is in hundredths of a percent/second. A value of 0 means there is no limit. Interpreted as a percentage change in output capability limit per second when used as a default ramp rate."},{"sh:path":{"@id":"setMaxA"},"sh:maxCount":1,"sh:node":{"@id":"CurrentRMSShape"},"rdfs:comment":"AC current maximum. Maximum AC current in RMS Amperes."},{"sh:path":{"@id":"setMaxAh"},"sh:maxCount":1,"sh:node":{"@id":"AmpereHourShape"},"rdfs:comment":"Maximum usable energy storage capacity of the DER, in AmpHours. Note: this may be different from physical capability."},{"sh:path":{"@id":"setMaxChargeRateVA"},"sh:maxCount":1,"sh:node":{"@id":"ApparentPowerShape"},"rdfs:comment":"Apparent power charge maximum. Maximum apparent power the DER can absorb from the grid in Volt-Amperes. May differ from the apparent power maximum (setMaxVA)."},{"sh:path":{"@id":"setMaxChargeRateW"},"sh:maxCount":1,"sh:node":{"@id":"ActivePowerShape"},"rdfs:comment":"Maximum rate of energy transfer received by the storage device, in Watts. Defaults to rtgMaxChargeRateW."},{"sh:path":{"@id":"setMaxDischargeRateVA"},"sh:maxCount":1,"sh:node":{"@id":"ApparentPowerShape"},"rdfs:comment":"Apparent power discharge maximum. Maximum apparent power the DER can deliver to the grid in Volt-Amperes. May differ from the apparent power maximum (setMaxVA)."},{"sh:path":{"@id":"setMaxDischargeRateW"},"sh:maxCount":1,"sh:node":{"@id":"ActivePowerShape"},"rdfs:comment":"Maximum rate of energy transfer delivered by the storage device, in Watts. Defaults to rtgMaxDischargeRateW."},{"sh:path":{"@id":"setMaxV"},"sh:maxCount":1,"sh:node":{"@id":"VoltageRMSShape"},"rdfs:comment":"AC voltage maximum setting."},{"sh:path":{"@id":"setMaxVA"},"sh:maxCount":1,"sh:node":{"@id":"ApparentPowerShape"},"rdfs:comment":"Set limit for maximum apparent power capability of the DER (in VA). Defaults to rtgMaxVA."},{"sh:path":{"@id":"setMaxVar"},"sh:maxCount":1,"sh:node":{"@id":"ReactivePowerShape"},"rdfs:comment":"Set limit for maximum reactive power delivered by the DER (in var). SHALL be a positive value &lt;= rtgMaxVar (default)."},{"sh:path":{"@id":"setMaxVarNeg"},"sh:maxCount":1,"sh:node":{"@id":"ReactivePowerShape"},"rdfs:comment":"Set limit for maximum reactive power received by the DER (in var). If present, SHALL be a negative value &gt;= rtgMaxVarNeg (default). If absent, defaults to negative setMaxVar."},{"sh:path":{"@id":"setMaxW"},"sh:minCount":1,"sh:maxCount":1,"sh:node":{"@id":"ActivePowerShape"},"rdfs:comment":"Set limit for maximum active power capability of the DER (in W). Defaults to rtgMaxW."},{"sh:path":{"@id":"setMaxWh"},"sh:maxCount":1,"sh:node":{"@id":"WattHourShape"},"rdfs:comment":"Maximum energy storage capacity of the DER, in WattHours. Note: this may be different from physical capability."},{"sh:path":{"@id":"setMinPFOverExcited"},"sh:maxCount":1,"sh:node":{"@id":"PowerFactorShape"},"rdfs:comment":"Set minimum Power Factor displacement limit of the DER when injecting reactive power (over-excited); SHALL be a positive value between 0.0 (typically &gt; 0.7) and 1.0.  SHALL be &gt;= rtgMinPFOverExcited (default)."},{"sh:path":{"@id":"setMinPFUnderExcited"},"sh:maxCount":1,"sh:node":{"@id":"PowerFactorShape"},"rdfs:comment":"Set minimum Power Factor displacement limit of the DER when absorbing reactive power (under-excited); SHALL be a positive value between 0.0 (typically &gt; 0.7) and 0.9999.  If present, SHALL be &gt;= rtgMinPFUnderExcited (default).  If absent, defaults to setMinPFOverExcited."},{"sh:path":{"@id":"setMinV"},"sh:maxCount":1,"sh:node":{"@id":"VoltageRMSShape"},"rdfs:comment":"AC voltage minimum setting."},{"sh:path":{"@id":"setSoftGradW"},"sh:maxCount":1,"sh:minInclusive":0,"sh:maxInclusive":65535,"sh:datatype":"xsd:unsignedShort","rdfs:comment":"Set soft-start rate of change (soft-start ramp rate) of active power output due to command or internal action, defined in %setWMax / second.  Resolution is in hundredths of a percent/second. A value of 0 means there is no limit. Interpreted as a percentage change in output capability limit per second when used as a ramp rate."},{"sh:path":{"@id":"setVNom"},"sh:maxCount":1,"sh:node":{"@id":"VoltageRMSShape"},"rdfs:comment":"AC voltage nominal setting."},{"sh:path":{"@id":"setVRef"},"sh:maxCount":1,"sh:node":{"@id":"VoltageRMSShape"},"rdfs:comment":"The nominal AC voltage (RMS) at the utility's point of common coupling."},{"sh:path":{"@id":"setVRefOfs"},"sh:maxCount":1,"sh:node":{"@id":"VoltageRMSShape"},"rdfs:comment":"The nominal AC voltage (RMS) offset between the DER's electrical connection point and the utility's point of common coupling."},{"sh:path":{"@id":"updatedTime"},"sh:minCount":1,"sh:maxCount":1,"sh:datatype":"xsd:integer","rdfs:comment":"Specifies the time at which the DER information was last updated."}]},{"@id":"DERAvailabilityShape","@type":"sh:NodeShape","sh:targetClass":{"@id":"DERAvailability"},"rdfs:comment":"Indicates current reserve generation status","sh:property":[{"sh:path":{"@id":"availabilityDuration"},"sh:maxCount":1,"sh:minInclusive":0,"sh:maxInclusive":4294967295,"sh:datatype":"xsd:unsignedInt","rdfs:comment":"Indicates number of seconds the DER will be able to deliver active power at the reservePercent level."},{"sh:path":{"@id":"maxChargeDuration"},"sh:maxCount":1,"sh:minInclusive":0,"sh:maxInclusive":4294967295,"sh:datatype":"xsd:unsignedInt","rdfs:comment":"Indicates number of seconds the DER will be able to receive active power at the reserveChargePercent level."},{"sh:path":{"@id":"readingTime"},"sh:minCount":1,"sh:maxCount":1,"sh:datatype":"xsd:integer","rdfs:comment":"The timestamp when the DER availability was last updated."},{"sh:path":{"@id":"reserveChargePercent"},"sh:maxCount":1,"sh:minInclusive":0,"sh:maxInclusive":65535,"sh:datatype":"xsd:integer","rdfs:comment":"Percent of continuous received active power (%setMaxChargeRateW) that is estimated to be available in reserve."},{"sh:path":{"@id":"reservePercent"},"sh:maxCount":1,"sh:minInclusive":0,"sh:maxInclusive":65535,"sh:datatype":"xsd:integer","rdfs:comment":"Percent of continuous delivered active power (%setMaxW) that is estimated to be available in reserve."},{"sh:path":{"@id":"statVarAvail"},"sh:maxCount":1,"sh:node":{"@id":"ReactivePowerShape"},"rdfs:comment":"Estimated reserve reactive power, in var.  Represents the lesser of received or delivered reactive power."},{"sh:path":{"@id":"statWAvail"},"sh:maxCount":1,"sh:node":{"@id":"ActivePowerShape"},"rdfs:comment":"Estimated reserve active power, in watts."}]},{"@id":"DERCapabilityShape","@type":"sh:NodeShape","sh:targetClass":{"@id":"DERCapability"},"rdfs:comment":"Distributed energy resource type and nameplate ratings.","sh:property":[{"sh:path":{"@id":"modesSupported"},"sh:in":["0","1","2","3","4","5","6","7","8","9","10","11","12","13","14","15","16","17","18","19","20","21","22","23","24","25","26"],"sh:minCount":1,"sh:maxCount":1,"sh:datatype":"xsd:string","rdfs:comment":"Bitmap indicating the DER Controls implemented by the device. See DERControlType for values."},{"sh:path":{"@id":"rtgAbnormalCategory"},"sh:maxCount":1,"sh:minInclusive":0,"sh:maxInclusive":255,"sh:datatype":"xsd:unsignedByte","rdfs:comment":"Abnormal operating performance category as defined by IEEE 1547-2018. One of:\n0 - not specified\n1 - Category I\n2 - Category II\n3 - Category III\nAll other values reserved."},{"sh:path":{"@id":"rtgMaxA"},"sh:maxCount":1,"sh:node":{"@id":"CurrentRMSShape"},"rdfs:comment":"Maximum continuous AC current capability of the DER, in Amperes (RMS)."},{"sh:path":{"@id":"rtgMaxAh"},"sh:maxCount":1,"sh:node":{"@id":"AmpereHourShape"},"rdfs:comment":"Usable energy storage capacity of the DER, in AmpHours."},{"sh:path":{"@id":"rtgMaxChargeRateVA"},"sh:maxCount":1,"sh:node":{"@id":"ApparentPowerShape"},"rdfs:comment":"Maximum apparent power charge rating in Volt-Amperes. May differ from the maximum apparent power rating."},{"sh:path":{"@id":"rtgMaxChargeRateW"},"sh:maxCount":1,"sh:node":{"@id":"ActivePowerShape"},"rdfs:comment":"Maximum rate of energy transfer received by the storage DER, in Watts."},{"sh:path":{"@id":"rtgMaxDischargeRateVA"},"sh:maxCount":1,"sh:node":{"@id":"ApparentPowerShape"},"rdfs:comment":"Maximum apparent power discharge rating in Volt-Amperes. May differ from the maximum apparent power rating."},{"sh:path":{"@id":"rtgMaxDischargeRateW"},"sh:maxCount":1,"sh:node":{"@id":"ActivePowerShape"},"rdfs:comment":"Maximum rate of energy transfer delivered by the storage DER, in Watts. Required for combined generation/storage DERs (e.g. DERType == 83)."},{"sh:path":{"@id":"rtgMaxV"},"sh:maxCount":1,"sh:node":{"@id":"VoltageRMSShape"},"rdfs:comment":"AC voltage maximum rating."},{"sh:path":{"@id":"rtgMaxVA"},"sh:maxCount":1,"sh:node":{"@id":"ApparentPowerShape"},"rdfs:comment":"Maximum continuous apparent power output capability of the DER, in VA."},{"sh:path":{"@id":"rtgMaxVar"},"sh:maxCount":1,"sh:node":{"@id":"ReactivePowerShape"},"rdfs:comment":"Maximum continuous reactive power delivered by the DER, in var."},{"sh:path":{"@id":"rtgMaxVarNeg"},"sh:maxCount":1,"sh:node":{"@id":"ReactivePowerShape"},"rdfs:comment":"Maximum continuous reactive power received by the DER, in var.  If absent, defaults to negative rtgMaxVar."},{"sh:path":{"@id":"rtgMaxW"},"sh:minCount":1,"sh:maxCount":1,"sh:node":{"@id":"ActivePowerShape"},"rdfs:comment":"Maximum continuous active power output capability of the DER, in watts. Represents combined generation plus storage output if DERType == 83."},{"sh:path":{"@id":"rtgMaxWh"},"sh:maxCount":1,"sh:node":{"@id":"WattHourShape"},"rdfs:comment":"Maximum energy storage capacity of the DER, in WattHours."},{"sh:path":{"@id":"rtgMinPFOverExcited"},"sh:maxCount":1,"sh:node":{"@id":"PowerFactorShape"},"rdfs:comment":"Minimum Power Factor displacement capability of the DER when injecting reactive power (over-excited); SHALL be a positive value between 0.0 (typically &gt; 0.7) and 1.0. If absent, defaults to unity."},{"sh:path":{"@id":"rtgMinPFUnderExcited"},"sh:maxCount":1,"sh:node":{"@id":"PowerFactorShape"},"rdfs:comment":"Minimum Power Factor displacement capability of the DER when absorbing reactive power (under-excited); SHALL be a positive value between 0.0 (typically &gt; 0.7) and 0.9999.  If absent, defaults to rtgMinPFOverExcited."},{"sh:path":{"@id":"rtgMinV"},"sh:maxCount":1,"sh:node":{"@id":"VoltageRMSShape"},"rdfs:comment":"AC voltage minimum rating."},{"sh:path":{"@id":"rtgNormalCategory"},"sh:maxCount":1,"sh:minInclusive":0,"sh:maxInclusive":255,"sh:datatype":"xsd:unsignedByte","rdfs:comment":"Normal operating performance category as defined by IEEE 1547-2018. One of:\n0 - not specified\n1 - Category A\n2 - Category B\nAll other values reserved."},{"sh:path":{"@id":"rtgOverExcitedPF"},"sh:maxCount":1,"sh:node":{"@id":"PowerFactorShape"},"rdfs:comment":"Specified over-excited power factor."},{"sh:path":{"@id":"rtgOverExcitedW"},"sh:maxCount":1,"sh:node":{"@id":"ActivePowerShape"},"rdfs:comment":"Active power rating in Watts at specified over-excited power factor (rtgOverExcitedPF). If present, rtgOverExcitedPF SHALL be present."},{"sh:path":{"@id":"rtgReactiveSusceptance"},"sh:maxCount":1,"sh:node":{"@id":"ReactiveSusceptanceShape"},"rdfs:comment":"Reactive susceptance that remains connected to the Area EPS in the cease to energize and trip state."},{"sh:path":{"@id":"rtgUnderExcitedPF"},"sh:maxCount":1,"sh:node":{"@id":"PowerFactorShape"},"rdfs:comment":"Specified under-excited power factor."},{"sh:path":{"@id":"rtgUnderExcitedW"},"sh:maxCount":1,"sh:node":{"@id":"ActivePowerShape"},"rdfs:comment":"Active power rating in Watts at specified under-excited power factor (rtgUnderExcitedPF). If present, rtgUnderExcitedPF SHALL be present."},{"sh:path":{"@id":"rtgVNom"},"sh:maxCount":1,"sh:node":{"@id":"VoltageRMSShape"},"rdfs:comment":"AC voltage nominal rating."},{"sh:path":{"@id":"type"},"sh:in":[0,1,2,3,4,5,6,80,81,82,83],"sh:minCount":1,"sh:maxCount":1,"sh:minInclusive":0,"sh:maxInclusive":255,"sh:datatype":"xsd:integer","rdfs:comment":"Type of DER; see DERType object"}]},{"@id":"DERControlBaseShape","@type":"sh:NodeShape","sh:targetClass":{"@id":"DERControlBase"},"rdfs:comment":"Distributed Energy Resource (DER) control values.","sh:property":[{"sh:path":{"@id":"opModConnect"},"sh:maxCount":1,"sh:datatype":"xsd:boolean","rdfs:comment":"Set DER as connected (true) or disconnected (false). Used in conjunction with ramp rate when re-connecting. Implies galvanic isolation."},{"sh:path":{"@id":"opModEnergize"},"sh:maxCount":1,"sh:datatype":"xsd:boolean","rdfs:comment":"Set DER as energized (true) or de-energized (false). Used in conjunction with ramp rate when re-energizing."},{"sh:path":{"@id":"opModFixedPFAbsorbW"},"sh:maxCount":1,"sh:node":{"@id":"PowerFactorWithExcitationShape"},"rdfs:comment":"The opModFixedPFAbsorbW function specifies a requested fixed Power Factor (PF) setting for when active power is being absorbed. The actual displacement SHALL be within the limits established by setMinPFOverExcited and setMinPFUnderExcited. If issued simultaneously with other reactive power controls (e.g. opModFixedVar) the control resulting in least var magnitude SHOULD take precedence."},{"sh:path":{"@id":"opModFixedPFInjectW"},"sh:maxCount":1,"sh:node":{"@id":"PowerFactorWithExcitationShape"},"rdfs:comment":"The opModFixedPFInjectW function specifies a requested fixed Power Factor (PF) setting for when active power is being injected. The actual displacement SHALL be within the limits established by setMinPFOverExcited and setMinPFUnderExcited. If issued simultaneously with other reactive power controls (e.g. opModFixedVar) the control resulting in least var magnitude SHOULD take precedence."},{"sh:path":{"@id":"opModFixedVar"},"sh:maxCount":1,"sh:node":{"@id":"FixedVarShape"},"rdfs:comment":"The opModFixedVar function specifies the delivered or received reactive power setpoint.  The context for the setpoint value is determined by refType and SHALL be one of %setMaxW, %setMaxVar, or %statVarAvail.  If issued simultaneously with other reactive power controls (e.g. opModFixedPFInjectW) the control resulting in least var magnitude SHOULD take precedence."},{"sh:path":{"@id":"opModFixedW"},"sh:maxCount":1,"sh:datatype":"xsd:integer","rdfs:comment":"The opModFixedW function specifies a requested charge or discharge mode setpoint, in %setMaxChargeRateW if negative value or %setMaxW or %setMaxDischargeRateW if positive value (in hundredths)."},{"sh:path":{"@id":"opModFreqDroop"},"sh:maxCount":1,"sh:node":{"@id":"FreqDroopTypeShape"},"rdfs:comment":"Specifies a frequency-watt operation. This operation limits active power generation or consumption when the line frequency deviates from nominal by a specified amount."},{"sh:path":{"@id":"opModFreqWatt"},"sh:maxCount":1,"sh:datatype":"xsd:string","rdfs:comment":"Specify DERCurveLink for curveType == 0.  The Frequency-Watt function limits active power generation or consumption when the line frequency deviates from nominal by a specified amount. The Frequency-Watt curve is specified as an array of Frequency-Watt pairs that are interpolated into a piecewise linear function with hysteresis.  The x value of each pair specifies a frequency in Hz. The y value specifies a corresponding active power output in %setMaxW."},{"sh:path":{"@id":"opModHFRTMayTrip"},"sh:maxCount":1,"sh:datatype":"xsd:string","rdfs:comment":"Specify DERCurveLink for curveType == 1. The High Frequency Ride-Through (HFRT) function is specified by one or two duration-frequency curves that define the operating region under high frequency conditions. Each HFRT curve is specified by an array of duration-frequency pairs that will be interpolated into a piecewise linear function that defines an operating region. The x value of each pair specifies a duration (time at a given frequency in seconds). The y value of each pair specifies a frequency, in Hz. This control specifies the \"may trip\" region."},{"sh:path":{"@id":"opModHFRTMustTrip"},"sh:maxCount":1,"sh:datatype":"xsd:string","rdfs:comment":"Specify DERCurveLink for curveType == 2.  The High Frequency Ride-Through (HFRT) function is specified by a duration-frequency curve that defines the operating region under high frequency conditions.  Each HFRT curve is specified by an array of duration-frequency pairs that will be interpolated into a piecewise linear function that defines an operating region.  The x value of each pair specifies a duration (time at a given frequency in seconds). The y value of each pair specifies a frequency, in Hz. This control specifies the \"must trip\" region."},{"sh:path":{"@id":"opModHVRTMayTrip"},"sh:maxCount":1,"sh:datatype":"xsd:string","rdfs:comment":"Specify DERCurveLink for curveType == 3. The High Voltage Ride-Through (HVRT) function is specified by one, two, or three duration-volt curves that define the operating region under high voltage conditions. Each HVRT curve is specified by an array of duration-volt pairs that will be interpolated into a piecewise linear function that defines an operating region. The x value of each pair specifies a duration (time at a given voltage in seconds). The y value of each pair specifies an effective percentage voltage, defined as ((locally measured voltage - setVRefOfs / setVRef). This control specifies the \"may trip\" region."},{"sh:path":{"@id":"opModHVRTMomentaryCessation"},"sh:maxCount":1,"sh:datatype":"xsd:string","rdfs:comment":"Specify DERCurveLink for curveType == 4.  The High Voltage Ride-Through (HVRT) function is specified by duration-volt curves that define the operating region under high voltage conditions.  Each HVRT curve is specified by an array of duration-volt pairs that will be interpolated into a piecewise linear function that defines an operating region.  The x value of each pair specifies a duration (time at a given voltage in seconds). The y value of each pair specifies an effective percent voltage, defined as ((locally measured voltage - setVRefOfs) / setVRef). This control specifies the \"momentary cessation\" region."},{"sh:path":{"@id":"opModHVRTMustTrip"},"sh:maxCount":1,"sh:datatype":"xsd:string","rdfs:comment":"Specify DERCurveLink for curveType == 5.  The High Voltage Ride-Through (HVRT) function is specified by duration-volt curves that define the operating region under high voltage conditions.  Each HVRT curve is specified by an array of duration-volt pairs that will be interpolated into a piecewise linear function that defines an operating region.  The x value of each pair specifies a duration (time at a given voltage in seconds). The y value of each pair specifies an effective percent voltage, defined as ((locally measured voltage - setVRefOfs) / setVRef). This control specifies the \"must trip\" region."},{"sh:path":{"@id":"opModLFRTMayTrip"},"sh:maxCount":1,"sh:datatype":"xsd:string","rdfs:comment":"Specify DERCurveLink for curveType == 6. The Low Frequency Ride-Through (LFRT) function is specified by one or two duration-frequency curves that define the operating region under low frequency conditions. Each LFRT curve is specified by an array of duration-frequency pairs that will be interpolated into a piecewise linear function that defines an operating region. The x value of each pair specifies a duration (time at a given frequency in seconds). The y value of each pair specifies a frequency, in Hz. This control specifies the \"may trip\" region."},{"sh:path":{"@id":"opModLFRTMustTrip"},"sh:maxCount":1,"sh:datatype":"xsd:string","rdfs:comment":"Specify DERCurveLink for curveType == 7.  The Low Frequency Ride-Through (LFRT) function is specified by a duration-frequency curve that defines the operating region under low frequency conditions.  Each LFRT curve is specified by an array of duration-frequency pairs that will be interpolated into a piecewise linear function that defines an operating region.  The x value of each pair specifies a duration (time at a given frequency in seconds). The y value of each pair specifies a frequency, in Hz. This control specifies the \"must trip\" region."},{"sh:path":{"@id":"opModLVRTMayTrip"},"sh:maxCount":1,"sh:datatype":"xsd:string","rdfs:comment":"Specify DERCurveLink for curveType == 8. The Low Voltage Ride-Through (LVRT) function is specified by one, two, or three duration-volt curves that define the operating region under low voltage conditions. Each LVRT curve is specified by an array of duration-volt pairs that will be interpolated into a piecewise linear function that defines an operating region. The x value of each pair specifies a duration (time at a given voltage in seconds). The y value of each pair specifies an effective percent voltage, defined as ((locally measured voltage - setVRefOfs) / setVRef). This control specifies the \"may trip\" region."},{"sh:path":{"@id":"opModLVRTMomentaryCessation"},"sh:maxCount":1,"sh:datatype":"xsd:string","rdfs:comment":"Specify DERCurveLink for curveType == 9.  The Low Voltage Ride-Through (LVRT) function is specified by duration-volt curves that define the operating region under low voltage conditions.  Each LVRT curve is specified by an array of duration-volt pairs that will be interpolated into a piecewise linear function that defines an operating region.  The x value of each pair specifies a duration (time at a given voltage in seconds). The y value of each pair specifies an effective percent voltage, defined as ((locally measured voltage - setVRefOfs) / setVRef). This control specifies the \"momentary cessation\" region."},{"sh:path":{"@id":"opModLVRTMustTrip"},"sh:maxCount":1,"sh:datatype":"xsd:string","rdfs:comment":"Specify DERCurveLink for curveType == 10.  The Low Voltage Ride-Through (LVRT) function is specified by duration-volt curves that define the operating region under low voltage conditions.  Each LVRT curve is specified by an array of duration-volt pairs that will be interpolated into a piecewise linear function that defines an operating region.  The x value of each pair specifies a duration (time at a given voltage in seconds). The y value of each pair specifies an effective percent voltage, defined as ((locally measured voltage - setVRefOfs) / setVRef). This control specifies the \"must trip\" region."},{"sh:path":{"@id":"opModMaxLimW"},"sh:maxCount":1,"sh:minInclusive":0,"sh:maxInclusive":65535,"sh:datatype":"xsd:integer","rdfs:comment":"The opModMaxLimW function sets the maximum active power generation level at the electrical coupling point as a percentage of set capacity (%setMaxW, in hundredths). This limitation may be met e.g. by reducing PV output or by using excess PV output to charge associated storage."},{"sh:path":{"@id":"opModTargetVar"},"sh:maxCount":1,"sh:node":{"@id":"ReactivePowerShape"},"rdfs:comment":"Target reactive power, in var. This control is likely to be more useful for aggregators, as individual DERs may not be able to maintain a target setting."},{"sh:path":{"@id":"opModTargetW"},"sh:maxCount":1,"sh:node":{"@id":"ActivePowerShape"},"rdfs:comment":"Target output power, in Watts. This control is likely to be more useful for aggregators, as individual DERs may not be able to maintain a target setting."},{"sh:path":{"@id":"opModVoltVar"},"sh:maxCount":1,"sh:datatype":"xsd:string","rdfs:comment":"Specify DERCurveLink for curveType == 11.  The static volt-var function provides over- or under-excited var compensation as a function of measured voltage. The volt-var curve is specified as an array of volt-var pairs that are interpolated into a piecewise linear function with hysteresis. The x value of each pair specifies an effective percent voltage, defined as ((locally measured voltage - setVRefOfs) / setVRef) and SHOULD support a domain of at least 0 - 135. If VRef is present in DERCurve, then the x value of each pair is additionally multiplied by (VRef / 10000). The y value specifies a target var output interpreted as a signed percentage (-100 to 100). The meaning of the y value is determined by yRefType and must be one of %setMaxW, %setMaxVar, or %statVarAvail."},{"sh:path":{"@id":"opModVoltWatt"},"sh:maxCount":1,"sh:datatype":"xsd:string","rdfs:comment":"Specify DERCurveLink for curveType == 12.  The Volt-Watt reduces active power output as a function of measured voltage. The Volt-Watt curve is specified as an array of Volt-Watt pairs that are interpolated into a piecewise linear function with hysteresis. The x value of each pair specifies an effective percent voltage, defined as ((locally measured voltage - setVRefOfs) / setVRef) and SHOULD support a domain of at least 0 - 135. The y value specifies an active power output interpreted as a percentage (0 - 100). The meaning of the y value is determined by yRefType and must be one of %setMaxW or %statWAvail."},{"sh:path":{"@id":"opModWattPF"},"sh:maxCount":1,"sh:datatype":"xsd:string","rdfs:comment":"Specify DERCurveLink for curveType == 13.  The Watt-PF function varies Power Factor (PF) as a function of delivered active power. The Watt-PF curve is specified as an array of Watt-PF coordinates that are interpolated into a piecewise linear function with hysteresis.  The x value of each pair specifies a watt setting in %setMaxW, (0 - 100). The PF output setting is a signed displacement in y value (PF sign SHALL be interpreted according to the EEI convention, where unity PF is considered unsigned). These settings are not expected to be updated very often during the life of the installation, therefore only a single curve is required.  If issued simultaneously with other reactive power controls (e.g. opModFixedPFInjectW) the control resulting in least var magnitude SHOULD take precedence."},{"sh:path":{"@id":"opModWattVar"},"sh:maxCount":1,"sh:datatype":"xsd:string","rdfs:comment":"Specify DERCurveLink for curveType == 14. The Watt-Var function varies vars as a function of delivered active power. The Watt-Var curve is specified as an array of Watt-Var pairs that are interpolated into a piecewise linear function with hysteresis. The x value of each pair specifies a watt setting in %setMaxW, (0-100). The y value specifies a target var output interpreted as a signed percentage (-100 to 100). The meaning of the y value is determined by yRefType and must be one of %setMaxW, %setMaxVar, or %statVarAvail."},{"sh:path":{"@id":"rampTms"},"sh:maxCount":1,"sh:minInclusive":0,"sh:maxInclusive":65535,"sh:datatype":"xsd:unsignedShort","rdfs:comment":"Requested ramp time, in hundredths of a second, for the device to transition from the current DERControl  mode setting(s) to the new mode setting(s). If absent, use default ramp rate (setGradW).  Resolution is 1/100 sec."}]},{"@id":"DERControlShape","@type":"sh:NodeShape","sh:targetClass":{"@id":"DERControl"},"rdfs:comment":"Distributed Energy Resource (DER) time/event-based control.","sh:property":[{"sh:path":{"@id":"DERControlBase"},"sh:minCount":1,"sh:maxCount":1,"sh:node":{"@id":"DERControlBaseShape"}},{"sh:path":{"@id":"deviceCategory"},"sh:in":["0","1","2","3","4","5","6","7","8","9","10","11","12","13","14","15","16","17","18","19","20","21","22","23","24","25"],"sh:maxCount":1,"sh:datatype":"xsd:string","rdfs:comment":"Specifies the bitmap indicating  the categories of devices that SHOULD respond. Devices SHOULD ignore events that do not indicate their device category. If not present, all devices SHOULD respond."}]},{"@id":"DERControlListShape","@type":"sh:NodeShape","sh:targetClass":{"@id":"DERControlList"},"rdfs:comment":"A List element to hold DERControl objects.","sh:property":[{"sh:path":{"@id":"DERControl"},"sh:node":{"@id":"DERControlShape"}}]},{"@id":"DERCurveShape","@type":"sh:NodeShape","sh:targetClass":{"@id":"DERCurve"},"rdfs:comment":"DER related curves such as Volt-Var mode curves. Relationship between an independent variable (X-axis) and a dependent variable (Y-axis).","sh:property":[{"sh:path":{"@id":"autonomousVRefEnable"},"sh:maxCount":1,"sh:datatype":"xsd:boolean","rdfs:comment":"If the curveType is opModVoltVar, then this field MAY be present. If the curveType is not opModVoltVar, then this field SHALL NOT be present. Enable/disable autonomous vRef adjustment. When enabled, the Volt-Var curve characteristic SHALL be adjusted autonomously as vRef changes and autonomousVRefTimeConstant SHALL be present. If a DER is able to support Volt-Var mode but is unable to support autonomous vRef adjustment, then the DER SHALL execute the curve without autonomous vRef adjustment. If not specified, then the value is false."},{"sh:path":{"@id":"autonomousVRefTimeConstant"},"sh:maxCount":1,"sh:minInclusive":0,"sh:maxInclusive":4294967295,"sh:datatype":"xsd:unsignedInt","rdfs:comment":"If the curveType is opModVoltVar, then this field MAY be present. If the curveType is not opModVoltVar, then this field SHALL NOT be present. Adjustment range for vRef time constant, in hundredths of a second."},{"sh:path":{"@id":"creationTime"},"sh:minCount":1,"sh:maxCount":1,"sh:datatype":"xsd:integer","rdfs:comment":"The time at which the object was created."},{"sh:path":{"@id":"CurveData"},"sh:minCount":1,"sh:maxCount":10,"sh:node":{"@id":"CurveDataShape"}},{"sh:path":{"@id":"curveType"},"sh:in":[0,1,2,3,4,5,6,7,8,9,10,11,12,13,14],"sh:minCount":1,"sh:maxCount":1,"sh:minInclusive":0,"sh:maxInclusive":255,"sh:datatype":"xsd:integer","rdfs:comment":"Specifies the associated curve-based control mode."},{"sh:path":{"@id":"openLoopTms"},"sh:maxCount":1,"sh:minInclusive":0,"sh:maxInclusive":65535,"sh:datatype":"xsd:unsignedShort","rdfs:comment":"Open loop response time, the time to ramp up to 90% of the new target in response to the change in voltage, in hundredths of a second. Resolution is 1/100 sec. A value of 0 is used to mean no limit. When not present, the device SHOULD follow its default behavior."},{"sh:path":{"@id":"rampDecTms"},"sh:maxCount":1,"sh:minInclusive":0,"sh:maxInclusive":65535,"sh:datatype":"xsd:unsignedShort","rdfs:comment":"Decreasing ramp rate, interpreted as a percentage change in output capability limit per second (e.g. %setMaxW / sec).  Resolution is in hundredths of a percent/second. A value of 0 means there is no limit. If absent, ramp rate defaults to setGradW."},{"sh:path":{"@id":"rampIncTms"},"sh:maxCount":1,"sh:minInclusive":0,"sh:maxInclusive":65535,"sh:datatype":"xsd:unsignedShort","rdfs:comment":"Increasing ramp rate, interpreted as a percentage change in output capability limit per second (e.g. %setMaxW / sec).  Resolution is in hundredths of a percent/second. A value of 0 means there is no limit. If absent, ramp rate defaults to rampDecTms."},{"sh:path":{"@id":"rampPT1Tms"},"sh:maxCount":1,"sh:minInclusive":0,"sh:maxInclusive":65535,"sh:datatype":"xsd:unsignedShort","rdfs:comment":"The configuration parameter for a low-pass filter, PT1 is a time, in hundredths of a second, in which the filter will settle to 95% of a step change in the input value. Resolution is 1/100 sec."},{"sh:path":{"@id":"vRef"},"sh:maxCount":1,"sh:minInclusive":0,"sh:maxInclusive":65535,"sh:datatype":"xsd:integer","rdfs:comment":"If the curveType is opModVoltVar, then this field MAY be present. If the curveType is not opModVoltVar, then this field SHALL NOT be present. The nominal AC voltage (RMS) adjustment to the voltage curve points for Volt-Var curves."},{"sh:path":{"@id":"xMultiplier"},"sh:in":[0,1,2,3,6,9],"sh:minCount":1,"sh:maxCount":1,"sh:datatype":"xsd:integer","rdfs:comment":"Exponent for X-axis value."},{"sh:path":{"@id":"yMultiplier"},"sh:in":[0,1,2,3,6,9],"sh:minCount":1,"sh:maxCount":1,"sh:datatype":"xsd:integer","rdfs:comment":"Exponent for Y-axis value."},{"sh:path":{"@id":"yRefType"},"sh:in":[0,1,2,3,4,5,6,7],"sh:minCount":1,"sh:maxCount":1,"sh:minInclusive":0,"sh:maxInclusive":255,"sh:datatype":"xsd:integer","rdfs:comment":"The Y-axis units context."}]},{"@id":"DERCurveListShape","@type":"sh:NodeShape","sh:targetClass":{"@id":"DERCurveList"},"rdfs:comment":"A List element to hold DERCurve objects.","sh:property":[{"sh:path":{"@id":"DERCurve"},"sh:node":{"@id":"DERCurveShape"}}]},{"@id":"CurveDataShape","@type":"sh:NodeShape","sh:targetClass":{"@id":"CurveData"},"rdfs:comment":"Data point values for defining a curve or schedule","sh:property":[{"sh:path":{"@id":"excitation"},"sh:maxCount":1,"sh:datatype":"xsd:boolean","rdfs:comment":"If yvalue is Power Factor, then this field SHALL be present. If yvalue is not Power Factor, then this field SHALL NOT be present.\nTrue when DER is absorbing reactive power (under-excited), false\nwhen DER is injecting reactive power (over-excited)."},{"sh:path":{"@id":"xvalue"},"sh:minCount":1,"sh:maxCount":1,"sh:datatype":"xsd:integer","rdfs:comment":"The data value of the X-axis (independent) variable, depending on the curve type. See definitions in DERControlBase for further information."},{"sh:path":{"@id":"yvalue"},"sh:minCount":1,"sh:maxCount":1,"sh:datatype":"xsd:integer","rdfs:comment":"The data value of the Y-axis (dependent) variable, depending on the curve type. See definitions in DERControlBase for further information. If yvalue is Power Factor, the excitation field SHALL be present and yvalue SHALL be a positive value. If yvalue is not Power Factor, the excitation field SHALL NOT be present."}]},{"@id":"DERProgramShape","@type":"sh:NodeShape","sh:targetClass":{"@id":"DERProgram"},"rdfs:comment":"Distributed Energy Resource program.","sh:property":[{"sh:path":{"@id":"ActiveDERControlListLink"},"sh:maxCount":1,"sh:datatype":"xsd:string"},{"sh:path":{"@id":"DefaultDERControlLink"},"sh:maxCount":1,"sh:datatype":"xsd:string"},{"sh:path":{"@id":"DERControlListLink"},"sh:maxCount":1,"sh:datatype":"xsd:string"},{"sh:path":{"@id":"DERCurveListLink"},"sh:maxCount":1,"sh:datatype":"xsd:string"},{"sh:path":{"@id":"primacy"},"sh:minCount":1,"sh:maxCount":1,"sh:minInclusive":0,"sh:maxInclusive":255,"sh:datatype":"xsd:integer","rdfs:comment":"Indicates the relative primacy of the provider of this Program."}]},{"@id":"DERProgramListShape","@type":"sh:NodeShape","sh:targetClass":{"@id":"DERProgramList"},"rdfs:comment":"A List element to hold DERProgram objects.","sh:property":[{"sh:path":{"@id":"DERProgram"},"sh:node":{"@id":"DERProgramShape"}},{"sh:path":{"@id":"pollRate"},"sh:maxCount":1,"sh:minInclusive":0,"sh:maxInclusive":4294967295,"sh:datatype":"xsd:unsignedInt","rdfs:comment":"The default polling rate for this function set (this resource and all resources below), in seconds. If not specified, a default of 900 seconds (15 minutes) is used. It is RECOMMENDED a client poll the resources of this function set every pollRate seconds.","sh:defaultValue":"900"}]},{"@id":"DERStatusShape","@type":"sh:NodeShape","sh:targetClass":{"@id":"DERStatus"},"rdfs:comment":"DER status information.","sh:property":[{"sh:path":{"@id":"alarmStatus"},"sh:maxCount":1,"sh:datatype":"xsd:hexBinary","rdfs:comment":"Bitmap indicating the status of DER alarms (see DER LogEvents for more details).\n0 - DER_FAULT_OVER_CURRENT\n1 - DER_FAULT_OVER_VOLTAGE\n2 - DER_FAULT_UNDER_VOLTAGE\n3 - DER_FAULT_OVER_FREQUENCY\n4 - DER_FAULT_UNDER_FREQUENCY\n5 - DER_FAULT_VOLTAGE_IMBALANCE\n6 - DER_FAULT_CURRENT_IMBALANCE\n7 - DER_FAULT_EMERGENCY_LOCAL\n8 - DER_FAULT_EMERGENCY_REMOTE\n9 - DER_FAULT_LOW_POWER_INPUT\n10 - DER_FAULT_PHASE_ROTATION\n11-31 - Reserved"},{"sh:path":{"@id":"genConnectStatus"},"sh:in":["0","1","2","3","4"],"sh:maxCount":1,"sh:node":{"@id":"ConnectStatusTypeShape"},"rdfs:comment":"Connect/status value for generator DER. \nSee ConnectStatusType for values."},{"sh:path":{"@id":"inverterStatus"},"sh:in":["0","1","2","3","4","5","6","7","8","9","10"],"sh:maxCount":1,"sh:node":{"@id":"InverterStatusTypeShape"},"rdfs:comment":"DER InverterStatus/value.\nSee InverterStatusType for values."},{"sh:path":{"@id":"localControlModeStatus"},"sh:maxCount":1,"sh:node":{"@id":"LocalControlModeStatusTypeShape"},"rdfs:comment":"The local control mode status.\nSee LocalControlModeStatusType for values."},{"sh:path":{"@id":"manufacturerStatus"},"sh:maxCount":1,"sh:node":{"@id":"ManufacturerStatusTypeShape"},"rdfs:comment":"Manufacturer status code."},{"sh:path":{"@id":"operationalModeStatus"},"sh:in":["0","1","2","3"],"sh:maxCount":1,"sh:node":{"@id":"OperationalModeStatusTypeShape"},"rdfs:comment":"Operational mode currently in use.\nSee OperationalModeStatusType for values."},{"sh:path":{"@id":"readingTime"},"sh:minCount":1,"sh:maxCount":1,"sh:datatype":"xsd:integer","rdfs:comment":"The timestamp when the current status was last updated."},{"sh:path":{"@id":"stateOfChargeStatus"},"sh:maxCount":1,"sh:node":{"@id":"StateOfChargeStatusTypeShape"},"rdfs:comment":"State of charge status.\nSee StateOfChargeStatusType for values."},{"sh:path":{"@id":"storageModeStatus"},"sh:maxCount":1,"sh:node":{"@id":"StorageModeStatusTypeShape"},"rdfs:comment":"Storage mode status.\nSee StorageModeStatusType for values."},{"sh:path":{"@id":"storConnectStatus"},"sh:in":["0","1","2","3","4"],"sh:maxCount":1,"sh:node":{"@id":"ConnectStatusTypeShape"},"rdfs:comment":"Connect/status value for storage DER.\nSee ConnectStatusType for values."}]},{"@id":"CurrentRMSShape","@type":"sh:NodeShape","sh:targetClass":{"@id":"CurrentRMS"},"rdfs:comment":"Average flow of charge through a conductor.","sh:property":[{"sh:path":{"@id":"multiplier"},"sh:in":[0,1,2,3,6,9],"sh:minCount":1,"sh:maxCount":1,"sh:datatype":"xsd:integer","rdfs:comment":"Specifies exponent of value."},{"sh:path":{"@id":"value"},"sh:minCount":1,"sh:maxCount":1,"sh:minInclusive":0,"sh:maxInclusive":65535,"sh:datatype":"xsd:unsignedShort","rdfs:comment":"Value in amperes RMS (uom 5)"}]},{"@id":"FixedPointTypeShape","@type":"sh:NodeShape","sh:targetClass":{"@id":"FixedPointType"},"rdfs:comment":"Abstract type for specifying a fixed-point value without a given unit of measure.","sh:property":[{"sh:path":{"@id":"multiplier"},"sh:in":[0,1,2,3,6,9],"sh:minCount":1,"sh:maxCount":1,"sh:datatype":"xsd:integer","rdfs:comment":"Specifies exponent of uom."},{"sh:path":{"@id":"value"},"sh:minCount":1,"sh:maxCount":1,"sh:datatype":"xsd:short","rdfs:comment":"Dimensionless value"}]},{"@id":"UnsignedFixedPointTypeShape","@type":"sh:NodeShape","sh:targetClass":{"@id":"UnsignedFixedPointType"},"rdfs:comment":"Abstract type for specifying an unsigned fixed-point value without a given unit of measure.","sh:property":[{"sh:path":{"@id":"multiplier"},"sh:in":[0,1,2,3,6,9],"sh:minCount":1,"sh:maxCount":1,"sh:datatype":"xsd:integer","rdfs:comment":"Specifies exponent of uom."},{"sh:path":{"@id":"value"},"sh:minCount":1,"sh:maxCount":1,"sh:minInclusive":0,"sh:maxInclusive":65535,"sh:datatype":"xsd:unsignedShort","rdfs:comment":"Dimensionless value"}]},{"@id":"ActivePowerShape","@type":"sh:NodeShape","sh:targetClass":{"@id":"ActivePower"},"rdfs:comment":"The active (real) power P (in W) is the product of root-mean-square (RMS) voltage, RMS current, and cos(theta) where theta is the phase angle of current relative to voltage.  It is the primary measure of the rate of flow of energy.","sh:property":[{"sh:path":{"@id":"multiplier"},"sh:in":[0,1,2,3,6,9],"sh:minCount":1,"sh:maxCount":1,"sh:datatype":"xsd:integer","rdfs:comment":"Specifies exponent for uom."},{"sh:path":{"@id":"value"},"sh:minCount":1,"sh:maxCount":1,"sh:datatype":"xsd:short","rdfs:comment":"Value in watts (uom 38)"}]},{"@id":"AmpereHourShape","@type":"sh:NodeShape","sh:targetClass":{"@id":"AmpereHour"},"rdfs:comment":"Available electric charge","sh:property":[{"sh:path":{"@id":"multiplier"},"sh:in":[0,1,2,3,6,9],"sh:minCount":1,"sh:maxCount":1,"sh:datatype":"xsd:integer","rdfs:comment":"Specifies exponent of uom."},{"sh:path":{"@id":"value"},"sh:minCount":1,"sh:maxCount":1,"sh:minInclusive":0,"sh:maxInclusive":65535,"sh:datatype":"xsd:unsignedShort","rdfs:comment":"Value in ampere-hours (uom 106)"}]},{"@id":"ApparentPowerShape","@type":"sh:NodeShape","sh:targetClass":{"@id":"ApparentPower"},"rdfs:comment":"The apparent power S (in VA) is the product of root mean square (RMS) voltage and RMS current.","sh:property":[{"sh:path":{"@id":"multiplier"},"sh:in":[0,1,2,3,6,9],"sh:minCount":1,"sh:maxCount":1,"sh:datatype":"xsd:integer","rdfs:comment":"Specifies exponent of uom."},{"sh:path":{"@id":"value"},"sh:minCount":1,"sh:maxCount":1,"sh:minInclusive":0,"sh:maxInclusive":65535,"sh:datatype":"xsd:unsignedShort","rdfs:comment":"Value in volt-amperes (uom 61)"}]},{"@id":"ReactivePowerShape","@type":"sh:NodeShape","sh:targetClass":{"@id":"ReactivePower"},"rdfs:comment":"The reactive power Q (in var) is the product of root mean square (RMS) voltage, RMS current, and sin(theta) where theta is the phase angle of current relative to voltage.","sh:property":[{"sh:path":{"@id":"multiplier"},"sh:in":[0,1,2,3,6,9],"sh:minCount":1,"sh:maxCount":1,"sh:datatype":"xsd:integer","rdfs:comment":"Specifies exponent of uom."},{"sh:path":{"@id":"value"},"sh:minCount":1,"sh:maxCount":1,"sh:datatype":"xsd:short","rdfs:comment":"Value in volt-amperes reactive (var) (uom 63)"}]},{"@id":"ReactiveSusceptanceShape","@type":"sh:NodeShape","sh:targetClass":{"@id":"ReactiveSusceptance"},"rdfs:comment":"Reactive susceptance","sh:property":[{"sh:path":{"@id":"multiplier"},"sh:in":[0,1,2,3,6,9],"sh:minCount":1,"sh:maxCount":1,"sh:datatype":"xsd:integer","rdfs:comment":"Specifies exponent of uom."},{"sh:path":{"@id":"value"},"sh:minCount":1,"sh:maxCount":1,"sh:minInclusive":0,"sh:maxInclusive":65535,"sh:datatype":"xsd:unsignedShort","rdfs:comment":"Value in siemens (uom 53)"}]},{"@id":"PowerFactorShape","@type":"sh:NodeShape","sh:targetClass":{"@id":"PowerFactor"},"rdfs:comment":"Specifies a setpoint for Displacement Power Factor, the ratio between apparent and active powers at the fundamental frequency (e.g. 60 Hz).","sh:property":[{"sh:path":{"@id":"displacement"},"sh:minCount":1,"sh:maxCount":1,"sh:minInclusive":0,"sh:maxInclusive":65535,"sh:datatype":"xsd:unsignedShort","rdfs:comment":"Significand of an unsigned value of cos(theta) between 0 and 1.0. E.g. a value of 0.95 may be specified as a displacement of 950 and a multiplier of -3."},{"sh:path":{"@id":"multiplier"},"sh:in":[0,1,2,3,6,9],"sh:minCount":1,"sh:maxCount":1,"sh:datatype":"xsd:integer","rdfs:comment":"Specifies exponent of 'displacement'."}]},{"@id":"PowerFactorWithExcitationShape","@type":"sh:NodeShape","sh:targetClass":{"@id":"PowerFactorWithExcitation"},"rdfs:comment":"Specifies a setpoint for Displacement Power Factor, the ratio between apparent and active powers at the fundamental frequency (e.g. 60 Hz) and includes an excitation flag.","sh:property":[{"sh:path":{"@id":"displacement"},"sh:minCount":1,"sh:maxCount":1,"sh:minInclusive":0,"sh:maxInclusive":65535,"sh:datatype":"xsd:unsignedShort","rdfs:comment":"Significand of an unsigned value of cos(theta) between 0 and 1.0. E.g. a value of 0.95 may be specified as a displacement of 950 and a multiplier of -3."},{"sh:path":{"@id":"excitation"},"sh:minCount":1,"sh:maxCount":1,"sh:datatype":"xsd:boolean","rdfs:comment":"True when DER is absorbing reactive power (under-excited), false\nwhen DER is injecting reactive power (over-excited)."},{"sh:path":{"@id":"multiplier"},"sh:in":[0,1,2,3,6,9],"sh:minCount":1,"sh:maxCount":1,"sh:datatype":"xsd:integer","rdfs:comment":"Specifies exponent of 'displacement'."}]},{"@id":"FixedVarShape","@type":"sh:NodeShape","sh:targetClass":{"@id":"FixedVar"},"rdfs:comment":"Specifies a signed setpoint for reactive power.","sh:property":[{"sh:path":{"@id":"refType"},"sh:in":[0,1,2,3,4,5,6,7],"sh:minCount":1,"sh:maxCount":1,"sh:minInclusive":0,"sh:maxInclusive":255,"sh:datatype":"xsd:integer","rdfs:comment":"Indicates whether to interpret 'value' as %setMaxVar or %statVarAvail."},{"sh:path":{"@id":"value"},"sh:minCount":1,"sh:maxCount":1,"sh:datatype":"xsd:integer","rdfs:comment":"Specify a signed setpoint for reactive power in % (see 'refType' for context)."}]},{"@id":"WattHourShape","@type":"sh:NodeShape","sh:targetClass":{"@id":"WattHour"},"rdfs:comment":"Active (real) energy","sh:property":[{"sh:path":{"@id":"multiplier"},"sh:in":[0,1,2,3,6,9],"sh:minCount":1,"sh:maxCount":1,"sh:datatype":"xsd:integer","rdfs:comment":"Specifies exponent of uom."},{"sh:path":{"@id":"value"},"sh:minCount":1,"sh:maxCount":1,"sh:minInclusive":0,"sh:maxInclusive":65535,"sh:datatype":"xsd:unsignedShort","rdfs:comment":"Value in watt-hours (uom 72)"}]},{"@id":"VoltageRMSShape","@type":"sh:NodeShape","sh:targetClass":{"@id":"VoltageRMS"},"rdfs:comment":"Average electric potential difference between two points.","sh:property":[{"sh:path":{"@id":"multiplier"},"sh:in":[0,1,2,3,6,9],"sh:minCount":1,"sh:maxCount":1,"sh:datatype":"xsd:integer","rdfs:comment":"Specifies exponent of uom."},{"sh:path":{"@id":"value"},"sh:minCount":1,"sh:maxCount":1,"sh:minInclusive":0,"sh:maxInclusive":65535,"sh:datatype":"xsd:unsignedShort","rdfs:comment":"Value in volts RMS (uom 29)"}]},{"@id":"ConnectStatusTypeShape","@type":"sh:NodeShape","sh:targetClass":{"@id":"ConnectStatusType"},"rdfs:comment":"DER ConnectStatus value (bitmap):\n0 - Connected\n1 - Available\n2 - Operating\n3 - Test\n4 - Fault / Error\nAll other values reserved.","sh:property":[{"sh:path":{"@id":"dateTime"},"sh:minCount":1,"sh:maxCount":1,"sh:datatype":"xsd:integer","rdfs:comment":"The date and time at which the state applied."},{"sh:path":{"@id":"value"},"sh:minCount":1,"sh:maxCount":1,"sh:datatype":"xsd:hexBinary","rdfs:comment":"The value indicating the state."}]},{"@id":"InverterStatusTypeShape","@type":"sh:NodeShape","sh:targetClass":{"@id":"InverterStatusType"},"rdfs:comment":"DER InverterStatus value:\n0 - N/A\n1 - off\n2 - sleeping (auto-shutdown) or DER is at low output power/voltage\n3 - starting up or ON but not producing power\n4 - tracking MPPT power point\n5 - forced power reduction/derating\n6 - shutting down\n7 - one or more faults exist\n8 - standby (service on unit) - DER may be at high output voltage/power\n9 - test mode\n10 - as defined in manufacturer status\nAll other values reserved.","sh:property":[{"sh:path":{"@id":"dateTime"},"sh:minCount":1,"sh:maxCount":1,"sh:datatype":"xsd:integer","rdfs:comment":"The date and time at which the state applied."},{"sh:path":{"@id":"value"},"sh:minCount":1,"sh:maxCount":1,"sh:minInclusive":0,"sh:maxInclusive":255,"sh:datatype":"xsd:unsignedByte","rdfs:comment":"The value indicating the state."}]},{"@id":"LocalControlModeStatusTypeShape","@type":"sh:NodeShape","sh:targetClass":{"@id":"LocalControlModeStatusType"},"rdfs:comment":"DER LocalControlModeStatus/value:\n0 \u2013 local control\n1 \u2013 remote control\nAll other values reserved.","sh:property":[{"sh:path":{"@id":"dateTime"},"sh:minCount":1,"sh:maxCount":1,"sh:datatype":"xsd:integer","rdfs:comment":"The date and time at which the state applied."},{"sh:path":{"@id":"value"},"sh:minCount":1,"sh:maxCount":1,"sh:minInclusive":0,"sh:maxInclusive":255,"sh:datatype":"xsd:unsignedByte","rdfs:comment":"The value indicating the state."}]},{"@id":"ManufacturerStatusTypeShape","@type":"sh:NodeShape","sh:targetClass":{"@id":"ManufacturerStatusType"},"rdfs:comment":"DER ManufacturerStatus/value: String data type","sh:property":[{"sh:path":{"@id":"dateTime"},"sh:minCount":1,"sh:maxCount":1,"sh:datatype":"xsd:integer","rdfs:comment":"The date and time at which the state applied."},{"sh:path":{"@id":"value"},"sh:minCount":1,"sh:maxCount":1,"sh:datatype":"xsd:string","rdfs:comment":"The value indicating the state."}]},{"@id":"OperationalModeStatusTypeShape","@type":"sh:NodeShape","sh:targetClass":{"@id":"OperationalModeStatusType"},"rdfs:comment":"DER OperationalModeStatus value:\n0 - Not applicable / Unknown\n1 - Off\n2 - Operational mode\n3 - Test mode\nAll other values reserved.","sh:property":[{"sh:path":{"@id":"dateTime"},"sh:minCount":1,"sh:maxCount":1,"sh:datatype":"xsd:integer","rdfs:comment":"The date and time at which the state applied."},{"sh:path":{"@id":"value"},"sh:minCount":1,"sh:maxCount":1,"sh:minInclusive":0,"sh:maxInclusive":255,"sh:datatype":"xsd:unsignedByte","rdfs:comment":"The value indicating the state."}]},{"@id":"StateOfChargeStatusTypeShape","@type":"sh:NodeShape","sh:targetClass":{"@id":"StateOfChargeStatusType"},"rdfs:comment":"DER StateOfChargeStatus value: Percent data type","sh:property":[{"sh:path":{"@id":"dateTime"},"sh:minCount":1,"sh:maxCount":1,"sh:datatype":"xsd:integer","rdfs:comment":"The date and time at which the state applied."},{"sh:path":{"@id":"value"},"sh:minCount":1,"sh:maxCount":1,"sh:minInclusive":0,"sh:maxInclusive":65535,"sh:datatype":"xsd:integer","rdfs:comment":"The value indicating the state."}]},{"@id":"StorageModeStatusTypeShape","@type":"sh:NodeShape","sh:targetClass":{"@id":"StorageModeStatusType"},"rdfs:comment":"DER StorageModeStatus value:\n0 \u2013 storage charging\n1 \u2013 storage discharging\n2 \u2013 storage holding\nAll other values reserved.","sh:property":[{"sh:path":{"@id":"dateTime"},"sh:minCount":1,"sh:maxCount":1,"sh:datatype":"xsd:integer","rdfs:comment":"The date and time at which the state applied."},{"sh:path":{"@id":"value"},"sh:minCount":1,"sh:maxCount":1,"sh:minInclusive":0,"sh:maxInclusive":255,"sh:datatype":"xsd:unsignedByte","rdfs:comment":"The value indicating the state."}]},{"@id":"IdentifiedObjectShape","@type":"sh:NodeShape","sh:targetClass":{"@id":"IdentifiedObject"},"rdfs:comment":"This is a root class to provide common naming attributes for all classes needing naming attributes","sh:property":[{"sh:path":{"@id":"mRID"},"sh:minCount":1,"sh:maxCount":1,"sh:datatype":"xsd:string","rdfs:comment":"The global identifier of the object."},{"sh:path":{"@id":"description"},"sh:maxCount":1,"sh:datatype":"xsd:string","rdfs:comment":"The description is a human readable text describing or naming the object."},{"sh:path":{"@id":"version"},"sh:maxCount":1,"sh:minInclusive":0,"sh:maxInclusive":65535,"sh:datatype":"xsd:integer","rdfs:comment":"Contains the version number of the object. See the type definition for details."}]},{"@id":"LinkShape","@type":"sh:NodeShape","sh:targetClass":{"@id":"Link"},"rdfs:comment":"Links provide a reference, via URI, to another resource.","sh:property":[{"sh:path":{"@id":"href"},"sh:minCount":1,"sh:maxCount":1,"sh:datatype":"xsd:anyURI","rdfs:comment":"A URI reference."}]},{"@id":"ListShape","@type":"sh:NodeShape","sh:targetClass":{"@id":"List"},"rdfs:comment":"Container to hold a collection of object instances or references. See Design Pattern section for additional details.","sh:property":[{"sh:path":{"@id":"all"},"sh:minCount":1,"sh:maxCount":1,"sh:minInclusive":0,"sh:maxInclusive":4294967295,"sh:datatype":"xsd:unsignedInt","rdfs:comment":"The number specifying \"all\" of the items in the list. Required on a response to a GET, ignored otherwise."},{"sh:path":{"@id":"results"},"sh:minCount":1,"sh:maxCount":1,"sh:minInclusive":0,"sh:maxInclusive":4294967295,"sh:datatype":"xsd:unsignedInt","rdfs:comment":"Indicates the number of items in this page of results."}]},{"@id":"ListLinkShape","@type":"sh:NodeShape","sh:targetClass":{"@id":"ListLink"},"rdfs:comment":"ListLinks provide a reference, via URI, to a List.","sh:property":[{"sh:path":{"@id":"all"},"sh:maxCount":1,"sh:minInclusive":0,"sh:maxInclusive":4294967295,"sh:datatype":"xsd:unsignedInt","rdfs:comment":"Indicates the total number of items in the referenced list. This attribute SHALL be present if the href is a local or relative URI. This attribute SHOULD NOT be present if the href is a remote or absolute URI, as the server may be unaware of changes to the value."}]},{"@id":"ResourceShape","@type":"sh:NodeShape","sh:targetClass":{"@id":"Resource"},"rdfs:comment":"A resource is an addressable unit of information, either a collection (List) or instance of an object (identifiedObject, or simply, Resource)","sh:property":[{"sh:path":{"@id":"href"},"sh:maxCount":1,"sh:datatype":"xsd:anyURI","rdfs:comment":"A reference to the resource address (URI). Required in a response to a GET, ignored otherwise."}]},{"@id":"RespondableIdentifiedObjectShape","@type":"sh:NodeShape","sh:targetClass":{"@id":"RespondableIdentifiedObject"},"rdfs:comment":"An IdentifiedObject to which a Response can be requested.","sh:property":[{"sh:path":{"@id":"mRID"},"sh:minCount":1,"sh:maxCount":1,"sh:datatype":"xsd:string","rdfs:comment":"The global identifier of the object."},{"sh:path":{"@id":"description"},"sh:maxCount":1,"sh:datatype":"xsd:string","rdfs:comment":"The description is a human readable text describing or naming the object."},{"sh:path":{"@id":"version"},"sh:maxCount":1,"sh:minInclusive":0,"sh:maxInclusive":65535,"sh:datatype":"xsd:integer","rdfs:comment":"Contains the version number of the object. See the type definition for details."}]},{"@id":"RespondableResourceShape","@type":"sh:NodeShape","sh:targetClass":{"@id":"RespondableResource"},"rdfs:comment":"A Resource to which a Response can be requested.","sh:property":[{"sh:path":{"@id":"replyTo"},"sh:maxCount":1,"sh:datatype":"xsd:anyURI","rdfs:comment":"A reference to the response resource address (URI). Required on a response to a GET if responseRequired is \"true\"."},{"sh:path":{"@id":"responseRequired"},"sh:maxCount":1,"sh:datatype":"xsd:hexBinary","rdfs:comment":"Indicates whether or not a response is required upon receipt, creation or update of this resource. Responses shall be posted to the collection specified in \"replyTo\". \n\nIf the resource has a deviceCategory field, devices that match one or more of the device types indicated in deviceCategory SHALL respond according to the rules listed below.  If the category does not match, the device SHALL NOT respond. If the resource does not have a deviceCategory field, a device receiving the resource SHALL respond according to the rules listed below.\n\nValue encoded as hex according to the following bit assignments, any combination is possible. \nSee Table 27 for the list of appropriate Response status codes to be sent for these purposes.\n0 - End device shall indicate that message was received \n1 - End device shall indicate specific response. \n2 - End user / customer response is required. \nAll other values reserved.","sh:defaultValue":"00"}]},{"@id":"RespondableSubscribableIdentifiedObjectShape","@type":"sh:NodeShape","sh:targetClass":{"@id":"RespondableSubscribableIdentifiedObject"},"rdfs:comment":"An IdentifiedObject to which a Response can be requested.","sh:property":[{"sh:path":{"@id":"mRID"},"sh:minCount":1,"sh:maxCount":1,"sh:datatype":"xsd:string","rdfs:comment":"The global identifier of the object."},{"sh:path":{"@id":"description"},"sh:maxCount":1,"sh:datatype":"xsd:string","rdfs:comment":"The description is a human readable text describing or naming the object."},{"sh:path":{"@id":"version"},"sh:maxCount":1,"sh:minInclusive":0,"sh:maxInclusive":65535,"sh:datatype":"xsd:integer","rdfs:comment":"Contains the version number of the object. See the type definition for details."},{"sh:path":{"@id":"subscribable"},"sh:in":[0,1,2,3],"sh:maxCount":1,"sh:minInclusive":0,"sh:maxInclusive":255,"sh:datatype":"xsd:integer","rdfs:comment":"Indicates whether or not subscriptions are supported for this resource, and whether or not conditional (thresholds) are supported. If not specified, is \"not subscribable\" (0).","sh:defaultValue":"0"}]},{"@id":"SubscribableIdentifiedObjectShape","@type":"sh:NodeShape","sh:targetClass":{"@id":"SubscribableIdentifiedObject"},"rdfs:comment":"An IdentifiedObject to which a Subscription can be requested.","sh:property":[{"sh:path":{"@id":"mRID"},"sh:minCount":1,"sh:maxCount":1,"sh:datatype":"xsd:string","rdfs:comment":"The global identifier of the object."},{"sh:path":{"@id":"description"},"sh:maxCount":1,"sh:datatype":"xsd:string","rdfs:comment":"The description is a human readable text describing or naming the object."},{"sh:path":{"@id":"version"},"sh:maxCount":1,"sh:minInclusive":0,"sh:maxInclusive":65535,"sh:datatype":"xsd:integer","rdfs:comment":"Contains the version number of the object. See the type definition for details."}]},{"@id":"SubscribableListShape","@type":"sh:NodeShape","sh:targetClass":{"@id":"SubscribableList"},"rdfs:comment":"A List to which a Subscription can be requested.","sh:property":[{"sh:path":{"@id":"all"},"sh:minCount":1,"sh:maxCount":1,"sh:minInclusive":0,"sh:maxInclusive":4294967295,"sh:datatype":"xsd:unsignedInt","rdfs:comment":"The number specifying \"all\" of the items in the list. Required on GET, ignored otherwise."},{"sh:path":{"@id":"results"},"sh:minCount":1,"sh:maxCount":1,"sh:minInclusive":0,"sh:maxInclusive":4294967295,"sh:datatype":"xsd:unsignedInt","rdfs:comment":"Indicates the number of items in this page of results."}]},{"@id":"SubscribableResourceShape","@type":"sh:NodeShape","sh:targetClass":{"@id":"SubscribableResource"},"rdfs:comment":"A Resource to which a Subscription can be requested.","sh:property":[{"sh:path":{"@id":"subscribable"},"sh:in":[0,1,2,3],"sh:maxCount":1,"sh:minInclusive":0,"sh:maxInclusive":255,"sh:datatype":"xsd:integer","rdfs:comment":"Indicates whether or not subscriptions are supported for this resource, and whether or not conditional (thresholds) are supported. If not specified, is \"not subscribable\" (0).","sh:defaultValue":"0"}]},{"@id":"ErrorShape","@type":"sh:NodeShape","sh:targetClass":{"@id":"Error"},"rdfs:comment":"Contains information about the nature of an error if a request could not be completed successfully.","sh:property":[{"sh:path":{"@id":"maxRetryDuration"},"sh:maxCount":1,"sh:minInclusive":0,"sh:maxInclusive":65535,"sh:datatype":"xsd:unsignedShort","rdfs:comment":"Contains the number of seconds the client SHOULD wait before retrying the request."},{"sh:path":{"@id":"reasonCode"},"sh:minCount":1,"sh:maxCount":1,"sh:minInclusive":0,"sh:maxInclusive":65535,"sh:datatype":"xsd:unsignedShort","rdfs:comment":"Code indicating the reason for failure.\n\n0 - Invalid request format\n1 - Invalid request values (e.g. invalid threshold values)\n2 - Resource limit reached\n3 - Conditional subscription field not supported\n4 - Maximum request frequency exceeded\nAll other values reserved"}]},{"@id":"EventShape","@type":"sh:NodeShape","sh:targetClass":{"@id":"Event"},"rdfs:comment":"An Event indicates information that applies to a particular period of time. Events SHALL be executed relative to the time of the server, as described in the Time function set section 11.1.","sh:property":[{"sh:path":{"@id":"creationTime"},"sh:minCount":1,"sh:maxCount":1,"sh:datatype":"xsd:integer","rdfs:comment":"The time at which the Event was created."},{"sh:path":{"@id":"EventStatus"},"sh:minCount":1,"sh:maxCount":1,"sh:node":{"@id":"EventStatusShape"}},{"sh:path":{"@id":"interval"},"sh:minCount":1,"sh:maxCount":1,"sh:node":{"@id":"DateTimeIntervalShape"},"rdfs:comment":"The period during which the Event applies."}]},{"@id":"EventStatusShape","@type":"sh:NodeShape","sh:targetClass":{"@id":"EventStatus"},"rdfs:comment":"Current status information relevant to a specific object. The Status object is used to indicate the current status of an Event. Devices can read the containing resource (e.g. TextMessage) to get the most up to date status of the event.  Devices can also subscribe to a specific resource instance to get updates when any of its attributes change, including the Status object.","sh:property":[{"sh:path":{"@id":"currentStatus"},"sh:minCount":1,"sh:maxCount":1,"sh:minInclusive":0,"sh:maxInclusive":255,"sh:datatype":"xsd:unsignedByte","rdfs:comment":"Field representing the current status type. \n\n0 = Scheduled\nThis status indicates that the event has been scheduled and the event has not yet started.  The server SHALL set the event to this status when the event is first scheduled and persist until the event has become active or has been cancelled.  For events with a start time less than or equal to the current time, this status SHALL never be indicated, the event SHALL start with a status of \u201cActive\u201d. \n\n1 = Active\nThis status indicates that the event is currently active. The server SHALL set the event to this status when the event reaches its earliest Effective Start Time.\n\n2 = Cancelled \nWhen events are cancelled, the Status.dateTime attribute SHALL be set to the time the cancellation occurred, which cannot be in the future.  The server is responsible for maintaining the cancelled event in its collection for the duration of the original event, or until the server has run out of space and needs to store a new event. Client devices SHALL be aware of Cancelled events, determine if the Cancelled event applies to them, and cancel the event immediately if applicable.\n\n3 = Cancelled with Randomization \nThe server is responsible for maintaining the cancelled event in its collection for the duration of the Effective Scheduled Period. Client devices SHALL be aware of Cancelled with Randomization events, determine if the Cancelled event applies to them, and cancel the event immediately, using the larger of (absolute value of randomizeStart) and (absolute value of randomizeDuration) as the end randomization, in seconds. This Status.type SHALL NOT be used with \"regular\" Events, only with specializations of RandomizableEvent.\n\n4 = Superseded\nEvents marked as Superseded by servers are events that may have been replaced by new events from the same program that target the exact same set of deviceCategory's (if applicable) AND DERControl controls (e.g., opModTargetW) (if applicable) and overlap for a given period of time. Servers SHALL mark an event as Superseded at the earliest Effective Start Time of the overlapping event. Servers are responsible for maintaining the Superseded event in their collection for the duration of the Effective Scheduled Period. \nClient devices encountering a Superseded event SHALL terminate execution of the event immediately and commence execution of the new event immediately, unless the current time is within the start randomization window of the superseded event, in which case the client SHALL obey the start randomization of the new event. This Status.type SHALL NOT be used with TextMessage, since multiple text messages can be active. \n\nAll other values reserved."},{"sh:path":{"@id":"dateTime"},"sh:minCount":1,"sh:maxCount":1,"sh:datatype":"xsd:integer","rdfs:comment":"The dateTime attribute will provide a timestamp of when the current status was defined. dateTime MUST be set to the time at which the status change occurred, not a time in the future or past."},{"sh:path":{"@id":"potentiallySuperseded"},"sh:minCount":1,"sh:maxCount":1,"sh:datatype":"xsd:boolean","rdfs:comment":"Set to true by a server of this event if there are events that overlap this event in time and also overlap in some, but not all, deviceCategory's (if applicable) AND DERControl controls (e.g., opModTargetW) (if applicable) in the same function set instance."},{"sh:path":{"@id":"potentiallySupersededTime"},"sh:maxCount":1,"sh:datatype":"xsd:integer","rdfs:comment":"Indicates the time that the potentiallySuperseded flag was set."},{"sh:path":{"@id":"reason"},"sh:maxCount":1,"sh:datatype":"xsd:string","rdfs:comment":"The Reason attribute allows a Service provider to provide a textual explanation of the status."}]},{"@id":"RandomizableEventShape","@type":"sh:NodeShape","sh:targetClass":{"@id":"RandomizableEvent"},"rdfs:comment":"An Event that can indicate time ranges over which the start time and duration SHALL be randomized.","sh:property":[{"sh:path":{"@id":"randomizeDuration"},"sh:maxCount":1,"sh:datatype":"xsd:integer","rdfs:comment":"Number of seconds boundary inside which a random value must be selected to be applied to the associated interval duration, to avoid sudden synchronized demand changes. If related to price level changes, sign may be ignored. Valid range is -3600 to 3600. If not specified, 0 is the default."},{"sh:path":{"@id":"randomizeStart"},"sh:maxCount":1,"sh:datatype":"xsd:integer","rdfs:comment":"Number of seconds boundary inside which a random value must be selected to be applied to the associated interval start time, to avoid sudden synchronized demand changes. If related to price level changes, sign may be ignored. Valid range is -3600 to 3600. If not specified, 0 is the default."}]},{"@id":"DateTimeIntervalShape","@type":"sh:NodeShape","sh:targetClass":{"@id":"DateTimeInterval"},"rdfs:comment":"Interval of date and time.","sh:property":[{"sh:path":{"@id":"duration"},"sh:minCount":1,"sh:maxCount":1,"sh:minInclusive":0,"sh:maxInclusive":4294967295,"sh:datatype":"xsd:unsignedInt","rdfs:comment":"Duration of the interval, in seconds."},{"sh:path":{"@id":"start"},"sh:minCount":1,"sh:maxCount":1,"sh:datatype":"xsd:integer","rdfs:comment":"Date and time of the start of the interval."}]},{"@id":"GPSLocationTypeShape","@type":"sh:NodeShape","sh:targetClass":{"@id":"GPSLocationType"},"rdfs:comment":"Specifies a GPS location, expressed in WGS 84 coordinates.","sh:property":[{"sh:path":{"@id":"lat"},"sh:minCount":1,"sh:maxCount":1,"sh:datatype":"xsd:string","rdfs:comment":"Specifies the latitude from equator. -90 (south) to +90 (north) in decimal degrees."},{"sh:path":{"@id":"lon"},"sh:minCount":1,"sh:maxCount":1,"sh:datatype":"xsd:string","rdfs:comment":"Specifies the longitude from Greenwich Meridian. -180 (west) to +180 (east) in decimal degrees."}]},{"@id":"RealEnergyShape","@type":"sh:NodeShape","sh:targetClass":{"@id":"RealEnergy"},"rdfs:comment":"Real electrical energy","sh:property":[{"sh:path":{"@id":"multiplier"},"sh:in":[0,1,2,3,6,9],"sh:minCount":1,"sh:maxCount":1,"sh:datatype":"xsd:integer","rdfs:comment":"Multiplier for 'unit'."},{"sh:path":{"@id":"value"},"sh:minCount":1,"sh:maxCount":1,"sh:datatype":"xsd:unsignedLong","rdfs:comment":"Value of the energy in Watt-hours. (uom 72)"}]},{"@id":"SignedRealEnergyShape","@type":"sh:NodeShape","sh:targetClass":{"@id":"SignedRealEnergy"},"rdfs:comment":"Real electrical energy, signed.","sh:property":[{"sh:path":{"@id":"multiplier"},"sh:in":[0,1,2,3,6,9],"sh:minCount":1,"sh:maxCount":1,"sh:datatype":"xsd:integer","rdfs:comment":"Multiplier for 'unit'."},{"sh:path":{"@id":"value"},"sh:minCount":1,"sh:maxCount":1,"sh:datatype":"xsd:long","rdfs:comment":"Value of the energy in Watt-hours. (uom 72)"}]},{"@id":"UnitValueTypeShape","@type":"sh:NodeShape","sh:targetClass":{"@id":"UnitValueType"},"rdfs:comment":"Type for specification of a specific value, with units and power of ten multiplier.","sh:property":[{"sh:path":{"@id":"multiplier"},"sh:in":[0,1,2,3,6,9],"sh:minCount":1,"sh:maxCount":1,"sh:datatype":"xsd:integer","rdfs:comment":"Multiplier for 'unit'."},{"sh:path":{"@id":"unit"},"sh:in":[0,5,6,23,29,31,33,38,42,61,63,65,67,69,71,72,73,106,119,122,125,128,129,130,131,132,133,134,137,140,155,169],"sh:minCount":1,"sh:maxCount":1,"sh:minInclusive":0,"sh:maxInclusive":255,"sh:datatype":"xsd:integer","rdfs:comment":"Unit in symbol"},{"sh:path":{"@id":"value"},"sh:minCount":1,"sh:maxCount":1,"sh:datatype":"xsd:integer","rdfs:comment":"Value in units specified"}]},{"@id":"MirrorMeterReadingShape","@type":"sh:NodeShape","sh:targetClass":{"@id":"MirrorMeterReading"},"rdfs:comment":"Mimic of MeterReading used for managing mirrors.","sh:property":[{"sh:path":{"@id":"lastUpdateTime"},"sh:maxCount":1,"sh:datatype":"xsd:integer","rdfs:comment":"The date and time of the last update."},{"sh:path":{"@id":"MirrorReadingSet"},"sh:node":{"@id":"MirrorReadingSetShape"}},{"sh:path":{"@id":"nextUpdateTime"},"sh:maxCount":1,"sh:datatype":"xsd:integer","rdfs:comment":"The date and time of the next planned update."},{"sh:path":{"@id":"Reading"},"sh:maxCount":1,"sh:node":{"@id":"ReadingShape"}},{"sh:path":{"@id":"ReadingType"},"sh:maxCount":1,"sh:node":{"@id":"ReadingTypeShape"}}]},{"@id":"MirrorMeterReadingListShape","@type":"sh:NodeShape","sh:targetClass":{"@id":"MirrorMeterReadingList"},"rdfs:comment":"A List of MirrorMeterReading instances.","sh:property":[{"sh:path":{"@id":"MirrorMeterReading"},"sh:node":{"@id":"MirrorMeterReadingShape"}}]},{"@id":"MirrorReadingSetShape","@type":"sh:NodeShape","sh:targetClass":{"@id":"MirrorReadingSet"},"rdfs:comment":"A set of Readings of the ReadingType indicated by the parent MeterReading.","sh:property":[{"sh:path":{"@id":"Reading"},"sh:node":{"@id":"ReadingShape"}}]},{"@id":"MirrorUsagePointShape","@type":"sh:NodeShape","sh:targetClass":{"@id":"MirrorUsagePoint"},"rdfs:comment":"A parallel to UsagePoint to support mirroring","sh:property":[{"sh:path":{"@id":"deviceLFDI"},"sh:minCount":1,"sh:maxCount":1,"sh:datatype":"xsd:hexBinary","rdfs:comment":"The LFDI of the device being mirrored."},{"sh:path":{"@id":"MirrorMeterReading"},"sh:node":{"@id":"MirrorMeterReadingShape"}},{"sh:path":{"@id":"postRate"},"sh:maxCount":1,"sh:minInclusive":0,"sh:maxInclusive":4294967295,"sh:datatype":"xsd:unsignedInt","rdfs:comment":"POST rate, or how often mirrored data should be POSTed, in seconds. A client MAY indicate a preferred postRate when POSTing MirrorUsagePoint. A server MAY add or modify postRate to indicate its preferred posting rate."}]},{"@id":"MirrorUsagePointListShape","@type":"sh:NodeShape","sh:targetClass":{"@id":"MirrorUsagePointList"},"rdfs:comment":"A List of MirrorUsagePoint instances.","sh:property":[{"sh:path":{"@id":"MirrorUsagePoint"},"sh:node":{"@id":"MirrorUsagePointShape"}},{"sh:path":{"@id":"pollRate"},"sh:maxCount":1,"sh:minInclusive":0,"sh:maxInclusive":4294967295,"sh:datatype":"xsd:unsignedInt","rdfs:comment":"The default polling rate for this function set (this resource and all resources below), in seconds. If not specified, a default of 900 seconds (15 minutes) is used. It is RECOMMENDED a client poll the resources of this function set every pollRate seconds.","sh:defaultValue":"900"}]},{"@id":"ReadingBaseShape","@type":"sh:NodeShape","sh:targetClass":{"@id":"ReadingBase"},"rdfs:comment":"Specific value measured by a meter or other asset. ReadingBase is abstract, used to define the elements common to Reading and IntervalReading.","sh:property":[{"sh:path":{"@id":"consumptionBlock"},"sh:in":[0,1,2,3,4,5,6,7,8,9,10,11,12,13,14,15,16],"sh:maxCount":1,"sh:minInclusive":0,"sh:maxInclusive":255,"sh:datatype":"xsd:integer","rdfs:comment":"Indicates the consumption block related to the reading. REQUIRED if ReadingType numberOfConsumptionBlocks is non-zero. If not specified, is assumed to be \"0 - N/A\"."},{"sh:path":{"@id":"qualityFlags"},"sh:maxCount":1,"sh:datatype":"xsd:hexBinary","rdfs:comment":"List of codes indicating the quality of the reading, using specification:\n\nBit 0 - valid: data that has gone through all required validation checks and either passed them all or has been verified \nBit 1 - manually edited: Replaced or approved by a human\nBit 2 - estimated using reference day: data value was replaced by a machine computed value based on analysis of historical data using the same type of measurement.\nBit 3 - estimated using linear interpolation: data value was computed using linear interpolation based on the readings before and after it\nBit 4 - questionable: data that has failed one or more checks\nBit 5 - derived: data that has been calculated (using logic or mathematical operations), not necessarily measured directly \nBit 6 - projected (forecast): data that has been calculated as a projection or forecast of future readings"},{"sh:path":{"@id":"timePeriod"},"sh:maxCount":1,"sh:node":{"@id":"DateTimeIntervalShape"},"rdfs:comment":"The time interval associated with the reading. If not specified, then defaults to the intervalLength specified in the associated ReadingType."},{"sh:path":{"@id":"touTier"},"sh:in":[0,1,2,3,4,5,6,7,8,9,10,11,12,13,14,15],"sh:maxCount":1,"sh:minInclusive":0,"sh:maxInclusive":255,"sh:datatype":"xsd:integer","rdfs:comment":"Indicates the time of use tier related to the reading. REQUIRED if ReadingType numberOfTouTiers is non-zero. If not specified, is assumed to be \"0 - N/A\"."},{"sh:path":{"@id":"value"},"sh:maxCount":1,"sh:datatype":"xsd:long","rdfs:comment":"Value in units specified by ReadingType"}]},{"@id":"ReadingSetBaseShape","@type":"sh:NodeShape","sh:targetClass":{"@id":"ReadingSetBase"},"rdfs:comment":"A set of Readings of the ReadingType indicated by the parent MeterReading. ReadingBase is abstract, used to define the elements common to ReadingSet and IntervalBlock.","sh:property":[{"sh:path":{"@id":"timePeriod"},"sh:minCount":1,"sh:maxCount":1,"sh:node":{"@id":"DateTimeIntervalShape"},"rdfs:comment":"Specifies the time range during which the contained readings were taken."}]},{"@id":"UsagePointBaseShape","@type":"sh:NodeShape","sh:targetClass":{"@id":"UsagePointBase"},"rdfs:comment":"Logical point on a network at which consumption or production is either physically measured (e.g. metered) or estimated (e.g. unmetered street lights). A container for associating ReadingType, Readings and ReadingSets.","sh:property":[{"sh:path":{"@id":"roleFlags"},"sh:minCount":1,"sh:maxCount":1,"sh:datatype":"xsd:string","rdfs:comment":"Specifies the roles that apply to the usage point."},{"sh:path":{"@id":"serviceCategoryKind"},"sh:in":[0,1,2,3,4,5,6],"sh:minCount":1,"sh:maxCount":1,"sh:minInclusive":0,"sh:maxInclusive":255,"sh:datatype":"xsd:integer","rdfs:comment":"The kind of service provided by this usage point."},{"sh:path":{"@id":"status"},"sh:minCount":1,"sh:maxCount":1,"sh:minInclusive":0,"sh:maxInclusive":255,"sh:datatype":"xsd:unsignedByte","rdfs:comment":"Specifies the current status of the service at this usage point.\n0 = off\n1 = on"}]},{"@id":"DeviceCapability","@type":"rdfs:Class","rdfs:comment":"Returned by the URI provided by DNS-SD, to allow clients to find the URIs to the resources in which they are interested.","rdfs:subClassOf":{"@id":"FunctionSetAssignmentsBase"}},{"@id":"AbstractDevice","@type":"rdfs:Class","rdfs:comment":"The EndDevice providing the resources available within the DeviceCapabilities.","rdfs:subClassOf":{"@id":"SubscribableResource"}},{"@id":"DeviceStatus","@type":"rdfs:Class","rdfs:comment":"Status of device","rdfs:subClassOf":{"@id":"Resource"}},{"@id":"EndDevice","@type":"rdfs:Class","rdfs:comment":"Asset container that performs one or more end device functions. Contains information about individual devices in the network.","rdfs:subClassOf":{"@id":"AbstractDevice"}},{"@id":"EndDeviceList","@type":"rdfs:Class","rdfs:comment":"A List element to hold EndDevice objects.","rdfs:subClassOf":{"@id":"SubscribableList"}},{"@id":"Registration","@type":"rdfs:Class","rdfs:comment":"Registration represents an authorization to access the resources on a host.","rdfs:subClassOf":{"@id":"Resource"}},{"@id":"SelfDevice","@type":"rdfs:Class","rdfs:comment":"The EndDevice providing the resources available within the DeviceCapabilities.","rdfs:subClassOf":{"@id":"AbstractDevice"}},{"@id":"Temperature","@type":"rdfs:Class","rdfs:comment":"Specification of a temperature."},{"@id":"FunctionSetAssignmentsBase","@type":"rdfs:Class","rdfs:comment":"Defines a collection of function set instances that are to be used by one or more devices as indicated by the EndDevice object(s) of the server.","rdfs:subClassOf":{"@id":"Resource"}},{"@id":"FunctionSetAssignments","@type":"rdfs:Class","rdfs:comment":"Provides an identifiable, subscribable collection of resources for a particular device to consume.","rdfs:subClassOf":{"@id":"FunctionSetAssignmentsBase"}},{"@id":"FunctionSetAssignmentsList","@type":"rdfs:Class","rdfs:comment":"A List element to hold FunctionSetAssignments objects.","rdfs:subClassOf":{"@id":"SubscribableList"}},{"@id":"Condition","@type":"rdfs:Class","rdfs:comment":"Indicates a condition that must be satisfied for the Notification to be triggered."},{"@id":"SubscriptionBase","@type":"rdfs:Class","rdfs:comment":"Holds the information related to a client subscription to receive updates to a resource automatically. The actual resources may be passed in the Notification by specifying a specific xsi:type for the Resource and passing the full representation.","rdfs:subClassOf":{"@id":"Resource"}},{"@id":"Subscription","@type":"rdfs:Class","rdfs:comment":"Holds the information related to a client subscription to receive updates to a resource automatically.","rdfs:subClassOf":{"@id":"SubscriptionBase"}},{"@id":"SubscriptionList","@type":"rdfs:Class","rdfs:comment":"A List element to hold Subscription objects.","rdfs:subClassOf":{"@id":"List"}},{"@id":"Notification","@type":"rdfs:Class","rdfs:comment":"Holds the information related to a client subscription to receive updates to a resource automatically. The actual resources may be passed in the Notification by specifying a specific xsi:type for the Resource and passing the full representation.","rdfs:subClassOf":{"@id":"SubscriptionBase"}},{"@id":"NotificationList","@type":"rdfs:Class","rdfs:comment":"A List element to hold Notification objects.","rdfs:subClassOf":{"@id":"List"}},{"@id":"DERControlResponse","@type":"rdfs:Class","rdfs:comment":"A response to a DERControl","rdfs:subClassOf":{"@id":"Response"}},{"@id":"FlowReservationResponseResponse","@type":"rdfs:Class","rdfs:comment":"A response to a FlowReservationResponse","rdfs:subClassOf":{"@id":"Response"}},{"@id":"AppliedTargetReduction","@type":"rdfs:Class","rdfs:comment":"Specifies the value of the TargetReduction applied by the device."},{"@id":"DrResponse","@type":"rdfs:Class","rdfs:comment":"A response to a Demand Response Load Control (EndDeviceControl) message.","rdfs:subClassOf":{"@id":"Response"}},{"@id":"PriceResponse","@type":"rdfs:Class","rdfs:comment":"A response related to a price message.","rdfs:subClassOf":{"@id":"Response"}},{"@id":"Response","@type":"rdfs:Class","rdfs:comment":"The Response object is the generic response data repository which is extended for specific function sets.","rdfs:subClassOf":{"@id":"Resource"}},{"@id":"ResponseList","@type":"rdfs:Class","rdfs:comment":"A List element to hold Response objects.","rdfs:subClassOf":{"@id":"List"}},{"@id":"ResponseSet","@type":"rdfs:Class","rdfs:comment":"A container for a ResponseList.","rdfs:subClassOf":{"@id":"IdentifiedObject"}},{"@id":"ResponseSetList","@type":"rdfs:Class","rdfs:comment":"A List element to hold ResponseSet objects.","rdfs:subClassOf":{"@id":"List"}},{"@id":"TextResponse","@type":"rdfs:Class","rdfs:comment":"A response to a text message","rdfs:subClassOf":{"@id":"Response"}},{"@id":"Time","@type":"rdfs:Class","rdfs:comment":"Contains the representation of time, constantly updated.","rdfs:subClassOf":{"@id":"Resource"}},{"@id":"DeviceInformation","@type":"rdfs:Class","rdfs:comment":"Contains identification and other information about the device that changes very infrequently, typically only when updates are applied, if ever.","rdfs:subClassOf":{"@id":"Resource"}},{"@id":"DRLCCapabilities","@type":"rdfs:Class","rdfs:comment":"Contains information about the static capabilities of the device, to allow service providers to know what types of functions are supported, what the normal operating ranges and limits are, and other similar information, in order to provide better suggestions of applicable programs to receive the maximum benefit."},{"@id":"SupportedLocale","@type":"rdfs:Class","rdfs:comment":"Specifies a locale that is supported","rdfs:subClassOf":{"@id":"Resource"}},{"@id":"SupportedLocaleList","@type":"rdfs:Class","rdfs:comment":"A List element to hold SupportedLocale objects.","rdfs:subClassOf":{"@id":"List"}},{"@id":"PowerStatus","@type":"rdfs:Class","rdfs:comment":"Contains the status of the device's power sources","rdfs:subClassOf":{"@id":"Resource"}},{"@id":"PowerSourceType","@type":"rdfs:Class","rdfs:comment":"0 - none\n1 - mains \n2 - battery\n3 - local generation\n4 - emergency \n5 - unknown\nAll other values reserved.","rdfs:subClassOf":{"@id":"UInt8"},"@enum":{"0":"none","1":"mains","2":"battery","3":"local generation","4":"emergency","5":"unknown"}},{"@id":"PEVInfo","@type":"rdfs:Class","rdfs:comment":"Contains attributes that can be exposed by PEVs and other devices that have charging requirements."},{"@id":"IEEE_802_15_4","@type":"rdfs:Class","rdfs:comment":"Contains 802.15.4 link layer specific attributes."},{"@id":"IPAddr","@type":"rdfs:Class","rdfs:comment":"An Internet Protocol address object.","rdfs:subClassOf":{"@id":"Resource"}},{"@id":"IPAddrList","@type":"rdfs:Class","rdfs:comment":"List of IPAddr instances.","rdfs:subClassOf":{"@id":"List"}},{"@id":"IPInterface","@type":"rdfs:Class","rdfs:comment":"Specific IPInterface resource.  This resource may be thought of as network status information for a specific network (IP) layer interface.","rdfs:subClassOf":{"@id":"Resource"}},{"@id":"IPInterfaceList","@type":"rdfs:Class","rdfs:comment":"List of IPInterface instances.","rdfs:subClassOf":{"@id":"List"}},{"@id":"LLInterface","@type":"rdfs:Class","rdfs:comment":"A link-layer interface object.","rdfs:subClassOf":{"@id":"Resource"}},{"@id":"LLInterfaceList","@type":"rdfs:Class","rdfs:comment":"List of LLInterface instances.","rdfs:subClassOf":{"@id":"List"}},{"@id":"loWPAN","@type":"rdfs:Class","rdfs:comment":"Contains information specific to 6LoWPAN."},{"@id":"Neighbor","@type":"rdfs:Class","rdfs:comment":"Contains 802.15.4 link layer specific attributes.","rdfs:subClassOf":{"@id":"Resource"}},{"@id":"NeighborList","@type":"rdfs:Class","rdfs:comment":"List of 15.4 neighbors.","rdfs:subClassOf":{"@id":"List"}},{"@id":"RPLInstance","@type":"rdfs:Class","rdfs:comment":"Specific RPLInstance resource.  This resource may be thought of as network status information for a specific RPL instance associated with IPInterface.","rdfs:subClassOf":{"@id":"Resource"}},{"@id":"RPLInstanceList","@type":"rdfs:Class","rdfs:comment":"List of RPLInstances associated with the IPinterface.","rdfs:subClassOf":{"@id":"List"}},{"@id":"RPLSourceRoutes","@type":"rdfs:Class","rdfs:comment":"A RPL source routes object.","rdfs:subClassOf":{"@id":"Resource"}},{"@id":"RPLSourceRoutesList","@type":"rdfs:Class","rdfs:comment":"List or RPL source routes if the hosting device is the DODAGroot","rdfs:subClassOf":{"@id":"List"}},{"@id":"LogEvent","@type":"rdfs:Class","rdfs:comment":"A time stamped instance of a significant event detected by the device.","rdfs:subClassOf":{"@id":"Resource"}},{"@id":"LogEventList","@type":"rdfs:Class","rdfs:comment":"A List element to hold LogEvent objects.","rdfs:subClassOf":{"@id":"SubscribableList"}},{"@id":"Configuration","@type":"rdfs:Class","rdfs:comment":"This resource contains various settings to control the operation of the device","rdfs:subClassOf":{"@id":"SubscribableResource"}},{"@id":"PowerConfiguration","@type":"rdfs:Class","rdfs:comment":"Contains configuration related to the device's power sources"},{"@id":"PriceResponseCfg","@type":"rdfs:Class","rdfs:comment":"Configuration data that specifies how price responsive devices SHOULD respond to price changes while acting upon a given RateComponent.","rdfs:subClassOf":{"@id":"Resource"}},{"@id":"PriceResponseCfgList","@type":"rdfs:Class","rdfs:comment":"A List element to hold PriceResponseCfg objects.","rdfs:subClassOf":{"@id":"List"}},{"@id":"TimeConfiguration","@type":"rdfs:Class","rdfs:comment":"Contains attributes related to the configuration of the time service."},{"@id":"File","@type":"rdfs:Class","rdfs:comment":"This resource contains various meta-data describing a file's characteristics.  The meta-data provides general file information and also is used to support filtered queries of file lists","rdfs:subClassOf":{"@id":"Resource"}},{"@id":"FileList","@type":"rdfs:Class","rdfs:comment":"A List element to hold File objects.","rdfs:subClassOf":{"@id":"List"}},{"@id":"FileStatus","@type":"rdfs:Class","rdfs:comment":"This object provides status of device file load and activation operations.","rdfs:subClassOf":{"@id":"Resource"}},{"@id":"LoadShedAvailabilityList","@type":"rdfs:Class","rdfs:comment":"A List element to hold LoadShedAvailability objects.","rdfs:subClassOf":{"@id":"List"}},{"@id":"ApplianceLoadReduction","@type":"rdfs:Class","rdfs:comment":"The ApplianceLoadReduction object is used by a Demand Response service provider to provide signals for ENERGY STAR compliant appliances. See the definition of ApplianceLoadReductionType for more information."},{"@id":"DemandResponseProgram","@type":"rdfs:Class","rdfs:comment":"Demand response program.","rdfs:subClassOf":{"@id":"IdentifiedObject"}},{"@id":"DemandResponseProgramList","@type":"rdfs:Class","rdfs:comment":"A List element to hold DemandResponseProgram objects.","rdfs:subClassOf":{"@id":"SubscribableList"}},{"@id":"DutyCycle","@type":"rdfs:Class","rdfs:comment":"Duty cycle control is a device specific issue and is managed by the device.  The duty cycle of the device under control should span the shortest practical time period in accordance with the nature of the device under control and the intent of the request for demand reduction.  The default factory setting SHOULD be three minutes for each 10% of duty cycle.  This indicates that the default time period over which a duty cycle is applied is 30 minutes, meaning a 10% duty cycle would cause a device to be ON for 3 minutes.   The \u201coff state\u201d SHALL precede the \u201con state\u201d."},{"@id":"EndDeviceControl","@type":"rdfs:Class","rdfs:comment":"Instructs an EndDevice to perform a specified action.","rdfs:subClassOf":{"@id":"RandomizableEvent"}},{"@id":"EndDeviceControlList","@type":"rdfs:Class","rdfs:comment":"A List element to hold EndDeviceControl objects.","rdfs:subClassOf":{"@id":"SubscribableList"}},{"@id":"LoadShedAvailability","@type":"rdfs:Class","rdfs:comment":"Indicates current consumption status and ability to shed load.","rdfs:subClassOf":{"@id":"Resource"}},{"@id":"Offset","@type":"rdfs:Class","rdfs:comment":"If a temperature offset is sent that causes the heating or cooling temperature set point to exceed the limit boundaries that are programmed into the device, the device SHALL respond by setting the temperature at the limit.\nIf an EDC is being targeted at multiple devices or to a device that controls multiple devices (e.g., EMS), it can provide multiple Offset types within one EDC. For events with multiple Offset types, a client SHALL select the Offset that best fits their operating function. \nAlternatively, an event with a single Offset type can be targeted at an EMS in order to request a percentage load reduction on the average energy usage of the entire premise. An EMS SHOULD use the Metering function set to determine the initial load in the premise, reduce energy consumption by controlling devices at its disposal, and at the conclusion of the event, once again use the Metering function set to determine if the desired load reduction was achieved."},{"@id":"SetPoint","@type":"rdfs:Class","rdfs:comment":"The SetPoint object is used to apply specific temperature set points to a temperature control device. The values of the heatingSetpoint and coolingSetpoint attributes SHALL be calculated as follows:\nCooling/Heating Temperature Set Point / 100 = temperature in degrees Celsius where -273.15\u00b0C &lt;= temperature &lt;= 327.67\u00b0C, corresponding to a Cooling and/or Heating Temperature Set Point. The maximum resolution this format allows is 0.01\u00b0C. \nThe field not present in a Response indicates that this field has not been used by the end device. \nIf a temperature is sent that exceeds the temperature limit boundaries that are programmed into the device, the device SHALL respond by setting the temperature at the limit."},{"@id":"TargetReduction","@type":"rdfs:Class","rdfs:comment":"The TargetReduction object is used by a Demand Response service provider to provide a RECOMMENDED threshold that a device/premises should maintain its consumption below. For example, a service provider can provide a RECOMMENDED threshold of some kWh for a 3-hour event. This means that the device/premises would maintain its consumption below the specified limit for the specified period."},{"@id":"MeterReading","@type":"rdfs:Class","rdfs:comment":"Set of values obtained from the meter.","rdfs:subClassOf":{"@id":"MeterReadingBase"}},{"@id":"MeterReadingList","@type":"rdfs:Class","rdfs:comment":"A List element to hold MeterReading objects.","rdfs:subClassOf":{"@id":"SubscribableList"}},{"@id":"Reading","@type":"rdfs:Class","rdfs:comment":"Specific value measured by a meter or other asset.","rdfs:subClassOf":{"@id":"ReadingBase"}},{"@id":"ReadingList","@type":"rdfs:Class","rdfs:comment":"A List element to hold Reading objects.","rdfs:subClassOf":{"@id":"SubscribableList"}},{"@id":"ReadingSet","@type":"rdfs:Class","rdfs:comment":"A set of Readings of the ReadingType indicated by the parent MeterReading.","rdfs:subClassOf":{"@id":"ReadingSetBase"}},{"@id":"ReadingSetList","@type":"rdfs:Class","rdfs:comment":"A List element to hold ReadingSet objects.","rdfs:subClassOf":{"@id":"SubscribableList"}},{"@id":"ReadingType","@type":"rdfs:Class","rdfs:comment":"Type of data conveyed by a specific Reading. See IEC 61968 Part 9 Annex C for full definitions of these values.","rdfs:subClassOf":{"@id":"Resource"}},{"@id":"UsagePoint","@type":"rdfs:Class","rdfs:comment":"Logical point on a network at which consumption or production is either physically measured (e.g. metered) or estimated (e.g. unmetered street lights).","rdfs:subClassOf":{"@id":"UsagePointBase"}},{"@id":"UsagePointList","@type":"rdfs:Class","rdfs:comment":"A List element to hold UsagePoint objects.","rdfs:subClassOf":{"@id":"SubscribableList"}},{"@id":"ConsumptionTariffInterval","@type":"rdfs:Class","rdfs:comment":"One of a sequence of thresholds defined in terms of consumption quantity of a service such as electricity, water, gas, etc. It defines the steps or blocks in a step tariff structure, where startValue simultaneously defines the entry value of this step and the closing value of the previous step. Where consumption is greater than startValue, it falls within this block and where consumption is less than or equal to startValue, it falls within one of the previous blocks.","rdfs:subClassOf":{"@id":"Resource"}},{"@id":"ConsumptionTariffIntervalList","@type":"rdfs:Class","rdfs:comment":"A List element to hold ConsumptionTariffInterval objects.","rdfs:subClassOf":{"@id":"List"}},{"@id":"CostKindType","@type":"rdfs:Class","rdfs:comment":"0 - Carbon Dioxide emissions, in grams per unit\n1 - Sulfur Dioxide emissions, in grams per unit\n2 - Nitrogen Oxides emissions, in grams per unit\n3 - Renewable generation, as a percentage of overall generation\nAll other values reserved.","rdfs:subClassOf":{"@id":"UInt8"},"@enum":{"0":"Carbon Dioxide emissions, in grams per unit","1":"Sulfur Dioxide emissions, in grams per unit","2":"Nitrogen Oxides emissions, in grams per unit","3":"Renewable generation, as a percentage of overall generation"}},{"@id":"EnvironmentalCost","@type":"rdfs:Class","rdfs:comment":"Provides alternative or secondary price information for the relevant RateComponent. Supports jurisdictions that seek to convey the environmental price per unit of the specified commodity not expressed in currency.\n\nImplementers and consumers can use this attribute to prioritize operations of their HAN devices (e.g., PEV charging during times of high availability of renewable electricity resources)."},{"@id":"RateComponent","@type":"rdfs:Class","rdfs:comment":"Specifies the applicable charges for a single component of the rate, which could be generation price or consumption price, for example.","rdfs:subClassOf":{"@id":"IdentifiedObject"}},{"@id":"RateComponentList","@type":"rdfs:Class","rdfs:comment":"A List element to hold RateComponent objects.","rdfs:subClassOf":{"@id":"List"}},{"@id":"TariffProfile","@type":"rdfs:Class","rdfs:comment":"A schedule of charges; structure that allows the definition of tariff structures such as step (block) and time of use (tier) when used in conjunction with TimeTariffInterval and ConsumptionTariffInterval.","rdfs:subClassOf":{"@id":"IdentifiedObject"}},{"@id":"TariffProfileList","@type":"rdfs:Class","rdfs:comment":"A List element to hold TariffProfile objects.","rdfs:subClassOf":{"@id":"SubscribableList"}},{"@id":"TimeTariffInterval","@type":"rdfs:Class","rdfs:comment":"Describes the time-differentiated portion of the RateComponent, if applicable, and provides the ability to specify multiple time intervals, each with its own consumption-based components and other attributes.","rdfs:subClassOf":{"@id":"RandomizableEvent"}},{"@id":"TimeTariffIntervalList","@type":"rdfs:Class","rdfs:comment":"A List element to hold TimeTariffInterval objects.","rdfs:subClassOf":{"@id":"SubscribableList"}},{"@id":"MessagingProgram","@type":"rdfs:Class","rdfs:comment":"Provides a container for collections of text messages.","rdfs:subClassOf":{"@id":"SubscribableIdentifiedObject"}},{"@id":"MessagingProgramList","@type":"rdfs:Class","rdfs:comment":"A List element to hold MessagingProgram objects.","rdfs:subClassOf":{"@id":"SubscribableList"}},{"@id":"PriorityType","@type":"rdfs:Class","rdfs:comment":"Indicates the priority of a message:\n0 - Low\n1 - Normal\n2 - High\n3 - Critical\nAll other values reserved.","rdfs:subClassOf":{"@id":"UInt8"},"@enum":{"0":"Low","1":"Normal","2":"High","3":"Critical"}},{"@id":"TextMessage","@type":"rdfs:Class","rdfs:comment":"Text message such as a notification.","rdfs:subClassOf":{"@id":"Event"}},{"@id":"TextMessageList","@type":"rdfs:Class","rdfs:comment":"A List element to hold TextMessage objects.","rdfs:subClassOf":{"@id":"SubscribableList"}},{"@id":"BillingPeriod","@type":"rdfs:Class","rdfs:comment":"A Billing Period relates to the period of time on which a customer is billed.  As an example the billing period interval for a particular customer might be 31 days starting on July 1, 2011. The start date and interval can change on each billing period. There may also be multiple billing periods related to a customer agreement to support different tariff structures.","rdfs:subClassOf":{"@id":"Resource"}},{"@id":"BillingPeriodList","@type":"rdfs:Class","rdfs:comment":"A List element to hold BillingPeriod objects.","rdfs:subClassOf":{"@id":"SubscribableList"}},{"@id":"BillingMeterReadingBase","@type":"rdfs:Class","rdfs:comment":"Contains historical, target, and projection readings of various types, possibly associated with charges.","rdfs:subClassOf":{"@id":"MeterReadingBase"}},{"@id":"BillingReading","@type":"rdfs:Class","rdfs:comment":"Data captured at regular intervals of time. Interval data could be captured as incremental data, absolute data, or relative data. The source for the data is usually a tariff quantity or an engineering quantity. Data is typically captured in time-tagged, uniform, fixed-length intervals of 5 min, 10 min, 15 min, 30 min, or 60 min. However, consumption aggregations can also be represented with this class.","rdfs:subClassOf":{"@id":"ReadingBase"}},{"@id":"BillingReadingList","@type":"rdfs:Class","rdfs:comment":"A List element to hold BillingReading objects.","rdfs:subClassOf":{"@id":"List"}},{"@id":"BillingReadingSet","@type":"rdfs:Class","rdfs:comment":"Time sequence of readings of the same reading type.","rdfs:subClassOf":{"@id":"ReadingSetBase"}},{"@id":"BillingReadingSetList","@type":"rdfs:Class","rdfs:comment":"A List element to hold BillingReadingSet objects.","rdfs:subClassOf":{"@id":"SubscribableList"}},{"@id":"Charge","@type":"rdfs:Class","rdfs:comment":"Charges contain charges on a customer bill.  These could be items like taxes, levies, surcharges, rebates, or others.  This is meant to allow the HAN device to retrieve enough information to be able to reconstruct an estimate of what the total bill would look like. \n\nProviders can provide line item billing, including multiple charge kinds (e.g. taxes, surcharges) at whatever granularity desired, using as many Charges as desired during a billing period. There can also be any number of Charges associated with different ReadingTypes to distinguish between TOU tiers, consumption blocks, or demand charges."},{"@id":"ChargeKind","@type":"rdfs:Class","rdfs:comment":"Kind of charge.\n0 - Consumption Charge\n1 - Rebate \n2 - Auxiliary Charge\n3 - Demand Charge\n4 - Tax Charge","rdfs:subClassOf":{"@id":"UInt8"},"@enum":{"0":"Consumption Charge","1":"Rebate","2":"Auxiliary Charge","3":"Demand Charge","4":"Tax Charge"}},{"@id":"CustomerAccount","@type":"rdfs:Class","rdfs:comment":"Assignment of a group of products and services purchased by the Customer through a CustomerAgreement, used as a mechanism for customer billing and payment. It contains common information from the various types of CustomerAgreements to create billings (invoices) for a Customer and receive payment.","rdfs:subClassOf":{"@id":"IdentifiedObject"}},{"@id":"CustomerAccountList","@type":"rdfs:Class","rdfs:comment":"A List element to hold CustomerAccount objects.","rdfs:subClassOf":{"@id":"SubscribableList"}},{"@id":"CustomerAgreement","@type":"rdfs:Class","rdfs:comment":"Agreement between the customer and the service supplier to pay for service at a specific service location. It records certain billing information about the type of service provided at the service location and is used during charge creation to determine the type of service.","rdfs:subClassOf":{"@id":"IdentifiedObject"}},{"@id":"CustomerAgreementList","@type":"rdfs:Class","rdfs:comment":"A List element to hold CustomerAgreement objects.","rdfs:subClassOf":{"@id":"SubscribableList"}},{"@id":"HistoricalReading","@type":"rdfs:Class","rdfs:comment":"To be used to present readings that have been processed and possibly corrected (as allowed, due to missing or incorrect data) by backend systems. This includes quality codes valid, verified, estimated, and derived / corrected.","rdfs:subClassOf":{"@id":"BillingMeterReadingBase"}},{"@id":"HistoricalReadingList","@type":"rdfs:Class","rdfs:comment":"A List element to hold HistoricalReading objects.","rdfs:subClassOf":{"@id":"List"}},{"@id":"ProjectionReading","@type":"rdfs:Class","rdfs:comment":"Contains values that forecast a future reading for the time or interval specified.","rdfs:subClassOf":{"@id":"BillingMeterReadingBase"}},{"@id":"ProjectionReadingList","@type":"rdfs:Class","rdfs:comment":"A List element to hold ProjectionReading objects.","rdfs:subClassOf":{"@id":"List"}},{"@id":"TargetReading","@type":"rdfs:Class","rdfs:comment":"Contains readings that specify a target or goal, such as a consumption target, to which billing incentives or other contractual ramifications may be associated.","rdfs:subClassOf":{"@id":"BillingMeterReadingBase"}},{"@id":"TargetReadingList","@type":"rdfs:Class","rdfs:comment":"A List element to hold TargetReading objects.","rdfs:subClassOf":{"@id":"List"}},{"@id":"ServiceSupplier","@type":"rdfs:Class","rdfs:comment":"Organisation that provides services to Customers.","rdfs:subClassOf":{"@id":"IdentifiedObject"}},{"@id":"ServiceSupplierList","@type":"rdfs:Class","rdfs:comment":"A List element to hold ServiceSupplier objects.","rdfs:subClassOf":{"@id":"List"}},{"@id":"AccountBalance","@type":"rdfs:Class","rdfs:comment":"AccountBalance contains the regular credit and emergency credit balance for this given service or commodity prepay instance. It may also contain status information concerning the balance data.","rdfs:subClassOf":{"@id":"Resource"}},{"@id":"AccountingUnit","@type":"rdfs:Class","rdfs:comment":"Unit for accounting; use either 'energyUnit' or 'currencyUnit' to specify the unit for 'value'."},{"@id":"CreditRegister","@type":"rdfs:Class","rdfs:comment":"CreditRegister instances define a credit-modifying transaction. Typically this would be a credit-adding transaction, but may be a subtracting transaction (perhaps in response to an out-of-band debt signal).","rdfs:subClassOf":{"@id":"IdentifiedObject"}},{"@id":"CreditRegisterList","@type":"rdfs:Class","rdfs:comment":"A List element to hold CreditRegister objects.","rdfs:subClassOf":{"@id":"List"}},{"@id":"Prepayment","@type":"rdfs:Class","rdfs:comment":"Prepayment (inherited from CIM SDPAccountingFunction)","rdfs:subClassOf":{"@id":"IdentifiedObject"}},{"@id":"PrepaymentList","@type":"rdfs:Class","rdfs:comment":"A List element to hold Prepayment objects.","rdfs:subClassOf":{"@id":"SubscribableList"}},{"@id":"PrepayModeType","@type":"rdfs:Class","rdfs:comment":"0 - Central Wallet\n1 - ESI\n2 - Local\n3 - Credit\nAll other values reserved.","rdfs:subClassOf":{"@id":"UInt8"},"@enum":{"0":"Central Wallet","1":"ESI","2":"Local","3":"Credit"}},{"@id":"PrepayOperationStatus","@type":"rdfs:Class","rdfs:comment":"PrepayOperationStatus describes the status of the service or commodity being conditionally controlled by the Prepayment function set.","rdfs:subClassOf":{"@id":"Resource"}},{"@id":"ServiceChange","@type":"rdfs:Class","rdfs:comment":"Specifies a change to the service status."},{"@id":"SupplyInterruptionOverride","@type":"rdfs:Class","rdfs:comment":"SupplyInterruptionOverride: There may be periods of time when social, regulatory or other concerns mean that service should not be interrupted, even when available credit has been exhausted. Each Prepayment instance links to a List of SupplyInterruptionOverride instances. Each SupplyInterruptionOverride defines a contiguous period of time during which supply SHALL NOT be interrupted.","rdfs:subClassOf":{"@id":"Resource"}},{"@id":"SupplyInterruptionOverrideList","@type":"rdfs:Class","rdfs:comment":"A List element to hold SupplyInterruptionOverride objects.","rdfs:subClassOf":{"@id":"List"}},{"@id":"CreditStatusType","@type":"rdfs:Class","rdfs:comment":"0 - Credit Ok\n1 - Credit Low\n2 - Credit Exhausted\n3 - Credit Negative\nAll other values reserved.","rdfs:subClassOf":{"@id":"UInt8"},"@enum":{"0":"Credit Ok","1":"Credit Low","2":"Credit Exhausted","3":"Credit Negative"}},{"@id":"CreditTypeType","@type":"rdfs:Class","rdfs:comment":"0 - Regular\n1 - Emergency\n2 - Regular, then Emergency\n3 - Emergency, then Regular\nAll other values reserved.","rdfs:subClassOf":{"@id":"UInt8"},"@enum":{"0":"Regular","1":"Emergency","2":"Regular, then Emergency","3":"Emergency, then Regular"}},{"@id":"CreditTypeChange","@type":"rdfs:Class","rdfs:comment":"Specifies a change to the credit type."},{"@id":"ServiceStatusType","@type":"rdfs:Class","rdfs:comment":"0 - Connected\n1 - Disconnected\n2 - Armed for Connect\n3 - Armed for Disconnect\n4 - No Contactor\n5 - Load Limited\nAll other values reserved.","rdfs:subClassOf":{"@id":"UInt8"},"@enum":{"0":"Connected","1":"Disconnected","2":"Armed for Connect","3":"Armed for Disconnect","4":"No Contactor","5":"Load Limited"}},{"@id":"RequestStatus","@type":"rdfs:Class","rdfs:comment":"The RequestStatus object is used to indicate the current status of a Flow Reservation Request."},{"@id":"FlowReservationRequest","@type":"rdfs:Class","rdfs:comment":"Used to request flow transactions. Client EndDevices submit a request for charging or discharging from the server. The server creates an associated FlowReservationResponse containing the charging parameters and interval to provide a lower aggregated demand at the premises, or within a larger part of the distribution system.","rdfs:subClassOf":{"@id":"IdentifiedObject"}},{"@id":"FlowReservationRequestList","@type":"rdfs:Class","rdfs:comment":"A List element to hold FlowReservationRequest objects.","rdfs:subClassOf":{"@id":"List"}},{"@id":"FlowReservationResponse","@type":"rdfs:Class","rdfs:comment":"The server may modify the charging or discharging parameters and interval to provide a lower aggregated demand at the premises, or within a larger part of the distribution system.","rdfs:subClassOf":{"@id":"Event"}},{"@id":"FlowReservationResponseList","@type":"rdfs:Class","rdfs:comment":"A List element to hold FlowReservationResponse objects.","rdfs:subClassOf":{"@id":"SubscribableList"}},{"@id":"DefaultDERControl","@type":"rdfs:Class","rdfs:comment":"Contains control mode information to be used if no active DERControl is found.","rdfs:subClassOf":{"@id":"SubscribableIdentifiedObject"}},{"@id":"FreqDroopType","@type":"rdfs:Class","rdfs:comment":"Type for Frequency-Droop (Frequency-Watt) operation."},{"@id":"DER","@type":"rdfs:Class","rdfs:comment":"Contains links to DER resources.","rdfs:subClassOf":{"@id":"SubscribableResource"}},{"@id":"DERList","@type":"rdfs:Class","rdfs:comment":"A List element to hold DER objects.","rdfs:subClassOf":{"@id":"List"}},{"@id":"DERSettings","@type":"rdfs:Class","rdfs:comment":"Distributed energy resource settings","rdfs:subClassOf":{"@id":"SubscribableResource"}},{"@id":"DERType","@type":"rdfs:Class","rdfs:comment":"0 - Not applicable / Unknown\n1 - Virtual or mixed DER\n2 - Reciprocating engine\n3 - Fuel cell\n4 - Photovoltaic system\n5 - Combined heat and power\n6 - Other generation system\n80 - Other storage system\n81 - Electric vehicle\n82 - EVSE\n83 - Combined PV and storage\nAll other values reserved.","rdfs:subClassOf":{"@id":"UInt8"},"@enum":{"0":"Not applicable / Unknown","1":"Virtual or mixed DER","2":"Reciprocating engine","3":"Fuel cell","4":"Photovoltaic system","5":"Combined heat and power","6":"Other generation system","80":"Other storage system","81":"Electric vehicle","82":"EVSE","83":"Combined PV and storage"}},{"@id":"DERAvailability","@type":"rdfs:Class","rdfs:comment":"Indicates current reserve generation status","rdfs:subClassOf":{"@id":"SubscribableResource"}},{"@id":"DERCapability","@type":"rdfs:Class","rdfs:comment":"Distributed energy resource type and nameplate ratings.","rdfs:subClassOf":{"@id":"Resource"}},{"@id":"DERControlBase","@type":"rdfs:Class","rdfs:comment":"Distributed Energy Resource (DER) control values."},{"@id":"DERControl","@type":"rdfs:Class","rdfs:comment":"Distributed Energy Resource (DER) time/event-based control.","rdfs:subClassOf":{"@id":"RandomizableEvent"}},{"@id":"DERControlList","@type":"rdfs:Class","rdfs:comment":"A List element to hold DERControl objects.","rdfs:subClassOf":{"@id":"SubscribableList"}},{"@id":"DERControlType","@type":"rdfs:Class","rdfs:comment":"Control modes supported by the DER.  Bit positions SHALL be defined as follows:\n0 - Charge mode\n1 - Discharge mode\n2 - opModConnect (Connect / Disconnect - implies galvanic isolation)\n3 - opModEnergize (Energize / De-Energize)\n4 - opModFixedPFAbsorbW (Fixed Power Factor Setpoint when absorbing active power)\n5 - opModFixedPFInjectW (Fixed Power Factor Setpoint when injecting active power)\n6 - opModFixedVar (Reactive Power Setpoint)\n7 - opModFixedW (Charge / Discharge Setpoint)\n8 - opModFreqDroop (Frequency-Watt Parameterized Mode)\n9 - opModFreqWatt (Frequency-Watt Curve Mode)\n10 - opModHFRTMayTrip (High Frequency Ride Through, May Trip Mode)\n11 - opModHFRTMustTrip (High Frequency Ride Through, Must Trip Mode)\n12 - opModHVRTMayTrip (High Voltage Ride Through, May Trip Mode)\n13 - opModHVRTMomentaryCessation (High Voltage Ride Through, Momentary Cessation Mode)\n14 - opModHVRTMustTrip (High Voltage Ride Through, Must Trip Mode)\n15 - opModLFRTMayTrip (Low Frequency Ride Through, May Trip Mode)\n16 - opModLFRTMustTrip (Low Frequency Ride Through, Must Trip Mode)\n17 - opModLVRTMayTrip (Low Voltage Ride Through, May Trip Mode)\n18 - opModLVRTMomentaryCessation (Low Voltage Ride Through, Momentary Cessation Mode)\n19 - opModLVRTMustTrip (Low Voltage Ride Through, Must Trip Mode)\n20 - opModMaxLimW (Maximum Active Power)\n21 - opModTargetVar (Target Reactive Power)\n22 - opModTargetW (Target Active Power)\n23 - opModVoltVar (Volt-Var Mode)\n24 - opModVoltWatt (Volt-Watt Mode)\n25 - opModWattPF (Watt-PowerFactor Mode)\n26 - opModWattVar (Watt-Var Mode)\nAll other values reserved.","rdfs:subClassOf":{"@id":"HexBinary32"},"@enum":{"0":"Charge mode","1":"Discharge mode","2":"opModConnect (Connect / Disconnect - implies galvanic isolation)","3":"opModEnergize (Energize / De-Energize)","4":"opModFixedPFAbsorbW (Fixed Power Factor Setpoint when absorbing active power)","5":"opModFixedPFInjectW (Fixed Power Factor Setpoint when injecting active power)","6":"opModFixedVar (Reactive Power Setpoint)","7":"opModFixedW (Charge / Discharge Setpoint)","8":"opModFreqDroop (Frequency-Watt Parameterized Mode)","9":"opModFreqWatt (Frequency-Watt Curve Mode)","10":"opModHFRTMayTrip (High Frequency Ride Through, May Trip Mode)","11":"opModHFRTMustTrip (High Frequency Ride Through, Must Trip Mode)","12":"opModHVRTMayTrip (High Voltage Ride Through, May Trip Mode)","13":"opModHVRTMomentaryCessation (High Voltage Ride Through, Momentary Cessation Mode)","14":"opModHVRTMustTrip (High Voltage Ride Through, Must Trip Mode)","15":"opModLFRTMayTrip (Low Frequency Ride Through, May Trip Mode)","16":"opModLFRTMustTrip (Low Frequency Ride Through, Must Trip Mode)","17":"opModLVRTMayTrip (Low Voltage Ride Through, May Trip Mode)","18":"opModLVRTMomentaryCessation (Low Voltage Ride Through, Momentary Cessation Mode)","19":"opModLVRTMustTrip (Low Voltage Ride Through, Must Trip Mode)","20":"opModMaxLimW (Maximum Active Power)","21":"opModTargetVar (Target Reactive Power)","22":"opModTargetW (Target Active Power)","23":"opModVoltVar (Volt-Var Mode)","24":"opModVoltWatt (Volt-Watt Mode)","25":"opModWattPF (Watt-PowerFactor Mode)","26":"opModWattVar (Watt-Var Mode)"}},{"@id":"DERCurve","@type":"rdfs:Class","rdfs:comment":"DER related curves such as Volt-Var mode curves. Relationship between an independent variable (X-axis) and a dependent variable (Y-axis).","rdfs:subClassOf":{"@id":"IdentifiedObject"}},{"@id":"CurrentDERProgramLink","@type":"rdfs:Class","rdfs:comment":"SHALL contain a Link to an instance of DERProgram.  If present, this is the DERProgram containing the currently active DERControl.","rdfs:subClassOf":{"@id":"Link"}},{"@id":"DERCurveList","@type":"rdfs:Class","rdfs:comment":"A List element to hold DERCurve objects.","rdfs:subClassOf":{"@id":"List"}},{"@id":"CurveData","@type":"rdfs:Class","rdfs:comment":"Data point values for defining a curve or schedule"},{"@id":"DERCurveType","@type":"rdfs:Class","rdfs:comment":"0 - opModFreqWatt (Frequency-Watt Curve Mode)\n1 - opModHFRTMayTrip (High Frequency Ride Through, May Trip Mode)\n2 - opModHFRTMustTrip (High Frequency Ride Through, Must Trip Mode)\n3 - opModHVRTMayTrip (High Voltage Ride Through, May Trip Mode)\n4 - opModHVRTMomentaryCessation (High Voltage Ride Through, Momentary Cessation Mode)\n5 - opModHVRTMustTrip (High Voltage Ride Through, Must Trip Mode)\n6 - opModLFRTMayTrip (Low Frequency Ride Through, May Trip Mode)\n7 - opModLFRTMustTrip (Low Frequency Ride Through, Must Trip Mode)\n8 - opModLVRTMayTrip (Low Voltage Ride Through, May Trip Mode)\n9 - opModLVRTMomentaryCessation (Low Voltage Ride Through, Momentary Cessation Mode)\n10 - opModLVRTMustTrip (Low Voltage Ride Through, Must Trip Mode)\n11 - opModVoltVar (Volt-Var Mode)\n12 - opModVoltWatt (Volt-Watt Mode)\n13 - opModWattPF (Watt-PowerFactor Mode)\n14 - opModWattVar (Watt-Var Mode)\nAll other values reserved.","rdfs:subClassOf":{"@id":"UInt8"},"@enum":{"0":"opModFreqWatt (Frequency-Watt Curve Mode)","1":"opModHFRTMayTrip (High Frequency Ride Through, May Trip Mode)","2":"opModHFRTMustTrip (High Frequency Ride Through, Must Trip Mode)","3":"opModHVRTMayTrip (High Voltage Ride Through, May Trip Mode)","4":"opModHVRTMomentaryCessation (High Voltage Ride Through, Momentary Cessation Mode)","5":"opModHVRTMustTrip (High Voltage Ride Through, Must Trip Mode)","6":"opModLFRTMayTrip (Low Frequency Ride Through, May Trip Mode)","7":"opModLFRTMustTrip (Low Frequency Ride Through, Must Trip Mode)","8":"opModLVRTMayTrip (Low Voltage Ride Through, May Trip Mode)","9":"opModLVRTMomentaryCessation (Low Voltage Ride Through, Momentary Cessation Mode)","10":"opModLVRTMustTrip (Low Voltage Ride Through, Must Trip Mode)","11":"opModVoltVar (Volt-Var Mode)","12":"opModVoltWatt (Volt-Watt Mode)","13":"opModWattPF (Watt-PowerFactor Mode)","14":"opModWattVar (Watt-Var Mode)"}},{"@id":"DERProgram","@type":"rdfs:Class","rdfs:comment":"Distributed Energy Resource program.","rdfs:subClassOf":{"@id":"SubscribableIdentifiedObject"}},{"@id":"DERProgramList","@type":"rdfs:Class","rdfs:comment":"A List element to hold DERProgram objects.","rdfs:subClassOf":{"@id":"SubscribableList"}},{"@id":"DERStatus","@type":"rdfs:Class","rdfs:comment":"DER status information.","rdfs:subClassOf":{"@id":"SubscribableResource"}},{"@id":"DERUnitRefType","@type":"rdfs:Class","rdfs:comment":"Specifies context for interpreting percent values:\n0 - N/A\n1 - %setMaxW\n2 - %setMaxVar\n3 - %statVarAvail\n4 - %setEffectiveV\n5 - %setMaxChargeRateW\n6 - %setMaxDischargeRateW\n7 - %statWAvail\nAll other values reserved.","rdfs:subClassOf":{"@id":"UInt8"},"@enum":{"0":"N/A","1":"%setMaxW","2":"%setMaxVar","3":"%statVarAvail","4":"%setEffectiveV","5":"%setMaxChargeRateW","6":"%setMaxDischargeRateW","7":"%statWAvail"}},{"@id":"CurrentRMS","@type":"rdfs:Class","rdfs:comment":"Average flow of charge through a conductor."},{"@id":"FixedPointType","@type":"rdfs:Class","rdfs:comment":"Abstract type for specifying a fixed-point value without a given unit of measure."},{"@id":"UnsignedFixedPointType","@type":"rdfs:Class","rdfs:comment":"Abstract type for specifying an unsigned fixed-point value without a given unit of measure."},{"@id":"ActivePower","@type":"rdfs:Class","rdfs:comment":"The active (real) power P (in W) is the product of root-mean-square (RMS) voltage, RMS current, and cos(theta) where theta is the phase angle of current relative to voltage.  It is the primary measure of the rate of flow of energy."},{"@id":"AmpereHour","@type":"rdfs:Class","rdfs:comment":"Available electric charge"},{"@id":"ApparentPower","@type":"rdfs:Class","rdfs:comment":"The apparent power S (in VA) is the product of root mean square (RMS) voltage and RMS current."},{"@id":"ReactivePower","@type":"rdfs:Class","rdfs:comment":"The reactive power Q (in var) is the product of root mean square (RMS) voltage, RMS current, and sin(theta) where theta is the phase angle of current relative to voltage."},{"@id":"ReactiveSusceptance","@type":"rdfs:Class","rdfs:comment":"Reactive susceptance"},{"@id":"PowerFactor","@type":"rdfs:Class","rdfs:comment":"Specifies a setpoint for Displacement Power Factor, the ratio between apparent and active powers at the fundamental frequency (e.g. 60 Hz)."},{"@id":"PowerFactorWithExcitation","@type":"rdfs:Class","rdfs:comment":"Specifies a setpoint for Displacement Power Factor, the ratio between apparent and active powers at the fundamental frequency (e.g. 60 Hz) and includes an excitation flag."},{"@id":"FixedVar","@type":"rdfs:Class","rdfs:comment":"Specifies a signed setpoint for reactive power."},{"@id":"WattHour","@type":"rdfs:Class","rdfs:comment":"Active (real) energy"},{"@id":"VoltageRMS","@type":"rdfs:Class","rdfs:comment":"Average electric potential difference between two points."},{"@id":"ConnectStatusType","@type":"rdfs:Class","rdfs:comment":"DER ConnectStatus value (bitmap):\n0 - Connected\n1 - Available\n2 - Operating\n3 - Test\n4 - Fault / Error\nAll other values reserved.","@enum":{"0":"Connected","1":"Available","2":"Operating","3":"Test","4":"Fault / Error"}},{"@id":"InverterStatusType","@type":"rdfs:Class","rdfs:comment":"DER InverterStatus value:\n0 - N/A\n1 - off\n2 - sleeping (auto-shutdown) or DER is at low output power/voltage\n3 - starting up or ON but not producing power\n4 - tracking MPPT power point\n5 - forced power reduction/derating\n6 - shutting down\n7 - one or more faults exist\n8 - standby (service on unit) - DER may be at high output voltage/power\n9 - test mode\n10 - as defined in manufacturer status\nAll other values reserved.","@enum":{"0":"N/A","1":"off","2":"sleeping (auto-shutdown) or DER is at low output power/voltage","3":"starting up or ON but not producing power","4":"tracking MPPT power point","5":"forced power reduction/derating","6":"shutting down","7":"one or more faults exist","8":"standby (service on unit) - DER may be at high output voltage/power","9":"test mode","10":"as defined in manufacturer status"}},{"@id":"LocalControlModeStatusType","@type":"rdfs:Class","rdfs:comment":"DER LocalControlModeStatus/value:\n0 \u2013 local control\n1 \u2013 remote control\nAll other values reserved."},{"@id":"ManufacturerStatusType","@type":"rdfs:Class","rdfs:comment":"DER ManufacturerStatus/value: String data type"},{"@id":"OperationalModeStatusType","@type":"rdfs:Class","rdfs:comment":"DER OperationalModeStatus value:\n0 - Not applicable / Unknown\n1 - Off\n2 - Operational mode\n3 - Test mode\nAll other values reserved.","@enum":{"0":"Not applicable / Unknown","1":"Off","2":"Operational mode","3":"Test mode"}},{"@id":"StateOfChargeStatusType","@type":"rdfs:Class","rdfs:comment":"DER StateOfChargeStatus value: Percent data type"},{"@id":"StorageModeStatusType","@type":"rdfs:Class","rdfs:comment":"DER StorageModeStatus value:\n0 \u2013 storage charging\n1 \u2013 storage discharging\n2 \u2013 storage holding\nAll other values reserved."},{"@id":"AccountBalanceLink","@type":"rdfs:Class","rdfs:comment":"SHALL contain a Link to an instance of AccountBalance.","rdfs:subClassOf":{"@id":"Link"}},{"@id":"ActiveBillingPeriodListLink","@type":"rdfs:Class","rdfs:comment":"SHALL contain a Link to a List of active BillingPeriod instances.","rdfs:subClassOf":{"@id":"ListLink"}},{"@id":"ActiveCreditRegisterListLink","@type":"rdfs:Class","rdfs:comment":"SHALL contain a Link to a List of active CreditRegister instances.","rdfs:subClassOf":{"@id":"ListLink"}},{"@id":"ActiveDERControlListLink","@type":"rdfs:Class","rdfs:comment":"SHALL contain a Link to a List of active DERControl instances.","rdfs:subClassOf":{"@id":"ListLink"}},{"@id":"ActiveEndDeviceControlListLink","@type":"rdfs:Class","rdfs:comment":"SHALL contain a Link to a List of active EndDeviceControl instances.","rdfs:subClassOf":{"@id":"ListLink"}},{"@id":"ActiveFlowReservationListLink","@type":"rdfs:Class","rdfs:comment":"SHALL contain a Link to a List of active FlowReservation instances.","rdfs:subClassOf":{"@id":"ListLink"}},{"@id":"ActiveProjectionReadingListLink","@type":"rdfs:Class","rdfs:comment":"SHALL contain a Link to a List of active ProjectionReading instances.","rdfs:subClassOf":{"@id":"ListLink"}},{"@id":"ActiveSupplyInterruptionOverrideListLink","@type":"rdfs:Class","rdfs:comment":"SHALL contain a Link to a List of active SupplyInterruptionOverride instances.","rdfs:subClassOf":{"@id":"ListLink"}},{"@id":"ActiveTargetReadingListLink","@type":"rdfs:Class","rdfs:comment":"SHALL contain a Link to a List of active TargetReading instances.","rdfs:subClassOf":{"@id":"ListLink"}},{"@id":"ActiveTextMessageListLink","@type":"rdfs:Class","rdfs:comment":"SHALL contain a Link to a List of active TextMessage instances.","rdfs:subClassOf":{"@id":"ListLink"}},{"@id":"ActiveTimeTariffIntervalListLink","@type":"rdfs:Class","rdfs:comment":"SHALL contain a Link to a List of active TimeTariffInterval instances.","rdfs:subClassOf":{"@id":"ListLink"}},{"@id":"AssociatedDERProgramListLink","@type":"rdfs:Class","rdfs:comment":"SHALL contain a Link to a List of DERPrograms having the DERControl(s) for this DER.","rdfs:subClassOf":{"@id":"ListLink"}},{"@id":"AssociatedUsagePointLink","@type":"rdfs:Class","rdfs:comment":"SHALL contain a Link to an instance of UsagePoint.  If present, this is the submeter that monitors the DER output.","rdfs:subClassOf":{"@id":"Link"}},{"@id":"BillingPeriodListLink","@type":"rdfs:Class","rdfs:comment":"SHALL contain a Link to a List of BillingPeriod instances.","rdfs:subClassOf":{"@id":"ListLink"}},{"@id":"BillingReadingListLink","@type":"rdfs:Class","rdfs:comment":"SHALL contain a Link to a List of BillingReading instances.","rdfs:subClassOf":{"@id":"ListLink"}},{"@id":"BillingReadingSetListLink","@type":"rdfs:Class","rdfs:comment":"SHALL contain a Link to a List of BillingReadingSet instances.","rdfs:subClassOf":{"@id":"ListLink"}},{"@id":"ConfigurationLink","@type":"rdfs:Class","rdfs:comment":"SHALL contain a Link to an instance of Configuration.","rdfs:subClassOf":{"@id":"Link"}},{"@id":"ConsumptionTariffIntervalListLink","@type":"rdfs:Class","rdfs:comment":"SHALL contain a Link to a List of ConsumptionTariffInterval instances.","rdfs:subClassOf":{"@id":"ListLink"}},{"@id":"CreditRegisterListLink","@type":"rdfs:Class","rdfs:comment":"SHALL contain a Link to a List of CreditRegister instances.","rdfs:subClassOf":{"@id":"ListLink"}},{"@id":"CustomerAccountLink","@type":"rdfs:Class","rdfs:comment":"SHALL contain a Link to an instance of CustomerAccount.","rdfs:subClassOf":{"@id":"Link"}},{"@id":"CustomerAccountListLink","@type":"rdfs:Class","rdfs:comment":"SHALL contain a Link to a List of CustomerAccount instances.","rdfs:subClassOf":{"@id":"ListLink"}},{"@id":"CustomerAgreementListLink","@type":"rdfs:Class","rdfs:comment":"SHALL contain a Link to a List of CustomerAgreement instances.","rdfs:subClassOf":{"@id":"ListLink"}},{"@id":"DemandResponseProgramLink","@type":"rdfs:Class","rdfs:comment":"SHALL contain a Link to an instance of DemandResponseProgram.","rdfs:subClassOf":{"@id":"Link"}},{"@id":"DemandResponseProgramListLink","@type":"rdfs:Class","rdfs:comment":"SHALL contain a Link to a List of DemandResponseProgram instances.","rdfs:subClassOf":{"@id":"ListLink"}},{"@id":"DERAvailabilityLink","@type":"rdfs:Class","rdfs:comment":"SHALL contain a Link to an instance of DERAvailability.","rdfs:subClassOf":{"@id":"Link"}},{"@id":"DefaultDERControlLink","@type":"rdfs:Class","rdfs:comment":"SHALL contain a Link to an instance of DefaultDERControl. This is the default mode of the DER which MAY be overridden by DERControl events.","rdfs:subClassOf":{"@id":"Link"}},{"@id":"DERCapabilityLink","@type":"rdfs:Class","rdfs:comment":"SHALL contain a Link to an instance of DERCapability.","rdfs:subClassOf":{"@id":"Link"}},{"@id":"DERControlListLink","@type":"rdfs:Class","rdfs:comment":"SHALL contain a Link to a List of DERControl instances.","rdfs:subClassOf":{"@id":"ListLink"}},{"@id":"DERCurveLink","@type":"rdfs:Class","rdfs:comment":"SHALL contain a Link to an instance of DERCurve.","rdfs:subClassOf":{"@id":"Link"}},{"@id":"DERCurveListLink","@type":"rdfs:Class","rdfs:comment":"SHALL contain a Link to a List of DERCurve instances.","rdfs:subClassOf":{"@id":"ListLink"}},{"@id":"DERLink","@type":"rdfs:Class","rdfs:comment":"SHALL contain a Link to an instance of DER.","rdfs:subClassOf":{"@id":"Link"}},{"@id":"DERListLink","@type":"rdfs:Class","rdfs:comment":"SHALL contain a Link to a List of DER instances.","rdfs:subClassOf":{"@id":"ListLink"}},{"@id":"DERProgramLink","@type":"rdfs:Class","rdfs:comment":"SHALL contain a Link to an instance of DERProgram.","rdfs:subClassOf":{"@id":"Link"}},{"@id":"DERProgramListLink","@type":"rdfs:Class","rdfs:comment":"SHALL contain a Link to a List of DERProgram instances.","rdfs:subClassOf":{"@id":"ListLink"}},{"@id":"DERSettingsLink","@type":"rdfs:Class","rdfs:comment":"SHALL contain a Link to an instance of DERSettings.","rdfs:subClassOf":{"@id":"Link"}},{"@id":"DERStatusLink","@type":"rdfs:Class","rdfs:comment":"SHALL contain a Link to an instance of DERStatus.","rdfs:subClassOf":{"@id":"Link"}},{"@id":"DeviceCapabilityLink","@type":"rdfs:Class","rdfs:comment":"SHALL contain a Link to an instance of DeviceCapability.","rdfs:subClassOf":{"@id":"Link"}},{"@id":"DeviceInformationLink","@type":"rdfs:Class","rdfs:comment":"SHALL contain a Link to an instance of DeviceInformation.","rdfs:subClassOf":{"@id":"Link"}},{"@id":"DeviceStatusLink","@type":"rdfs:Class","rdfs:comment":"SHALL contain a Link to an instance of DeviceStatus.","rdfs:subClassOf":{"@id":"Link"}},{"@id":"EndDeviceControlListLink","@type":"rdfs:Class","rdfs:comment":"SHALL contain a Link to a List of EndDeviceControl instances.","rdfs:subClassOf":{"@id":"ListLink"}},{"@id":"EndDeviceLink","@type":"rdfs:Class","rdfs:comment":"SHALL contain a Link to an instance of EndDevice.","rdfs:subClassOf":{"@id":"Link"}},{"@id":"EndDeviceListLink","@type":"rdfs:Class","rdfs:comment":"SHALL contain a Link to a List of EndDevice instances.","rdfs:subClassOf":{"@id":"ListLink"}},{"@id":"FileLink","@type":"rdfs:Class","rdfs:comment":"This element MUST be set to the URI of the most recent File being loaded/activated by the LD. In the case of file status 0, this element MUST be omitted.","rdfs:subClassOf":{"@id":"Link"}},{"@id":"FileListLink","@type":"rdfs:Class","rdfs:comment":"SHALL contain a Link to a List of File instances.","rdfs:subClassOf":{"@id":"ListLink"}},{"@id":"FileStatusLink","@type":"rdfs:Class","rdfs:comment":"SHALL contain a Link to an instance of FileStatus.","rdfs:subClassOf":{"@id":"Link"}},{"@id":"FlowReservationRequestListLink","@type":"rdfs:Class","rdfs:comment":"SHALL contain a Link to a List of FlowReservationRequest instances.","rdfs:subClassOf":{"@id":"ListLink"}},{"@id":"FlowReservationResponseListLink","@type":"rdfs:Class","rdfs:comment":"SHALL contain a Link to a List of FlowReservationResponse instances.","rdfs:subClassOf":{"@id":"ListLink"}},{"@id":"FunctionSetAssignmentsListLink","@type":"rdfs:Class","rdfs:comment":"SHALL contain a Link to a List of FunctionSetAssignments instances.","rdfs:subClassOf":{"@id":"ListLink"}},{"@id":"HistoricalReadingListLink","@type":"rdfs:Class","rdfs:comment":"SHALL contain a Link to a List of HistoricalReading instances.","rdfs:subClassOf":{"@id":"ListLink"}},{"@id":"IPAddrListLink","@type":"rdfs:Class","rdfs:comment":"SHALL contain a Link to a List of IPAddr instances.","rdfs:subClassOf":{"@id":"ListLink"}},{"@id":"IPInterfaceListLink","@type":"rdfs:Class","rdfs:comment":"SHALL contain a Link to a List of IPInterface instances.","rdfs:subClassOf":{"@id":"ListLink"}},{"@id":"LLInterfaceListLink","@type":"rdfs:Class","rdfs:comment":"SHALL contain a Link to a List of LLInterface instances.","rdfs:subClassOf":{"@id":"ListLink"}},{"@id":"LoadShedAvailabilityListLink","@type":"rdfs:Class","rdfs:comment":"SHALL contain a Link to a List of LoadShedAvailability instances.","rdfs:subClassOf":{"@id":"ListLink"}},{"@id":"LogEventListLink","@type":"rdfs:Class","rdfs:comment":"SHALL contain a Link to a List of LogEvent instances.","rdfs:subClassOf":{"@id":"ListLink"}},{"@id":"MessagingProgramListLink","@type":"rdfs:Class","rdfs:comment":"SHALL contain a Link to a List of MessagingProgram instances.","rdfs:subClassOf":{"@id":"ListLink"}},{"@id":"MeterReadingLink","@type":"rdfs:Class","rdfs:comment":"SHALL contain a Link to an instance of MeterReading.","rdfs:subClassOf":{"@id":"Link"}},{"@id":"MeterReadingListLink","@type":"rdfs:Class","rdfs:comment":"SHALL contain a Link to a List of MeterReading instances.","rdfs:subClassOf":{"@id":"ListLink"}},{"@id":"MirrorUsagePointListLink","@type":"rdfs:Class","rdfs:comment":"SHALL contain a Link to a List of MirrorUsagePoint instances.","rdfs:subClassOf":{"@id":"ListLink"}},{"@id":"NeighborListLink","@type":"rdfs:Class","rdfs:comment":"SHALL contain a Link to a List of Neighbor instances.","rdfs:subClassOf":{"@id":"ListLink"}},{"@id":"NotificationListLink","@type":"rdfs:Class","rdfs:comment":"SHALL contain a Link to a List of Notification instances.","rdfs:subClassOf":{"@id":"ListLink"}},{"@id":"PowerStatusLink","@type":"rdfs:Class","rdfs:comment":"SHALL contain a Link to an instance of PowerStatus.","rdfs:subClassOf":{"@id":"Link"}},{"@id":"PrepaymentLink","@type":"rdfs:Class","rdfs:comment":"SHALL contain a Link to an instance of Prepayment.","rdfs:subClassOf":{"@id":"Link"}},{"@id":"PrepaymentListLink","@type":"rdfs:Class","rdfs:comment":"SHALL contain a Link to a List of Prepayment instances.","rdfs:subClassOf":{"@id":"ListLink"}},{"@id":"PrepayOperationStatusLink","@type":"rdfs:Class","rdfs:comment":"SHALL contain a Link to an instance of PrepayOperationStatus.","rdfs:subClassOf":{"@id":"Link"}},{"@id":"PriceResponseCfgListLink","@type":"rdfs:Class","rdfs:comment":"SHALL contain a Link to a List of PriceResponseCfg instances.","rdfs:subClassOf":{"@id":"ListLink"}},{"@id":"ProjectionReadingListLink","@type":"rdfs:Class","rdfs:comment":"SHALL contain a Link to a List of ProjectionReading instances.","rdfs:subClassOf":{"@id":"ListLink"}},{"@id":"RateComponentLink","@type":"rdfs:Class","rdfs:comment":"SHALL contain a Link to an instance of RateComponent.","rdfs:subClassOf":{"@id":"Link"}},{"@id":"RateComponentListLink","@type":"rdfs:Class","rdfs:comment":"SHALL contain a Link to a List of RateComponent instances.","rdfs:subClassOf":{"@id":"ListLink"}},{"@id":"ReadingLink","@type":"rdfs:Class","rdfs:comment":"A Link to a Reading.","rdfs:subClassOf":{"@id":"Link"}},{"@id":"ReadingListLink","@type":"rdfs:Class","rdfs:comment":"SHALL contain a Link to a List of Reading instances.","rdfs:subClassOf":{"@id":"ListLink"}},{"@id":"ReadingSetListLink","@type":"rdfs:Class","rdfs:comment":"SHALL contain a Link to a List of ReadingSet instances.","rdfs:subClassOf":{"@id":"ListLink"}},{"@id":"ReadingTypeLink","@type":"rdfs:Class","rdfs:comment":"SHALL contain a Link to an instance of ReadingType.","rdfs:subClassOf":{"@id":"Link"}},{"@id":"RegistrationLink","@type":"rdfs:Class","rdfs:comment":"SHALL contain a Link to an instance of Registration.","rdfs:subClassOf":{"@id":"Link"}},{"@id":"ResponseListLink","@type":"rdfs:Class","rdfs:comment":"SHALL contain a Link to a List of Response instances.","rdfs:subClassOf":{"@id":"ListLink"}},{"@id":"ResponseSetListLink","@type":"rdfs:Class","rdfs:comment":"SHALL contain a Link to a List of ResponseSet instances.","rdfs:subClassOf":{"@id":"ListLink"}},{"@id":"RPLInstanceListLink","@type":"rdfs:Class","rdfs:comment":"SHALL contain a Link to a List of RPLInterface instances.","rdfs:subClassOf":{"@id":"ListLink"}},{"@id":"RPLSourceRoutesListLink","@type":"rdfs:Class","rdfs:comment":"SHALL contain a Link to a List of RPLSourceRoutes instances.","rdfs:subClassOf":{"@id":"ListLink"}},{"@id":"SelfDeviceLink","@type":"rdfs:Class","rdfs:comment":"SHALL contain a Link to an instance of SelfDevice.","rdfs:subClassOf":{"@id":"Link"}},{"@id":"ServiceSupplierLink","@type":"rdfs:Class","rdfs:comment":"SHALL contain a Link to an instance of ServiceSupplier.","rdfs:subClassOf":{"@id":"Link"}},{"@id":"SubscriptionListLink","@type":"rdfs:Class","rdfs:comment":"SHALL contain a Link to a List of Subscription instances.","rdfs:subClassOf":{"@id":"ListLink"}},{"@id":"SupplyInterruptionOverrideListLink","@type":"rdfs:Class","rdfs:comment":"SHALL contain a Link to a List of SupplyInterruptionOverride instances.","rdfs:subClassOf":{"@id":"ListLink"}},{"@id":"SupportedLocaleListLink","@type":"rdfs:Class","rdfs:comment":"SHALL contain a Link to a List of SupportedLocale instances.","rdfs:subClassOf":{"@id":"ListLink"}},{"@id":"TargetReadingListLink","@type":"rdfs:Class","rdfs:comment":"SHALL contain a Link to a List of TargetReading instances.","rdfs:subClassOf":{"@id":"ListLink"}},{"@id":"TariffProfileLink","@type":"rdfs:Class","rdfs:comment":"SHALL contain a Link to an instance of TariffProfile.","rdfs:subClassOf":{"@id":"Link"}},{"@id":"TariffProfileListLink","@type":"rdfs:Class","rdfs:comment":"SHALL contain a Link to a List of TariffProfile instances.","rdfs:subClassOf":{"@id":"ListLink"}},{"@id":"TextMessageListLink","@type":"rdfs:Class","rdfs:comment":"SHALL contain a Link to a List of TextMessage instances.","rdfs:subClassOf":{"@id":"ListLink"}},{"@id":"TimeLink","@type":"rdfs:Class","rdfs:comment":"SHALL contain a Link to an instance of Time.","rdfs:subClassOf":{"@id":"Link"}},{"@id":"TimeTariffIntervalListLink","@type":"rdfs:Class","rdfs:comment":"SHALL contain a Link to a List of TimeTariffInterval instances.","rdfs:subClassOf":{"@id":"ListLink"}},{"@id":"UsagePointLink","@type":"rdfs:Class","rdfs:comment":"SHALL contain a Link to an instance of UsagePoint.","rdfs:subClassOf":{"@id":"Link"}},{"@id":"UsagePointListLink","@type":"rdfs:Class","rdfs:comment":"SHALL contain a Link to a List of UsagePoint instances.","rdfs:subClassOf":{"@id":"ListLink"}},{"@id":"IdentifiedObject","@type":"rdfs:Class","rdfs:comment":"This is a root class to provide common naming attributes for all classes needing naming attributes","rdfs:subClassOf":{"@id":"Resource"}},{"@id":"Link","@type":"rdfs:Class","rdfs:comment":"Links provide a reference, via URI, to another resource."},{"@id":"List","@type":"rdfs:Class","rdfs:comment":"Container to hold a collection of object instances or references. See Design Pattern section for additional details.","rdfs:subClassOf":{"@id":"Resource"}},{"@id":"ListLink","@type":"rdfs:Class","rdfs:comment":"ListLinks provide a reference, via URI, to a List.","rdfs:subClassOf":{"@id":"Link"}},{"@id":"Resource","@type":"rdfs:Class","rdfs:comment":"A resource is an addressable unit of information, either a collection (List) or instance of an object (identifiedObject, or simply, Resource)"},{"@id":"RespondableIdentifiedObject","@type":"rdfs:Class","rdfs:comment":"An IdentifiedObject to which a Response can be requested.","rdfs:subClassOf":{"@id":"RespondableResource"}},{"@id":"RespondableResource","@type":"rdfs:Class","rdfs:comment":"A Resource to which a Response can be requested.","rdfs:subClassOf":{"@id":"Resource"}},{"@id":"RespondableSubscribableIdentifiedObject","@type":"rdfs:Class","rdfs:comment":"An IdentifiedObject to which a Response can be requested.","rdfs:subClassOf":{"@id":"RespondableResource"}},{"@id":"SubscribableIdentifiedObject","@type":"rdfs:Class","rdfs:comment":"An IdentifiedObject to which a Subscription can be requested.","rdfs:subClassOf":{"@id":"SubscribableResource"}},{"@id":"SubscribableList","@type":"rdfs:Class","rdfs:comment":"A List to which a Subscription can be requested.","rdfs:subClassOf":{"@id":"SubscribableResource"}},{"@id":"SubscribableResource","@type":"rdfs:Class","rdfs:comment":"A Resource to which a Subscription can be requested.","rdfs:subClassOf":{"@id":"Resource"}},{"@id":"Error","@type":"rdfs:Class","rdfs:comment":"Contains information about the nature of an error if a request could not be completed successfully."},{"@id":"Event","@type":"rdfs:Class","rdfs:comment":"An Event indicates information that applies to a particular period of time. Events SHALL be executed relative to the time of the server, as described in the Time function set section 11.1.","rdfs:subClassOf":{"@id":"RespondableSubscribableIdentifiedObject"}},{"@id":"EventStatus","@type":"rdfs:Class","rdfs:comment":"Current status information relevant to a specific object. The Status object is used to indicate the current status of an Event. Devices can read the containing resource (e.g. TextMessage) to get the most up to date status of the event.  Devices can also subscribe to a specific resource instance to get updates when any of its attributes change, including the Status object."},{"@id":"RandomizableEvent","@type":"rdfs:Class","rdfs:comment":"An Event that can indicate time ranges over which the start time and duration SHALL be randomized.","rdfs:subClassOf":{"@id":"Event"}},{"@id":"AccumulationBehaviourType","@type":"rdfs:Class","rdfs:comment":"0 = Not Applicable (default, if not specified)\n\n3 = Cumulative\nThe sum of the previous billing period values. Note: \u201cCumulative\u201d is commonly used in conjunction with \u201cdemand.\u201d Each demand reset causes the maximum demand value for the present billing period (since the last demand reset) to accumulate as an accumulative total of all maximum demands. So instead of \u201czeroing\u201d the demand register, a demand reset has the affect of adding the present maximum demand to this accumulating total.\n\n4 = DeltaData\nThe difference between the value at the end of the prescribed interval and the beginning of the interval. This is used for incremental interval data. \nNote: One common application would be for load profile data, another use might be to report the number of events within an interval (such as the number of equipment energizations within the specified period of time.)\n\n6 = Indicating\nAs if a needle is swung out on the meter face to a value to indicate the current value. (Note: An \u201cindicating\u201d value is typically measured over hundreds of milliseconds or greater, or may imply a \u201cpusher\u201d mechanism to capture a value. Compare this to \u201cinstantaneous\u201d which is measured over a shorter period of time.) \n\n9 = Summation\nA form of accumulation which is selective with respect to time. \nNote : \u201cSummation\u201d could be considered a specialization of \u201cBulk Quantity\u201d according to the rules of inheritance where \u201cSummation\u201d selectively accumulates pulses over a timing pattern, and \u201cBulkQuantity\u201d accumulates pulses all of the time.\n\n12 = Instantaneous\nTypically measured over the fastest period of time allowed by the definition of the metric (usually milliseconds or tens of milliseconds.) (Note: \u201cInstantaneous\u201d was moved to attribute #3 in 61968-9Ed2 from attribute #1 in 61968-9Ed1.)\n\nAll other values reserved.","rdfs:subClassOf":{"@id":"UInt8"},"@enum":{"0":"Not Applicable","3":"Cumulative","4":"DeltaData","6":"Indicating","9":"Summation","12":"Instantaneous"}},{"@id":"ApplianceLoadReductionType","@type":"rdfs:Class","rdfs:comment":"0 - Delay Appliance Load\nParameter requesting the appliance to respond by providing a moderate load reduction for the duration of a delay period.  Typically referring to a \u201cnon-emergency\u201d event in which appliances can continue operating if already in a load consuming period.\n\n1 - Temporary Appliance Load Reduction\nParameter requesting the appliance to respond by providing an aggressive load reduction for a short time period.  Typically referring to an \u201cemergency/spinning reserve\u201d event in which an appliance should start shedding load if currently in a load consuming period. \n\n* Full definition of how appliances react when receiving each parameter is document in the EPA document - ENERGY STAR\u00ae Program Requirements, Product Specification for Residential Refrigerators and Freezers, Eligibility Criteria 5, Draft 2 Version 5.0.\n\nAll other values reserved.","rdfs:subClassOf":{"@id":"UInt8"},"@enum":{"0":"Delay Appliance Load","1":"Temporary Appliance Load Reduction"}},{"@id":"CommodityType","@type":"rdfs:Class","rdfs:comment":"0 = Not Applicable (default, if not specified)\n1 = Electricity secondary metered value (a premises meter is typically on the low voltage, or secondary, side of a service transformer)\n2 = Electricity primary metered value (measured on the high voltage, or primary, side of the service transformer)\n4 = Air\n7 = NaturalGas\n8 = Propane\n9 = PotableWater\n10 = Steam\n11 = WasteWater\n12 = HeatingFluid\n13 = CoolingFluid\nAll other values reserved.","rdfs:subClassOf":{"@id":"UInt8"},"@enum":{"0":"Not Applicable","1":"Electricity secondary metered value (a premises meter is typically on the low voltage, or secondary, side of a service transformer)","2":"Electricity primary metered value (measured on the high voltage, or primary, side of the service transformer)","4":"Air","7":"NaturalGas","8":"Propane","9":"PotableWater","10":"Steam","11":"WasteWater","12":"HeatingFluid","13":"CoolingFluid"}},{"@id":"ConsumptionBlockType","@type":"rdfs:Class","rdfs:comment":"0 = Not Applicable (default, if not specified)\n1 = Block 1\n2 = Block 2\n3 = Block 3\n4 = Block 4\n5 = Block 5\n6 = Block 6\n7 = Block 7\n8 = Block 8\n9 = Block 9\n10 = Block 10\n11 = Block 11\n12 = Block 12\n13 = Block 13\n14 = Block 14\n15 = Block 15\n16 = Block 16\nAll other values reserved.","rdfs:subClassOf":{"@id":"UInt8"},"@enum":{"0":"Not Applicable","1":"Block 1","2":"Block 2","3":"Block 3","4":"Block 4","5":"Block 5","6":"Block 6","7":"Block 7","8":"Block 8","9":"Block 9","10":"Block 10","11":"Block 11","12":"Block 12","13":"Block 13","14":"Block 14","15":"Block 15","16":"Block 16"}},{"@id":"CurrencyCode","@type":"rdfs:Class","rdfs:comment":"Follows codes defined in [ISO 4217]. \n0 - Not Applicable (default, if not specified)\n36 - Australian Dollar\n124 - Canadian Dollar\n840 - US Dollar\n978 - Euro\nThis is not a complete list.","rdfs:subClassOf":{"@id":"UInt16"},"@enum":{"0":"Not Applicable","36":"Australian Dollar","124":"Canadian Dollar","840":"US Dollar","978":"Euro"}},{"@id":"DataQualifierType","@type":"rdfs:Class","rdfs:comment":"0 = Not Applicable (default, if not specified)\n2 = Average\n8 = Maximum\n9 = Minimum\n12 = Normal\n29 = Standard Deviation of a Population (typically indicated by a lower case sigma)\n30 = Standard Deviation of a Sample Drawn from a Population (typically indicated by a lower case 's')\nAll other values reserved.","rdfs:subClassOf":{"@id":"UInt8"},"@enum":{"0":"Not Applicable","2":"Average","8":"Maximum","9":"Minimum","12":"Normal","29":"Standard Deviation of a Population (typically indicated by a lower case sigma)","30":"Standard Deviation of a Sample Drawn from a Population (typically indicated by a lower case 's')"}},{"@id":"DateTimeInterval","@type":"rdfs:Class","rdfs:comment":"Interval of date and time."},{"@id":"DeviceCategoryType","@type":"rdfs:Class","rdfs:comment":"The Device category types defined.\nBit positions SHALL be defined as follows:\n0 - Programmable Communicating Thermostat\n1 - Strip Heaters\n2 - Baseboard Heaters\n3 - Water Heater\n4 - Pool Pump\n5 - Sauna\n6 - Hot Tub\n7 - Smart Appliance\n8 - Irrigation Pump\n9 - Managed Commercial and Industrial (C&amp;I) Loads\n10 - Simple Misc. (Residential On/Off) Loads\n11 - Exterior Lighting\n12 - Interior Lighting\n13 - Load Control Switch\n14 - Energy Management System\n15 - Smart Energy Module\n16 - Electric Vehicle\n17 - EVSE\n18 - Virtual or Mixed DER\n19 - Reciprocating Engine\n20 - Fuel Cell\n21 - Photovoltaic System\n22 - Combined Heat and Power\n23 - Combined PV and Storage\n24 - Other Generation System\n25 - Other Storage System\nAll other values reserved.","rdfs:subClassOf":{"@id":"HexBinary32"},"@enum":{"0":"Programmable Communicating Thermostat","1":"Strip Heaters","2":"Baseboard Heaters","3":"Water Heater","4":"Pool Pump","5":"Sauna","6":"Hot Tub","7":"Smart Appliance","8":"Irrigation Pump","9":"Managed Commercial and Industrial (C&amp;I) Loads","10":"Simple Misc. (Residential On/Off) Loads","11":"Exterior Lighting","12":"Interior Lighting","13":"Load Control Switch","14":"Energy Management System","15":"Smart Energy Module","16":"Electric Vehicle","17":"EVSE","18":"Virtual or Mixed DER","19":"Reciprocating Engine","20":"Fuel Cell","21":"Photovoltaic System","22":"Combined Heat and Power","23":"Combined PV and Storage","24":"Other Generation System","25":"Other Storage System"}},{"@id":"DstRuleType","@type":"rdfs:Class","rdfs:comment":"Bit map encoded rule from which is calculated the start or end time, within the current year, to which daylight savings time offset must be applied. \n\nThe rule encoding:\nBits  0 - 11: seconds 0 - 3599\nBits 12 - 16: hours 0 - 23\nBits 17 - 19: day of the week 0 = not applicable, 1 - 7 (Monday = 1)\nBits 20 - 24: day of the month 0 = not applicable, 1 - 31\nBits 25 - 27: operator  (detailed below)\nBits 28 - 31: month 1 - 12\n\nRule value of 0xFFFFFFFF means rule processing/DST correction is disabled.\n\nThe operators:\n\n0: DST starts/ends on the Day of the Month\n1: DST starts/ends on the Day of the Week that is on or after the Day of the Month\n2: DST starts/ends on the first occurrence of the Day of the Week in a month\n3: DST starts/ends on the second occurrence of the Day of the Week in a month\n4: DST starts/ends on the third occurrence of the Day of the Week in a month\n5: DST starts/ends on the forth occurrence of the Day of the Week in a month\n6: DST starts/ends on the fifth occurrence of the Day of the Week in a month\n7: DST starts/ends on the last occurrence of the Day of the Week in a month\n\nAn example: DST starts on third Friday in March at 1:45 AM.  The rule...\nSeconds: 2700\nHours: 1\nDay of Week: 5\nDay of Month: 0\nOperator: 4\nMonth: 3","rdfs:subClassOf":{"@id":"HexBinary32"},"@enum":{"0":"DST starts/ends on the Day of the Month","1":"DST starts/ends on the Day of the Week that is on or after the Day of the Month","2":"DST starts/ends on the first occurrence of the Day of the Week in a month","3":"DST starts/ends on the second occurrence of the Day of the Week in a month","4":"DST starts/ends on the third occurrence of the Day of the Week in a month","5":"DST starts/ends on the forth occurrence of the Day of the Week in a month","6":"DST starts/ends on the fifth occurrence of the Day of the Week in a month","7":"DST starts/ends on the last occurrence of the Day of the Week in a month"}},{"@id":"FlowDirectionType","@type":"rdfs:Class","rdfs:comment":"0 = Not Applicable (default, if not specified)\n1 = Forward (delivered to customer)\n19 = Reverse (received from customer)\nAll other values reserved.","rdfs:subClassOf":{"@id":"UInt8"},"@enum":{"0":"Not Applicable","1":"Forward (delivered to customer)","19":"Reverse (received from customer)"}},{"@id":"GPSLocationType","@type":"rdfs:Class","rdfs:comment":"Specifies a GPS location, expressed in WGS 84 coordinates."},{"@id":"KindType","@type":"rdfs:Class","rdfs:comment":"0 = Not Applicable (default, if not specified)\n3 = Currency\n8 = Demand\n12 = Energy\n37 = Power\nAll other values reserved.","rdfs:subClassOf":{"@id":"UInt8"},"@enum":{"0":"Not Applicable","3":"Currency","8":"Demand","12":"Energy","37":"Power"}},{"@id":"LocaleType","@type":"rdfs:Class","rdfs:comment":"[RFC 4646] identifier of a language-region","rdfs:subClassOf":{"@id":"String42"}},{"@id":"mRIDType","@type":"rdfs:Class","rdfs:comment":"A master resource identifier. The IANA PEN [PEN] provider ID SHALL be specified in bits 0-31, the least-significant bits, and objects created by that provider SHALL be assigned unique IDs with the remaining 96 bits. \n0xFFFFFFFFFFFFFFFFFFFFFFFF[XXXXXXXX], where [XXXXXXXX] is the PEN, is reserved for a object that is being created (e.g., a ReadingSet for the current time that is still accumulating). \nExcept for this special reserved identifier, each modification of an object (resource) representation MUST have a different \"version\".","rdfs:subClassOf":{"@id":"HexBinary128"}},{"@id":"OneHourRangeType","@type":"rdfs:Class","rdfs:comment":"A signed time offset, typically applied to a Time value, expressed in seconds, with range -3600 to 3600.","rdfs:subClassOf":{"@id":"Int16"}},{"@id":"PENType","@type":"rdfs:Class","rdfs:comment":"IANA Private Enterprise Number [PEN].","rdfs:subClassOf":{"@id":"UInt32"}},{"@id":"PerCent","@type":"rdfs:Class","rdfs:comment":"Used for percentages, specified in hundredths of a percent, 0 - 10000. (10000 = 100%)","rdfs:subClassOf":{"@id":"UInt16"}},{"@id":"PhaseCode","@type":"rdfs:Class","rdfs:comment":"0 = Not Applicable (default, if not specified)\n32 = Phase C (and S2)\n33 = Phase CN (and S2N)\n40 = Phase CA\n64 = Phase B\n65 = Phase BN\n66 = Phase BC\n128 = Phase A (and S1)\n129 = Phase AN (and S1N)\n132 = Phase AB\n224 = Phase ABC\nAll other values reserved.","rdfs:subClassOf":{"@id":"UInt8"},"@enum":{"0":"Not Applicable","32":"Phase C (and S2)","33":"Phase CN (and S2N)","40":"Phase CA","64":"Phase B","65":"Phase BN","66":"Phase BC","128":"Phase A (and S1)","129":"Phase AN (and S1N)","132":"Phase AB","224":"Phase ABC"}},{"@id":"PINType","@type":"rdfs:Class","rdfs:comment":"6 digit unsigned decimal integer (0 - 999999). \n(Note that this only requires 20 bits, if it can be allocated.)","rdfs:subClassOf":{"@id":"UInt32"}},{"@id":"PowerOfTenMultiplierType","@type":"rdfs:Class","rdfs:comment":"-9 = nano=x10^-9\n-6 = micro=x10^-6\n-3 = milli=x10^-3\n0 = none=x1 (default, if not specified)\n1 = deca=x10\n2 = hecto=x100\n3 = kilo=x1000\n6 = Mega=x10^6\n9 = Giga=x10^9\nThis is not a complete list. Any integer between -9 and 9 SHALL be supported, indicating the power of ten multiplier for the units.","rdfs:subClassOf":{"@id":"Int8"},"@enum":{"0":"none=x1","1":"deca=x10","2":"hecto=x100","3":"kilo=x1000","6":"Mega=x10^6","9":"Giga=x10^9"}},{"@id":"PrimacyType","@type":"rdfs:Class","rdfs:comment":"Values possible for indication of \"Primary\" provider: \n0: In home energy management system\n1: Contracted premises service provider\n2: Non-contractual service provider\n3 - 64: Reserved\n65 - 191: User-defined\n192 - 255: Reserved\n\nLower numbers indicate higher priority.","rdfs:subClassOf":{"@id":"UInt8"},"@enum":{"0":"In home energy management system","1":"Contracted premises service provider","2":"Non-contractual service provider"}},{"@id":"RealEnergy","@type":"rdfs:Class","rdfs:comment":"Real electrical energy"},{"@id":"RoleFlagsType","@type":"rdfs:Class","rdfs:comment":"Specifies the roles that apply to a usage point.\nBit 0 - isMirror - SHALL be set if the server is not the measurement device\nBit 1 - isPremisesAggregationPoint - SHALL be set if the UsagePoint is the point of delivery for a premises\nBit 2 - isPEV - SHALL be set if the usage applies to an electric vehicle\nBit 3 - isDER - SHALL be set if the usage applies to a distributed energy resource, capable of delivering power to the grid.\nBit 4 - isRevenueQuality - SHALL be set if usage was measured by a device certified as revenue quality\nBit 5 - isDC - SHALL be set if the usage point measures direct current \nBit 6 - isSubmeter - SHALL be set if the usage point is not a premises aggregation point\nBit 7-15 - Reserved","rdfs:subClassOf":{"@id":"HexBinary16"}},{"@id":"ServiceKind","@type":"rdfs:Class","rdfs:comment":"Service kind\n0 - electricity\n1 - gas\n2 - water\n3 - time\n4 - pressure\n5 - heat\n6 - cooling\nAll other values reserved.","rdfs:subClassOf":{"@id":"UInt8"},"@enum":{"0":"electricity","1":"gas","2":"water","3":"time","4":"pressure","5":"heat","6":"cooling"}},{"@id":"SFDIType","@type":"rdfs:Class","rdfs:comment":"Unsigned integer, max inclusive 687194767359, which is 2^36-1 (68719476735), with added check digit. See Section 8.3.2 for check digit calculation.","rdfs:subClassOf":{"@id":"UInt40"}},{"@id":"SignedPerCent","@type":"rdfs:Class","rdfs:comment":"Used for signed percentages, specified in hundredths of a percent, -10000 - 10000. (10000 = 100%)","rdfs:subClassOf":{"@id":"Int16"}},{"@id":"SignedRealEnergy","@type":"rdfs:Class","rdfs:comment":"Real electrical energy, signed."},{"@id":"TimeOffsetType","@type":"rdfs:Class","rdfs:comment":"A signed time offset, typically applied to a Time value, expressed in seconds.","rdfs:subClassOf":{"@id":"Int32"}},{"@id":"TimeType","@type":"rdfs:Class","rdfs:comment":"Time is a signed 64 bit value representing the number of seconds since 0 hours, 0 minutes, 0 seconds, on the 1st of January, 1970, in UTC, not counting leap seconds.","rdfs:subClassOf":{"@id":"Int64"}},{"@id":"TOUType","@type":"rdfs:Class","rdfs:comment":"0 = Not Applicable (default, if not specified)\n1 = TOU A\n2 = TOU B\n3 = TOU C\n4 = TOU D\n5 = TOU E\n6 = TOU F\n7 = TOU G\n8 = TOU H\n9 = TOU I\n10 = TOU J\n11 = TOU K\n12 = TOU L\n13 = TOU M\n14 = TOU N\n15 = TOU O\nAll other values reserved.","rdfs:subClassOf":{"@id":"UInt8"},"@enum":{"0":"Not Applicable","1":"TOU A","2":"TOU B","3":"TOU C","4":"TOU D","5":"TOU E","6":"TOU F","7":"TOU G","8":"TOU H","9":"TOU I","10":"TOU J","11":"TOU K","12":"TOU L","13":"TOU M","14":"TOU N","15":"TOU O"}},{"@id":"UnitType","@type":"rdfs:Class","rdfs:comment":"The unit types defined for end device control target reductions.\n0 - kWh \n1 - kW  \n2 - Watts \n3 - Cubic Meters \n4 - Cubic Feet \n5 - US Gallons \n6 - Imperial Gallons \n7 - BTUs \n8 - Liters \n9 - kPA (gauge) \n10 - kPA (absolute)  \n11 - Mega Joule \n12 - Unitless\nAll other values reserved.","rdfs:subClassOf":{"@id":"UInt8"},"@enum":{"0":"kWh","1":"kW","2":"Watts","3":"Cubic Meters","4":"Cubic Feet","5":"US Gallons","6":"Imperial Gallons","7":"BTUs","8":"Liters","9":"kPA (gauge)","10":"kPA (absolute)","11":"Mega Joule","12":"Unitless"}},{"@id":"UnitValueType","@type":"rdfs:Class","rdfs:comment":"Type for specification of a specific value, with units and power of ten multiplier."},{"@id":"UomType","@type":"rdfs:Class","rdfs:comment":"The following values are recommended values sourced from the unit of measure enumeration in IEC 61968-9 [61968]. Other values from the unit of measure enumeration in IEC 61968-9 [61968] MAY be used.\n0 = Not Applicable (default, if not specified)\n5 = A (Current in Amperes (RMS))\n6 = Kelvin (Temperature)\n23 = Degrees Celsius (Relative temperature)\n29 = Voltage\n31 = J (Energy joule)\n33 = Hz (Frequency)\n38 =W (Real power in Watts)\n42 = m3 (Cubic Meter)\n61 = VA (Apparent power)\n63 = var (Reactive power)\n65 = CosTheta (Displacement Power Factor)\n67 = V\u00b2 (Volts squared)\n69 = A\u00b2 (Amp squared)\n71 = VAh (Apparent energy)\n72 = Wh (Real energy in Watt-hours)\n73 = varh (Reactive energy)\n106 = Ah (Ampere-hours / Available Charge)\n119 = ft3 (Cubic Feet)\n122 = ft3/h (Cubic Feet per Hour)\n125 = m3/h (Cubic Meter per Hour)\n128 = US gl (US Gallons)\n129 = US gl/h (US Gallons per Hour)\n130 = IMP gl (Imperial Gallons)\n131 = IMP gl/h (Imperial Gallons per Hour)\n132 = BTU\n133 = BTU/h\n134 = Liter\n137 = L/h (Liters per Hour)\n140 = PA(gauge)\n155 = PA(absolute)\n169 = Therm","rdfs:subClassOf":{"@id":"UInt8"},"@enum":{"0":"Not Applicable","5":"A (Current in Amperes (RMS))","6":"Kelvin (Temperature)","23":"Degrees Celsius (Relative temperature)","29":"Voltage","31":"J (Energy joule)","33":"Hz (Frequency)","38":"W (Real power in Watts)","42":"m3 (Cubic Meter)","61":"VA (Apparent power)","63":"var (Reactive power)","65":"CosTheta (Displacement Power Factor)","67":"V\u00b2 (Volts squared)","69":"A\u00b2 (Amp squared)","71":"VAh (Apparent energy)","72":"Wh (Real energy in Watt-hours)","73":"varh (Reactive energy)","106":"Ah (Ampere-hours / Available Charge)","119":"ft3 (Cubic Feet)","122":"ft3/h (Cubic Feet per Hour)","125":"m3/h (Cubic Meter per Hour)","128":"US gl (US Gallons)","129":"US gl/h (US Gallons per Hour)","130":"IMP gl (Imperial Gallons)","131":"IMP gl/h (Imperial Gallons per Hour)","132":"BTU","133":"BTU/h","134":"Liter","137":"L/h (Liters per Hour)","140":"PA(gauge)","155":"PA(absolute)","169":"Therm"}},{"@id":"VersionType","@type":"rdfs:Class","rdfs:comment":"Version SHALL indicate a distinct identifier for each revision of an IdentifiedObject. If not specified, a default version of \"0\" (initial version) SHALL be assumed. Upon modification of any IdentifiedObject, the mRID SHALL remain the same, but the version SHALL be incremented. Servers MAY NOT modify objects that they did not create, unless they were notified of the change from the entity controlling the object's PEN.","rdfs:subClassOf":{"@id":"UInt16"}},{"@id":"MirrorMeterReading","@type":"rdfs:Class","rdfs:comment":"Mimic of MeterReading used for managing mirrors.","rdfs:subClassOf":{"@id":"MeterReadingBase"}},{"@id":"MirrorMeterReadingList","@type":"rdfs:Class","rdfs:comment":"A List of MirrorMeterReading instances.","rdfs:subClassOf":{"@id":"List"}},{"@id":"MeterReadingBase","@type":"rdfs:Class","rdfs:comment":"A container for associating ReadingType, Readings and ReadingSets.","rdfs:subClassOf":{"@id":"IdentifiedObject"}},{"@id":"MirrorReadingSet","@type":"rdfs:Class","rdfs:comment":"A set of Readings of the ReadingType indicated by the parent MeterReading.","rdfs:subClassOf":{"@id":"ReadingSetBase"}},{"@id":"MirrorUsagePoint","@type":"rdfs:Class","rdfs:comment":"A parallel to UsagePoint to support mirroring","rdfs:subClassOf":{"@id":"UsagePointBase"}},{"@id":"MirrorUsagePointList","@type":"rdfs:Class","rdfs:comment":"A List of MirrorUsagePoint instances.","rdfs:subClassOf":{"@id":"List"}},{"@id":"ReadingBase","@type":"rdfs:Class","rdfs:comment":"Specific value measured by a meter or other asset. ReadingBase is abstract, used to define the elements common to Reading and IntervalReading.","rdfs:subClassOf":{"@id":"Resource"}},{"@id":"ReadingSetBase","@type":"rdfs:Class","rdfs:comment":"A set of Readings of the ReadingType indicated by the parent MeterReading. ReadingBase is abstract, used to define the elements common to ReadingSet and IntervalBlock.","rdfs:subClassOf":{"@id":"IdentifiedObject"}},{"@id":"UsagePointBase","@type":"rdfs:Class","rdfs:comment":"Logical point on a network at which consumption or production is either physically measured (e.g. metered) or estimated (e.g. unmetered street lights). A container for associating ReadingType, Readings and ReadingSets.","rdfs:subClassOf":{"@id":"IdentifiedObject"}},{"@id":"SubscribableType","@type":"rdfs:Class","rdfs:comment":"The subscribable values.\n0 - Resource does not support subscriptions\n1 - Resource supports non-conditional subscriptions\n2 - Resource supports conditional subscriptions\n3 - Resource supports both conditional and non-conditional subscriptions\nAll other values reserved.","@enum":{"0":"Resource does not support subscriptions","1":"Resource supports non-conditional subscriptions","2":"Resource supports conditional subscriptions","3":"Resource supports both conditional and non-conditional subscriptions"}},{"@id":"HexBinary8","@type":"rdfs:Class","rdfs:comment":"An 8-bit field encoded as a hex string (2 hex characters). Where applicable, bit 0, or the least significant bit, goes on the right. Note that hexBinary requires pairs of hex characters, so an odd number of characters requires a leading \"0\"."},{"@id":"HexBinary16","@type":"rdfs:Class","rdfs:comment":"A 16-bit field encoded as a hex string (4 hex characters max). Where applicable, bit 0, or the least significant bit, goes on the right. Note that hexBinary requires pairs of hex characters, so an odd number of characters requires a leading \"0\"."},{"@id":"HexBinary32","@type":"rdfs:Class","rdfs:comment":"A 32-bit field encoded as a hex string (8 hex characters max). Where applicable, bit 0, or the least significant bit, goes on the right. Note that hexBinary requires pairs of hex characters, so an odd number of characters requires a leading \"0\"."},{"@id":"HexBinary48","@type":"rdfs:Class","rdfs:comment":"A 48-bit field encoded as a hex string (12 hex characters max). Where applicable, bit 0, or the least significant bit, goes on the right. Note that hexBinary requires pairs of hex characters, so an odd number of characters requires a leading \"0\"."},{"@id":"HexBinary64","@type":"rdfs:Class","rdfs:comment":"A 64-bit field encoded as a hex string (16 hex characters max). Where applicable, bit 0, or the least significant bit, goes on the right. Note that hexBinary requires pairs of hex characters, so an odd number of characters requires a leading \"0\"."},{"@id":"HexBinary128","@type":"rdfs:Class","rdfs:comment":"A 128-bit field encoded as a hex string (32 hex characters max). Where applicable, bit 0, or the least significant bit, goes on the right. Note that hexBinary requires pairs of hex characters, so an odd number of characters requires a leading \"0\"."},{"@id":"HexBinary160","@type":"rdfs:Class","rdfs:comment":"A 160-bit field encoded as a hex string (40 hex characters max). Where applicable, bit 0, or the least significant bit, goes on the right. Note that hexBinary requires pairs of hex characters, so an odd number of characters requires a leading \"0\"."},{"@id":"String6","@type":"rdfs:Class","rdfs:comment":"Character string of max length 6. In order to limit internal storage, implementations SHALL reduce the length of strings using multi-byte characters so that the string may be stored using \"maxLength\" octets in the given encoding."},{"@id":"String16","@type":"rdfs:Class","rdfs:comment":"Character string of max length 16. In order to limit internal storage, implementations SHALL reduce the length of strings using multi-byte characters so that the string may be stored using \"maxLength\" octets in the given encoding."},{"@id":"String20","@type":"rdfs:Class","rdfs:comment":"Character string of max length 20. In order to limit internal storage, implementations SHALL reduce the length of strings using multi-byte characters so that the string may be stored using \"maxLength\" octets in the given encoding."},{"@id":"String32","@type":"rdfs:Class","rdfs:comment":"Character string of max length 32. In order to limit internal storage, implementations SHALL reduce the length of strings using multi-byte characters so that the string may be stored using \"maxLength\" octets in the given encoding."},{"@id":"String42","@type":"rdfs:Class","rdfs:comment":"Character string of max length 42. In order to limit internal storage, implementations SHALL reduce the length of strings using multi-byte characters so that the string may be stored using \"maxLength\" octets in the given encoding."},{"@id":"String192","@type":"rdfs:Class","rdfs:comment":"Character string of max length 192. For all string types, in order to limit internal storage, implementations SHALL reduce the length of strings using multi-byte characters so that the string may be stored using \"maxLength\" octets in the given encoding."},{"@id":"UInt8","@type":"rdfs:Class","rdfs:comment":"Unsigned integer, max inclusive 255 (2^8-1)"},{"@id":"UInt16","@type":"rdfs:Class","rdfs:comment":"Unsigned integer, max inclusive 65535 (2^16-1)"},{"@id":"UInt32","@type":"rdfs:Class","rdfs:comment":"Unsigned integer, max inclusive 4294967295 (2^32-1)"},{"@id":"UInt40","@type":"rdfs:Class","rdfs:comment":"Unsigned integer, max inclusive 1099511627775 (2^40-1)"},{"@id":"UInt48","@type":"rdfs:Class","rdfs:comment":"Unsigned integer, max inclusive 281474976710655 (2^48-1)"},{"@id":"UInt64","@type":"rdfs:Class","rdfs:comment":"Unsigned integer, max inclusive 18446744073709551615 (2^64-1)"},{"@id":"Int8","@type":"rdfs:Class","rdfs:comment":"Signed integer, min -128 max +127"},{"@id":"Int16","@type":"rdfs:Class","rdfs:comment":"Signed integer, min -32768 max +32767"},{"@id":"Int32","@type":"rdfs:Class","rdfs:comment":"Signed integer, max inclusive 2147483647 (2^31), min inclusive -2147483647 (same as xs:int)"},{"@id":"Int48","@type":"rdfs:Class","rdfs:comment":"Signed integer, max inclusive 140737488355328 (2^47), min inclusive -140737488355328"},{"@id":"Int64","@type":"rdfs:Class","rdfs:comment":"Signed integer, max inclusive 9223372036854775807 (2^63), min inclusive -9223372036854775808 (same as xs:long)"},{"@id":"EndDeviceListLink","@type":"rdf:Property","rdfs:domain":{"@id":"DeviceCapability"},"rdfs:range":{"@id":"EndDeviceListLink"},"owl:minCardinality":0},{"@id":"MirrorUsagePointListLink","@type":"rdf:Property","rdfs:domain":{"@id":"DeviceCapability"},"rdfs:range":{"@id":"MirrorUsagePointListLink"},"owl:minCardinality":0},{"@id":"SelfDeviceLink","@type":"rdf:Property","rdfs:domain":{"@id":"DeviceCapability"},"rdfs:range":{"@id":"SelfDeviceLink"},"owl:minCardinality":0},{"@id":"pollRate","@type":"rdf:Property","rdfs:domain":{"@id":"DeviceCapability"},"rdfs:range":{"@id":"UInt32"},"rdfs:comment":"The default polling rate for this function set (this resource and all resources below), in seconds. If not specified, a default of 900 seconds (15 minutes) is used. It is RECOMMENDED a client poll the resources of this function set every pollRate seconds.","owl:minCardinality":0},{"@id":"ConfigurationLink","@type":"rdf:Property","rdfs:domain":{"@id":"AbstractDevice"},"rdfs:range":{"@id":"ConfigurationLink"},"owl:minCardinality":0},{"@id":"DERListLink","@type":"rdf:Property","rdfs:domain":{"@id":"AbstractDevice"},"rdfs:range":{"@id":"DERListLink"},"owl:minCardinality":0},{"@id":"deviceCategory","@type":"rdf:Property","rdfs:domain":{"@id":"AbstractDevice"},"rdfs:range":{"@id":"DeviceCategoryType"},"rdfs:comment":"This field is for use in devices that can adjust energy usage (e.g., demand response, distributed energy resources).  For devices that do not respond to EndDeviceControls or DERControls (for instance, an ESI), this field should not have any bits set.","owl:minCardinality":0},{"@id":"DeviceInformationLink","@type":"rdf:Property","rdfs:domain":{"@id":"AbstractDevice"},"rdfs:range":{"@id":"DeviceInformationLink"},"owl:minCardinality":0},{"@id":"DeviceStatusLink","@type":"rdf:Property","rdfs:domain":{"@id":"AbstractDevice"},"rdfs:range":{"@id":"DeviceStatusLink"},"owl:minCardinality":0},{"@id":"FileStatusLink","@type":"rdf:Property","rdfs:domain":{"@id":"AbstractDevice"},"rdfs:range":{"@id":"FileStatusLink"},"owl:minCardinality":0},{"@id":"IPInterfaceListLink","@type":"rdf:Property","rdfs:domain":{"@id":"AbstractDevice"},"rdfs:range":{"@id":"IPInterfaceListLink"},"owl:minCardinality":0},{"@id":"lFDI","@type":"rdf:Property","rdfs:domain":{"@id":"AbstractDevice"},"rdfs:range":{"@id":"HexBinary160"},"rdfs:comment":"Long form of device identifier. See the Security section for additional details.","owl:minCardinality":0},{"@id":"LoadShedAvailabilityListLink","@type":"rdf:Property","rdfs:domain":{"@id":"AbstractDevice"},"rdfs:range":{"@id":"LoadShedAvailabilityListLink"},"owl:minCardinality":0},{"@id":"LogEventListLink","@type":"rdf:Property","rdfs:domain":{"@id":"AbstractDevice"},"rdfs:range":{"@id":"LogEventListLink"},"owl:minCardinality":0},{"@id":"PowerStatusLink","@type":"rdf:Property","rdfs:domain":{"@id":"AbstractDevice"},"rdfs:range":{"@id":"PowerStatusLink"},"owl:minCardinality":0},{"@id":"sFDI","@type":"rdf:Property","rdfs:domain":{"@id":"AbstractDevice"},"rdfs:range":{"@id":"SFDIType"},"rdfs:comment":"Short form of device identifier, WITH the checksum digit. See the Security section for additional details."},{"@id":"changedTime","@type":"rdf:Property","rdfs:domain":{"@id":"DeviceStatus"},"rdfs:range":{"@id":"TimeType"},"rdfs:comment":"The time at which the reported values were recorded."},{"@id":"onCount","@type":"rdf:Property","rdfs:domain":{"@id":"DeviceStatus"},"rdfs:range":{"@id":"UInt16"},"rdfs:comment":"The number of times that the device has been turned on: Count of \"device on\" times, since the last time the counter was reset","owl:minCardinality":0},{"@id":"opState","@type":"rdf:Property","rdfs:domain":{"@id":"DeviceStatus"},"rdfs:range":{"@id":"UInt8"},"rdfs:comment":"Device operational state: \n0 - Not applicable / Unknown\n1 - Not operating\n2 - Operating\n3 - Starting up\n4 - Shutting down\n5 - At disconnect level\n6 - kW ramping\n7 - kVar ramping","owl:minCardinality":0},{"@id":"opTime","@type":"rdf:Property","rdfs:domain":{"@id":"DeviceStatus"},"rdfs:range":{"@id":"UInt32"},"rdfs:comment":"Total time device has operated: re-settable: Accumulated time in seconds since the last time the counter was reset.","owl:minCardinality":0},{"@id":"Temperature","@type":"rdf:Property","rdfs:domain":{"@id":"DeviceStatus"},"rdfs:range":{"@id":"Temperature"},"owl:minCardinality":0},{"@id":"TimeLink","@type":"rdf:Property","rdfs:domain":{"@id":"DeviceStatus"},"rdfs:range":{"@id":"TimeLink"},"owl:minCardinality":0},{"@id":"pollRate","@type":"rdf:Property","rdfs:domain":{"@id":"DeviceStatus"},"rdfs:range":{"@id":"UInt32"},"rdfs:comment":"The default polling rate for this function set (this resource and all resources below), in seconds. If not specified, a default of 900 seconds (15 minutes) is used. It is RECOMMENDED a client poll the resources of this function set every pollRate seconds.","owl:minCardinality":0},{"@id":"changedTime","@type":"rdf:Property","rdfs:domain":{"@id":"EndDevice"},"rdfs:range":{"@id":"TimeType"},"rdfs:comment":"The time at which this resource was last modified or created."},{"@id":"enabled","@type":"rdf:Property","rdfs:domain":{"@id":"EndDevice"},"rdfs:range":"xsd:boolean","rdfs:comment":"This attribute indicates whether or not an EndDevice is enabled, or registered, on the server. If a server sets this attribute to false, the device is no longer registered. It should be noted that servers can delete EndDevice instances, but using this attribute for some time is more convenient for clients.","owl:minCardinality":0},{"@id":"FlowReservationRequestListLink","@type":"rdf:Property","rdfs:domain":{"@id":"EndDevice"},"rdfs:range":{"@id":"FlowReservationRequestListLink"},"owl:minCardinality":0},{"@id":"FlowReservationResponseListLink","@type":"rdf:Property","rdfs:domain":{"@id":"EndDevice"},"rdfs:range":{"@id":"FlowReservationResponseListLink"},"owl:minCardinality":0},{"@id":"FunctionSetAssignmentsListLink","@type":"rdf:Property","rdfs:domain":{"@id":"EndDevice"},"rdfs:range":{"@id":"FunctionSetAssignmentsListLink"},"owl:minCardinality":0},{"@id":"postRate","@type":"rdf:Property","rdfs:domain":{"@id":"EndDevice"},"rdfs:range":{"@id":"UInt32"},"rdfs:comment":"POST rate, or how often EndDevice and subordinate resources should be POSTed, in seconds. A client MAY indicate a preferred postRate when POSTing EndDevice. A server MAY add or modify postRate to indicate its preferred posting rate.","owl:minCardinality":0},{"@id":"RegistrationLink","@type":"rdf:Property","rdfs:domain":{"@id":"EndDevice"},"rdfs:range":{"@id":"RegistrationLink"},"owl:minCardinality":0},{"@id":"SubscriptionListLink","@type":"rdf:Property","rdfs:domain":{"@id":"EndDevice"},"rdfs:range":{"@id":"SubscriptionListLink"},"owl:minCardinality":0},{"@id":"EndDevice","@type":"rdf:Property","rdfs:domain":{"@id":"EndDeviceList"},"rdfs:range":{"@id":"EndDevice"},"owl:minCardinality":0},{"@id":"pollRate","@type":"rdf:Property","rdfs:domain":{"@id":"EndDeviceList"},"rdfs:range":{"@id":"UInt32"},"rdfs:comment":"The default polling rate for this function set (this resource and all resources below), in seconds. If not specified, a default of 900 seconds (15 minutes) is used. It is RECOMMENDED a client poll the resources of this function set every pollRate seconds.","owl:minCardinality":0},{"@id":"dateTimeRegistered","@type":"rdf:Property","rdfs:domain":{"@id":"Registration"},"rdfs:range":{"@id":"TimeType"},"rdfs:comment":"Contains the time at which this registration was created, by which clients MAY prioritize information providers with the most recent registrations, when no additional direction from the consumer is available."},{"@id":"pIN","@type":"rdf:Property","rdfs:domain":{"@id":"Registration"},"rdfs:range":{"@id":"PINType"},"rdfs:comment":"Contains the registration PIN number associated with the device, including the checksum digit."},{"@id":"pollRate","@type":"rdf:Property","rdfs:domain":{"@id":"Registration"},"rdfs:range":{"@id":"UInt32"},"rdfs:comment":"The default polling rate for this function set (this resource and all resources below), in seconds. If not specified, a default of 900 seconds (15 minutes) is used. It is RECOMMENDED a client poll the resources of this function set every pollRate seconds.","owl:minCardinality":0},{"@id":"pollRate","@type":"rdf:Property","rdfs:domain":{"@id":"SelfDevice"},"rdfs:range":{"@id":"UInt32"},"rdfs:comment":"The default polling rate for this function set (this resource and all resources below), in seconds. If not specified, a default of 900 seconds (15 minutes) is used. It is RECOMMENDED a client poll the resources of this function set every pollRate seconds.","owl:minCardinality":0},{"@id":"multiplier","@type":"rdf:Property","rdfs:domain":{"@id":"Temperature"},"rdfs:range":{"@id":"PowerOfTenMultiplierType"},"rdfs:comment":"Multiplier for 'unit'."},{"@id":"subject","@type":"rdf:Property","rdfs:domain":{"@id":"Temperature"},"rdfs:range":{"@id":"UInt8"},"rdfs:comment":"The subject of the temperature measurement\n0 - Enclosure\n1 - Transformer\n2 - HeatSink"},{"@id":"value","@type":"rdf:Property","rdfs:domain":{"@id":"Temperature"},"rdfs:range":{"@id":"Int16"},"rdfs:comment":"Value in Degrees Celsius (uom 23)."},{"@id":"CustomerAccountListLink","@type":"rdf:Property","rdfs:domain":{"@id":"FunctionSetAssignmentsBase"},"rdfs:range":{"@id":"CustomerAccountListLink"},"owl:minCardinality":0},{"@id":"DemandResponseProgramListLink","@type":"rdf:Property","rdfs:domain":{"@id":"FunctionSetAssignmentsBase"},"rdfs:range":{"@id":"DemandResponseProgramListLink"},"owl:minCardinality":0},{"@id":"DERProgramListLink","@type":"rdf:Property","rdfs:domain":{"@id":"FunctionSetAssignmentsBase"},"rdfs:range":{"@id":"DERProgramListLink"},"owl:minCardinality":0},{"@id":"FileListLink","@type":"rdf:Property","rdfs:domain":{"@id":"FunctionSetAssignmentsBase"},"rdfs:range":{"@id":"FileListLink"},"owl:minCardinality":0},{"@id":"MessagingProgramListLink","@type":"rdf:Property","rdfs:domain":{"@id":"FunctionSetAssignmentsBase"},"rdfs:range":{"@id":"MessagingProgramListLink"},"owl:minCardinality":0},{"@id":"PrepaymentListLink","@type":"rdf:Property","rdfs:domain":{"@id":"FunctionSetAssignmentsBase"},"rdfs:range":{"@id":"PrepaymentListLink"},"owl:minCardinality":0},{"@id":"ResponseSetListLink","@type":"rdf:Property","rdfs:domain":{"@id":"FunctionSetAssignmentsBase"},"rdfs:range":{"@id":"ResponseSetListLink"},"owl:minCardinality":0},{"@id":"TariffProfileListLink","@type":"rdf:Property","rdfs:domain":{"@id":"FunctionSetAssignmentsBase"},"rdfs:range":{"@id":"TariffProfileListLink"},"owl:minCardinality":0},{"@id":"TimeLink","@type":"rdf:Property","rdfs:domain":{"@id":"FunctionSetAssignmentsBase"},"rdfs:range":{"@id":"TimeLink"},"owl:minCardinality":0},{"@id":"UsagePointListLink","@type":"rdf:Property","rdfs:domain":{"@id":"FunctionSetAssignmentsBase"},"rdfs:range":{"@id":"UsagePointListLink"},"owl:minCardinality":0},{"@id":"mRID","@type":"rdf:Property","rdfs:domain":{"@id":"FunctionSetAssignments"},"rdfs:range":{"@id":"mRIDType"},"rdfs:comment":"The global identifier of the object."},{"@id":"description","@type":"rdf:Property","rdfs:domain":{"@id":"FunctionSetAssignments"},"rdfs:range":{"@id":"String32"},"rdfs:comment":"The description is a human readable text describing or naming the object.","owl:minCardinality":0},{"@id":"version","@type":"rdf:Property","rdfs:domain":{"@id":"FunctionSetAssignments"},"rdfs:range":{"@id":"VersionType"},"rdfs:comment":"Contains the version number of the object. See the type definition for details.","owl:minCardinality":0},{"@id":"subscribable","@type":"rdf:Property","rdfs:domain":{"@id":"FunctionSetAssignments"},"rdfs:range":{"@id":"SubscribableType"},"rdfs:comment":"Indicates whether or not subscriptions are supported for this resource, and whether or not conditional (thresholds) are supported. If not specified, is \"not subscribable\" (0).","owl:minCardinality":0},{"@id":"FunctionSetAssignments","@type":"rdf:Property","rdfs:domain":{"@id":"FunctionSetAssignmentsList"},"rdfs:range":{"@id":"FunctionSetAssignments"},"owl:minCardinality":0},{"@id":"pollRate","@type":"rdf:Property","rdfs:domain":{"@id":"FunctionSetAssignmentsList"},"rdfs:range":{"@id":"UInt32"},"rdfs:comment":"The default polling rate for this function set (this resource and all resources below), in seconds. If not specified, a default of 900 seconds (15 minutes) is used. It is RECOMMENDED a client poll the resources of this function set every pollRate seconds.","owl:minCardinality":0},{"@id":"attributeIdentifier","@type":"rdf:Property","rdfs:domain":{"@id":"Condition"},"rdfs:range":{"@id":"UInt8"},"rdfs:comment":"0 = Reading value\n1-255 = Reserved"},{"@id":"lowerThreshold","@type":"rdf:Property","rdfs:domain":{"@id":"Condition"},"rdfs:range":{"@id":"Int48"},"rdfs:comment":"The value of the lower threshold"},{"@id":"upperThreshold","@type":"rdf:Property","rdfs:domain":{"@id":"Condition"},"rdfs:range":{"@id":"Int48"},"rdfs:comment":"The value of the upper threshold"},{"@id":"subscribedResource","@type":"rdf:Property","rdfs:domain":{"@id":"SubscriptionBase"},"rdfs:range":"xsd:anyURI","rdfs:comment":"The resource for which the subscription applies. Query string parameters SHALL NOT be specified when subscribing to list resources.  Should a query string parameter be specified, servers SHALL ignore them."},{"@id":"Condition","@type":"rdf:Property","rdfs:domain":{"@id":"Subscription"},"rdfs:range":{"@id":"Condition"},"owl:minCardinality":0},{"@id":"encoding","@type":"rdf:Property","rdfs:domain":{"@id":"Subscription"},"rdfs:range":{"@id":"UInt8"},"rdfs:comment":"0 - application/sep+xml\n1 - application/sep-exi\n2-255 - reserved"},{"@id":"level","@type":"rdf:Property","rdfs:domain":{"@id":"Subscription"},"rdfs:range":{"@id":"String16"},"rdfs:comment":"Contains the preferred schema and extensibility level indication such as \"+S1\""},{"@id":"limit","@type":"rdf:Property","rdfs:domain":{"@id":"Subscription"},"rdfs:range":{"@id":"UInt32"},"rdfs:comment":"This element is used to indicate the maximum number of list items that should be included in a notification when the subscribed resource changes. This limit is meant to be functionally equivalent to the \u2018limit\u2019 query string parameter, but applies to both list resources as well as other resources.  For list resources, if a limit of \u20180\u2019 is specified, then notifications SHALL contain a list resource with results=\u20190\u2019 (equivalent to a simple change notification).  For list resources, if a limit greater than \u20180\u2019 is specified, then notifications SHALL contain a list resource with results equal to the limit specified (or less, should the list contain fewer items than the limit specified or should the server be unable to provide the requested number of items for any reason) and follow the same rules for list resources (e.g., ordering).  For non-list resources, if a limit of \u20180\u2019 is specified, then notifications SHALL NOT contain a resource representation (equivalent to a simple change notification).  For non-list resources, if a limit greater than \u20180\u2019 is specified, then notifications SHALL contain the representation of the changed resource."},{"@id":"notificationURI","@type":"rdf:Property","rdfs:domain":{"@id":"Subscription"},"rdfs:range":"xsd:anyURI","rdfs:comment":"The resource to which to post the notifications about the requested subscribed resource. Because this URI will exist on a server other than the one being POSTed to, this attribute SHALL be a fully-qualified absolute URI, not a relative reference."},{"@id":"Subscription","@type":"rdf:Property","rdfs:domain":{"@id":"SubscriptionList"},"rdfs:range":{"@id":"Subscription"},"owl:minCardinality":0},{"@id":"pollRate","@type":"rdf:Property","rdfs:domain":{"@id":"SubscriptionList"},"rdfs:range":{"@id":"UInt32"},"rdfs:comment":"The default polling rate for this function set (this resource and all resources below), in seconds. If not specified, a default of 900 seconds (15 minutes) is used. It is RECOMMENDED a client poll the resources of this function set every pollRate seconds.","owl:minCardinality":0},{"@id":"newResourceURI","@type":"rdf:Property","rdfs:domain":{"@id":"Notification"},"rdfs:range":"xsd:anyURI","rdfs:comment":"The new location of the resource, if moved. This attribute SHALL be a fully-qualified absolute URI, not a relative reference.","owl:minCardinality":0},{"@id":"Resource","@type":"rdf:Property","rdfs:domain":{"@id":"Notification"},"rdfs:range":{"@id":"Resource"},"owl:minCardinality":0},{"@id":"status","@type":"rdf:Property","rdfs:domain":{"@id":"Notification"},"rdfs:range":{"@id":"UInt8"},"rdfs:comment":"0 = Default Status\n1 = Subscription canceled, no additional information\n2 = Subscription canceled, resource moved\n3 = Subscription canceled, resource definition changed (e.g., a new version of IEEE 2030.5)\n4 = Subscription canceled, resource deleted\nAll other values reserved."},{"@id":"subscriptionURI","@type":"rdf:Property","rdfs:domain":{"@id":"Notification"},"rdfs:range":"xsd:anyURI","rdfs:comment":"The subscription from which this notification was triggered. This attribute SHALL be a fully-qualified absolute URI, not a relative reference."},{"@id":"Notification","@type":"rdf:Property","rdfs:domain":{"@id":"NotificationList"},"rdfs:range":{"@id":"Notification"},"owl:minCardinality":0},{"@id":"type","@type":"rdf:Property","rdfs:domain":{"@id":"AppliedTargetReduction"},"rdfs:range":{"@id":"UnitType"},"rdfs:comment":"Enumerated field representing the type of reduction requested."},{"@id":"value","@type":"rdf:Property","rdfs:domain":{"@id":"AppliedTargetReduction"},"rdfs:range":{"@id":"UInt16"},"rdfs:comment":"Indicates the requested amount of the relevant commodity to be reduced."},{"@id":"ApplianceLoadReduction","@type":"rdf:Property","rdfs:domain":{"@id":"DrResponse"},"rdfs:range":{"@id":"ApplianceLoadReduction"},"owl:minCardinality":0},{"@id":"AppliedTargetReduction","@type":"rdf:Property","rdfs:domain":{"@id":"DrResponse"},"rdfs:range":{"@id":"AppliedTargetReduction"},"owl:minCardinality":0},{"@id":"DutyCycle","@type":"rdf:Property","rdfs:domain":{"@id":"DrResponse"},"rdfs:range":{"@id":"DutyCycle"},"owl:minCardinality":0},{"@id":"Offset","@type":"rdf:Property","rdfs:domain":{"@id":"DrResponse"},"rdfs:range":{"@id":"Offset"},"owl:minCardinality":0},{"@id":"overrideDuration","@type":"rdf:Property","rdfs:domain":{"@id":"DrResponse"},"rdfs:range":{"@id":"UInt16"},"rdfs:comment":"Indicates the amount of time, in seconds, that the client partially opts-out during the demand response event. When overriding within the allowed override duration, the client SHALL send a partial opt-out (Response status code 8) for partial opt-out upon completion, with the total time the event was overridden (this attribute) populated. The client SHALL send a no participation status response (status type 10) if the user partially opts-out for longer than EndDeviceControl.overrideDuration.","owl:minCardinality":0},{"@id":"SetPoint","@type":"rdf:Property","rdfs:domain":{"@id":"DrResponse"},"rdfs:range":{"@id":"SetPoint"},"owl:minCardinality":0},{"@id":"createdDateTime","@type":"rdf:Property","rdfs:domain":{"@id":"Response"},"rdfs:range":{"@id":"TimeType"},"rdfs:comment":"The createdDateTime field contains the date and time when the acknowledgement/status occurred in the client. The client will provide the timestamp to ensure the proper time is captured in case the response is delayed in reaching the server (server receipt time would not be the same as the actual confirmation time). The time reported from the client should be relative to the time server indicated by the FunctionSetAssignment that also indicated the event resource; if no FunctionSetAssignment exists, the time of the server where the event resource was hosted.","owl:minCardinality":0},{"@id":"endDeviceLFDI","@type":"rdf:Property","rdfs:domain":{"@id":"Response"},"rdfs:range":{"@id":"HexBinary160"},"rdfs:comment":"Contains the LFDI of the device providing the response."},{"@id":"status","@type":"rdf:Property","rdfs:domain":{"@id":"Response"},"rdfs:range":{"@id":"UInt8"},"rdfs:comment":"The status field contains the acknowledgement or status. Each event type (DRLC, DER, Price, or Text) can return different status information (e.g. an Acknowledge will be returned for a Price event where a DRLC event can return Event Received, Event Started, and Event Completed). The Status field value definitions are defined in Table 27: Response Types by Function Set.","owl:minCardinality":0},{"@id":"subject","@type":"rdf:Property","rdfs:domain":{"@id":"Response"},"rdfs:range":{"@id":"mRIDType"},"rdfs:comment":"The subject field provides a method to match the response with the originating event. It is populated with the mRID of the original object."},{"@id":"Response","@type":"rdf:Property","rdfs:domain":{"@id":"ResponseList"},"rdfs:range":{"@id":"Response"},"owl:minCardinality":0},{"@id":"ResponseListLink","@type":"rdf:Property","rdfs:domain":{"@id":"ResponseSet"},"rdfs:range":{"@id":"ResponseListLink"},"owl:minCardinality":0},{"@id":"ResponseSet","@type":"rdf:Property","rdfs:domain":{"@id":"ResponseSetList"},"rdfs:range":{"@id":"ResponseSet"},"owl:minCardinality":0},{"@id":"pollRate","@type":"rdf:Property","rdfs:domain":{"@id":"ResponseSetList"},"rdfs:range":{"@id":"UInt32"},"rdfs:comment":"The default polling rate for this function set (this resource and all resources below), in seconds. If not specified, a default of 900 seconds (15 minutes) is used. It is RECOMMENDED a client poll the resources of this function set every pollRate seconds.","owl:minCardinality":0},{"@id":"currentTime","@type":"rdf:Property","rdfs:domain":{"@id":"Time"},"rdfs:range":{"@id":"TimeType"},"rdfs:comment":"The current time, in the format defined by TimeType."},{"@id":"dstEndTime","@type":"rdf:Property","rdfs:domain":{"@id":"Time"},"rdfs:range":{"@id":"TimeType"},"rdfs:comment":"Time at which daylight savings ends (dstOffset no longer applied).  Result of dstEndRule calculation."},{"@id":"dstOffset","@type":"rdf:Property","rdfs:domain":{"@id":"Time"},"rdfs:range":{"@id":"TimeOffsetType"},"rdfs:comment":"Daylight savings time offset from local standard time. A typical practice is advancing clocks one hour when daylight savings time is in effect, which would result in a positive dstOffset."},{"@id":"dstStartTime","@type":"rdf:Property","rdfs:domain":{"@id":"Time"},"rdfs:range":{"@id":"TimeType"},"rdfs:comment":"Time at which daylight savings begins (apply dstOffset).  Result of dstStartRule calculation."},{"@id":"localTime","@type":"rdf:Property","rdfs:domain":{"@id":"Time"},"rdfs:range":{"@id":"TimeType"},"rdfs:comment":"Local time: localTime = currentTime + tzOffset (+ dstOffset when in effect).","owl:minCardinality":0},{"@id":"quality","@type":"rdf:Property","rdfs:domain":{"@id":"Time"},"rdfs:range":{"@id":"UInt8"},"rdfs:comment":"Metric indicating the quality of the time source from which the service acquired time. Lower (smaller) quality enumeration values are assumed to be more accurate.\n3 - time obtained from external authoritative source such as NTP\n4 - time obtained from level 3 source\n5 - time manually set or obtained from level 4 source\n6 - time obtained from level 5 source\n7 - time intentionally uncoordinated\nAll other values are reserved for future use."},{"@id":"tzOffset","@type":"rdf:Property","rdfs:domain":{"@id":"Time"},"rdfs:range":{"@id":"TimeOffsetType"},"rdfs:comment":"Local time zone offset from currentTime. Does not include any daylight savings time offsets. For American time zones, a negative tzOffset SHALL be used (eg, EST = GMT-5 which is -18000)."},{"@id":"pollRate","@type":"rdf:Property","rdfs:domain":{"@id":"Time"},"rdfs:range":{"@id":"UInt32"},"rdfs:comment":"The default polling rate for this function set (this resource and all resources below), in seconds. If not specified, a default of 900 seconds (15 minutes) is used. It is RECOMMENDED a client poll the resources of this function set every pollRate seconds.","owl:minCardinality":0},{"@id":"DRLCCapabilities","@type":"rdf:Property","rdfs:domain":{"@id":"DeviceInformation"},"rdfs:range":{"@id":"DRLCCapabilities"},"owl:minCardinality":0},{"@id":"functionsImplemented","@type":"rdf:Property","rdfs:domain":{"@id":"DeviceInformation"},"rdfs:range":{"@id":"HexBinary64"},"rdfs:comment":"Bitmap indicating the function sets used by the device as a client.\n0 - Device Capability\n1 - Self Device Resource\n2 - End Device Resource\n3 - Function Set Assignments\n4 - Subscription/Notification Mechanism\n5 - Response\n6 - Time\n7 - Device Information\n8 - Power Status\n9 - Network Status\n10 - Log Event\n11 - Configuration Resource\n12 - Software Download\n13 - DRLC\n14 - Metering\n15 - Pricing\n16 - Messaging\n17 - Billing\n18 - Prepayment\n19 - Flow Reservation\n20 - DER Control","owl:minCardinality":0},{"@id":"gpsLocation","@type":"rdf:Property","rdfs:domain":{"@id":"DeviceInformation"},"rdfs:range":{"@id":"GPSLocationType"},"rdfs:comment":"GPS location of this device.","owl:minCardinality":0},{"@id":"lFDI","@type":"rdf:Property","rdfs:domain":{"@id":"DeviceInformation"},"rdfs:range":{"@id":"HexBinary160"},"rdfs:comment":"Long form device identifier. See the Security section for full details."},{"@id":"mfDate","@type":"rdf:Property","rdfs:domain":{"@id":"DeviceInformation"},"rdfs:range":{"@id":"TimeType"},"rdfs:comment":"Date/time of manufacture"},{"@id":"mfHwVer","@type":"rdf:Property","rdfs:domain":{"@id":"DeviceInformation"},"rdfs:range":{"@id":"String32"},"rdfs:comment":"Manufacturer hardware version"},{"@id":"mfID","@type":"rdf:Property","rdfs:domain":{"@id":"DeviceInformation"},"rdfs:range":{"@id":"PENType"},"rdfs:comment":"The manufacturer's IANA Enterprise Number."},{"@id":"mfInfo","@type":"rdf:Property","rdfs:domain":{"@id":"DeviceInformation"},"rdfs:range":{"@id":"String32"},"rdfs:comment":"Manufacturer dependent information related to the manufacture of this device","owl:minCardinality":0},{"@id":"mfModel","@type":"rdf:Property","rdfs:domain":{"@id":"DeviceInformation"},"rdfs:range":{"@id":"String32"},"rdfs:comment":"Manufacturer's model number"},{"@id":"mfSerNum","@type":"rdf:Property","rdfs:domain":{"@id":"DeviceInformation"},"rdfs:range":{"@id":"String32"},"rdfs:comment":"Manufacturer assigned serial number"},{"@id":"primaryPower","@type":"rdf:Property","rdfs:domain":{"@id":"DeviceInformation"},"rdfs:range":{"@id":"PowerSourceType"},"rdfs:comment":"Primary source of power."},{"@id":"secondaryPower","@type":"rdf:Property","rdfs:domain":{"@id":"DeviceInformation"},"rdfs:range":{"@id":"PowerSourceType"},"rdfs:comment":"Secondary source of power"},{"@id":"SupportedLocaleListLink","@type":"rdf:Property","rdfs:domain":{"@id":"DeviceInformation"},"rdfs:range":{"@id":"SupportedLocaleListLink"},"owl:minCardinality":0},{"@id":"swActTime","@type":"rdf:Property","rdfs:domain":{"@id":"DeviceInformation"},"rdfs:range":{"@id":"TimeType"},"rdfs:comment":"Activation date/time of currently running software"},{"@id":"swVer","@type":"rdf:Property","rdfs:domain":{"@id":"DeviceInformation"},"rdfs:range":{"@id":"String32"},"rdfs:comment":"Currently running software version"},{"@id":"pollRate","@type":"rdf:Property","rdfs:domain":{"@id":"DeviceInformation"},"rdfs:range":{"@id":"UInt32"},"rdfs:comment":"The default polling rate for this function set (this resource and all resources below), in seconds. If not specified, a default of 900 seconds (15 minutes) is used. It is RECOMMENDED a client poll the resources of this function set every pollRate seconds.","owl:minCardinality":0},{"@id":"averageEnergy","@type":"rdf:Property","rdfs:domain":{"@id":"DRLCCapabilities"},"rdfs:range":{"@id":"RealEnergy"},"rdfs:comment":"The average hourly energy usage when in normal operating mode."},{"@id":"maxDemand","@type":"rdf:Property","rdfs:domain":{"@id":"DRLCCapabilities"},"rdfs:range":{"@id":"ActivePower"},"rdfs:comment":"The maximum demand rating of this end device."},{"@id":"optionsImplemented","@type":"rdf:Property","rdfs:domain":{"@id":"DRLCCapabilities"},"rdfs:range":{"@id":"HexBinary32"},"rdfs:comment":"Bitmap indicating the DRLC options implemented by the device.\n0 - Target reduction (kWh)\n1 - Target reduction (kW)\n2 - Target reduction (Watts)\n3 - Target reduction (Cubic Meters)\n4 - Target reduction (Cubic Feet)\n5 - Target reduction (US Gallons)\n6 - Target reduction (Imperial Gallons)\n7 - Target reduction (BTUs)\n8 - Target reduction (Liters)\n9 - Target reduction (kPA (gauge))\n10 - Target reduction (kPA (absolute))\n11 - Target reduction (Mega Joule)\n12 - Target reduction (Unitless)\n13-15 - Reserved\n16 - Temperature set point\n17 - Temperature offset\n18 - Duty cycle\n19 - Load adjustment percentage\n20 - Appliance load reduction\n21-31 - Reserved"},{"@id":"locale","@type":"rdf:Property","rdfs:domain":{"@id":"SupportedLocale"},"rdfs:range":{"@id":"LocaleType"},"rdfs:comment":"The code for a locale that is supported"},{"@id":"SupportedLocale","@type":"rdf:Property","rdfs:domain":{"@id":"SupportedLocaleList"},"rdfs:range":{"@id":"SupportedLocale"},"owl:minCardinality":0},{"@id":"batteryStatus","@type":"rdf:Property","rdfs:domain":{"@id":"PowerStatus"},"rdfs:range":{"@id":"UInt8"},"rdfs:comment":"Battery system status\n\n0 = unknown\n1 = normal (more than LowChargeThreshold remaining)\n2 = low (less than LowChargeThreshold remaining) \n3 = depleted (0% charge remaining)\n4 = not applicable (mains powered only)"},{"@id":"changedTime","@type":"rdf:Property","rdfs:domain":{"@id":"PowerStatus"},"rdfs:range":{"@id":"TimeType"},"rdfs:comment":"The time at which the reported values were recorded."},{"@id":"currentPowerSource","@type":"rdf:Property","rdfs:domain":{"@id":"PowerStatus"},"rdfs:range":{"@id":"PowerSourceType"},"rdfs:comment":"This value will be fixed for devices powered by a single source.  This value may change for devices able to transition between multiple power sources (mains to battery backup, etc.)."},{"@id":"estimatedChargeRemaining","@type":"rdf:Property","rdfs:domain":{"@id":"PowerStatus"},"rdfs:range":{"@id":"PerCent"},"rdfs:comment":"Estimate of remaining battery charge as a percent of full charge.","owl:minCardinality":0},{"@id":"estimatedTimeRemaining","@type":"rdf:Property","rdfs:domain":{"@id":"PowerStatus"},"rdfs:range":{"@id":"UInt32"},"rdfs:comment":"Estimated time (in seconds) to total battery charge depletion (under current load)","owl:minCardinality":0},{"@id":"PEVInfo","@type":"rdf:Property","rdfs:domain":{"@id":"PowerStatus"},"rdfs:range":{"@id":"PEVInfo"},"owl:minCardinality":0},{"@id":"sessionTimeOnBattery","@type":"rdf:Property","rdfs:domain":{"@id":"PowerStatus"},"rdfs:range":{"@id":"UInt32"},"rdfs:comment":"If the device has a battery, this is the time since the device last switched to battery power, or the time since the device was restarted, whichever is less, in seconds.","owl:minCardinality":0},{"@id":"totalTimeOnBattery","@type":"rdf:Property","rdfs:domain":{"@id":"PowerStatus"},"rdfs:range":{"@id":"UInt32"},"rdfs:comment":"If the device has a battery, this is the total time the device has been on battery power, in seconds. It may be reset when the battery is replaced.","owl:minCardinality":0},{"@id":"pollRate","@type":"rdf:Property","rdfs:domain":{"@id":"PowerStatus"},"rdfs:range":{"@id":"UInt32"},"rdfs:comment":"The default polling rate for this function set (this resource and all resources below), in seconds. If not specified, a default of 900 seconds (15 minutes) is used. It is RECOMMENDED a client poll the resources of this function set every pollRate seconds.","owl:minCardinality":0},{"@id":"chargingPowerNow","@type":"rdf:Property","rdfs:domain":{"@id":"PEVInfo"},"rdfs:range":{"@id":"ActivePower"},"rdfs:comment":"This is the actual power flow in or out of the charger or inverter. This is calculated by the vehicle based on actual measurements. This number is positive for charging."},{"@id":"energyRequestNow","@type":"rdf:Property","rdfs:domain":{"@id":"PEVInfo"},"rdfs:range":{"@id":"RealEnergy"},"rdfs:comment":"This is the amount of energy that must be transferred from the grid to EVSE and PEV to achieve the target state of charge allowing for charger efficiency and any vehicle and EVSE parasitic loads. This is calculated by the vehicle and changes throughout the connection as forward or reverse power flow change the battery state of charge.  This number is positive for charging."},{"@id":"maxForwardPower","@type":"rdf:Property","rdfs:domain":{"@id":"PEVInfo"},"rdfs:range":{"@id":"ActivePower"},"rdfs:comment":"This is maximum power transfer capability that could be used for charging the PEV to perform the requested energy transfer.  It is the lower of the vehicle or EVSE physical power limitations. It is not based on economic considerations. The vehicle may draw less power than this value based on its charging cycle. The vehicle defines this parameter. This number is positive for charging power flow."},{"@id":"minimumChargingDuration","@type":"rdf:Property","rdfs:domain":{"@id":"PEVInfo"},"rdfs:range":{"@id":"UInt32"},"rdfs:comment":"This is computed by the PEV based on the charging profile to complete the energy transfer if the maximum power is authorized.  The value will never be smaller than the ratio of the energy request to the power request because the charging profile may not allow the maximum power to be used throughout the transfer.   This is a critical parameter for determining whether any slack time exists in the charging cycle between the current time and the TCIN."},{"@id":"targetStateOfCharge","@type":"rdf:Property","rdfs:domain":{"@id":"PEVInfo"},"rdfs:range":{"@id":"PerCent"},"rdfs:comment":"This is the target state of charge that is to be achieved during charging before the time of departure (TCIN).  The default value is 100%. The value cannot be set to a value less than the actual state of charge."},{"@id":"timeChargeIsNeeded","@type":"rdf:Property","rdfs:domain":{"@id":"PEVInfo"},"rdfs:range":{"@id":"TimeType"},"rdfs:comment":"Time Charge is Needed (TCIN) is the time that the PEV is expected to depart. The value is manually entered using controls and displays in the vehicle or on the EVSE or using a mobile device.  It is authenticated and saved by the PEV.  This value may be updated during a charging session."},{"@id":"timeChargingStatusPEV","@type":"rdf:Property","rdfs:domain":{"@id":"PEVInfo"},"rdfs:range":{"@id":"TimeType"},"rdfs:comment":"This is the time that the parameters are updated, except for changes to TCIN."},{"@id":"capabilityInfo","@type":"rdf:Property","rdfs:domain":{"@id":"IEEE_802_15_4"},"rdfs:range":{"@id":"HexBinary8"},"rdfs:comment":"As defined by IEEE 802.15.4"},{"@id":"NeighborListLink","@type":"rdf:Property","rdfs:domain":{"@id":"IEEE_802_15_4"},"rdfs:range":{"@id":"NeighborListLink"},"owl:minCardinality":0},{"@id":"shortAddress","@type":"rdf:Property","rdfs:domain":{"@id":"IEEE_802_15_4"},"rdfs:range":{"@id":"UInt16"},"rdfs:comment":"As defined by IEEE 802.15.4"},{"@id":"address","@type":"rdf:Property","rdfs:domain":{"@id":"IPAddr"},"rdfs:range":{"@id":"HexBinary128"},"rdfs:comment":"An IP address value."},{"@id":"RPLInstanceListLink","@type":"rdf:Property","rdfs:domain":{"@id":"IPAddr"},"rdfs:range":{"@id":"RPLInstanceListLink"},"owl:minCardinality":0},{"@id":"IPAddr","@type":"rdf:Property","rdfs:domain":{"@id":"IPAddrList"},"rdfs:range":{"@id":"IPAddr"},"owl:minCardinality":0},{"@id":"ifDescr","@type":"rdf:Property","rdfs:domain":{"@id":"IPInterface"},"rdfs:range":{"@id":"String192"},"rdfs:comment":"Use rules from [RFC 2863].","owl:minCardinality":0},{"@id":"ifHighSpeed","@type":"rdf:Property","rdfs:domain":{"@id":"IPInterface"},"rdfs:range":{"@id":"UInt32"},"rdfs:comment":"Use rules from [RFC 2863].","owl:minCardinality":0},{"@id":"ifInBroadcastPkts","@type":"rdf:Property","rdfs:domain":{"@id":"IPInterface"},"rdfs:range":{"@id":"UInt32"},"rdfs:comment":"Use rules from [RFC 2863].","owl:minCardinality":0},{"@id":"ifIndex","@type":"rdf:Property","rdfs:domain":{"@id":"IPInterface"},"rdfs:range":{"@id":"UInt32"},"rdfs:comment":"Use rules from [RFC 2863].","owl:minCardinality":0},{"@id":"ifInDiscards","@type":"rdf:Property","rdfs:domain":{"@id":"IPInterface"},"rdfs:range":{"@id":"UInt32"},"rdfs:comment":"Use rules from [RFC 2863]. Can be thought of as Input Datagrams Discarded.","owl:minCardinality":0},{"@id":"ifInErrors","@type":"rdf:Property","rdfs:domain":{"@id":"IPInterface"},"rdfs:range":{"@id":"UInt32"},"rdfs:comment":"Use rules from [RFC 2863].","owl:minCardinality":0},{"@id":"ifInMulticastPkts","@type":"rdf:Property","rdfs:domain":{"@id":"IPInterface"},"rdfs:range":{"@id":"UInt32"},"rdfs:comment":"Use rules from [RFC 2863]. Can be thought of as Multicast Datagrams Received.","owl:minCardinality":0},{"@id":"ifInOctets","@type":"rdf:Property","rdfs:domain":{"@id":"IPInterface"},"rdfs:range":{"@id":"UInt32"},"rdfs:comment":"Use rules from [RFC 2863]. Can be thought of as Bytes Received.","owl:minCardinality":0},{"@id":"ifInUcastPkts","@type":"rdf:Property","rdfs:domain":{"@id":"IPInterface"},"rdfs:range":{"@id":"UInt32"},"rdfs:comment":"Use rules from [RFC 2863]. Can be thought of as Datagrams Received.","owl:minCardinality":0},{"@id":"ifInUnknownProtos","@type":"rdf:Property","rdfs:domain":{"@id":"IPInterface"},"rdfs:range":{"@id":"UInt32"},"rdfs:comment":"Use rules from [RFC 2863]. Can be thought of as Datagrams with Unknown Protocol Received.","owl:minCardinality":0},{"@id":"ifMtu","@type":"rdf:Property","rdfs:domain":{"@id":"IPInterface"},"rdfs:range":{"@id":"UInt32"},"rdfs:comment":"Use rules from [RFC 2863].","owl:minCardinality":0},{"@id":"ifName","@type":"rdf:Property","rdfs:domain":{"@id":"IPInterface"},"rdfs:range":{"@id":"String16"},"rdfs:comment":"Use rules from [RFC 2863].","owl:minCardinality":0},{"@id":"ifOperStatus","@type":"rdf:Property","rdfs:domain":{"@id":"IPInterface"},"rdfs:range":{"@id":"UInt8"},"rdfs:comment":"Use rules and assignments from [RFC 2863].","owl:minCardinality":0},{"@id":"ifOutBroadcastPkts","@type":"rdf:Property","rdfs:domain":{"@id":"IPInterface"},"rdfs:range":{"@id":"UInt32"},"rdfs:comment":"Use rules from [RFC 2863]. Can be thought of as Broadcast Datagrams Sent.","owl:minCardinality":0},{"@id":"ifOutDiscards","@type":"rdf:Property","rdfs:domain":{"@id":"IPInterface"},"rdfs:range":{"@id":"UInt32"},"rdfs:comment":"Use rules from [RFC 2863]. Can be thought of as Output Datagrams Discarded.","owl:minCardinality":0},{"@id":"ifOutErrors","@type":"rdf:Property","rdfs:domain":{"@id":"IPInterface"},"rdfs:range":{"@id":"UInt32"},"rdfs:comment":"Use rules from [RFC 2863].","owl:minCardinality":0},{"@id":"ifOutMulticastPkts","@type":"rdf:Property","rdfs:domain":{"@id":"IPInterface"},"rdfs:range":{"@id":"UInt32"},"rdfs:comment":"Use rules from [RFC 2863]. Can be thought of as Multicast Datagrams Sent.","owl:minCardinality":0},{"@id":"ifOutOctets","@type":"rdf:Property","rdfs:domain":{"@id":"IPInterface"},"rdfs:range":{"@id":"UInt32"},"rdfs:comment":"Use rules from [RFC 2863]. Can be thought of as Bytes Sent.","owl:minCardinality":0},{"@id":"ifOutUcastPkts","@type":"rdf:Property","rdfs:domain":{"@id":"IPInterface"},"rdfs:range":{"@id":"UInt32"},"rdfs:comment":"Use rules from [RFC 2863]. Can be thought of as Datagrams Sent.","owl:minCardinality":0},{"@id":"ifPromiscuousMode","@type":"rdf:Property","rdfs:domain":{"@id":"IPInterface"},"rdfs:range":"xsd:boolean","rdfs:comment":"Use rules from [RFC 2863].","owl:minCardinality":0},{"@id":"ifSpeed","@type":"rdf:Property","rdfs:domain":{"@id":"IPInterface"},"rdfs:range":{"@id":"UInt32"},"rdfs:comment":"Use rules from [RFC 2863].","owl:minCardinality":0},{"@id":"ifType","@type":"rdf:Property","rdfs:domain":{"@id":"IPInterface"},"rdfs:range":{"@id":"UInt16"},"rdfs:comment":"Use rules and assignments from [RFC 2863].","owl:minCardinality":0},{"@id":"IPAddrListLink","@type":"rdf:Property","rdfs:domain":{"@id":"IPInterface"},"rdfs:range":{"@id":"IPAddrListLink"},"owl:minCardinality":0},{"@id":"lastResetTime","@type":"rdf:Property","rdfs:domain":{"@id":"IPInterface"},"rdfs:range":{"@id":"Int64"},"rdfs:comment":"Similar to ifLastChange in [RFC 2863].","owl:minCardinality":0},{"@id":"lastUpdatedTime","@type":"rdf:Property","rdfs:domain":{"@id":"IPInterface"},"rdfs:range":{"@id":"Int64"},"rdfs:comment":"The date/time of the reported status.","owl:minCardinality":0},{"@id":"LLInterfaceListLink","@type":"rdf:Property","rdfs:domain":{"@id":"IPInterface"},"rdfs:range":{"@id":"LLInterfaceListLink"},"owl:minCardinality":0},{"@id":"IPInterface","@type":"rdf:Property","rdfs:domain":{"@id":"IPInterfaceList"},"rdfs:range":{"@id":"IPInterface"},"owl:minCardinality":0},{"@id":"pollRate","@type":"rdf:Property","rdfs:domain":{"@id":"IPInterfaceList"},"rdfs:range":{"@id":"UInt32"},"rdfs:comment":"The default polling rate for this function set (this resource and all resources below), in seconds. If not specified, a default of 900 seconds (15 minutes) is used. It is RECOMMENDED a client poll the resources of this function set every pollRate seconds.","owl:minCardinality":0},{"@id":"CRCerrors","@type":"rdf:Property","rdfs:domain":{"@id":"LLInterface"},"rdfs:range":{"@id":"UInt32"},"rdfs:comment":"Contains the number of CRC errors since reset."},{"@id":"EUI64","@type":"rdf:Property","rdfs:domain":{"@id":"LLInterface"},"rdfs:range":{"@id":"HexBinary64"},"rdfs:comment":"Contains the EUI-64 of the link layer interface. 48 bit MAC addresses SHALL be changed into an EUI-64 using the method defined in [RFC 4291], Appendix A. (The method is to insert \"0xFFFE\" as described in the reference.)"},{"@id":"IEEE_802_15_4","@type":"rdf:Property","rdfs:domain":{"@id":"LLInterface"},"rdfs:range":{"@id":"IEEE_802_15_4"},"owl:minCardinality":0},{"@id":"linkLayerType","@type":"rdf:Property","rdfs:domain":{"@id":"LLInterface"},"rdfs:range":{"@id":"UInt8"},"rdfs:comment":"Specifies the type of link layer interface associated with the IPInterface. Values are below.\n0 = Unspecified \n1 = IEEE 802.3 (Ethernet)\n2 = IEEE 802.11 (WLAN)\n3 = IEEE 802.15 (PAN)\n4 = IEEE 1901 (PLC)\nAll other values reserved."},{"@id":"LLAckNotRx","@type":"rdf:Property","rdfs:domain":{"@id":"LLInterface"},"rdfs:range":{"@id":"UInt32"},"rdfs:comment":"Number of times an ACK was not received for a frame transmitted (when ACK was requested).","owl:minCardinality":0},{"@id":"LLCSMAFail","@type":"rdf:Property","rdfs:domain":{"@id":"LLInterface"},"rdfs:range":{"@id":"UInt32"},"rdfs:comment":"Number of times CSMA failed.","owl:minCardinality":0},{"@id":"LLFramesDropRx","@type":"rdf:Property","rdfs:domain":{"@id":"LLInterface"},"rdfs:range":{"@id":"UInt32"},"rdfs:comment":"Number of dropped receive frames.","owl:minCardinality":0},{"@id":"LLFramesDropTx","@type":"rdf:Property","rdfs:domain":{"@id":"LLInterface"},"rdfs:range":{"@id":"UInt32"},"rdfs:comment":"Number of dropped transmit frames.","owl:minCardinality":0},{"@id":"LLFramesRx","@type":"rdf:Property","rdfs:domain":{"@id":"LLInterface"},"rdfs:range":{"@id":"UInt32"},"rdfs:comment":"Number of link layer frames received.","owl:minCardinality":0},{"@id":"LLFramesTx","@type":"rdf:Property","rdfs:domain":{"@id":"LLInterface"},"rdfs:range":{"@id":"UInt32"},"rdfs:comment":"Number of link layer frames transmitted.","owl:minCardinality":0},{"@id":"LLMediaAccessFail","@type":"rdf:Property","rdfs:domain":{"@id":"LLInterface"},"rdfs:range":{"@id":"UInt32"},"rdfs:comment":"Number of times access to media failed.","owl:minCardinality":0},{"@id":"LLOctetsRx","@type":"rdf:Property","rdfs:domain":{"@id":"LLInterface"},"rdfs:range":{"@id":"UInt32"},"rdfs:comment":"Number of Bytes received.","owl:minCardinality":0},{"@id":"LLOctetsTx","@type":"rdf:Property","rdfs:domain":{"@id":"LLInterface"},"rdfs:range":{"@id":"UInt32"},"rdfs:comment":"Number of Bytes transmitted.","owl:minCardinality":0},{"@id":"LLRetryCount","@type":"rdf:Property","rdfs:domain":{"@id":"LLInterface"},"rdfs:range":{"@id":"UInt32"},"rdfs:comment":"Number of MAC transmit retries.","owl:minCardinality":0},{"@id":"LLSecurityErrorRx","@type":"rdf:Property","rdfs:domain":{"@id":"LLInterface"},"rdfs:range":{"@id":"UInt32"},"rdfs:comment":"Number of receive security errors.","owl:minCardinality":0},{"@id":"loWPAN","@type":"rdf:Property","rdfs:domain":{"@id":"LLInterface"},"rdfs:range":{"@id":"loWPAN"},"owl:minCardinality":0},{"@id":"LLInterface","@type":"rdf:Property","rdfs:domain":{"@id":"LLInterfaceList"},"rdfs:range":{"@id":"LLInterface"},"owl:minCardinality":0},{"@id":"octetsRx","@type":"rdf:Property","rdfs:domain":{"@id":"loWPAN"},"rdfs:range":{"@id":"UInt32"},"rdfs:comment":"Number of Bytes received","owl:minCardinality":0},{"@id":"octetsTx","@type":"rdf:Property","rdfs:domain":{"@id":"loWPAN"},"rdfs:range":{"@id":"UInt32"},"rdfs:comment":"Number of Bytes transmitted","owl:minCardinality":0},{"@id":"packetsRx","@type":"rdf:Property","rdfs:domain":{"@id":"loWPAN"},"rdfs:range":{"@id":"UInt32"},"rdfs:comment":"Number of packets received"},{"@id":"packetsTx","@type":"rdf:Property","rdfs:domain":{"@id":"loWPAN"},"rdfs:range":{"@id":"UInt32"},"rdfs:comment":"Number of packets transmitted"},{"@id":"rxFragError","@type":"rdf:Property","rdfs:domain":{"@id":"loWPAN"},"rdfs:range":{"@id":"UInt32"},"rdfs:comment":"Number of errors receiving fragments"},{"@id":"isChild","@type":"rdf:Property","rdfs:domain":{"@id":"Neighbor"},"rdfs:range":"xsd:boolean","rdfs:comment":"True if the neighbor is a child."},{"@id":"linkQuality","@type":"rdf:Property","rdfs:domain":{"@id":"Neighbor"},"rdfs:range":{"@id":"UInt8"},"rdfs:comment":"The quality of the link, as defined by 802.15.4"},{"@id":"shortAddress","@type":"rdf:Property","rdfs:domain":{"@id":"Neighbor"},"rdfs:range":{"@id":"UInt16"},"rdfs:comment":"As defined by IEEE 802.15.4"},{"@id":"Neighbor","@type":"rdf:Property","rdfs:domain":{"@id":"NeighborList"},"rdfs:range":{"@id":"Neighbor"},"owl:minCardinality":0},{"@id":"DODAGid","@type":"rdf:Property","rdfs:domain":{"@id":"RPLInstance"},"rdfs:range":{"@id":"UInt8"},"rdfs:comment":"See [RFC 6550]."},{"@id":"DODAGroot","@type":"rdf:Property","rdfs:domain":{"@id":"RPLInstance"},"rdfs:range":"xsd:boolean","rdfs:comment":"See [RFC 6550]."},{"@id":"flags","@type":"rdf:Property","rdfs:domain":{"@id":"RPLInstance"},"rdfs:range":{"@id":"UInt8"},"rdfs:comment":"See [RFC 6550]."},{"@id":"groundedFlag","@type":"rdf:Property","rdfs:domain":{"@id":"RPLInstance"},"rdfs:range":"xsd:boolean","rdfs:comment":"See [RFC 6550]."},{"@id":"MOP","@type":"rdf:Property","rdfs:domain":{"@id":"RPLInstance"},"rdfs:range":{"@id":"UInt8"},"rdfs:comment":"See [RFC 6550]."},{"@id":"PRF","@type":"rdf:Property","rdfs:domain":{"@id":"RPLInstance"},"rdfs:range":{"@id":"UInt8"},"rdfs:comment":"See [RFC 6550]."},{"@id":"rank","@type":"rdf:Property","rdfs:domain":{"@id":"RPLInstance"},"rdfs:range":{"@id":"UInt16"},"rdfs:comment":"See [RFC 6550]."},{"@id":"RPLInstanceID","@type":"rdf:Property","rdfs:domain":{"@id":"RPLInstance"},"rdfs:range":{"@id":"UInt8"},"rdfs:comment":"See [RFC 6550]."},{"@id":"RPLSourceRoutesListLink","@type":"rdf:Property","rdfs:domain":{"@id":"RPLInstance"},"rdfs:range":{"@id":"RPLSourceRoutesListLink"},"owl:minCardinality":0},{"@id":"versionNumber","@type":"rdf:Property","rdfs:domain":{"@id":"RPLInstance"},"rdfs:range":{"@id":"UInt8"},"rdfs:comment":"See [RFC 6550]."},{"@id":"RPLInstance","@type":"rdf:Property","rdfs:domain":{"@id":"RPLInstanceList"},"rdfs:range":{"@id":"RPLInstance"},"owl:minCardinality":0},{"@id":"DestAddress","@type":"rdf:Property","rdfs:domain":{"@id":"RPLSourceRoutes"},"rdfs:range":{"@id":"HexBinary128"},"rdfs:comment":"See [RFC 6554]."},{"@id":"SourceRoute","@type":"rdf:Property","rdfs:domain":{"@id":"RPLSourceRoutes"},"rdfs:range":{"@id":"HexBinary128"},"rdfs:comment":"See [RFC 6554]."},{"@id":"RPLSourceRoutes","@type":"rdf:Property","rdfs:domain":{"@id":"RPLSourceRoutesList"},"rdfs:range":{"@id":"RPLSourceRoutes"},"owl:minCardinality":0},{"@id":"createdDateTime","@type":"rdf:Property","rdfs:domain":{"@id":"LogEvent"},"rdfs:range":{"@id":"TimeType"},"rdfs:comment":"The date and time that the event occurred."},{"@id":"details","@type":"rdf:Property","rdfs:domain":{"@id":"LogEvent"},"rdfs:range":{"@id":"String32"},"rdfs:comment":"Human readable text that MAY be used to transmit additional details about the event. A host MAY remove this field when received.","owl:minCardinality":0},{"@id":"extendedData","@type":"rdf:Property","rdfs:domain":{"@id":"LogEvent"},"rdfs:range":{"@id":"UInt32"},"rdfs:comment":"May be used to transmit additional details about the event.","owl:minCardinality":0},{"@id":"functionSet","@type":"rdf:Property","rdfs:domain":{"@id":"LogEvent"},"rdfs:range":{"@id":"UInt8"},"rdfs:comment":"If the profileID indicates this is IEEE 2030.5, the functionSet is defined by IEEE 2030.5 and SHALL be one of the values from the table below (IEEE 2030.5 function set identifiers). If the profileID is anything else, the functionSet is defined by the identified profile. \n0\tGeneral (not specific to a function set)\n1\tPublish and Subscribe\n2\tEnd Device\n3\tFunction Set Assignment\n4\tResponse\n5\tDemand Response and Load Control\n6\tMetering\n7\tPricing\n8\tMessaging\n9\tBilling\n10\tPrepayment\n11\tDistributed Energy Resources\n12\tTime\n13\tSoftware  Download\n14\tDevice Information\n15\tPower Status\n16\tNetwork Status\n17\tLog Event List\n18\tConfiguration\n19\tSecurity\nAll other values are reserved."},{"@id":"logEventCode","@type":"rdf:Property","rdfs:domain":{"@id":"LogEvent"},"rdfs:range":{"@id":"UInt8"},"rdfs:comment":"An 8 bit unsigned integer. logEventCodes are scoped to a profile and a function set. If the profile is IEEE 2030.5, the logEventCode is defined by IEEE 2030.5 within one of the function sets of IEEE 2030.5. If the profile is anything else, the logEventCode is defined by the specified profile."},{"@id":"logEventID","@type":"rdf:Property","rdfs:domain":{"@id":"LogEvent"},"rdfs:range":{"@id":"UInt16"},"rdfs:comment":"This 16-bit value, combined with createdDateTime, profileID, and logEventPEN, should provide a reasonable level of uniqueness."},{"@id":"logEventPEN","@type":"rdf:Property","rdfs:domain":{"@id":"LogEvent"},"rdfs:range":{"@id":"PENType"},"rdfs:comment":"The Private Enterprise Number(PEN) of the entity that defined the profileID, functionSet, and logEventCode of the logEvent. IEEE 2030.5-assigned logEventCodes SHALL use the IEEE 2030.5 PEN.  Combinations of profileID, functionSet, and logEventCode SHALL have unique meaning within a logEventPEN and are defined by the owner of the PEN."},{"@id":"profileID","@type":"rdf:Property","rdfs:domain":{"@id":"LogEvent"},"rdfs:range":{"@id":"UInt8"},"rdfs:comment":"The profileID identifies which profile (HA, BA, SE, etc) defines the following event information.\n0\tNot profile specific.\n1\tVendor Defined\n2\tIEEE 2030.5\n3\tHome Automation\n4\tBuilding Automation\nAll other values are reserved."},{"@id":"LogEvent","@type":"rdf:Property","rdfs:domain":{"@id":"LogEventList"},"rdfs:range":{"@id":"LogEvent"},"owl:minCardinality":0},{"@id":"pollRate","@type":"rdf:Property","rdfs:domain":{"@id":"LogEventList"},"rdfs:range":{"@id":"UInt32"},"rdfs:comment":"The default polling rate for this function set (this resource and all resources below), in seconds. If not specified, a default of 900 seconds (15 minutes) is used. It is RECOMMENDED a client poll the resources of this function set every pollRate seconds.","owl:minCardinality":0},{"@id":"currentLocale","@type":"rdf:Property","rdfs:domain":{"@id":"Configuration"},"rdfs:range":{"@id":"LocaleType"},"rdfs:comment":"[RFC 4646] identifier of the language-region currently in use."},{"@id":"PowerConfiguration","@type":"rdf:Property","rdfs:domain":{"@id":"Configuration"},"rdfs:range":{"@id":"PowerConfiguration"},"owl:minCardinality":0},{"@id":"PriceResponseCfgListLink","@type":"rdf:Property","rdfs:domain":{"@id":"Configuration"},"rdfs:range":{"@id":"PriceResponseCfgListLink"},"owl:minCardinality":0},{"@id":"TimeConfiguration","@type":"rdf:Property","rdfs:domain":{"@id":"Configuration"},"rdfs:range":{"@id":"TimeConfiguration"},"owl:minCardinality":0},{"@id":"userDeviceName","@type":"rdf:Property","rdfs:domain":{"@id":"Configuration"},"rdfs:range":{"@id":"String32"},"rdfs:comment":"User assigned, convenience name used for network browsing displays, etc.  Example \"My Thermostat\""},{"@id":"pollRate","@type":"rdf:Property","rdfs:domain":{"@id":"Configuration"},"rdfs:range":{"@id":"UInt32"},"rdfs:comment":"The default polling rate for this function set (this resource and all resources below), in seconds. If not specified, a default of 900 seconds (15 minutes) is used. It is RECOMMENDED a client poll the resources of this function set every pollRate seconds.","owl:minCardinality":0},{"@id":"batteryInstallTime","@type":"rdf:Property","rdfs:domain":{"@id":"PowerConfiguration"},"rdfs:range":{"@id":"TimeType"},"rdfs:comment":"Time/Date at which battery was installed,","owl:minCardinality":0},{"@id":"lowChargeThreshold","@type":"rdf:Property","rdfs:domain":{"@id":"PowerConfiguration"},"rdfs:range":{"@id":"UInt32"},"rdfs:comment":"In context of the PowerStatus resource, this is the value of EstimatedTimeRemaining below which BatteryStatus \"low\" is indicated and the PS_LOW_BATTERY is raised.","owl:minCardinality":0},{"@id":"consumeThreshold","@type":"rdf:Property","rdfs:domain":{"@id":"PriceResponseCfg"},"rdfs:range":{"@id":"Int32"},"rdfs:comment":"Price responsive clients acting upon the associated RateComponent SHOULD consume the associated commodity while the price is less than this threshold."},{"@id":"maxReductionThreshold","@type":"rdf:Property","rdfs:domain":{"@id":"PriceResponseCfg"},"rdfs:range":{"@id":"Int32"},"rdfs:comment":"Price responsive clients acting upon the associated RateComponent SHOULD reduce consumption to the maximum extent possible while the price is greater than this threshold."},{"@id":"RateComponentLink","@type":"rdf:Property","rdfs:domain":{"@id":"PriceResponseCfg"},"rdfs:range":{"@id":"RateComponentLink"}},{"@id":"PriceResponseCfg","@type":"rdf:Property","rdfs:domain":{"@id":"PriceResponseCfgList"},"rdfs:range":{"@id":"PriceResponseCfg"},"owl:minCardinality":0},{"@id":"dstEndRule","@type":"rdf:Property","rdfs:domain":{"@id":"TimeConfiguration"},"rdfs:range":{"@id":"DstRuleType"},"rdfs:comment":"Rule to calculate end of daylight savings time in the current year.  Result of dstEndRule must be greater than result of dstStartRule."},{"@id":"dstOffset","@type":"rdf:Property","rdfs:domain":{"@id":"TimeConfiguration"},"rdfs:range":{"@id":"TimeOffsetType"},"rdfs:comment":"Daylight savings time offset from local standard time."},{"@id":"dstStartRule","@type":"rdf:Property","rdfs:domain":{"@id":"TimeConfiguration"},"rdfs:range":{"@id":"DstRuleType"},"rdfs:comment":"Rule to calculate start of daylight savings time in the current year. Result of dstEndRule must be greater than result of dstStartRule."},{"@id":"tzOffset","@type":"rdf:Property","rdfs:domain":{"@id":"TimeConfiguration"},"rdfs:range":{"@id":"TimeOffsetType"},"rdfs:comment":"Local time zone offset from UTCTime. Does not include any daylight savings time offsets."},{"@id":"activateTime","@type":"rdf:Property","rdfs:domain":{"@id":"File"},"rdfs:range":{"@id":"TimeType"},"rdfs:comment":"This element MUST be set to the date/time at which this file is activated. If the activation time is less than or equal to current time, the LD MUST immediately place the file into the activated state (in the case of a firmware file, the file is now the running image).  If the activation time is greater than the current time, the LD MUST wait until the specified activation time is reached, then MUST place the file into the activated state. Omission of this element means that the LD MUST NOT take any action to activate the file until a subsequent GET to this File resource provides an activateTime.","owl:minCardinality":0},{"@id":"fileURI","@type":"rdf:Property","rdfs:domain":{"@id":"File"},"rdfs:range":"xsd:anyURI","rdfs:comment":"This element MUST be set to the URI location of the file binary artifact.  This is the BLOB (binary large object) that is actually loaded by the LD"},{"@id":"lFDI","@type":"rdf:Property","rdfs:domain":{"@id":"File"},"rdfs:range":{"@id":"HexBinary160"},"rdfs:comment":"This element MUST be set to the LFDI of the device for which this file in targeted.","owl:minCardinality":0},{"@id":"mfHwVer","@type":"rdf:Property","rdfs:domain":{"@id":"File"},"rdfs:range":{"@id":"String32"},"rdfs:comment":"This element MUST be set to the hardware version for which this file is targeted.","owl:minCardinality":0},{"@id":"mfID","@type":"rdf:Property","rdfs:domain":{"@id":"File"},"rdfs:range":{"@id":"PENType"},"rdfs:comment":"This element MUST be set to the manufacturer's Private Enterprise Number (assigned by IANA)."},{"@id":"mfModel","@type":"rdf:Property","rdfs:domain":{"@id":"File"},"rdfs:range":{"@id":"String32"},"rdfs:comment":"This element MUST be set to the manufacturer model number for which this file is targeted. The syntax and semantics are left to the manufacturer."},{"@id":"mfSerNum","@type":"rdf:Property","rdfs:domain":{"@id":"File"},"rdfs:range":{"@id":"String32"},"rdfs:comment":"This element MUST be set to the manufacturer serial number for which this file is targeted. The syntax and semantics are left to the manufacturer.","owl:minCardinality":0},{"@id":"mfVer","@type":"rdf:Property","rdfs:domain":{"@id":"File"},"rdfs:range":{"@id":"String16"},"rdfs:comment":"This element MUST be set to the software version information for this file. The syntax and semantics are left to the manufacturer."},{"@id":"size","@type":"rdf:Property","rdfs:domain":{"@id":"File"},"rdfs:range":{"@id":"UInt32"},"rdfs:comment":"This element MUST be set to the total size (in bytes) of the file referenced by fileURI."},{"@id":"type","@type":"rdf:Property","rdfs:domain":{"@id":"File"},"rdfs:range":{"@id":"HexBinary16"},"rdfs:comment":"A value indicating the type of the file.  MUST be one of the following values:\n00 = Software Image\n01 = Security Credential\n02 = Configuration\n03 = Log\n04\u20137FFF = reserved\n8000-FFFF = Manufacturer defined"},{"@id":"File","@type":"rdf:Property","rdfs:domain":{"@id":"FileList"},"rdfs:range":{"@id":"File"},"owl:minCardinality":0},{"@id":"pollRate","@type":"rdf:Property","rdfs:domain":{"@id":"FileList"},"rdfs:range":{"@id":"UInt32"},"rdfs:comment":"The default polling rate for this function set (this resource and all resources below), in seconds. If not specified, a default of 900 seconds (15 minutes) is used. It is RECOMMENDED a client poll the resources of this function set every pollRate seconds.","owl:minCardinality":0},{"@id":"activateTime","@type":"rdf:Property","rdfs:domain":{"@id":"FileStatus"},"rdfs:range":{"@id":"TimeType"},"rdfs:comment":"Date/time at which this File, referred to by FileLink, will be activated. Omission of or presence and value of this element MUST exactly match omission or presence and value of the activateTime element from the File resource.","owl:minCardinality":0},{"@id":"FileLink","@type":"rdf:Property","rdfs:domain":{"@id":"FileStatus"},"rdfs:range":{"@id":"FileLink"},"owl:minCardinality":0},{"@id":"loadPercent","@type":"rdf:Property","rdfs:domain":{"@id":"FileStatus"},"rdfs:range":{"@id":"UInt8"},"rdfs:comment":"This element MUST be set to the percentage of the file, indicated by FileLink, that was loaded during the latest load attempt. This value MUST be reset to 0 each time a load attempt is started for the File indicated by FileLink. This value MUST be increased when an LD receives HTTP response containing file content. This value MUST be set to 100 when the full content of the file has been received by the LD"},{"@id":"nextRequestAttempt","@type":"rdf:Property","rdfs:domain":{"@id":"FileStatus"},"rdfs:range":{"@id":"TimeType"},"rdfs:comment":"This element MUST be set to the time at which the LD will issue its next GET request for file content from the File indicated by FileLink"},{"@id":"request503Count","@type":"rdf:Property","rdfs:domain":{"@id":"FileStatus"},"rdfs:range":{"@id":"UInt16"},"rdfs:comment":"This value MUST be reset to 0 when FileLink is first pointed at a new File. This value MUST be incremented each time an \n\nLD receives a 503 error from the FS."},{"@id":"requestFailCount","@type":"rdf:Property","rdfs:domain":{"@id":"FileStatus"},"rdfs:range":{"@id":"UInt16"},"rdfs:comment":"This value MUST be reset to 0 when FileLink is first pointed at a new File. This value MUST be incremented each time a GET request for file content failed. 503 errors MUST be excluded from this counter."},{"@id":"status","@type":"rdf:Property","rdfs:domain":{"@id":"FileStatus"},"rdfs:range":{"@id":"UInt8"},"rdfs:comment":"Current loading status of the file indicated by FileLink. This element MUST be set to one of the following values:\n0 - No load operation in progress\n1 - File load in progress (first request for file content has been issued by LD)\n2 - File load failed\n3 - File loaded successfully (full content of file has been received by the LD), signature verification in progress\n4 - File signature verification failed\n5 - File signature verified, waiting to activate file.\n6 - File activation failed\n7 - File activation in progress  \n8 - File activated successfully (this state may not be reached/persisted through an image activation)\n9-255 - Reserved for future use."},{"@id":"statusTime","@type":"rdf:Property","rdfs:domain":{"@id":"FileStatus"},"rdfs:range":{"@id":"TimeType"},"rdfs:comment":"This element MUST be set to the time at which file status transitioned to the value indicated in the status element."},{"@id":"pollRate","@type":"rdf:Property","rdfs:domain":{"@id":"FileStatus"},"rdfs:range":{"@id":"UInt32"},"rdfs:comment":"The default polling rate for this function set (this resource and all resources below), in seconds. If not specified, a default of 900 seconds (15 minutes) is used. It is RECOMMENDED a client poll the resources of this function set every pollRate seconds.","owl:minCardinality":0},{"@id":"LoadShedAvailability","@type":"rdf:Property","rdfs:domain":{"@id":"LoadShedAvailabilityList"},"rdfs:range":{"@id":"LoadShedAvailability"},"owl:minCardinality":0},{"@id":"pollRate","@type":"rdf:Property","rdfs:domain":{"@id":"LoadShedAvailabilityList"},"rdfs:range":{"@id":"UInt32"},"rdfs:comment":"The default polling rate for this function set (this resource and all resources below), in seconds. If not specified, a default of 900 seconds (15 minutes) is used. It is RECOMMENDED a client poll the resources of this function set every pollRate seconds.","owl:minCardinality":0},{"@id":"type","@type":"rdf:Property","rdfs:domain":{"@id":"ApplianceLoadReduction"},"rdfs:range":{"@id":"ApplianceLoadReductionType"},"rdfs:comment":"Indicates the type of appliance load reduction requested."},{"@id":"ActiveEndDeviceControlListLink","@type":"rdf:Property","rdfs:domain":{"@id":"DemandResponseProgram"},"rdfs:range":{"@id":"ActiveEndDeviceControlListLink"},"owl:minCardinality":0},{"@id":"availabilityUpdatePercentChangeThreshold","@type":"rdf:Property","rdfs:domain":{"@id":"DemandResponseProgram"},"rdfs:range":{"@id":"PerCent"},"rdfs:comment":"This attribute allows program providers to specify the requested granularity of updates to LoadShedAvailability sheddablePercent. If not present, or set to 0, then updates to LoadShedAvailability SHALL NOT be provided. If present and greater than zero, then clients SHALL provide their LoadShedAvailability if it has not previously been provided, and thereafter if the difference between the previously provided value and the current value of LoadShedAvailability sheddablePercent is greater than availabilityUpdatePercentChangeThreshold.","owl:minCardinality":0},{"@id":"availabilityUpdatePowerChangeThreshold","@type":"rdf:Property","rdfs:domain":{"@id":"DemandResponseProgram"},"rdfs:range":{"@id":"ActivePower"},"rdfs:comment":"This attribute allows program providers to specify the requested granularity of updates to LoadShedAvailability sheddablePower. If not present, or set to 0, then updates to LoadShedAvailability SHALL NOT be provided. If present and greater than zero, then clients SHALL provide their LoadShedAvailability if it has not previously been provided, and thereafter if the difference between the previously provided value and the current value of LoadShedAvailability sheddablePower is greater than availabilityUpdatePowerChangeThreshold.","owl:minCardinality":0},{"@id":"EndDeviceControlListLink","@type":"rdf:Property","rdfs:domain":{"@id":"DemandResponseProgram"},"rdfs:range":{"@id":"EndDeviceControlListLink"},"owl:minCardinality":0},{"@id":"primacy","@type":"rdf:Property","rdfs:domain":{"@id":"DemandResponseProgram"},"rdfs:range":{"@id":"PrimacyType"},"rdfs:comment":"Indicates the relative primacy of the provider of this program."},{"@id":"DemandResponseProgram","@type":"rdf:Property","rdfs:domain":{"@id":"DemandResponseProgramList"},"rdfs:range":{"@id":"DemandResponseProgram"},"owl:minCardinality":0},{"@id":"pollRate","@type":"rdf:Property","rdfs:domain":{"@id":"DemandResponseProgramList"},"rdfs:range":{"@id":"UInt32"},"rdfs:comment":"The default polling rate for this function set (this resource and all resources below), in seconds. If not specified, a default of 900 seconds (15 minutes) is used. It is RECOMMENDED a client poll the resources of this function set every pollRate seconds.","owl:minCardinality":0},{"@id":"normalValue","@type":"rdf:Property","rdfs:domain":{"@id":"DutyCycle"},"rdfs:range":{"@id":"UInt8"},"rdfs:comment":"Contains the maximum On state duty cycle applied by the end device, as a percentage of time.  The field not present indicates that this field has not been used by the end device."},{"@id":"ApplianceLoadReduction","@type":"rdf:Property","rdfs:domain":{"@id":"EndDeviceControl"},"rdfs:range":{"@id":"ApplianceLoadReduction"},"owl:minCardinality":0},{"@id":"deviceCategory","@type":"rdf:Property","rdfs:domain":{"@id":"EndDeviceControl"},"rdfs:range":{"@id":"DeviceCategoryType"},"rdfs:comment":"Specifies the bitmap indicating  the categories of devices that SHOULD respond. Devices SHOULD ignore events that do not indicate their device category."},{"@id":"drProgramMandatory","@type":"rdf:Property","rdfs:domain":{"@id":"EndDeviceControl"},"rdfs:range":"xsd:boolean","rdfs:comment":"A flag to indicate if the EndDeviceControl is considered a mandatory event as defined by the service provider issuing the EndDeviceControl. The drProgramMandatory flag alerts the client/user that they will be subject to penalty or ineligibility based on the service provider\u2019s program rules for that deviceCategory."},{"@id":"DutyCycle","@type":"rdf:Property","rdfs:domain":{"@id":"EndDeviceControl"},"rdfs:range":{"@id":"DutyCycle"},"owl:minCardinality":0},{"@id":"loadShiftForward","@type":"rdf:Property","rdfs:domain":{"@id":"EndDeviceControl"},"rdfs:range":"xsd:boolean","rdfs:comment":"Indicates that the event intends to increase consumption. A value of true indicates the intention to increase usage value, and a value of false indicates the intention to decrease usage."},{"@id":"Offset","@type":"rdf:Property","rdfs:domain":{"@id":"EndDeviceControl"},"rdfs:range":{"@id":"Offset"},"owl:minCardinality":0},{"@id":"overrideDuration","@type":"rdf:Property","rdfs:domain":{"@id":"EndDeviceControl"},"rdfs:range":{"@id":"UInt16"},"rdfs:comment":"The overrideDuration attribute provides a duration, in seconds, for which a client device is allowed to override this EndDeviceControl and still meet the contractual agreement with a service provider without opting out. If overrideDuration is not specified, then it SHALL default to 0.","owl:minCardinality":0},{"@id":"SetPoint","@type":"rdf:Property","rdfs:domain":{"@id":"EndDeviceControl"},"rdfs:range":{"@id":"SetPoint"},"owl:minCardinality":0},{"@id":"TargetReduction","@type":"rdf:Property","rdfs:domain":{"@id":"EndDeviceControl"},"rdfs:range":{"@id":"TargetReduction"},"owl:minCardinality":0},{"@id":"EndDeviceControl","@type":"rdf:Property","rdfs:domain":{"@id":"EndDeviceControlList"},"rdfs:range":{"@id":"EndDeviceControl"},"owl:minCardinality":0},{"@id":"availabilityDuration","@type":"rdf:Property","rdfs:domain":{"@id":"LoadShedAvailability"},"rdfs:range":{"@id":"UInt32"},"rdfs:comment":"Indicates for how many seconds the consuming device will be able to reduce consumption at the maximum response level.","owl:minCardinality":0},{"@id":"DemandResponseProgramLink","@type":"rdf:Property","rdfs:domain":{"@id":"LoadShedAvailability"},"rdfs:range":{"@id":"DemandResponseProgramLink"},"owl:minCardinality":0},{"@id":"sheddablePercent","@type":"rdf:Property","rdfs:domain":{"@id":"LoadShedAvailability"},"rdfs:range":{"@id":"PerCent"},"rdfs:comment":"Maximum percent of current operating load that is estimated to be sheddable.","owl:minCardinality":0},{"@id":"sheddablePower","@type":"rdf:Property","rdfs:domain":{"@id":"LoadShedAvailability"},"rdfs:range":{"@id":"ActivePower"},"rdfs:comment":"Maximum amount of current operating load that is estimated to be sheddable, in Watts.","owl:minCardinality":0},{"@id":"coolingOffset","@type":"rdf:Property","rdfs:domain":{"@id":"Offset"},"rdfs:range":{"@id":"UInt8"},"rdfs:comment":"The value change requested for the cooling offset, in degree C / 10. The value should be added to the normal set point for cooling, or if loadShiftForward is true, then the value should be subtracted from the normal set point.","owl:minCardinality":0},{"@id":"heatingOffset","@type":"rdf:Property","rdfs:domain":{"@id":"Offset"},"rdfs:range":{"@id":"UInt8"},"rdfs:comment":"The value change requested for the heating offset, in degree C / 10. The value should be subtracted for heating, or if loadShiftForward is true, then the value should be added to the normal set point.","owl:minCardinality":0},{"@id":"loadAdjustmentPercentageOffset","@type":"rdf:Property","rdfs:domain":{"@id":"Offset"},"rdfs:range":{"@id":"PerCent"},"rdfs:comment":"The value change requested for the load adjustment percentage. The value should be subtracted from the normal setting, or if loadShiftForward is true, then the value should be added to the normal setting.","owl:minCardinality":0},{"@id":"coolingSetpoint","@type":"rdf:Property","rdfs:domain":{"@id":"SetPoint"},"rdfs:range":{"@id":"Int16"},"rdfs:comment":"This attribute represents the cooling temperature set point in degrees Celsius / 100. (Hundredths of a degree C)","owl:minCardinality":0},{"@id":"heatingSetpoint","@type":"rdf:Property","rdfs:domain":{"@id":"SetPoint"},"rdfs:range":{"@id":"Int16"},"rdfs:comment":"This attribute represents the heating temperature set point in degrees Celsius / 100. (Hundredths of a degree C)","owl:minCardinality":0},{"@id":"type","@type":"rdf:Property","rdfs:domain":{"@id":"TargetReduction"},"rdfs:range":{"@id":"UnitType"},"rdfs:comment":"Indicates the type of reduction requested."},{"@id":"value","@type":"rdf:Property","rdfs:domain":{"@id":"TargetReduction"},"rdfs:range":{"@id":"UInt16"},"rdfs:comment":"Indicates the requested amount of the relevant commodity to be reduced."},{"@id":"RateComponentListLink","@type":"rdf:Property","rdfs:domain":{"@id":"MeterReading"},"rdfs:range":{"@id":"RateComponentListLink"},"owl:minCardinality":0},{"@id":"ReadingLink","@type":"rdf:Property","rdfs:domain":{"@id":"MeterReading"},"rdfs:range":{"@id":"ReadingLink"},"owl:minCardinality":0},{"@id":"ReadingSetListLink","@type":"rdf:Property","rdfs:domain":{"@id":"MeterReading"},"rdfs:range":{"@id":"ReadingSetListLink"},"owl:minCardinality":0},{"@id":"ReadingTypeLink","@type":"rdf:Property","rdfs:domain":{"@id":"MeterReading"},"rdfs:range":{"@id":"ReadingTypeLink"}},{"@id":"MeterReading","@type":"rdf:Property","rdfs:domain":{"@id":"MeterReadingList"},"rdfs:range":{"@id":"MeterReading"},"owl:minCardinality":0},{"@id":"localID","@type":"rdf:Property","rdfs:domain":{"@id":"Reading"},"rdfs:range":{"@id":"HexBinary16"},"rdfs:comment":"The local identifier for this reading within the reading set. localIDs are assigned in order of creation time. For interval data, this value SHALL increase with each interval time, and for block/tier readings, localID SHALL not be specified.","owl:minCardinality":0},{"@id":"subscribable","@type":"rdf:Property","rdfs:domain":{"@id":"Reading"},"rdfs:range":{"@id":"SubscribableType"},"rdfs:comment":"Indicates whether or not subscriptions are supported for this resource, and whether or not conditional (thresholds) are supported. If not specified, is \"not subscribable\" (0).","owl:minCardinality":0},{"@id":"Reading","@type":"rdf:Property","rdfs:domain":{"@id":"ReadingList"},"rdfs:range":{"@id":"Reading"},"owl:minCardinality":0},{"@id":"ReadingListLink","@type":"rdf:Property","rdfs:domain":{"@id":"ReadingSet"},"rdfs:range":{"@id":"ReadingListLink"},"owl:minCardinality":0},{"@id":"ReadingSet","@type":"rdf:Property","rdfs:domain":{"@id":"ReadingSetList"},"rdfs:range":{"@id":"ReadingSet"},"owl:minCardinality":0},{"@id":"accumulationBehaviour","@type":"rdf:Property","rdfs:domain":{"@id":"ReadingType"},"rdfs:range":{"@id":"AccumulationBehaviourType"},"rdfs:comment":"The \u201caccumulation behaviour\u201d indicates how the value is represented to accumulate over time.","owl:minCardinality":0},{"@id":"calorificValue","@type":"rdf:Property","rdfs:domain":{"@id":"ReadingType"},"rdfs:range":{"@id":"UnitValueType"},"rdfs:comment":"The amount of heat generated when a given mass of fuel is completely burned. The CalorificValue is used to convert the measured volume or mass of gas into kWh. The CalorificValue attribute represents the current active value.","owl:minCardinality":0},{"@id":"commodity","@type":"rdf:Property","rdfs:domain":{"@id":"ReadingType"},"rdfs:range":{"@id":"CommodityType"},"rdfs:comment":"Indicates the commodity applicable to this ReadingType.","owl:minCardinality":0},{"@id":"conversionFactor","@type":"rdf:Property","rdfs:domain":{"@id":"ReadingType"},"rdfs:range":{"@id":"UnitValueType"},"rdfs:comment":"Accounts for changes in the volume of gas based on temperature and pressure. The ConversionFactor attribute represents the current active value. The ConversionFactor is dimensionless. The default value for the ConversionFactor is 1, which means no conversion is applied. A price server can advertise a new/different value at any time.","owl:minCardinality":0},{"@id":"dataQualifier","@type":"rdf:Property","rdfs:domain":{"@id":"ReadingType"},"rdfs:range":{"@id":"DataQualifierType"},"rdfs:comment":"The data type can be used to describe a salient attribute of the data. Possible values are average, absolute, and etc.","owl:minCardinality":0},{"@id":"flowDirection","@type":"rdf:Property","rdfs:domain":{"@id":"ReadingType"},"rdfs:range":{"@id":"FlowDirectionType"},"rdfs:comment":"Anything involving current might have a flow direction. Possible values include forward and reverse.","owl:minCardinality":0},{"@id":"intervalLength","@type":"rdf:Property","rdfs:domain":{"@id":"ReadingType"},"rdfs:range":{"@id":"UInt32"},"rdfs:comment":"Default interval length specified in seconds.","owl:minCardinality":0},{"@id":"kind","@type":"rdf:Property","rdfs:domain":{"@id":"ReadingType"},"rdfs:range":{"@id":"KindType"},"rdfs:comment":"Compound class that contains kindCategory and kindIndex","owl:minCardinality":0},{"@id":"maxNumberOfIntervals","@type":"rdf:Property","rdfs:domain":{"@id":"ReadingType"},"rdfs:range":{"@id":"UInt8"},"rdfs:comment":"To be populated for mirrors of interval data to set the expected number of intervals per ReadingSet. Servers may discard intervals received that exceed this number.","owl:minCardinality":0},{"@id":"numberOfConsumptionBlocks","@type":"rdf:Property","rdfs:domain":{"@id":"ReadingType"},"rdfs:range":{"@id":"UInt8"},"rdfs:comment":"Number of consumption blocks. 0 means not applicable, and is the default if not specified. The value needs to be at least 1 if any actual prices are provided.","owl:minCardinality":0},{"@id":"numberOfTouTiers","@type":"rdf:Property","rdfs:domain":{"@id":"ReadingType"},"rdfs:range":{"@id":"UInt8"},"rdfs:comment":"The number of TOU tiers that can be used by any resource configured by this ReadingType. Servers SHALL populate this value with the largest touTier value that will <i>ever</i> be used while this ReadingType is in effect. Servers SHALL set numberOfTouTiers equal to the number of standard TOU tiers plus the number of CPP tiers that may be used while this ReadingType is in effect. Servers SHALL specify a value between 0 and 255 (inclusive) for numberOfTouTiers (servers providing flat rate pricing SHOULD set numberOfTouTiers to 0, as in practice there is no difference between having no tiers and having one tier).","owl:minCardinality":0},{"@id":"phase","@type":"rdf:Property","rdfs:domain":{"@id":"ReadingType"},"rdfs:range":{"@id":"PhaseCode"},"rdfs:comment":"Contains phase information associated with the type.","owl:minCardinality":0},{"@id":"powerOfTenMultiplier","@type":"rdf:Property","rdfs:domain":{"@id":"ReadingType"},"rdfs:range":{"@id":"PowerOfTenMultiplierType"},"rdfs:comment":"Indicates the power of ten multiplier applicable to the unit of measure of this ReadingType.","owl:minCardinality":0},{"@id":"subIntervalLength","@type":"rdf:Property","rdfs:domain":{"@id":"ReadingType"},"rdfs:range":{"@id":"UInt32"},"rdfs:comment":"Default sub-interval length specified in seconds for Readings of ReadingType. Some demand calculations are done over a number of smaller intervals. For example, in a rolling demand calculation, the demand value is defined as the rolling sum of smaller intervals over the intervalLength. The subintervalLength is the length of the smaller interval in this calculation. It SHALL be an integral division of the intervalLength. The number of sub-intervals can be calculated by dividing the intervalLength by the subintervalLength.","owl:minCardinality":0},{"@id":"supplyLimit","@type":"rdf:Property","rdfs:domain":{"@id":"ReadingType"},"rdfs:range":{"@id":"UInt48"},"rdfs:comment":"Reflects the supply limit set in the meter. This value can be compared to the Reading value to understand if limits are being approached or exceeded. Units follow the same definition as in this ReadingType.","owl:minCardinality":0},{"@id":"tieredConsumptionBlocks","@type":"rdf:Property","rdfs:domain":{"@id":"ReadingType"},"rdfs:range":"xsd:boolean","rdfs:comment":"Specifies whether or not the consumption blocks are differentiated by TOUTier or not. Default is false, if not specified.\ntrue = consumption accumulated over individual tiers\nfalse = consumption accumulated over all tiers","owl:minCardinality":0},{"@id":"uom","@type":"rdf:Property","rdfs:domain":{"@id":"ReadingType"},"rdfs:range":{"@id":"UomType"},"rdfs:comment":"Indicates the measurement type for the units of measure for the readings of this type.","owl:minCardinality":0},{"@id":"deviceLFDI","@type":"rdf:Property","rdfs:domain":{"@id":"UsagePoint"},"rdfs:range":{"@id":"HexBinary160"},"rdfs:comment":"The LFDI of the source device. This attribute SHALL be present when mirroring.","owl:minCardinality":0},{"@id":"MeterReadingListLink","@type":"rdf:Property","rdfs:domain":{"@id":"UsagePoint"},"rdfs:range":{"@id":"MeterReadingListLink"},"owl:minCardinality":0},{"@id":"UsagePoint","@type":"rdf:Property","rdfs:domain":{"@id":"UsagePointList"},"rdfs:range":{"@id":"UsagePoint"},"owl:minCardinality":0},{"@id":"pollRate","@type":"rdf:Property","rdfs:domain":{"@id":"UsagePointList"},"rdfs:range":{"@id":"UInt32"},"rdfs:comment":"The default polling rate for this function set (this resource and all resources below), in seconds. If not specified, a default of 900 seconds (15 minutes) is used. It is RECOMMENDED a client poll the resources of this function set every pollRate seconds.","owl:minCardinality":0},{"@id":"consumptionBlock","@type":"rdf:Property","rdfs:domain":{"@id":"ConsumptionTariffInterval"},"rdfs:range":{"@id":"ConsumptionBlockType"},"rdfs:comment":"Indicates the consumption block related to the reading. If not specified, is assumed to be \"0 - N/A\"."},{"@id":"EnvironmentalCost","@type":"rdf:Property","rdfs:domain":{"@id":"ConsumptionTariffInterval"},"rdfs:range":{"@id":"EnvironmentalCost"},"owl:minCardinality":0},{"@id":"price","@type":"rdf:Property","rdfs:domain":{"@id":"ConsumptionTariffInterval"},"rdfs:range":{"@id":"Int32"},"rdfs:comment":"The charge for this rate component, per unit of measure defined by the associated ReadingType, in currency specified in TariffProfile. \n\nThe Pricing service provider determines the appropriate price attribute value based on its applicable regulatory rules. For example, price could be net or inclusive of applicable taxes, fees, or levies.\n\nThe Billing function set provides the ability to represent billing information in a more detailed manner.","owl:minCardinality":0},{"@id":"startValue","@type":"rdf:Property","rdfs:domain":{"@id":"ConsumptionTariffInterval"},"rdfs:range":{"@id":"UInt48"},"rdfs:comment":"The lowest level of consumption that defines the starting point of this consumption step or block. Thresholds start at zero for each billing period.    \n\nIf specified, the first ConsumptionTariffInterval.startValue for a TimeTariffInteral instance SHALL begin at \"0.\" Subsequent ConsumptionTariffInterval.startValue elements SHALL be greater than the previous one."},{"@id":"ConsumptionTariffInterval","@type":"rdf:Property","rdfs:domain":{"@id":"ConsumptionTariffIntervalList"},"rdfs:range":{"@id":"ConsumptionTariffInterval"},"owl:minCardinality":0},{"@id":"amount","@type":"rdf:Property","rdfs:domain":{"@id":"EnvironmentalCost"},"rdfs:range":{"@id":"UInt32"},"rdfs:comment":"The estimated or actual environmental or other cost, per commodity unit defined by the ReadingType, for this RateComponent (e.g., grams of carbon dioxide emissions each per kWh)."},{"@id":"costKind","@type":"rdf:Property","rdfs:domain":{"@id":"EnvironmentalCost"},"rdfs:range":{"@id":"CostKindType"},"rdfs:comment":"The kind of cost referred to in the amount."},{"@id":"costLevel","@type":"rdf:Property","rdfs:domain":{"@id":"EnvironmentalCost"},"rdfs:range":{"@id":"UInt8"},"rdfs:comment":"The relative level of the amount attribute.  In conjunction with numCostLevels, this attribute informs a device of the relative scarcity of the amount attribute (e.g., a high or low availability of renewable generation).\n\nnumCostLevels and costLevel values SHALL ascend in order of scarcity, where \"0\" signals the lowest relative cost and higher values signal increasing cost.  For example, if numCostLevels is equal to \u201c3,\u201d then if the lowest relative costLevel were equal to \u201c0,\u201d devices would assume this is the lowest relative period to operate.  Likewise, if the costLevel in the next TimeTariffInterval instance is equal to \u201c1,\u201d then the device would assume it is relatively more expensive, in environmental terms, to operate during this TimeTariffInterval instance than the previous one.\n\nThere is no limit to the number of relative price levels other than that indicated in the attribute type, but for practicality, service providers should strive for simplicity and recognize the diminishing returns derived from increasing the numCostLevel value greater than four."},{"@id":"numCostLevels","@type":"rdf:Property","rdfs:domain":{"@id":"EnvironmentalCost"},"rdfs:range":{"@id":"UInt8"},"rdfs:comment":"The number of all relative cost levels. \n\nIn conjunction with costLevel, numCostLevels signals the relative scarcity of the commodity for the duration of the TimeTariffInterval instance (e.g., a relative indication of cost). This is useful in providing context for nominal cost signals to consumers or devices that might see a range of amount values from different service providres or from the same service provider."},{"@id":"ActiveTimeTariffIntervalListLink","@type":"rdf:Property","rdfs:domain":{"@id":"RateComponent"},"rdfs:range":{"@id":"ActiveTimeTariffIntervalListLink"},"owl:minCardinality":0},{"@id":"flowRateEndLimit","@type":"rdf:Property","rdfs:domain":{"@id":"RateComponent"},"rdfs:range":{"@id":"UnitValueType"},"rdfs:comment":"Specifies the maximum flow rate (e.g. kW for electricity) for which this RateComponent applies, for the usage point and given rate / tariff. \n\nIn combination with flowRateStartLimit, allows a service provider to define the demand or output characteristics for the particular tariff design.  If a server includes the flowRateEndLimit attribute, then it SHALL also include flowRateStartLimit attribute.\n\nFor example, a service provider\u2019s tariff limits customers to 20 kWs of demand for the given rate structure.  Above this threshold (from 20-50 kWs), there are different demand charges per unit of consumption.  The service provider can use flowRateStartLimit and flowRateEndLimit to describe the demand characteristics of the different rates.  Similarly, these attributes can be used to describe limits on premises DERs that might be producing a commodity and sending it back into the distribution network. \n\nNote: At the time of writing, service provider tariffs with demand-based components were not originally identified as being in scope, and service provider tariffs vary widely in their use of demand components and the method for computing charges.  It is expected that industry groups (e.g., OpenSG) will document requirements in the future that the IEEE 2030.5 community can then use as source material for the next version of IEEE 2030.5.","owl:minCardinality":0},{"@id":"flowRateStartLimit","@type":"rdf:Property","rdfs:domain":{"@id":"RateComponent"},"rdfs:range":{"@id":"UnitValueType"},"rdfs:comment":"Specifies the minimum flow rate (e.g., kW for electricity) for which this RateComponent applies, for the usage point and given rate / tariff.\n\nIn combination with flowRateEndLimit, allows a service provider to define the demand or output characteristics for the particular tariff design.  If a server includes the flowRateStartLimit attribute, then it SHALL also include flowRateEndLimit attribute.","owl:minCardinality":0},{"@id":"ReadingTypeLink","@type":"rdf:Property","rdfs:domain":{"@id":"RateComponent"},"rdfs:range":{"@id":"ReadingTypeLink"},"rdfs:comment":"Provides indication of the ReadingType with which this price is associated."},{"@id":"roleFlags","@type":"rdf:Property","rdfs:domain":{"@id":"RateComponent"},"rdfs:range":{"@id":"RoleFlagsType"},"rdfs:comment":"Specifies the roles that this usage point has been assigned."},{"@id":"TimeTariffIntervalListLink","@type":"rdf:Property","rdfs:domain":{"@id":"RateComponent"},"rdfs:range":{"@id":"TimeTariffIntervalListLink"}},{"@id":"RateComponent","@type":"rdf:Property","rdfs:domain":{"@id":"RateComponentList"},"rdfs:range":{"@id":"RateComponent"},"owl:minCardinality":0},{"@id":"currency","@type":"rdf:Property","rdfs:domain":{"@id":"TariffProfile"},"rdfs:range":{"@id":"CurrencyCode"},"rdfs:comment":"The currency code indicating the currency for this TariffProfile.","owl:minCardinality":0},{"@id":"pricePowerOfTenMultiplier","@type":"rdf:Property","rdfs:domain":{"@id":"TariffProfile"},"rdfs:range":{"@id":"PowerOfTenMultiplierType"},"rdfs:comment":"Indicates the power of ten multiplier for the price attribute.","owl:minCardinality":0},{"@id":"primacy","@type":"rdf:Property","rdfs:domain":{"@id":"TariffProfile"},"rdfs:range":{"@id":"PrimacyType"},"rdfs:comment":"Indicates the relative primacy of the provider of this program."},{"@id":"rateCode","@type":"rdf:Property","rdfs:domain":{"@id":"TariffProfile"},"rdfs:range":{"@id":"String20"},"rdfs:comment":"The rate code for this tariff profile.  Provided by the Pricing service provider per its internal business needs and practices and provides a method to identify the specific rate code for the TariffProfile instance.  This would typically not be communicated to the user except to facilitate troubleshooting due to its service provider-specific technical nature.","owl:minCardinality":0},{"@id":"RateComponentListLink","@type":"rdf:Property","rdfs:domain":{"@id":"TariffProfile"},"rdfs:range":{"@id":"RateComponentListLink"},"owl:minCardinality":0},{"@id":"serviceCategoryKind","@type":"rdf:Property","rdfs:domain":{"@id":"TariffProfile"},"rdfs:range":{"@id":"ServiceKind"},"rdfs:comment":"The kind of service provided by this usage point."},{"@id":"TariffProfile","@type":"rdf:Property","rdfs:domain":{"@id":"TariffProfileList"},"rdfs:range":{"@id":"TariffProfile"},"owl:minCardinality":0},{"@id":"pollRate","@type":"rdf:Property","rdfs:domain":{"@id":"TariffProfileList"},"rdfs:range":{"@id":"UInt32"},"rdfs:comment":"The default polling rate for this function set (this resource and all resources below), in seconds. If not specified, a default of 900 seconds (15 minutes) is used. It is RECOMMENDED a client poll the resources of this function set every pollRate seconds.","owl:minCardinality":0},{"@id":"ConsumptionTariffIntervalListLink","@type":"rdf:Property","rdfs:domain":{"@id":"TimeTariffInterval"},"rdfs:range":{"@id":"ConsumptionTariffIntervalListLink"},"owl:minCardinality":0},{"@id":"touTier","@type":"rdf:Property","rdfs:domain":{"@id":"TimeTariffInterval"},"rdfs:range":{"@id":"TOUType"},"rdfs:comment":"Indicates the time of use tier related to the reading. If not specified, is assumed to be \"0 - N/A\"."},{"@id":"TimeTariffInterval","@type":"rdf:Property","rdfs:domain":{"@id":"TimeTariffIntervalList"},"rdfs:range":{"@id":"TimeTariffInterval"},"owl:minCardinality":0},{"@id":"ActiveTextMessageListLink","@type":"rdf:Property","rdfs:domain":{"@id":"MessagingProgram"},"rdfs:range":{"@id":"ActiveTextMessageListLink"},"owl:minCardinality":0},{"@id":"locale","@type":"rdf:Property","rdfs:domain":{"@id":"MessagingProgram"},"rdfs:range":{"@id":"LocaleType"},"rdfs:comment":"Indicates the language and region of the messages in this collection."},{"@id":"primacy","@type":"rdf:Property","rdfs:domain":{"@id":"MessagingProgram"},"rdfs:range":{"@id":"PrimacyType"},"rdfs:comment":"Indicates the relative primacy of the provider of this program."},{"@id":"TextMessageListLink","@type":"rdf:Property","rdfs:domain":{"@id":"MessagingProgram"},"rdfs:range":{"@id":"TextMessageListLink"},"owl:minCardinality":0},{"@id":"MessagingProgram","@type":"rdf:Property","rdfs:domain":{"@id":"MessagingProgramList"},"rdfs:range":{"@id":"MessagingProgram"},"owl:minCardinality":0},{"@id":"pollRate","@type":"rdf:Property","rdfs:domain":{"@id":"MessagingProgramList"},"rdfs:range":{"@id":"UInt32"},"rdfs:comment":"The default polling rate for this function set (this resource and all resources below), in seconds. If not specified, a default of 900 seconds (15 minutes) is used. It is RECOMMENDED a client poll the resources of this function set every pollRate seconds.","owl:minCardinality":0},{"@id":"originator","@type":"rdf:Property","rdfs:domain":{"@id":"TextMessage"},"rdfs:range":{"@id":"String20"},"rdfs:comment":"Indicates the human-readable name of the publisher of the message","owl:minCardinality":0},{"@id":"priority","@type":"rdf:Property","rdfs:domain":{"@id":"TextMessage"},"rdfs:range":{"@id":"PriorityType"},"rdfs:comment":"The priority is used to inform the client of the priority of the particular message.  Devices with constrained or limited resources for displaying Messages should use this attribute to determine how to handle displaying currently active Messages (e.g. if a device uses a scrolling method with a single Message viewable at a time it MAY want to push a low priority Message to the background and bring a newly received higher priority Message to the foreground)."},{"@id":"textMessage","@type":"rdf:Property","rdfs:domain":{"@id":"TextMessage"},"rdfs:range":"xsd:string","rdfs:comment":"The textMessage attribute contains the actual UTF-8 encoded text to be displayed in conjunction with the messageLength attribute which contains the overall length of the textMessage attribute.  Clients and servers SHALL support a reception of a Message of 100 bytes in length.  Messages that exceed the clients display size will be left to the client to choose what method to handle the message (truncation, scrolling, etc.)."},{"@id":"TextMessage","@type":"rdf:Property","rdfs:domain":{"@id":"TextMessageList"},"rdfs:range":{"@id":"TextMessage"},"owl:minCardinality":0},{"@id":"billLastPeriod","@type":"rdf:Property","rdfs:domain":{"@id":"BillingPeriod"},"rdfs:range":{"@id":"Int48"},"rdfs:comment":"The amount of the bill for the previous billing period.","owl:minCardinality":0},{"@id":"billToDate","@type":"rdf:Property","rdfs:domain":{"@id":"BillingPeriod"},"rdfs:range":{"@id":"Int48"},"rdfs:comment":"The bill amount related to the billing period as of the statusTimeStamp.","owl:minCardinality":0},{"@id":"interval","@type":"rdf:Property","rdfs:domain":{"@id":"BillingPeriod"},"rdfs:range":{"@id":"DateTimeInterval"},"rdfs:comment":"The time interval for this billing period."},{"@id":"statusTimeStamp","@type":"rdf:Property","rdfs:domain":{"@id":"BillingPeriod"},"rdfs:range":{"@id":"TimeType"},"rdfs:comment":"The date / time of the last update of this resource.","owl:minCardinality":0},{"@id":"BillingPeriod","@type":"rdf:Property","rdfs:domain":{"@id":"BillingPeriodList"},"rdfs:range":{"@id":"BillingPeriod"},"owl:minCardinality":0},{"@id":"BillingReadingSetListLink","@type":"rdf:Property","rdfs:domain":{"@id":"BillingMeterReadingBase"},"rdfs:range":{"@id":"BillingReadingSetListLink"},"owl:minCardinality":0},{"@id":"ReadingTypeLink","@type":"rdf:Property","rdfs:domain":{"@id":"BillingMeterReadingBase"},"rdfs:range":{"@id":"ReadingTypeLink"},"owl:minCardinality":0},{"@id":"Charge","@type":"rdf:Property","rdfs:domain":{"@id":"BillingReading"},"rdfs:range":{"@id":"Charge"},"owl:minCardinality":0},{"@id":"BillingReading","@type":"rdf:Property","rdfs:domain":{"@id":"BillingReadingList"},"rdfs:range":{"@id":"BillingReading"},"owl:minCardinality":0},{"@id":"BillingReadingListLink","@type":"rdf:Property","rdfs:domain":{"@id":"BillingReadingSet"},"rdfs:range":{"@id":"BillingReadingListLink"},"owl:minCardinality":0},{"@id":"BillingReadingSet","@type":"rdf:Property","rdfs:domain":{"@id":"BillingReadingSetList"},"rdfs:range":{"@id":"BillingReadingSet"},"owl:minCardinality":0},{"@id":"description","@type":"rdf:Property","rdfs:domain":{"@id":"Charge"},"rdfs:range":{"@id":"String20"},"rdfs:comment":"A description of the charge.","owl:minCardinality":0},{"@id":"kind","@type":"rdf:Property","rdfs:domain":{"@id":"Charge"},"rdfs:range":{"@id":"ChargeKind"},"rdfs:comment":"The type (kind) of charge.","owl:minCardinality":0},{"@id":"value","@type":"rdf:Property","rdfs:domain":{"@id":"Charge"},"rdfs:range":{"@id":"Int32"},"rdfs:comment":"A monetary charge."},{"@id":"currency","@type":"rdf:Property","rdfs:domain":{"@id":"CustomerAccount"},"rdfs:range":{"@id":"UInt16"},"rdfs:comment":"The ISO 4217 code indicating the currency applicable to the bill amounts in the summary. See list at http://www.unece.org/cefact/recommendations/rec09/rec09_ecetrd203.pdf"},{"@id":"customerAccount","@type":"rdf:Property","rdfs:domain":{"@id":"CustomerAccount"},"rdfs:range":{"@id":"String42"},"rdfs:comment":"The account number for the customer (if applicable).","owl:minCardinality":0},{"@id":"CustomerAgreementListLink","@type":"rdf:Property","rdfs:domain":{"@id":"CustomerAccount"},"rdfs:range":{"@id":"CustomerAgreementListLink"},"owl:minCardinality":0},{"@id":"customerName","@type":"rdf:Property","rdfs:domain":{"@id":"CustomerAccount"},"rdfs:range":{"@id":"String42"},"rdfs:comment":"The name of the customer.","owl:minCardinality":0},{"@id":"pricePowerOfTenMultiplier","@type":"rdf:Property","rdfs:domain":{"@id":"CustomerAccount"},"rdfs:range":{"@id":"PowerOfTenMultiplierType"},"rdfs:comment":"Indicates the power of ten multiplier for the prices in this function set."},{"@id":"ServiceSupplierLink","@type":"rdf:Property","rdfs:domain":{"@id":"CustomerAccount"},"rdfs:range":{"@id":"ServiceSupplierLink"},"owl:minCardinality":0},{"@id":"CustomerAccount","@type":"rdf:Property","rdfs:domain":{"@id":"CustomerAccountList"},"rdfs:range":{"@id":"CustomerAccount"},"owl:minCardinality":0},{"@id":"pollRate","@type":"rdf:Property","rdfs:domain":{"@id":"CustomerAccountList"},"rdfs:range":{"@id":"UInt32"},"rdfs:comment":"The default polling rate for this function set (this resource and all resources below), in seconds. If not specified, a default of 900 seconds (15 minutes) is used. It is RECOMMENDED a client poll the resources of this function set every pollRate seconds.","owl:minCardinality":0},{"@id":"ActiveBillingPeriodListLink","@type":"rdf:Property","rdfs:domain":{"@id":"CustomerAgreement"},"rdfs:range":{"@id":"ActiveBillingPeriodListLink"},"owl:minCardinality":0},{"@id":"ActiveProjectionReadingListLink","@type":"rdf:Property","rdfs:domain":{"@id":"CustomerAgreement"},"rdfs:range":{"@id":"ActiveProjectionReadingListLink"},"owl:minCardinality":0},{"@id":"ActiveTargetReadingListLink","@type":"rdf:Property","rdfs:domain":{"@id":"CustomerAgreement"},"rdfs:range":{"@id":"ActiveTargetReadingListLink"},"owl:minCardinality":0},{"@id":"BillingPeriodListLink","@type":"rdf:Property","rdfs:domain":{"@id":"CustomerAgreement"},"rdfs:range":{"@id":"BillingPeriodListLink"},"owl:minCardinality":0},{"@id":"HistoricalReadingListLink","@type":"rdf:Property","rdfs:domain":{"@id":"CustomerAgreement"},"rdfs:range":{"@id":"HistoricalReadingListLink"},"owl:minCardinality":0},{"@id":"PrepaymentLink","@type":"rdf:Property","rdfs:domain":{"@id":"CustomerAgreement"},"rdfs:range":{"@id":"PrepaymentLink"},"owl:minCardinality":0},{"@id":"ProjectionReadingListLink","@type":"rdf:Property","rdfs:domain":{"@id":"CustomerAgreement"},"rdfs:range":{"@id":"ProjectionReadingListLink"},"owl:minCardinality":0},{"@id":"serviceAccount","@type":"rdf:Property","rdfs:domain":{"@id":"CustomerAgreement"},"rdfs:range":{"@id":"String42"},"rdfs:comment":"The account number of the service account (if applicable).","owl:minCardinality":0},{"@id":"serviceLocation","@type":"rdf:Property","rdfs:domain":{"@id":"CustomerAgreement"},"rdfs:range":{"@id":"String42"},"rdfs:comment":"The address or textual description of the service location.","owl:minCardinality":0},{"@id":"TargetReadingListLink","@type":"rdf:Property","rdfs:domain":{"@id":"CustomerAgreement"},"rdfs:range":{"@id":"TargetReadingListLink"},"owl:minCardinality":0},{"@id":"TariffProfileLink","@type":"rdf:Property","rdfs:domain":{"@id":"CustomerAgreement"},"rdfs:range":{"@id":"TariffProfileLink"},"owl:minCardinality":0},{"@id":"UsagePointLink","@type":"rdf:Property","rdfs:domain":{"@id":"CustomerAgreement"},"rdfs:range":{"@id":"UsagePointLink"},"owl:minCardinality":0},{"@id":"CustomerAgreement","@type":"rdf:Property","rdfs:domain":{"@id":"CustomerAgreementList"},"rdfs:range":{"@id":"CustomerAgreement"},"owl:minCardinality":0},{"@id":"HistoricalReading","@type":"rdf:Property","rdfs:domain":{"@id":"HistoricalReadingList"},"rdfs:range":{"@id":"HistoricalReading"},"owl:minCardinality":0},{"@id":"ProjectionReading","@type":"rdf:Property","rdfs:domain":{"@id":"ProjectionReadingList"},"rdfs:range":{"@id":"ProjectionReading"},"owl:minCardinality":0},{"@id":"TargetReading","@type":"rdf:Property","rdfs:domain":{"@id":"TargetReadingList"},"rdfs:range":{"@id":"TargetReading"},"owl:minCardinality":0},{"@id":"email","@type":"rdf:Property","rdfs:domain":{"@id":"ServiceSupplier"},"rdfs:range":{"@id":"String32"},"rdfs:comment":"E-mail address for this service supplier.","owl:minCardinality":0},{"@id":"phone","@type":"rdf:Property","rdfs:domain":{"@id":"ServiceSupplier"},"rdfs:range":{"@id":"String20"},"rdfs:comment":"Human-readable phone number for this service supplier.","owl:minCardinality":0},{"@id":"providerID","@type":"rdf:Property","rdfs:domain":{"@id":"ServiceSupplier"},"rdfs:range":{"@id":"UInt32"},"rdfs:comment":"Contains the IANA PEN for the commodity provider.","owl:minCardinality":0},{"@id":"web","@type":"rdf:Property","rdfs:domain":{"@id":"ServiceSupplier"},"rdfs:range":{"@id":"String42"},"rdfs:comment":"Website URI address for this service supplier.","owl:minCardinality":0},{"@id":"ServiceSupplier","@type":"rdf:Property","rdfs:domain":{"@id":"ServiceSupplierList"},"rdfs:range":{"@id":"ServiceSupplier"},"owl:minCardinality":0},{"@id":"availableCredit","@type":"rdf:Property","rdfs:domain":{"@id":"AccountBalance"},"rdfs:range":{"@id":"AccountingUnit"},"rdfs:comment":"AvailableCredit shows the balance of the sum of credits minus the sum of charges. In a Central Wallet mode this value may be passed down to the Prepayment server via an out-of-band mechanism. In Local or ESI modes, this value may be calculated based upon summation of CreditRegister transactions minus consumption charges calculated using Metering (and possibly Pricing) function set data. This value may be negative; for instance, if disconnection is prevented due to a Supply Interruption Override."},{"@id":"creditStatus","@type":"rdf:Property","rdfs:domain":{"@id":"AccountBalance"},"rdfs:range":{"@id":"CreditStatusType"},"rdfs:comment":"CreditStatus identifies whether the present value of availableCredit is considered OK, low, exhausted, or negative.","owl:minCardinality":0},{"@id":"emergencyCredit","@type":"rdf:Property","rdfs:domain":{"@id":"AccountBalance"},"rdfs:range":{"@id":"AccountingUnit"},"rdfs:comment":"EmergencyCredit is the amount of credit still available for the given service or commodity prepayment instance. If both availableCredit and emergyCredit are exhausted, then service will typically be disconnected.","owl:minCardinality":0},{"@id":"emergencyCreditStatus","@type":"rdf:Property","rdfs:domain":{"@id":"AccountBalance"},"rdfs:range":{"@id":"CreditStatusType"},"rdfs:comment":"EmergencyCreditStatus identifies whether the present value of emergencyCredit is considered OK, low, exhausted, or negative.","owl:minCardinality":0},{"@id":"energyUnit","@type":"rdf:Property","rdfs:domain":{"@id":"AccountingUnit"},"rdfs:range":{"@id":"RealEnergy"},"rdfs:comment":"Unit of service.","owl:minCardinality":0},{"@id":"monetaryUnit","@type":"rdf:Property","rdfs:domain":{"@id":"AccountingUnit"},"rdfs:range":{"@id":"CurrencyCode"},"rdfs:comment":"Unit of currency."},{"@id":"multiplier","@type":"rdf:Property","rdfs:domain":{"@id":"AccountingUnit"},"rdfs:range":{"@id":"PowerOfTenMultiplierType"},"rdfs:comment":"Multiplier for the 'energyUnit' or 'monetaryUnit'."},{"@id":"value","@type":"rdf:Property","rdfs:domain":{"@id":"AccountingUnit"},"rdfs:range":{"@id":"Int32"},"rdfs:comment":"Value of the monetary aspect"},{"@id":"creditAmount","@type":"rdf:Property","rdfs:domain":{"@id":"CreditRegister"},"rdfs:range":{"@id":"AccountingUnit"},"rdfs:comment":"CreditAmount is the amount of credit being added by a particular CreditRegister transaction. Negative values indicate that credit is being subtracted."},{"@id":"creditType","@type":"rdf:Property","rdfs:domain":{"@id":"CreditRegister"},"rdfs:range":{"@id":"CreditTypeType"},"rdfs:comment":"CreditType indicates whether the credit transaction applies to regular or emergency credit.","owl:minCardinality":0},{"@id":"effectiveTime","@type":"rdf:Property","rdfs:domain":{"@id":"CreditRegister"},"rdfs:range":{"@id":"TimeType"},"rdfs:comment":"EffectiveTime identifies the time at which the credit transaction goes into effect. For credit addition transactions, this is typically the moment at which the transaction takes place. For credit subtraction transactions, (e.g., non-fuel debt recovery transactions initiated from a back-haul or ESI) this may be a future time at which credit is deducted."},{"@id":"token","@type":"rdf:Property","rdfs:domain":{"@id":"CreditRegister"},"rdfs:range":{"@id":"String32"},"rdfs:comment":"Token is security data that authenticates the legitimacy of the transaction. The details of this token are not defined by IEEE 2030.5. How a Prepayment server handles this field is left as vendor specific implementation or will be defined by one or more other standards."},{"@id":"CreditRegister","@type":"rdf:Property","rdfs:domain":{"@id":"CreditRegisterList"},"rdfs:range":{"@id":"CreditRegister"},"owl:minCardinality":0},{"@id":"AccountBalanceLink","@type":"rdf:Property","rdfs:domain":{"@id":"Prepayment"},"rdfs:range":{"@id":"AccountBalanceLink"}},{"@id":"ActiveCreditRegisterListLink","@type":"rdf:Property","rdfs:domain":{"@id":"Prepayment"},"rdfs:range":{"@id":"ActiveCreditRegisterListLink"},"owl:minCardinality":0},{"@id":"ActiveSupplyInterruptionOverrideListLink","@type":"rdf:Property","rdfs:domain":{"@id":"Prepayment"},"rdfs:range":{"@id":"ActiveSupplyInterruptionOverrideListLink"},"owl:minCardinality":0},{"@id":"creditExpiryLevel","@type":"rdf:Property","rdfs:domain":{"@id":"Prepayment"},"rdfs:range":{"@id":"AccountingUnit"},"rdfs:comment":"CreditExpiryLevel is the set point for availableCredit at which the service level may be changed. The typical value for this attribute is 0, regardless of whether the account balance is measured in a monetary or commodity basis. The units for this attribute SHALL match the units used for availableCredit.","owl:minCardinality":0},{"@id":"CreditRegisterListLink","@type":"rdf:Property","rdfs:domain":{"@id":"Prepayment"},"rdfs:range":{"@id":"CreditRegisterListLink"}},{"@id":"lowCreditWarningLevel","@type":"rdf:Property","rdfs:domain":{"@id":"Prepayment"},"rdfs:range":{"@id":"AccountingUnit"},"rdfs:comment":"LowCreditWarningLevel is the set point for availableCredit at which the creditStatus attribute in the AccountBalance resource SHALL indicate that available credit is low. The units for this attribute SHALL match the units used for availableCredit. Typically, this value is set by the service provider.","owl:minCardinality":0},{"@id":"lowEmergencyCreditWarningLevel","@type":"rdf:Property","rdfs:domain":{"@id":"Prepayment"},"rdfs:range":{"@id":"AccountingUnit"},"rdfs:comment":"LowEmergencyCreditWarningLevel is the set point for emergencyCredit at which the creditStatus attribute in the AccountBalance resource SHALL indicate that emergencycredit is low. The units for this attribute SHALL match the units used for availableCredit. Typically, this value is set by the service provider.","owl:minCardinality":0},{"@id":"prepayMode","@type":"rdf:Property","rdfs:domain":{"@id":"Prepayment"},"rdfs:range":{"@id":"PrepayModeType"},"rdfs:comment":"PrepayMode specifies whether the given Prepayment instance is operating in Credit, Central Wallet, ESI, or Local prepayment mode. The Credit mode indicates that prepayment is not presently in effect. The other modes are described in the Overview Section above."},{"@id":"PrepayOperationStatusLink","@type":"rdf:Property","rdfs:domain":{"@id":"Prepayment"},"rdfs:range":{"@id":"PrepayOperationStatusLink"}},{"@id":"SupplyInterruptionOverrideListLink","@type":"rdf:Property","rdfs:domain":{"@id":"Prepayment"},"rdfs:range":{"@id":"SupplyInterruptionOverrideListLink"}},{"@id":"UsagePoint","@type":"rdf:Property","rdfs:domain":{"@id":"Prepayment"},"rdfs:range":{"@id":"UsagePoint"},"owl:minCardinality":0},{"@id":"UsagePointLink","@type":"rdf:Property","rdfs:domain":{"@id":"Prepayment"},"rdfs:range":{"@id":"UsagePointLink"},"owl:minCardinality":0},{"@id":"Prepayment","@type":"rdf:Property","rdfs:domain":{"@id":"PrepaymentList"},"rdfs:range":{"@id":"Prepayment"},"owl:minCardinality":0},{"@id":"pollRate","@type":"rdf:Property","rdfs:domain":{"@id":"PrepaymentList"},"rdfs:range":{"@id":"UInt32"},"rdfs:comment":"The default polling rate for this function set (this resource and all resources below), in seconds. If not specified, a default of 900 seconds (15 minutes) is used. It is RECOMMENDED a client poll the resources of this function set every pollRate seconds.","owl:minCardinality":0},{"@id":"creditTypeChange","@type":"rdf:Property","rdfs:domain":{"@id":"PrepayOperationStatus"},"rdfs:range":{"@id":"CreditTypeChange"},"rdfs:comment":"CreditTypeChange is used to define a pending change of creditTypeInUse, which will activate at a specified time.","owl:minCardinality":0},{"@id":"creditTypeInUse","@type":"rdf:Property","rdfs:domain":{"@id":"PrepayOperationStatus"},"rdfs:range":{"@id":"CreditTypeType"},"rdfs:comment":"CreditTypeInUse identifies whether the present mode of operation is consuming regular credit or emergency credit.","owl:minCardinality":0},{"@id":"serviceChange","@type":"rdf:Property","rdfs:domain":{"@id":"PrepayOperationStatus"},"rdfs:range":{"@id":"ServiceChange"},"rdfs:comment":"ServiceChange is used to define a pending change of serviceStatus, which will activate at a specified time.","owl:minCardinality":0},{"@id":"serviceStatus","@type":"rdf:Property","rdfs:domain":{"@id":"PrepayOperationStatus"},"rdfs:range":{"@id":"ServiceStatusType"},"rdfs:comment":"ServiceStatus identifies whether the service is connected or disconnected, or armed for connection or disconnection."},{"@id":"newStatus","@type":"rdf:Property","rdfs:domain":{"@id":"ServiceChange"},"rdfs:range":{"@id":"ServiceStatusType"},"rdfs:comment":"The new service status, to take effect at the time specified by startTime"},{"@id":"startTime","@type":"rdf:Property","rdfs:domain":{"@id":"ServiceChange"},"rdfs:range":{"@id":"TimeType"},"rdfs:comment":"The date/time when the change is to take effect."},{"@id":"description","@type":"rdf:Property","rdfs:domain":{"@id":"SupplyInterruptionOverride"},"rdfs:range":{"@id":"String32"},"rdfs:comment":"The description is a human readable text describing or naming the object.","owl:minCardinality":0},{"@id":"interval","@type":"rdf:Property","rdfs:domain":{"@id":"SupplyInterruptionOverride"},"rdfs:range":{"@id":"DateTimeInterval"},"rdfs:comment":"Interval defines the period of time during which supply should not be interrupted."},{"@id":"SupplyInterruptionOverride","@type":"rdf:Property","rdfs:domain":{"@id":"SupplyInterruptionOverrideList"},"rdfs:range":{"@id":"SupplyInterruptionOverride"},"owl:minCardinality":0},{"@id":"newType","@type":"rdf:Property","rdfs:domain":{"@id":"CreditTypeChange"},"rdfs:range":{"@id":"CreditTypeType"},"rdfs:comment":"The new credit type, to take effect at the time specified by startTime"},{"@id":"startTime","@type":"rdf:Property","rdfs:domain":{"@id":"CreditTypeChange"},"rdfs:range":{"@id":"TimeType"},"rdfs:comment":"The date/time when the change is to take effect."},{"@id":"dateTime","@type":"rdf:Property","rdfs:domain":{"@id":"RequestStatus"},"rdfs:range":{"@id":"TimeType"},"rdfs:comment":"The dateTime attribute will provide a timestamp of when the request status was set. dateTime MUST be set to the time at which the status change occurred, not a time in the future or past."},{"@id":"requestStatus","@type":"rdf:Property","rdfs:domain":{"@id":"RequestStatus"},"rdfs:range":{"@id":"UInt8"},"rdfs:comment":"Field representing the request status type. \n0 = Requested\n1 = Cancelled\nAll other values reserved."},{"@id":"creationTime","@type":"rdf:Property","rdfs:domain":{"@id":"FlowReservationRequest"},"rdfs:range":{"@id":"TimeType"},"rdfs:comment":"The time at which the request was created."},{"@id":"durationRequested","@type":"rdf:Property","rdfs:domain":{"@id":"FlowReservationRequest"},"rdfs:range":{"@id":"UInt16"},"rdfs:comment":"A value that is calculated by the storage device that defines the minimum duration, in seconds, that it will take to complete the actual flow transaction, including any ramp times and conditioning times, if applicable.","owl:minCardinality":0},{"@id":"energyRequested","@type":"rdf:Property","rdfs:domain":{"@id":"FlowReservationRequest"},"rdfs:range":{"@id":"SignedRealEnergy"},"rdfs:comment":"Indicates the total amount of energy, in Watt-Hours, requested to be transferred between the storage device and the electric power system. Positive values indicate charging and negative values indicate discharging. This sign convention is different than for the DER function where discharging is positive.  Note that the energyRequestNow attribute in the PowerStatus Object must always represent a charging solution and it is not allowed to have a negative value."},{"@id":"intervalRequested","@type":"rdf:Property","rdfs:domain":{"@id":"FlowReservationRequest"},"rdfs:range":{"@id":"DateTimeInterval"},"rdfs:comment":"The time window during which the flow reservation is needed. For example, if an electric vehicle is set with a 7:00 AM time charge is needed, and price drops to the lowest tier at 11:00 PM, then this window would likely be from 11:00 PM until 7:00 AM."},{"@id":"powerRequested","@type":"rdf:Property","rdfs:domain":{"@id":"FlowReservationRequest"},"rdfs:range":{"@id":"ActivePower"},"rdfs:comment":"Indicates the sustained level of power, in Watts, that is requested. For charging this is calculated by the storage device and it represents the charging system capability (which for an electric vehicle must also account for any power limitations due to the EVSE control pilot). For discharging, a lower value than the inverter capability can be used as a target."},{"@id":"RequestStatus","@type":"rdf:Property","rdfs:domain":{"@id":"FlowReservationRequest"},"rdfs:range":{"@id":"RequestStatus"}},{"@id":"FlowReservationRequest","@type":"rdf:Property","rdfs:domain":{"@id":"FlowReservationRequestList"},"rdfs:range":{"@id":"FlowReservationRequest"},"owl:minCardinality":0},{"@id":"pollRate","@type":"rdf:Property","rdfs:domain":{"@id":"FlowReservationRequestList"},"rdfs:range":{"@id":"UInt32"},"rdfs:comment":"The default polling rate for this function set (this resource and all resources below), in seconds. If not specified, a default of 900 seconds (15 minutes) is used. It is RECOMMENDED a client poll the resources of this function set every pollRate seconds.","owl:minCardinality":0},{"@id":"energyAvailable","@type":"rdf:Property","rdfs:domain":{"@id":"FlowReservationResponse"},"rdfs:range":{"@id":"SignedRealEnergy"},"rdfs:comment":"Indicates the amount of energy available."},{"@id":"powerAvailable","@type":"rdf:Property","rdfs:domain":{"@id":"FlowReservationResponse"},"rdfs:range":{"@id":"ActivePower"},"rdfs:comment":"Indicates the amount of power available."},{"@id":"subject","@type":"rdf:Property","rdfs:domain":{"@id":"FlowReservationResponse"},"rdfs:range":{"@id":"mRIDType"},"rdfs:comment":"The subject field provides a method to match the response with the originating event. It is populated with the mRID of the corresponding FlowReservationRequest object."},{"@id":"FlowReservationResponse","@type":"rdf:Property","rdfs:domain":{"@id":"FlowReservationResponseList"},"rdfs:range":{"@id":"FlowReservationResponse"},"owl:minCardinality":0},{"@id":"pollRate","@type":"rdf:Property","rdfs:domain":{"@id":"FlowReservationResponseList"},"rdfs:range":{"@id":"UInt32"},"rdfs:comment":"The default polling rate for this function set (this resource and all resources below), in seconds. If not specified, a default of 900 seconds (15 minutes) is used. It is RECOMMENDED a client poll the resources of this function set every pollRate seconds.","owl:minCardinality":0},{"@id":"DERControlBase","@type":"rdf:Property","rdfs:domain":{"@id":"DefaultDERControl"},"rdfs:range":{"@id":"DERControlBase"}},{"@id":"setESDelay","@type":"rdf:Property","rdfs:domain":{"@id":"DefaultDERControl"},"rdfs:range":{"@id":"UInt32"},"rdfs:comment":"Enter service delay, in hundredths of a second. When present, this value SHALL update the value of the corresponding setting (DERSettings::setESDelay).","owl:minCardinality":0},{"@id":"setESHighFreq","@type":"rdf:Property","rdfs:domain":{"@id":"DefaultDERControl"},"rdfs:range":{"@id":"UInt16"},"rdfs:comment":"Enter service frequency high. Specified in hundredths of Hz. When present, this value SHALL update the value of the corresponding setting (DERSettings::setESHighFreq).","owl:minCardinality":0},{"@id":"setESHighVolt","@type":"rdf:Property","rdfs:domain":{"@id":"DefaultDERControl"},"rdfs:range":{"@id":"Int16"},"rdfs:comment":"Enter service voltage high. Specified as an effective percent voltage, defined as (100% * (locally measured voltage - setVRefOfs) / setVRef), in hundredths of a percent. When present, this value SHALL update the value of the corresponding setting (DERSettings::setESHighVolt).","owl:minCardinality":0},{"@id":"setESLowFreq","@type":"rdf:Property","rdfs:domain":{"@id":"DefaultDERControl"},"rdfs:range":{"@id":"UInt16"},"rdfs:comment":"Enter service frequency low. Specified in hundredths of Hz. When present, this value SHALL update the value of the corresponding setting (DERSettings::setESLowFreq).","owl:minCardinality":0},{"@id":"setESLowVolt","@type":"rdf:Property","rdfs:domain":{"@id":"DefaultDERControl"},"rdfs:range":{"@id":"Int16"},"rdfs:comment":"Enter service voltage low. Specified as an effective percent voltage, defined as (100% * (locally measured voltage - setVRefOfs) / setVRef), in hundredths of a percent. When present, this value SHALL update the value of the corresponding setting (DERSettings::setESLowVolt).","owl:minCardinality":0},{"@id":"setESRampTms","@type":"rdf:Property","rdfs:domain":{"@id":"DefaultDERControl"},"rdfs:range":{"@id":"UInt32"},"rdfs:comment":"Enter service ramp time, in hundredths of a second. When present, this value SHALL update the value of the corresponding setting (DERSettings::setESRampTms).","owl:minCardinality":0},{"@id":"setESRandomDelay","@type":"rdf:Property","rdfs:domain":{"@id":"DefaultDERControl"},"rdfs:range":{"@id":"UInt32"},"rdfs:comment":"Enter service randomized delay, in hundredths of a second. When present, this value SHALL update the value of the corresponding setting (DERSettings::setESRandomDelay).","owl:minCardinality":0},{"@id":"setGradW","@type":"rdf:Property","rdfs:domain":{"@id":"DefaultDERControl"},"rdfs:range":{"@id":"UInt16"},"rdfs:comment":"Set default rate of change (ramp rate) of active power output due to command or internal action, defined in %setWMax / second.  Resolution is in hundredths of a percent/second. A value of 0 means there is no limit. Interpreted as a percentage change in output capability limit per second when used as a default ramp rate. When present, this value SHALL update the value of the corresponding setting (DERSettings::setGradW).","owl:minCardinality":0},{"@id":"setSoftGradW","@type":"rdf:Property","rdfs:domain":{"@id":"DefaultDERControl"},"rdfs:range":{"@id":"UInt16"},"rdfs:comment":"Set soft-start rate of change (soft-start ramp rate) of active power output due to command or internal action, defined in %setWMax / second.  Resolution is in hundredths of a percent/second. A value of 0 means there is no limit. Interpreted as a percentage change in output capability limit per second when used as a ramp rate. When present, this value SHALL update the value of the corresponding setting (DERSettings::setSoftGradW).","owl:minCardinality":0},{"@id":"dBOF","@type":"rdf:Property","rdfs:domain":{"@id":"FreqDroopType"},"rdfs:range":{"@id":"UInt32"},"rdfs:comment":"Frequency droop dead band for over-frequency conditions. In thousandths of Hz."},{"@id":"dBUF","@type":"rdf:Property","rdfs:domain":{"@id":"FreqDroopType"},"rdfs:range":{"@id":"UInt32"},"rdfs:comment":"Frequency droop dead band for under-frequency conditions. In thousandths of Hz."},{"@id":"kOF","@type":"rdf:Property","rdfs:domain":{"@id":"FreqDroopType"},"rdfs:range":{"@id":"UInt16"},"rdfs:comment":"Frequency droop per-unit frequency change for over-frequency conditions corresponding to 1 per-unit power output change. In thousandths, unitless."},{"@id":"kUF","@type":"rdf:Property","rdfs:domain":{"@id":"FreqDroopType"},"rdfs:range":{"@id":"UInt16"},"rdfs:comment":"Frequency droop per-unit frequency change for under-frequency conditions corresponding to 1 per-unit power output change. In thousandths, unitless."},{"@id":"openLoopTms","@type":"rdf:Property","rdfs:domain":{"@id":"FreqDroopType"},"rdfs:range":{"@id":"UInt16"},"rdfs:comment":"Open loop response time, the duration from a step change in control signal input until the output changes by 90% of its final change before any overshoot, in hundredths of a second. Resolution is 1/100 sec. A value of 0 is used to mean no limit."},{"@id":"AssociatedDERProgramListLink","@type":"rdf:Property","rdfs:domain":{"@id":"DER"},"rdfs:range":{"@id":"AssociatedDERProgramListLink"},"owl:minCardinality":0},{"@id":"AssociatedUsagePointLink","@type":"rdf:Property","rdfs:domain":{"@id":"DER"},"rdfs:range":{"@id":"AssociatedUsagePointLink"},"owl:minCardinality":0},{"@id":"CurrentDERProgramLink","@type":"rdf:Property","rdfs:domain":{"@id":"DER"},"rdfs:range":{"@id":"CurrentDERProgramLink"},"owl:minCardinality":0},{"@id":"DERAvailabilityLink","@type":"rdf:Property","rdfs:domain":{"@id":"DER"},"rdfs:range":{"@id":"DERAvailabilityLink"},"owl:minCardinality":0},{"@id":"DERCapabilityLink","@type":"rdf:Property","rdfs:domain":{"@id":"DER"},"rdfs:range":{"@id":"DERCapabilityLink"},"owl:minCardinality":0},{"@id":"DERSettingsLink","@type":"rdf:Property","rdfs:domain":{"@id":"DER"},"rdfs:range":{"@id":"DERSettingsLink"},"owl:minCardinality":0},{"@id":"DERStatusLink","@type":"rdf:Property","rdfs:domain":{"@id":"DER"},"rdfs:range":{"@id":"DERStatusLink"},"owl:minCardinality":0},{"@id":"DER","@type":"rdf:Property","rdfs:domain":{"@id":"DERList"},"rdfs:range":{"@id":"DER"},"owl:minCardinality":0},{"@id":"pollRate","@type":"rdf:Property","rdfs:domain":{"@id":"DERList"},"rdfs:range":{"@id":"UInt32"},"rdfs:comment":"The default polling rate for this function set (this resource and all resources below), in seconds. If not specified, a default of 900 seconds (15 minutes) is used. It is RECOMMENDED a client poll the resources of this function set every pollRate seconds.","owl:minCardinality":0},{"@id":"modesEnabled","@type":"rdf:Property","rdfs:domain":{"@id":"DERSettings"},"rdfs:range":{"@id":"DERControlType"},"rdfs:comment":"Bitmap indicating the DER Controls enabled on the device. See DERControlType for values. If a control is supported (see DERCapability::modesSupported), but not enabled, the control will not be executed if encountered.","owl:minCardinality":0},{"@id":"setESDelay","@type":"rdf:Property","rdfs:domain":{"@id":"DERSettings"},"rdfs:range":{"@id":"UInt32"},"rdfs:comment":"Enter service delay, in hundredths of a second.","owl:minCardinality":0},{"@id":"setESHighFreq","@type":"rdf:Property","rdfs:domain":{"@id":"DERSettings"},"rdfs:range":{"@id":"UInt16"},"rdfs:comment":"Enter service frequency high. Specified in hundredths of Hz.","owl:minCardinality":0},{"@id":"setESHighVolt","@type":"rdf:Property","rdfs:domain":{"@id":"DERSettings"},"rdfs:range":{"@id":"Int16"},"rdfs:comment":"Enter service voltage high. Specified as an effective percent voltage, defined as (100% * (locally measured voltage - setVRefOfs) / setVRef), in hundredths of a percent.","owl:minCardinality":0},{"@id":"setESLowFreq","@type":"rdf:Property","rdfs:domain":{"@id":"DERSettings"},"rdfs:range":{"@id":"UInt16"},"rdfs:comment":"Enter service frequency low. Specified in hundredths of Hz.","owl:minCardinality":0},{"@id":"setESLowVolt","@type":"rdf:Property","rdfs:domain":{"@id":"DERSettings"},"rdfs:range":{"@id":"Int16"},"rdfs:comment":"Enter service voltage low. Specified as an effective percent voltage, defined as (100% * (locally measured voltage - setVRefOfs) / setVRef), in hundredths of a percent.","owl:minCardinality":0},{"@id":"setESRampTms","@type":"rdf:Property","rdfs:domain":{"@id":"DERSettings"},"rdfs:range":{"@id":"UInt32"},"rdfs:comment":"Enter service ramp time, in hundredths of a second.","owl:minCardinality":0},{"@id":"setESRandomDelay","@type":"rdf:Property","rdfs:domain":{"@id":"DERSettings"},"rdfs:range":{"@id":"UInt32"},"rdfs:comment":"Enter service randomized delay, in hundredths of a second.","owl:minCardinality":0},{"@id":"setGradW","@type":"rdf:Property","rdfs:domain":{"@id":"DERSettings"},"rdfs:range":{"@id":"UInt16"},"rdfs:comment":"Set default rate of change (ramp rate) of active power output due to command or internal action, defined in %setWMax / second.  Resolution is in hundredths of a percent/second. A value of 0 means there is no limit. Interpreted as a percentage change in output capability limit per second when used as a default ramp rate."},{"@id":"setMaxA","@type":"rdf:Property","rdfs:domain":{"@id":"DERSettings"},"rdfs:range":{"@id":"CurrentRMS"},"rdfs:comment":"AC current maximum. Maximum AC current in RMS Amperes.","owl:minCardinality":0},{"@id":"setMaxAh","@type":"rdf:Property","rdfs:domain":{"@id":"DERSettings"},"rdfs:range":{"@id":"AmpereHour"},"rdfs:comment":"Maximum usable energy storage capacity of the DER, in AmpHours. Note: this may be different from physical capability.","owl:minCardinality":0},{"@id":"setMaxChargeRateVA","@type":"rdf:Property","rdfs:domain":{"@id":"DERSettings"},"rdfs:range":{"@id":"ApparentPower"},"rdfs:comment":"Apparent power charge maximum. Maximum apparent power the DER can absorb from the grid in Volt-Amperes. May differ from the apparent power maximum (setMaxVA).","owl:minCardinality":0},{"@id":"setMaxChargeRateW","@type":"rdf:Property","rdfs:domain":{"@id":"DERSettings"},"rdfs:range":{"@id":"ActivePower"},"rdfs:comment":"Maximum rate of energy transfer received by the storage device, in Watts. Defaults to rtgMaxChargeRateW.","owl:minCardinality":0},{"@id":"setMaxDischargeRateVA","@type":"rdf:Property","rdfs:domain":{"@id":"DERSettings"},"rdfs:range":{"@id":"ApparentPower"},"rdfs:comment":"Apparent power discharge maximum. Maximum apparent power the DER can deliver to the grid in Volt-Amperes. May differ from the apparent power maximum (setMaxVA).","owl:minCardinality":0},{"@id":"setMaxDischargeRateW","@type":"rdf:Property","rdfs:domain":{"@id":"DERSettings"},"rdfs:range":{"@id":"ActivePower"},"rdfs:comment":"Maximum rate of energy transfer delivered by the storage device, in Watts. Defaults to rtgMaxDischargeRateW.","owl:minCardinality":0},{"@id":"setMaxV","@type":"rdf:Property","rdfs:domain":{"@id":"DERSettings"},"rdfs:range":{"@id":"VoltageRMS"},"rdfs:comment":"AC voltage maximum setting.","owl:minCardinality":0},{"@id":"setMaxVA","@type":"rdf:Property","rdfs:domain":{"@id":"DERSettings"},"rdfs:range":{"@id":"ApparentPower"},"rdfs:comment":"Set limit for maximum apparent power capability of the DER (in VA). Defaults to rtgMaxVA.","owl:minCardinality":0},{"@id":"setMaxVar","@type":"rdf:Property","rdfs:domain":{"@id":"DERSettings"},"rdfs:range":{"@id":"ReactivePower"},"rdfs:comment":"Set limit for maximum reactive power delivered by the DER (in var). SHALL be a positive value &lt;= rtgMaxVar (default).","owl:minCardinality":0},{"@id":"setMaxVarNeg","@type":"rdf:Property","rdfs:domain":{"@id":"DERSettings"},"rdfs:range":{"@id":"ReactivePower"},"rdfs:comment":"Set limit for maximum reactive power received by the DER (in var). If present, SHALL be a negative value &gt;= rtgMaxVarNeg (default). If absent, defaults to negative setMaxVar.","owl:minCardinality":0},{"@id":"setMaxW","@type":"rdf:Property","rdfs:domain":{"@id":"DERSettings"},"rdfs:range":{"@id":"ActivePower"},"rdfs:comment":"Set limit for maximum active power capability of the DER (in W). Defaults to rtgMaxW."},{"@id":"setMaxWh","@type":"rdf:Property","rdfs:domain":{"@id":"DERSettings"},"rdfs:range":{"@id":"WattHour"},"rdfs:comment":"Maximum energy storage capacity of the DER, in WattHours. Note: this may be different from physical capability.","owl:minCardinality":0},{"@id":"setMinPFOverExcited","@type":"rdf:Property","rdfs:domain":{"@id":"DERSettings"},"rdfs:range":{"@id":"PowerFactor"},"rdfs:comment":"Set minimum Power Factor displacement limit of the DER when injecting reactive power (over-excited); SHALL be a positive value between 0.0 (typically &gt; 0.7) and 1.0.  SHALL be &gt;= rtgMinPFOverExcited (default).","owl:minCardinality":0},{"@id":"setMinPFUnderExcited","@type":"rdf:Property","rdfs:domain":{"@id":"DERSettings"},"rdfs:range":{"@id":"PowerFactor"},"rdfs:comment":"Set minimum Power Factor displacement limit of the DER when absorbing reactive power (under-excited); SHALL be a positive value between 0.0 (typically &gt; 0.7) and 0.9999.  If present, SHALL be &gt;= rtgMinPFUnderExcited (default).  If absent, defaults to setMinPFOverExcited.","owl:minCardinality":0},{"@id":"setMinV","@type":"rdf:Property","rdfs:domain":{"@id":"DERSettings"},"rdfs:range":{"@id":"VoltageRMS"},"rdfs:comment":"AC voltage minimum setting.","owl:minCardinality":0},{"@id":"setSoftGradW","@type":"rdf:Property","rdfs:domain":{"@id":"DERSettings"},"rdfs:range":{"@id":"UInt16"},"rdfs:comment":"Set soft-start rate of change (soft-start ramp rate) of active power output due to command or internal action, defined in %setWMax / second.  Resolution is in hundredths of a percent/second. A value of 0 means there is no limit. Interpreted as a percentage change in output capability limit per second when used as a ramp rate.","owl:minCardinality":0},{"@id":"setVNom","@type":"rdf:Property","rdfs:domain":{"@id":"DERSettings"},"rdfs:range":{"@id":"VoltageRMS"},"rdfs:comment":"AC voltage nominal setting.","owl:minCardinality":0},{"@id":"setVRef","@type":"rdf:Property","rdfs:domain":{"@id":"DERSettings"},"rdfs:range":{"@id":"VoltageRMS"},"rdfs:comment":"The nominal AC voltage (RMS) at the utility's point of common coupling.","owl:minCardinality":0},{"@id":"setVRefOfs","@type":"rdf:Property","rdfs:domain":{"@id":"DERSettings"},"rdfs:range":{"@id":"VoltageRMS"},"rdfs:comment":"The nominal AC voltage (RMS) offset between the DER's electrical connection point and the utility's point of common coupling.","owl:minCardinality":0},{"@id":"updatedTime","@type":"rdf:Property","rdfs:domain":{"@id":"DERSettings"},"rdfs:range":{"@id":"TimeType"},"rdfs:comment":"Specifies the time at which the DER information was last updated."},{"@id":"availabilityDuration","@type":"rdf:Property","rdfs:domain":{"@id":"DERAvailability"},"rdfs:range":{"@id":"UInt32"},"rdfs:comment":"Indicates number of seconds the DER will be able to deliver active power at the reservePercent level.","owl:minCardinality":0},{"@id":"maxChargeDuration","@type":"rdf:Property","rdfs:domain":{"@id":"DERAvailability"},"rdfs:range":{"@id":"UInt32"},"rdfs:comment":"Indicates number of seconds the DER will be able to receive active power at the reserveChargePercent level.","owl:minCardinality":0},{"@id":"readingTime","@type":"rdf:Property","rdfs:domain":{"@id":"DERAvailability"},"rdfs:range":{"@id":"TimeType"},"rdfs:comment":"The timestamp when the DER availability was last updated."},{"@id":"reserveChargePercent","@type":"rdf:Property","rdfs:domain":{"@id":"DERAvailability"},"rdfs:range":{"@id":"PerCent"},"rdfs:comment":"Percent of continuous received active power (%setMaxChargeRateW) that is estimated to be available in reserve.","owl:minCardinality":0},{"@id":"reservePercent","@type":"rdf:Property","rdfs:domain":{"@id":"DERAvailability"},"rdfs:range":{"@id":"PerCent"},"rdfs:comment":"Percent of continuous delivered active power (%setMaxW) that is estimated to be available in reserve.","owl:minCardinality":0},{"@id":"statVarAvail","@type":"rdf:Property","rdfs:domain":{"@id":"DERAvailability"},"rdfs:range":{"@id":"ReactivePower"},"rdfs:comment":"Estimated reserve reactive power, in var.  Represents the lesser of received or delivered reactive power.","owl:minCardinality":0},{"@id":"statWAvail","@type":"rdf:Property","rdfs:domain":{"@id":"DERAvailability"},"rdfs:range":{"@id":"ActivePower"},"rdfs:comment":"Estimated reserve active power, in watts.","owl:minCardinality":0},{"@id":"modesSupported","@type":"rdf:Property","rdfs:domain":{"@id":"DERCapability"},"rdfs:range":{"@id":"DERControlType"},"rdfs:comment":"Bitmap indicating the DER Controls implemented by the device. See DERControlType for values."},{"@id":"rtgAbnormalCategory","@type":"rdf:Property","rdfs:domain":{"@id":"DERCapability"},"rdfs:range":{"@id":"UInt8"},"rdfs:comment":"Abnormal operating performance category as defined by IEEE 1547-2018. One of:\n0 - not specified\n1 - Category I\n2 - Category II\n3 - Category III\nAll other values reserved.","owl:minCardinality":0},{"@id":"rtgMaxA","@type":"rdf:Property","rdfs:domain":{"@id":"DERCapability"},"rdfs:range":{"@id":"CurrentRMS"},"rdfs:comment":"Maximum continuous AC current capability of the DER, in Amperes (RMS).","owl:minCardinality":0},{"@id":"rtgMaxAh","@type":"rdf:Property","rdfs:domain":{"@id":"DERCapability"},"rdfs:range":{"@id":"AmpereHour"},"rdfs:comment":"Usable energy storage capacity of the DER, in AmpHours.","owl:minCardinality":0},{"@id":"rtgMaxChargeRateVA","@type":"rdf:Property","rdfs:domain":{"@id":"DERCapability"},"rdfs:range":{"@id":"ApparentPower"},"rdfs:comment":"Maximum apparent power charge rating in Volt-Amperes. May differ from the maximum apparent power rating.","owl:minCardinality":0},{"@id":"rtgMaxChargeRateW","@type":"rdf:Property","rdfs:domain":{"@id":"DERCapability"},"rdfs:range":{"@id":"ActivePower"},"rdfs:comment":"Maximum rate of energy transfer received by the storage DER, in Watts.","owl:minCardinality":0},{"@id":"rtgMaxDischargeRateVA","@type":"rdf:Property","rdfs:domain":{"@id":"DERCapability"},"rdfs:range":{"@id":"ApparentPower"},"rdfs:comment":"Maximum apparent power discharge rating in Volt-Amperes. May differ from the maximum apparent power rating.","owl:minCardinality":0},{"@id":"rtgMaxDischargeRateW","@type":"rdf:Property","rdfs:domain":{"@id":"DERCapability"},"rdfs:range":{"@id":"ActivePower"},"rdfs:comment":"Maximum rate of energy transfer delivered by the storage DER, in Watts. Required for combined generation/storage DERs (e.g. DERType == 83).","owl:minCardinality":0},{"@id":"rtgMaxV","@type":"rdf:Property","rdfs:domain":{"@id":"DERCapability"},"rdfs:range":{"@id":"VoltageRMS"},"rdfs:comment":"AC voltage maximum rating.","owl:minCardinality":0},{"@id":"rtgMaxVA","@type":"rdf:Property","rdfs:domain":{"@id":"DERCapability"},"rdfs:range":{"@id":"ApparentPower"},"rdfs:comment":"Maximum continuous apparent power output capability of the DER, in VA.","owl:minCardinality":0},{"@id":"rtgMaxVar","@type":"rdf:Property","rdfs:domain":{"@id":"DERCapability"},"rdfs:range":{"@id":"ReactivePower"},"rdfs:comment":"Maximum continuous reactive power delivered by the DER, in var.","owl:minCardinality":0},{"@id":"rtgMaxVarNeg","@type":"rdf:Property","rdfs:domain":{"@id":"DERCapability"},"rdfs:range":{"@id":"ReactivePower"},"rdfs:comment":"Maximum continuous reactive power received by the DER, in var.  If absent, defaults to negative rtgMaxVar.","owl:minCardinality":0},{"@id":"rtgMaxW","@type":"rdf:Property","rdfs:domain":{"@id":"DERCapability"},"rdfs:range":{"@id":"ActivePower"},"rdfs:comment":"Maximum continuous active power output capability of the DER, in watts. Represents combined generation plus storage output if DERType == 83."},{"@id":"rtgMaxWh","@type":"rdf:Property","rdfs:domain":{"@id":"DERCapability"},"rdfs:range":{"@id":"WattHour"},"rdfs:comment":"Maximum energy storage capacity of the DER, in WattHours.","owl:minCardinality":0},{"@id":"rtgMinPFOverExcited","@type":"rdf:Property","rdfs:domain":{"@id":"DERCapability"},"rdfs:range":{"@id":"PowerFactor"},"rdfs:comment":"Minimum Power Factor displacement capability of the DER when injecting reactive power (over-excited); SHALL be a positive value between 0.0 (typically &gt; 0.7) and 1.0. If absent, defaults to unity.","owl:minCardinality":0},{"@id":"rtgMinPFUnderExcited","@type":"rdf:Property","rdfs:domain":{"@id":"DERCapability"},"rdfs:range":{"@id":"PowerFactor"},"rdfs:comment":"Minimum Power Factor displacement capability of the DER when absorbing reactive power (under-excited); SHALL be a positive value between 0.0 (typically &gt; 0.7) and 0.9999.  If absent, defaults to rtgMinPFOverExcited.","owl:minCardinality":0},{"@id":"rtgMinV","@type":"rdf:Property","rdfs:domain":{"@id":"DERCapability"},"rdfs:range":{"@id":"VoltageRMS"},"rdfs:comment":"AC voltage minimum rating.","owl:minCardinality":0},{"@id":"rtgNormalCategory","@type":"rdf:Property","rdfs:domain":{"@id":"DERCapability"},"rdfs:range":{"@id":"UInt8"},"rdfs:comment":"Normal operating performance category as defined by IEEE 1547-2018. One of:\n0 - not specified\n1 - Category A\n2 - Category B\nAll other values reserved.","owl:minCardinality":0},{"@id":"rtgOverExcitedPF","@type":"rdf:Property","rdfs:domain":{"@id":"DERCapability"},"rdfs:range":{"@id":"PowerFactor"},"rdfs:comment":"Specified over-excited power factor.","owl:minCardinality":0},{"@id":"rtgOverExcitedW","@type":"rdf:Property","rdfs:domain":{"@id":"DERCapability"},"rdfs:range":{"@id":"ActivePower"},"rdfs:comment":"Active power rating in Watts at specified over-excited power factor (rtgOverExcitedPF). If present, rtgOverExcitedPF SHALL be present.","owl:minCardinality":0},{"@id":"rtgReactiveSusceptance","@type":"rdf:Property","rdfs:domain":{"@id":"DERCapability"},"rdfs:range":{"@id":"ReactiveSusceptance"},"rdfs:comment":"Reactive susceptance that remains connected to the Area EPS in the cease to energize and trip state.","owl:minCardinality":0},{"@id":"rtgUnderExcitedPF","@type":"rdf:Property","rdfs:domain":{"@id":"DERCapability"},"rdfs:range":{"@id":"PowerFactor"},"rdfs:comment":"Specified under-excited power factor.","owl:minCardinality":0},{"@id":"rtgUnderExcitedW","@type":"rdf:Property","rdfs:domain":{"@id":"DERCapability"},"rdfs:range":{"@id":"ActivePower"},"rdfs:comment":"Active power rating in Watts at specified under-excited power factor (rtgUnderExcitedPF). If present, rtgUnderExcitedPF SHALL be present.","owl:minCardinality":0},{"@id":"rtgVNom","@type":"rdf:Property","rdfs:domain":{"@id":"DERCapability"},"rdfs:range":{"@id":"VoltageRMS"},"rdfs:comment":"AC voltage nominal rating.","owl:minCardinality":0},{"@id":"type","@type":"rdf:Property","rdfs:domain":{"@id":"DERCapability"},"rdfs:range":{"@id":"DERType"},"rdfs:comment":"Type of DER; see DERType object"},{"@id":"opModConnect","@type":"rdf:Property","rdfs:domain":{"@id":"DERControlBase"},"rdfs:range":"xsd:boolean","rdfs:comment":"Set DER as connected (true) or disconnected (false). Used in conjunction with ramp rate when re-connecting. Implies galvanic isolation.","owl:minCardinality":0},{"@id":"opModEnergize","@type":"rdf:Property","rdfs:domain":{"@id":"DERControlBase"},"rdfs:range":"xsd:boolean","rdfs:comment":"Set DER as energized (true) or de-energized (false). Used in conjunction with ramp rate when re-energizing.","owl:minCardinality":0},{"@id":"opModFixedPFAbsorbW","@type":"rdf:Property","rdfs:domain":{"@id":"DERControlBase"},"rdfs:range":{"@id":"PowerFactorWithExcitation"},"rdfs:comment":"The opModFixedPFAbsorbW function specifies a requested fixed Power Factor (PF) setting for when active power is being absorbed. The actual displacement SHALL be within the limits established by setMinPFOverExcited and setMinPFUnderExcited. If issued simultaneously with other reactive power controls (e.g. opModFixedVar) the control resulting in least var magnitude SHOULD take precedence.","owl:minCardinality":0},{"@id":"opModFixedPFInjectW","@type":"rdf:Property","rdfs:domain":{"@id":"DERControlBase"},"rdfs:range":{"@id":"PowerFactorWithExcitation"},"rdfs:comment":"The opModFixedPFInjectW function specifies a requested fixed Power Factor (PF) setting for when active power is being injected. The actual displacement SHALL be within the limits established by setMinPFOverExcited and setMinPFUnderExcited. If issued simultaneously with other reactive power controls (e.g. opModFixedVar) the control resulting in least var magnitude SHOULD take precedence.","owl:minCardinality":0},{"@id":"opModFixedVar","@type":"rdf:Property","rdfs:domain":{"@id":"DERControlBase"},"rdfs:range":{"@id":"FixedVar"},"rdfs:comment":"The opModFixedVar function specifies the delivered or received reactive power setpoint.  The context for the setpoint value is determined by refType and SHALL be one of %setMaxW, %setMaxVar, or %statVarAvail.  If issued simultaneously with other reactive power controls (e.g. opModFixedPFInjectW) the control resulting in least var magnitude SHOULD take precedence.","owl:minCardinality":0},{"@id":"opModFixedW","@type":"rdf:Property","rdfs:domain":{"@id":"DERControlBase"},"rdfs:range":{"@id":"SignedPerCent"},"rdfs:comment":"The opModFixedW function specifies a requested charge or discharge mode setpoint, in %setMaxChargeRateW if negative value or %setMaxW or %setMaxDischargeRateW if positive value (in hundredths).","owl:minCardinality":0},{"@id":"opModFreqDroop","@type":"rdf:Property","rdfs:domain":{"@id":"DERControlBase"},"rdfs:range":{"@id":"FreqDroopType"},"rdfs:comment":"Specifies a frequency-watt operation. This operation limits active power generation or consumption when the line frequency deviates from nominal by a specified amount.","owl:minCardinality":0},{"@id":"opModFreqWatt","@type":"rdf:Property","rdfs:domain":{"@id":"DERControlBase"},"rdfs:range":{"@id":"DERCurveLink"},"rdfs:comment":"Specify DERCurveLink for curveType == 0.  The Frequency-Watt function limits active power generation or consumption when the line frequency deviates from nominal by a specified amount. The Frequency-Watt curve is specified as an array of Frequency-Watt pairs that are interpolated into a piecewise linear function with hysteresis.  The x value of each pair specifies a frequency in Hz. The y value specifies a corresponding active power output in %setMaxW.","owl:minCardinality":0},{"@id":"opModHFRTMayTrip","@type":"rdf:Property","rdfs:domain":{"@id":"DERControlBase"},"rdfs:range":{"@id":"DERCurveLink"},"rdfs:comment":"Specify DERCurveLink for curveType == 1. The High Frequency Ride-Through (HFRT) function is specified by one or two duration-frequency curves that define the operating region under high frequency conditions. Each HFRT curve is specified by an array of duration-frequency pairs that will be interpolated into a piecewise linear function that defines an operating region. The x value of each pair specifies a duration (time at a given frequency in seconds). The y value of each pair specifies a frequency, in Hz. This control specifies the \"may trip\" region.","owl:minCardinality":0},{"@id":"opModHFRTMustTrip","@type":"rdf:Property","rdfs:domain":{"@id":"DERControlBase"},"rdfs:range":{"@id":"DERCurveLink"},"rdfs:comment":"Specify DERCurveLink for curveType == 2.  The High Frequency Ride-Through (HFRT) function is specified by a duration-frequency curve that defines the operating region under high frequency conditions.  Each HFRT curve is specified by an array of duration-frequency pairs that will be interpolated into a piecewise linear function that defines an operating region.  The x value of each pair specifies a duration (time at a given frequency in seconds). The y value of each pair specifies a frequency, in Hz. This control specifies the \"must trip\" region.","owl:minCardinality":0},{"@id":"opModHVRTMayTrip","@type":"rdf:Property","rdfs:domain":{"@id":"DERControlBase"},"rdfs:range":{"@id":"DERCurveLink"},"rdfs:comment":"Specify DERCurveLink for curveType == 3. The High Voltage Ride-Through (HVRT) function is specified by one, two, or three duration-volt curves that define the operating region under high voltage conditions. Each HVRT curve is specified by an array of duration-volt pairs that will be interpolated into a piecewise linear function that defines an operating region. The x value of each pair specifies a duration (time at a given voltage in seconds). The y value of each pair specifies an effective percentage voltage, defined as ((locally measured voltage - setVRefOfs / setVRef). This control specifies the \"may trip\" region.","owl:minCardinality":0},{"@id":"opModHVRTMomentaryCessation","@type":"rdf:Property","rdfs:domain":{"@id":"DERControlBase"},"rdfs:range":{"@id":"DERCurveLink"},"rdfs:comment":"Specify DERCurveLink for curveType == 4.  The High Voltage Ride-Through (HVRT) function is specified by duration-volt curves that define the operating region under high voltage conditions.  Each HVRT curve is specified by an array of duration-volt pairs that will be interpolated into a piecewise linear function that defines an operating region.  The x value of each pair specifies a duration (time at a given voltage in seconds). The y value of each pair specifies an effective percent voltage, defined as ((locally measured voltage - setVRefOfs) / setVRef). This control specifies the \"momentary cessation\" region.","owl:minCardinality":0},{"@id":"opModHVRTMustTrip","@type":"rdf:Property","rdfs:domain":{"@id":"DERControlBase"},"rdfs:range":{"@id":"DERCurveLink"},"rdfs:comment":"Specify DERCurveLink for curveType == 5.  The High Voltage Ride-Through (HVRT) function is specified by duration-volt curves that define the operating region under high voltage conditions.  Each HVRT curve is specified by an array of duration-volt pairs that will be interpolated into a piecewise linear function that defines an operating region.  The x value of each pair specifies a duration (time at a given voltage in seconds). The y value of each pair specifies an effective percent voltage, defined as ((locally measured voltage - setVRefOfs) / setVRef). This control specifies the \"must trip\" region.","owl:minCardinality":0},{"@id":"opModLFRTMayTrip","@type":"rdf:Property","rdfs:domain":{"@id":"DERControlBase"},"rdfs:range":{"@id":"DERCurveLink"},"rdfs:comment":"Specify DERCurveLink for curveType == 6. The Low Frequency Ride-Through (LFRT) function is specified by one or two duration-frequency curves that define the operating region under low frequency conditions. Each LFRT curve is specified by an array of duration-frequency pairs that will be interpolated into a piecewise linear function that defines an operating region. The x value of each pair specifies a duration (time at a given frequency in seconds). The y value of each pair specifies a frequency, in Hz. This control specifies the \"may trip\" region.","owl:minCardinality":0},{"@id":"opModLFRTMustTrip","@type":"rdf:Property","rdfs:domain":{"@id":"DERControlBase"},"rdfs:range":{"@id":"DERCurveLink"},"rdfs:comment":"Specify DERCurveLink for curveType == 7.  The Low Frequency Ride-Through (LFRT) function is specified by a duration-frequency curve that defines the operating region under low frequency conditions.  Each LFRT curve is specified by an array of duration-frequency pairs that will be interpolated into a piecewise linear function that defines an operating region.  The x value of each pair specifies a duration (time at a given frequency in seconds). The y value of each pair specifies a frequency, in Hz. This control specifies the \"must trip\" region.","owl:minCardinality":0},{"@id":"opModLVRTMayTrip","@type":"rdf:Property","rdfs:domain":{"@id":"DERControlBase"},"rdfs:range":{"@id":"DERCurveLink"},"rdfs:comment":"Specify DERCurveLink for curveType == 8. The Low Voltage Ride-Through (LVRT) function is specified by one, two, or three duration-volt curves that define the operating region under low voltage conditions. Each LVRT curve is specified by an array of duration-volt pairs that will be interpolated into a piecewise linear function that defines an operating region. The x value of each pair specifies a duration (time at a given voltage in seconds). The y value of each pair specifies an effective percent voltage, defined as ((locally measured voltage - setVRefOfs) / setVRef). This control specifies the \"may trip\" region.","owl:minCardinality":0},{"@id":"opModLVRTMomentaryCessation","@type":"rdf:Property","rdfs:domain":{"@id":"DERControlBase"},"rdfs:range":{"@id":"DERCurveLink"},"rdfs:comment":"Specify DERCurveLink for curveType == 9.  The Low Voltage Ride-Through (LVRT) function is specified by duration-volt curves that define the operating region under low voltage conditions.  Each LVRT curve is specified by an array of duration-volt pairs that will be interpolated into a piecewise linear function that defines an operating region.  The x value of each pair specifies a duration (time at a given voltage in seconds). The y value of each pair specifies an effective percent voltage, defined as ((locally measured voltage - setVRefOfs) / setVRef). This control specifies the \"momentary cessation\" region.","owl:minCardinality":0},{"@id":"opModLVRTMustTrip","@type":"rdf:Property","rdfs:domain":{"@id":"DERControlBase"},"rdfs:range":{"@id":"DERCurveLink"},"rdfs:comment":"Specify DERCurveLink for curveType == 10.  The Low Voltage Ride-Through (LVRT) function is specified by duration-volt curves that define the operating region under low voltage conditions.  Each LVRT curve is specified by an array of duration-volt pairs that will be interpolated into a piecewise linear function that defines an operating region.  The x value of each pair specifies a duration (time at a given voltage in seconds). The y value of each pair specifies an effective percent voltage, defined as ((locally measured voltage - setVRefOfs) / setVRef). This control specifies the \"must trip\" region.","owl:minCardinality":0},{"@id":"opModMaxLimW","@type":"rdf:Property","rdfs:domain":{"@id":"DERControlBase"},"rdfs:range":{"@id":"PerCent"},"rdfs:comment":"The opModMaxLimW function sets the maximum active power generation level at the electrical coupling point as a percentage of set capacity (%setMaxW, in hundredths). This limitation may be met e.g. by reducing PV output or by using excess PV output to charge associated storage.","owl:minCardinality":0},{"@id":"opModTargetVar","@type":"rdf:Property","rdfs:domain":{"@id":"DERControlBase"},"rdfs:range":{"@id":"ReactivePower"},"rdfs:comment":"Target reactive power, in var. This control is likely to be more useful for aggregators, as individual DERs may not be able to maintain a target setting.","owl:minCardinality":0},{"@id":"opModTargetW","@type":"rdf:Property","rdfs:domain":{"@id":"DERControlBase"},"rdfs:range":{"@id":"ActivePower"},"rdfs:comment":"Target output power, in Watts. This control is likely to be more useful for aggregators, as individual DERs may not be able to maintain a target setting.","owl:minCardinality":0},{"@id":"opModVoltVar","@type":"rdf:Property","rdfs:domain":{"@id":"DERControlBase"},"rdfs:range":{"@id":"DERCurveLink"},"rdfs:comment":"Specify DERCurveLink for curveType == 11.  The static volt-var function provides over- or under-excited var compensation as a function of measured voltage. The volt-var curve is specified as an array of volt-var pairs that are interpolated into a piecewise linear function with hysteresis. The x value of each pair specifies an effective percent voltage, defined as ((locally measured voltage - setVRefOfs) / setVRef) and SHOULD support a domain of at least 0 - 135. If VRef is present in DERCurve, then the x value of each pair is additionally multiplied by (VRef / 10000). The y value specifies a target var output interpreted as a signed percentage (-100 to 100). The meaning of the y value is determined by yRefType and must be one of %setMaxW, %setMaxVar, or %statVarAvail.","owl:minCardinality":0},{"@id":"opModVoltWatt","@type":"rdf:Property","rdfs:domain":{"@id":"DERControlBase"},"rdfs:range":{"@id":"DERCurveLink"},"rdfs:comment":"Specify DERCurveLink for curveType == 12.  The Volt-Watt reduces active power output as a function of measured voltage. The Volt-Watt curve is specified as an array of Volt-Watt pairs that are interpolated into a piecewise linear function with hysteresis. The x value of each pair specifies an effective percent voltage, defined as ((locally measured voltage - setVRefOfs) / setVRef) and SHOULD support a domain of at least 0 - 135. The y value specifies an active power output interpreted as a percentage (0 - 100). The meaning of the y value is determined by yRefType and must be one of %setMaxW or %statWAvail.","owl:minCardinality":0},{"@id":"opModWattPF","@type":"rdf:Property","rdfs:domain":{"@id":"DERControlBase"},"rdfs:range":{"@id":"DERCurveLink"},"rdfs:comment":"Specify DERCurveLink for curveType == 13.  The Watt-PF function varies Power Factor (PF) as a function of delivered active power. The Watt-PF curve is specified as an array of Watt-PF coordinates that are interpolated into a piecewise linear function with hysteresis.  The x value of each pair specifies a watt setting in %setMaxW, (0 - 100). The PF output setting is a signed displacement in y value (PF sign SHALL be interpreted according to the EEI convention, where unity PF is considered unsigned). These settings are not expected to be updated very often during the life of the installation, therefore only a single curve is required.  If issued simultaneously with other reactive power controls (e.g. opModFixedPFInjectW) the control resulting in least var magnitude SHOULD take precedence.","owl:minCardinality":0},{"@id":"opModWattVar","@type":"rdf:Property","rdfs:domain":{"@id":"DERControlBase"},"rdfs:range":{"@id":"DERCurveLink"},"rdfs:comment":"Specify DERCurveLink for curveType == 14. The Watt-Var function varies vars as a function of delivered active power. The Watt-Var curve is specified as an array of Watt-Var pairs that are interpolated into a piecewise linear function with hysteresis. The x value of each pair specifies a watt setting in %setMaxW, (0-100). The y value specifies a target var output interpreted as a signed percentage (-100 to 100). The meaning of the y value is determined by yRefType and must be one of %setMaxW, %setMaxVar, or %statVarAvail.","owl:minCardinality":0},{"@id":"rampTms","@type":"rdf:Property","rdfs:domain":{"@id":"DERControlBase"},"rdfs:range":{"@id":"UInt16"},"rdfs:comment":"Requested ramp time, in hundredths of a second, for the device to transition from the current DERControl  mode setting(s) to the new mode setting(s). If absent, use default ramp rate (setGradW).  Resolution is 1/100 sec.","owl:minCardinality":0},{"@id":"DERControlBase","@type":"rdf:Property","rdfs:domain":{"@id":"DERControl"},"rdfs:range":{"@id":"DERControlBase"}},{"@id":"deviceCategory","@type":"rdf:Property","rdfs:domain":{"@id":"DERControl"},"rdfs:range":{"@id":"DeviceCategoryType"},"rdfs:comment":"Specifies the bitmap indicating  the categories of devices that SHOULD respond. Devices SHOULD ignore events that do not indicate their device category. If not present, all devices SHOULD respond.","owl:minCardinality":0},{"@id":"DERControl","@type":"rdf:Property","rdfs:domain":{"@id":"DERControlList"},"rdfs:range":{"@id":"DERControl"},"owl:minCardinality":0},{"@id":"autonomousVRefEnable","@type":"rdf:Property","rdfs:domain":{"@id":"DERCurve"},"rdfs:range":"xsd:boolean","rdfs:comment":"If the curveType is opModVoltVar, then this field MAY be present. If the curveType is not opModVoltVar, then this field SHALL NOT be present. Enable/disable autonomous vRef adjustment. When enabled, the Volt-Var curve characteristic SHALL be adjusted autonomously as vRef changes and autonomousVRefTimeConstant SHALL be present. If a DER is able to support Volt-Var mode but is unable to support autonomous vRef adjustment, then the DER SHALL execute the curve without autonomous vRef adjustment. If not specified, then the value is false.","owl:minCardinality":0},{"@id":"autonomousVRefTimeConstant","@type":"rdf:Property","rdfs:domain":{"@id":"DERCurve"},"rdfs:range":{"@id":"UInt32"},"rdfs:comment":"If the curveType is opModVoltVar, then this field MAY be present. If the curveType is not opModVoltVar, then this field SHALL NOT be present. Adjustment range for vRef time constant, in hundredths of a second.","owl:minCardinality":0},{"@id":"creationTime","@type":"rdf:Property","rdfs:domain":{"@id":"DERCurve"},"rdfs:range":{"@id":"TimeType"},"rdfs:comment":"The time at which the object was created."},{"@id":"CurveData","@type":"rdf:Property","rdfs:domain":{"@id":"DERCurve"},"rdfs:range":{"@id":"CurveData"},"owl:maxCardinality":10},{"@id":"curveType","@type":"rdf:Property","rdfs:domain":{"@id":"DERCurve"},"rdfs:range":{"@id":"DERCurveType"},"rdfs:comment":"Specifies the associated curve-based control mode."},{"@id":"openLoopTms","@type":"rdf:Property","rdfs:domain":{"@id":"DERCurve"},"rdfs:range":{"@id":"UInt16"},"rdfs:comment":"Open loop response time, the time to ramp up to 90% of the new target in response to the change in voltage, in hundredths of a second. Resolution is 1/100 sec. A value of 0 is used to mean no limit. When not present, the device SHOULD follow its default behavior.","owl:minCardinality":0},{"@id":"rampDecTms","@type":"rdf:Property","rdfs:domain":{"@id":"DERCurve"},"rdfs:range":{"@id":"UInt16"},"rdfs:comment":"Decreasing ramp rate, interpreted as a percentage change in output capability limit per second (e.g. %setMaxW / sec).  Resolution is in hundredths of a percent/second. A value of 0 means there is no limit. If absent, ramp rate defaults to setGradW.","owl:minCardinality":0},{"@id":"rampIncTms","@type":"rdf:Property","rdfs:domain":{"@id":"DERCurve"},"rdfs:range":{"@id":"UInt16"},"rdfs:comment":"Increasing ramp rate, interpreted as a percentage change in output capability limit per second (e.g. %setMaxW / sec).  Resolution is in hundredths of a percent/second. A value of 0 means there is no limit. If absent, ramp rate defaults to rampDecTms.","owl:minCardinality":0},{"@id":"rampPT1Tms","@type":"rdf:Property","rdfs:domain":{"@id":"DERCurve"},"rdfs:range":{"@id":"UInt16"},"rdfs:comment":"The configuration parameter for a low-pass filter, PT1 is a time, in hundredths of a second, in which the filter will settle to 95% of a step change in the input value. Resolution is 1/100 sec.","owl:minCardinality":0},{"@id":"vRef","@type":"rdf:Property","rdfs:domain":{"@id":"DERCurve"},"rdfs:range":{"@id":"PerCent"},"rdfs:comment":"If the curveType is opModVoltVar, then this field MAY be present. If the curveType is not opModVoltVar, then this field SHALL NOT be present. The nominal AC voltage (RMS) adjustment to the voltage curve points for Volt-Var curves.","owl:minCardinality":0},{"@id":"xMultiplier","@type":"rdf:Property","rdfs:domain":{"@id":"DERCurve"},"rdfs:range":{"@id":"PowerOfTenMultiplierType"},"rdfs:comment":"Exponent for X-axis value."},{"@id":"yMultiplier","@type":"rdf:Property","rdfs:domain":{"@id":"DERCurve"},"rdfs:range":{"@id":"PowerOfTenMultiplierType"},"rdfs:comment":"Exponent for Y-axis value."},{"@id":"yRefType","@type":"rdf:Property","rdfs:domain":{"@id":"DERCurve"},"rdfs:range":{"@id":"DERUnitRefType"},"rdfs:comment":"The Y-axis units context."},{"@id":"DERCurve","@type":"rdf:Property","rdfs:domain":{"@id":"DERCurveList"},"rdfs:range":{"@id":"DERCurve"},"owl:minCardinality":0},{"@id":"excitation","@type":"rdf:Property","rdfs:domain":{"@id":"CurveData"},"rdfs:range":"xsd:boolean","rdfs:comment":"If yvalue is Power Factor, then this field SHALL be present. If yvalue is not Power Factor, then this field SHALL NOT be present.\nTrue when DER is absorbing reactive power (under-excited), false\nwhen DER is injecting reactive power (over-excited).","owl:minCardinality":0},{"@id":"xvalue","@type":"rdf:Property","rdfs:domain":{"@id":"CurveData"},"rdfs:range":{"@id":"Int32"},"rdfs:comment":"The data value of the X-axis (independent) variable, depending on the curve type. See definitions in DERControlBase for further information."},{"@id":"yvalue","@type":"rdf:Property","rdfs:domain":{"@id":"CurveData"},"rdfs:range":{"@id":"Int32"},"rdfs:comment":"The data value of the Y-axis (dependent) variable, depending on the curve type. See definitions in DERControlBase for further information. If yvalue is Power Factor, the excitation field SHALL be present and yvalue SHALL be a positive value. If yvalue is not Power Factor, the excitation field SHALL NOT be present."},{"@id":"ActiveDERControlListLink","@type":"rdf:Property","rdfs:domain":{"@id":"DERProgram"},"rdfs:range":{"@id":"ActiveDERControlListLink"},"owl:minCardinality":0},{"@id":"DefaultDERControlLink","@type":"rdf:Property","rdfs:domain":{"@id":"DERProgram"},"rdfs:range":{"@id":"DefaultDERControlLink"},"owl:minCardinality":0},{"@id":"DERControlListLink","@type":"rdf:Property","rdfs:domain":{"@id":"DERProgram"},"rdfs:range":{"@id":"DERControlListLink"},"owl:minCardinality":0},{"@id":"DERCurveListLink","@type":"rdf:Property","rdfs:domain":{"@id":"DERProgram"},"rdfs:range":{"@id":"DERCurveListLink"},"owl:minCardinality":0},{"@id":"primacy","@type":"rdf:Property","rdfs:domain":{"@id":"DERProgram"},"rdfs:range":{"@id":"PrimacyType"},"rdfs:comment":"Indicates the relative primacy of the provider of this Program."},{"@id":"DERProgram","@type":"rdf:Property","rdfs:domain":{"@id":"DERProgramList"},"rdfs:range":{"@id":"DERProgram"},"owl:minCardinality":0},{"@id":"pollRate","@type":"rdf:Property","rdfs:domain":{"@id":"DERProgramList"},"rdfs:range":{"@id":"UInt32"},"rdfs:comment":"The default polling rate for this function set (this resource and all resources below), in seconds. If not specified, a default of 900 seconds (15 minutes) is used. It is RECOMMENDED a client poll the resources of this function set every pollRate seconds.","owl:minCardinality":0},{"@id":"alarmStatus","@type":"rdf:Property","rdfs:domain":{"@id":"DERStatus"},"rdfs:range":{"@id":"HexBinary32"},"rdfs:comment":"Bitmap indicating the status of DER alarms (see DER LogEvents for more details).\n0 - DER_FAULT_OVER_CURRENT\n1 - DER_FAULT_OVER_VOLTAGE\n2 - DER_FAULT_UNDER_VOLTAGE\n3 - DER_FAULT_OVER_FREQUENCY\n4 - DER_FAULT_UNDER_FREQUENCY\n5 - DER_FAULT_VOLTAGE_IMBALANCE\n6 - DER_FAULT_CURRENT_IMBALANCE\n7 - DER_FAULT_EMERGENCY_LOCAL\n8 - DER_FAULT_EMERGENCY_REMOTE\n9 - DER_FAULT_LOW_POWER_INPUT\n10 - DER_FAULT_PHASE_ROTATION\n11-31 - Reserved","owl:minCardinality":0},{"@id":"genConnectStatus","@type":"rdf:Property","rdfs:domain":{"@id":"DERStatus"},"rdfs:range":{"@id":"ConnectStatusType"},"rdfs:comment":"Connect/status value for generator DER. \nSee ConnectStatusType for values.","owl:minCardinality":0},{"@id":"inverterStatus","@type":"rdf:Property","rdfs:domain":{"@id":"DERStatus"},"rdfs:range":{"@id":"InverterStatusType"},"rdfs:comment":"DER InverterStatus/value.\nSee InverterStatusType for values.","owl:minCardinality":0},{"@id":"localControlModeStatus","@type":"rdf:Property","rdfs:domain":{"@id":"DERStatus"},"rdfs:range":{"@id":"LocalControlModeStatusType"},"rdfs:comment":"The local control mode status.\nSee LocalControlModeStatusType for values.","owl:minCardinality":0},{"@id":"manufacturerStatus","@type":"rdf:Property","rdfs:domain":{"@id":"DERStatus"},"rdfs:range":{"@id":"ManufacturerStatusType"},"rdfs:comment":"Manufacturer status code.","owl:minCardinality":0},{"@id":"operationalModeStatus","@type":"rdf:Property","rdfs:domain":{"@id":"DERStatus"},"rdfs:range":{"@id":"OperationalModeStatusType"},"rdfs:comment":"Operational mode currently in use.\nSee OperationalModeStatusType for values.","owl:minCardinality":0},{"@id":"readingTime","@type":"rdf:Property","rdfs:domain":{"@id":"DERStatus"},"rdfs:range":{"@id":"TimeType"},"rdfs:comment":"The timestamp when the current status was last updated."},{"@id":"stateOfChargeStatus","@type":"rdf:Property","rdfs:domain":{"@id":"DERStatus"},"rdfs:range":{"@id":"StateOfChargeStatusType"},"rdfs:comment":"State of charge status.\nSee StateOfChargeStatusType for values.","owl:minCardinality":0},{"@id":"storageModeStatus","@type":"rdf:Property","rdfs:domain":{"@id":"DERStatus"},"rdfs:range":{"@id":"StorageModeStatusType"},"rdfs:comment":"Storage mode status.\nSee StorageModeStatusType for values.","owl:minCardinality":0},{"@id":"storConnectStatus","@type":"rdf:Property","rdfs:domain":{"@id":"DERStatus"},"rdfs:range":{"@id":"ConnectStatusType"},"rdfs:comment":"Connect/status value for storage DER.\nSee ConnectStatusType for values.","owl:minCardinality":0},{"@id":"multiplier","@type":"rdf:Property","rdfs:domain":{"@id":"CurrentRMS"},"rdfs:range":{"@id":"PowerOfTenMultiplierType"},"rdfs:comment":"Specifies exponent of value."},{"@id":"value","@type":"rdf:Property","rdfs:domain":{"@id":"CurrentRMS"},"rdfs:range":{"@id":"UInt16"},"rdfs:comment":"Value in amperes RMS (uom 5)"},{"@id":"multiplier","@type":"rdf:Property","rdfs:domain":{"@id":"FixedPointType"},"rdfs:range":{"@id":"PowerOfTenMultiplierType"},"rdfs:comment":"Specifies exponent of uom."},{"@id":"value","@type":"rdf:Property","rdfs:domain":{"@id":"FixedPointType"},"rdfs:range":{"@id":"Int16"},"rdfs:comment":"Dimensionless value"},{"@id":"multiplier","@type":"rdf:Property","rdfs:domain":{"@id":"UnsignedFixedPointType"},"rdfs:range":{"@id":"PowerOfTenMultiplierType"},"rdfs:comment":"Specifies exponent of uom."},{"@id":"value","@type":"rdf:Property","rdfs:domain":{"@id":"UnsignedFixedPointType"},"rdfs:range":{"@id":"UInt16"},"rdfs:comment":"Dimensionless value"},{"@id":"multiplier","@type":"rdf:Property","rdfs:domain":{"@id":"ActivePower"},"rdfs:range":{"@id":"PowerOfTenMultiplierType"},"rdfs:comment":"Specifies exponent for uom."},{"@id":"value","@type":"rdf:Property","rdfs:domain":{"@id":"ActivePower"},"rdfs:range":{"@id":"Int16"},"rdfs:comment":"Value in watts (uom 38)"},{"@id":"multiplier","@type":"rdf:Property","rdfs:domain":{"@id":"AmpereHour"},"rdfs:range":{"@id":"PowerOfTenMultiplierType"},"rdfs:comment":"Specifies exponent of uom."},{"@id":"value","@type":"rdf:Property","rdfs:domain":{"@id":"AmpereHour"},"rdfs:range":{"@id":"UInt16"},"rdfs:comment":"Value in ampere-hours (uom 106)"},{"@id":"multiplier","@type":"rdf:Property","rdfs:domain":{"@id":"ApparentPower"},"rdfs:range":{"@id":"PowerOfTenMultiplierType"},"rdfs:comment":"Specifies exponent of uom."},{"@id":"value","@type":"rdf:Property","rdfs:domain":{"@id":"ApparentPower"},"rdfs:range":{"@id":"UInt16"},"rdfs:comment":"Value in volt-amperes (uom 61)"},{"@id":"multiplier","@type":"rdf:Property","rdfs:domain":{"@id":"ReactivePower"},"rdfs:range":{"@id":"PowerOfTenMultiplierType"},"rdfs:comment":"Specifies exponent of uom."},{"@id":"value","@type":"rdf:Property","rdfs:domain":{"@id":"ReactivePower"},"rdfs:range":{"@id":"Int16"},"rdfs:comment":"Value in volt-amperes reactive (var) (uom 63)"},{"@id":"multiplier","@type":"rdf:Property","rdfs:domain":{"@id":"ReactiveSusceptance"},"rdfs:range":{"@id":"PowerOfTenMultiplierType"},"rdfs:comment":"Specifies exponent of uom."},{"@id":"value","@type":"rdf:Property","rdfs:domain":{"@id":"ReactiveSusceptance"},"rdfs:range":{"@id":"UInt16"},"rdfs:comment":"Value in siemens (uom 53)"},{"@id":"displacement","@type":"rdf:Property","rdfs:domain":{"@id":"PowerFactor"},"rdfs:range":{"@id":"UInt16"},"rdfs:comment":"Significand of an unsigned value of cos(theta) between 0 and 1.0. E.g. a value of 0.95 may be specified as a displacement of 950 and a multiplier of -3."},{"@id":"multiplier","@type":"rdf:Property","rdfs:domain":{"@id":"PowerFactor"},"rdfs:range":{"@id":"PowerOfTenMultiplierType"},"rdfs:comment":"Specifies exponent of 'displacement'."},{"@id":"displacement","@type":"rdf:Property","rdfs:domain":{"@id":"PowerFactorWithExcitation"},"rdfs:range":{"@id":"UInt16"},"rdfs:comment":"Significand of an unsigned value of cos(theta) between 0 and 1.0. E.g. a value of 0.95 may be specified as a displacement of 950 and a multiplier of -3."},{"@id":"excitation","@type":"rdf:Property","rdfs:domain":{"@id":"PowerFactorWithExcitation"},"rdfs:range":"xsd:boolean","rdfs:comment":"True when DER is absorbing reactive power (under-excited), false\nwhen DER is injecting reactive power (over-excited)."},{"@id":"multiplier","@type":"rdf:Property","rdfs:domain":{"@id":"PowerFactorWithExcitation"},"rdfs:range":{"@id":"PowerOfTenMultiplierType"},"rdfs:comment":"Specifies exponent of 'displacement'."},{"@id":"refType","@type":"rdf:Property","rdfs:domain":{"@id":"FixedVar"},"rdfs:range":{"@id":"DERUnitRefType"},"rdfs:comment":"Indicates whether to interpret 'value' as %setMaxVar or %statVarAvail."},{"@id":"value","@type":"rdf:Property","rdfs:domain":{"@id":"FixedVar"},"rdfs:range":{"@id":"SignedPerCent"},"rdfs:comment":"Specify a signed setpoint for reactive power in % (see 'refType' for context)."},{"@id":"multiplier","@type":"rdf:Property","rdfs:domain":{"@id":"WattHour"},"rdfs:range":{"@id":"PowerOfTenMultiplierType"},"rdfs:comment":"Specifies exponent of uom."},{"@id":"value","@type":"rdf:Property","rdfs:domain":{"@id":"WattHour"},"rdfs:range":{"@id":"UInt16"},"rdfs:comment":"Value in watt-hours (uom 72)"},{"@id":"multiplier","@type":"rdf:Property","rdfs:domain":{"@id":"VoltageRMS"},"rdfs:range":{"@id":"PowerOfTenMultiplierType"},"rdfs:comment":"Specifies exponent of uom."},{"@id":"value","@type":"rdf:Property","rdfs:domain":{"@id":"VoltageRMS"},"rdfs:range":{"@id":"UInt16"},"rdfs:comment":"Value in volts RMS (uom 29)"},{"@id":"dateTime","@type":"rdf:Property","rdfs:domain":{"@id":"ConnectStatusType"},"rdfs:range":{"@id":"TimeType"},"rdfs:comment":"The date and time at which the state applied."},{"@id":"value","@type":"rdf:Property","rdfs:domain":{"@id":"ConnectStatusType"},"rdfs:range":{"@id":"HexBinary8"},"rdfs:comment":"The value indicating the state."},{"@id":"dateTime","@type":"rdf:Property","rdfs:domain":{"@id":"InverterStatusType"},"rdfs:range":{"@id":"TimeType"},"rdfs:comment":"The date and time at which the state applied."},{"@id":"value","@type":"rdf:Property","rdfs:domain":{"@id":"InverterStatusType"},"rdfs:range":{"@id":"UInt8"},"rdfs:comment":"The value indicating the state."},{"@id":"dateTime","@type":"rdf:Property","rdfs:domain":{"@id":"LocalControlModeStatusType"},"rdfs:range":{"@id":"TimeType"},"rdfs:comment":"The date and time at which the state applied."},{"@id":"value","@type":"rdf:Property","rdfs:domain":{"@id":"LocalControlModeStatusType"},"rdfs:range":{"@id":"UInt8"},"rdfs:comment":"The value indicating the state."},{"@id":"dateTime","@type":"rdf:Property","rdfs:domain":{"@id":"ManufacturerStatusType"},"rdfs:range":{"@id":"TimeType"},"rdfs:comment":"The date and time at which the state applied."},{"@id":"value","@type":"rdf:Property","rdfs:domain":{"@id":"ManufacturerStatusType"},"rdfs:range":{"@id":"String6"},"rdfs:comment":"The value indicating the state."},{"@id":"dateTime","@type":"rdf:Property","rdfs:domain":{"@id":"OperationalModeStatusType"},"rdfs:range":{"@id":"TimeType"},"rdfs:comment":"The date and time at which the state applied."},{"@id":"value","@type":"rdf:Property","rdfs:domain":{"@id":"OperationalModeStatusType"},"rdfs:range":{"@id":"UInt8"},"rdfs:comment":"The value indicating the state."},{"@id":"dateTime","@type":"rdf:Property","rdfs:domain":{"@id":"StateOfChargeStatusType"},"rdfs:range":{"@id":"TimeType"},"rdfs:comment":"The date and time at which the state applied."},{"@id":"value","@type":"rdf:Property","rdfs:domain":{"@id":"StateOfChargeStatusType"},"rdfs:range":{"@id":"PerCent"},"rdfs:comment":"The value indicating the state."},{"@id":"dateTime","@type":"rdf:Property","rdfs:domain":{"@id":"StorageModeStatusType"},"rdfs:range":{"@id":"TimeType"},"rdfs:comment":"The date and time at which the state applied."},{"@id":"value","@type":"rdf:Property","rdfs:domain":{"@id":"StorageModeStatusType"},"rdfs:range":{"@id":"UInt8"},"rdfs:comment":"The value indicating the state."},{"@id":"mRID","@type":"rdf:Property","rdfs:domain":{"@id":"IdentifiedObject"},"rdfs:range":{"@id":"mRIDType"},"rdfs:comment":"The global identifier of the object."},{"@id":"description","@type":"rdf:Property","rdfs:domain":{"@id":"IdentifiedObject"},"rdfs:range":{"@id":"String32"},"rdfs:comment":"The description is a human readable text describing or naming the object.","owl:minCardinality":0},{"@id":"version","@type":"rdf:Property","rdfs:domain":{"@id":"IdentifiedObject"},"rdfs:range":{"@id":"VersionType"},"rdfs:comment":"Contains the version number of the object. See the type definition for details.","owl:minCardinality":0},{"@id":"href","@type":"rdf:Property","rdfs:domain":{"@id":"Link"},"rdfs:range":"xsd:anyURI","rdfs:comment":"A URI reference."},{"@id":"all","@type":"rdf:Property","rdfs:domain":{"@id":"List"},"rdfs:range":{"@id":"UInt32"},"rdfs:comment":"The number specifying \"all\" of the items in the list. Required on a response to a GET, ignored otherwise."},{"@id":"results","@type":"rdf:Property","rdfs:domain":{"@id":"List"},"rdfs:range":{"@id":"UInt32"},"rdfs:comment":"Indicates the number of items in this page of results."},{"@id":"all","@type":"rdf:Property","rdfs:domain":{"@id":"ListLink"},"rdfs:range":{"@id":"UInt32"},"rdfs:comment":"Indicates the total number of items in the referenced list. This attribute SHALL be present if the href is a local or relative URI. This attribute SHOULD NOT be present if the href is a remote or absolute URI, as the server may be unaware of changes to the value.","owl:minCardinality":0},{"@id":"href","@type":"rdf:Property","rdfs:domain":{"@id":"Resource"},"rdfs:range":"xsd:anyURI","rdfs:comment":"A reference to the resource address (URI). Required in a response to a GET, ignored otherwise.","owl:minCardinality":0},{"@id":"mRID","@type":"rdf:Property","rdfs:domain":{"@id":"RespondableIdentifiedObject"},"rdfs:range":{"@id":"mRIDType"},"rdfs:comment":"The global identifier of the object."},{"@id":"description","@type":"rdf:Property","rdfs:domain":{"@id":"RespondableIdentifiedObject"},"rdfs:range":{"@id":"String32"},"rdfs:comment":"The description is a human readable text describing or naming the object.","owl:minCardinality":0},{"@id":"version","@type":"rdf:Property","rdfs:domain":{"@id":"RespondableIdentifiedObject"},"rdfs:range":{"@id":"VersionType"},"rdfs:comment":"Contains the version number of the object. See the type definition for details.","owl:minCardinality":0},{"@id":"replyTo","@type":"rdf:Property","rdfs:domain":{"@id":"RespondableResource"},"rdfs:range":"xsd:anyURI","rdfs:comment":"A reference to the response resource address (URI). Required on a response to a GET if responseRequired is \"true\".","owl:minCardinality":0},{"@id":"responseRequired","@type":"rdf:Property","rdfs:domain":{"@id":"RespondableResource"},"rdfs:range":{"@id":"HexBinary8"},"rdfs:comment":"Indicates whether or not a response is required upon receipt, creation or update of this resource. Responses shall be posted to the collection specified in \"replyTo\". \n\nIf the resource has a deviceCategory field, devices that match one or more of the device types indicated in deviceCategory SHALL respond according to the rules listed below.  If the category does not match, the device SHALL NOT respond. If the resource does not have a deviceCategory field, a device receiving the resource SHALL respond according to the rules listed below.\n\nValue encoded as hex according to the following bit assignments, any combination is possible. \nSee Table 27 for the list of appropriate Response status codes to be sent for these purposes.\n0 - End device shall indicate that message was received \n1 - End device shall indicate specific response. \n2 - End user / customer response is required. \nAll other values reserved.","owl:minCardinality":0},{"@id":"mRID","@type":"rdf:Property","rdfs:domain":{"@id":"RespondableSubscribableIdentifiedObject"},"rdfs:range":{"@id":"mRIDType"},"rdfs:comment":"The global identifier of the object."},{"@id":"description","@type":"rdf:Property","rdfs:domain":{"@id":"RespondableSubscribableIdentifiedObject"},"rdfs:range":{"@id":"String32"},"rdfs:comment":"The description is a human readable text describing or naming the object.","owl:minCardinality":0},{"@id":"version","@type":"rdf:Property","rdfs:domain":{"@id":"RespondableSubscribableIdentifiedObject"},"rdfs:range":{"@id":"VersionType"},"rdfs:comment":"Contains the version number of the object. See the type definition for details.","owl:minCardinality":0},{"@id":"subscribable","@type":"rdf:Property","rdfs:domain":{"@id":"RespondableSubscribableIdentifiedObject"},"rdfs:range":{"@id":"SubscribableType"},"rdfs:comment":"Indicates whether or not subscriptions are supported for this resource, and whether or not conditional (thresholds) are supported. If not specified, is \"not subscribable\" (0).","owl:minCardinality":0},{"@id":"mRID","@type":"rdf:Property","rdfs:domain":{"@id":"SubscribableIdentifiedObject"},"rdfs:range":{"@id":"mRIDType"},"rdfs:comment":"The global identifier of the object."},{"@id":"description","@type":"rdf:Property","rdfs:domain":{"@id":"SubscribableIdentifiedObject"},"rdfs:range":{"@id":"String32"},"rdfs:comment":"The description is a human readable text describing or naming the object.","owl:minCardinality":0},{"@id":"version","@type":"rdf:Property","rdfs:domain":{"@id":"SubscribableIdentifiedObject"},"rdfs:range":{"@id":"VersionType"},"rdfs:comment":"Contains the version number of the object. See the type definition for details.","owl:minCardinality":0},{"@id":"all","@type":"rdf:Property","rdfs:domain":{"@id":"SubscribableList"},"rdfs:range":{"@id":"UInt32"},"rdfs:comment":"The number specifying \"all\" of the items in the list. Required on GET, ignored otherwise."},{"@id":"results","@type":"rdf:Property","rdfs:domain":{"@id":"SubscribableList"},"rdfs:range":{"@id":"UInt32"},"rdfs:comment":"Indicates the number of items in this page of results."},{"@id":"subscribable","@type":"rdf:Property","rdfs:domain":{"@id":"SubscribableResource"},"rdfs:range":{"@id":"SubscribableType"},"rdfs:comment":"Indicates whether or not subscriptions are supported for this resource, and whether or not conditional (thresholds) are supported. If not specified, is \"not subscribable\" (0).","owl:minCardinality":0},{"@id":"maxRetryDuration","@type":"rdf:Property","rdfs:domain":{"@id":"Error"},"rdfs:range":{"@id":"UInt16"},"rdfs:comment":"Contains the number of seconds the client SHOULD wait before retrying the request.","owl:minCardinality":0},{"@id":"reasonCode","@type":"rdf:Property","rdfs:domain":{"@id":"Error"},"rdfs:range":{"@id":"UInt16"},"rdfs:comment":"Code indicating the reason for failure.\n\n0 - Invalid request format\n1 - Invalid request values (e.g. invalid threshold values)\n2 - Resource limit reached\n3 - Conditional subscription field not supported\n4 - Maximum request frequency exceeded\nAll other values reserved"},{"@id":"creationTime","@type":"rdf:Property","rdfs:domain":{"@id":"Event"},"rdfs:range":{"@id":"TimeType"},"rdfs:comment":"The time at which the Event was created."},{"@id":"EventStatus","@type":"rdf:Property","rdfs:domain":{"@id":"Event"},"rdfs:range":{"@id":"EventStatus"}},{"@id":"interval","@type":"rdf:Property","rdfs:domain":{"@id":"Event"},"rdfs:range":{"@id":"DateTimeInterval"},"rdfs:comment":"The period during which the Event applies."},{"@id":"currentStatus","@type":"rdf:Property","rdfs:domain":{"@id":"EventStatus"},"rdfs:range":{"@id":"UInt8"},"rdfs:comment":"Field representing the current status type. \n\n0 = Scheduled\nThis status indicates that the event has been scheduled and the event has not yet started.  The server SHALL set the event to this status when the event is first scheduled and persist until the event has become active or has been cancelled.  For events with a start time less than or equal to the current time, this status SHALL never be indicated, the event SHALL start with a status of \u201cActive\u201d. \n\n1 = Active\nThis status indicates that the event is currently active. The server SHALL set the event to this status when the event reaches its earliest Effective Start Time.\n\n2 = Cancelled \nWhen events are cancelled, the Status.dateTime attribute SHALL be set to the time the cancellation occurred, which cannot be in the future.  The server is responsible for maintaining the cancelled event in its collection for the duration of the original event, or until the server has run out of space and needs to store a new event. Client devices SHALL be aware of Cancelled events, determine if the Cancelled event applies to them, and cancel the event immediately if applicable.\n\n3 = Cancelled with Randomization \nThe server is responsible for maintaining the cancelled event in its collection for the duration of the Effective Scheduled Period. Client devices SHALL be aware of Cancelled with Randomization events, determine if the Cancelled event applies to them, and cancel the event immediately, using the larger of (absolute value of randomizeStart) and (absolute value of randomizeDuration) as the end randomization, in seconds. This Status.type SHALL NOT be used with \"regular\" Events, only with specializations of RandomizableEvent.\n\n4 = Superseded\nEvents marked as Superseded by servers are events that may have been replaced by new events from the same program that target the exact same set of deviceCategory's (if applicable) AND DERControl controls (e.g., opModTargetW) (if applicable) and overlap for a given period of time. Servers SHALL mark an event as Superseded at the earliest Effective Start Time of the overlapping event. Servers are responsible for maintaining the Superseded event in their collection for the duration of the Effective Scheduled Period. \nClient devices encountering a Superseded event SHALL terminate execution of the event immediately and commence execution of the new event immediately, unless the current time is within the start randomization window of the superseded event, in which case the client SHALL obey the start randomization of the new event. This Status.type SHALL NOT be used with TextMessage, since multiple text messages can be active. \n\nAll other values reserved."},{"@id":"dateTime","@type":"rdf:Property","rdfs:domain":{"@id":"EventStatus"},"rdfs:range":{"@id":"TimeType"},"rdfs:comment":"The dateTime attribute will provide a timestamp of when the current status was defined. dateTime MUST be set to the time at which the status change occurred, not a time in the future or past."},{"@id":"potentiallySuperseded","@type":"rdf:Property","rdfs:domain":{"@id":"EventStatus"},"rdfs:range":"xsd:boolean","rdfs:comment":"Set to true by a server of this event if there are events that overlap this event in time and also overlap in some, but not all, deviceCategory's (if applicable) AND DERControl controls (e.g., opModTargetW) (if applicable) in the same function set instance."},{"@id":"potentiallySupersededTime","@type":"rdf:Property","rdfs:domain":{"@id":"EventStatus"},"rdfs:range":{"@id":"TimeType"},"rdfs:comment":"Indicates the time that the potentiallySuperseded flag was set.","owl:minCardinality":0},{"@id":"reason","@type":"rdf:Property","rdfs:domain":{"@id":"EventStatus"},"rdfs:range":{"@id":"String192"},"rdfs:comment":"The Reason attribute allows a Service provider to provide a textual explanation of the status.","owl:minCardinality":0},{"@id":"randomizeDuration","@type":"rdf:Property","rdfs:domain":{"@id":"RandomizableEvent"},"rdfs:range":{"@id":"OneHourRangeType"},"rdfs:comment":"Number of seconds boundary inside which a random value must be selected to be applied to the associated interval duration, to avoid sudden synchronized demand changes. If related to price level changes, sign may be ignored. Valid range is -3600 to 3600. If not specified, 0 is the default.","owl:minCardinality":0},{"@id":"randomizeStart","@type":"rdf:Property","rdfs:domain":{"@id":"RandomizableEvent"},"rdfs:range":{"@id":"OneHourRangeType"},"rdfs:comment":"Number of seconds boundary inside which a random value must be selected to be applied to the associated interval start time, to avoid sudden synchronized demand changes. If related to price level changes, sign may be ignored. Valid range is -3600 to 3600. If not specified, 0 is the default.","owl:minCardinality":0},{"@id":"duration","@type":"rdf:Property","rdfs:domain":{"@id":"DateTimeInterval"},"rdfs:range":{"@id":"UInt32"},"rdfs:comment":"Duration of the interval, in seconds."},{"@id":"start","@type":"rdf:Property","rdfs:domain":{"@id":"DateTimeInterval"},"rdfs:range":{"@id":"TimeType"},"rdfs:comment":"Date and time of the start of the interval."},{"@id":"lat","@type":"rdf:Property","rdfs:domain":{"@id":"GPSLocationType"},"rdfs:range":{"@id":"String32"},"rdfs:comment":"Specifies the latitude from equator. -90 (south) to +90 (north) in decimal degrees."},{"@id":"lon","@type":"rdf:Property","rdfs:domain":{"@id":"GPSLocationType"},"rdfs:range":{"@id":"String32"},"rdfs:comment":"Specifies the longitude from Greenwich Meridian. -180 (west) to +180 (east) in decimal degrees."},{"@id":"multiplier","@type":"rdf:Property","rdfs:domain":{"@id":"RealEnergy"},"rdfs:range":{"@id":"PowerOfTenMultiplierType"},"rdfs:comment":"Multiplier for 'unit'."},{"@id":"value","@type":"rdf:Property","rdfs:domain":{"@id":"RealEnergy"},"rdfs:range":{"@id":"UInt48"},"rdfs:comment":"Value of the energy in Watt-hours. (uom 72)"},{"@id":"multiplier","@type":"rdf:Property","rdfs:domain":{"@id":"SignedRealEnergy"},"rdfs:range":{"@id":"PowerOfTenMultiplierType"},"rdfs:comment":"Multiplier for 'unit'."},{"@id":"value","@type":"rdf:Property","rdfs:domain":{"@id":"SignedRealEnergy"},"rdfs:range":{"@id":"Int48"},"rdfs:comment":"Value of the energy in Watt-hours. (uom 72)"},{"@id":"multiplier","@type":"rdf:Property","rdfs:domain":{"@id":"UnitValueType"},"rdfs:range":{"@id":"PowerOfTenMultiplierType"},"rdfs:comment":"Multiplier for 'unit'."},{"@id":"unit","@type":"rdf:Property","rdfs:domain":{"@id":"UnitValueType"},"rdfs:range":{"@id":"UomType"},"rdfs:comment":"Unit in symbol"},{"@id":"value","@type":"rdf:Property","rdfs:domain":{"@id":"UnitValueType"},"rdfs:range":{"@id":"Int32"},"rdfs:comment":"Value in units specified"},{"@id":"lastUpdateTime","@type":"rdf:Property","rdfs:domain":{"@id":"MirrorMeterReading"},"rdfs:range":{"@id":"TimeType"},"rdfs:comment":"The date and time of the last update.","owl:minCardinality":0},{"@id":"MirrorReadingSet","@type":"rdf:Property","rdfs:domain":{"@id":"MirrorMeterReading"},"rdfs:range":{"@id":"MirrorReadingSet"},"owl:minCardinality":0},{"@id":"nextUpdateTime","@type":"rdf:Property","rdfs:domain":{"@id":"MirrorMeterReading"},"rdfs:range":{"@id":"TimeType"},"rdfs:comment":"The date and time of the next planned update.","owl:minCardinality":0},{"@id":"Reading","@type":"rdf:Property","rdfs:domain":{"@id":"MirrorMeterReading"},"rdfs:range":{"@id":"Reading"},"owl:minCardinality":0},{"@id":"ReadingType","@type":"rdf:Property","rdfs:domain":{"@id":"MirrorMeterReading"},"rdfs:range":{"@id":"ReadingType"},"owl:minCardinality":0},{"@id":"MirrorMeterReading","@type":"rdf:Property","rdfs:domain":{"@id":"MirrorMeterReadingList"},"rdfs:range":{"@id":"MirrorMeterReading"},"owl:minCardinality":0},{"@id":"Reading","@type":"rdf:Property","rdfs:domain":{"@id":"MirrorReadingSet"},"rdfs:range":{"@id":"Reading"},"owl:minCardinality":0},{"@id":"deviceLFDI","@type":"rdf:Property","rdfs:domain":{"@id":"MirrorUsagePoint"},"rdfs:range":{"@id":"HexBinary160"},"rdfs:comment":"The LFDI of the device being mirrored."},{"@id":"MirrorMeterReading","@type":"rdf:Property","rdfs:domain":{"@id":"MirrorUsagePoint"},"rdfs:range":{"@id":"MirrorMeterReading"},"owl:minCardinality":0},{"@id":"postRate","@type":"rdf:Property","rdfs:domain":{"@id":"MirrorUsagePoint"},"rdfs:range":{"@id":"UInt32"},"rdfs:comment":"POST rate, or how often mirrored data should be POSTed, in seconds. A client MAY indicate a preferred postRate when POSTing MirrorUsagePoint. A server MAY add or modify postRate to indicate its preferred posting rate.","owl:minCardinality":0},{"@id":"MirrorUsagePoint","@type":"rdf:Property","rdfs:domain":{"@id":"MirrorUsagePointList"},"rdfs:range":{"@id":"MirrorUsagePoint"},"owl:minCardinality":0},{"@id":"pollRate","@type":"rdf:Property","rdfs:domain":{"@id":"MirrorUsagePointList"},"rdfs:range":{"@id":"UInt32"},"rdfs:comment":"The default polling rate for this function set (this resource and all resources below), in seconds. If not specified, a default of 900 seconds (15 minutes) is used. It is RECOMMENDED a client poll the resources of this function set every pollRate seconds.","owl:minCardinality":0},{"@id":"consumptionBlock","@type":"rdf:Property","rdfs:domain":{"@id":"ReadingBase"},"rdfs:range":{"@id":"ConsumptionBlockType"},"rdfs:comment":"Indicates the consumption block related to the reading. REQUIRED if ReadingType numberOfConsumptionBlocks is non-zero. If not specified, is assumed to be \"0 - N/A\".","owl:minCardinality":0},{"@id":"qualityFlags","@type":"rdf:Property","rdfs:domain":{"@id":"ReadingBase"},"rdfs:range":{"@id":"HexBinary16"},"rdfs:comment":"List of codes indicating the quality of the reading, using specification:\n\nBit 0 - valid: data that has gone through all required validation checks and either passed them all or has been verified \nBit 1 - manually edited: Replaced or approved by a human\nBit 2 - estimated using reference day: data value was replaced by a machine computed value based on analysis of historical data using the same type of measurement.\nBit 3 - estimated using linear interpolation: data value was computed using linear interpolation based on the readings before and after it\nBit 4 - questionable: data that has failed one or more checks\nBit 5 - derived: data that has been calculated (using logic or mathematical operations), not necessarily measured directly \nBit 6 - projected (forecast): data that has been calculated as a projection or forecast of future readings","owl:minCardinality":0},{"@id":"timePeriod","@type":"rdf:Property","rdfs:domain":{"@id":"ReadingBase"},"rdfs:range":{"@id":"DateTimeInterval"},"rdfs:comment":"The time interval associated with the reading. If not specified, then defaults to the intervalLength specified in the associated ReadingType.","owl:minCardinality":0},{"@id":"touTier","@type":"rdf:Property","rdfs:domain":{"@id":"ReadingBase"},"rdfs:range":{"@id":"TOUType"},"rdfs:comment":"Indicates the time of use tier related to the reading. REQUIRED if ReadingType numberOfTouTiers is non-zero. If not specified, is assumed to be \"0 - N/A\".","owl:minCardinality":0},{"@id":"value","@type":"rdf:Property","rdfs:domain":{"@id":"ReadingBase"},"rdfs:range":{"@id":"Int48"},"rdfs:comment":"Value in units specified by ReadingType","owl:minCardinality":0},{"@id":"timePeriod","@type":"rdf:Property","rdfs:domain":{"@id":"ReadingSetBase"},"rdfs:range":{"@id":"DateTimeInterval"},"rdfs:comment":"Specifies the time range during which the contained readings were taken."},{"@id":"roleFlags","@type":"rdf:Property","rdfs:domain":{"@id":"UsagePointBase"},"rdfs:range":{"@id":"RoleFlagsType"},"rdfs:comment":"Specifies the roles that apply to the usage point."},{"@id":"serviceCategoryKind","@type":"rdf:Property","rdfs:domain":{"@id":"UsagePointBase"},"rdfs:range":{"@id":"ServiceKind"},"rdfs:comment":"The kind of service provided by this usage point."},{"@id":"status","@type":"rdf:Property","rdfs:domain":{"@id":"UsagePointBase"},"rdfs:range":{"@id":"UInt8"},"rdfs:comment":"Specifies the current status of the service at this usage point.\n0 = off\n1 = on"}]}