{"@context":{"@version":1.1,"ocpp":"https://schemas.ocpp.org/2.1.0/","schema":"https://schema.org/","rdf":"http://www.w3.org/1999/02/22-rdf-syntax-ns#","rdfs":"http://www.w3.org/2000/01/rdf-schema#","xsd":"http://www.w3.org/2001/XMLSchema#"},"@graph":[{"@id":"ocpp:CustomDataType","@type":"rdfs:Class","rdfs:label":"CustomDataType","rdfs:comment":"This class does not get 'AdditionalProperties = false' in the schema generation, so it can be extended with arbitrary JSON properties to allow adding custom data."},{"@id":"ocpp:GenericStatusEnumType","@type":"schema:Enumeration","schema:name":"GenericStatusEnumType","rdfs:comment":"Result of operation.\r\n","schema:hasEnumerationMember":[{"@id":"ocpp:Accepted"},{"@id":"ocpp:Rejected"}]},{"@id":"ocpp:Accepted","@type":["ocpp:GenericStatusEnumType","schema:Enumeration"],"schema:name":"Accepted","schema:identifier":"Accepted"},{"@id":"ocpp:Rejected","@type":["ocpp:GenericStatusEnumType","schema:Enumeration"],"schema:name":"Rejected","schema:identifier":"Rejected"},{"@id":"ocpp:StatusInfoType","@type":"rdfs:Class","rdfs:label":"StatusInfoType","rdfs:comment":"Element providing more information about the status.\r\n"},{"@id":"ocpp:PeriodicEventStreamParamsType","@type":"rdfs:Class","rdfs:label":"PeriodicEventStreamParamsType"},{"@id":"ocpp:HashAlgorithmEnumType","@type":"schema:Enumeration","schema:name":"HashAlgorithmEnumType","rdfs:comment":"Used algorithms for the hashes provided.\r\n","schema:hasEnumerationMember":[{"@id":"ocpp:SHA256"},{"@id":"ocpp:SHA384"},{"@id":"ocpp:SHA512"}]},{"@id":"ocpp:SHA256","@type":["ocpp:HashAlgorithmEnumType","schema:Enumeration"],"schema:name":"SHA256","schema:identifier":"SHA256"},{"@id":"ocpp:SHA384","@type":["ocpp:HashAlgorithmEnumType","schema:Enumeration"],"schema:name":"SHA384","schema:identifier":"SHA384"},{"@id":"ocpp:SHA512","@type":["ocpp:HashAlgorithmEnumType","schema:Enumeration"],"schema:name":"SHA512","schema:identifier":"SHA512"},{"@id":"ocpp:AdditionalInfoType","@type":"rdfs:Class","rdfs:label":"AdditionalInfoType","rdfs:comment":"Contains a case insensitive identifier to use for the authorization and the type of authorization to support multiple forms of identifiers.\r\n"},{"@id":"ocpp:IdTokenType","@type":"rdfs:Class","rdfs:label":"IdTokenType","rdfs:comment":"Contains a case insensitive identifier to use for the authorization and the type of authorization to support multiple forms of identifiers.\r\n"},{"@id":"ocpp:OCSPRequestDataType","@type":"rdfs:Class","rdfs:label":"OCSPRequestDataType","rdfs:comment":"Information about a certificate for an OCSP check.\r\n"},{"@id":"ocpp:AuthorizationStatusEnumType","@type":"schema:Enumeration","schema:name":"AuthorizationStatusEnumType","rdfs:comment":"Current status of the ID Token.\r\n","schema:hasEnumerationMember":[{"@id":"ocpp:Accepted"},{"@id":"ocpp:Blocked"},{"@id":"ocpp:ConcurrentTx"},{"@id":"ocpp:Expired"},{"@id":"ocpp:Invalid"},{"@id":"ocpp:NoCredit"},{"@id":"ocpp:NotAllowedTypeEVSE"},{"@id":"ocpp:NotAtThisLocation"},{"@id":"ocpp:NotAtThisTime"},{"@id":"ocpp:Unknown"}]},{"@id":"ocpp:Accepted","@type":["ocpp:AuthorizationStatusEnumType","schema:Enumeration"],"schema:name":"Accepted","schema:identifier":"Accepted"},{"@id":"ocpp:Blocked","@type":["ocpp:AuthorizationStatusEnumType","schema:Enumeration"],"schema:name":"Blocked","schema:identifier":"Blocked"},{"@id":"ocpp:ConcurrentTx","@type":["ocpp:AuthorizationStatusEnumType","schema:Enumeration"],"schema:name":"ConcurrentTx","schema:identifier":"ConcurrentTx"},{"@id":"ocpp:Expired","@type":["ocpp:AuthorizationStatusEnumType","schema:Enumeration"],"schema:name":"Expired","schema:identifier":"Expired"},{"@id":"ocpp:Invalid","@type":["ocpp:AuthorizationStatusEnumType","schema:Enumeration"],"schema:name":"Invalid","schema:identifier":"Invalid"},{"@id":"ocpp:NoCredit","@type":["ocpp:AuthorizationStatusEnumType","schema:Enumeration"],"schema:name":"NoCredit","schema:identifier":"NoCredit"},{"@id":"ocpp:NotAllowedTypeEVSE","@type":["ocpp:AuthorizationStatusEnumType","schema:Enumeration"],"schema:name":"NotAllowedTypeEVSE","schema:identifier":"NotAllowedTypeEVSE"},{"@id":"ocpp:NotAtThisLocation","@type":["ocpp:AuthorizationStatusEnumType","schema:Enumeration"],"schema:name":"NotAtThisLocation","schema:identifier":"NotAtThisLocation"},{"@id":"ocpp:NotAtThisTime","@type":["ocpp:AuthorizationStatusEnumType","schema:Enumeration"],"schema:name":"NotAtThisTime","schema:identifier":"NotAtThisTime"},{"@id":"ocpp:Unknown","@type":["ocpp:AuthorizationStatusEnumType","schema:Enumeration"],"schema:name":"Unknown","schema:identifier":"Unknown"},{"@id":"ocpp:AuthorizeCertificateStatusEnumType","@type":"schema:Enumeration","schema:name":"AuthorizeCertificateStatusEnumType","rdfs:comment":"Certificate status information. \r\n- if all certificates are valid: return 'Accepted'.\r\n- if one of the certificates was revoked, return 'CertificateRevoked'.\r\n","schema:hasEnumerationMember":[{"@id":"ocpp:Accepted"},{"@id":"ocpp:SignatureError"},{"@id":"ocpp:CertificateExpired"},{"@id":"ocpp:CertificateRevoked"},{"@id":"ocpp:NoCertificateAvailable"},{"@id":"ocpp:CertChainError"},{"@id":"ocpp:ContractCancelled"}]},{"@id":"ocpp:Accepted","@type":["ocpp:AuthorizeCertificateStatusEnumType","schema:Enumeration"],"schema:name":"Accepted","schema:identifier":"Accepted"},{"@id":"ocpp:SignatureError","@type":["ocpp:AuthorizeCertificateStatusEnumType","schema:Enumeration"],"schema:name":"SignatureError","schema:identifier":"SignatureError"},{"@id":"ocpp:CertificateExpired","@type":["ocpp:AuthorizeCertificateStatusEnumType","schema:Enumeration"],"schema:name":"CertificateExpired","schema:identifier":"CertificateExpired"},{"@id":"ocpp:CertificateRevoked","@type":["ocpp:AuthorizeCertificateStatusEnumType","schema:Enumeration"],"schema:name":"CertificateRevoked","schema:identifier":"CertificateRevoked"},{"@id":"ocpp:NoCertificateAvailable","@type":["ocpp:AuthorizeCertificateStatusEnumType","schema:Enumeration"],"schema:name":"NoCertificateAvailable","schema:identifier":"NoCertificateAvailable"},{"@id":"ocpp:CertChainError","@type":["ocpp:AuthorizeCertificateStatusEnumType","schema:Enumeration"],"schema:name":"CertChainError","schema:identifier":"CertChainError"},{"@id":"ocpp:ContractCancelled","@type":["ocpp:AuthorizeCertificateStatusEnumType","schema:Enumeration"],"schema:name":"ContractCancelled","schema:identifier":"ContractCancelled"},{"@id":"ocpp:DayOfWeekEnumType","@type":"schema:Enumeration","schema:name":"DayOfWeekEnumType","schema:hasEnumerationMember":[{"@id":"ocpp:Monday"},{"@id":"ocpp:Tuesday"},{"@id":"ocpp:Wednesday"},{"@id":"ocpp:Thursday"},{"@id":"ocpp:Friday"},{"@id":"ocpp:Saturday"},{"@id":"ocpp:Sunday"}]},{"@id":"ocpp:Monday","@type":["ocpp:DayOfWeekEnumType","schema:Enumeration"],"schema:name":"Monday","schema:identifier":"Monday"},{"@id":"ocpp:Tuesday","@type":["ocpp:DayOfWeekEnumType","schema:Enumeration"],"schema:name":"Tuesday","schema:identifier":"Tuesday"},{"@id":"ocpp:Wednesday","@type":["ocpp:DayOfWeekEnumType","schema:Enumeration"],"schema:name":"Wednesday","schema:identifier":"Wednesday"},{"@id":"ocpp:Thursday","@type":["ocpp:DayOfWeekEnumType","schema:Enumeration"],"schema:name":"Thursday","schema:identifier":"Thursday"},{"@id":"ocpp:Friday","@type":["ocpp:DayOfWeekEnumType","schema:Enumeration"],"schema:name":"Friday","schema:identifier":"Friday"},{"@id":"ocpp:Saturday","@type":["ocpp:DayOfWeekEnumType","schema:Enumeration"],"schema:name":"Saturday","schema:identifier":"Saturday"},{"@id":"ocpp:Sunday","@type":["ocpp:DayOfWeekEnumType","schema:Enumeration"],"schema:name":"Sunday","schema:identifier":"Sunday"},{"@id":"ocpp:EnergyTransferModeEnumType","@type":"schema:Enumeration","schema:name":"EnergyTransferModeEnumType","rdfs:comment":"Mode of energy transfer requested by the EV.\r\n","schema:hasEnumerationMember":[{"@id":"ocpp:AC_single_phase"},{"@id":"ocpp:AC_two_phase"},{"@id":"ocpp:AC_three_phase"},{"@id":"ocpp:DC"},{"@id":"ocpp:AC_BPT"},{"@id":"ocpp:AC_BPT_DER"},{"@id":"ocpp:AC_DER"},{"@id":"ocpp:DC_BPT"},{"@id":"ocpp:DC_ACDP"},{"@id":"ocpp:DC_ACDP_BPT"},{"@id":"ocpp:WPT"}]},{"@id":"ocpp:AC_single_phase","@type":["ocpp:EnergyTransferModeEnumType","schema:Enumeration"],"schema:name":"AC_single_phase","schema:identifier":"AC_single_phase"},{"@id":"ocpp:AC_two_phase","@type":["ocpp:EnergyTransferModeEnumType","schema:Enumeration"],"schema:name":"AC_two_phase","schema:identifier":"AC_two_phase"},{"@id":"ocpp:AC_three_phase","@type":["ocpp:EnergyTransferModeEnumType","schema:Enumeration"],"schema:name":"AC_three_phase","schema:identifier":"AC_three_phase"},{"@id":"ocpp:DC","@type":["ocpp:EnergyTransferModeEnumType","schema:Enumeration"],"schema:name":"DC","schema:identifier":"DC"},{"@id":"ocpp:AC_BPT","@type":["ocpp:EnergyTransferModeEnumType","schema:Enumeration"],"schema:name":"AC_BPT","schema:identifier":"AC_BPT"},{"@id":"ocpp:AC_BPT_DER","@type":["ocpp:EnergyTransferModeEnumType","schema:Enumeration"],"schema:name":"AC_BPT_DER","schema:identifier":"AC_BPT_DER"},{"@id":"ocpp:AC_DER","@type":["ocpp:EnergyTransferModeEnumType","schema:Enumeration"],"schema:name":"AC_DER","schema:identifier":"AC_DER"},{"@id":"ocpp:DC_BPT","@type":["ocpp:EnergyTransferModeEnumType","schema:Enumeration"],"schema:name":"DC_BPT","schema:identifier":"DC_BPT"},{"@id":"ocpp:DC_ACDP","@type":["ocpp:EnergyTransferModeEnumType","schema:Enumeration"],"schema:name":"DC_ACDP","schema:identifier":"DC_ACDP"},{"@id":"ocpp:DC_ACDP_BPT","@type":["ocpp:EnergyTransferModeEnumType","schema:Enumeration"],"schema:name":"DC_ACDP_BPT","schema:identifier":"DC_ACDP_BPT"},{"@id":"ocpp:WPT","@type":["ocpp:EnergyTransferModeEnumType","schema:Enumeration"],"schema:name":"WPT","schema:identifier":"WPT"},{"@id":"ocpp:EvseKindEnumType","@type":"schema:Enumeration","schema:name":"EvseKindEnumType","rdfs:comment":"Type of EVSE (AC, DC) this tariff applies to.\r\n","schema:hasEnumerationMember":[{"@id":"ocpp:AC"},{"@id":"ocpp:DC"}]},{"@id":"ocpp:AC","@type":["ocpp:EvseKindEnumType","schema:Enumeration"],"schema:name":"AC","schema:identifier":"AC"},{"@id":"ocpp:DC","@type":["ocpp:EvseKindEnumType","schema:Enumeration"],"schema:name":"DC","schema:identifier":"DC"},{"@id":"ocpp:MessageFormatEnumType","@type":"schema:Enumeration","schema:name":"MessageFormatEnumType","rdfs:comment":"Format of the message.\r\n","schema:hasEnumerationMember":[{"@id":"ocpp:ASCII"},{"@id":"ocpp:HTML"},{"@id":"ocpp:URI"},{"@id":"ocpp:UTF8"},{"@id":"ocpp:QRCODE"}]},{"@id":"ocpp:ASCII","@type":["ocpp:MessageFormatEnumType","schema:Enumeration"],"schema:name":"ASCII","schema:identifier":"ASCII"},{"@id":"ocpp:HTML","@type":["ocpp:MessageFormatEnumType","schema:Enumeration"],"schema:name":"HTML","schema:identifier":"HTML"},{"@id":"ocpp:URI","@type":["ocpp:MessageFormatEnumType","schema:Enumeration"],"schema:name":"URI","schema:identifier":"URI"},{"@id":"ocpp:UTF8","@type":["ocpp:MessageFormatEnumType","schema:Enumeration"],"schema:name":"UTF8","schema:identifier":"UTF8"},{"@id":"ocpp:QRCODE","@type":["ocpp:MessageFormatEnumType","schema:Enumeration"],"schema:name":"QRCODE","schema:identifier":"QRCODE"},{"@id":"ocpp:IdTokenInfoType","@type":"rdfs:Class","rdfs:label":"IdTokenInfoType","rdfs:comment":"Contains status information about an identifier.\r\nIt is advised to not stop charging for a token that expires during charging, as ExpiryDate is only used for caching purposes. If ExpiryDate is not given, the status has no end date.\r\n"},{"@id":"ocpp:MessageContentType","@type":"rdfs:Class","rdfs:label":"MessageContentType","rdfs:comment":"Contains message details, for a message to be displayed on a Charging Station.\r\n\r\n"},{"@id":"ocpp:PriceType","@type":"rdfs:Class","rdfs:label":"PriceType","rdfs:comment":"Price with and without tax. At least one of _exclTax_, _inclTax_ must be present.\r\n"},{"@id":"ocpp:TariffConditionsFixedType","@type":"rdfs:Class","rdfs:label":"TariffConditionsFixedType","rdfs:comment":"These conditions describe if a FixedPrice applies at start of the transaction.\r\n\r\nWhen more than one restriction is set, they are to be treated as a logical AND. All need to be valid before this price is active.\r\n\r\nNOTE: _startTimeOfDay_ and _endTimeOfDay_ are in local time, because it is the time in the tariff as it is shown to the EV driver at the Charging Station.\r\nA Charging Station will convert this to the internal time zone that it uses (which is recommended to be UTC, see section Generic chapter 3.1) when performing cost calculation.\r\n\r\n"},{"@id":"ocpp:TariffConditionsType","@type":"rdfs:Class","rdfs:label":"TariffConditionsType","rdfs:comment":"These conditions describe if and when a TariffEnergyType or TariffTimeType applies during a transaction.\r\n\r\nWhen more than one restriction is set, they are to be treated as a logical AND. All need to be valid before this price is active.\r\n\r\nFor reverse energy flow (discharging) negative values of energy, power and current are used.\r\n\r\nNOTE: _minXXX_ (where XXX = Kwh/A/Kw) must be read as \"closest to zero\", and _maxXXX_ as \"furthest from zero\". For example, a *charging* power range from 10 kW to 50 kWh is given by _minPower_ = 10000 and _maxPower_ = 50000, and a *discharging* power range from -10 kW to -50 kW is given by _minPower_ = -10 and _maxPower_ = -50.\r\n\r\nNOTE: _startTimeOfDay_ and _endTimeOfDay_ are in local time, because it is the time in the tariff as it is shown to the EV driver at the Charging Station.\r\nA Charging Station will convert this to the internal time zone that it uses (which is recommended to be UTC, see section Generic chapter 3.1) when performing cost calculation.\r\n\r\n"},{"@id":"ocpp:TariffEnergyPriceType","@type":"rdfs:Class","rdfs:label":"TariffEnergyPriceType","rdfs:comment":"Tariff with optional conditions for an energy price.\r\n"},{"@id":"ocpp:TariffEnergyType","@type":"rdfs:Class","rdfs:label":"TariffEnergyType","rdfs:comment":"Price elements and tax for energy\r\n"},{"@id":"ocpp:TariffFixedPriceType","@type":"rdfs:Class","rdfs:label":"TariffFixedPriceType","rdfs:comment":"Tariff with optional conditions for a fixed price.\r\n"},{"@id":"ocpp:TariffFixedType","@type":"rdfs:Class","rdfs:label":"TariffFixedType"},{"@id":"ocpp:TariffTimePriceType","@type":"rdfs:Class","rdfs:label":"TariffTimePriceType","rdfs:comment":"Tariff with optional conditions for a time duration price.\r\n"},{"@id":"ocpp:TariffTimeType","@type":"rdfs:Class","rdfs:label":"TariffTimeType","rdfs:comment":"Price elements and tax for time\r\n\r\n"},{"@id":"ocpp:TariffType","@type":"rdfs:Class","rdfs:label":"TariffType","rdfs:comment":"A tariff is described by fields with prices for:\r\nenergy,\r\ncharging time,\r\nidle time,\r\nfixed fee,\r\nreservation time,\r\nreservation fixed fee. +\r\nEach of these fields may have (optional) conditions that specify when a price is applicable. +\r\nThe _description_ contains a human-readable explanation of the tariff to be shown to the user. +\r\nThe other fields are parameters that define the tariff. These are used by the charging station to calculate the price.\r\n"},{"@id":"ocpp:TaxRateType","@type":"rdfs:Class","rdfs:label":"TaxRateType","rdfs:comment":"Tax percentage\r\n"},{"@id":"ocpp:BatterySwapEventEnumType","@type":"schema:Enumeration","schema:name":"BatterySwapEventEnumType","rdfs:comment":"Battery in/out\r\n","schema:hasEnumerationMember":[{"@id":"ocpp:BatteryIn"},{"@id":"ocpp:BatteryOut"},{"@id":"ocpp:BatteryOutTimeout"}]},{"@id":"ocpp:BatteryIn","@type":["ocpp:BatterySwapEventEnumType","schema:Enumeration"],"schema:name":"BatteryIn","schema:identifier":"BatteryIn"},{"@id":"ocpp:BatteryOut","@type":["ocpp:BatterySwapEventEnumType","schema:Enumeration"],"schema:name":"BatteryOut","schema:identifier":"BatteryOut"},{"@id":"ocpp:BatteryOutTimeout","@type":["ocpp:BatterySwapEventEnumType","schema:Enumeration"],"schema:name":"BatteryOutTimeout","schema:identifier":"BatteryOutTimeout"},{"@id":"ocpp:BatteryDataType","@type":"rdfs:Class","rdfs:label":"BatteryDataType"},{"@id":"ocpp:BootReasonEnumType","@type":"schema:Enumeration","schema:name":"BootReasonEnumType","rdfs:comment":"This contains the reason for sending this message to the CSMS.\r\n","schema:hasEnumerationMember":[{"@id":"ocpp:ApplicationReset"},{"@id":"ocpp:FirmwareUpdate"},{"@id":"ocpp:LocalReset"},{"@id":"ocpp:PowerUp"},{"@id":"ocpp:RemoteReset"},{"@id":"ocpp:ScheduledReset"},{"@id":"ocpp:Triggered"},{"@id":"ocpp:Unknown"},{"@id":"ocpp:Watchdog"}]},{"@id":"ocpp:ApplicationReset","@type":["ocpp:BootReasonEnumType","schema:Enumeration"],"schema:name":"ApplicationReset","schema:identifier":"ApplicationReset"},{"@id":"ocpp:FirmwareUpdate","@type":["ocpp:BootReasonEnumType","schema:Enumeration"],"schema:name":"FirmwareUpdate","schema:identifier":"FirmwareUpdate"},{"@id":"ocpp:LocalReset","@type":["ocpp:BootReasonEnumType","schema:Enumeration"],"schema:name":"LocalReset","schema:identifier":"LocalReset"},{"@id":"ocpp:PowerUp","@type":["ocpp:BootReasonEnumType","schema:Enumeration"],"schema:name":"PowerUp","schema:identifier":"PowerUp"},{"@id":"ocpp:RemoteReset","@type":["ocpp:BootReasonEnumType","schema:Enumeration"],"schema:name":"RemoteReset","schema:identifier":"RemoteReset"},{"@id":"ocpp:ScheduledReset","@type":["ocpp:BootReasonEnumType","schema:Enumeration"],"schema:name":"ScheduledReset","schema:identifier":"ScheduledReset"},{"@id":"ocpp:Triggered","@type":["ocpp:BootReasonEnumType","schema:Enumeration"],"schema:name":"Triggered","schema:identifier":"Triggered"},{"@id":"ocpp:Unknown","@type":["ocpp:BootReasonEnumType","schema:Enumeration"],"schema:name":"Unknown","schema:identifier":"Unknown"},{"@id":"ocpp:Watchdog","@type":["ocpp:BootReasonEnumType","schema:Enumeration"],"schema:name":"Watchdog","schema:identifier":"Watchdog"},{"@id":"ocpp:ChargingStationType","@type":"rdfs:Class","rdfs:label":"ChargingStationType","rdfs:comment":"The physical system where an Electrical Vehicle (EV) can be charged.\r\n"},{"@id":"ocpp:ModemType","@type":"rdfs:Class","rdfs:label":"ModemType","rdfs:comment":"Defines parameters required for initiating and maintaining wireless communication with other devices.\r\n"},{"@id":"ocpp:RegistrationStatusEnumType","@type":"schema:Enumeration","schema:name":"RegistrationStatusEnumType","rdfs:comment":"This contains whether the Charging Station has been registered\r\nwithin the CSMS.\r\n","schema:hasEnumerationMember":[{"@id":"ocpp:Accepted"},{"@id":"ocpp:Pending"},{"@id":"ocpp:Rejected"}]},{"@id":"ocpp:Accepted","@type":["ocpp:RegistrationStatusEnumType","schema:Enumeration"],"schema:name":"Accepted","schema:identifier":"Accepted"},{"@id":"ocpp:Pending","@type":["ocpp:RegistrationStatusEnumType","schema:Enumeration"],"schema:name":"Pending","schema:identifier":"Pending"},{"@id":"ocpp:Rejected","@type":["ocpp:RegistrationStatusEnumType","schema:Enumeration"],"schema:name":"Rejected","schema:identifier":"Rejected"},{"@id":"ocpp:CancelReservationStatusEnumType","@type":"schema:Enumeration","schema:name":"CancelReservationStatusEnumType","rdfs:comment":"This indicates the success or failure of the canceling of a reservation by CSMS.\r\n","schema:hasEnumerationMember":[{"@id":"ocpp:Accepted"},{"@id":"ocpp:Rejected"}]},{"@id":"ocpp:Accepted","@type":["ocpp:CancelReservationStatusEnumType","schema:Enumeration"],"schema:name":"Accepted","schema:identifier":"Accepted"},{"@id":"ocpp:Rejected","@type":["ocpp:CancelReservationStatusEnumType","schema:Enumeration"],"schema:name":"Rejected","schema:identifier":"Rejected"},{"@id":"ocpp:CertificateSigningUseEnumType","@type":"schema:Enumeration","schema:name":"CertificateSigningUseEnumType","rdfs:comment":"Indicates the type of certificate that is to be signed. When omitted the certificate is to be used for both the 15118 connection (if implemented) and the Charging Station to CSMS connection.\r\n\r\n","schema:hasEnumerationMember":[{"@id":"ocpp:ChargingStationCertificate"},{"@id":"ocpp:V2GCertificate"},{"@id":"ocpp:V2G20Certificate"}]},{"@id":"ocpp:ChargingStationCertificate","@type":["ocpp:CertificateSigningUseEnumType","schema:Enumeration"],"schema:name":"ChargingStationCertificate","schema:identifier":"ChargingStationCertificate"},{"@id":"ocpp:V2GCertificate","@type":["ocpp:CertificateSigningUseEnumType","schema:Enumeration"],"schema:name":"V2GCertificate","schema:identifier":"V2GCertificate"},{"@id":"ocpp:V2G20Certificate","@type":["ocpp:CertificateSigningUseEnumType","schema:Enumeration"],"schema:name":"V2G20Certificate","schema:identifier":"V2G20Certificate"},{"@id":"ocpp:CertificateSignedStatusEnumType","@type":"schema:Enumeration","schema:name":"CertificateSignedStatusEnumType","rdfs:comment":"Returns whether certificate signing has been accepted, otherwise rejected.\r\n","schema:hasEnumerationMember":[{"@id":"ocpp:Accepted"},{"@id":"ocpp:Rejected"}]},{"@id":"ocpp:Accepted","@type":["ocpp:CertificateSignedStatusEnumType","schema:Enumeration"],"schema:name":"Accepted","schema:identifier":"Accepted"},{"@id":"ocpp:Rejected","@type":["ocpp:CertificateSignedStatusEnumType","schema:Enumeration"],"schema:name":"Rejected","schema:identifier":"Rejected"},{"@id":"ocpp:OperationalStatusEnumType","@type":"schema:Enumeration","schema:name":"OperationalStatusEnumType","rdfs:comment":"This contains the type of availability change that the Charging Station should perform.\r\n\r\n","schema:hasEnumerationMember":[{"@id":"ocpp:Inoperative"},{"@id":"ocpp:Operative"}]},{"@id":"ocpp:Inoperative","@type":["ocpp:OperationalStatusEnumType","schema:Enumeration"],"schema:name":"Inoperative","schema:identifier":"Inoperative"},{"@id":"ocpp:Operative","@type":["ocpp:OperationalStatusEnumType","schema:Enumeration"],"schema:name":"Operative","schema:identifier":"Operative"},{"@id":"ocpp:EVSEType","@type":"rdfs:Class","rdfs:label":"EVSEType","rdfs:comment":"Electric Vehicle Supply Equipment\r\n"},{"@id":"ocpp:ChangeAvailabilityStatusEnumType","@type":"schema:Enumeration","schema:name":"ChangeAvailabilityStatusEnumType","rdfs:comment":"This indicates whether the Charging Station is able to perform the availability change.\r\n","schema:hasEnumerationMember":[{"@id":"ocpp:Accepted"},{"@id":"ocpp:Rejected"},{"@id":"ocpp:Scheduled"}]},{"@id":"ocpp:Accepted","@type":["ocpp:ChangeAvailabilityStatusEnumType","schema:Enumeration"],"schema:name":"Accepted","schema:identifier":"Accepted"},{"@id":"ocpp:Rejected","@type":["ocpp:ChangeAvailabilityStatusEnumType","schema:Enumeration"],"schema:name":"Rejected","schema:identifier":"Rejected"},{"@id":"ocpp:Scheduled","@type":["ocpp:ChangeAvailabilityStatusEnumType","schema:Enumeration"],"schema:name":"Scheduled","schema:identifier":"Scheduled"},{"@id":"ocpp:TariffChangeStatusEnumType","@type":"schema:Enumeration","schema:name":"TariffChangeStatusEnumType","rdfs:comment":"Status of the operation\r\n","schema:hasEnumerationMember":[{"@id":"ocpp:Accepted"},{"@id":"ocpp:Rejected"},{"@id":"ocpp:TooManyElements"},{"@id":"ocpp:ConditionNotSupported"},{"@id":"ocpp:TxNotFound"},{"@id":"ocpp:NoCurrencyChange"}]},{"@id":"ocpp:Accepted","@type":["ocpp:TariffChangeStatusEnumType","schema:Enumeration"],"schema:name":"Accepted","schema:identifier":"Accepted"},{"@id":"ocpp:Rejected","@type":["ocpp:TariffChangeStatusEnumType","schema:Enumeration"],"schema:name":"Rejected","schema:identifier":"Rejected"},{"@id":"ocpp:TooManyElements","@type":["ocpp:TariffChangeStatusEnumType","schema:Enumeration"],"schema:name":"TooManyElements","schema:identifier":"TooManyElements"},{"@id":"ocpp:ConditionNotSupported","@type":["ocpp:TariffChangeStatusEnumType","schema:Enumeration"],"schema:name":"ConditionNotSupported","schema:identifier":"ConditionNotSupported"},{"@id":"ocpp:TxNotFound","@type":["ocpp:TariffChangeStatusEnumType","schema:Enumeration"],"schema:name":"TxNotFound","schema:identifier":"TxNotFound"},{"@id":"ocpp:NoCurrencyChange","@type":["ocpp:TariffChangeStatusEnumType","schema:Enumeration"],"schema:name":"NoCurrencyChange","schema:identifier":"NoCurrencyChange"},{"@id":"ocpp:ClearCacheStatusEnumType","@type":"schema:Enumeration","schema:name":"ClearCacheStatusEnumType","rdfs:comment":"Accepted if the Charging Station has executed the request, otherwise rejected.\r\n","schema:hasEnumerationMember":[{"@id":"ocpp:Accepted"},{"@id":"ocpp:Rejected"}]},{"@id":"ocpp:Accepted","@type":["ocpp:ClearCacheStatusEnumType","schema:Enumeration"],"schema:name":"Accepted","schema:identifier":"Accepted"},{"@id":"ocpp:Rejected","@type":["ocpp:ClearCacheStatusEnumType","schema:Enumeration"],"schema:name":"Rejected","schema:identifier":"Rejected"},{"@id":"ocpp:ChargingProfilePurposeEnumType","@type":"schema:Enumeration","schema:name":"ChargingProfilePurposeEnumType","rdfs:comment":"Defines the purpose of the schedule transferred by this profile\r\n","schema:hasEnumerationMember":[{"@id":"ocpp:ChargingStationExternalConstraints"},{"@id":"ocpp:ChargingStationMaxProfile"},{"@id":"ocpp:TxDefaultProfile"},{"@id":"ocpp:TxProfile"},{"@id":"ocpp:PriorityCharging"},{"@id":"ocpp:LocalGeneration"}]},{"@id":"ocpp:ChargingStationExternalConstraints","@type":["ocpp:ChargingProfilePurposeEnumType","schema:Enumeration"],"schema:name":"ChargingStationExternalConstraints","schema:identifier":"ChargingStationExternalConstraints"},{"@id":"ocpp:ChargingStationMaxProfile","@type":["ocpp:ChargingProfilePurposeEnumType","schema:Enumeration"],"schema:name":"ChargingStationMaxProfile","schema:identifier":"ChargingStationMaxProfile"},{"@id":"ocpp:TxDefaultProfile","@type":["ocpp:ChargingProfilePurposeEnumType","schema:Enumeration"],"schema:name":"TxDefaultProfile","schema:identifier":"TxDefaultProfile"},{"@id":"ocpp:TxProfile","@type":["ocpp:ChargingProfilePurposeEnumType","schema:Enumeration"],"schema:name":"TxProfile","schema:identifier":"TxProfile"},{"@id":"ocpp:PriorityCharging","@type":["ocpp:ChargingProfilePurposeEnumType","schema:Enumeration"],"schema:name":"PriorityCharging","schema:identifier":"PriorityCharging"},{"@id":"ocpp:LocalGeneration","@type":["ocpp:ChargingProfilePurposeEnumType","schema:Enumeration"],"schema:name":"LocalGeneration","schema:identifier":"LocalGeneration"},{"@id":"ocpp:ClearChargingProfileType","@type":"rdfs:Class","rdfs:label":"ClearChargingProfileType","rdfs:comment":"A ClearChargingProfileType is a filter for charging profiles to be cleared by ClearChargingProfileRequest.\r\n\r\n"},{"@id":"ocpp:ClearChargingProfileStatusEnumType","@type":"schema:Enumeration","schema:name":"ClearChargingProfileStatusEnumType","rdfs:comment":"Indicates if the Charging Station was able to execute the request.\r\n","schema:hasEnumerationMember":[{"@id":"ocpp:Accepted"},{"@id":"ocpp:Unknown"}]},{"@id":"ocpp:Accepted","@type":["ocpp:ClearChargingProfileStatusEnumType","schema:Enumeration"],"schema:name":"Accepted","schema:identifier":"Accepted"},{"@id":"ocpp:Unknown","@type":["ocpp:ClearChargingProfileStatusEnumType","schema:Enumeration"],"schema:name":"Unknown","schema:identifier":"Unknown"},{"@id":"ocpp:DERControlEnumType","@type":"schema:Enumeration","schema:name":"DERControlEnumType","rdfs:comment":"Type of control.  Determines which setting field below is used.\r\n\r\n","schema:hasEnumerationMember":[{"@id":"ocpp:EnterService"},{"@id":"ocpp:FreqDroop"},{"@id":"ocpp:FreqWatt"},{"@id":"ocpp:FixedPFAbsorb"},{"@id":"ocpp:FixedPFInject"},{"@id":"ocpp:FixedVar"},{"@id":"ocpp:Gradients"},{"@id":"ocpp:HFMustTrip"},{"@id":"ocpp:HFMayTrip"},{"@id":"ocpp:HVMustTrip"},{"@id":"ocpp:HVMomCess"},{"@id":"ocpp:HVMayTrip"},{"@id":"ocpp:LimitMaxDischarge"},{"@id":"ocpp:LFMustTrip"},{"@id":"ocpp:LVMustTrip"},{"@id":"ocpp:LVMomCess"},{"@id":"ocpp:LVMayTrip"},{"@id":"ocpp:PowerMonitoringMustTrip"},{"@id":"ocpp:VoltVar"},{"@id":"ocpp:VoltWatt"},{"@id":"ocpp:WattPF"},{"@id":"ocpp:WattVar"}]},{"@id":"ocpp:EnterService","@type":["ocpp:DERControlEnumType","schema:Enumeration"],"schema:name":"EnterService","schema:identifier":"EnterService"},{"@id":"ocpp:FreqDroop","@type":["ocpp:DERControlEnumType","schema:Enumeration"],"schema:name":"FreqDroop","schema:identifier":"FreqDroop"},{"@id":"ocpp:FreqWatt","@type":["ocpp:DERControlEnumType","schema:Enumeration"],"schema:name":"FreqWatt","schema:identifier":"FreqWatt"},{"@id":"ocpp:FixedPFAbsorb","@type":["ocpp:DERControlEnumType","schema:Enumeration"],"schema:name":"FixedPFAbsorb","schema:identifier":"FixedPFAbsorb"},{"@id":"ocpp:FixedPFInject","@type":["ocpp:DERControlEnumType","schema:Enumeration"],"schema:name":"FixedPFInject","schema:identifier":"FixedPFInject"},{"@id":"ocpp:FixedVar","@type":["ocpp:DERControlEnumType","schema:Enumeration"],"schema:name":"FixedVar","schema:identifier":"FixedVar"},{"@id":"ocpp:Gradients","@type":["ocpp:DERControlEnumType","schema:Enumeration"],"schema:name":"Gradients","schema:identifier":"Gradients"},{"@id":"ocpp:HFMustTrip","@type":["ocpp:DERControlEnumType","schema:Enumeration"],"schema:name":"HFMustTrip","schema:identifier":"HFMustTrip"},{"@id":"ocpp:HFMayTrip","@type":["ocpp:DERControlEnumType","schema:Enumeration"],"schema:name":"HFMayTrip","schema:identifier":"HFMayTrip"},{"@id":"ocpp:HVMustTrip","@type":["ocpp:DERControlEnumType","schema:Enumeration"],"schema:name":"HVMustTrip","schema:identifier":"HVMustTrip"},{"@id":"ocpp:HVMomCess","@type":["ocpp:DERControlEnumType","schema:Enumeration"],"schema:name":"HVMomCess","schema:identifier":"HVMomCess"},{"@id":"ocpp:HVMayTrip","@type":["ocpp:DERControlEnumType","schema:Enumeration"],"schema:name":"HVMayTrip","schema:identifier":"HVMayTrip"},{"@id":"ocpp:LimitMaxDischarge","@type":["ocpp:DERControlEnumType","schema:Enumeration"],"schema:name":"LimitMaxDischarge","schema:identifier":"LimitMaxDischarge"},{"@id":"ocpp:LFMustTrip","@type":["ocpp:DERControlEnumType","schema:Enumeration"],"schema:name":"LFMustTrip","schema:identifier":"LFMustTrip"},{"@id":"ocpp:LVMustTrip","@type":["ocpp:DERControlEnumType","schema:Enumeration"],"schema:name":"LVMustTrip","schema:identifier":"LVMustTrip"},{"@id":"ocpp:LVMomCess","@type":["ocpp:DERControlEnumType","schema:Enumeration"],"schema:name":"LVMomCess","schema:identifier":"LVMomCess"},{"@id":"ocpp:LVMayTrip","@type":["ocpp:DERControlEnumType","schema:Enumeration"],"schema:name":"LVMayTrip","schema:identifier":"LVMayTrip"},{"@id":"ocpp:PowerMonitoringMustTrip","@type":["ocpp:DERControlEnumType","schema:Enumeration"],"schema:name":"PowerMonitoringMustTrip","schema:identifier":"PowerMonitoringMustTrip"},{"@id":"ocpp:VoltVar","@type":["ocpp:DERControlEnumType","schema:Enumeration"],"schema:name":"VoltVar","schema:identifier":"VoltVar"},{"@id":"ocpp:VoltWatt","@type":["ocpp:DERControlEnumType","schema:Enumeration"],"schema:name":"VoltWatt","schema:identifier":"VoltWatt"},{"@id":"ocpp:WattPF","@type":["ocpp:DERControlEnumType","schema:Enumeration"],"schema:name":"WattPF","schema:identifier":"WattPF"},{"@id":"ocpp:WattVar","@type":["ocpp:DERControlEnumType","schema:Enumeration"],"schema:name":"WattVar","schema:identifier":"WattVar"},{"@id":"ocpp:DERControlStatusEnumType","@type":"schema:Enumeration","schema:name":"DERControlStatusEnumType","rdfs:comment":"Result of operation.\r\n\r\n","schema:hasEnumerationMember":[{"@id":"ocpp:Accepted"},{"@id":"ocpp:Rejected"},{"@id":"ocpp:NotSupported"},{"@id":"ocpp:NotFound"}]},{"@id":"ocpp:Accepted","@type":["ocpp:DERControlStatusEnumType","schema:Enumeration"],"schema:name":"Accepted","schema:identifier":"Accepted"},{"@id":"ocpp:Rejected","@type":["ocpp:DERControlStatusEnumType","schema:Enumeration"],"schema:name":"Rejected","schema:identifier":"Rejected"},{"@id":"ocpp:NotSupported","@type":["ocpp:DERControlStatusEnumType","schema:Enumeration"],"schema:name":"NotSupported","schema:identifier":"NotSupported"},{"@id":"ocpp:NotFound","@type":["ocpp:DERControlStatusEnumType","schema:Enumeration"],"schema:name":"NotFound","schema:identifier":"NotFound"},{"@id":"ocpp:ClearMessageStatusEnumType","@type":"schema:Enumeration","schema:name":"ClearMessageStatusEnumType","rdfs:comment":"Returns whether the Charging Station has been able to remove the message.\r\n","schema:hasEnumerationMember":[{"@id":"ocpp:Accepted"},{"@id":"ocpp:Unknown"},{"@id":"ocpp:Rejected"}]},{"@id":"ocpp:Accepted","@type":["ocpp:ClearMessageStatusEnumType","schema:Enumeration"],"schema:name":"Accepted","schema:identifier":"Accepted"},{"@id":"ocpp:Unknown","@type":["ocpp:ClearMessageStatusEnumType","schema:Enumeration"],"schema:name":"Unknown","schema:identifier":"Unknown"},{"@id":"ocpp:Rejected","@type":["ocpp:ClearMessageStatusEnumType","schema:Enumeration"],"schema:name":"Rejected","schema:identifier":"Rejected"},{"@id":"ocpp:TariffClearStatusEnumType","@type":"schema:Enumeration","schema:name":"TariffClearStatusEnumType","schema:hasEnumerationMember":[{"@id":"ocpp:Accepted"},{"@id":"ocpp:Rejected"},{"@id":"ocpp:NoTariff"}]},{"@id":"ocpp:Accepted","@type":["ocpp:TariffClearStatusEnumType","schema:Enumeration"],"schema:name":"Accepted","schema:identifier":"Accepted"},{"@id":"ocpp:Rejected","@type":["ocpp:TariffClearStatusEnumType","schema:Enumeration"],"schema:name":"Rejected","schema:identifier":"Rejected"},{"@id":"ocpp:NoTariff","@type":["ocpp:TariffClearStatusEnumType","schema:Enumeration"],"schema:name":"NoTariff","schema:identifier":"NoTariff"},{"@id":"ocpp:ClearTariffsResultType","@type":"rdfs:Class","rdfs:label":"ClearTariffsResultType"},{"@id":"ocpp:ClearMonitoringStatusEnumType","@type":"schema:Enumeration","schema:name":"ClearMonitoringStatusEnumType","rdfs:comment":"Result of the clear request for this monitor, identified by its Id.\r\n\r\n","schema:hasEnumerationMember":[{"@id":"ocpp:Accepted"},{"@id":"ocpp:Rejected"},{"@id":"ocpp:NotFound"}]},{"@id":"ocpp:Accepted","@type":["ocpp:ClearMonitoringStatusEnumType","schema:Enumeration"],"schema:name":"Accepted","schema:identifier":"Accepted"},{"@id":"ocpp:Rejected","@type":["ocpp:ClearMonitoringStatusEnumType","schema:Enumeration"],"schema:name":"Rejected","schema:identifier":"Rejected"},{"@id":"ocpp:NotFound","@type":["ocpp:ClearMonitoringStatusEnumType","schema:Enumeration"],"schema:name":"NotFound","schema:identifier":"NotFound"},{"@id":"ocpp:ClearMonitoringResultType","@type":"rdfs:Class","rdfs:label":"ClearMonitoringResultType"},{"@id":"ocpp:CertificateHashDataType","@type":"rdfs:Class","rdfs:label":"CertificateHashDataType"},{"@id":"ocpp:CustomerInformationStatusEnumType","@type":"schema:Enumeration","schema:name":"CustomerInformationStatusEnumType","rdfs:comment":"Indicates whether the request was accepted.\r\n","schema:hasEnumerationMember":[{"@id":"ocpp:Accepted"},{"@id":"ocpp:Rejected"},{"@id":"ocpp:Invalid"}]},{"@id":"ocpp:Accepted","@type":["ocpp:CustomerInformationStatusEnumType","schema:Enumeration"],"schema:name":"Accepted","schema:identifier":"Accepted"},{"@id":"ocpp:Rejected","@type":["ocpp:CustomerInformationStatusEnumType","schema:Enumeration"],"schema:name":"Rejected","schema:identifier":"Rejected"},{"@id":"ocpp:Invalid","@type":["ocpp:CustomerInformationStatusEnumType","schema:Enumeration"],"schema:name":"Invalid","schema:identifier":"Invalid"},{"@id":"ocpp:DataTransferStatusEnumType","@type":"schema:Enumeration","schema:name":"DataTransferStatusEnumType","rdfs:comment":"This indicates the success or failure of the data transfer.\r\n","schema:hasEnumerationMember":[{"@id":"ocpp:Accepted"},{"@id":"ocpp:Rejected"},{"@id":"ocpp:UnknownMessageId"},{"@id":"ocpp:UnknownVendorId"}]},{"@id":"ocpp:Accepted","@type":["ocpp:DataTransferStatusEnumType","schema:Enumeration"],"schema:name":"Accepted","schema:identifier":"Accepted"},{"@id":"ocpp:Rejected","@type":["ocpp:DataTransferStatusEnumType","schema:Enumeration"],"schema:name":"Rejected","schema:identifier":"Rejected"},{"@id":"ocpp:UnknownMessageId","@type":["ocpp:DataTransferStatusEnumType","schema:Enumeration"],"schema:name":"UnknownMessageId","schema:identifier":"UnknownMessageId"},{"@id":"ocpp:UnknownVendorId","@type":["ocpp:DataTransferStatusEnumType","schema:Enumeration"],"schema:name":"UnknownVendorId","schema:identifier":"UnknownVendorId"},{"@id":"ocpp:DeleteCertificateStatusEnumType","@type":"schema:Enumeration","schema:name":"DeleteCertificateStatusEnumType","rdfs:comment":"Charging Station indicates if it can process the request.\r\n","schema:hasEnumerationMember":[{"@id":"ocpp:Accepted"},{"@id":"ocpp:Failed"},{"@id":"ocpp:NotFound"}]},{"@id":"ocpp:Accepted","@type":["ocpp:DeleteCertificateStatusEnumType","schema:Enumeration"],"schema:name":"Accepted","schema:identifier":"Accepted"},{"@id":"ocpp:Failed","@type":["ocpp:DeleteCertificateStatusEnumType","schema:Enumeration"],"schema:name":"Failed","schema:identifier":"Failed"},{"@id":"ocpp:NotFound","@type":["ocpp:DeleteCertificateStatusEnumType","schema:Enumeration"],"schema:name":"NotFound","schema:identifier":"NotFound"},{"@id":"ocpp:FirmwareStatusEnumType","@type":"schema:Enumeration","schema:name":"FirmwareStatusEnumType","rdfs:comment":"This contains the progress status of the firmware installation.\r\n","schema:hasEnumerationMember":[{"@id":"ocpp:Downloaded"},{"@id":"ocpp:DownloadFailed"},{"@id":"ocpp:Downloading"},{"@id":"ocpp:DownloadScheduled"},{"@id":"ocpp:DownloadPaused"},{"@id":"ocpp:Idle"},{"@id":"ocpp:InstallationFailed"},{"@id":"ocpp:Installing"},{"@id":"ocpp:Installed"},{"@id":"ocpp:InstallRebooting"},{"@id":"ocpp:InstallScheduled"},{"@id":"ocpp:InstallVerificationFailed"},{"@id":"ocpp:InvalidSignature"},{"@id":"ocpp:SignatureVerified"}]},{"@id":"ocpp:Downloaded","@type":["ocpp:FirmwareStatusEnumType","schema:Enumeration"],"schema:name":"Downloaded","schema:identifier":"Downloaded"},{"@id":"ocpp:DownloadFailed","@type":["ocpp:FirmwareStatusEnumType","schema:Enumeration"],"schema:name":"DownloadFailed","schema:identifier":"DownloadFailed"},{"@id":"ocpp:Downloading","@type":["ocpp:FirmwareStatusEnumType","schema:Enumeration"],"schema:name":"Downloading","schema:identifier":"Downloading"},{"@id":"ocpp:DownloadScheduled","@type":["ocpp:FirmwareStatusEnumType","schema:Enumeration"],"schema:name":"DownloadScheduled","schema:identifier":"DownloadScheduled"},{"@id":"ocpp:DownloadPaused","@type":["ocpp:FirmwareStatusEnumType","schema:Enumeration"],"schema:name":"DownloadPaused","schema:identifier":"DownloadPaused"},{"@id":"ocpp:Idle","@type":["ocpp:FirmwareStatusEnumType","schema:Enumeration"],"schema:name":"Idle","schema:identifier":"Idle"},{"@id":"ocpp:InstallationFailed","@type":["ocpp:FirmwareStatusEnumType","schema:Enumeration"],"schema:name":"InstallationFailed","schema:identifier":"InstallationFailed"},{"@id":"ocpp:Installing","@type":["ocpp:FirmwareStatusEnumType","schema:Enumeration"],"schema:name":"Installing","schema:identifier":"Installing"},{"@id":"ocpp:Installed","@type":["ocpp:FirmwareStatusEnumType","schema:Enumeration"],"schema:name":"Installed","schema:identifier":"Installed"},{"@id":"ocpp:InstallRebooting","@type":["ocpp:FirmwareStatusEnumType","schema:Enumeration"],"schema:name":"InstallRebooting","schema:identifier":"InstallRebooting"},{"@id":"ocpp:InstallScheduled","@type":["ocpp:FirmwareStatusEnumType","schema:Enumeration"],"schema:name":"InstallScheduled","schema:identifier":"InstallScheduled"},{"@id":"ocpp:InstallVerificationFailed","@type":["ocpp:FirmwareStatusEnumType","schema:Enumeration"],"schema:name":"InstallVerificationFailed","schema:identifier":"InstallVerificationFailed"},{"@id":"ocpp:InvalidSignature","@type":["ocpp:FirmwareStatusEnumType","schema:Enumeration"],"schema:name":"InvalidSignature","schema:identifier":"InvalidSignature"},{"@id":"ocpp:SignatureVerified","@type":["ocpp:FirmwareStatusEnumType","schema:Enumeration"],"schema:name":"SignatureVerified","schema:identifier":"SignatureVerified"},{"@id":"ocpp:CertificateActionEnumType","@type":"schema:Enumeration","schema:name":"CertificateActionEnumType","rdfs:comment":"Defines whether certificate needs to be installed or updated.\r\n","schema:hasEnumerationMember":[{"@id":"ocpp:Install"},{"@id":"ocpp:Update"}]},{"@id":"ocpp:Install","@type":["ocpp:CertificateActionEnumType","schema:Enumeration"],"schema:name":"Install","schema:identifier":"Install"},{"@id":"ocpp:Update","@type":["ocpp:CertificateActionEnumType","schema:Enumeration"],"schema:name":"Update","schema:identifier":"Update"},{"@id":"ocpp:Iso15118EVCertificateStatusEnumType","@type":"schema:Enumeration","schema:name":"Iso15118EVCertificateStatusEnumType","rdfs:comment":"Indicates whether the message was processed properly.\r\n","schema:hasEnumerationMember":[{"@id":"ocpp:Accepted"},{"@id":"ocpp:Failed"}]},{"@id":"ocpp:Accepted","@type":["ocpp:Iso15118EVCertificateStatusEnumType","schema:Enumeration"],"schema:name":"Accepted","schema:identifier":"Accepted"},{"@id":"ocpp:Failed","@type":["ocpp:Iso15118EVCertificateStatusEnumType","schema:Enumeration"],"schema:name":"Failed","schema:identifier":"Failed"},{"@id":"ocpp:ReportBaseEnumType","@type":"schema:Enumeration","schema:name":"ReportBaseEnumType","rdfs:comment":"This field specifies the report base.\r\n","schema:hasEnumerationMember":[{"@id":"ocpp:ConfigurationInventory"},{"@id":"ocpp:FullInventory"},{"@id":"ocpp:SummaryInventory"}]},{"@id":"ocpp:ConfigurationInventory","@type":["ocpp:ReportBaseEnumType","schema:Enumeration"],"schema:name":"ConfigurationInventory","schema:identifier":"ConfigurationInventory"},{"@id":"ocpp:FullInventory","@type":["ocpp:ReportBaseEnumType","schema:Enumeration"],"schema:name":"FullInventory","schema:identifier":"FullInventory"},{"@id":"ocpp:SummaryInventory","@type":["ocpp:ReportBaseEnumType","schema:Enumeration"],"schema:name":"SummaryInventory","schema:identifier":"SummaryInventory"},{"@id":"ocpp:GenericDeviceModelStatusEnumType","@type":"schema:Enumeration","schema:name":"GenericDeviceModelStatusEnumType","rdfs:comment":"Indicates whether the Charging Station was able to accept the request.\r\n","schema:hasEnumerationMember":[{"@id":"ocpp:Accepted"},{"@id":"ocpp:Rejected"},{"@id":"ocpp:NotSupported"},{"@id":"ocpp:EmptyResultSet"}]},{"@id":"ocpp:Accepted","@type":["ocpp:GenericDeviceModelStatusEnumType","schema:Enumeration"],"schema:name":"Accepted","schema:identifier":"Accepted"},{"@id":"ocpp:Rejected","@type":["ocpp:GenericDeviceModelStatusEnumType","schema:Enumeration"],"schema:name":"Rejected","schema:identifier":"Rejected"},{"@id":"ocpp:NotSupported","@type":["ocpp:GenericDeviceModelStatusEnumType","schema:Enumeration"],"schema:name":"NotSupported","schema:identifier":"NotSupported"},{"@id":"ocpp:EmptyResultSet","@type":["ocpp:GenericDeviceModelStatusEnumType","schema:Enumeration"],"schema:name":"EmptyResultSet","schema:identifier":"EmptyResultSet"},{"@id":"ocpp:CertificateStatusSourceEnumType","@type":"schema:Enumeration","schema:name":"CertificateStatusSourceEnumType","rdfs:comment":"Source of status: OCSP, CRL\r\n","schema:hasEnumerationMember":[{"@id":"ocpp:CRL"},{"@id":"ocpp:OCSP"}]},{"@id":"ocpp:CRL","@type":["ocpp:CertificateStatusSourceEnumType","schema:Enumeration"],"schema:name":"CRL","schema:identifier":"CRL"},{"@id":"ocpp:OCSP","@type":["ocpp:CertificateStatusSourceEnumType","schema:Enumeration"],"schema:name":"OCSP","schema:identifier":"OCSP"},{"@id":"ocpp:CertificateStatusRequestInfoType","@type":"rdfs:Class","rdfs:label":"CertificateStatusRequestInfoType","rdfs:comment":"Data necessary to request the revocation status of a certificate.\r\n"},{"@id":"ocpp:CertificateStatusEnumType","@type":"schema:Enumeration","schema:name":"CertificateStatusEnumType","rdfs:comment":"Status of certificate: good, revoked or unknown.\r\n","schema:hasEnumerationMember":[{"@id":"ocpp:Good"},{"@id":"ocpp:Revoked"},{"@id":"ocpp:Unknown"},{"@id":"ocpp:Failed"}]},{"@id":"ocpp:Good","@type":["ocpp:CertificateStatusEnumType","schema:Enumeration"],"schema:name":"Good","schema:identifier":"Good"},{"@id":"ocpp:Revoked","@type":["ocpp:CertificateStatusEnumType","schema:Enumeration"],"schema:name":"Revoked","schema:identifier":"Revoked"},{"@id":"ocpp:Unknown","@type":["ocpp:CertificateStatusEnumType","schema:Enumeration"],"schema:name":"Unknown","schema:identifier":"Unknown"},{"@id":"ocpp:Failed","@type":["ocpp:CertificateStatusEnumType","schema:Enumeration"],"schema:name":"Failed","schema:identifier":"Failed"},{"@id":"ocpp:CertificateStatusType","@type":"rdfs:Class","rdfs:label":"CertificateStatusType","rdfs:comment":"Revocation status of certificate\r\n"},{"@id":"ocpp:GetCertificateStatusEnumType","@type":"schema:Enumeration","schema:name":"GetCertificateStatusEnumType","rdfs:comment":"This indicates whether the charging station was able to retrieve the OCSP certificate status.\r\n","schema:hasEnumerationMember":[{"@id":"ocpp:Accepted"},{"@id":"ocpp:Failed"}]},{"@id":"ocpp:Accepted","@type":["ocpp:GetCertificateStatusEnumType","schema:Enumeration"],"schema:name":"Accepted","schema:identifier":"Accepted"},{"@id":"ocpp:Failed","@type":["ocpp:GetCertificateStatusEnumType","schema:Enumeration"],"schema:name":"Failed","schema:identifier":"Failed"},{"@id":"ocpp:ChargingProfileCriterionType","@type":"rdfs:Class","rdfs:label":"ChargingProfileCriterionType","rdfs:comment":"A ChargingProfileCriterionType is a filter for charging profiles to be selected by a GetChargingProfilesRequest.\r\n\r\n"},{"@id":"ocpp:GetChargingProfileStatusEnumType","@type":"schema:Enumeration","schema:name":"GetChargingProfileStatusEnumType","rdfs:comment":"This indicates whether the Charging Station is able to process this request and will send &lt;&lt;reportchargingprofilesrequest, ReportChargingProfilesRequest&gt;&gt; messages.\r\n","schema:hasEnumerationMember":[{"@id":"ocpp:Accepted"},{"@id":"ocpp:NoProfiles"}]},{"@id":"ocpp:Accepted","@type":["ocpp:GetChargingProfileStatusEnumType","schema:Enumeration"],"schema:name":"Accepted","schema:identifier":"Accepted"},{"@id":"ocpp:NoProfiles","@type":["ocpp:GetChargingProfileStatusEnumType","schema:Enumeration"],"schema:name":"NoProfiles","schema:identifier":"NoProfiles"},{"@id":"ocpp:ChargingRateUnitEnumType","@type":"schema:Enumeration","schema:name":"ChargingRateUnitEnumType","rdfs:comment":"The unit of measure in which limits and setpoints are expressed.\r\n","schema:hasEnumerationMember":[{"@id":"ocpp:W"},{"@id":"ocpp:A"}]},{"@id":"ocpp:W","@type":["ocpp:ChargingRateUnitEnumType","schema:Enumeration"],"schema:name":"W","schema:identifier":"W"},{"@id":"ocpp:A","@type":["ocpp:ChargingRateUnitEnumType","schema:Enumeration"],"schema:name":"A","schema:identifier":"A"},{"@id":"ocpp:OperationModeEnumType","@type":"schema:Enumeration","schema:name":"OperationModeEnumType","rdfs:comment":"*(2.1)* The _operationMode_ that is currently in effect for the transaction.\r\n","schema:hasEnumerationMember":[{"@id":"ocpp:Idle"},{"@id":"ocpp:ChargingOnly"},{"@id":"ocpp:CentralSetpoint"},{"@id":"ocpp:ExternalSetpoint"},{"@id":"ocpp:ExternalLimits"},{"@id":"ocpp:CentralFrequency"},{"@id":"ocpp:LocalFrequency"},{"@id":"ocpp:LocalLoadBalancing"}]},{"@id":"ocpp:Idle","@type":["ocpp:OperationModeEnumType","schema:Enumeration"],"schema:name":"Idle","schema:identifier":"Idle"},{"@id":"ocpp:ChargingOnly","@type":["ocpp:OperationModeEnumType","schema:Enumeration"],"schema:name":"ChargingOnly","schema:identifier":"ChargingOnly"},{"@id":"ocpp:CentralSetpoint","@type":["ocpp:OperationModeEnumType","schema:Enumeration"],"schema:name":"CentralSetpoint","schema:identifier":"CentralSetpoint"},{"@id":"ocpp:ExternalSetpoint","@type":["ocpp:OperationModeEnumType","schema:Enumeration"],"schema:name":"ExternalSetpoint","schema:identifier":"ExternalSetpoint"},{"@id":"ocpp:ExternalLimits","@type":["ocpp:OperationModeEnumType","schema:Enumeration"],"schema:name":"ExternalLimits","schema:identifier":"ExternalLimits"},{"@id":"ocpp:CentralFrequency","@type":["ocpp:OperationModeEnumType","schema:Enumeration"],"schema:name":"CentralFrequency","schema:identifier":"CentralFrequency"},{"@id":"ocpp:LocalFrequency","@type":["ocpp:OperationModeEnumType","schema:Enumeration"],"schema:name":"LocalFrequency","schema:identifier":"LocalFrequency"},{"@id":"ocpp:LocalLoadBalancing","@type":["ocpp:OperationModeEnumType","schema:Enumeration"],"schema:name":"LocalLoadBalancing","schema:identifier":"LocalLoadBalancing"},{"@id":"ocpp:ChargingSchedulePeriodType","@type":"rdfs:Class","rdfs:label":"ChargingSchedulePeriodType","rdfs:comment":"Charging schedule period structure defines a time period in a charging schedule. It is used in: CompositeScheduleType and in ChargingScheduleType. When used in a NotifyEVChargingScheduleRequest only _startPeriod_, _limit_, _limit_L2_, _limit_L3_ are relevant.\r\n"},{"@id":"ocpp:CompositeScheduleType","@type":"rdfs:Class","rdfs:label":"CompositeScheduleType"},{"@id":"ocpp:V2XFreqWattPointType","@type":"rdfs:Class","rdfs:label":"V2XFreqWattPointType","rdfs:comment":"*(2.1)* A point of a frequency-watt curve.\r\n"},{"@id":"ocpp:V2XSignalWattPointType","@type":"rdfs:Class","rdfs:label":"V2XSignalWattPointType","rdfs:comment":"*(2.1)* A point of a signal-watt curve.\r\n"},{"@id":"ocpp:MessagePriorityEnumType","@type":"schema:Enumeration","schema:name":"MessagePriorityEnumType","rdfs:comment":"With what priority should this message be shown\r\n","schema:hasEnumerationMember":[{"@id":"ocpp:AlwaysFront"},{"@id":"ocpp:InFront"},{"@id":"ocpp:NormalCycle"}]},{"@id":"ocpp:AlwaysFront","@type":["ocpp:MessagePriorityEnumType","schema:Enumeration"],"schema:name":"AlwaysFront","schema:identifier":"AlwaysFront"},{"@id":"ocpp:InFront","@type":["ocpp:MessagePriorityEnumType","schema:Enumeration"],"schema:name":"InFront","schema:identifier":"InFront"},{"@id":"ocpp:NormalCycle","@type":["ocpp:MessagePriorityEnumType","schema:Enumeration"],"schema:name":"NormalCycle","schema:identifier":"NormalCycle"},{"@id":"ocpp:MessageStateEnumType","@type":"schema:Enumeration","schema:name":"MessageStateEnumType","rdfs:comment":"During what state should this message be shown. When omitted this message should be shown in any state of the Charging Station.\r\n","schema:hasEnumerationMember":[{"@id":"ocpp:Charging"},{"@id":"ocpp:Faulted"},{"@id":"ocpp:Idle"},{"@id":"ocpp:Unavailable"},{"@id":"ocpp:Suspended"},{"@id":"ocpp:Discharging"}]},{"@id":"ocpp:Charging","@type":["ocpp:MessageStateEnumType","schema:Enumeration"],"schema:name":"Charging","schema:identifier":"Charging"},{"@id":"ocpp:Faulted","@type":["ocpp:MessageStateEnumType","schema:Enumeration"],"schema:name":"Faulted","schema:identifier":"Faulted"},{"@id":"ocpp:Idle","@type":["ocpp:MessageStateEnumType","schema:Enumeration"],"schema:name":"Idle","schema:identifier":"Idle"},{"@id":"ocpp:Unavailable","@type":["ocpp:MessageStateEnumType","schema:Enumeration"],"schema:name":"Unavailable","schema:identifier":"Unavailable"},{"@id":"ocpp:Suspended","@type":["ocpp:MessageStateEnumType","schema:Enumeration"],"schema:name":"Suspended","schema:identifier":"Suspended"},{"@id":"ocpp:Discharging","@type":["ocpp:MessageStateEnumType","schema:Enumeration"],"schema:name":"Discharging","schema:identifier":"Discharging"},{"@id":"ocpp:GetDisplayMessagesStatusEnumType","@type":"schema:Enumeration","schema:name":"GetDisplayMessagesStatusEnumType","rdfs:comment":"Indicates if the Charging Station has Display Messages that match the request criteria in the &lt;&lt;getdisplaymessagesrequest,GetDisplayMessagesRequest&gt;&gt;\r\n","schema:hasEnumerationMember":[{"@id":"ocpp:Accepted"},{"@id":"ocpp:Unknown"}]},{"@id":"ocpp:Accepted","@type":["ocpp:GetDisplayMessagesStatusEnumType","schema:Enumeration"],"schema:name":"Accepted","schema:identifier":"Accepted"},{"@id":"ocpp:Unknown","@type":["ocpp:GetDisplayMessagesStatusEnumType","schema:Enumeration"],"schema:name":"Unknown","schema:identifier":"Unknown"},{"@id":"ocpp:GetCertificateIdUseEnumType","@type":"schema:Enumeration","schema:name":"GetCertificateIdUseEnumType","rdfs:comment":"Indicates the type of the requested certificate(s).\r\n","schema:hasEnumerationMember":[{"@id":"ocpp:V2GRootCertificate"},{"@id":"ocpp:MORootCertificate"},{"@id":"ocpp:CSMSRootCertificate"},{"@id":"ocpp:V2GCertificateChain"},{"@id":"ocpp:ManufacturerRootCertificate"},{"@id":"ocpp:OEMRootCertificate"}]},{"@id":"ocpp:V2GRootCertificate","@type":["ocpp:GetCertificateIdUseEnumType","schema:Enumeration"],"schema:name":"V2GRootCertificate","schema:identifier":"V2GRootCertificate"},{"@id":"ocpp:MORootCertificate","@type":["ocpp:GetCertificateIdUseEnumType","schema:Enumeration"],"schema:name":"MORootCertificate","schema:identifier":"MORootCertificate"},{"@id":"ocpp:CSMSRootCertificate","@type":["ocpp:GetCertificateIdUseEnumType","schema:Enumeration"],"schema:name":"CSMSRootCertificate","schema:identifier":"CSMSRootCertificate"},{"@id":"ocpp:V2GCertificateChain","@type":["ocpp:GetCertificateIdUseEnumType","schema:Enumeration"],"schema:name":"V2GCertificateChain","schema:identifier":"V2GCertificateChain"},{"@id":"ocpp:ManufacturerRootCertificate","@type":["ocpp:GetCertificateIdUseEnumType","schema:Enumeration"],"schema:name":"ManufacturerRootCertificate","schema:identifier":"ManufacturerRootCertificate"},{"@id":"ocpp:OEMRootCertificate","@type":["ocpp:GetCertificateIdUseEnumType","schema:Enumeration"],"schema:name":"OEMRootCertificate","schema:identifier":"OEMRootCertificate"},{"@id":"ocpp:GetInstalledCertificateStatusEnumType","@type":"schema:Enumeration","schema:name":"GetInstalledCertificateStatusEnumType","rdfs:comment":"Charging Station indicates if it can process the request.\r\n","schema:hasEnumerationMember":[{"@id":"ocpp:Accepted"},{"@id":"ocpp:NotFound"}]},{"@id":"ocpp:Accepted","@type":["ocpp:GetInstalledCertificateStatusEnumType","schema:Enumeration"],"schema:name":"Accepted","schema:identifier":"Accepted"},{"@id":"ocpp:NotFound","@type":["ocpp:GetInstalledCertificateStatusEnumType","schema:Enumeration"],"schema:name":"NotFound","schema:identifier":"NotFound"},{"@id":"ocpp:CertificateHashDataChainType","@type":"rdfs:Class","rdfs:label":"CertificateHashDataChainType"},{"@id":"ocpp:LogEnumType","@type":"schema:Enumeration","schema:name":"LogEnumType","rdfs:comment":"This contains the type of log file that the Charging Station\r\nshould send.\r\n","schema:hasEnumerationMember":[{"@id":"ocpp:DiagnosticsLog"},{"@id":"ocpp:SecurityLog"},{"@id":"ocpp:DataCollectorLog"}]},{"@id":"ocpp:DiagnosticsLog","@type":["ocpp:LogEnumType","schema:Enumeration"],"schema:name":"DiagnosticsLog","schema:identifier":"DiagnosticsLog"},{"@id":"ocpp:SecurityLog","@type":["ocpp:LogEnumType","schema:Enumeration"],"schema:name":"SecurityLog","schema:identifier":"SecurityLog"},{"@id":"ocpp:DataCollectorLog","@type":["ocpp:LogEnumType","schema:Enumeration"],"schema:name":"DataCollectorLog","schema:identifier":"DataCollectorLog"},{"@id":"ocpp:LogParametersType","@type":"rdfs:Class","rdfs:label":"LogParametersType","rdfs:comment":"Generic class for the configuration of logging entries.\r\n"},{"@id":"ocpp:LogStatusEnumType","@type":"schema:Enumeration","schema:name":"LogStatusEnumType","rdfs:comment":"This field indicates whether the Charging Station was able to accept the request.\r\n","schema:hasEnumerationMember":[{"@id":"ocpp:Accepted"},{"@id":"ocpp:Rejected"},{"@id":"ocpp:AcceptedCanceled"}]},{"@id":"ocpp:Accepted","@type":["ocpp:LogStatusEnumType","schema:Enumeration"],"schema:name":"Accepted","schema:identifier":"Accepted"},{"@id":"ocpp:Rejected","@type":["ocpp:LogStatusEnumType","schema:Enumeration"],"schema:name":"Rejected","schema:identifier":"Rejected"},{"@id":"ocpp:AcceptedCanceled","@type":["ocpp:LogStatusEnumType","schema:Enumeration"],"schema:name":"AcceptedCanceled","schema:identifier":"AcceptedCanceled"},{"@id":"ocpp:MonitoringCriterionEnumType","@type":"schema:Enumeration","schema:name":"MonitoringCriterionEnumType","schema:hasEnumerationMember":[{"@id":"ocpp:ThresholdMonitoring"},{"@id":"ocpp:DeltaMonitoring"},{"@id":"ocpp:PeriodicMonitoring"}]},{"@id":"ocpp:ThresholdMonitoring","@type":["ocpp:MonitoringCriterionEnumType","schema:Enumeration"],"schema:name":"ThresholdMonitoring","schema:identifier":"ThresholdMonitoring"},{"@id":"ocpp:DeltaMonitoring","@type":["ocpp:MonitoringCriterionEnumType","schema:Enumeration"],"schema:name":"DeltaMonitoring","schema:identifier":"DeltaMonitoring"},{"@id":"ocpp:PeriodicMonitoring","@type":["ocpp:MonitoringCriterionEnumType","schema:Enumeration"],"schema:name":"PeriodicMonitoring","schema:identifier":"PeriodicMonitoring"},{"@id":"ocpp:ComponentType","@type":"rdfs:Class","rdfs:label":"ComponentType","rdfs:comment":"A physical or logical component\r\n"},{"@id":"ocpp:ComponentVariableType","@type":"rdfs:Class","rdfs:label":"ComponentVariableType","rdfs:comment":"Class to report components, variables and variable attributes and characteristics.\r\n"},{"@id":"ocpp:VariableType","@type":"rdfs:Class","rdfs:label":"VariableType","rdfs:comment":"Reference key to a component-variable.\r\n"},{"@id":"ocpp:ConstantStreamDataType","@type":"rdfs:Class","rdfs:label":"ConstantStreamDataType"},{"@id":"ocpp:ComponentCriterionEnumType","@type":"schema:Enumeration","schema:name":"ComponentCriterionEnumType","schema:hasEnumerationMember":[{"@id":"ocpp:Active"},{"@id":"ocpp:Available"},{"@id":"ocpp:Enabled"},{"@id":"ocpp:Problem"}]},{"@id":"ocpp:Active","@type":["ocpp:ComponentCriterionEnumType","schema:Enumeration"],"schema:name":"Active","schema:identifier":"Active"},{"@id":"ocpp:Available","@type":["ocpp:ComponentCriterionEnumType","schema:Enumeration"],"schema:name":"Available","schema:identifier":"Available"},{"@id":"ocpp:Enabled","@type":["ocpp:ComponentCriterionEnumType","schema:Enumeration"],"schema:name":"Enabled","schema:identifier":"Enabled"},{"@id":"ocpp:Problem","@type":["ocpp:ComponentCriterionEnumType","schema:Enumeration"],"schema:name":"Problem","schema:identifier":"Problem"},{"@id":"ocpp:TariffGetStatusEnumType","@type":"schema:Enumeration","schema:name":"TariffGetStatusEnumType","rdfs:comment":"Status of operation\r\n","schema:hasEnumerationMember":[{"@id":"ocpp:Accepted"},{"@id":"ocpp:Rejected"},{"@id":"ocpp:NoTariff"}]},{"@id":"ocpp:Accepted","@type":["ocpp:TariffGetStatusEnumType","schema:Enumeration"],"schema:name":"Accepted","schema:identifier":"Accepted"},{"@id":"ocpp:Rejected","@type":["ocpp:TariffGetStatusEnumType","schema:Enumeration"],"schema:name":"Rejected","schema:identifier":"Rejected"},{"@id":"ocpp:NoTariff","@type":["ocpp:TariffGetStatusEnumType","schema:Enumeration"],"schema:name":"NoTariff","schema:identifier":"NoTariff"},{"@id":"ocpp:TariffKindEnumType","@type":"schema:Enumeration","schema:name":"TariffKindEnumType","rdfs:comment":"Kind of tariff (driver/default)\r\n","schema:hasEnumerationMember":[{"@id":"ocpp:DefaultTariff"},{"@id":"ocpp:DriverTariff"}]},{"@id":"ocpp:DefaultTariff","@type":["ocpp:TariffKindEnumType","schema:Enumeration"],"schema:name":"DefaultTariff","schema:identifier":"DefaultTariff"},{"@id":"ocpp:DriverTariff","@type":["ocpp:TariffKindEnumType","schema:Enumeration"],"schema:name":"DriverTariff","schema:identifier":"DriverTariff"},{"@id":"ocpp:TariffAssignmentType","@type":"rdfs:Class","rdfs:label":"TariffAssignmentType","rdfs:comment":"Shows assignment of tariffs to EVSE or IdToken.\r\n"},{"@id":"ocpp:AttributeEnumType","@type":"schema:Enumeration","schema:name":"AttributeEnumType","rdfs:comment":"Type of attribute: Actual, Target, MinSet, MaxSet. Default is Actual when omitted.\r\n","schema:hasEnumerationMember":[{"@id":"ocpp:Actual"},{"@id":"ocpp:Target"},{"@id":"ocpp:MinSet"},{"@id":"ocpp:MaxSet"}]},{"@id":"ocpp:Actual","@type":["ocpp:AttributeEnumType","schema:Enumeration"],"schema:name":"Actual","schema:identifier":"Actual"},{"@id":"ocpp:Target","@type":["ocpp:AttributeEnumType","schema:Enumeration"],"schema:name":"Target","schema:identifier":"Target"},{"@id":"ocpp:MinSet","@type":["ocpp:AttributeEnumType","schema:Enumeration"],"schema:name":"MinSet","schema:identifier":"MinSet"},{"@id":"ocpp:MaxSet","@type":["ocpp:AttributeEnumType","schema:Enumeration"],"schema:name":"MaxSet","schema:identifier":"MaxSet"},{"@id":"ocpp:GetVariableDataType","@type":"rdfs:Class","rdfs:label":"GetVariableDataType","rdfs:comment":"Class to hold parameters for GetVariables request.\r\n"},{"@id":"ocpp:GetVariableStatusEnumType","@type":"schema:Enumeration","schema:name":"GetVariableStatusEnumType","schema:hasEnumerationMember":[{"@id":"ocpp:Accepted"},{"@id":"ocpp:Rejected"},{"@id":"ocpp:UnknownComponent"},{"@id":"ocpp:UnknownVariable"},{"@id":"ocpp:NotSupportedAttributeType"}]},{"@id":"ocpp:Accepted","@type":["ocpp:GetVariableStatusEnumType","schema:Enumeration"],"schema:name":"Accepted","schema:identifier":"Accepted"},{"@id":"ocpp:Rejected","@type":["ocpp:GetVariableStatusEnumType","schema:Enumeration"],"schema:name":"Rejected","schema:identifier":"Rejected"},{"@id":"ocpp:UnknownComponent","@type":["ocpp:GetVariableStatusEnumType","schema:Enumeration"],"schema:name":"UnknownComponent","schema:identifier":"UnknownComponent"},{"@id":"ocpp:UnknownVariable","@type":["ocpp:GetVariableStatusEnumType","schema:Enumeration"],"schema:name":"UnknownVariable","schema:identifier":"UnknownVariable"},{"@id":"ocpp:NotSupportedAttributeType","@type":["ocpp:GetVariableStatusEnumType","schema:Enumeration"],"schema:name":"NotSupportedAttributeType","schema:identifier":"NotSupportedAttributeType"},{"@id":"ocpp:GetVariableResultType","@type":"rdfs:Class","rdfs:label":"GetVariableResultType","rdfs:comment":"Class to hold results of GetVariables request.\r\n"},{"@id":"ocpp:InstallCertificateUseEnumType","@type":"schema:Enumeration","schema:name":"InstallCertificateUseEnumType","rdfs:comment":"Indicates the certificate type that is sent.\r\n","schema:hasEnumerationMember":[{"@id":"ocpp:V2GRootCertificate"},{"@id":"ocpp:MORootCertificate"},{"@id":"ocpp:ManufacturerRootCertificate"},{"@id":"ocpp:CSMSRootCertificate"},{"@id":"ocpp:OEMRootCertificate"}]},{"@id":"ocpp:V2GRootCertificate","@type":["ocpp:InstallCertificateUseEnumType","schema:Enumeration"],"schema:name":"V2GRootCertificate","schema:identifier":"V2GRootCertificate"},{"@id":"ocpp:MORootCertificate","@type":["ocpp:InstallCertificateUseEnumType","schema:Enumeration"],"schema:name":"MORootCertificate","schema:identifier":"MORootCertificate"},{"@id":"ocpp:ManufacturerRootCertificate","@type":["ocpp:InstallCertificateUseEnumType","schema:Enumeration"],"schema:name":"ManufacturerRootCertificate","schema:identifier":"ManufacturerRootCertificate"},{"@id":"ocpp:CSMSRootCertificate","@type":["ocpp:InstallCertificateUseEnumType","schema:Enumeration"],"schema:name":"CSMSRootCertificate","schema:identifier":"CSMSRootCertificate"},{"@id":"ocpp:OEMRootCertificate","@type":["ocpp:InstallCertificateUseEnumType","schema:Enumeration"],"schema:name":"OEMRootCertificate","schema:identifier":"OEMRootCertificate"},{"@id":"ocpp:InstallCertificateStatusEnumType","@type":"schema:Enumeration","schema:name":"InstallCertificateStatusEnumType","rdfs:comment":"Charging Station indicates if installation was successful.\r\n","schema:hasEnumerationMember":[{"@id":"ocpp:Accepted"},{"@id":"ocpp:Rejected"},{"@id":"ocpp:Failed"}]},{"@id":"ocpp:Accepted","@type":["ocpp:InstallCertificateStatusEnumType","schema:Enumeration"],"schema:name":"Accepted","schema:identifier":"Accepted"},{"@id":"ocpp:Rejected","@type":["ocpp:InstallCertificateStatusEnumType","schema:Enumeration"],"schema:name":"Rejected","schema:identifier":"Rejected"},{"@id":"ocpp:Failed","@type":["ocpp:InstallCertificateStatusEnumType","schema:Enumeration"],"schema:name":"Failed","schema:identifier":"Failed"},{"@id":"ocpp:UploadLogStatusEnumType","@type":"schema:Enumeration","schema:name":"UploadLogStatusEnumType","rdfs:comment":"This contains the status of the log upload.\r\n","schema:hasEnumerationMember":[{"@id":"ocpp:BadMessage"},{"@id":"ocpp:Idle"},{"@id":"ocpp:NotSupportedOperation"},{"@id":"ocpp:PermissionDenied"},{"@id":"ocpp:Uploaded"},{"@id":"ocpp:UploadFailure"},{"@id":"ocpp:Uploading"},{"@id":"ocpp:AcceptedCanceled"}]},{"@id":"ocpp:BadMessage","@type":["ocpp:UploadLogStatusEnumType","schema:Enumeration"],"schema:name":"BadMessage","schema:identifier":"BadMessage"},{"@id":"ocpp:Idle","@type":["ocpp:UploadLogStatusEnumType","schema:Enumeration"],"schema:name":"Idle","schema:identifier":"Idle"},{"@id":"ocpp:NotSupportedOperation","@type":["ocpp:UploadLogStatusEnumType","schema:Enumeration"],"schema:name":"NotSupportedOperation","schema:identifier":"NotSupportedOperation"},{"@id":"ocpp:PermissionDenied","@type":["ocpp:UploadLogStatusEnumType","schema:Enumeration"],"schema:name":"PermissionDenied","schema:identifier":"PermissionDenied"},{"@id":"ocpp:Uploaded","@type":["ocpp:UploadLogStatusEnumType","schema:Enumeration"],"schema:name":"Uploaded","schema:identifier":"Uploaded"},{"@id":"ocpp:UploadFailure","@type":["ocpp:UploadLogStatusEnumType","schema:Enumeration"],"schema:name":"UploadFailure","schema:identifier":"UploadFailure"},{"@id":"ocpp:Uploading","@type":["ocpp:UploadLogStatusEnumType","schema:Enumeration"],"schema:name":"Uploading","schema:identifier":"Uploading"},{"@id":"ocpp:AcceptedCanceled","@type":["ocpp:UploadLogStatusEnumType","schema:Enumeration"],"schema:name":"AcceptedCanceled","schema:identifier":"AcceptedCanceled"},{"@id":"ocpp:LocationEnumType","@type":"schema:Enumeration","schema:name":"LocationEnumType","rdfs:comment":"Indicates where the measured value has been sampled. Default =  \"Outlet\"\r\n\r\n","schema:hasEnumerationMember":[{"@id":"ocpp:Body"},{"@id":"ocpp:Cable"},{"@id":"ocpp:EV"},{"@id":"ocpp:Inlet"},{"@id":"ocpp:Outlet"},{"@id":"ocpp:Upstream"}]},{"@id":"ocpp:Body","@type":["ocpp:LocationEnumType","schema:Enumeration"],"schema:name":"Body","schema:identifier":"Body"},{"@id":"ocpp:Cable","@type":["ocpp:LocationEnumType","schema:Enumeration"],"schema:name":"Cable","schema:identifier":"Cable"},{"@id":"ocpp:EV","@type":["ocpp:LocationEnumType","schema:Enumeration"],"schema:name":"EV","schema:identifier":"EV"},{"@id":"ocpp:Inlet","@type":["ocpp:LocationEnumType","schema:Enumeration"],"schema:name":"Inlet","schema:identifier":"Inlet"},{"@id":"ocpp:Outlet","@type":["ocpp:LocationEnumType","schema:Enumeration"],"schema:name":"Outlet","schema:identifier":"Outlet"},{"@id":"ocpp:Upstream","@type":["ocpp:LocationEnumType","schema:Enumeration"],"schema:name":"Upstream","schema:identifier":"Upstream"},{"@id":"ocpp:MeasurandEnumType","@type":"schema:Enumeration","schema:name":"MeasurandEnumType","rdfs:comment":"Type of measurement. Default = \"Energy.Active.Import.Register\"\r\n","schema:hasEnumerationMember":[{"@id":"ocpp:Current.Export"},{"@id":"ocpp:Current.Export.Offered"},{"@id":"ocpp:Current.Export.Minimum"},{"@id":"ocpp:Current.Import"},{"@id":"ocpp:Current.Import.Offered"},{"@id":"ocpp:Current.Import.Minimum"},{"@id":"ocpp:Current.Offered"},{"@id":"ocpp:Display.PresentSOC"},{"@id":"ocpp:Display.MinimumSOC"},{"@id":"ocpp:Display.TargetSOC"},{"@id":"ocpp:Display.MaximumSOC"},{"@id":"ocpp:Display.RemainingTimeToMinimumSOC"},{"@id":"ocpp:Display.RemainingTimeToTargetSOC"},{"@id":"ocpp:Display.RemainingTimeToMaximumSOC"},{"@id":"ocpp:Display.ChargingComplete"},{"@id":"ocpp:Display.BatteryEnergyCapacity"},{"@id":"ocpp:Display.InletHot"},{"@id":"ocpp:Energy.Active.Export.Interval"},{"@id":"ocpp:Energy.Active.Export.Register"},{"@id":"ocpp:Energy.Active.Import.Interval"},{"@id":"ocpp:Energy.Active.Import.Register"},{"@id":"ocpp:Energy.Active.Import.CableLoss"},{"@id":"ocpp:Energy.Active.Import.LocalGeneration.Register"},{"@id":"ocpp:Energy.Active.Net"},{"@id":"ocpp:Energy.Active.Setpoint.Interval"},{"@id":"ocpp:Energy.Apparent.Export"},{"@id":"ocpp:Energy.Apparent.Import"},{"@id":"ocpp:Energy.Apparent.Net"},{"@id":"ocpp:Energy.Reactive.Export.Interval"},{"@id":"ocpp:Energy.Reactive.Export.Register"},{"@id":"ocpp:Energy.Reactive.Import.Interval"},{"@id":"ocpp:Energy.Reactive.Import.Register"},{"@id":"ocpp:Energy.Reactive.Net"},{"@id":"ocpp:EnergyRequest.Target"},{"@id":"ocpp:EnergyRequest.Minimum"},{"@id":"ocpp:EnergyRequest.Maximum"},{"@id":"ocpp:EnergyRequest.Minimum.V2X"},{"@id":"ocpp:EnergyRequest.Maximum.V2X"},{"@id":"ocpp:EnergyRequest.Bulk"},{"@id":"ocpp:Frequency"},{"@id":"ocpp:Power.Active.Export"},{"@id":"ocpp:Power.Active.Import"},{"@id":"ocpp:Power.Active.Setpoint"},{"@id":"ocpp:Power.Active.Residual"},{"@id":"ocpp:Power.Export.Minimum"},{"@id":"ocpp:Power.Export.Offered"},{"@id":"ocpp:Power.Factor"},{"@id":"ocpp:Power.Import.Offered"},{"@id":"ocpp:Power.Import.Minimum"},{"@id":"ocpp:Power.Offered"},{"@id":"ocpp:Power.Reactive.Export"},{"@id":"ocpp:Power.Reactive.Import"},{"@id":"ocpp:SoC"},{"@id":"ocpp:Voltage"},{"@id":"ocpp:Voltage.Minimum"},{"@id":"ocpp:Voltage.Maximum"}]},{"@id":"ocpp:Current.Export","@type":["ocpp:MeasurandEnumType","schema:Enumeration"],"schema:name":"Current.Export","schema:identifier":"Current.Export"},{"@id":"ocpp:Current.Export.Offered","@type":["ocpp:MeasurandEnumType","schema:Enumeration"],"schema:name":"Current.Export.Offered","schema:identifier":"Current.Export.Offered"},{"@id":"ocpp:Current.Export.Minimum","@type":["ocpp:MeasurandEnumType","schema:Enumeration"],"schema:name":"Current.Export.Minimum","schema:identifier":"Current.Export.Minimum"},{"@id":"ocpp:Current.Import","@type":["ocpp:MeasurandEnumType","schema:Enumeration"],"schema:name":"Current.Import","schema:identifier":"Current.Import"},{"@id":"ocpp:Current.Import.Offered","@type":["ocpp:MeasurandEnumType","schema:Enumeration"],"schema:name":"Current.Import.Offered","schema:identifier":"Current.Import.Offered"},{"@id":"ocpp:Current.Import.Minimum","@type":["ocpp:MeasurandEnumType","schema:Enumeration"],"schema:name":"Current.Import.Minimum","schema:identifier":"Current.Import.Minimum"},{"@id":"ocpp:Current.Offered","@type":["ocpp:MeasurandEnumType","schema:Enumeration"],"schema:name":"Current.Offered","schema:identifier":"Current.Offered"},{"@id":"ocpp:Display.PresentSOC","@type":["ocpp:MeasurandEnumType","schema:Enumeration"],"schema:name":"Display.PresentSOC","schema:identifier":"Display.PresentSOC"},{"@id":"ocpp:Display.MinimumSOC","@type":["ocpp:MeasurandEnumType","schema:Enumeration"],"schema:name":"Display.MinimumSOC","schema:identifier":"Display.MinimumSOC"},{"@id":"ocpp:Display.TargetSOC","@type":["ocpp:MeasurandEnumType","schema:Enumeration"],"schema:name":"Display.TargetSOC","schema:identifier":"Display.TargetSOC"},{"@id":"ocpp:Display.MaximumSOC","@type":["ocpp:MeasurandEnumType","schema:Enumeration"],"schema:name":"Display.MaximumSOC","schema:identifier":"Display.MaximumSOC"},{"@id":"ocpp:Display.RemainingTimeToMinimumSOC","@type":["ocpp:MeasurandEnumType","schema:Enumeration"],"schema:name":"Display.RemainingTimeToMinimumSOC","schema:identifier":"Display.RemainingTimeToMinimumSOC"},{"@id":"ocpp:Display.RemainingTimeToTargetSOC","@type":["ocpp:MeasurandEnumType","schema:Enumeration"],"schema:name":"Display.RemainingTimeToTargetSOC","schema:identifier":"Display.RemainingTimeToTargetSOC"},{"@id":"ocpp:Display.RemainingTimeToMaximumSOC","@type":["ocpp:MeasurandEnumType","schema:Enumeration"],"schema:name":"Display.RemainingTimeToMaximumSOC","schema:identifier":"Display.RemainingTimeToMaximumSOC"},{"@id":"ocpp:Display.ChargingComplete","@type":["ocpp:MeasurandEnumType","schema:Enumeration"],"schema:name":"Display.ChargingComplete","schema:identifier":"Display.ChargingComplete"},{"@id":"ocpp:Display.BatteryEnergyCapacity","@type":["ocpp:MeasurandEnumType","schema:Enumeration"],"schema:name":"Display.BatteryEnergyCapacity","schema:identifier":"Display.BatteryEnergyCapacity"},{"@id":"ocpp:Display.InletHot","@type":["ocpp:MeasurandEnumType","schema:Enumeration"],"schema:name":"Display.InletHot","schema:identifier":"Display.InletHot"},{"@id":"ocpp:Energy.Active.Export.Interval","@type":["ocpp:MeasurandEnumType","schema:Enumeration"],"schema:name":"Energy.Active.Export.Interval","schema:identifier":"Energy.Active.Export.Interval"},{"@id":"ocpp:Energy.Active.Export.Register","@type":["ocpp:MeasurandEnumType","schema:Enumeration"],"schema:name":"Energy.Active.Export.Register","schema:identifier":"Energy.Active.Export.Register"},{"@id":"ocpp:Energy.Active.Import.Interval","@type":["ocpp:MeasurandEnumType","schema:Enumeration"],"schema:name":"Energy.Active.Import.Interval","schema:identifier":"Energy.Active.Import.Interval"},{"@id":"ocpp:Energy.Active.Import.Register","@type":["ocpp:MeasurandEnumType","schema:Enumeration"],"schema:name":"Energy.Active.Import.Register","schema:identifier":"Energy.Active.Import.Register"},{"@id":"ocpp:Energy.Active.Import.CableLoss","@type":["ocpp:MeasurandEnumType","schema:Enumeration"],"schema:name":"Energy.Active.Import.CableLoss","schema:identifier":"Energy.Active.Import.CableLoss"},{"@id":"ocpp:Energy.Active.Import.LocalGeneration.Register","@type":["ocpp:MeasurandEnumType","schema:Enumeration"],"schema:name":"Energy.Active.Import.LocalGeneration.Register","schema:identifier":"Energy.Active.Import.LocalGeneration.Register"},{"@id":"ocpp:Energy.Active.Net","@type":["ocpp:MeasurandEnumType","schema:Enumeration"],"schema:name":"Energy.Active.Net","schema:identifier":"Energy.Active.Net"},{"@id":"ocpp:Energy.Active.Setpoint.Interval","@type":["ocpp:MeasurandEnumType","schema:Enumeration"],"schema:name":"Energy.Active.Setpoint.Interval","schema:identifier":"Energy.Active.Setpoint.Interval"},{"@id":"ocpp:Energy.Apparent.Export","@type":["ocpp:MeasurandEnumType","schema:Enumeration"],"schema:name":"Energy.Apparent.Export","schema:identifier":"Energy.Apparent.Export"},{"@id":"ocpp:Energy.Apparent.Import","@type":["ocpp:MeasurandEnumType","schema:Enumeration"],"schema:name":"Energy.Apparent.Import","schema:identifier":"Energy.Apparent.Import"},{"@id":"ocpp:Energy.Apparent.Net","@type":["ocpp:MeasurandEnumType","schema:Enumeration"],"schema:name":"Energy.Apparent.Net","schema:identifier":"Energy.Apparent.Net"},{"@id":"ocpp:Energy.Reactive.Export.Interval","@type":["ocpp:MeasurandEnumType","schema:Enumeration"],"schema:name":"Energy.Reactive.Export.Interval","schema:identifier":"Energy.Reactive.Export.Interval"},{"@id":"ocpp:Energy.Reactive.Export.Register","@type":["ocpp:MeasurandEnumType","schema:Enumeration"],"schema:name":"Energy.Reactive.Export.Register","schema:identifier":"Energy.Reactive.Export.Register"},{"@id":"ocpp:Energy.Reactive.Import.Interval","@type":["ocpp:MeasurandEnumType","schema:Enumeration"],"schema:name":"Energy.Reactive.Import.Interval","schema:identifier":"Energy.Reactive.Import.Interval"},{"@id":"ocpp:Energy.Reactive.Import.Register","@type":["ocpp:MeasurandEnumType","schema:Enumeration"],"schema:name":"Energy.Reactive.Import.Register","schema:identifier":"Energy.Reactive.Import.Register"},{"@id":"ocpp:Energy.Reactive.Net","@type":["ocpp:MeasurandEnumType","schema:Enumeration"],"schema:name":"Energy.Reactive.Net","schema:identifier":"Energy.Reactive.Net"},{"@id":"ocpp:EnergyRequest.Target","@type":["ocpp:MeasurandEnumType","schema:Enumeration"],"schema:name":"EnergyRequest.Target","schema:identifier":"EnergyRequest.Target"},{"@id":"ocpp:EnergyRequest.Minimum","@type":["ocpp:MeasurandEnumType","schema:Enumeration"],"schema:name":"EnergyRequest.Minimum","schema:identifier":"EnergyRequest.Minimum"},{"@id":"ocpp:EnergyRequest.Maximum","@type":["ocpp:MeasurandEnumType","schema:Enumeration"],"schema:name":"EnergyRequest.Maximum","schema:identifier":"EnergyRequest.Maximum"},{"@id":"ocpp:EnergyRequest.Minimum.V2X","@type":["ocpp:MeasurandEnumType","schema:Enumeration"],"schema:name":"EnergyRequest.Minimum.V2X","schema:identifier":"EnergyRequest.Minimum.V2X"},{"@id":"ocpp:EnergyRequest.Maximum.V2X","@type":["ocpp:MeasurandEnumType","schema:Enumeration"],"schema:name":"EnergyRequest.Maximum.V2X","schema:identifier":"EnergyRequest.Maximum.V2X"},{"@id":"ocpp:EnergyRequest.Bulk","@type":["ocpp:MeasurandEnumType","schema:Enumeration"],"schema:name":"EnergyRequest.Bulk","schema:identifier":"EnergyRequest.Bulk"},{"@id":"ocpp:Frequency","@type":["ocpp:MeasurandEnumType","schema:Enumeration"],"schema:name":"Frequency","schema:identifier":"Frequency"},{"@id":"ocpp:Power.Active.Export","@type":["ocpp:MeasurandEnumType","schema:Enumeration"],"schema:name":"Power.Active.Export","schema:identifier":"Power.Active.Export"},{"@id":"ocpp:Power.Active.Import","@type":["ocpp:MeasurandEnumType","schema:Enumeration"],"schema:name":"Power.Active.Import","schema:identifier":"Power.Active.Import"},{"@id":"ocpp:Power.Active.Setpoint","@type":["ocpp:MeasurandEnumType","schema:Enumeration"],"schema:name":"Power.Active.Setpoint","schema:identifier":"Power.Active.Setpoint"},{"@id":"ocpp:Power.Active.Residual","@type":["ocpp:MeasurandEnumType","schema:Enumeration"],"schema:name":"Power.Active.Residual","schema:identifier":"Power.Active.Residual"},{"@id":"ocpp:Power.Export.Minimum","@type":["ocpp:MeasurandEnumType","schema:Enumeration"],"schema:name":"Power.Export.Minimum","schema:identifier":"Power.Export.Minimum"},{"@id":"ocpp:Power.Export.Offered","@type":["ocpp:MeasurandEnumType","schema:Enumeration"],"schema:name":"Power.Export.Offered","schema:identifier":"Power.Export.Offered"},{"@id":"ocpp:Power.Factor","@type":["ocpp:MeasurandEnumType","schema:Enumeration"],"schema:name":"Power.Factor","schema:identifier":"Power.Factor"},{"@id":"ocpp:Power.Import.Offered","@type":["ocpp:MeasurandEnumType","schema:Enumeration"],"schema:name":"Power.Import.Offered","schema:identifier":"Power.Import.Offered"},{"@id":"ocpp:Power.Import.Minimum","@type":["ocpp:MeasurandEnumType","schema:Enumeration"],"schema:name":"Power.Import.Minimum","schema:identifier":"Power.Import.Minimum"},{"@id":"ocpp:Power.Offered","@type":["ocpp:MeasurandEnumType","schema:Enumeration"],"schema:name":"Power.Offered","schema:identifier":"Power.Offered"},{"@id":"ocpp:Power.Reactive.Export","@type":["ocpp:MeasurandEnumType","schema:Enumeration"],"schema:name":"Power.Reactive.Export","schema:identifier":"Power.Reactive.Export"},{"@id":"ocpp:Power.Reactive.Import","@type":["ocpp:MeasurandEnumType","schema:Enumeration"],"schema:name":"Power.Reactive.Import","schema:identifier":"Power.Reactive.Import"},{"@id":"ocpp:SoC","@type":["ocpp:MeasurandEnumType","schema:Enumeration"],"schema:name":"SoC","schema:identifier":"SoC"},{"@id":"ocpp:Voltage","@type":["ocpp:MeasurandEnumType","schema:Enumeration"],"schema:name":"Voltage","schema:identifier":"Voltage"},{"@id":"ocpp:Voltage.Minimum","@type":["ocpp:MeasurandEnumType","schema:Enumeration"],"schema:name":"Voltage.Minimum","schema:identifier":"Voltage.Minimum"},{"@id":"ocpp:Voltage.Maximum","@type":["ocpp:MeasurandEnumType","schema:Enumeration"],"schema:name":"Voltage.Maximum","schema:identifier":"Voltage.Maximum"},{"@id":"ocpp:PhaseEnumType","@type":"schema:Enumeration","schema:name":"PhaseEnumType","rdfs:comment":"Indicates how the measured value is to be interpreted. For instance between L1 and neutral (L1-N) Please note that not all values of phase are applicable to all Measurands. When phase is absent, the measured value is interpreted as an overall value.\r\n","schema:hasEnumerationMember":[{"@id":"ocpp:L1"},{"@id":"ocpp:L2"},{"@id":"ocpp:L3"},{"@id":"ocpp:N"},{"@id":"ocpp:L1-N"},{"@id":"ocpp:L2-N"},{"@id":"ocpp:L3-N"},{"@id":"ocpp:L1-L2"},{"@id":"ocpp:L2-L3"},{"@id":"ocpp:L3-L1"}]},{"@id":"ocpp:L1","@type":["ocpp:PhaseEnumType","schema:Enumeration"],"schema:name":"L1","schema:identifier":"L1"},{"@id":"ocpp:L2","@type":["ocpp:PhaseEnumType","schema:Enumeration"],"schema:name":"L2","schema:identifier":"L2"},{"@id":"ocpp:L3","@type":["ocpp:PhaseEnumType","schema:Enumeration"],"schema:name":"L3","schema:identifier":"L3"},{"@id":"ocpp:N","@type":["ocpp:PhaseEnumType","schema:Enumeration"],"schema:name":"N","schema:identifier":"N"},{"@id":"ocpp:L1-N","@type":["ocpp:PhaseEnumType","schema:Enumeration"],"schema:name":"L1-N","schema:identifier":"L1-N"},{"@id":"ocpp:L2-N","@type":["ocpp:PhaseEnumType","schema:Enumeration"],"schema:name":"L2-N","schema:identifier":"L2-N"},{"@id":"ocpp:L3-N","@type":["ocpp:PhaseEnumType","schema:Enumeration"],"schema:name":"L3-N","schema:identifier":"L3-N"},{"@id":"ocpp:L1-L2","@type":["ocpp:PhaseEnumType","schema:Enumeration"],"schema:name":"L1-L2","schema:identifier":"L1-L2"},{"@id":"ocpp:L2-L3","@type":["ocpp:PhaseEnumType","schema:Enumeration"],"schema:name":"L2-L3","schema:identifier":"L2-L3"},{"@id":"ocpp:L3-L1","@type":["ocpp:PhaseEnumType","schema:Enumeration"],"schema:name":"L3-L1","schema:identifier":"L3-L1"},{"@id":"ocpp:ReadingContextEnumType","@type":"schema:Enumeration","schema:name":"ReadingContextEnumType","rdfs:comment":"Type of detail value: start, end or sample. Default = \"Sample.Periodic\"\r\n","schema:hasEnumerationMember":[{"@id":"ocpp:Interruption.Begin"},{"@id":"ocpp:Interruption.End"},{"@id":"ocpp:Other"},{"@id":"ocpp:Sample.Clock"},{"@id":"ocpp:Sample.Periodic"},{"@id":"ocpp:Transaction.Begin"},{"@id":"ocpp:Transaction.End"},{"@id":"ocpp:Trigger"}]},{"@id":"ocpp:Interruption.Begin","@type":["ocpp:ReadingContextEnumType","schema:Enumeration"],"schema:name":"Interruption.Begin","schema:identifier":"Interruption.Begin"},{"@id":"ocpp:Interruption.End","@type":["ocpp:ReadingContextEnumType","schema:Enumeration"],"schema:name":"Interruption.End","schema:identifier":"Interruption.End"},{"@id":"ocpp:Other","@type":["ocpp:ReadingContextEnumType","schema:Enumeration"],"schema:name":"Other","schema:identifier":"Other"},{"@id":"ocpp:Sample.Clock","@type":["ocpp:ReadingContextEnumType","schema:Enumeration"],"schema:name":"Sample.Clock","schema:identifier":"Sample.Clock"},{"@id":"ocpp:Sample.Periodic","@type":["ocpp:ReadingContextEnumType","schema:Enumeration"],"schema:name":"Sample.Periodic","schema:identifier":"Sample.Periodic"},{"@id":"ocpp:Transaction.Begin","@type":["ocpp:ReadingContextEnumType","schema:Enumeration"],"schema:name":"Transaction.Begin","schema:identifier":"Transaction.Begin"},{"@id":"ocpp:Transaction.End","@type":["ocpp:ReadingContextEnumType","schema:Enumeration"],"schema:name":"Transaction.End","schema:identifier":"Transaction.End"},{"@id":"ocpp:Trigger","@type":["ocpp:ReadingContextEnumType","schema:Enumeration"],"schema:name":"Trigger","schema:identifier":"Trigger"},{"@id":"ocpp:MeterValueType","@type":"rdfs:Class","rdfs:label":"MeterValueType","rdfs:comment":"Collection of one or more sampled values in MeterValuesRequest and TransactionEvent. All sampled values in a MeterValue are sampled at the same point in time.\r\n"},{"@id":"ocpp:SampledValueType","@type":"rdfs:Class","rdfs:label":"SampledValueType","rdfs:comment":"Single sampled value in MeterValues. Each value can be accompanied by optional fields.\r\n\r\nTo save on mobile data usage, default values of all of the optional fields are such that. The value without any additional fields will be interpreted, as a register reading of active import energy in Wh (Watt-hour) units.\r\n"},{"@id":"ocpp:SignedMeterValueType","@type":"rdfs:Class","rdfs:label":"SignedMeterValueType","rdfs:comment":"Represent a signed version of the meter value.\r\n"},{"@id":"ocpp:UnitOfMeasureType","@type":"rdfs:Class","rdfs:label":"UnitOfMeasureType","rdfs:comment":"Represents a UnitOfMeasure with a multiplier\r\n"},{"@id":"ocpp:NotifyAllowedEnergyTransferStatusEnumType","@type":"schema:Enumeration","schema:name":"NotifyAllowedEnergyTransferStatusEnumType","schema:hasEnumerationMember":[{"@id":"ocpp:Accepted"},{"@id":"ocpp:Rejected"}]},{"@id":"ocpp:Accepted","@type":["ocpp:NotifyAllowedEnergyTransferStatusEnumType","schema:Enumeration"],"schema:name":"Accepted","schema:identifier":"Accepted"},{"@id":"ocpp:Rejected","@type":["ocpp:NotifyAllowedEnergyTransferStatusEnumType","schema:Enumeration"],"schema:name":"Rejected","schema:identifier":"Rejected"},{"@id":"ocpp:CostKindEnumType","@type":"schema:Enumeration","schema:name":"CostKindEnumType","rdfs:comment":"The kind of cost referred to in the message element amount\r\n","schema:hasEnumerationMember":[{"@id":"ocpp:CarbonDioxideEmission"},{"@id":"ocpp:RelativePricePercentage"},{"@id":"ocpp:RenewableGenerationPercentage"}]},{"@id":"ocpp:CarbonDioxideEmission","@type":["ocpp:CostKindEnumType","schema:Enumeration"],"schema:name":"CarbonDioxideEmission","schema:identifier":"CarbonDioxideEmission"},{"@id":"ocpp:RelativePricePercentage","@type":["ocpp:CostKindEnumType","schema:Enumeration"],"schema:name":"RelativePricePercentage","schema:identifier":"RelativePricePercentage"},{"@id":"ocpp:RenewableGenerationPercentage","@type":["ocpp:CostKindEnumType","schema:Enumeration"],"schema:name":"RenewableGenerationPercentage","schema:identifier":"RenewableGenerationPercentage"},{"@id":"ocpp:AbsolutePriceScheduleType","@type":"rdfs:Class","rdfs:label":"AbsolutePriceScheduleType","rdfs:comment":"The AbsolutePriceScheduleType is modeled after the same type that is defined in ISO 15118-20, such that if it is supplied by an EMSP as a signed EXI message, the conversion from EXI to JSON (in OCPP) and back to EXI (for ISO 15118-20) does not change the digest and therefore does not invalidate the signature.\r\n\r\nimage::images/AbsolutePriceSchedule-Simple.png[]\r\n\r\n"},{"@id":"ocpp:AdditionalSelectedServicesType","@type":"rdfs:Class","rdfs:label":"AdditionalSelectedServicesType","rdfs:comment":"Part of ISO 15118-20 price schedule.\r\n\r\n"},{"@id":"ocpp:ChargingLimitType","@type":"rdfs:Class","rdfs:label":"ChargingLimitType"},{"@id":"ocpp:ChargingScheduleType","@type":"rdfs:Class","rdfs:label":"ChargingScheduleType","rdfs:comment":"Charging schedule structure defines a list of charging periods, as used in: NotifyEVChargingScheduleRequest and ChargingProfileType. When used in a NotifyEVChargingScheduleRequest only _duration_ and _chargingSchedulePeriod_ are relevant and _chargingRateUnit_ must be 'W'. +\r\nAn ISO 15118-20 session may provide either an _absolutePriceSchedule_ or a _priceLevelSchedule_. An ISO 15118-2 session can only provide a_salesTariff_ element. The field _digestValue_ is used when price schedule or sales tariff are signed.\r\n\r\nimage::images/ChargingSchedule-Simple.png[]\r\n\r\n\r\n"},{"@id":"ocpp:ConsumptionCostType","@type":"rdfs:Class","rdfs:label":"ConsumptionCostType"},{"@id":"ocpp:CostType","@type":"rdfs:Class","rdfs:label":"CostType"},{"@id":"ocpp:LimitAtSoCType","@type":"rdfs:Class","rdfs:label":"LimitAtSoCType"},{"@id":"ocpp:OverstayRuleListType","@type":"rdfs:Class","rdfs:label":"OverstayRuleListType","rdfs:comment":"Part of ISO 15118-20 price schedule.\r\n\r\n"},{"@id":"ocpp:OverstayRuleType","@type":"rdfs:Class","rdfs:label":"OverstayRuleType","rdfs:comment":"Part of ISO 15118-20 price schedule.\r\n\r\n"},{"@id":"ocpp:PriceLevelScheduleEntryType","@type":"rdfs:Class","rdfs:label":"PriceLevelScheduleEntryType","rdfs:comment":"Part of ISO 15118-20 price schedule.\r\n"},{"@id":"ocpp:PriceLevelScheduleType","@type":"rdfs:Class","rdfs:label":"PriceLevelScheduleType","rdfs:comment":"The PriceLevelScheduleType is modeled after the same type that is defined in ISO 15118-20, such that if it is supplied by an EMSP as a signed EXI message, the conversion from EXI to JSON (in OCPP) and back to EXI (for ISO 15118-20) does not change the digest and therefore does not invalidate the signature.\r\n"},{"@id":"ocpp:PriceRuleStackType","@type":"rdfs:Class","rdfs:label":"PriceRuleStackType","rdfs:comment":"Part of ISO 15118-20 price schedule.\r\n"},{"@id":"ocpp:PriceRuleType","@type":"rdfs:Class","rdfs:label":"PriceRuleType","rdfs:comment":"Part of ISO 15118-20 price schedule.\r\n\r\n"},{"@id":"ocpp:RationalNumberType","@type":"rdfs:Class","rdfs:label":"RationalNumberType","rdfs:comment":"Part of ISO 15118-20 price schedule.\r\n\r\n"},{"@id":"ocpp:RelativeTimeIntervalType","@type":"rdfs:Class","rdfs:label":"RelativeTimeIntervalType"},{"@id":"ocpp:SalesTariffEntryType","@type":"rdfs:Class","rdfs:label":"SalesTariffEntryType"},{"@id":"ocpp:SalesTariffType","@type":"rdfs:Class","rdfs:label":"SalesTariffType","rdfs:comment":"A SalesTariff provided by a Mobility Operator (EMSP) .\r\nNOTE: This dataType is based on dataTypes from &lt;&lt;ref-ISOIEC15118-2,ISO 15118-2&gt;&gt;.\r\n"},{"@id":"ocpp:TaxRuleType","@type":"rdfs:Class","rdfs:label":"TaxRuleType","rdfs:comment":"Part of ISO 15118-20 price schedule.\r\n\r\n"},{"@id":"ocpp:GridEventFaultEnumType","@type":"schema:Enumeration","schema:name":"GridEventFaultEnumType","rdfs:comment":"Type of grid event that caused this\r\n\r\n","schema:hasEnumerationMember":[{"@id":"ocpp:CurrentImbalance"},{"@id":"ocpp:LocalEmergency"},{"@id":"ocpp:LowInputPower"},{"@id":"ocpp:OverCurrent"},{"@id":"ocpp:OverFrequency"},{"@id":"ocpp:OverVoltage"},{"@id":"ocpp:PhaseRotation"},{"@id":"ocpp:RemoteEmergency"},{"@id":"ocpp:UnderFrequency"},{"@id":"ocpp:UnderVoltage"},{"@id":"ocpp:VoltageImbalance"}]},{"@id":"ocpp:CurrentImbalance","@type":["ocpp:GridEventFaultEnumType","schema:Enumeration"],"schema:name":"CurrentImbalance","schema:identifier":"CurrentImbalance"},{"@id":"ocpp:LocalEmergency","@type":["ocpp:GridEventFaultEnumType","schema:Enumeration"],"schema:name":"LocalEmergency","schema:identifier":"LocalEmergency"},{"@id":"ocpp:LowInputPower","@type":["ocpp:GridEventFaultEnumType","schema:Enumeration"],"schema:name":"LowInputPower","schema:identifier":"LowInputPower"},{"@id":"ocpp:OverCurrent","@type":["ocpp:GridEventFaultEnumType","schema:Enumeration"],"schema:name":"OverCurrent","schema:identifier":"OverCurrent"},{"@id":"ocpp:OverFrequency","@type":["ocpp:GridEventFaultEnumType","schema:Enumeration"],"schema:name":"OverFrequency","schema:identifier":"OverFrequency"},{"@id":"ocpp:OverVoltage","@type":["ocpp:GridEventFaultEnumType","schema:Enumeration"],"schema:name":"OverVoltage","schema:identifier":"OverVoltage"},{"@id":"ocpp:PhaseRotation","@type":["ocpp:GridEventFaultEnumType","schema:Enumeration"],"schema:name":"PhaseRotation","schema:identifier":"PhaseRotation"},{"@id":"ocpp:RemoteEmergency","@type":["ocpp:GridEventFaultEnumType","schema:Enumeration"],"schema:name":"RemoteEmergency","schema:identifier":"RemoteEmergency"},{"@id":"ocpp:UnderFrequency","@type":["ocpp:GridEventFaultEnumType","schema:Enumeration"],"schema:name":"UnderFrequency","schema:identifier":"UnderFrequency"},{"@id":"ocpp:UnderVoltage","@type":["ocpp:GridEventFaultEnumType","schema:Enumeration"],"schema:name":"UnderVoltage","schema:identifier":"UnderVoltage"},{"@id":"ocpp:VoltageImbalance","@type":["ocpp:GridEventFaultEnumType","schema:Enumeration"],"schema:name":"VoltageImbalance","schema:identifier":"VoltageImbalance"},{"@id":"ocpp:MessageInfoType","@type":"rdfs:Class","rdfs:label":"MessageInfoType","rdfs:comment":"Contains message details, for a message to be displayed on a Charging Station.\r\n"},{"@id":"ocpp:ControlModeEnumType","@type":"schema:Enumeration","schema:name":"ControlModeEnumType","rdfs:comment":"*(2.1)* Indicates whether EV wants to operate in Dynamic or Scheduled mode. When absent, Scheduled mode is assumed for backwards compatibility. +\r\n*ISO 15118-20:* +\r\nServiceSelectionReq(SelectedEnergyTransferService)\r\n","schema:hasEnumerationMember":[{"@id":"ocpp:ScheduledControl"},{"@id":"ocpp:DynamicControl"}]},{"@id":"ocpp:ScheduledControl","@type":["ocpp:ControlModeEnumType","schema:Enumeration"],"schema:name":"ScheduledControl","schema:identifier":"ScheduledControl"},{"@id":"ocpp:DynamicControl","@type":["ocpp:ControlModeEnumType","schema:Enumeration"],"schema:name":"DynamicControl","schema:identifier":"DynamicControl"},{"@id":"ocpp:IslandingDetectionEnumType","@type":"schema:Enumeration","schema:name":"IslandingDetectionEnumType","schema:hasEnumerationMember":[{"@id":"ocpp:NoAntiIslandingSupport"},{"@id":"ocpp:RoCoF"},{"@id":"ocpp:UVP_OVP"},{"@id":"ocpp:UFP_OFP"},{"@id":"ocpp:VoltageVectorShift"},{"@id":"ocpp:ZeroCrossingDetection"},{"@id":"ocpp:OtherPassive"},{"@id":"ocpp:ImpedanceMeasurement"},{"@id":"ocpp:ImpedanceAtFrequency"},{"@id":"ocpp:SlipModeFrequencyShift"},{"@id":"ocpp:SandiaFrequencyShift"},{"@id":"ocpp:SandiaVoltageShift"},{"@id":"ocpp:FrequencyJump"},{"@id":"ocpp:RCLQFactor"},{"@id":"ocpp:OtherActive"}]},{"@id":"ocpp:NoAntiIslandingSupport","@type":["ocpp:IslandingDetectionEnumType","schema:Enumeration"],"schema:name":"NoAntiIslandingSupport","schema:identifier":"NoAntiIslandingSupport"},{"@id":"ocpp:RoCoF","@type":["ocpp:IslandingDetectionEnumType","schema:Enumeration"],"schema:name":"RoCoF","schema:identifier":"RoCoF"},{"@id":"ocpp:UVP_OVP","@type":["ocpp:IslandingDetectionEnumType","schema:Enumeration"],"schema:name":"UVP_OVP","schema:identifier":"UVP_OVP"},{"@id":"ocpp:UFP_OFP","@type":["ocpp:IslandingDetectionEnumType","schema:Enumeration"],"schema:name":"UFP_OFP","schema:identifier":"UFP_OFP"},{"@id":"ocpp:VoltageVectorShift","@type":["ocpp:IslandingDetectionEnumType","schema:Enumeration"],"schema:name":"VoltageVectorShift","schema:identifier":"VoltageVectorShift"},{"@id":"ocpp:ZeroCrossingDetection","@type":["ocpp:IslandingDetectionEnumType","schema:Enumeration"],"schema:name":"ZeroCrossingDetection","schema:identifier":"ZeroCrossingDetection"},{"@id":"ocpp:OtherPassive","@type":["ocpp:IslandingDetectionEnumType","schema:Enumeration"],"schema:name":"OtherPassive","schema:identifier":"OtherPassive"},{"@id":"ocpp:ImpedanceMeasurement","@type":["ocpp:IslandingDetectionEnumType","schema:Enumeration"],"schema:name":"ImpedanceMeasurement","schema:identifier":"ImpedanceMeasurement"},{"@id":"ocpp:ImpedanceAtFrequency","@type":["ocpp:IslandingDetectionEnumType","schema:Enumeration"],"schema:name":"ImpedanceAtFrequency","schema:identifier":"ImpedanceAtFrequency"},{"@id":"ocpp:SlipModeFrequencyShift","@type":["ocpp:IslandingDetectionEnumType","schema:Enumeration"],"schema:name":"SlipModeFrequencyShift","schema:identifier":"SlipModeFrequencyShift"},{"@id":"ocpp:SandiaFrequencyShift","@type":["ocpp:IslandingDetectionEnumType","schema:Enumeration"],"schema:name":"SandiaFrequencyShift","schema:identifier":"SandiaFrequencyShift"},{"@id":"ocpp:SandiaVoltageShift","@type":["ocpp:IslandingDetectionEnumType","schema:Enumeration"],"schema:name":"SandiaVoltageShift","schema:identifier":"SandiaVoltageShift"},{"@id":"ocpp:FrequencyJump","@type":["ocpp:IslandingDetectionEnumType","schema:Enumeration"],"schema:name":"FrequencyJump","schema:identifier":"FrequencyJump"},{"@id":"ocpp:RCLQFactor","@type":["ocpp:IslandingDetectionEnumType","schema:Enumeration"],"schema:name":"RCLQFactor","schema:identifier":"RCLQFactor"},{"@id":"ocpp:OtherActive","@type":["ocpp:IslandingDetectionEnumType","schema:Enumeration"],"schema:name":"OtherActive","schema:identifier":"OtherActive"},{"@id":"ocpp:MobilityNeedsModeEnumType","@type":"schema:Enumeration","schema:name":"MobilityNeedsModeEnumType","rdfs:comment":"*(2.1)* Value of EVCC indicates that EV determines min/target SOC and departure time. +\r\nA value of EVCC_SECC indicates that charging station or CSMS may also update min/target SOC and departure time. +\r\n*ISO 15118-20:* +\r\nServiceSelectionReq(SelectedEnergyTransferService)\r\n","schema:hasEnumerationMember":[{"@id":"ocpp:EVCC"},{"@id":"ocpp:EVCC_SECC"}]},{"@id":"ocpp:EVCC","@type":["ocpp:MobilityNeedsModeEnumType","schema:Enumeration"],"schema:name":"EVCC","schema:identifier":"EVCC"},{"@id":"ocpp:EVCC_SECC","@type":["ocpp:MobilityNeedsModeEnumType","schema:Enumeration"],"schema:name":"EVCC_SECC","schema:identifier":"EVCC_SECC"},{"@id":"ocpp:ACChargingParametersType","@type":"rdfs:Class","rdfs:label":"ACChargingParametersType","rdfs:comment":"EV AC charging parameters for ISO 15118-2\r\n\r\n"},{"@id":"ocpp:ChargingNeedsType","@type":"rdfs:Class","rdfs:label":"ChargingNeedsType"},{"@id":"ocpp:DCChargingParametersType","@type":"rdfs:Class","rdfs:label":"DCChargingParametersType","rdfs:comment":"EV DC charging parameters for ISO 15118-2\r\n"},{"@id":"ocpp:DERChargingParametersType","@type":"rdfs:Class","rdfs:label":"DERChargingParametersType","rdfs:comment":"*(2.1)* DERChargingParametersType is used in ChargingNeedsType during an ISO 15118-20 session for AC_BPT_DER to report the inverter settings related to DER control that were agreed between EVSE and EV.\r\n\r\nFields starting with \"ev\" contain values from the EV.\r\nOther fields contain a value that is supported by both EV and EVSE.\r\n\r\nDERChargingParametersType type is only relevant in case of an ISO 15118-20 AC_BPT_DER/AC_DER charging session.\r\n\r\nNOTE: All these fields have values greater or equal to zero (i.e. are non-negative)\r\n\r\n"},{"@id":"ocpp:EVAbsolutePriceScheduleEntryType","@type":"rdfs:Class","rdfs:label":"EVAbsolutePriceScheduleEntryType","rdfs:comment":"*(2.1)* An entry in price schedule over time for which EV is willing to discharge.\r\n"},{"@id":"ocpp:EVAbsolutePriceScheduleType","@type":"rdfs:Class","rdfs:label":"EVAbsolutePriceScheduleType","rdfs:comment":"*(2.1)* Price schedule of EV energy offer.\r\n"},{"@id":"ocpp:EVEnergyOfferType","@type":"rdfs:Class","rdfs:label":"EVEnergyOfferType","rdfs:comment":"*(2.1)* A schedule of the energy amount over time that EV is willing to discharge. A negative value indicates the willingness to discharge under specific conditions, a positive value indicates that the EV currently is not able to offer energy to discharge. \r\n"},{"@id":"ocpp:EVPowerScheduleEntryType","@type":"rdfs:Class","rdfs:label":"EVPowerScheduleEntryType","rdfs:comment":"*(2.1)* An entry in schedule of the energy amount over time that EV is willing to discharge. A negative value indicates the willingness to discharge under specific conditions, a positive value indicates that the EV currently is not able to offer energy to discharge.\r\n"},{"@id":"ocpp:EVPowerScheduleType","@type":"rdfs:Class","rdfs:label":"EVPowerScheduleType","rdfs:comment":"*(2.1)* Schedule of EV energy offer.\r\n"},{"@id":"ocpp:EVPriceRuleType","@type":"rdfs:Class","rdfs:label":"EVPriceRuleType","rdfs:comment":"*(2.1)* An entry in price schedule over time for which EV is willing to discharge.\r\n"},{"@id":"ocpp:V2XChargingParametersType","@type":"rdfs:Class","rdfs:label":"V2XChargingParametersType","rdfs:comment":"Charging parameters for ISO 15118-20, also supporting V2X charging/discharging.+\r\nAll values are greater or equal to zero, with the exception of EVMinEnergyRequest, EVMaxEnergyRequest, EVTargetEnergyRequest, EVMinV2XEnergyRequest and EVMaxV2XEnergyRequest.\r\n"},{"@id":"ocpp:NotifyEVChargingNeedsStatusEnumType","@type":"schema:Enumeration","schema:name":"NotifyEVChargingNeedsStatusEnumType","rdfs:comment":"Returns whether the CSMS has been able to process the message successfully. It does not imply that the evChargingNeeds can be met with the current charging profile.\r\n","schema:hasEnumerationMember":[{"@id":"ocpp:Accepted"},{"@id":"ocpp:Rejected"},{"@id":"ocpp:Processing"},{"@id":"ocpp:NoChargingProfile"}]},{"@id":"ocpp:Accepted","@type":["ocpp:NotifyEVChargingNeedsStatusEnumType","schema:Enumeration"],"schema:name":"Accepted","schema:identifier":"Accepted"},{"@id":"ocpp:Rejected","@type":["ocpp:NotifyEVChargingNeedsStatusEnumType","schema:Enumeration"],"schema:name":"Rejected","schema:identifier":"Rejected"},{"@id":"ocpp:Processing","@type":["ocpp:NotifyEVChargingNeedsStatusEnumType","schema:Enumeration"],"schema:name":"Processing","schema:identifier":"Processing"},{"@id":"ocpp:NoChargingProfile","@type":["ocpp:NotifyEVChargingNeedsStatusEnumType","schema:Enumeration"],"schema:name":"NoChargingProfile","schema:identifier":"NoChargingProfile"},{"@id":"ocpp:EventNotificationEnumType","@type":"schema:Enumeration","schema:name":"EventNotificationEnumType","rdfs:comment":"*(2.1)* Type of monitor.\r\n","schema:hasEnumerationMember":[{"@id":"ocpp:HardWiredNotification"},{"@id":"ocpp:HardWiredMonitor"},{"@id":"ocpp:PreconfiguredMonitor"},{"@id":"ocpp:CustomMonitor"}]},{"@id":"ocpp:HardWiredNotification","@type":["ocpp:EventNotificationEnumType","schema:Enumeration"],"schema:name":"HardWiredNotification","schema:identifier":"HardWiredNotification"},{"@id":"ocpp:HardWiredMonitor","@type":["ocpp:EventNotificationEnumType","schema:Enumeration"],"schema:name":"HardWiredMonitor","schema:identifier":"HardWiredMonitor"},{"@id":"ocpp:PreconfiguredMonitor","@type":["ocpp:EventNotificationEnumType","schema:Enumeration"],"schema:name":"PreconfiguredMonitor","schema:identifier":"PreconfiguredMonitor"},{"@id":"ocpp:CustomMonitor","@type":["ocpp:EventNotificationEnumType","schema:Enumeration"],"schema:name":"CustomMonitor","schema:identifier":"CustomMonitor"},{"@id":"ocpp:EventTriggerEnumType","@type":"schema:Enumeration","schema:name":"EventTriggerEnumType","rdfs:comment":"Type of trigger for this event, e.g. exceeding a threshold value.\r\n\r\n","schema:hasEnumerationMember":[{"@id":"ocpp:Alerting"},{"@id":"ocpp:Delta"},{"@id":"ocpp:Periodic"}]},{"@id":"ocpp:Alerting","@type":["ocpp:EventTriggerEnumType","schema:Enumeration"],"schema:name":"Alerting","schema:identifier":"Alerting"},{"@id":"ocpp:Delta","@type":["ocpp:EventTriggerEnumType","schema:Enumeration"],"schema:name":"Delta","schema:identifier":"Delta"},{"@id":"ocpp:Periodic","@type":["ocpp:EventTriggerEnumType","schema:Enumeration"],"schema:name":"Periodic","schema:identifier":"Periodic"},{"@id":"ocpp:EventDataType","@type":"rdfs:Class","rdfs:label":"EventDataType","rdfs:comment":"Class to report an event notification for a component-variable.\r\n"},{"@id":"ocpp:MonitorEnumType","@type":"schema:Enumeration","schema:name":"MonitorEnumType","rdfs:comment":"The type of this monitor, e.g. a threshold, delta or periodic monitor. \r\n\r\n","schema:hasEnumerationMember":[{"@id":"ocpp:UpperThreshold"},{"@id":"ocpp:LowerThreshold"},{"@id":"ocpp:Delta"},{"@id":"ocpp:Periodic"},{"@id":"ocpp:PeriodicClockAligned"},{"@id":"ocpp:TargetDelta"},{"@id":"ocpp:TargetDeltaRelative"}]},{"@id":"ocpp:UpperThreshold","@type":["ocpp:MonitorEnumType","schema:Enumeration"],"schema:name":"UpperThreshold","schema:identifier":"UpperThreshold"},{"@id":"ocpp:LowerThreshold","@type":["ocpp:MonitorEnumType","schema:Enumeration"],"schema:name":"LowerThreshold","schema:identifier":"LowerThreshold"},{"@id":"ocpp:Delta","@type":["ocpp:MonitorEnumType","schema:Enumeration"],"schema:name":"Delta","schema:identifier":"Delta"},{"@id":"ocpp:Periodic","@type":["ocpp:MonitorEnumType","schema:Enumeration"],"schema:name":"Periodic","schema:identifier":"Periodic"},{"@id":"ocpp:PeriodicClockAligned","@type":["ocpp:MonitorEnumType","schema:Enumeration"],"schema:name":"PeriodicClockAligned","schema:identifier":"PeriodicClockAligned"},{"@id":"ocpp:TargetDelta","@type":["ocpp:MonitorEnumType","schema:Enumeration"],"schema:name":"TargetDelta","schema:identifier":"TargetDelta"},{"@id":"ocpp:TargetDeltaRelative","@type":["ocpp:MonitorEnumType","schema:Enumeration"],"schema:name":"TargetDeltaRelative","schema:identifier":"TargetDeltaRelative"},{"@id":"ocpp:MonitoringDataType","@type":"rdfs:Class","rdfs:label":"MonitoringDataType","rdfs:comment":"Class to hold parameters of SetVariableMonitoring request.\r\n"},{"@id":"ocpp:VariableMonitoringType","@type":"rdfs:Class","rdfs:label":"VariableMonitoringType","rdfs:comment":"A monitoring setting for a variable.\r\n"},{"@id":"ocpp:StreamDataElementType","@type":"rdfs:Class","rdfs:label":"StreamDataElementType"},{"@id":"ocpp:DataEnumType","@type":"schema:Enumeration","schema:name":"DataEnumType","rdfs:comment":"Data type of this variable.\r\n","schema:hasEnumerationMember":[{"@id":"ocpp:string"},{"@id":"ocpp:decimal"},{"@id":"ocpp:integer"},{"@id":"ocpp:dateTime"},{"@id":"ocpp:boolean"},{"@id":"ocpp:OptionList"},{"@id":"ocpp:SequenceList"},{"@id":"ocpp:MemberList"}]},{"@id":"ocpp:string","@type":["ocpp:DataEnumType","schema:Enumeration"],"schema:name":"string","schema:identifier":"string"},{"@id":"ocpp:decimal","@type":["ocpp:DataEnumType","schema:Enumeration"],"schema:name":"decimal","schema:identifier":"decimal"},{"@id":"ocpp:integer","@type":["ocpp:DataEnumType","schema:Enumeration"],"schema:name":"integer","schema:identifier":"integer"},{"@id":"ocpp:dateTime","@type":["ocpp:DataEnumType","schema:Enumeration"],"schema:name":"dateTime","schema:identifier":"dateTime"},{"@id":"ocpp:boolean","@type":["ocpp:DataEnumType","schema:Enumeration"],"schema:name":"boolean","schema:identifier":"boolean"},{"@id":"ocpp:OptionList","@type":["ocpp:DataEnumType","schema:Enumeration"],"schema:name":"OptionList","schema:identifier":"OptionList"},{"@id":"ocpp:SequenceList","@type":["ocpp:DataEnumType","schema:Enumeration"],"schema:name":"SequenceList","schema:identifier":"SequenceList"},{"@id":"ocpp:MemberList","@type":["ocpp:DataEnumType","schema:Enumeration"],"schema:name":"MemberList","schema:identifier":"MemberList"},{"@id":"ocpp:MutabilityEnumType","@type":"schema:Enumeration","schema:name":"MutabilityEnumType","rdfs:comment":"Defines the mutability of this attribute. Default is ReadWrite when omitted.\r\n","schema:hasEnumerationMember":[{"@id":"ocpp:ReadOnly"},{"@id":"ocpp:WriteOnly"},{"@id":"ocpp:ReadWrite"}]},{"@id":"ocpp:ReadOnly","@type":["ocpp:MutabilityEnumType","schema:Enumeration"],"schema:name":"ReadOnly","schema:identifier":"ReadOnly"},{"@id":"ocpp:WriteOnly","@type":["ocpp:MutabilityEnumType","schema:Enumeration"],"schema:name":"WriteOnly","schema:identifier":"WriteOnly"},{"@id":"ocpp:ReadWrite","@type":["ocpp:MutabilityEnumType","schema:Enumeration"],"schema:name":"ReadWrite","schema:identifier":"ReadWrite"},{"@id":"ocpp:ReportDataType","@type":"rdfs:Class","rdfs:label":"ReportDataType","rdfs:comment":"Class to report components, variables and variable attributes and characteristics.\r\n"},{"@id":"ocpp:VariableAttributeType","@type":"rdfs:Class","rdfs:label":"VariableAttributeType","rdfs:comment":"Attribute data of a variable.\r\n"},{"@id":"ocpp:VariableCharacteristicsType","@type":"rdfs:Class","rdfs:label":"VariableCharacteristicsType","rdfs:comment":"Fixed read-only parameters of a variable.\r\n"},{"@id":"ocpp:PaymentStatusEnumType","@type":"schema:Enumeration","schema:name":"PaymentStatusEnumType","rdfs:comment":"The status of the settlement attempt.\r\n\r\n","schema:hasEnumerationMember":[{"@id":"ocpp:Settled"},{"@id":"ocpp:Canceled"},{"@id":"ocpp:Rejected"},{"@id":"ocpp:Failed"}]},{"@id":"ocpp:Settled","@type":["ocpp:PaymentStatusEnumType","schema:Enumeration"],"schema:name":"Settled","schema:identifier":"Settled"},{"@id":"ocpp:Canceled","@type":["ocpp:PaymentStatusEnumType","schema:Enumeration"],"schema:name":"Canceled","schema:identifier":"Canceled"},{"@id":"ocpp:Rejected","@type":["ocpp:PaymentStatusEnumType","schema:Enumeration"],"schema:name":"Rejected","schema:identifier":"Rejected"},{"@id":"ocpp:Failed","@type":["ocpp:PaymentStatusEnumType","schema:Enumeration"],"schema:name":"Failed","schema:identifier":"Failed"},{"@id":"ocpp:AddressType","@type":"rdfs:Class","rdfs:label":"AddressType","rdfs:comment":"*(2.1)* A generic address format.\r\n"},{"@id":"ocpp:PublishFirmwareStatusEnumType","@type":"schema:Enumeration","schema:name":"PublishFirmwareStatusEnumType","rdfs:comment":"This contains the progress status of the publishfirmware\r\ninstallation.\r\n","schema:hasEnumerationMember":[{"@id":"ocpp:Idle"},{"@id":"ocpp:DownloadScheduled"},{"@id":"ocpp:Downloading"},{"@id":"ocpp:Downloaded"},{"@id":"ocpp:Published"},{"@id":"ocpp:DownloadFailed"},{"@id":"ocpp:DownloadPaused"},{"@id":"ocpp:InvalidChecksum"},{"@id":"ocpp:ChecksumVerified"},{"@id":"ocpp:PublishFailed"}]},{"@id":"ocpp:Idle","@type":["ocpp:PublishFirmwareStatusEnumType","schema:Enumeration"],"schema:name":"Idle","schema:identifier":"Idle"},{"@id":"ocpp:DownloadScheduled","@type":["ocpp:PublishFirmwareStatusEnumType","schema:Enumeration"],"schema:name":"DownloadScheduled","schema:identifier":"DownloadScheduled"},{"@id":"ocpp:Downloading","@type":["ocpp:PublishFirmwareStatusEnumType","schema:Enumeration"],"schema:name":"Downloading","schema:identifier":"Downloading"},{"@id":"ocpp:Downloaded","@type":["ocpp:PublishFirmwareStatusEnumType","schema:Enumeration"],"schema:name":"Downloaded","schema:identifier":"Downloaded"},{"@id":"ocpp:Published","@type":["ocpp:PublishFirmwareStatusEnumType","schema:Enumeration"],"schema:name":"Published","schema:identifier":"Published"},{"@id":"ocpp:DownloadFailed","@type":["ocpp:PublishFirmwareStatusEnumType","schema:Enumeration"],"schema:name":"DownloadFailed","schema:identifier":"DownloadFailed"},{"@id":"ocpp:DownloadPaused","@type":["ocpp:PublishFirmwareStatusEnumType","schema:Enumeration"],"schema:name":"DownloadPaused","schema:identifier":"DownloadPaused"},{"@id":"ocpp:InvalidChecksum","@type":["ocpp:PublishFirmwareStatusEnumType","schema:Enumeration"],"schema:name":"InvalidChecksum","schema:identifier":"InvalidChecksum"},{"@id":"ocpp:ChecksumVerified","@type":["ocpp:PublishFirmwareStatusEnumType","schema:Enumeration"],"schema:name":"ChecksumVerified","schema:identifier":"ChecksumVerified"},{"@id":"ocpp:PublishFailed","@type":["ocpp:PublishFirmwareStatusEnumType","schema:Enumeration"],"schema:name":"PublishFailed","schema:identifier":"PublishFailed"},{"@id":"ocpp:ChargingProfileStatusEnumType","@type":"schema:Enumeration","schema:name":"ChargingProfileStatusEnumType","rdfs:comment":"Returns whether message was processed successfully.\r\n","schema:hasEnumerationMember":[{"@id":"ocpp:Accepted"},{"@id":"ocpp:Rejected"}]},{"@id":"ocpp:Accepted","@type":["ocpp:ChargingProfileStatusEnumType","schema:Enumeration"],"schema:name":"Accepted","schema:identifier":"Accepted"},{"@id":"ocpp:Rejected","@type":["ocpp:ChargingProfileStatusEnumType","schema:Enumeration"],"schema:name":"Rejected","schema:identifier":"Rejected"},{"@id":"ocpp:ChargingScheduleUpdateType","@type":"rdfs:Class","rdfs:label":"ChargingScheduleUpdateType","rdfs:comment":"Updates to a ChargingSchedulePeriodType for dynamic charging profiles.\r\n\r\n"},{"@id":"ocpp:ChargingProfileKindEnumType","@type":"schema:Enumeration","schema:name":"ChargingProfileKindEnumType","rdfs:comment":"Indicates the kind of schedule.\r\n","schema:hasEnumerationMember":[{"@id":"ocpp:Absolute"},{"@id":"ocpp:Recurring"},{"@id":"ocpp:Relative"},{"@id":"ocpp:Dynamic"}]},{"@id":"ocpp:Absolute","@type":["ocpp:ChargingProfileKindEnumType","schema:Enumeration"],"schema:name":"Absolute","schema:identifier":"Absolute"},{"@id":"ocpp:Recurring","@type":["ocpp:ChargingProfileKindEnumType","schema:Enumeration"],"schema:name":"Recurring","schema:identifier":"Recurring"},{"@id":"ocpp:Relative","@type":["ocpp:ChargingProfileKindEnumType","schema:Enumeration"],"schema:name":"Relative","schema:identifier":"Relative"},{"@id":"ocpp:Dynamic","@type":["ocpp:ChargingProfileKindEnumType","schema:Enumeration"],"schema:name":"Dynamic","schema:identifier":"Dynamic"},{"@id":"ocpp:RecurrencyKindEnumType","@type":"schema:Enumeration","schema:name":"RecurrencyKindEnumType","rdfs:comment":"Indicates the start point of a recurrence.\r\n","schema:hasEnumerationMember":[{"@id":"ocpp:Daily"},{"@id":"ocpp:Weekly"}]},{"@id":"ocpp:Daily","@type":["ocpp:RecurrencyKindEnumType","schema:Enumeration"],"schema:name":"Daily","schema:identifier":"Daily"},{"@id":"ocpp:Weekly","@type":["ocpp:RecurrencyKindEnumType","schema:Enumeration"],"schema:name":"Weekly","schema:identifier":"Weekly"},{"@id":"ocpp:ChargingProfileType","@type":"rdfs:Class","rdfs:label":"ChargingProfileType","rdfs:comment":"A ChargingProfile consists of 1 to 3 ChargingSchedules with a list of ChargingSchedulePeriods, describing the amount of power or current that can be delivered per time interval.\r\n\r\nimage::images/ChargingProfile-Simple.png[]\r\n\r\n"},{"@id":"ocpp:DERUnitEnumType","@type":"schema:Enumeration","schema:name":"DERUnitEnumType","rdfs:comment":"Unit of the setpoint.\r\n","schema:hasEnumerationMember":[{"@id":"ocpp:Not_Applicable"},{"@id":"ocpp:PctMaxW"},{"@id":"ocpp:PctMaxVar"},{"@id":"ocpp:PctWAvail"},{"@id":"ocpp:PctVarAvail"},{"@id":"ocpp:PctEffectiveV"}]},{"@id":"ocpp:Not_Applicable","@type":["ocpp:DERUnitEnumType","schema:Enumeration"],"schema:name":"Not_Applicable","schema:identifier":"Not_Applicable"},{"@id":"ocpp:PctMaxW","@type":["ocpp:DERUnitEnumType","schema:Enumeration"],"schema:name":"PctMaxW","schema:identifier":"PctMaxW"},{"@id":"ocpp:PctMaxVar","@type":["ocpp:DERUnitEnumType","schema:Enumeration"],"schema:name":"PctMaxVar","schema:identifier":"PctMaxVar"},{"@id":"ocpp:PctWAvail","@type":["ocpp:DERUnitEnumType","schema:Enumeration"],"schema:name":"PctWAvail","schema:identifier":"PctWAvail"},{"@id":"ocpp:PctVarAvail","@type":["ocpp:DERUnitEnumType","schema:Enumeration"],"schema:name":"PctVarAvail","schema:identifier":"PctVarAvail"},{"@id":"ocpp:PctEffectiveV","@type":["ocpp:DERUnitEnumType","schema:Enumeration"],"schema:name":"PctEffectiveV","schema:identifier":"PctEffectiveV"},{"@id":"ocpp:PowerDuringCessationEnumType","@type":"schema:Enumeration","schema:name":"PowerDuringCessationEnumType","rdfs:comment":"Parameter is only sent, if the EV has to feed-in power or reactive power during fault-ride through (FRT) as defined by HVMomCess curve and LVMomCess curve.\r\n\r\n\r\n","schema:hasEnumerationMember":[{"@id":"ocpp:Active"},{"@id":"ocpp:Reactive"}]},{"@id":"ocpp:Active","@type":["ocpp:PowerDuringCessationEnumType","schema:Enumeration"],"schema:name":"Active","schema:identifier":"Active"},{"@id":"ocpp:Reactive","@type":["ocpp:PowerDuringCessationEnumType","schema:Enumeration"],"schema:name":"Reactive","schema:identifier":"Reactive"},{"@id":"ocpp:DERCurveGetType","@type":"rdfs:Class","rdfs:label":"DERCurveGetType"},{"@id":"ocpp:DERCurvePointsType","@type":"rdfs:Class","rdfs:label":"DERCurvePointsType"},{"@id":"ocpp:DERCurveType","@type":"rdfs:Class","rdfs:label":"DERCurveType"},{"@id":"ocpp:EnterServiceGetType","@type":"rdfs:Class","rdfs:label":"EnterServiceGetType"},{"@id":"ocpp:EnterServiceType","@type":"rdfs:Class","rdfs:label":"EnterServiceType"},{"@id":"ocpp:FixedPFGetType","@type":"rdfs:Class","rdfs:label":"FixedPFGetType"},{"@id":"ocpp:FixedPFType","@type":"rdfs:Class","rdfs:label":"FixedPFType"},{"@id":"ocpp:FixedVarGetType","@type":"rdfs:Class","rdfs:label":"FixedVarGetType"},{"@id":"ocpp:FixedVarType","@type":"rdfs:Class","rdfs:label":"FixedVarType"},{"@id":"ocpp:FreqDroopGetType","@type":"rdfs:Class","rdfs:label":"FreqDroopGetType"},{"@id":"ocpp:FreqDroopType","@type":"rdfs:Class","rdfs:label":"FreqDroopType"},{"@id":"ocpp:GradientGetType","@type":"rdfs:Class","rdfs:label":"GradientGetType"},{"@id":"ocpp:GradientType","@type":"rdfs:Class","rdfs:label":"GradientType"},{"@id":"ocpp:HysteresisType","@type":"rdfs:Class","rdfs:label":"HysteresisType"},{"@id":"ocpp:LimitMaxDischargeGetType","@type":"rdfs:Class","rdfs:label":"LimitMaxDischargeGetType"},{"@id":"ocpp:LimitMaxDischargeType","@type":"rdfs:Class","rdfs:label":"LimitMaxDischargeType"},{"@id":"ocpp:ReactivePowerParamsType","@type":"rdfs:Class","rdfs:label":"ReactivePowerParamsType"},{"@id":"ocpp:VoltageParamsType","@type":"rdfs:Class","rdfs:label":"VoltageParamsType"},{"@id":"ocpp:RequestStartStopStatusEnumType","@type":"schema:Enumeration","schema:name":"RequestStartStopStatusEnumType","rdfs:comment":"Status indicating whether Charging Station accepts the request to stop a transaction.\r\n","schema:hasEnumerationMember":[{"@id":"ocpp:Accepted"},{"@id":"ocpp:Rejected"}]},{"@id":"ocpp:Accepted","@type":["ocpp:RequestStartStopStatusEnumType","schema:Enumeration"],"schema:name":"Accepted","schema:identifier":"Accepted"},{"@id":"ocpp:Rejected","@type":["ocpp:RequestStartStopStatusEnumType","schema:Enumeration"],"schema:name":"Rejected","schema:identifier":"Rejected"},{"@id":"ocpp:ReservationUpdateStatusEnumType","@type":"schema:Enumeration","schema:name":"ReservationUpdateStatusEnumType","rdfs:comment":"The updated reservation status.\r\n","schema:hasEnumerationMember":[{"@id":"ocpp:Expired"},{"@id":"ocpp:Removed"},{"@id":"ocpp:NoTransaction"}]},{"@id":"ocpp:Expired","@type":["ocpp:ReservationUpdateStatusEnumType","schema:Enumeration"],"schema:name":"Expired","schema:identifier":"Expired"},{"@id":"ocpp:Removed","@type":["ocpp:ReservationUpdateStatusEnumType","schema:Enumeration"],"schema:name":"Removed","schema:identifier":"Removed"},{"@id":"ocpp:NoTransaction","@type":["ocpp:ReservationUpdateStatusEnumType","schema:Enumeration"],"schema:name":"NoTransaction","schema:identifier":"NoTransaction"},{"@id":"ocpp:ReserveNowStatusEnumType","@type":"schema:Enumeration","schema:name":"ReserveNowStatusEnumType","rdfs:comment":"This indicates the success or failure of the reservation.\r\n","schema:hasEnumerationMember":[{"@id":"ocpp:Accepted"},{"@id":"ocpp:Faulted"},{"@id":"ocpp:Occupied"},{"@id":"ocpp:Rejected"},{"@id":"ocpp:Unavailable"}]},{"@id":"ocpp:Accepted","@type":["ocpp:ReserveNowStatusEnumType","schema:Enumeration"],"schema:name":"Accepted","schema:identifier":"Accepted"},{"@id":"ocpp:Faulted","@type":["ocpp:ReserveNowStatusEnumType","schema:Enumeration"],"schema:name":"Faulted","schema:identifier":"Faulted"},{"@id":"ocpp:Occupied","@type":["ocpp:ReserveNowStatusEnumType","schema:Enumeration"],"schema:name":"Occupied","schema:identifier":"Occupied"},{"@id":"ocpp:Rejected","@type":["ocpp:ReserveNowStatusEnumType","schema:Enumeration"],"schema:name":"Rejected","schema:identifier":"Rejected"},{"@id":"ocpp:Unavailable","@type":["ocpp:ReserveNowStatusEnumType","schema:Enumeration"],"schema:name":"Unavailable","schema:identifier":"Unavailable"},{"@id":"ocpp:ResetEnumType","@type":"schema:Enumeration","schema:name":"ResetEnumType","rdfs:comment":"This contains the type of reset that the Charging Station or EVSE should perform.\r\n","schema:hasEnumerationMember":[{"@id":"ocpp:Immediate"},{"@id":"ocpp:OnIdle"},{"@id":"ocpp:ImmediateAndResume"}]},{"@id":"ocpp:Immediate","@type":["ocpp:ResetEnumType","schema:Enumeration"],"schema:name":"Immediate","schema:identifier":"Immediate"},{"@id":"ocpp:OnIdle","@type":["ocpp:ResetEnumType","schema:Enumeration"],"schema:name":"OnIdle","schema:identifier":"OnIdle"},{"@id":"ocpp:ImmediateAndResume","@type":["ocpp:ResetEnumType","schema:Enumeration"],"schema:name":"ImmediateAndResume","schema:identifier":"ImmediateAndResume"},{"@id":"ocpp:ResetStatusEnumType","@type":"schema:Enumeration","schema:name":"ResetStatusEnumType","rdfs:comment":"This indicates whether the Charging Station is able to perform the reset.\r\n","schema:hasEnumerationMember":[{"@id":"ocpp:Accepted"},{"@id":"ocpp:Rejected"},{"@id":"ocpp:Scheduled"}]},{"@id":"ocpp:Accepted","@type":["ocpp:ResetStatusEnumType","schema:Enumeration"],"schema:name":"Accepted","schema:identifier":"Accepted"},{"@id":"ocpp:Rejected","@type":["ocpp:ResetStatusEnumType","schema:Enumeration"],"schema:name":"Rejected","schema:identifier":"Rejected"},{"@id":"ocpp:Scheduled","@type":["ocpp:ResetStatusEnumType","schema:Enumeration"],"schema:name":"Scheduled","schema:identifier":"Scheduled"},{"@id":"ocpp:UpdateEnumType","@type":"schema:Enumeration","schema:name":"UpdateEnumType","rdfs:comment":"This contains the type of update (full or differential) of this request.\r\n","schema:hasEnumerationMember":[{"@id":"ocpp:Differential"},{"@id":"ocpp:Full"}]},{"@id":"ocpp:Differential","@type":["ocpp:UpdateEnumType","schema:Enumeration"],"schema:name":"Differential","schema:identifier":"Differential"},{"@id":"ocpp:Full","@type":["ocpp:UpdateEnumType","schema:Enumeration"],"schema:name":"Full","schema:identifier":"Full"},{"@id":"ocpp:AuthorizationData","@type":"rdfs:Class","rdfs:label":"AuthorizationData","rdfs:comment":"Contains the identifier to use for authorization.\r\n"},{"@id":"ocpp:SendLocalListStatusEnumType","@type":"schema:Enumeration","schema:name":"SendLocalListStatusEnumType","rdfs:comment":"This indicates whether the Charging Station has successfully received and applied the update of the Local Authorization List.\r\n","schema:hasEnumerationMember":[{"@id":"ocpp:Accepted"},{"@id":"ocpp:Failed"},{"@id":"ocpp:VersionMismatch"}]},{"@id":"ocpp:Accepted","@type":["ocpp:SendLocalListStatusEnumType","schema:Enumeration"],"schema:name":"Accepted","schema:identifier":"Accepted"},{"@id":"ocpp:Failed","@type":["ocpp:SendLocalListStatusEnumType","schema:Enumeration"],"schema:name":"Failed","schema:identifier":"Failed"},{"@id":"ocpp:VersionMismatch","@type":["ocpp:SendLocalListStatusEnumType","schema:Enumeration"],"schema:name":"VersionMismatch","schema:identifier":"VersionMismatch"},{"@id":"ocpp:TariffSetStatusEnumType","@type":"schema:Enumeration","schema:name":"TariffSetStatusEnumType","schema:hasEnumerationMember":[{"@id":"ocpp:Accepted"},{"@id":"ocpp:Rejected"},{"@id":"ocpp:TooManyElements"},{"@id":"ocpp:ConditionNotSupported"},{"@id":"ocpp:DuplicateTariffId"}]},{"@id":"ocpp:Accepted","@type":["ocpp:TariffSetStatusEnumType","schema:Enumeration"],"schema:name":"Accepted","schema:identifier":"Accepted"},{"@id":"ocpp:Rejected","@type":["ocpp:TariffSetStatusEnumType","schema:Enumeration"],"schema:name":"Rejected","schema:identifier":"Rejected"},{"@id":"ocpp:TooManyElements","@type":["ocpp:TariffSetStatusEnumType","schema:Enumeration"],"schema:name":"TooManyElements","schema:identifier":"TooManyElements"},{"@id":"ocpp:ConditionNotSupported","@type":["ocpp:TariffSetStatusEnumType","schema:Enumeration"],"schema:name":"ConditionNotSupported","schema:identifier":"ConditionNotSupported"},{"@id":"ocpp:DuplicateTariffId","@type":["ocpp:TariffSetStatusEnumType","schema:Enumeration"],"schema:name":"DuplicateTariffId","schema:identifier":"DuplicateTariffId"},{"@id":"ocpp:DisplayMessageStatusEnumType","@type":"schema:Enumeration","schema:name":"DisplayMessageStatusEnumType","rdfs:comment":"This indicates whether the Charging Station is able to display the message.\r\n","schema:hasEnumerationMember":[{"@id":"ocpp:Accepted"},{"@id":"ocpp:NotSupportedMessageFormat"},{"@id":"ocpp:Rejected"},{"@id":"ocpp:NotSupportedPriority"},{"@id":"ocpp:NotSupportedState"},{"@id":"ocpp:UnknownTransaction"},{"@id":"ocpp:LanguageNotSupported"}]},{"@id":"ocpp:Accepted","@type":["ocpp:DisplayMessageStatusEnumType","schema:Enumeration"],"schema:name":"Accepted","schema:identifier":"Accepted"},{"@id":"ocpp:NotSupportedMessageFormat","@type":["ocpp:DisplayMessageStatusEnumType","schema:Enumeration"],"schema:name":"NotSupportedMessageFormat","schema:identifier":"NotSupportedMessageFormat"},{"@id":"ocpp:Rejected","@type":["ocpp:DisplayMessageStatusEnumType","schema:Enumeration"],"schema:name":"Rejected","schema:identifier":"Rejected"},{"@id":"ocpp:NotSupportedPriority","@type":["ocpp:DisplayMessageStatusEnumType","schema:Enumeration"],"schema:name":"NotSupportedPriority","schema:identifier":"NotSupportedPriority"},{"@id":"ocpp:NotSupportedState","@type":["ocpp:DisplayMessageStatusEnumType","schema:Enumeration"],"schema:name":"NotSupportedState","schema:identifier":"NotSupportedState"},{"@id":"ocpp:UnknownTransaction","@type":["ocpp:DisplayMessageStatusEnumType","schema:Enumeration"],"schema:name":"UnknownTransaction","schema:identifier":"UnknownTransaction"},{"@id":"ocpp:LanguageNotSupported","@type":["ocpp:DisplayMessageStatusEnumType","schema:Enumeration"],"schema:name":"LanguageNotSupported","schema:identifier":"LanguageNotSupported"},{"@id":"ocpp:MonitoringBaseEnumType","@type":"schema:Enumeration","schema:name":"MonitoringBaseEnumType","rdfs:comment":"Specify which monitoring base will be set\r\n","schema:hasEnumerationMember":[{"@id":"ocpp:All"},{"@id":"ocpp:FactoryDefault"},{"@id":"ocpp:HardWiredOnly"}]},{"@id":"ocpp:All","@type":["ocpp:MonitoringBaseEnumType","schema:Enumeration"],"schema:name":"All","schema:identifier":"All"},{"@id":"ocpp:FactoryDefault","@type":["ocpp:MonitoringBaseEnumType","schema:Enumeration"],"schema:name":"FactoryDefault","schema:identifier":"FactoryDefault"},{"@id":"ocpp:HardWiredOnly","@type":["ocpp:MonitoringBaseEnumType","schema:Enumeration"],"schema:name":"HardWiredOnly","schema:identifier":"HardWiredOnly"},{"@id":"ocpp:APNAuthenticationEnumType","@type":"schema:Enumeration","schema:name":"APNAuthenticationEnumType","rdfs:comment":"Authentication method.\r\n","schema:hasEnumerationMember":[{"@id":"ocpp:PAP"},{"@id":"ocpp:CHAP"},{"@id":"ocpp:NONE"},{"@id":"ocpp:AUTO"}]},{"@id":"ocpp:PAP","@type":["ocpp:APNAuthenticationEnumType","schema:Enumeration"],"schema:name":"PAP","schema:identifier":"PAP"},{"@id":"ocpp:CHAP","@type":["ocpp:APNAuthenticationEnumType","schema:Enumeration"],"schema:name":"CHAP","schema:identifier":"CHAP"},{"@id":"ocpp:NONE","@type":["ocpp:APNAuthenticationEnumType","schema:Enumeration"],"schema:name":"NONE","schema:identifier":"NONE"},{"@id":"ocpp:AUTO","@type":["ocpp:APNAuthenticationEnumType","schema:Enumeration"],"schema:name":"AUTO","schema:identifier":"AUTO"},{"@id":"ocpp:OCPPInterfaceEnumType","@type":"schema:Enumeration","schema:name":"OCPPInterfaceEnumType","rdfs:comment":"Applicable Network Interface. Charging Station is allowed to use a different network interface to connect if the given one does not work.\r\n","schema:hasEnumerationMember":[{"@id":"ocpp:Wired0"},{"@id":"ocpp:Wired1"},{"@id":"ocpp:Wired2"},{"@id":"ocpp:Wired3"},{"@id":"ocpp:Wireless0"},{"@id":"ocpp:Wireless1"},{"@id":"ocpp:Wireless2"},{"@id":"ocpp:Wireless3"},{"@id":"ocpp:Any"}]},{"@id":"ocpp:Wired0","@type":["ocpp:OCPPInterfaceEnumType","schema:Enumeration"],"schema:name":"Wired0","schema:identifier":"Wired0"},{"@id":"ocpp:Wired1","@type":["ocpp:OCPPInterfaceEnumType","schema:Enumeration"],"schema:name":"Wired1","schema:identifier":"Wired1"},{"@id":"ocpp:Wired2","@type":["ocpp:OCPPInterfaceEnumType","schema:Enumeration"],"schema:name":"Wired2","schema:identifier":"Wired2"},{"@id":"ocpp:Wired3","@type":["ocpp:OCPPInterfaceEnumType","schema:Enumeration"],"schema:name":"Wired3","schema:identifier":"Wired3"},{"@id":"ocpp:Wireless0","@type":["ocpp:OCPPInterfaceEnumType","schema:Enumeration"],"schema:name":"Wireless0","schema:identifier":"Wireless0"},{"@id":"ocpp:Wireless1","@type":["ocpp:OCPPInterfaceEnumType","schema:Enumeration"],"schema:name":"Wireless1","schema:identifier":"Wireless1"},{"@id":"ocpp:Wireless2","@type":["ocpp:OCPPInterfaceEnumType","schema:Enumeration"],"schema:name":"Wireless2","schema:identifier":"Wireless2"},{"@id":"ocpp:Wireless3","@type":["ocpp:OCPPInterfaceEnumType","schema:Enumeration"],"schema:name":"Wireless3","schema:identifier":"Wireless3"},{"@id":"ocpp:Any","@type":["ocpp:OCPPInterfaceEnumType","schema:Enumeration"],"schema:name":"Any","schema:identifier":"Any"},{"@id":"ocpp:OCPPTransportEnumType","@type":"schema:Enumeration","schema:name":"OCPPTransportEnumType","rdfs:comment":"Defines the transport protocol (e.g. SOAP or JSON). Note: SOAP is not supported in OCPP 2.x, but is supported by earlier versions of OCPP.\r\n","schema:hasEnumerationMember":[{"@id":"ocpp:SOAP"},{"@id":"ocpp:JSON"}]},{"@id":"ocpp:SOAP","@type":["ocpp:OCPPTransportEnumType","schema:Enumeration"],"schema:name":"SOAP","schema:identifier":"SOAP"},{"@id":"ocpp:JSON","@type":["ocpp:OCPPTransportEnumType","schema:Enumeration"],"schema:name":"JSON","schema:identifier":"JSON"},{"@id":"ocpp:OCPPVersionEnumType","@type":"schema:Enumeration","schema:name":"OCPPVersionEnumType","rdfs:comment":"*(2.1)* This field is ignored, since the OCPP version to use is determined during the websocket handshake. The field is only kept for backwards compatibility with the OCPP 2.0.1 JSON schema.\r\n","schema:hasEnumerationMember":[{"@id":"ocpp:OCPP12"},{"@id":"ocpp:OCPP15"},{"@id":"ocpp:OCPP16"},{"@id":"ocpp:OCPP20"},{"@id":"ocpp:OCPP201"},{"@id":"ocpp:OCPP21"}]},{"@id":"ocpp:OCPP12","@type":["ocpp:OCPPVersionEnumType","schema:Enumeration"],"schema:name":"OCPP12","schema:identifier":"OCPP12"},{"@id":"ocpp:OCPP15","@type":["ocpp:OCPPVersionEnumType","schema:Enumeration"],"schema:name":"OCPP15","schema:identifier":"OCPP15"},{"@id":"ocpp:OCPP16","@type":["ocpp:OCPPVersionEnumType","schema:Enumeration"],"schema:name":"OCPP16","schema:identifier":"OCPP16"},{"@id":"ocpp:OCPP20","@type":["ocpp:OCPPVersionEnumType","schema:Enumeration"],"schema:name":"OCPP20","schema:identifier":"OCPP20"},{"@id":"ocpp:OCPP201","@type":["ocpp:OCPPVersionEnumType","schema:Enumeration"],"schema:name":"OCPP201","schema:identifier":"OCPP201"},{"@id":"ocpp:OCPP21","@type":["ocpp:OCPPVersionEnumType","schema:Enumeration"],"schema:name":"OCPP21","schema:identifier":"OCPP21"},{"@id":"ocpp:VPNEnumType","@type":"schema:Enumeration","schema:name":"VPNEnumType","rdfs:comment":"Type of VPN\r\n","schema:hasEnumerationMember":[{"@id":"ocpp:IKEv2"},{"@id":"ocpp:IPSec"},{"@id":"ocpp:L2TP"},{"@id":"ocpp:PPTP"}]},{"@id":"ocpp:IKEv2","@type":["ocpp:VPNEnumType","schema:Enumeration"],"schema:name":"IKEv2","schema:identifier":"IKEv2"},{"@id":"ocpp:IPSec","@type":["ocpp:VPNEnumType","schema:Enumeration"],"schema:name":"IPSec","schema:identifier":"IPSec"},{"@id":"ocpp:L2TP","@type":["ocpp:VPNEnumType","schema:Enumeration"],"schema:name":"L2TP","schema:identifier":"L2TP"},{"@id":"ocpp:PPTP","@type":["ocpp:VPNEnumType","schema:Enumeration"],"schema:name":"PPTP","schema:identifier":"PPTP"},{"@id":"ocpp:APNType","@type":"rdfs:Class","rdfs:label":"APNType","rdfs:comment":"Collection of configuration data needed to make a data-connection over a cellular network.\r\n\r\nNOTE: When asking a GSM modem to dial in, it is possible to specify which mobile operator should be used. This can be done with the mobile country code (MCC) in combination with a mobile network code (MNC). Example: If your preferred network is Vodafone Netherlands, the MCC=204 and the MNC=04 which means the key PreferredNetwork = 20404 Some modems allows to specify a preferred network, which means, if this network is not available, a different network is used. If you specify UseOnlyPreferredNetwork and this network is not available, the modem will not dial in.\r\n"},{"@id":"ocpp:NetworkConnectionProfileType","@type":"rdfs:Class","rdfs:label":"NetworkConnectionProfileType","rdfs:comment":"The NetworkConnectionProfile defines the functional and technical parameters of a communication link.\r\n"},{"@id":"ocpp:VPNType","@type":"rdfs:Class","rdfs:label":"VPNType","rdfs:comment":"VPN Configuration settings\r\n"},{"@id":"ocpp:SetNetworkProfileStatusEnumType","@type":"schema:Enumeration","schema:name":"SetNetworkProfileStatusEnumType","rdfs:comment":"Result of operation.\r\n","schema:hasEnumerationMember":[{"@id":"ocpp:Accepted"},{"@id":"ocpp:Rejected"},{"@id":"ocpp:Failed"}]},{"@id":"ocpp:Accepted","@type":["ocpp:SetNetworkProfileStatusEnumType","schema:Enumeration"],"schema:name":"Accepted","schema:identifier":"Accepted"},{"@id":"ocpp:Rejected","@type":["ocpp:SetNetworkProfileStatusEnumType","schema:Enumeration"],"schema:name":"Rejected","schema:identifier":"Rejected"},{"@id":"ocpp:Failed","@type":["ocpp:SetNetworkProfileStatusEnumType","schema:Enumeration"],"schema:name":"Failed","schema:identifier":"Failed"},{"@id":"ocpp:SetMonitoringDataType","@type":"rdfs:Class","rdfs:label":"SetMonitoringDataType","rdfs:comment":"Class to hold parameters of SetVariableMonitoring request.\r\n"},{"@id":"ocpp:SetMonitoringStatusEnumType","@type":"schema:Enumeration","schema:name":"SetMonitoringStatusEnumType","rdfs:comment":"Status is OK if a value could be returned. Otherwise this will indicate the reason why a value could not be returned.\r\n","schema:hasEnumerationMember":[{"@id":"ocpp:Accepted"},{"@id":"ocpp:UnknownComponent"},{"@id":"ocpp:UnknownVariable"},{"@id":"ocpp:UnsupportedMonitorType"},{"@id":"ocpp:Rejected"},{"@id":"ocpp:Duplicate"}]},{"@id":"ocpp:Accepted","@type":["ocpp:SetMonitoringStatusEnumType","schema:Enumeration"],"schema:name":"Accepted","schema:identifier":"Accepted"},{"@id":"ocpp:UnknownComponent","@type":["ocpp:SetMonitoringStatusEnumType","schema:Enumeration"],"schema:name":"UnknownComponent","schema:identifier":"UnknownComponent"},{"@id":"ocpp:UnknownVariable","@type":["ocpp:SetMonitoringStatusEnumType","schema:Enumeration"],"schema:name":"UnknownVariable","schema:identifier":"UnknownVariable"},{"@id":"ocpp:UnsupportedMonitorType","@type":["ocpp:SetMonitoringStatusEnumType","schema:Enumeration"],"schema:name":"UnsupportedMonitorType","schema:identifier":"UnsupportedMonitorType"},{"@id":"ocpp:Rejected","@type":["ocpp:SetMonitoringStatusEnumType","schema:Enumeration"],"schema:name":"Rejected","schema:identifier":"Rejected"},{"@id":"ocpp:Duplicate","@type":["ocpp:SetMonitoringStatusEnumType","schema:Enumeration"],"schema:name":"Duplicate","schema:identifier":"Duplicate"},{"@id":"ocpp:SetMonitoringResultType","@type":"rdfs:Class","rdfs:label":"SetMonitoringResultType","rdfs:comment":"Class to hold result of SetVariableMonitoring request.\r\n"},{"@id":"ocpp:SetVariableDataType","@type":"rdfs:Class","rdfs:label":"SetVariableDataType"},{"@id":"ocpp:SetVariableStatusEnumType","@type":"schema:Enumeration","schema:name":"SetVariableStatusEnumType","rdfs:comment":"Result status of setting the variable.\r\n","schema:hasEnumerationMember":[{"@id":"ocpp:Accepted"},{"@id":"ocpp:Rejected"},{"@id":"ocpp:UnknownComponent"},{"@id":"ocpp:UnknownVariable"},{"@id":"ocpp:NotSupportedAttributeType"},{"@id":"ocpp:RebootRequired"}]},{"@id":"ocpp:Accepted","@type":["ocpp:SetVariableStatusEnumType","schema:Enumeration"],"schema:name":"Accepted","schema:identifier":"Accepted"},{"@id":"ocpp:Rejected","@type":["ocpp:SetVariableStatusEnumType","schema:Enumeration"],"schema:name":"Rejected","schema:identifier":"Rejected"},{"@id":"ocpp:UnknownComponent","@type":["ocpp:SetVariableStatusEnumType","schema:Enumeration"],"schema:name":"UnknownComponent","schema:identifier":"UnknownComponent"},{"@id":"ocpp:UnknownVariable","@type":["ocpp:SetVariableStatusEnumType","schema:Enumeration"],"schema:name":"UnknownVariable","schema:identifier":"UnknownVariable"},{"@id":"ocpp:NotSupportedAttributeType","@type":["ocpp:SetVariableStatusEnumType","schema:Enumeration"],"schema:name":"NotSupportedAttributeType","schema:identifier":"NotSupportedAttributeType"},{"@id":"ocpp:RebootRequired","@type":["ocpp:SetVariableStatusEnumType","schema:Enumeration"],"schema:name":"RebootRequired","schema:identifier":"RebootRequired"},{"@id":"ocpp:SetVariableResultType","@type":"rdfs:Class","rdfs:label":"SetVariableResultType"},{"@id":"ocpp:ConnectorStatusEnumType","@type":"schema:Enumeration","schema:name":"ConnectorStatusEnumType","rdfs:comment":"This contains the current status of the Connector.\r\n","schema:hasEnumerationMember":[{"@id":"ocpp:Available"},{"@id":"ocpp:Occupied"},{"@id":"ocpp:Reserved"},{"@id":"ocpp:Unavailable"},{"@id":"ocpp:Faulted"}]},{"@id":"ocpp:Available","@type":["ocpp:ConnectorStatusEnumType","schema:Enumeration"],"schema:name":"Available","schema:identifier":"Available"},{"@id":"ocpp:Occupied","@type":["ocpp:ConnectorStatusEnumType","schema:Enumeration"],"schema:name":"Occupied","schema:identifier":"Occupied"},{"@id":"ocpp:Reserved","@type":["ocpp:ConnectorStatusEnumType","schema:Enumeration"],"schema:name":"Reserved","schema:identifier":"Reserved"},{"@id":"ocpp:Unavailable","@type":["ocpp:ConnectorStatusEnumType","schema:Enumeration"],"schema:name":"Unavailable","schema:identifier":"Unavailable"},{"@id":"ocpp:Faulted","@type":["ocpp:ConnectorStatusEnumType","schema:Enumeration"],"schema:name":"Faulted","schema:identifier":"Faulted"},{"@id":"ocpp:ChargingStateEnumType","@type":"schema:Enumeration","schema:name":"ChargingStateEnumType","rdfs:comment":"Current charging state, is required when state\r\nhas changed. Omitted when there is no communication between EVSE and EV, because no cable is plugged in.\r\n","schema:hasEnumerationMember":[{"@id":"ocpp:EVConnected"},{"@id":"ocpp:Charging"},{"@id":"ocpp:SuspendedEV"},{"@id":"ocpp:SuspendedEVSE"},{"@id":"ocpp:Idle"}]},{"@id":"ocpp:EVConnected","@type":["ocpp:ChargingStateEnumType","schema:Enumeration"],"schema:name":"EVConnected","schema:identifier":"EVConnected"},{"@id":"ocpp:Charging","@type":["ocpp:ChargingStateEnumType","schema:Enumeration"],"schema:name":"Charging","schema:identifier":"Charging"},{"@id":"ocpp:SuspendedEV","@type":["ocpp:ChargingStateEnumType","schema:Enumeration"],"schema:name":"SuspendedEV","schema:identifier":"SuspendedEV"},{"@id":"ocpp:SuspendedEVSE","@type":["ocpp:ChargingStateEnumType","schema:Enumeration"],"schema:name":"SuspendedEVSE","schema:identifier":"SuspendedEVSE"},{"@id":"ocpp:Idle","@type":["ocpp:ChargingStateEnumType","schema:Enumeration"],"schema:name":"Idle","schema:identifier":"Idle"},{"@id":"ocpp:CostDimensionEnumType","@type":"schema:Enumeration","schema:name":"CostDimensionEnumType","rdfs:comment":"Type of cost dimension: energy, power, time, etc.\r\n\r\n","schema:hasEnumerationMember":[{"@id":"ocpp:Energy"},{"@id":"ocpp:MaxCurrent"},{"@id":"ocpp:MinCurrent"},{"@id":"ocpp:MaxPower"},{"@id":"ocpp:MinPower"},{"@id":"ocpp:IdleTIme"},{"@id":"ocpp:ChargingTime"}]},{"@id":"ocpp:Energy","@type":["ocpp:CostDimensionEnumType","schema:Enumeration"],"schema:name":"Energy","schema:identifier":"Energy"},{"@id":"ocpp:MaxCurrent","@type":["ocpp:CostDimensionEnumType","schema:Enumeration"],"schema:name":"MaxCurrent","schema:identifier":"MaxCurrent"},{"@id":"ocpp:MinCurrent","@type":["ocpp:CostDimensionEnumType","schema:Enumeration"],"schema:name":"MinCurrent","schema:identifier":"MinCurrent"},{"@id":"ocpp:MaxPower","@type":["ocpp:CostDimensionEnumType","schema:Enumeration"],"schema:name":"MaxPower","schema:identifier":"MaxPower"},{"@id":"ocpp:MinPower","@type":["ocpp:CostDimensionEnumType","schema:Enumeration"],"schema:name":"MinPower","schema:identifier":"MinPower"},{"@id":"ocpp:IdleTIme","@type":["ocpp:CostDimensionEnumType","schema:Enumeration"],"schema:name":"IdleTIme","schema:identifier":"IdleTIme"},{"@id":"ocpp:ChargingTime","@type":["ocpp:CostDimensionEnumType","schema:Enumeration"],"schema:name":"ChargingTime","schema:identifier":"ChargingTime"},{"@id":"ocpp:PreconditioningStatusEnumType","@type":"schema:Enumeration","schema:name":"PreconditioningStatusEnumType","rdfs:comment":"*(2.1)* The current preconditioning status of the BMS in the EV. Default value is Unknown.\r\n","schema:hasEnumerationMember":[{"@id":"ocpp:Unknown"},{"@id":"ocpp:Ready"},{"@id":"ocpp:NotReady"},{"@id":"ocpp:Preconditioning"}]},{"@id":"ocpp:Unknown","@type":["ocpp:PreconditioningStatusEnumType","schema:Enumeration"],"schema:name":"Unknown","schema:identifier":"Unknown"},{"@id":"ocpp:Ready","@type":["ocpp:PreconditioningStatusEnumType","schema:Enumeration"],"schema:name":"Ready","schema:identifier":"Ready"},{"@id":"ocpp:NotReady","@type":["ocpp:PreconditioningStatusEnumType","schema:Enumeration"],"schema:name":"NotReady","schema:identifier":"NotReady"},{"@id":"ocpp:Preconditioning","@type":["ocpp:PreconditioningStatusEnumType","schema:Enumeration"],"schema:name":"Preconditioning","schema:identifier":"Preconditioning"},{"@id":"ocpp:ReasonEnumType","@type":"schema:Enumeration","schema:name":"ReasonEnumType","rdfs:comment":"The _stoppedReason_ is the reason/event that initiated the process of stopping the transaction. It will normally be the user stopping authorization via card (Local or MasterPass) or app (Remote), but it can also be CSMS revoking authorization (DeAuthorized), or disconnecting the EV when TxStopPoint = EVConnected (EVDisconnected). Most other reasons are related to technical faults or energy limitations. +\r\nMAY only be omitted when _stoppedReason_ is \"Local\"\r\n\r\n\r\n","schema:hasEnumerationMember":[{"@id":"ocpp:DeAuthorized"},{"@id":"ocpp:EmergencyStop"},{"@id":"ocpp:EnergyLimitReached"},{"@id":"ocpp:EVDisconnected"},{"@id":"ocpp:GroundFault"},{"@id":"ocpp:ImmediateReset"},{"@id":"ocpp:MasterPass"},{"@id":"ocpp:Local"},{"@id":"ocpp:LocalOutOfCredit"},{"@id":"ocpp:Other"},{"@id":"ocpp:OvercurrentFault"},{"@id":"ocpp:PowerLoss"},{"@id":"ocpp:PowerQuality"},{"@id":"ocpp:Reboot"},{"@id":"ocpp:Remote"},{"@id":"ocpp:SOCLimitReached"},{"@id":"ocpp:StoppedByEV"},{"@id":"ocpp:TimeLimitReached"},{"@id":"ocpp:Timeout"},{"@id":"ocpp:ReqEnergyTransferRejected"}]},{"@id":"ocpp:DeAuthorized","@type":["ocpp:ReasonEnumType","schema:Enumeration"],"schema:name":"DeAuthorized","schema:identifier":"DeAuthorized"},{"@id":"ocpp:EmergencyStop","@type":["ocpp:ReasonEnumType","schema:Enumeration"],"schema:name":"EmergencyStop","schema:identifier":"EmergencyStop"},{"@id":"ocpp:EnergyLimitReached","@type":["ocpp:ReasonEnumType","schema:Enumeration"],"schema:name":"EnergyLimitReached","schema:identifier":"EnergyLimitReached"},{"@id":"ocpp:EVDisconnected","@type":["ocpp:ReasonEnumType","schema:Enumeration"],"schema:name":"EVDisconnected","schema:identifier":"EVDisconnected"},{"@id":"ocpp:GroundFault","@type":["ocpp:ReasonEnumType","schema:Enumeration"],"schema:name":"GroundFault","schema:identifier":"GroundFault"},{"@id":"ocpp:ImmediateReset","@type":["ocpp:ReasonEnumType","schema:Enumeration"],"schema:name":"ImmediateReset","schema:identifier":"ImmediateReset"},{"@id":"ocpp:MasterPass","@type":["ocpp:ReasonEnumType","schema:Enumeration"],"schema:name":"MasterPass","schema:identifier":"MasterPass"},{"@id":"ocpp:Local","@type":["ocpp:ReasonEnumType","schema:Enumeration"],"schema:name":"Local","schema:identifier":"Local"},{"@id":"ocpp:LocalOutOfCredit","@type":["ocpp:ReasonEnumType","schema:Enumeration"],"schema:name":"LocalOutOfCredit","schema:identifier":"LocalOutOfCredit"},{"@id":"ocpp:Other","@type":["ocpp:ReasonEnumType","schema:Enumeration"],"schema:name":"Other","schema:identifier":"Other"},{"@id":"ocpp:OvercurrentFault","@type":["ocpp:ReasonEnumType","schema:Enumeration"],"schema:name":"OvercurrentFault","schema:identifier":"OvercurrentFault"},{"@id":"ocpp:PowerLoss","@type":["ocpp:ReasonEnumType","schema:Enumeration"],"schema:name":"PowerLoss","schema:identifier":"PowerLoss"},{"@id":"ocpp:PowerQuality","@type":["ocpp:ReasonEnumType","schema:Enumeration"],"schema:name":"PowerQuality","schema:identifier":"PowerQuality"},{"@id":"ocpp:Reboot","@type":["ocpp:ReasonEnumType","schema:Enumeration"],"schema:name":"Reboot","schema:identifier":"Reboot"},{"@id":"ocpp:Remote","@type":["ocpp:ReasonEnumType","schema:Enumeration"],"schema:name":"Remote","schema:identifier":"Remote"},{"@id":"ocpp:SOCLimitReached","@type":["ocpp:ReasonEnumType","schema:Enumeration"],"schema:name":"SOCLimitReached","schema:identifier":"SOCLimitReached"},{"@id":"ocpp:StoppedByEV","@type":["ocpp:ReasonEnumType","schema:Enumeration"],"schema:name":"StoppedByEV","schema:identifier":"StoppedByEV"},{"@id":"ocpp:TimeLimitReached","@type":["ocpp:ReasonEnumType","schema:Enumeration"],"schema:name":"TimeLimitReached","schema:identifier":"TimeLimitReached"},{"@id":"ocpp:Timeout","@type":["ocpp:ReasonEnumType","schema:Enumeration"],"schema:name":"Timeout","schema:identifier":"Timeout"},{"@id":"ocpp:ReqEnergyTransferRejected","@type":["ocpp:ReasonEnumType","schema:Enumeration"],"schema:name":"ReqEnergyTransferRejected","schema:identifier":"ReqEnergyTransferRejected"},{"@id":"ocpp:TariffCostEnumType","@type":"schema:Enumeration","schema:name":"TariffCostEnumType","rdfs:comment":"Type of cost: normal or the minimum or maximum cost.\r\n","schema:hasEnumerationMember":[{"@id":"ocpp:NormalCost"},{"@id":"ocpp:MinCost"},{"@id":"ocpp:MaxCost"}]},{"@id":"ocpp:NormalCost","@type":["ocpp:TariffCostEnumType","schema:Enumeration"],"schema:name":"NormalCost","schema:identifier":"NormalCost"},{"@id":"ocpp:MinCost","@type":["ocpp:TariffCostEnumType","schema:Enumeration"],"schema:name":"MinCost","schema:identifier":"MinCost"},{"@id":"ocpp:MaxCost","@type":["ocpp:TariffCostEnumType","schema:Enumeration"],"schema:name":"MaxCost","schema:identifier":"MaxCost"},{"@id":"ocpp:TransactionEventEnumType","@type":"schema:Enumeration","schema:name":"TransactionEventEnumType","rdfs:comment":"This contains the type of this event.\r\nThe first TransactionEvent of a transaction SHALL contain: \"Started\" The last TransactionEvent of a transaction SHALL contain: \"Ended\" All others SHALL contain: \"Updated\"\r\n","schema:hasEnumerationMember":[{"@id":"ocpp:Ended"},{"@id":"ocpp:Started"},{"@id":"ocpp:Updated"}]},{"@id":"ocpp:Ended","@type":["ocpp:TransactionEventEnumType","schema:Enumeration"],"schema:name":"Ended","schema:identifier":"Ended"},{"@id":"ocpp:Started","@type":["ocpp:TransactionEventEnumType","schema:Enumeration"],"schema:name":"Started","schema:identifier":"Started"},{"@id":"ocpp:Updated","@type":["ocpp:TransactionEventEnumType","schema:Enumeration"],"schema:name":"Updated","schema:identifier":"Updated"},{"@id":"ocpp:TriggerReasonEnumType","@type":"schema:Enumeration","schema:name":"TriggerReasonEnumType","rdfs:comment":"Reason the Charging Station sends this message to the CSMS\r\n","schema:hasEnumerationMember":[{"@id":"ocpp:AbnormalCondition"},{"@id":"ocpp:Authorized"},{"@id":"ocpp:CablePluggedIn"},{"@id":"ocpp:ChargingRateChanged"},{"@id":"ocpp:ChargingStateChanged"},{"@id":"ocpp:CostLimitReached"},{"@id":"ocpp:Deauthorized"},{"@id":"ocpp:EnergyLimitReached"},{"@id":"ocpp:EVCommunicationLost"},{"@id":"ocpp:EVConnectTimeout"},{"@id":"ocpp:EVDeparted"},{"@id":"ocpp:EVDetected"},{"@id":"ocpp:LimitSet"},{"@id":"ocpp:MeterValueClock"},{"@id":"ocpp:MeterValuePeriodic"},{"@id":"ocpp:OperationModeChanged"},{"@id":"ocpp:RemoteStart"},{"@id":"ocpp:RemoteStop"},{"@id":"ocpp:ResetCommand"},{"@id":"ocpp:RunningCost"},{"@id":"ocpp:SignedDataReceived"},{"@id":"ocpp:SoCLimitReached"},{"@id":"ocpp:StopAuthorized"},{"@id":"ocpp:TariffChanged"},{"@id":"ocpp:TariffNotAccepted"},{"@id":"ocpp:TimeLimitReached"},{"@id":"ocpp:Trigger"},{"@id":"ocpp:TxResumed"},{"@id":"ocpp:UnlockCommand"}]},{"@id":"ocpp:AbnormalCondition","@type":["ocpp:TriggerReasonEnumType","schema:Enumeration"],"schema:name":"AbnormalCondition","schema:identifier":"AbnormalCondition"},{"@id":"ocpp:Authorized","@type":["ocpp:TriggerReasonEnumType","schema:Enumeration"],"schema:name":"Authorized","schema:identifier":"Authorized"},{"@id":"ocpp:CablePluggedIn","@type":["ocpp:TriggerReasonEnumType","schema:Enumeration"],"schema:name":"CablePluggedIn","schema:identifier":"CablePluggedIn"},{"@id":"ocpp:ChargingRateChanged","@type":["ocpp:TriggerReasonEnumType","schema:Enumeration"],"schema:name":"ChargingRateChanged","schema:identifier":"ChargingRateChanged"},{"@id":"ocpp:ChargingStateChanged","@type":["ocpp:TriggerReasonEnumType","schema:Enumeration"],"schema:name":"ChargingStateChanged","schema:identifier":"ChargingStateChanged"},{"@id":"ocpp:CostLimitReached","@type":["ocpp:TriggerReasonEnumType","schema:Enumeration"],"schema:name":"CostLimitReached","schema:identifier":"CostLimitReached"},{"@id":"ocpp:Deauthorized","@type":["ocpp:TriggerReasonEnumType","schema:Enumeration"],"schema:name":"Deauthorized","schema:identifier":"Deauthorized"},{"@id":"ocpp:EnergyLimitReached","@type":["ocpp:TriggerReasonEnumType","schema:Enumeration"],"schema:name":"EnergyLimitReached","schema:identifier":"EnergyLimitReached"},{"@id":"ocpp:EVCommunicationLost","@type":["ocpp:TriggerReasonEnumType","schema:Enumeration"],"schema:name":"EVCommunicationLost","schema:identifier":"EVCommunicationLost"},{"@id":"ocpp:EVConnectTimeout","@type":["ocpp:TriggerReasonEnumType","schema:Enumeration"],"schema:name":"EVConnectTimeout","schema:identifier":"EVConnectTimeout"},{"@id":"ocpp:EVDeparted","@type":["ocpp:TriggerReasonEnumType","schema:Enumeration"],"schema:name":"EVDeparted","schema:identifier":"EVDeparted"},{"@id":"ocpp:EVDetected","@type":["ocpp:TriggerReasonEnumType","schema:Enumeration"],"schema:name":"EVDetected","schema:identifier":"EVDetected"},{"@id":"ocpp:LimitSet","@type":["ocpp:TriggerReasonEnumType","schema:Enumeration"],"schema:name":"LimitSet","schema:identifier":"LimitSet"},{"@id":"ocpp:MeterValueClock","@type":["ocpp:TriggerReasonEnumType","schema:Enumeration"],"schema:name":"MeterValueClock","schema:identifier":"MeterValueClock"},{"@id":"ocpp:MeterValuePeriodic","@type":["ocpp:TriggerReasonEnumType","schema:Enumeration"],"schema:name":"MeterValuePeriodic","schema:identifier":"MeterValuePeriodic"},{"@id":"ocpp:OperationModeChanged","@type":["ocpp:TriggerReasonEnumType","schema:Enumeration"],"schema:name":"OperationModeChanged","schema:identifier":"OperationModeChanged"},{"@id":"ocpp:RemoteStart","@type":["ocpp:TriggerReasonEnumType","schema:Enumeration"],"schema:name":"RemoteStart","schema:identifier":"RemoteStart"},{"@id":"ocpp:RemoteStop","@type":["ocpp:TriggerReasonEnumType","schema:Enumeration"],"schema:name":"RemoteStop","schema:identifier":"RemoteStop"},{"@id":"ocpp:ResetCommand","@type":["ocpp:TriggerReasonEnumType","schema:Enumeration"],"schema:name":"ResetCommand","schema:identifier":"ResetCommand"},{"@id":"ocpp:RunningCost","@type":["ocpp:TriggerReasonEnumType","schema:Enumeration"],"schema:name":"RunningCost","schema:identifier":"RunningCost"},{"@id":"ocpp:SignedDataReceived","@type":["ocpp:TriggerReasonEnumType","schema:Enumeration"],"schema:name":"SignedDataReceived","schema:identifier":"SignedDataReceived"},{"@id":"ocpp:SoCLimitReached","@type":["ocpp:TriggerReasonEnumType","schema:Enumeration"],"schema:name":"SoCLimitReached","schema:identifier":"SoCLimitReached"},{"@id":"ocpp:StopAuthorized","@type":["ocpp:TriggerReasonEnumType","schema:Enumeration"],"schema:name":"StopAuthorized","schema:identifier":"StopAuthorized"},{"@id":"ocpp:TariffChanged","@type":["ocpp:TriggerReasonEnumType","schema:Enumeration"],"schema:name":"TariffChanged","schema:identifier":"TariffChanged"},{"@id":"ocpp:TariffNotAccepted","@type":["ocpp:TriggerReasonEnumType","schema:Enumeration"],"schema:name":"TariffNotAccepted","schema:identifier":"TariffNotAccepted"},{"@id":"ocpp:TimeLimitReached","@type":["ocpp:TriggerReasonEnumType","schema:Enumeration"],"schema:name":"TimeLimitReached","schema:identifier":"TimeLimitReached"},{"@id":"ocpp:Trigger","@type":["ocpp:TriggerReasonEnumType","schema:Enumeration"],"schema:name":"Trigger","schema:identifier":"Trigger"},{"@id":"ocpp:TxResumed","@type":["ocpp:TriggerReasonEnumType","schema:Enumeration"],"schema:name":"TxResumed","schema:identifier":"TxResumed"},{"@id":"ocpp:UnlockCommand","@type":["ocpp:TriggerReasonEnumType","schema:Enumeration"],"schema:name":"UnlockCommand","schema:identifier":"UnlockCommand"},{"@id":"ocpp:ChargingPeriodType","@type":"rdfs:Class","rdfs:label":"ChargingPeriodType","rdfs:comment":"A ChargingPeriodType consists of a start time, and a list of possible values that influence this period, for example: amount of energy charged this period, maximum current during this period etc.\r\n\r\n"},{"@id":"ocpp:CostDetailsType","@type":"rdfs:Class","rdfs:label":"CostDetailsType","rdfs:comment":"CostDetailsType contains the cost as calculated by Charging Station based on provided TariffType.\r\n\r\nNOTE: Reservation is not shown as a _chargingPeriod_, because it took place outside of the transaction.\r\n\r\n"},{"@id":"ocpp:CostDimensionType","@type":"rdfs:Class","rdfs:label":"CostDimensionType","rdfs:comment":"Volume consumed of cost dimension.\r\n"},{"@id":"ocpp:TotalCostType","@type":"rdfs:Class","rdfs:label":"TotalCostType","rdfs:comment":"This contains the cost calculated during a transaction. It is used both for running cost and final cost of the transaction.\r\n"},{"@id":"ocpp:TotalPriceType","@type":"rdfs:Class","rdfs:label":"TotalPriceType","rdfs:comment":"Total cost with and without tax. Contains the total of energy, charging time, idle time, fixed and reservation costs including and/or excluding tax.\r\n"},{"@id":"ocpp:TotalUsageType","@type":"rdfs:Class","rdfs:label":"TotalUsageType","rdfs:comment":"This contains the calculated usage of energy, charging time and idle time during a transaction.\r\n"},{"@id":"ocpp:TransactionLimitType","@type":"rdfs:Class","rdfs:label":"TransactionLimitType","rdfs:comment":"Cost, energy, time or SoC limit for a transaction.\r\n"},{"@id":"ocpp:TransactionType","@type":"rdfs:Class","rdfs:label":"TransactionType"},{"@id":"ocpp:MessageTriggerEnumType","@type":"schema:Enumeration","schema:name":"MessageTriggerEnumType","rdfs:comment":"Type of message to be triggered.\r\n","schema:hasEnumerationMember":[{"@id":"ocpp:BootNotification"},{"@id":"ocpp:LogStatusNotification"},{"@id":"ocpp:FirmwareStatusNotification"},{"@id":"ocpp:Heartbeat"},{"@id":"ocpp:MeterValues"},{"@id":"ocpp:SignChargingStationCertificate"},{"@id":"ocpp:SignV2GCertificate"},{"@id":"ocpp:SignV2G20Certificate"},{"@id":"ocpp:StatusNotification"},{"@id":"ocpp:TransactionEvent"},{"@id":"ocpp:SignCombinedCertificate"},{"@id":"ocpp:PublishFirmwareStatusNotification"},{"@id":"ocpp:CustomTrigger"}]},{"@id":"ocpp:BootNotification","@type":["ocpp:MessageTriggerEnumType","schema:Enumeration"],"schema:name":"BootNotification","schema:identifier":"BootNotification"},{"@id":"ocpp:LogStatusNotification","@type":["ocpp:MessageTriggerEnumType","schema:Enumeration"],"schema:name":"LogStatusNotification","schema:identifier":"LogStatusNotification"},{"@id":"ocpp:FirmwareStatusNotification","@type":["ocpp:MessageTriggerEnumType","schema:Enumeration"],"schema:name":"FirmwareStatusNotification","schema:identifier":"FirmwareStatusNotification"},{"@id":"ocpp:Heartbeat","@type":["ocpp:MessageTriggerEnumType","schema:Enumeration"],"schema:name":"Heartbeat","schema:identifier":"Heartbeat"},{"@id":"ocpp:MeterValues","@type":["ocpp:MessageTriggerEnumType","schema:Enumeration"],"schema:name":"MeterValues","schema:identifier":"MeterValues"},{"@id":"ocpp:SignChargingStationCertificate","@type":["ocpp:MessageTriggerEnumType","schema:Enumeration"],"schema:name":"SignChargingStationCertificate","schema:identifier":"SignChargingStationCertificate"},{"@id":"ocpp:SignV2GCertificate","@type":["ocpp:MessageTriggerEnumType","schema:Enumeration"],"schema:name":"SignV2GCertificate","schema:identifier":"SignV2GCertificate"},{"@id":"ocpp:SignV2G20Certificate","@type":["ocpp:MessageTriggerEnumType","schema:Enumeration"],"schema:name":"SignV2G20Certificate","schema:identifier":"SignV2G20Certificate"},{"@id":"ocpp:StatusNotification","@type":["ocpp:MessageTriggerEnumType","schema:Enumeration"],"schema:name":"StatusNotification","schema:identifier":"StatusNotification"},{"@id":"ocpp:TransactionEvent","@type":["ocpp:MessageTriggerEnumType","schema:Enumeration"],"schema:name":"TransactionEvent","schema:identifier":"TransactionEvent"},{"@id":"ocpp:SignCombinedCertificate","@type":["ocpp:MessageTriggerEnumType","schema:Enumeration"],"schema:name":"SignCombinedCertificate","schema:identifier":"SignCombinedCertificate"},{"@id":"ocpp:PublishFirmwareStatusNotification","@type":["ocpp:MessageTriggerEnumType","schema:Enumeration"],"schema:name":"PublishFirmwareStatusNotification","schema:identifier":"PublishFirmwareStatusNotification"},{"@id":"ocpp:CustomTrigger","@type":["ocpp:MessageTriggerEnumType","schema:Enumeration"],"schema:name":"CustomTrigger","schema:identifier":"CustomTrigger"},{"@id":"ocpp:TriggerMessageStatusEnumType","@type":"schema:Enumeration","schema:name":"TriggerMessageStatusEnumType","rdfs:comment":"Indicates whether the Charging Station will send the requested notification or not.\r\n","schema:hasEnumerationMember":[{"@id":"ocpp:Accepted"},{"@id":"ocpp:Rejected"},{"@id":"ocpp:NotImplemented"}]},{"@id":"ocpp:Accepted","@type":["ocpp:TriggerMessageStatusEnumType","schema:Enumeration"],"schema:name":"Accepted","schema:identifier":"Accepted"},{"@id":"ocpp:Rejected","@type":["ocpp:TriggerMessageStatusEnumType","schema:Enumeration"],"schema:name":"Rejected","schema:identifier":"Rejected"},{"@id":"ocpp:NotImplemented","@type":["ocpp:TriggerMessageStatusEnumType","schema:Enumeration"],"schema:name":"NotImplemented","schema:identifier":"NotImplemented"},{"@id":"ocpp:UnlockStatusEnumType","@type":"schema:Enumeration","schema:name":"UnlockStatusEnumType","rdfs:comment":"This indicates whether the Charging Station has unlocked the connector.\r\n","schema:hasEnumerationMember":[{"@id":"ocpp:Unlocked"},{"@id":"ocpp:UnlockFailed"},{"@id":"ocpp:OngoingAuthorizedTransaction"},{"@id":"ocpp:UnknownConnector"}]},{"@id":"ocpp:Unlocked","@type":["ocpp:UnlockStatusEnumType","schema:Enumeration"],"schema:name":"Unlocked","schema:identifier":"Unlocked"},{"@id":"ocpp:UnlockFailed","@type":["ocpp:UnlockStatusEnumType","schema:Enumeration"],"schema:name":"UnlockFailed","schema:identifier":"UnlockFailed"},{"@id":"ocpp:OngoingAuthorizedTransaction","@type":["ocpp:UnlockStatusEnumType","schema:Enumeration"],"schema:name":"OngoingAuthorizedTransaction","schema:identifier":"OngoingAuthorizedTransaction"},{"@id":"ocpp:UnknownConnector","@type":["ocpp:UnlockStatusEnumType","schema:Enumeration"],"schema:name":"UnknownConnector","schema:identifier":"UnknownConnector"},{"@id":"ocpp:UnpublishFirmwareStatusEnumType","@type":"schema:Enumeration","schema:name":"UnpublishFirmwareStatusEnumType","rdfs:comment":"Indicates whether the Local Controller succeeded in unpublishing the firmware.\r\n","schema:hasEnumerationMember":[{"@id":"ocpp:DownloadOngoing"},{"@id":"ocpp:NoFirmware"},{"@id":"ocpp:Unpublished"}]},{"@id":"ocpp:DownloadOngoing","@type":["ocpp:UnpublishFirmwareStatusEnumType","schema:Enumeration"],"schema:name":"DownloadOngoing","schema:identifier":"DownloadOngoing"},{"@id":"ocpp:NoFirmware","@type":["ocpp:UnpublishFirmwareStatusEnumType","schema:Enumeration"],"schema:name":"NoFirmware","schema:identifier":"NoFirmware"},{"@id":"ocpp:Unpublished","@type":["ocpp:UnpublishFirmwareStatusEnumType","schema:Enumeration"],"schema:name":"Unpublished","schema:identifier":"Unpublished"},{"@id":"ocpp:FirmwareType","@type":"rdfs:Class","rdfs:label":"FirmwareType","rdfs:comment":"Represents a copy of the firmware that can be loaded/updated on the Charging Station.\r\n"},{"@id":"ocpp:UpdateFirmwareStatusEnumType","@type":"schema:Enumeration","schema:name":"UpdateFirmwareStatusEnumType","rdfs:comment":"This field indicates whether the Charging Station was able to accept the request.\r\n\r\n","schema:hasEnumerationMember":[{"@id":"ocpp:Accepted"},{"@id":"ocpp:Rejected"},{"@id":"ocpp:AcceptedCanceled"},{"@id":"ocpp:InvalidCertificate"},{"@id":"ocpp:RevokedCertificate"}]},{"@id":"ocpp:Accepted","@type":["ocpp:UpdateFirmwareStatusEnumType","schema:Enumeration"],"schema:name":"Accepted","schema:identifier":"Accepted"},{"@id":"ocpp:Rejected","@type":["ocpp:UpdateFirmwareStatusEnumType","schema:Enumeration"],"schema:name":"Rejected","schema:identifier":"Rejected"},{"@id":"ocpp:AcceptedCanceled","@type":["ocpp:UpdateFirmwareStatusEnumType","schema:Enumeration"],"schema:name":"AcceptedCanceled","schema:identifier":"AcceptedCanceled"},{"@id":"ocpp:InvalidCertificate","@type":["ocpp:UpdateFirmwareStatusEnumType","schema:Enumeration"],"schema:name":"InvalidCertificate","schema:identifier":"InvalidCertificate"},{"@id":"ocpp:RevokedCertificate","@type":["ocpp:UpdateFirmwareStatusEnumType","schema:Enumeration"],"schema:name":"RevokedCertificate","schema:identifier":"RevokedCertificate"},{"@id":"ocpp:PriorityChargingStatusEnumType","@type":"schema:Enumeration","schema:name":"PriorityChargingStatusEnumType","rdfs:comment":"Result of the request.\r\n","schema:hasEnumerationMember":[{"@id":"ocpp:Accepted"},{"@id":"ocpp:Rejected"},{"@id":"ocpp:NoProfile"}]},{"@id":"ocpp:Accepted","@type":["ocpp:PriorityChargingStatusEnumType","schema:Enumeration"],"schema:name":"Accepted","schema:identifier":"Accepted"},{"@id":"ocpp:Rejected","@type":["ocpp:PriorityChargingStatusEnumType","schema:Enumeration"],"schema:name":"Rejected","schema:identifier":"Rejected"},{"@id":"ocpp:NoProfile","@type":["ocpp:PriorityChargingStatusEnumType","schema:Enumeration"],"schema:name":"NoProfile","schema:identifier":"NoProfile"},{"@id":"ocpp:PaymentBrandEnumType","@type":"schema:Enumeration","schema:name":"PaymentBrandEnumType","rdfs:comment":"Enumeration values from paymentbrand.csv","schema:hasEnumerationMember":[{"@id":"ocpp:AMEX"},{"@id":"ocpp:ApplePay"},{"@id":"ocpp:Bancontact"},{"@id":"ocpp:BankAxept"},{"@id":"ocpp:Carnet"},{"@id":"ocpp:CartesBancaires"},{"@id":"ocpp:Dankort"},{"@id":"ocpp:Diners"},{"@id":"ocpp:Discover"},{"@id":"ocpp:EftposAustralia"},{"@id":"ocpp:Elo"},{"@id":"ocpp:Girocard"},{"@id":"ocpp:GooglePay"},{"@id":"ocpp:Hipercard"},{"@id":"ocpp:Interac"},{"@id":"ocpp:JCB"},{"@id":"ocpp:Maestro"},{"@id":"ocpp:Mastercard"},{"@id":"ocpp:SamsungPay"},{"@id":"ocpp:UnionPay"},{"@id":"ocpp:VPay"},{"@id":"ocpp:Visa"}]},{"@id":"ocpp:AMEX","@type":["ocpp:PaymentBrandEnumType","schema:Enumeration"],"schema:name":"AMEX","schema:identifier":"AMEX"},{"@id":"ocpp:ApplePay","@type":["ocpp:PaymentBrandEnumType","schema:Enumeration"],"schema:name":"ApplePay","schema:identifier":"ApplePay"},{"@id":"ocpp:Bancontact","@type":["ocpp:PaymentBrandEnumType","schema:Enumeration"],"schema:name":"Bancontact","schema:identifier":"Bancontact"},{"@id":"ocpp:BankAxept","@type":["ocpp:PaymentBrandEnumType","schema:Enumeration"],"schema:name":"BankAxept","schema:identifier":"BankAxept"},{"@id":"ocpp:Carnet","@type":["ocpp:PaymentBrandEnumType","schema:Enumeration"],"schema:name":"Carnet","schema:identifier":"Carnet"},{"@id":"ocpp:CartesBancaires","@type":["ocpp:PaymentBrandEnumType","schema:Enumeration"],"schema:name":"CartesBancaires","schema:identifier":"CartesBancaires"},{"@id":"ocpp:Dankort","@type":["ocpp:PaymentBrandEnumType","schema:Enumeration"],"schema:name":"Dankort","schema:identifier":"Dankort"},{"@id":"ocpp:Diners","@type":["ocpp:PaymentBrandEnumType","schema:Enumeration"],"schema:name":"Diners","schema:identifier":"Diners"},{"@id":"ocpp:Discover","@type":["ocpp:PaymentBrandEnumType","schema:Enumeration"],"schema:name":"Discover","schema:identifier":"Discover"},{"@id":"ocpp:EftposAustralia","@type":["ocpp:PaymentBrandEnumType","schema:Enumeration"],"schema:name":"EftposAustralia","schema:identifier":"EftposAustralia"},{"@id":"ocpp:Elo","@type":["ocpp:PaymentBrandEnumType","schema:Enumeration"],"schema:name":"Elo","schema:identifier":"Elo"},{"@id":"ocpp:Girocard","@type":["ocpp:PaymentBrandEnumType","schema:Enumeration"],"schema:name":"Girocard","schema:identifier":"Girocard"},{"@id":"ocpp:GooglePay","@type":["ocpp:PaymentBrandEnumType","schema:Enumeration"],"schema:name":"GooglePay","schema:identifier":"GooglePay"},{"@id":"ocpp:Hipercard","@type":["ocpp:PaymentBrandEnumType","schema:Enumeration"],"schema:name":"Hipercard","schema:identifier":"Hipercard"},{"@id":"ocpp:Interac","@type":["ocpp:PaymentBrandEnumType","schema:Enumeration"],"schema:name":"Interac","schema:identifier":"Interac"},{"@id":"ocpp:JCB","@type":["ocpp:PaymentBrandEnumType","schema:Enumeration"],"schema:name":"JCB","schema:identifier":"JCB"},{"@id":"ocpp:Maestro","@type":["ocpp:PaymentBrandEnumType","schema:Enumeration"],"schema:name":"Maestro","schema:identifier":"Maestro"},{"@id":"ocpp:Mastercard","@type":["ocpp:PaymentBrandEnumType","schema:Enumeration"],"schema:name":"Mastercard","schema:identifier":"Mastercard"},{"@id":"ocpp:SamsungPay","@type":["ocpp:PaymentBrandEnumType","schema:Enumeration"],"schema:name":"SamsungPay","schema:identifier":"SamsungPay"},{"@id":"ocpp:UnionPay","@type":["ocpp:PaymentBrandEnumType","schema:Enumeration"],"schema:name":"UnionPay","schema:identifier":"UnionPay"},{"@id":"ocpp:VPay","@type":["ocpp:PaymentBrandEnumType","schema:Enumeration"],"schema:name":"VPay","schema:identifier":"VPay"},{"@id":"ocpp:Visa","@type":["ocpp:PaymentBrandEnumType","schema:Enumeration"],"schema:name":"Visa","schema:identifier":"Visa"},{"@id":"ocpp:UnitOfMeasureEnumType","@type":"schema:Enumeration","schema:name":"UnitOfMeasureEnumType","rdfs:comment":"Enumeration values from units_of_measure.csv","schema:hasEnumerationMember":[{"@id":"ocpp:A"},{"@id":"ocpp:ASU"},{"@id":"ocpp:B"},{"@id":"ocpp:Celsius"},{"@id":"ocpp:dB"},{"@id":"ocpp:dBm"},{"@id":"ocpp:Deg"},{"@id":"ocpp:Fahrenheit"},{"@id":"ocpp:Hz"},{"@id":"ocpp:mHz"},{"@id":"ocpp:K"},{"@id":"ocpp:lx"},{"@id":"ocpp:m"},{"@id":"ocpp:ms2"},{"@id":"ocpp:N"},{"@id":"ocpp:Ohm"},{"@id":"ocpp:kPa"},{"@id":"ocpp:Percent"},{"@id":"ocpp:RH"},{"@id":"ocpp:RPM"},{"@id":"ocpp:s"},{"@id":"ocpp:V"},{"@id":"ocpp:VA"},{"@id":"ocpp:kVA"},{"@id":"ocpp:VAh"},{"@id":"ocpp:kVAh"},{"@id":"ocpp:var"},{"@id":"ocpp:kvar"},{"@id":"ocpp:varh"},{"@id":"ocpp:kvarh"},{"@id":"ocpp:W"},{"@id":"ocpp:kW"},{"@id":"ocpp:Wh"},{"@id":"ocpp:kWh"}]},{"@id":"ocpp:A","@type":["ocpp:UnitOfMeasureEnumType","schema:Enumeration"],"schema:name":"A","schema:identifier":"A"},{"@id":"ocpp:ASU","@type":["ocpp:UnitOfMeasureEnumType","schema:Enumeration"],"schema:name":"ASU","schema:identifier":"ASU"},{"@id":"ocpp:B","@type":["ocpp:UnitOfMeasureEnumType","schema:Enumeration"],"schema:name":"B","schema:identifier":"B"},{"@id":"ocpp:Celsius","@type":["ocpp:UnitOfMeasureEnumType","schema:Enumeration"],"schema:name":"Celsius","schema:identifier":"Celsius"},{"@id":"ocpp:dB","@type":["ocpp:UnitOfMeasureEnumType","schema:Enumeration"],"schema:name":"dB","schema:identifier":"dB"},{"@id":"ocpp:dBm","@type":["ocpp:UnitOfMeasureEnumType","schema:Enumeration"],"schema:name":"dBm","schema:identifier":"dBm"},{"@id":"ocpp:Deg","@type":["ocpp:UnitOfMeasureEnumType","schema:Enumeration"],"schema:name":"Deg","schema:identifier":"Deg"},{"@id":"ocpp:Fahrenheit","@type":["ocpp:UnitOfMeasureEnumType","schema:Enumeration"],"schema:name":"Fahrenheit","schema:identifier":"Fahrenheit"},{"@id":"ocpp:Hz","@type":["ocpp:UnitOfMeasureEnumType","schema:Enumeration"],"schema:name":"Hz","schema:identifier":"Hz"},{"@id":"ocpp:mHz","@type":["ocpp:UnitOfMeasureEnumType","schema:Enumeration"],"schema:name":"mHz","schema:identifier":"mHz"},{"@id":"ocpp:K","@type":["ocpp:UnitOfMeasureEnumType","schema:Enumeration"],"schema:name":"K","schema:identifier":"K"},{"@id":"ocpp:lx","@type":["ocpp:UnitOfMeasureEnumType","schema:Enumeration"],"schema:name":"lx","schema:identifier":"lx"},{"@id":"ocpp:m","@type":["ocpp:UnitOfMeasureEnumType","schema:Enumeration"],"schema:name":"m","schema:identifier":"m"},{"@id":"ocpp:ms2","@type":["ocpp:UnitOfMeasureEnumType","schema:Enumeration"],"schema:name":"ms2","schema:identifier":"ms2"},{"@id":"ocpp:N","@type":["ocpp:UnitOfMeasureEnumType","schema:Enumeration"],"schema:name":"N","schema:identifier":"N"},{"@id":"ocpp:Ohm","@type":["ocpp:UnitOfMeasureEnumType","schema:Enumeration"],"schema:name":"Ohm","schema:identifier":"Ohm"},{"@id":"ocpp:kPa","@type":["ocpp:UnitOfMeasureEnumType","schema:Enumeration"],"schema:name":"kPa","schema:identifier":"kPa"},{"@id":"ocpp:Percent","@type":["ocpp:UnitOfMeasureEnumType","schema:Enumeration"],"schema:name":"Percent","schema:identifier":"Percent"},{"@id":"ocpp:RH","@type":["ocpp:UnitOfMeasureEnumType","schema:Enumeration"],"schema:name":"RH","schema:identifier":"RH"},{"@id":"ocpp:RPM","@type":["ocpp:UnitOfMeasureEnumType","schema:Enumeration"],"schema:name":"RPM","schema:identifier":"RPM"},{"@id":"ocpp:s","@type":["ocpp:UnitOfMeasureEnumType","schema:Enumeration"],"schema:name":"s","schema:identifier":"s"},{"@id":"ocpp:V","@type":["ocpp:UnitOfMeasureEnumType","schema:Enumeration"],"schema:name":"V","schema:identifier":"V"},{"@id":"ocpp:VA","@type":["ocpp:UnitOfMeasureEnumType","schema:Enumeration"],"schema:name":"VA","schema:identifier":"VA"},{"@id":"ocpp:kVA","@type":["ocpp:UnitOfMeasureEnumType","schema:Enumeration"],"schema:name":"kVA","schema:identifier":"kVA"},{"@id":"ocpp:VAh","@type":["ocpp:UnitOfMeasureEnumType","schema:Enumeration"],"schema:name":"VAh","schema:identifier":"VAh"},{"@id":"ocpp:kVAh","@type":["ocpp:UnitOfMeasureEnumType","schema:Enumeration"],"schema:name":"kVAh","schema:identifier":"kVAh"},{"@id":"ocpp:var","@type":["ocpp:UnitOfMeasureEnumType","schema:Enumeration"],"schema:name":"var","schema:identifier":"var"},{"@id":"ocpp:kvar","@type":["ocpp:UnitOfMeasureEnumType","schema:Enumeration"],"schema:name":"kvar","schema:identifier":"kvar"},{"@id":"ocpp:varh","@type":["ocpp:UnitOfMeasureEnumType","schema:Enumeration"],"schema:name":"varh","schema:identifier":"varh"},{"@id":"ocpp:kvarh","@type":["ocpp:UnitOfMeasureEnumType","schema:Enumeration"],"schema:name":"kvarh","schema:identifier":"kvarh"},{"@id":"ocpp:W","@type":["ocpp:UnitOfMeasureEnumType","schema:Enumeration"],"schema:name":"W","schema:identifier":"W"},{"@id":"ocpp:kW","@type":["ocpp:UnitOfMeasureEnumType","schema:Enumeration"],"schema:name":"kW","schema:identifier":"kW"},{"@id":"ocpp:Wh","@type":["ocpp:UnitOfMeasureEnumType","schema:Enumeration"],"schema:name":"Wh","schema:identifier":"Wh"},{"@id":"ocpp:kWh","@type":["ocpp:UnitOfMeasureEnumType","schema:Enumeration"],"schema:name":"kWh","schema:identifier":"kWh"},{"@id":"ocpp:SigningMethodEnumType","@type":"schema:Enumeration","schema:name":"SigningMethodEnumType","rdfs:comment":"Enumeration values from signingmethod.csv","schema:hasEnumerationMember":[{"@id":"ocpp:ECDSA-secp192k1-SHA256"},{"@id":"ocpp:ECDSA-secp256k1-SHA256"},{"@id":"ocpp:ECDSA-secp192r1-SHA256"},{"@id":"ocpp:ECDSA-secp256r1-SHA256"},{"@id":"ocpp:ECDSA-brainpool256r1-SHA256"},{"@id":"ocpp:ECDSA-secp384r1-SHA256"},{"@id":"ocpp:ECDSA-brainpool384r1-SHA256"}]},{"@id":"ocpp:ECDSA-secp192k1-SHA256","@type":["ocpp:SigningMethodEnumType","schema:Enumeration"],"schema:name":"ECDSA-secp192k1-SHA256","schema:identifier":"ECDSA-secp192k1-SHA256"},{"@id":"ocpp:ECDSA-secp256k1-SHA256","@type":["ocpp:SigningMethodEnumType","schema:Enumeration"],"schema:name":"ECDSA-secp256k1-SHA256","schema:identifier":"ECDSA-secp256k1-SHA256"},{"@id":"ocpp:ECDSA-secp192r1-SHA256","@type":["ocpp:SigningMethodEnumType","schema:Enumeration"],"schema:name":"ECDSA-secp192r1-SHA256","schema:identifier":"ECDSA-secp192r1-SHA256"},{"@id":"ocpp:ECDSA-secp256r1-SHA256","@type":["ocpp:SigningMethodEnumType","schema:Enumeration"],"schema:name":"ECDSA-secp256r1-SHA256","schema:identifier":"ECDSA-secp256r1-SHA256"},{"@id":"ocpp:ECDSA-brainpool256r1-SHA256","@type":["ocpp:SigningMethodEnumType","schema:Enumeration"],"schema:name":"ECDSA-brainpool256r1-SHA256","schema:identifier":"ECDSA-brainpool256r1-SHA256"},{"@id":"ocpp:ECDSA-secp384r1-SHA256","@type":["ocpp:SigningMethodEnumType","schema:Enumeration"],"schema:name":"ECDSA-secp384r1-SHA256","schema:identifier":"ECDSA-secp384r1-SHA256"},{"@id":"ocpp:ECDSA-brainpool384r1-SHA256","@type":["ocpp:SigningMethodEnumType","schema:Enumeration"],"schema:name":"ECDSA-brainpool384r1-SHA256","schema:identifier":"ECDSA-brainpool384r1-SHA256"},{"@id":"ocpp:PaymentRecognitionEnumType","@type":"schema:Enumeration","schema:name":"PaymentRecognitionEnumType","rdfs:comment":"Enumeration values from paymentrecognition.csv","schema:hasEnumerationMember":[{"@id":"ocpp:CC"},{"@id":"ocpp:Debit"},{"@id":"ocpp:Alipay"},{"@id":"ocpp:ApplePay"},{"@id":"ocpp:GooglePay"},{"@id":"ocpp:GrabPay"},{"@id":"ocpp:PayPal"},{"@id":"ocpp:SamsungPay"},{"@id":"ocpp:WeChatPay"}]},{"@id":"ocpp:CC","@type":["ocpp:PaymentRecognitionEnumType","schema:Enumeration"],"schema:name":"CC","schema:identifier":"CC"},{"@id":"ocpp:Debit","@type":["ocpp:PaymentRecognitionEnumType","schema:Enumeration"],"schema:name":"Debit","schema:identifier":"Debit"},{"@id":"ocpp:Alipay","@type":["ocpp:PaymentRecognitionEnumType","schema:Enumeration"],"schema:name":"Alipay","schema:identifier":"Alipay"},{"@id":"ocpp:ApplePay","@type":["ocpp:PaymentRecognitionEnumType","schema:Enumeration"],"schema:name":"ApplePay","schema:identifier":"ApplePay"},{"@id":"ocpp:GooglePay","@type":["ocpp:PaymentRecognitionEnumType","schema:Enumeration"],"schema:name":"GooglePay","schema:identifier":"GooglePay"},{"@id":"ocpp:GrabPay","@type":["ocpp:PaymentRecognitionEnumType","schema:Enumeration"],"schema:name":"GrabPay","schema:identifier":"GrabPay"},{"@id":"ocpp:PayPal","@type":["ocpp:PaymentRecognitionEnumType","schema:Enumeration"],"schema:name":"PayPal","schema:identifier":"PayPal"},{"@id":"ocpp:SamsungPay","@type":["ocpp:PaymentRecognitionEnumType","schema:Enumeration"],"schema:name":"SamsungPay","schema:identifier":"SamsungPay"},{"@id":"ocpp:WeChatPay","@type":["ocpp:PaymentRecognitionEnumType","schema:Enumeration"],"schema:name":"WeChatPay","schema:identifier":"WeChatPay"},{"@id":"ocpp:ConnectorEnumType","@type":"schema:Enumeration","schema:name":"ConnectorEnumType","rdfs:comment":"Enumeration values from connectorenumtype.csv","schema:hasEnumerationMember":[{"@id":"ocpp:cCCS1"},{"@id":"ocpp:cCCS2"},{"@id":"ocpp:cChaoJi"},{"@id":"ocpp:cG105"},{"@id":"ocpp:cGBT-DC"},{"@id":"ocpp:cLECCS"},{"@id":"ocpp:cMCS"},{"@id":"ocpp:cNACS"},{"@id":"ocpp:cNACS-CCS1"},{"@id":"ocpp:cCCS1-NACS"},{"@id":"ocpp:cTesla"},{"@id":"ocpp:cType1"},{"@id":"ocpp:cType2"},{"@id":"ocpp:cUltraChaoJi"},{"@id":"ocpp:s309-1P-16A"},{"@id":"ocpp:s309-1P-32A"},{"@id":"ocpp:s309-3P-16A"},{"@id":"ocpp:s309-3P-32A"},{"@id":"ocpp:sBS1361"},{"@id":"ocpp:sCEE-7-7"},{"@id":"ocpp:sType1"},{"@id":"ocpp:sType2"},{"@id":"ocpp:sType3"},{"@id":"ocpp:wInductive"},{"@id":"ocpp:wResonant"},{"@id":"ocpp:Other1PhMax16A"},{"@id":"ocpp:Other1PhOver16A"},{"@id":"ocpp:Other3Ph"},{"@id":"ocpp:Pan"},{"@id":"ocpp:Undetermined"},{"@id":"ocpp:Unknown"}]},{"@id":"ocpp:cCCS1","@type":["ocpp:ConnectorEnumType","schema:Enumeration"],"schema:name":"cCCS1","schema:identifier":"cCCS1"},{"@id":"ocpp:cCCS2","@type":["ocpp:ConnectorEnumType","schema:Enumeration"],"schema:name":"cCCS2","schema:identifier":"cCCS2"},{"@id":"ocpp:cChaoJi","@type":["ocpp:ConnectorEnumType","schema:Enumeration"],"schema:name":"cChaoJi","schema:identifier":"cChaoJi"},{"@id":"ocpp:cG105","@type":["ocpp:ConnectorEnumType","schema:Enumeration"],"schema:name":"cG105","schema:identifier":"cG105"},{"@id":"ocpp:cGBT-DC","@type":["ocpp:ConnectorEnumType","schema:Enumeration"],"schema:name":"cGBT-DC","schema:identifier":"cGBT-DC"},{"@id":"ocpp:cLECCS","@type":["ocpp:ConnectorEnumType","schema:Enumeration"],"schema:name":"cLECCS","schema:identifier":"cLECCS"},{"@id":"ocpp:cMCS","@type":["ocpp:ConnectorEnumType","schema:Enumeration"],"schema:name":"cMCS","schema:identifier":"cMCS"},{"@id":"ocpp:cNACS","@type":["ocpp:ConnectorEnumType","schema:Enumeration"],"schema:name":"cNACS","schema:identifier":"cNACS"},{"@id":"ocpp:cNACS-CCS1","@type":["ocpp:ConnectorEnumType","schema:Enumeration"],"schema:name":"cNACS-CCS1","schema:identifier":"cNACS-CCS1"},{"@id":"ocpp:cCCS1-NACS","@type":["ocpp:ConnectorEnumType","schema:Enumeration"],"schema:name":"cCCS1-NACS","schema:identifier":"cCCS1-NACS"},{"@id":"ocpp:cTesla","@type":["ocpp:ConnectorEnumType","schema:Enumeration"],"schema:name":"cTesla","schema:identifier":"cTesla"},{"@id":"ocpp:cType1","@type":["ocpp:ConnectorEnumType","schema:Enumeration"],"schema:name":"cType1","schema:identifier":"cType1"},{"@id":"ocpp:cType2","@type":["ocpp:ConnectorEnumType","schema:Enumeration"],"schema:name":"cType2","schema:identifier":"cType2"},{"@id":"ocpp:cUltraChaoJi","@type":["ocpp:ConnectorEnumType","schema:Enumeration"],"schema:name":"cUltraChaoJi","schema:identifier":"cUltraChaoJi"},{"@id":"ocpp:s309-1P-16A","@type":["ocpp:ConnectorEnumType","schema:Enumeration"],"schema:name":"s309-1P-16A","schema:identifier":"s309-1P-16A"},{"@id":"ocpp:s309-1P-32A","@type":["ocpp:ConnectorEnumType","schema:Enumeration"],"schema:name":"s309-1P-32A","schema:identifier":"s309-1P-32A"},{"@id":"ocpp:s309-3P-16A","@type":["ocpp:ConnectorEnumType","schema:Enumeration"],"schema:name":"s309-3P-16A","schema:identifier":"s309-3P-16A"},{"@id":"ocpp:s309-3P-32A","@type":["ocpp:ConnectorEnumType","schema:Enumeration"],"schema:name":"s309-3P-32A","schema:identifier":"s309-3P-32A"},{"@id":"ocpp:sBS1361","@type":["ocpp:ConnectorEnumType","schema:Enumeration"],"schema:name":"sBS1361","schema:identifier":"sBS1361"},{"@id":"ocpp:sCEE-7-7","@type":["ocpp:ConnectorEnumType","schema:Enumeration"],"schema:name":"sCEE-7-7","schema:identifier":"sCEE-7-7"},{"@id":"ocpp:sType1","@type":["ocpp:ConnectorEnumType","schema:Enumeration"],"schema:name":"sType1","schema:identifier":"sType1"},{"@id":"ocpp:sType2","@type":["ocpp:ConnectorEnumType","schema:Enumeration"],"schema:name":"sType2","schema:identifier":"sType2"},{"@id":"ocpp:sType3","@type":["ocpp:ConnectorEnumType","schema:Enumeration"],"schema:name":"sType3","schema:identifier":"sType3"},{"@id":"ocpp:wInductive","@type":["ocpp:ConnectorEnumType","schema:Enumeration"],"schema:name":"wInductive","schema:identifier":"wInductive"},{"@id":"ocpp:wResonant","@type":["ocpp:ConnectorEnumType","schema:Enumeration"],"schema:name":"wResonant","schema:identifier":"wResonant"},{"@id":"ocpp:Other1PhMax16A","@type":["ocpp:ConnectorEnumType","schema:Enumeration"],"schema:name":"Other1PhMax16A","schema:identifier":"Other1PhMax16A"},{"@id":"ocpp:Other1PhOver16A","@type":["ocpp:ConnectorEnumType","schema:Enumeration"],"schema:name":"Other1PhOver16A","schema:identifier":"Other1PhOver16A"},{"@id":"ocpp:Other3Ph","@type":["ocpp:ConnectorEnumType","schema:Enumeration"],"schema:name":"Other3Ph","schema:identifier":"Other3Ph"},{"@id":"ocpp:Pan","@type":["ocpp:ConnectorEnumType","schema:Enumeration"],"schema:name":"Pan","schema:identifier":"Pan"},{"@id":"ocpp:Undetermined","@type":["ocpp:ConnectorEnumType","schema:Enumeration"],"schema:name":"Undetermined","schema:identifier":"Undetermined"},{"@id":"ocpp:Unknown","@type":["ocpp:ConnectorEnumType","schema:Enumeration"],"schema:name":"Unknown","schema:identifier":"Unknown"},{"@id":"ocpp:IdTokenEnumType","@type":"schema:Enumeration","schema:name":"IdTokenEnumType","rdfs:comment":"Enumeration values from idtokenenumtype.csv","schema:hasEnumerationMember":[{"@id":"ocpp:Central"},{"@id":"ocpp:DirectPayment"},{"@id":"ocpp:eMAID"},{"@id":"ocpp:EVCCID"},{"@id":"ocpp:ISO14443"},{"@id":"ocpp:ISO15693"},{"@id":"ocpp:KeyCode"},{"@id":"ocpp:Local"},{"@id":"ocpp:MacAddress"},{"@id":"ocpp:NoAuthorization"},{"@id":"ocpp:VIN"}]},{"@id":"ocpp:Central","@type":["ocpp:IdTokenEnumType","schema:Enumeration"],"schema:name":"Central","schema:identifier":"Central"},{"@id":"ocpp:DirectPayment","@type":["ocpp:IdTokenEnumType","schema:Enumeration"],"schema:name":"DirectPayment","schema:identifier":"DirectPayment"},{"@id":"ocpp:eMAID","@type":["ocpp:IdTokenEnumType","schema:Enumeration"],"schema:name":"eMAID","schema:identifier":"eMAID"},{"@id":"ocpp:EVCCID","@type":["ocpp:IdTokenEnumType","schema:Enumeration"],"schema:name":"EVCCID","schema:identifier":"EVCCID"},{"@id":"ocpp:ISO14443","@type":["ocpp:IdTokenEnumType","schema:Enumeration"],"schema:name":"ISO14443","schema:identifier":"ISO14443"},{"@id":"ocpp:ISO15693","@type":["ocpp:IdTokenEnumType","schema:Enumeration"],"schema:name":"ISO15693","schema:identifier":"ISO15693"},{"@id":"ocpp:KeyCode","@type":["ocpp:IdTokenEnumType","schema:Enumeration"],"schema:name":"KeyCode","schema:identifier":"KeyCode"},{"@id":"ocpp:Local","@type":["ocpp:IdTokenEnumType","schema:Enumeration"],"schema:name":"Local","schema:identifier":"Local"},{"@id":"ocpp:MacAddress","@type":["ocpp:IdTokenEnumType","schema:Enumeration"],"schema:name":"MacAddress","schema:identifier":"MacAddress"},{"@id":"ocpp:NoAuthorization","@type":["ocpp:IdTokenEnumType","schema:Enumeration"],"schema:name":"NoAuthorization","schema:identifier":"NoAuthorization"},{"@id":"ocpp:VIN","@type":["ocpp:IdTokenEnumType","schema:Enumeration"],"schema:name":"VIN","schema:identifier":"VIN"},{"@id":"ocpp:AdditionalInfoTypeAdHocEnumType","@type":"schema:Enumeration","schema:name":"AdditionalInfoTypeAdHocEnumType","rdfs:comment":"Enumeration values from additional_info_types_adhoc.csv","schema:hasEnumerationMember":[{"@id":"ocpp:PspRef"},{"@id":"ocpp:SessionRef"},{"@id":"ocpp:MerchantRef"},{"@id":"ocpp:PaymentBrand"},{"@id":"ocpp:ReadingMethod"},{"@id":"ocpp:PaymentRecognition"},{"@id":"ocpp:CardBin"},{"@id":"ocpp:CardLast4Digits"},{"@id":"ocpp:CardExpiryDate"},{"@id":"ocpp:HashedCardNr"},{"@id":"ocpp:WalletUserId"}]},{"@id":"ocpp:PspRef","@type":["ocpp:AdditionalInfoTypeAdHocEnumType","schema:Enumeration"],"schema:name":"PspRef","schema:identifier":"PspRef"},{"@id":"ocpp:SessionRef","@type":["ocpp:AdditionalInfoTypeAdHocEnumType","schema:Enumeration"],"schema:name":"SessionRef","schema:identifier":"SessionRef"},{"@id":"ocpp:MerchantRef","@type":["ocpp:AdditionalInfoTypeAdHocEnumType","schema:Enumeration"],"schema:name":"MerchantRef","schema:identifier":"MerchantRef"},{"@id":"ocpp:PaymentBrand","@type":["ocpp:AdditionalInfoTypeAdHocEnumType","schema:Enumeration"],"schema:name":"PaymentBrand","schema:identifier":"PaymentBrand"},{"@id":"ocpp:ReadingMethod","@type":["ocpp:AdditionalInfoTypeAdHocEnumType","schema:Enumeration"],"schema:name":"ReadingMethod","schema:identifier":"ReadingMethod"},{"@id":"ocpp:PaymentRecognition","@type":["ocpp:AdditionalInfoTypeAdHocEnumType","schema:Enumeration"],"schema:name":"PaymentRecognition","schema:identifier":"PaymentRecognition"},{"@id":"ocpp:CardBin","@type":["ocpp:AdditionalInfoTypeAdHocEnumType","schema:Enumeration"],"schema:name":"CardBin","schema:identifier":"CardBin"},{"@id":"ocpp:CardLast4Digits","@type":["ocpp:AdditionalInfoTypeAdHocEnumType","schema:Enumeration"],"schema:name":"CardLast4Digits","schema:identifier":"CardLast4Digits"},{"@id":"ocpp:CardExpiryDate","@type":["ocpp:AdditionalInfoTypeAdHocEnumType","schema:Enumeration"],"schema:name":"CardExpiryDate","schema:identifier":"CardExpiryDate"},{"@id":"ocpp:HashedCardNr","@type":["ocpp:AdditionalInfoTypeAdHocEnumType","schema:Enumeration"],"schema:name":"HashedCardNr","schema:identifier":"HashedCardNr"},{"@id":"ocpp:WalletUserId","@type":["ocpp:AdditionalInfoTypeAdHocEnumType","schema:Enumeration"],"schema:name":"WalletUserId","schema:identifier":"WalletUserId"},{"@id":"ocpp:ChargingLimitSourceEnumType","@type":"schema:Enumeration","schema:name":"ChargingLimitSourceEnumType","rdfs:comment":"Enumeration values from charginglimitsourceenumtype.csv","schema:hasEnumerationMember":[{"@id":"ocpp:EMS"},{"@id":"ocpp:Other"},{"@id":"ocpp:SO"},{"@id":"ocpp:CSO"}]},{"@id":"ocpp:EMS","@type":["ocpp:ChargingLimitSourceEnumType","schema:Enumeration"],"schema:name":"EMS","schema:identifier":"EMS"},{"@id":"ocpp:Other","@type":["ocpp:ChargingLimitSourceEnumType","schema:Enumeration"],"schema:name":"Other","schema:identifier":"Other"},{"@id":"ocpp:SO","@type":["ocpp:ChargingLimitSourceEnumType","schema:Enumeration"],"schema:name":"SO","schema:identifier":"SO"},{"@id":"ocpp:CSO","@type":["ocpp:ChargingLimitSourceEnumType","schema:Enumeration"],"schema:name":"CSO","schema:identifier":"CSO"},{"@id":"ocpp:AdditionalInfoTypeEnumType","@type":"schema:Enumeration","schema:name":"AdditionalInfoTypeEnumType","rdfs:comment":"Enumeration values from additional_info_types.csv","schema:hasEnumerationMember":[{"@id":"ocpp:EVCCID"},{"@id":"ocpp:ISO14443SubType"}]},{"@id":"ocpp:EVCCID","@type":["ocpp:AdditionalInfoTypeEnumType","schema:Enumeration"],"schema:name":"EVCCID","schema:identifier":"EVCCID"},{"@id":"ocpp:ISO14443SubType","@type":["ocpp:AdditionalInfoTypeEnumType","schema:Enumeration"],"schema:name":"ISO14443SubType","schema:identifier":"ISO14443SubType"},{"@id":"ocpp:additionalInfo","@type":"rdf:Property","rdfs:label":"additionalInfo","rdfs:comment":"Additional text to provide detailed information.\r\n","rdfs:domain":["ocpp:StatusInfoType","ocpp:IdTokenType"],"schema:rangeIncludes":"xsd:string"},{"@id":"ocpp:customData","@type":"rdf:Property","rdfs:label":"customData","rdfs:comment":"Property customData","rdfs:domain":["ocpp:StatusInfoType","ocpp:PeriodicEventStreamParamsType","ocpp:AdditionalInfoType","ocpp:IdTokenType","ocpp:OCSPRequestDataType"]},{"@id":"ocpp:type","@type":"rdf:Property","rdfs:label":"type","rdfs:comment":"_additionalInfo_ can be used to send extra information to CSMS in addition to the regular authorization with _IdToken_. _AdditionalInfo_ contains one or more custom _types_, which need to be agreed upon by all parties involved. When the _type_ is not supported, the CSMS/Charging Station MAY ignore the _additionalInfo_.\r\n\r\n","rdfs:domain":["ocpp:AdditionalInfoType","ocpp:IdTokenType","ocpp:TaxRateType","ocpp:VariableMonitoringType","ocpp:VariableAttributeType"],"schema:rangeIncludes":"xsd:string"},{"@id":"ocpp:idToken","@type":"rdf:Property","rdfs:label":"idToken","rdfs:comment":"*(2.1)* IdToken is case insensitive. Might hold the hidden id of an RFID tag, but can for example also contain a UUID.\r\n","rdfs:domain":["ocpp:IdTokenType","ocpp:AuthorizationData"],"schema:rangeIncludes":"xsd:string"},{"@id":"ocpp:hashAlgorithm","@type":"rdf:Property","rdfs:label":"hashAlgorithm","rdfs:comment":"Property hashAlgorithm","rdfs:domain":["ocpp:OCSPRequestDataType","ocpp:CertificateHashDataType"]},{"@id":"ocpp:issuerNameHash","@type":"rdf:Property","rdfs:label":"issuerNameHash","rdfs:comment":"The hash of the issuers distinguished\r\nname (DN), that must be calculated over the DER\r\nencoding of the issuers name field in the certificate\r\nbeing checked.\r\n\r\n","rdfs:domain":["ocpp:OCSPRequestDataType","ocpp:CertificateHashDataType"],"schema:rangeIncludes":"xsd:string"},{"@id":"ocpp:issuerKeyHash","@type":"rdf:Property","rdfs:label":"issuerKeyHash","rdfs:comment":"The hash of the DER encoded public key:\r\nthe value (excluding tag and length) of the subject\r\npublic key field in the issuers certificate.\r\n","rdfs:domain":["ocpp:OCSPRequestDataType","ocpp:CertificateHashDataType"],"schema:rangeIncludes":"xsd:string"},{"@id":"ocpp:serialNumber","@type":"rdf:Property","rdfs:label":"serialNumber","rdfs:comment":"The string representation of the\r\nhexadecimal value of the serial number without the\r\nprefix \"0x\" and without leading zeroes.\r\n","rdfs:domain":["ocpp:OCSPRequestDataType","ocpp:BatteryDataType","ocpp:ChargingStationType","ocpp:CertificateHashDataType"],"schema:rangeIncludes":"xsd:string"},{"@id":"ocpp:status","@type":"rdf:Property","rdfs:label":"status","rdfs:comment":"Property status","rdfs:domain":["ocpp:IdTokenInfoType","ocpp:ClearTariffsResultType","ocpp:ClearMonitoringResultType","ocpp:CertificateStatusType","ocpp:SetMonitoringResultType"]},{"@id":"ocpp:evseId","@type":"rdf:Property","rdfs:label":"evseId","rdfs:comment":"Specifies the id of the EVSE for which to clear charging profiles. An evseId of zero (0) specifies the charging profile for the overall Charging Station. Absence of this parameter means the clearing applies to all charging profiles that match the other criteria in the request.\r\n\r\n","rdfs:domain":["ocpp:IdTokenInfoType","ocpp:BatteryDataType","ocpp:ClearChargingProfileType","ocpp:CompositeScheduleType"],"schema:rangeIncludes":"xsd:integer"},{"@id":"ocpp:language","@type":"rdf:Property","rdfs:label":"language","rdfs:comment":"String that indicates what language is used for the human readable strings in the price schedule. Based on ISO 639.\r\n","rdfs:domain":["ocpp:MessageContentType","ocpp:AbsolutePriceScheduleType"],"schema:rangeIncludes":"xsd:string"},{"@id":"ocpp:exclTax","@type":"rdf:Property","rdfs:label":"exclTax","rdfs:comment":"Price/cost excluding tax. Can be absent if _inclTax_ is present.\r\n","rdfs:domain":["ocpp:PriceType","ocpp:TotalPriceType"],"schema:rangeIncludes":"xsd:double"},{"@id":"ocpp:inclTax","@type":"rdf:Property","rdfs:label":"inclTax","rdfs:comment":"Price/cost including tax. Can be absent if _exclTax_ is present.\r\n","rdfs:domain":["ocpp:PriceType","ocpp:TotalPriceType"],"schema:rangeIncludes":"xsd:double"},{"@id":"ocpp:taxRates","@type":"rdf:Property","rdfs:label":"taxRates","rdfs:comment":"Property taxRates","rdfs:domain":["ocpp:PriceType","ocpp:TariffEnergyType","ocpp:TariffFixedType","ocpp:TariffTimeType"]},{"@id":"ocpp:startTimeOfDay","@type":"rdf:Property","rdfs:label":"startTimeOfDay","rdfs:comment":"Start time of day in local time. +\r\nFormat as per RFC 3339: time-hour \":\" time-minute  +\r\nMust be in 24h format with leading zeros. Hour/Minute separator: \":\"\r\nRegex: ([0-1][0-9]\\|2[0-3]):[0-5][0-9]\r\n","rdfs:domain":["ocpp:TariffConditionsFixedType","ocpp:TariffConditionsType"],"schema:rangeIncludes":"xsd:string"},{"@id":"ocpp:endTimeOfDay","@type":"rdf:Property","rdfs:label":"endTimeOfDay","rdfs:comment":"End time of day in local time. Same syntax as _startTimeOfDay_. +\r\n    If end time &lt; start time then the period wraps around to the next day. +\r\n    To stop at end of the day use: 00:00.\r\n","rdfs:domain":["ocpp:TariffConditionsFixedType","ocpp:TariffConditionsType"],"schema:rangeIncludes":"xsd:string"},{"@id":"ocpp:dayOfWeek","@type":"rdf:Property","rdfs:label":"dayOfWeek","rdfs:comment":"Day(s) of the week this is tariff applies.\r\n","rdfs:domain":["ocpp:TariffConditionsFixedType","ocpp:TariffConditionsType"]},{"@id":"ocpp:validFromDate","@type":"rdf:Property","rdfs:label":"validFromDate","rdfs:comment":"Start date in local time, for example: 2015-12-24.\r\nValid from this day (inclusive). +\r\nFormat as per RFC 3339: full-date  + \r\n\r\nRegex: ([12][0-9]{3})-(0[1-9]\\|1[0-2])-(0[1-9]\\|[12][0-9]\\|3[01])\r\n","rdfs:domain":["ocpp:TariffConditionsFixedType","ocpp:TariffConditionsType"],"schema:rangeIncludes":"xsd:string"},{"@id":"ocpp:validToDate","@type":"rdf:Property","rdfs:label":"validToDate","rdfs:comment":"End date in local time, for example: 2015-12-27.\r\n    Valid until this day (exclusive). Same syntax as _validFromDate_.\r\n","rdfs:domain":["ocpp:TariffConditionsFixedType","ocpp:TariffConditionsType"],"schema:rangeIncludes":"xsd:string"},{"@id":"ocpp:evseKind","@type":"rdf:Property","rdfs:label":"evseKind","rdfs:comment":"Property evseKind","rdfs:domain":["ocpp:TariffConditionsFixedType","ocpp:TariffConditionsType"]},{"@id":"ocpp:maxEnergy","@type":"rdf:Property","rdfs:label":"maxEnergy","rdfs:comment":"Maximum consumed energy in Wh, for example 50000 Wh.\r\n    Valid until this amount of energy (exclusive) being used.\r\n","rdfs:domain":["ocpp:TariffConditionsType","ocpp:TransactionLimitType"],"schema:rangeIncludes":"xsd:double"},{"@id":"ocpp:maxTime","@type":"rdf:Property","rdfs:label":"maxTime","rdfs:comment":"Maximum duration in seconds the transaction (charging &amp; idle) MUST last (exclusive).\r\n      When the duration of a transaction is shorter than the defined value, this price is or becomes active.\r\n      After that moment, this price is no longer active.\r\n","rdfs:domain":["ocpp:TariffConditionsType","ocpp:TransactionLimitType"],"schema:rangeIncludes":"xsd:integer"},{"@id":"ocpp:conditions","@type":"rdf:Property","rdfs:label":"conditions","rdfs:comment":"Property conditions","rdfs:domain":["ocpp:TariffEnergyPriceType","ocpp:TariffFixedPriceType","ocpp:TariffTimePriceType"]},{"@id":"ocpp:prices","@type":"rdf:Property","rdfs:label":"prices","rdfs:comment":"Property prices","rdfs:domain":["ocpp:TariffEnergyType","ocpp:TariffFixedType","ocpp:TariffTimeType"]},{"@id":"ocpp:tariffId","@type":"rdf:Property","rdfs:label":"tariffId","rdfs:comment":"Id of tariff for which _status_ is reported. If no tariffs were found, then this field is absent, and _status_ will be `NoTariff`.\r\n","rdfs:domain":["ocpp:TariffType","ocpp:ClearTariffsResultType","ocpp:TariffAssignmentType","ocpp:ChargingPeriodType","ocpp:TransactionType"],"schema:rangeIncludes":"xsd:string"},{"@id":"ocpp:currency","@type":"rdf:Property","rdfs:label":"currency","rdfs:comment":"Currency of the costs in ISO 4217 Code.\r\n\r\n","rdfs:domain":["ocpp:TariffType","ocpp:AbsolutePriceScheduleType","ocpp:EVAbsolutePriceScheduleType","ocpp:TotalCostType"],"schema:rangeIncludes":"xsd:string"},{"@id":"ocpp:energy","@type":"rdf:Property","rdfs:label":"energy","rdfs:comment":"Property energy","rdfs:domain":["ocpp:TariffType","ocpp:TotalCostType","ocpp:TotalUsageType"],"schema:rangeIncludes":"xsd:double"},{"@id":"ocpp:validFrom","@type":"rdf:Property","rdfs:label":"validFrom","rdfs:comment":"Point in time at which the profile starts to be valid. If absent, the profile is valid as soon as it is received by the Charging Station.\r\n","rdfs:domain":["ocpp:TariffType","ocpp:TariffAssignmentType","ocpp:ChargingProfileType"],"schema:rangeIncludes":"xsd:string"},{"@id":"ocpp:chargingTime","@type":"rdf:Property","rdfs:label":"chargingTime","rdfs:comment":"Total duration of the charging session (including the duration of charging and not charging), in seconds.\r\n\r\n\r\n","rdfs:domain":["ocpp:TariffType","ocpp:TotalCostType","ocpp:TotalUsageType"],"schema:rangeIncludes":"xsd:integer"},{"@id":"ocpp:idleTime","@type":"rdf:Property","rdfs:label":"idleTime","rdfs:comment":"Total duration of the charging session where the EV was not charging (no energy was transferred between EVSE and EV), in seconds.\r\n\r\n\r\n","rdfs:domain":["ocpp:TariffType","ocpp:TotalCostType","ocpp:TotalUsageType"],"schema:rangeIncludes":"xsd:integer"},{"@id":"ocpp:reservationTime","@type":"rdf:Property","rdfs:label":"reservationTime","rdfs:comment":"Total time of reservation in seconds.\r\n","rdfs:domain":["ocpp:TariffType","ocpp:TotalCostType","ocpp:TotalUsageType"],"schema:rangeIncludes":"xsd:integer"},{"@id":"ocpp:reservationFixed","@type":"rdf:Property","rdfs:label":"reservationFixed","rdfs:comment":"Property reservationFixed","rdfs:domain":["ocpp:TariffType","ocpp:TotalCostType"]},{"@id":"ocpp:maxCost","@type":"rdf:Property","rdfs:label":"maxCost","rdfs:comment":"Maximum allowed cost of transaction in currency of tariff.\r\n","rdfs:domain":["ocpp:TariffType","ocpp:TransactionLimitType"],"schema:rangeIncludes":"xsd:double"},{"@id":"ocpp:id","@type":"rdf:Property","rdfs:label":"id","rdfs:comment":"Id given to the VariableMonitor by the Charging Station. The Id is only returned when status is accepted. Installed VariableMonitors should have unique id's but the id's of removed Installed monitors should have unique id's but the id's of removed monitors MAY be reused.\r\n","rdfs:domain":["ocpp:EVSEType","ocpp:ClearMonitoringResultType","ocpp:ConstantStreamDataType","ocpp:ChargingScheduleType","ocpp:SalesTariffType"],"schema:rangeIncludes":"xsd:string"},{"@id":"ocpp:chargingProfilePurpose","@type":"rdf:Property","rdfs:label":"chargingProfilePurpose","rdfs:comment":"Property chargingProfilePurpose","rdfs:domain":["ocpp:ClearChargingProfileType","ocpp:ChargingProfileCriterionType","ocpp:ChargingProfileType"]},{"@id":"ocpp:stackLevel","@type":"rdf:Property","rdfs:label":"stackLevel","rdfs:comment":"Value determining level in hierarchy stack of profiles. Higher values have precedence over lower values. Lowest level is 0.\r\n","rdfs:domain":["ocpp:ClearChargingProfileType","ocpp:ChargingProfileCriterionType","ocpp:ChargingProfileType"],"schema:rangeIncludes":"xsd:integer"},{"@id":"ocpp:statusInfo","@type":"rdf:Property","rdfs:label":"statusInfo","rdfs:comment":"Property statusInfo","rdfs:domain":["ocpp:ClearTariffsResultType","ocpp:ClearMonitoringResultType","ocpp:SetMonitoringResultType"]},{"@id":"ocpp:certificateHashData","@type":"rdf:Property","rdfs:label":"certificateHashData","rdfs:comment":"Property certificateHashData","rdfs:domain":["ocpp:CertificateStatusRequestInfoType","ocpp:CertificateStatusType","ocpp:CertificateHashDataChainType"]},{"@id":"ocpp:source","@type":"rdf:Property","rdfs:label":"source","rdfs:comment":"Property source","rdfs:domain":["ocpp:CertificateStatusRequestInfoType","ocpp:CertificateStatusType"]},{"@id":"ocpp:chargingLimitSource","@type":"rdf:Property","rdfs:label":"chargingLimitSource","rdfs:comment":"For which charging limit sources, charging profiles SHALL be reported. If omitted, the Charging Station SHALL not filter on chargingLimitSource. Values defined in Appendix as ChargingLimitSourceEnumStringType.\r\n","rdfs:domain":["ocpp:ChargingProfileCriterionType","ocpp:ChargingLimitType"],"schema:rangeIncludes":"xsd:string"},{"@id":"ocpp:startPeriod","@type":"rdf:Property","rdfs:label":"startPeriod","rdfs:comment":"Start of the period, in seconds from the start of schedule. The value of StartPeriod also defines the stop time of the previous period.\r\n","rdfs:domain":["ocpp:ChargingSchedulePeriodType","ocpp:ChargingPeriodType"],"schema:rangeIncludes":"xsd:string"},{"@id":"ocpp:limit","@type":"rdf:Property","rdfs:label":"limit","rdfs:comment":"Optional only when not required by the _operationMode_, as in CentralSetpoint, ExternalSetpoint, ExternalLimits, LocalFrequency,  LocalLoadBalancing. +\r\nCharging rate limit during the schedule period, in the applicable _chargingRateUnit_. \r\nThis SHOULD be a non-negative value; a negative value is only supported for backwards compatibility with older systems that use a negative value to specify a discharging limit.\r\nWhen using _chargingRateUnit_ = `W`, this field represents the sum of the power of all phases, unless values are provided for L2 and L3, in which case this field represents phase L1.\r\n","rdfs:domain":["ocpp:ChargingSchedulePeriodType","ocpp:LimitAtSoCType","ocpp:ChargingScheduleUpdateType"],"schema:rangeIncludes":"xsd:double"},{"@id":"ocpp:limit_L2","@type":"rdf:Property","rdfs:label":"limit_L2","rdfs:comment":"*(2.1)* Charging rate limit on phase L2  in the applicable _chargingRateUnit_. \r\n","rdfs:domain":["ocpp:ChargingSchedulePeriodType","ocpp:ChargingScheduleUpdateType"],"schema:rangeIncludes":"xsd:double"},{"@id":"ocpp:limit_L3","@type":"rdf:Property","rdfs:label":"limit_L3","rdfs:comment":"*(2.1)* Charging rate limit on phase L3  in the applicable _chargingRateUnit_. \r\n","rdfs:domain":["ocpp:ChargingSchedulePeriodType","ocpp:ChargingScheduleUpdateType"],"schema:rangeIncludes":"xsd:double"},{"@id":"ocpp:dischargeLimit","@type":"rdf:Property","rdfs:label":"dischargeLimit","rdfs:comment":"*(2.1)* Limit in _chargingRateUnit_ that the EV is allowed to discharge with. Note, these are negative values in order to be consistent with _setpoint_, which can be positive and negative.  +\r\nFor AC this field represents the sum of all phases, unless values are provided for L2 and L3, in which case this field represents phase L1.\r\n","rdfs:domain":["ocpp:ChargingSchedulePeriodType","ocpp:ChargingScheduleUpdateType"],"schema:rangeIncludes":"xsd:double"},{"@id":"ocpp:dischargeLimit_L2","@type":"rdf:Property","rdfs:label":"dischargeLimit_L2","rdfs:comment":"*(2.1)* Limit in _chargingRateUnit_ on phase L2 that the EV is allowed to discharge with. \r\n","rdfs:domain":["ocpp:ChargingSchedulePeriodType","ocpp:ChargingScheduleUpdateType"],"schema:rangeIncludes":"xsd:double"},{"@id":"ocpp:dischargeLimit_L3","@type":"rdf:Property","rdfs:label":"dischargeLimit_L3","rdfs:comment":"*(2.1)* Limit in _chargingRateUnit_ on phase L3 that the EV is allowed to discharge with. \r\n","rdfs:domain":["ocpp:ChargingSchedulePeriodType","ocpp:ChargingScheduleUpdateType"],"schema:rangeIncludes":"xsd:double"},{"@id":"ocpp:setpoint","@type":"rdf:Property","rdfs:label":"setpoint","rdfs:comment":"*(2.1)* Setpoint in _chargingRateUnit_ that the EV should follow as close as possible. Use negative values for discharging. +\r\nWhen a limit and/or _dischargeLimit_ are given the overshoot when following _setpoint_ must remain within these values.\r\nThis field represents the sum of all phases, unless values are provided for L2 and L3, in which case this field represents phase L1.\r\n","rdfs:domain":["ocpp:ChargingSchedulePeriodType","ocpp:ChargingScheduleUpdateType","ocpp:FixedVarType"],"schema:rangeIncludes":"xsd:double"},{"@id":"ocpp:setpoint_L2","@type":"rdf:Property","rdfs:label":"setpoint_L2","rdfs:comment":"*(2.1)* Setpoint in _chargingRateUnit_ that the EV should follow on phase L2 as close as possible.\r\n","rdfs:domain":["ocpp:ChargingSchedulePeriodType","ocpp:ChargingScheduleUpdateType"],"schema:rangeIncludes":"xsd:double"},{"@id":"ocpp:setpoint_L3","@type":"rdf:Property","rdfs:label":"setpoint_L3","rdfs:comment":"*(2.1)* Setpoint in _chargingRateUnit_ that the EV should follow on phase L3 as close as possible. \r\n","rdfs:domain":["ocpp:ChargingSchedulePeriodType","ocpp:ChargingScheduleUpdateType"],"schema:rangeIncludes":"xsd:double"},{"@id":"ocpp:setpointReactive","@type":"rdf:Property","rdfs:label":"setpointReactive","rdfs:comment":"*(2.1)* Setpoint for reactive power (or current) in _chargingRateUnit_ that the EV should follow as closely as possible. Positive values for inductive, negative for capacitive reactive power or current.  +\r\nThis field represents the sum of all phases, unless values are provided for L2 and L3, in which case this field represents phase L1.\r\n","rdfs:domain":["ocpp:ChargingSchedulePeriodType","ocpp:ChargingScheduleUpdateType"],"schema:rangeIncludes":"xsd:double"},{"@id":"ocpp:setpointReactive_L2","@type":"rdf:Property","rdfs:label":"setpointReactive_L2","rdfs:comment":"*(2.1)* Setpoint for reactive power (or current) in _chargingRateUnit_ that the EV should follow on phase L2 as closely as possible. \r\n","rdfs:domain":["ocpp:ChargingSchedulePeriodType","ocpp:ChargingScheduleUpdateType"],"schema:rangeIncludes":"xsd:double"},{"@id":"ocpp:setpointReactive_L3","@type":"rdf:Property","rdfs:label":"setpointReactive_L3","rdfs:comment":"*(2.1)* Setpoint for reactive power (or current) in _chargingRateUnit_ that the EV should follow on phase L3 as closely as possible. \r\n","rdfs:domain":["ocpp:ChargingSchedulePeriodType","ocpp:ChargingScheduleUpdateType"],"schema:rangeIncludes":"xsd:double"},{"@id":"ocpp:operationMode","@type":"rdf:Property","rdfs:label":"operationMode","rdfs:comment":"Property operationMode","rdfs:domain":["ocpp:ChargingSchedulePeriodType","ocpp:TransactionType"]},{"@id":"ocpp:duration","@type":"rdf:Property","rdfs:label":"duration","rdfs:comment":"Duration of the charging schedule in seconds. If the duration is left empty, the last period will continue indefinitely or until end of the transaction in case startSchedule is absent.\r\n","rdfs:domain":["ocpp:CompositeScheduleType","ocpp:ChargingScheduleType","ocpp:PriceLevelScheduleEntryType","ocpp:PriceRuleStackType","ocpp:RelativeTimeIntervalType"],"schema:rangeIncludes":"xsd:integer"},{"@id":"ocpp:chargingRateUnit","@type":"rdf:Property","rdfs:label":"chargingRateUnit","rdfs:comment":"Property chargingRateUnit","rdfs:domain":["ocpp:CompositeScheduleType","ocpp:ChargingScheduleType"]},{"@id":"ocpp:chargingSchedulePeriod","@type":"rdf:Property","rdfs:label":"chargingSchedulePeriod","rdfs:comment":"Property chargingSchedulePeriod","rdfs:domain":["ocpp:CompositeScheduleType","ocpp:ChargingScheduleType"]},{"@id":"ocpp:power","@type":"rdf:Property","rdfs:label":"power","rdfs:comment":"Defines maximum amount of power for the duration of this EVPowerScheduleEntry to be discharged from the EV battery through EVSE power outlet. Negative values are used for discharging.\r\n","rdfs:domain":["ocpp:V2XFreqWattPointType","ocpp:V2XSignalWattPointType","ocpp:EVPowerScheduleEntryType"],"schema:rangeIncludes":"xsd:double"},{"@id":"ocpp:name","@type":"rdf:Property","rdfs:label":"name","rdfs:comment":"Name of the component. Name should be taken from the list of standardized component names whenever possible. Case Insensitive. strongly advised to use Camel Case.\r\n","rdfs:domain":["ocpp:ComponentType","ocpp:VariableType","ocpp:AddressType"],"schema:rangeIncludes":"xsd:string"},{"@id":"ocpp:instance","@type":"rdf:Property","rdfs:label":"instance","rdfs:comment":"Name of instance in case the component exists as multiple instances. Case Insensitive. strongly advised to use Camel Case.\r\n","rdfs:domain":["ocpp:ComponentType","ocpp:VariableType"],"schema:rangeIncludes":"xsd:string"},{"@id":"ocpp:component","@type":"rdf:Property","rdfs:label":"component","rdfs:comment":"Property component","rdfs:domain":["ocpp:ComponentVariableType","ocpp:GetVariableDataType","ocpp:GetVariableResultType","ocpp:EventDataType","ocpp:MonitoringDataType"]},{"@id":"ocpp:variable","@type":"rdf:Property","rdfs:label":"variable","rdfs:comment":"Property variable","rdfs:domain":["ocpp:ComponentVariableType","ocpp:GetVariableDataType","ocpp:GetVariableResultType","ocpp:EventDataType","ocpp:MonitoringDataType"]},{"@id":"ocpp:variableMonitoringId","@type":"rdf:Property","rdfs:label":"variableMonitoringId","rdfs:comment":"Id of monitor used to report his event. It can be a preconfigured or hardwired monitor.\r\n","rdfs:domain":["ocpp:ConstantStreamDataType","ocpp:EventDataType"],"schema:rangeIncludes":"xsd:integer"},{"@id":"ocpp:attributeType","@type":"rdf:Property","rdfs:label":"attributeType","rdfs:comment":"Property attributeType","rdfs:domain":["ocpp:GetVariableDataType","ocpp:GetVariableResultType","ocpp:SetVariableDataType","ocpp:SetVariableResultType"]},{"@id":"ocpp:attributeStatus","@type":"rdf:Property","rdfs:label":"attributeStatus","rdfs:comment":"Property attributeStatus","rdfs:domain":["ocpp:GetVariableResultType","ocpp:SetVariableResultType"]},{"@id":"ocpp:attributeStatusInfo","@type":"rdf:Property","rdfs:label":"attributeStatusInfo","rdfs:comment":"Property attributeStatusInfo","rdfs:domain":["ocpp:GetVariableResultType","ocpp:SetVariableResultType"]},{"@id":"ocpp:attributeValue","@type":"rdf:Property","rdfs:label":"attributeValue","rdfs:comment":"Value of requested attribute type of component-variable. This field can only be empty when the given status is NOT accepted.\r\n\r\nThe Configuration Variable &lt;&lt;configkey-reporting-value-size,ReportingValueSize&gt;&gt; can be used to limit GetVariableResult.attributeValue, VariableAttribute.value and EventData.actualValue. The max size of these values will always remain equal. \r\n\r\n","rdfs:domain":["ocpp:GetVariableResultType","ocpp:SetVariableDataType"],"schema:rangeIncludes":"xsd:string"},{"@id":"ocpp:timestamp","@type":"rdf:Property","rdfs:label":"timestamp","rdfs:comment":"Timestamp of the moment the report was generated.\r\n","rdfs:domain":["ocpp:MeterValueType","ocpp:EventDataType"],"schema:rangeIncludes":"xsd:string"},{"@id":"ocpp:value","@type":"rdf:Property","rdfs:label":"value","rdfs:comment":"Value of the attribute. May only be omitted when mutability is set to 'WriteOnly'.\r\n\r\nThe Configuration Variable &lt;&lt;configkey-reporting-value-size,ReportingValueSize&gt;&gt; can be used to limit GetVariableResult.attributeValue, VariableAttribute.value and EventData.actualValue. The max size of these values will always remain equal. \r\n","rdfs:domain":["ocpp:SampledValueType","ocpp:RationalNumberType","ocpp:VariableMonitoringType","ocpp:VariableAttributeType","ocpp:SetMonitoringDataType"],"schema:rangeIncludes":"xsd:string"},{"@id":"ocpp:location","@type":"rdf:Property","rdfs:label":"location","rdfs:comment":"URI defining the origin of the firmware.\r\n","rdfs:domain":["ocpp:SampledValueType","ocpp:FirmwareType"],"schema:rangeIncludes":"xsd:string"},{"@id":"ocpp:unit","@type":"rdf:Property","rdfs:label":"unit","rdfs:comment":"Unit of the value. Default = \"Wh\" if the (default) measurand is an \"Energy\" type.\r\nThis field SHALL use a value from the list Standardized Units of Measurements in Part 2 Appendices. \r\nIf an applicable unit is available in that list, otherwise a \"custom\" unit might be used.\r\n","rdfs:domain":["ocpp:UnitOfMeasureType","ocpp:VariableCharacteristicsType","ocpp:FixedVarType"],"schema:rangeIncludes":"xsd:string"},{"@id":"ocpp:timeAnchor","@type":"rdf:Property","rdfs:label":"timeAnchor","rdfs:comment":"The time that defines the starting point for the EVEnergyOffer.\r\n","rdfs:domain":["ocpp:AbsolutePriceScheduleType","ocpp:PriceLevelScheduleType","ocpp:EVAbsolutePriceScheduleType","ocpp:EVPowerScheduleType"],"schema:rangeIncludes":"xsd:string"},{"@id":"ocpp:priceScheduleDescription","@type":"rdf:Property","rdfs:label":"priceScheduleDescription","rdfs:comment":"Description of the price schedule.\r\n","rdfs:domain":["ocpp:AbsolutePriceScheduleType","ocpp:PriceLevelScheduleType"],"schema:rangeIncludes":"xsd:string"},{"@id":"ocpp:priceAlgorithm","@type":"rdf:Property","rdfs:label":"priceAlgorithm","rdfs:comment":"A string in URN notation which shall uniquely identify an algorithm that defines how to compute an energy fee sum for a specific power profile based on the EnergyFee information from the PriceRule elements.\r\n","rdfs:domain":["ocpp:AbsolutePriceScheduleType","ocpp:EVAbsolutePriceScheduleType"],"schema:rangeIncludes":"xsd:string"},{"@id":"ocpp:startTime","@type":"rdf:Property","rdfs:label":"startTime","rdfs:comment":"Time in seconds after trigger of the parent Overstay Rules for this particular fee to apply.\r\n","rdfs:domain":["ocpp:OverstayRuleType","ocpp:DERCurveType","ocpp:FixedPFType","ocpp:FixedVarType","ocpp:FreqDroopType"],"schema:rangeIncludes":"xsd:string"},{"@id":"ocpp:energyFee","@type":"rdf:Property","rdfs:label":"energyFee","rdfs:comment":"Cost per kWh.\r\n","rdfs:domain":["ocpp:PriceRuleType","ocpp:EVPriceRuleType"],"schema:rangeIncludes":"xsd:double"},{"@id":"ocpp:powerRangeStart","@type":"rdf:Property","rdfs:label":"powerRangeStart","rdfs:comment":"The EnergyFee applies between this value and the value of the PowerRangeStart of the subsequent EVPriceRule. If the power is below this value, the EnergyFee of the previous EVPriceRule applies. Negative values are used for discharging.\r\n","rdfs:domain":["ocpp:PriceRuleType","ocpp:EVPriceRuleType"],"schema:rangeIncludes":"xsd:double"},{"@id":"ocpp:priority","@type":"rdf:Property","rdfs:label":"priority","rdfs:comment":"Priority of setting (0=highest)\r\n\r\n\r\n","rdfs:domain":["ocpp:MessageInfoType","ocpp:DERCurveType","ocpp:EnterServiceType","ocpp:FixedPFType","ocpp:FixedVarType"],"schema:rangeIncludes":"xsd:integer"},{"@id":"ocpp:transactionId","@type":"rdf:Property","rdfs:label":"transactionId","rdfs:comment":"SHALL only be included if ChargingProfilePurpose is set to TxProfile in a SetChargingProfileRequest. The transactionId is used to match the profile to a specific transaction.\r\n","rdfs:domain":["ocpp:MessageInfoType","ocpp:EventDataType","ocpp:ChargingProfileType","ocpp:TransactionType"],"schema:rangeIncludes":"xsd:string"},{"@id":"ocpp:energyAmount","@type":"rdf:Property","rdfs:label":"energyAmount","rdfs:comment":"Amount of energy requested (in Wh). This includes energy required for preconditioning.\r\nRelates to: +\r\n*ISO 15118-2*: AC_EVChargeParameterType: EAmount +\r\n*ISO 15118-20*: Dynamic/Scheduled_SEReqControlModeType: EVTargetEnergyRequest\r\n\r\n","rdfs:domain":["ocpp:ACChargingParametersType","ocpp:DCChargingParametersType"],"schema:rangeIncludes":"xsd:double"},{"@id":"ocpp:evMaxCurrent","@type":"rdf:Property","rdfs:label":"evMaxCurrent","rdfs:comment":"Maximum current (amps) supported by the electric vehicle (per phase). Includes cable capacity.\r\nRelates to: +\r\n*ISO 15118-2*: AC_EVChargeParameterType: EVMaxCurrent\r\n\r\n","rdfs:domain":["ocpp:ACChargingParametersType","ocpp:DCChargingParametersType"],"schema:rangeIncludes":"xsd:double"},{"@id":"ocpp:evMaxVoltage","@type":"rdf:Property","rdfs:label":"evMaxVoltage","rdfs:comment":"Maximum voltage supported by the electric vehicle.\r\nRelates to: +\r\n*ISO 15118-2*: DC_EVChargeParameterType: EVMaximumVoltageLimit\r\n\r\n","rdfs:domain":["ocpp:ACChargingParametersType","ocpp:DCChargingParametersType"],"schema:rangeIncludes":"xsd:double"},{"@id":"ocpp:eventNotificationType","@type":"rdf:Property","rdfs:label":"eventNotificationType","rdfs:comment":"Property eventNotificationType","rdfs:domain":["ocpp:EventDataType","ocpp:VariableMonitoringType"]},{"@id":"ocpp:severity","@type":"rdf:Property","rdfs:label":"severity","rdfs:comment":"The severity that will be assigned to an event that is triggered by this monitor. The severity range is 0-9, with 0 as the highest and 9 as the lowest severity level.\r\n\r\nThe severity levels have the following meaning: +\r\n*0-Danger* +\r\nIndicates lives are potentially in danger. Urgent attention is needed and action should be taken immediately. +\r\n*1-Hardware Failure* +\r\nIndicates that the Charging Station is unable to continue regular operations due to Hardware issues. Action is required. +\r\n*2-System Failure* +\r\nIndicates that the Charging Station is unable to continue regular operations due to software or minor hardware issues. Action is required. +\r\n*3-Critical* +\r\nIndicates a critical error. Action is required. +\r\n*4-Error* +\r\nIndicates a non-urgent error. Action is required. +\r\n*5-Alert* +\r\nIndicates an alert event. Default severity for any type of monitoring event.  +\r\n*6-Warning* +\r\nIndicates a warning event. Action may be required. +\r\n*7-Notice* +\r\nIndicates an unusual event. No immediate action is required. +\r\n*8-Informational* +\r\nIndicates a regular operational event. May be used for reporting, measuring throughput, etc. No action is required. +\r\n*9-Debug* +\r\nIndicates information useful to developers for debugging, not useful during operations.\r\n\r\n","rdfs:domain":["ocpp:EventDataType","ocpp:VariableMonitoringType","ocpp:SetMonitoringDataType","ocpp:SetMonitoringResultType"],"schema:rangeIncludes":"xsd:integer"},{"@id":"ocpp:transaction","@type":"rdf:Property","rdfs:label":"transaction","rdfs:comment":"Monitor only active when a transaction is ongoing on a component relevant to this transaction. Default = false.\r\n\r\n","rdfs:domain":["ocpp:VariableMonitoringType","ocpp:SetMonitoringDataType"],"schema:rangeIncludes":"xsd:boolean"},{"@id":"ocpp:isDefault","@type":"rdf:Property","rdfs:label":"isDefault","rdfs:comment":"True if setting is a default control.\r\n","rdfs:domain":["ocpp:DERCurveGetType","ocpp:FixedPFGetType","ocpp:FixedVarGetType","ocpp:FreqDroopGetType","ocpp:LimitMaxDischargeGetType"],"schema:rangeIncludes":"xsd:boolean"},{"@id":"ocpp:isSuperseded","@type":"rdf:Property","rdfs:label":"isSuperseded","rdfs:comment":"True if this setting is superseded by a higher priority setting (i.e. lower value of _priority_)\r\n\r\n","rdfs:domain":["ocpp:DERCurveGetType","ocpp:FixedPFGetType","ocpp:FixedVarGetType","ocpp:FreqDroopGetType","ocpp:LimitMaxDischargeGetType"],"schema:rangeIncludes":"xsd:boolean"},{"@id":"ocpp:responseTime","@type":"rdf:Property","rdfs:label":"responseTime","rdfs:comment":"Open loop response time, the time to ramp up to 90% of the new target in response to the change in voltage, in seconds. A value of 0 is used to mean no limit. When not present, the device should follow its default behavior.\r\n\r\n\r\n","rdfs:domain":["ocpp:DERCurveType","ocpp:FreqDroopType"],"schema:rangeIncludes":"xsd:double"},{"@id":"ocpp:gradient","@type":"rdf:Property","rdfs:label":"gradient","rdfs:comment":"Default ramp rate in seconds (0 if not applicable)\r\n\r\n\r\n","rdfs:domain":["ocpp:GradientGetType","ocpp:GradientType"],"schema:rangeIncludes":"xsd:double"},{"@id":"ocpp:apn","@type":"rdf:Property","rdfs:label":"apn","rdfs:comment":"The Access Point Name as an URL.\r\n","rdfs:domain":["ocpp:APNType","ocpp:NetworkConnectionProfileType"],"schema:rangeIncludes":"xsd:string"}]}